@prefix APDU: <http://bacowl.sourceforge.net/2012/bacnet/APDU#> .
@prefix AbortPDU: <http://bacowl.sourceforge.net/2012/bacnet/AbortPDU#> .
@prefix AbortReason: <http://bacowl.sourceforge.net/2012/bacnet/AbortReason#> .
@prefix AccessAuthenticationFactorDisable: <http://bacowl.sourceforge.net/2012/bacnet/AccessAuthenticationFactorDisable#> .
@prefix AccessCredentialDisable: <http://bacowl.sourceforge.net/2012/bacnet/AccessCredentialDisable#> .
@prefix AccessCredentialDisableReason: <http://bacowl.sourceforge.net/2012/bacnet/AccessCredentialDisableReason#> .
@prefix AccessCredentialObject: <http://bacowl.sourceforge.net/2012/bacnet/AccessCredentialObject#> .
@prefix AccessDoorObject: <http://bacowl.sourceforge.net/2012/bacnet/AccessDoorObject#> .
@prefix AccessEvent: <http://bacowl.sourceforge.net/2012/bacnet/AccessEvent#> .
@prefix AccessPassbackMode: <http://bacowl.sourceforge.net/2012/bacnet/AccessPassbackMode#> .
@prefix AccessPointObject: <http://bacowl.sourceforge.net/2012/bacnet/AccessPointObject#> .
@prefix AccessRightsObject: <http://bacowl.sourceforge.net/2012/bacnet/AccessRightsObject#> .
@prefix AccessRule: <http://bacowl.sourceforge.net/2012/bacnet/AccessRule#> .
@prefix AccessRuleLocationSpecifier: <http://bacowl.sourceforge.net/2012/bacnet/AccessRuleLocationSpecifier#> .
@prefix AccessRuleTimeRangeSpecifier: <http://bacowl.sourceforge.net/2012/bacnet/AccessRuleTimeRangeSpecifier#> .
@prefix AccessUserObject: <http://bacowl.sourceforge.net/2012/bacnet/AccessUserObject#> .
@prefix AccessUserType: <http://bacowl.sourceforge.net/2012/bacnet/AccessUserType#> .
@prefix AccessZoneObject: <http://bacowl.sourceforge.net/2012/bacnet/AccessZoneObject#> .
@prefix AccessZoneOccupancyState: <http://bacowl.sourceforge.net/2012/bacnet/AccessZoneOccupancyState#> .
@prefix AccumulatorObject: <http://bacowl.sourceforge.net/2012/bacnet/AccumulatorObject#> .
@prefix AccumulatorRecord: <http://bacowl.sourceforge.net/2012/bacnet/AccumulatorRecord#> .
@prefix AccumulatorRecordAccumulatorStatus: <http://bacowl.sourceforge.net/2012/bacnet/AccumulatorRecordAccumulatorStatus#> .
@prefix AcknowledgeAlarmRequest: <http://bacowl.sourceforge.net/2012/bacnet/AcknowledgeAlarmRequest#> .
@prefix Action: <http://bacowl.sourceforge.net/2012/bacnet/Action#> .
@prefix ActionCommand: <http://bacowl.sourceforge.net/2012/bacnet/ActionCommand#> .
@prefix ActionList: <http://bacowl.sourceforge.net/2012/bacnet/ActionList#> .
@prefix AddListElementRequest: <http://bacowl.sourceforge.net/2012/bacnet/AddListElementRequest#> .
@prefix Address: <http://bacowl.sourceforge.net/2012/bacnet/Address#> .
@prefix AddressBinding: <http://bacowl.sourceforge.net/2012/bacnet/AddressBinding#> .
@prefix AnalogInputObject: <http://bacowl.sourceforge.net/2012/bacnet/AnalogInputObject#> .
@prefix AnalogOutputObject: <http://bacowl.sourceforge.net/2012/bacnet/AnalogOutputObject#> .
@prefix AnalogValueObject: <http://bacowl.sourceforge.net/2012/bacnet/AnalogValueObject#> .
@prefix AssignedAccessRights: <http://bacowl.sourceforge.net/2012/bacnet/AssignedAccessRights#> .
@prefix AtomicReadFileACK: <http://bacowl.sourceforge.net/2012/bacnet/AtomicReadFileACK#> .
@prefix AtomicReadFileACKAccessMethodChoice: <http://bacowl.sourceforge.net/2012/bacnet/AtomicReadFileACKAccessMethodChoice#> .
@prefix AtomicReadFileACKAccessMethodRecordAccess: <http://bacowl.sourceforge.net/2012/bacnet/AtomicReadFileACKAccessMethodRecordAccess#> .
@prefix AtomicReadFileACKAccessMethodStreamAccess: <http://bacowl.sourceforge.net/2012/bacnet/AtomicReadFileACKAccessMethodStreamAccess#> .
@prefix AtomicReadFileRequest: <http://bacowl.sourceforge.net/2012/bacnet/AtomicReadFileRequest#> .
@prefix AtomicReadFileRequestAccessMethodChoice: <http://bacowl.sourceforge.net/2012/bacnet/AtomicReadFileRequestAccessMethodChoice#> .
@prefix AtomicReadFileRequestAccessMethodChoiceRecordAccess: <http://bacowl.sourceforge.net/2012/bacnet/AtomicReadFileRequestAccessMethodChoiceRecordAccess#> .
@prefix AtomicReadFileRequestAccessMethodChoiceStreamAccess: <http://bacowl.sourceforge.net/2012/bacnet/AtomicReadFileRequestAccessMethodChoiceStreamAccess#> .
@prefix AtomicWriteFileACK: <http://bacowl.sourceforge.net/2012/bacnet/AtomicWriteFileACK#> .
@prefix AtomicWriteFileRequest: <http://bacowl.sourceforge.net/2012/bacnet/AtomicWriteFileRequest#> .
@prefix AtomicWriteFileRequestAccessMethodChoice: <http://bacowl.sourceforge.net/2012/bacnet/AtomicWriteFileRequestAccessMethodChoice#> .
@prefix AtomicWriteFileRequestAccessMethodChoiceRecordAccess: <http://bacowl.sourceforge.net/2012/bacnet/AtomicWriteFileRequestAccessMethodChoiceRecordAccess#> .
@prefix AtomicWriteFileRequestAccessMethodChoiceStreamAccess: <http://bacowl.sourceforge.net/2012/bacnet/AtomicWriteFileRequestAccessMethodChoiceStreamAccess#> .
@prefix AuthenticateACK: <http://bacowl.sourceforge.net/2012/bacnet/AuthenticateACK#> .
@prefix AuthenticateRequest: <http://bacowl.sourceforge.net/2012/bacnet/AuthenticateRequest#> .
@prefix AuthenticationFactor: <http://bacowl.sourceforge.net/2012/bacnet/AuthenticationFactor#> .
@prefix AuthenticationFactorFormat: <http://bacowl.sourceforge.net/2012/bacnet/AuthenticationFactorFormat#> .
@prefix AuthenticationFactorType: <http://bacowl.sourceforge.net/2012/bacnet/AuthenticationFactorType#> .
@prefix AuthenticationPolicy: <http://bacowl.sourceforge.net/2012/bacnet/AuthenticationPolicy#> .
@prefix AuthenticationPolicyPolicy: <http://bacowl.sourceforge.net/2012/bacnet/AuthenticationPolicyPolicy#> .
@prefix AuthenticationStatus: <http://bacowl.sourceforge.net/2012/bacnet/AuthenticationStatus#> .
@prefix AuthorizationException: <http://bacowl.sourceforge.net/2012/bacnet/AuthorizationException#> .
@prefix AuthorizationMode: <http://bacowl.sourceforge.net/2012/bacnet/AuthorizationMode#> .
@prefix AveragingObject: <http://bacowl.sourceforge.net/2012/bacnet/AveragingObject#> .
@prefix BACnet: <http://bacowl.sourceforge.net/2012/bacnet#> .
@prefix BackupState: <http://bacowl.sourceforge.net/2012/bacnet/BackupState#> .
@prefix BinaryInputObject: <http://bacowl.sourceforge.net/2012/bacnet/BinaryInputObject#> .
@prefix BinaryOutputObject: <http://bacowl.sourceforge.net/2012/bacnet/BinaryOutputObject#> .
@prefix BinaryPV: <http://bacowl.sourceforge.net/2012/bacnet/BinaryPV#> .
@prefix BinaryValueObject: <http://bacowl.sourceforge.net/2012/bacnet/BinaryValueObject#> .
@prefix Bit: <http://bacowl.sourceforge.net/2012/bacnet/Bit#> .
@prefix BitStringValueObject: <http://bacowl.sourceforge.net/2012/bacnet/BitStringValueObject#> .
@prefix COVNotificationParameters: <http://bacowl.sourceforge.net/2012/bacnet/COVNotificationParameters#> .
@prefix COVSubscription: <http://bacowl.sourceforge.net/2012/bacnet/COVSubscription#> .
@prefix CalendarEntry: <http://bacowl.sourceforge.net/2012/bacnet/CalendarEntry#> .
@prefix CalendarObject: <http://bacowl.sourceforge.net/2012/bacnet/CalendarObject#> .
@prefix ChangeListError: <http://bacowl.sourceforge.net/2012/bacnet/ChangeListError#> .
@prefix ChannelValue: <http://bacowl.sourceforge.net/2012/bacnet/ChannelValue#> .
@prefix CharacterStringValueObject: <http://bacowl.sourceforge.net/2012/bacnet/CharacterStringValueObject#> .
@prefix ClientCOV: <http://bacowl.sourceforge.net/2012/bacnet/ClientCOV#> .
@prefix CommandObject: <http://bacowl.sourceforge.net/2012/bacnet/CommandObject#> .
@prefix ConfirmedCOVNotificationRequest: <http://bacowl.sourceforge.net/2012/bacnet/ConfirmedCOVNotificationRequest#> .
@prefix ConfirmedEventNotificationRequest: <http://bacowl.sourceforge.net/2012/bacnet/ConfirmedEventNotificationRequest#> .
@prefix ConfirmedPrivateTransferACK: <http://bacowl.sourceforge.net/2012/bacnet/ConfirmedPrivateTransferACK#> .
@prefix ConfirmedPrivateTransferError: <http://bacowl.sourceforge.net/2012/bacnet/ConfirmedPrivateTransferError#> .
@prefix ConfirmedPrivateTransferRequest: <http://bacowl.sourceforge.net/2012/bacnet/ConfirmedPrivateTransferRequest#> .
@prefix ConfirmedServiceChoice: <http://bacowl.sourceforge.net/2012/bacnet/ConfirmedServiceChoice#> .
@prefix ConfirmedTextMessageRequest: <http://bacowl.sourceforge.net/2012/bacnet/ConfirmedTextMessageRequest#> .
@prefix ConfirmedTextMessageRequestMessageClass: <http://bacowl.sourceforge.net/2012/bacnet/ConfirmedTextMessageRequestMessageClass#> .
@prefix ConfirmedTextMessageRequestMessagePriority: <http://bacowl.sourceforge.net/2012/bacnet/ConfirmedTextMessageRequestMessagePriority#> .
@prefix CreateObjectACK: <http://bacowl.sourceforge.net/2012/bacnet/CreateObjectACK#> .
@prefix CreateObjectError: <http://bacowl.sourceforge.net/2012/bacnet/CreateObjectError#> .
@prefix CreateObjectRequest: <http://bacowl.sourceforge.net/2012/bacnet/CreateObjectRequest#> .
@prefix CreateObjectRequestObjectSpecifier: <http://bacowl.sourceforge.net/2012/bacnet/CreateObjectRequestObjectSpecifier#> .
@prefix CredentialAuthenticationFactor: <http://bacowl.sourceforge.net/2012/bacnet/CredentialAuthenticationFactor#> .
@prefix CredentialDataInputObject: <http://bacowl.sourceforge.net/2012/bacnet/CredentialDataInputObject#> .
@prefix DailySchedule: <http://bacowl.sourceforge.net/2012/bacnet/DailySchedule#> .
@prefix DatePatternValueObject: <http://bacowl.sourceforge.net/2012/bacnet/DatePatternValueObject#> .
@prefix DateRange: <http://bacowl.sourceforge.net/2012/bacnet/DateRange#> .
@prefix DateTime: <http://bacowl.sourceforge.net/2012/bacnet/DateTime#> .
@prefix DateTimePatternValueObject: <http://bacowl.sourceforge.net/2012/bacnet/DateTimePatternValueObject#> .
@prefix DateTimeValueObject: <http://bacowl.sourceforge.net/2012/bacnet/DateTimeValueObject#> .
@prefix DateValueObject: <http://bacowl.sourceforge.net/2012/bacnet/DateValueObject#> .
@prefix DaysOfWeek: <http://bacowl.sourceforge.net/2012/bacnet/DaysOfWeek#> .
@prefix DeleteObjectRequest: <http://bacowl.sourceforge.net/2012/bacnet/DeleteObjectRequest#> .
@prefix Destination: <http://bacowl.sourceforge.net/2012/bacnet/Destination#> .
@prefix DeviceAddress: <http://bacowl.sourceforge.net/2012/bacnet/DeviceAddress#> .
@prefix DeviceCommunicationControlRequest: <http://bacowl.sourceforge.net/2012/bacnet/DeviceCommunicationControlRequest#> .
@prefix DeviceCommunicationControlRequestEnableDisable: <http://bacowl.sourceforge.net/2012/bacnet/DeviceCommunicationControlRequestEnableDisable#> .
@prefix DeviceObject: <http://bacowl.sourceforge.net/2012/bacnet/DeviceObject#> .
@prefix DeviceObjectPropertyReference: <http://bacowl.sourceforge.net/2012/bacnet/DeviceObjectPropertyReference#> .
@prefix DeviceObjectPropertyValue: <http://bacowl.sourceforge.net/2012/bacnet/DeviceObjectPropertyValue#> .
@prefix DeviceObjectReference: <http://bacowl.sourceforge.net/2012/bacnet/DeviceObjectReference#> .
@prefix DeviceStatus: <http://bacowl.sourceforge.net/2012/bacnet/DeviceStatus#> .
@prefix DoorAlarmState: <http://bacowl.sourceforge.net/2012/bacnet/DoorAlarmState#> .
@prefix DoorSecuredStatus: <http://bacowl.sourceforge.net/2012/bacnet/DoorSecuredStatus#> .
@prefix DoorStatus: <http://bacowl.sourceforge.net/2012/bacnet/DoorStatus#> .
@prefix DoorValue: <http://bacowl.sourceforge.net/2012/bacnet/DoorValue#> .
@prefix Element: <http://bacowl.sourceforge.net/2012/bacnet/Element#> .
@prefix EngineeringUnits: <http://bacowl.sourceforge.net/2012/bacnet/EngineeringUnits#> .
@prefix Enumerated: <http://bacowl.sourceforge.net/2012/bacnet/Enumerated#> .
@prefix Error: <http://bacowl.sourceforge.net/2012/bacnet/Error#> .
@prefix ErrorClass: <http://bacowl.sourceforge.net/2012/bacnet/ErrorClass#> .
@prefix ErrorCode: <http://bacowl.sourceforge.net/2012/bacnet/ErrorCode#> .
@prefix ErrorType: <http://bacowl.sourceforge.net/2012/bacnet/ErrorType#> .
@prefix EventEnrollmentObject: <http://bacowl.sourceforge.net/2012/bacnet/EventEnrollmentObject#> .
@prefix EventLogObject: <http://bacowl.sourceforge.net/2012/bacnet/EventLogObject#> .
@prefix EventLogRecord: <http://bacowl.sourceforge.net/2012/bacnet/EventLogRecord#> .
@prefix EventLogRecordLogDatum: <http://bacowl.sourceforge.net/2012/bacnet/EventLogRecordLogDatum#> .
@prefix EventNotificationParameters: <http://bacowl.sourceforge.net/2012/bacnet/EventNotificationParameters#> .
@prefix EventParameter: <http://bacowl.sourceforge.net/2012/bacnet/EventParameter#> .
@prefix EventParameterAccessEvent: <http://bacowl.sourceforge.net/2012/bacnet/EventParameterAccessEvent#> .
@prefix EventParameterAccessEventAccessEvent: <http://bacowl.sourceforge.net/2012/bacnet/EventParameterAccessEventAccessEvent#> .
@prefix EventParameterBufferReady: <http://bacowl.sourceforge.net/2012/bacnet/EventParameterBufferReady#> .
@prefix EventParameterChangeOfBitstring: <http://bacowl.sourceforge.net/2012/bacnet/EventParameterChangeOfBitstring#> .
@prefix EventParameterChangeOfCharacterString: <http://bacowl.sourceforge.net/2012/bacnet/EventParameterChangeOfCharacterString#> .
@prefix EventParameterChangeOfLifeSafety: <http://bacowl.sourceforge.net/2012/bacnet/EventParameterChangeOfLifeSafety#> .
@prefix EventParameterChangeOfState: <http://bacowl.sourceforge.net/2012/bacnet/EventParameterChangeOfState#> .
@prefix EventParameterChangeOfStatusFlags: <http://bacowl.sourceforge.net/2012/bacnet/EventParameterChangeOfStatusFlags#> .
@prefix EventParameterChangeOfValue: <http://bacowl.sourceforge.net/2012/bacnet/EventParameterChangeOfValue#> .
@prefix EventParameterChangeOfValueCOVCriteria: <http://bacowl.sourceforge.net/2012/bacnet/EventParameterChangeOfValueCOVCriteria#> .
@prefix EventParameterCommandFailure: <http://bacowl.sourceforge.net/2012/bacnet/EventParameterCommandFailure#> .
@prefix EventParameterDoubleOutOfRange: <http://bacowl.sourceforge.net/2012/bacnet/EventParameterDoubleOutOfRange#> .
@prefix EventParameterExtended: <http://bacowl.sourceforge.net/2012/bacnet/EventParameterExtended#> .
@prefix EventParameterExtendedParameters: <http://bacowl.sourceforge.net/2012/bacnet/EventParameterExtendedParameters#> .
@prefix EventParameterFloatingLimit: <http://bacowl.sourceforge.net/2012/bacnet/EventParameterFloatingLimit#> .
@prefix EventParameterOutOfRange: <http://bacowl.sourceforge.net/2012/bacnet/EventParameterOutOfRange#> .
@prefix EventParameterSignedOutOfRange: <http://bacowl.sourceforge.net/2012/bacnet/EventParameterSignedOutOfRange#> .
@prefix EventParameterUnsignedOutOfRange: <http://bacowl.sourceforge.net/2012/bacnet/EventParameterUnsignedOutOfRange#> .
@prefix EventParameterUnsignedRange: <http://bacowl.sourceforge.net/2012/bacnet/EventParameterUnsignedRange#> .
@prefix EventState: <http://bacowl.sourceforge.net/2012/bacnet/EventState#> .
@prefix EventTransitionBits: <http://bacowl.sourceforge.net/2012/bacnet/EventTransitionBits#> .
@prefix EventType: <http://bacowl.sourceforge.net/2012/bacnet/EventType#> .
@prefix FileAccessMethod: <http://bacowl.sourceforge.net/2012/bacnet/FileAccessMethod#> .
@prefix FileObject: <http://bacowl.sourceforge.net/2012/bacnet/FileObject#> .
@prefix GetAlarmSummaryACK: <http://bacowl.sourceforge.net/2012/bacnet/GetAlarmSummaryACK#> .
@prefix GetAlarmSummaryAlarmSummary: <http://bacowl.sourceforge.net/2012/bacnet/GetAlarmSummaryAlarmSummary#> .
@prefix GetAlarmSummaryRequest: <http://bacowl.sourceforge.net/2012/bacnet/GetAlarmSummaryRequest#> .
@prefix GetEnrollmentSummaryACK: <http://bacowl.sourceforge.net/2012/bacnet/GetEnrollmentSummaryACK#> .
@prefix GetEnrollmentSummaryEnrollmentSummary: <http://bacowl.sourceforge.net/2012/bacnet/GetEnrollmentSummaryEnrollmentSummary#> .
@prefix GetEnrollmentSummaryRequest: <http://bacowl.sourceforge.net/2012/bacnet/GetEnrollmentSummaryRequest#> .
@prefix GetEnrollmentSummaryRequestAcknowledgmentFilterType: <http://bacowl.sourceforge.net/2012/bacnet/GetEnrollmentSummaryRequestAcknowledgmentFilterType#> .
@prefix GetEnrollmentSummaryRequestEventStateFilterType: <http://bacowl.sourceforge.net/2012/bacnet/GetEnrollmentSummaryRequestEventStateFilterType#> .
@prefix GetEventInformationACK: <http://bacowl.sourceforge.net/2012/bacnet/GetEventInformationACK#> .
@prefix GetEventInformationEventSummary: <http://bacowl.sourceforge.net/2012/bacnet/GetEventInformationEventSummary#> .
@prefix GetEventInformationRequest: <http://bacowl.sourceforge.net/2012/bacnet/GetEventInformationRequest#> .
@prefix GlobalGroupObject: <http://bacowl.sourceforge.net/2012/bacnet/GlobalGroupObject#> .
@prefix GroupChannelValue: <http://bacowl.sourceforge.net/2012/bacnet/GroupChannelValue#> .
@prefix GroupObject: <http://bacowl.sourceforge.net/2012/bacnet/GroupObject#> .
@prefix IAmRequest: <http://bacowl.sourceforge.net/2012/bacnet/IAmRequest#> .
@prefix IHaveRequest: <http://bacowl.sourceforge.net/2012/bacnet/IHaveRequest#> .
@prefix IntegerValueObject: <http://bacowl.sourceforge.net/2012/bacnet/IntegerValueObject#> .
@prefix KeyIdentifier: <http://bacowl.sourceforge.net/2012/bacnet/KeyIdentifier#> .
@prefix LargeAnalogValueObject: <http://bacowl.sourceforge.net/2012/bacnet/LargeAnalogValueObject#> .
@prefix LifeSafetyMode: <http://bacowl.sourceforge.net/2012/bacnet/LifeSafetyMode#> .
@prefix LifeSafetyOperation: <http://bacowl.sourceforge.net/2012/bacnet/LifeSafetyOperation#> .
@prefix LifeSafetyOperationRequest: <http://bacowl.sourceforge.net/2012/bacnet/LifeSafetyOperationRequest#> .
@prefix LifeSafetyPointObject: <http://bacowl.sourceforge.net/2012/bacnet/LifeSafetyPointObject#> .
@prefix LifeSafetyState: <http://bacowl.sourceforge.net/2012/bacnet/LifeSafetyState#> .
@prefix LifeSafetyZoneObject: <http://bacowl.sourceforge.net/2012/bacnet/LifeSafetyZoneObject#> .
@prefix LightingInProgress: <http://bacowl.sourceforge.net/2012/bacnet/LightingInProgress#> .
@prefix LightingOperation: <http://bacowl.sourceforge.net/2012/bacnet/LightingOperation#> .
@prefix LightingTransition: <http://bacowl.sourceforge.net/2012/bacnet/LightingTransition#> .
@prefix LimitEnable: <http://bacowl.sourceforge.net/2012/bacnet/LimitEnable#> .
@prefix LoadControlObject: <http://bacowl.sourceforge.net/2012/bacnet/LoadControlObject#> .
@prefix LockStatus: <http://bacowl.sourceforge.net/2012/bacnet/LockStatus#> .
@prefix LogData: <http://bacowl.sourceforge.net/2012/bacnet/LogData#> .
@prefix LogDataLogData: <http://bacowl.sourceforge.net/2012/bacnet/LogDataLogData#> .
@prefix LogMultipleRecord: <http://bacowl.sourceforge.net/2012/bacnet/LogMultipleRecord#> .
@prefix LogRecord: <http://bacowl.sourceforge.net/2012/bacnet/LogRecord#> .
@prefix LogRecordLogDatum: <http://bacowl.sourceforge.net/2012/bacnet/LogRecordLogDatum#> .
@prefix LogStatus: <http://bacowl.sourceforge.net/2012/bacnet/LogStatus#> .
@prefix LoggingType: <http://bacowl.sourceforge.net/2012/bacnet/LoggingType#> .
@prefix LoopObject: <http://bacowl.sourceforge.net/2012/bacnet/LoopObject#> .
@prefix Maintenance: <http://bacowl.sourceforge.net/2012/bacnet/Maintenance#> .
@prefix MultiStateInputObject: <http://bacowl.sourceforge.net/2012/bacnet/MultiStateInputObject#> .
@prefix MultiStateOutputObject: <http://bacowl.sourceforge.net/2012/bacnet/MultiStateOutputObject#> .
@prefix MultiStateValueObject: <http://bacowl.sourceforge.net/2012/bacnet/MultiStateValueObject#> .
@prefix NetworkSecurityObject: <http://bacowl.sourceforge.net/2012/bacnet/NetworkSecurityObject#> .
@prefix NetworkSecurityPolicy: <http://bacowl.sourceforge.net/2012/bacnet/NetworkSecurityPolicy#> .
@prefix NodeType: <http://bacowl.sourceforge.net/2012/bacnet/NodeType#> .
@prefix NotificationClassObject: <http://bacowl.sourceforge.net/2012/bacnet/NotificationClassObject#> .
@prefix NotificationParameters: <http://bacowl.sourceforge.net/2012/bacnet/NotificationParameters#> .
@prefix NotificationParametersAccessEventType: <http://bacowl.sourceforge.net/2012/bacnet/NotificationParametersAccessEventType#> .
@prefix NotificationParametersBufferReady: <http://bacowl.sourceforge.net/2012/bacnet/NotificationParametersBufferReady#> .
@prefix NotificationParametersChangeOfBitstring: <http://bacowl.sourceforge.net/2012/bacnet/NotificationParametersChangeOfBitstring#> .
@prefix NotificationParametersChangeOfCharacterStringType: <http://bacowl.sourceforge.net/2012/bacnet/NotificationParametersChangeOfCharacterStringType#> .
@prefix NotificationParametersChangeOfLifeSafety: <http://bacowl.sourceforge.net/2012/bacnet/NotificationParametersChangeOfLifeSafety#> .
@prefix NotificationParametersChangeOfState: <http://bacowl.sourceforge.net/2012/bacnet/NotificationParametersChangeOfState#> .
@prefix NotificationParametersChangeOfStatusFlagsType: <http://bacowl.sourceforge.net/2012/bacnet/NotificationParametersChangeOfStatusFlagsType#> .
@prefix NotificationParametersChangeOfValue: <http://bacowl.sourceforge.net/2012/bacnet/NotificationParametersChangeOfValue#> .
@prefix NotificationParametersChangeOfValueNewValue: <http://bacowl.sourceforge.net/2012/bacnet/NotificationParametersChangeOfValueNewValue#> .
@prefix NotificationParametersCommandFailure: <http://bacowl.sourceforge.net/2012/bacnet/NotificationParametersCommandFailure#> .
@prefix NotificationParametersComplexEventType: <http://bacowl.sourceforge.net/2012/bacnet/NotificationParametersComplexEventType#> .
@prefix NotificationParametersDoubleOutOfRangeType: <http://bacowl.sourceforge.net/2012/bacnet/NotificationParametersDoubleOutOfRangeType#> .
@prefix NotificationParametersExtended: <http://bacowl.sourceforge.net/2012/bacnet/NotificationParametersExtended#> .
@prefix NotificationParametersExtendedParametersType: <http://bacowl.sourceforge.net/2012/bacnet/NotificationParametersExtendedParametersType#> .
@prefix NotificationParametersFloatingLimit: <http://bacowl.sourceforge.net/2012/bacnet/NotificationParametersFloatingLimit#> .
@prefix NotificationParametersOutOfRange: <http://bacowl.sourceforge.net/2012/bacnet/NotificationParametersOutOfRange#> .
@prefix NotificationParametersSignedOutOfRangeType: <http://bacowl.sourceforge.net/2012/bacnet/NotificationParametersSignedOutOfRangeType#> .
@prefix NotificationParametersUnsignedOutOfRangeType: <http://bacowl.sourceforge.net/2012/bacnet/NotificationParametersUnsignedOutOfRangeType#> .
@prefix NotificationParametersUnsignedRange: <http://bacowl.sourceforge.net/2012/bacnet/NotificationParametersUnsignedRange#> .
@prefix NotifyType: <http://bacowl.sourceforge.net/2012/bacnet/NotifyType#> .
@prefix Null: <http://bacowl.sourceforge.net/2012/bacnet/Null#> .
@prefix Object: <http://bacowl.sourceforge.net/2012/bacnet/Object#> .
@prefix ObjectIdentifier: <http://bacowl.sourceforge.net/2012/bacnet/ObjectIdentifier#> .
@prefix ObjectPropertyReference: <http://bacowl.sourceforge.net/2012/bacnet/ObjectPropertyReference#> .
@prefix ObjectPropertyValue: <http://bacowl.sourceforge.net/2012/bacnet/ObjectPropertyValue#> .
@prefix ObjectType: <http://bacowl.sourceforge.net/2012/bacnet/ObjectType#> .
@prefix ObjectTypesSupported: <http://bacowl.sourceforge.net/2012/bacnet/ObjectTypesSupported#> .
@prefix OctetStringValueObject: <http://bacowl.sourceforge.net/2012/bacnet/OctetStringValueObject#> .
@prefix OptionalCharacterString: <http://bacowl.sourceforge.net/2012/bacnet/OptionalCharacterString#> .
@prefix Polarity: <http://bacowl.sourceforge.net/2012/bacnet/Polarity#> .
@prefix PositiveIntegerValueObject: <http://bacowl.sourceforge.net/2012/bacnet/PositiveIntegerValueObject#> .
@prefix Prescale: <http://bacowl.sourceforge.net/2012/bacnet/Prescale#> .
@prefix PriorityValue: <http://bacowl.sourceforge.net/2012/bacnet/PriorityValue#> .
@prefix ProgramError: <http://bacowl.sourceforge.net/2012/bacnet/ProgramError#> .
@prefix ProgramObject: <http://bacowl.sourceforge.net/2012/bacnet/ProgramObject#> .
@prefix ProgramRequest: <http://bacowl.sourceforge.net/2012/bacnet/ProgramRequest#> .
@prefix ProgramState: <http://bacowl.sourceforge.net/2012/bacnet/ProgramState#> .
@prefix Property: <http://bacowl.sourceforge.net/2012/bacnet/Property#> .
@prefix PropertyAccessResult: <http://bacowl.sourceforge.net/2012/bacnet/PropertyAccessResult#> .
@prefix PropertyAccessResultAccessResult: <http://bacowl.sourceforge.net/2012/bacnet/PropertyAccessResultAccessResult#> .
@prefix PropertyIdentifier: <http://bacowl.sourceforge.net/2012/bacnet/PropertyIdentifier#> .
@prefix PropertyReference: <http://bacowl.sourceforge.net/2012/bacnet/PropertyReference#> .
@prefix PropertyStates: <http://bacowl.sourceforge.net/2012/bacnet/PropertyStates#> .
@prefix PropertyValue: <http://bacowl.sourceforge.net/2012/bacnet/PropertyValue#> .
@prefix PulseConverterObject: <http://bacowl.sourceforge.net/2012/bacnet/PulseConverterObject#> .
@prefix Range: <http://bacowl.sourceforge.net/2012/bacnet/Range#> .
@prefix RangeByPosition: <http://bacowl.sourceforge.net/2012/bacnet/RangeByPosition#> .
@prefix RangeBySequenceNumber: <http://bacowl.sourceforge.net/2012/bacnet/RangeBySequenceNumber#> .
@prefix RangeByTime: <http://bacowl.sourceforge.net/2012/bacnet/RangeByTime#> .
@prefix ReadAccessResult: <http://bacowl.sourceforge.net/2012/bacnet/ReadAccessResult#> .
@prefix ReadAccessResultElement: <http://bacowl.sourceforge.net/2012/bacnet/ReadAccessResultElement#> .
@prefix ReadAccessResultElementChoice: <http://bacowl.sourceforge.net/2012/bacnet/ReadAccessResultElementChoice#> .
@prefix ReadAccessSpecification: <http://bacowl.sourceforge.net/2012/bacnet/ReadAccessSpecification#> .
@prefix ReadPropertyACK: <http://bacowl.sourceforge.net/2012/bacnet/ReadPropertyACK#> .
@prefix ReadPropertyMultipleACK: <http://bacowl.sourceforge.net/2012/bacnet/ReadPropertyMultipleACK#> .
@prefix ReadPropertyMultipleRequest: <http://bacowl.sourceforge.net/2012/bacnet/ReadPropertyMultipleRequest#> .
@prefix ReadPropertyRequest: <http://bacowl.sourceforge.net/2012/bacnet/ReadPropertyRequest#> .
@prefix ReadRangeACK: <http://bacowl.sourceforge.net/2012/bacnet/ReadRangeACK#> .
@prefix ReadRangeRequest: <http://bacowl.sourceforge.net/2012/bacnet/ReadRangeRequest#> .
@prefix Recipient: <http://bacowl.sourceforge.net/2012/bacnet/Recipient#> .
@prefix RecipientProcess: <http://bacowl.sourceforge.net/2012/bacnet/RecipientProcess#> .
@prefix ReinitializeDeviceRequest: <http://bacowl.sourceforge.net/2012/bacnet/ReinitializeDeviceRequest#> .
@prefix ReinitializeDeviceRequestReinitializedStateOfDevice: <http://bacowl.sourceforge.net/2012/bacnet/ReinitializeDeviceRequestReinitializedStateOfDevice#> .
@prefix RejectPDU: <http://bacowl.sourceforge.net/2012/bacnet/RejectPDU#> .
@prefix RejectReason: <http://bacowl.sourceforge.net/2012/bacnet/RejectReason#> .
@prefix Reliability: <http://bacowl.sourceforge.net/2012/bacnet/Reliability#> .
@prefix RemoveListElementRequest: <http://bacowl.sourceforge.net/2012/bacnet/RemoveListElementRequest#> .
@prefix RequestKeyRequest: <http://bacowl.sourceforge.net/2012/bacnet/RequestKeyRequest#> .
@prefix RestartReason: <http://bacowl.sourceforge.net/2012/bacnet/RestartReason#> .
@prefix ResultFlags: <http://bacowl.sourceforge.net/2012/bacnet/ResultFlags#> .
@prefix Scale: <http://bacowl.sourceforge.net/2012/bacnet/Scale#> .
@prefix ScheduleObject: <http://bacowl.sourceforge.net/2012/bacnet/ScheduleObject#> .
@prefix SecurityKeySet: <http://bacowl.sourceforge.net/2012/bacnet/SecurityKeySet#> .
@prefix SecurityLevel: <http://bacowl.sourceforge.net/2012/bacnet/SecurityLevel#> .
@prefix SecurityPolicy: <http://bacowl.sourceforge.net/2012/bacnet/SecurityPolicy#> .
@prefix Segmentation: <http://bacowl.sourceforge.net/2012/bacnet/Segmentation#> .
@prefix Sequence: <http://bacowl.sourceforge.net/2012/bacnet/Sequence#> .
@prefix SequenceElement: <http://bacowl.sourceforge.net/2012/bacnet/SequenceElement#> .
@prefix SequenceOf: <http://bacowl.sourceforge.net/2012/bacnet/SequenceOf#> .
@prefix ServicesSupported: <http://bacowl.sourceforge.net/2012/bacnet/ServicesSupported#> .
@prefix SetpointReference: <http://bacowl.sourceforge.net/2012/bacnet/SetpointReference#> .
@prefix ShedLevel: <http://bacowl.sourceforge.net/2012/bacnet/ShedLevel#> .
@prefix ShedState: <http://bacowl.sourceforge.net/2012/bacnet/ShedState#> .
@prefix SilencedState: <http://bacowl.sourceforge.net/2012/bacnet/SilencedState#> .
@prefix SpecialEvent: <http://bacowl.sourceforge.net/2012/bacnet/SpecialEvent#> .
@prefix SpecialEventPeriod: <http://bacowl.sourceforge.net/2012/bacnet/SpecialEventPeriod#> .
@prefix StatusFlags: <http://bacowl.sourceforge.net/2012/bacnet/StatusFlags#> .
@prefix StructuredViewObject: <http://bacowl.sourceforge.net/2012/bacnet/StructuredViewObject#> .
@prefix SubscribeCOVPropertyRequest: <http://bacowl.sourceforge.net/2012/bacnet/SubscribeCOVPropertyRequest#> .
@prefix SubscribeCOVRequest: <http://bacowl.sourceforge.net/2012/bacnet/SubscribeCOVRequest#> .
@prefix TimePatternValueObject: <http://bacowl.sourceforge.net/2012/bacnet/TimePatternValueObject#> .
@prefix TimeStamp: <http://bacowl.sourceforge.net/2012/bacnet/TimeStamp#> .
@prefix TimeSynchronizationRequest: <http://bacowl.sourceforge.net/2012/bacnet/TimeSynchronizationRequest#> .
@prefix TimeValue: <http://bacowl.sourceforge.net/2012/bacnet/TimeValue#> .
@prefix TimeValueObject: <http://bacowl.sourceforge.net/2012/bacnet/TimeValueObject#> .
@prefix TrendLogMultipleObject: <http://bacowl.sourceforge.net/2012/bacnet/TrendLogMultipleObject#> .
@prefix TrendLogObject: <http://bacowl.sourceforge.net/2012/bacnet/TrendLogObject#> .
@prefix UTCTimeSynchronizationRequest: <http://bacowl.sourceforge.net/2012/bacnet/UTCTimeSynchronizationRequest#> .
@prefix UnconfirmedCOVNotificationRequest: <http://bacowl.sourceforge.net/2012/bacnet/UnconfirmedCOVNotificationRequest#> .
@prefix UnconfirmedEventNotificationRequest: <http://bacowl.sourceforge.net/2012/bacnet/UnconfirmedEventNotificationRequest#> .
@prefix UnconfirmedPrivateTransferRequest: <http://bacowl.sourceforge.net/2012/bacnet/UnconfirmedPrivateTransferRequest#> .
@prefix UnconfirmedServiceChoice: <http://bacowl.sourceforge.net/2012/bacnet/UnconfirmedServiceChoice#> .
@prefix UnconfirmedTextMessageRequest: <http://bacowl.sourceforge.net/2012/bacnet/UnconfirmedTextMessageRequest#> .
@prefix UnconfirmedTextMessageRequestMessageClass: <http://bacowl.sourceforge.net/2012/bacnet/UnconfirmedTextMessageRequestMessageClass#> .
@prefix UnconfirmedTextMessageRequestMessagePriority: <http://bacowl.sourceforge.net/2012/bacnet/UnconfirmedTextMessageRequestMessagePriority#> .
@prefix VTClass: <http://bacowl.sourceforge.net/2012/bacnet/VTClass#> .
@prefix VTCloseError: <http://bacowl.sourceforge.net/2012/bacnet/VTCloseError#> .
@prefix VTCloseRequest: <http://bacowl.sourceforge.net/2012/bacnet/VTCloseRequest#> .
@prefix VTDataACK: <http://bacowl.sourceforge.net/2012/bacnet/VTDataACK#> .
@prefix VTDataRequest: <http://bacowl.sourceforge.net/2012/bacnet/VTDataRequest#> .
@prefix VTOpenACK: <http://bacowl.sourceforge.net/2012/bacnet/VTOpenACK#> .
@prefix VTOpenRequest: <http://bacowl.sourceforge.net/2012/bacnet/VTOpenRequest#> .
@prefix VTSession: <http://bacowl.sourceforge.net/2012/bacnet/VTSession#> .
@prefix Vendor: <http://bacowl.sourceforge.net/2012/bacnet/Vendor#> .
@prefix WhoHasLimits: <http://bacowl.sourceforge.net/2012/bacnet/WhoHasLimits#> .
@prefix WhoHasObject: <http://bacowl.sourceforge.net/2012/bacnet/WhoHasObject#> .
@prefix WhoHasRequest: <http://bacowl.sourceforge.net/2012/bacnet/WhoHasRequest#> .
@prefix WhoIsRequest: <http://bacowl.sourceforge.net/2012/bacnet/WhoIsRequest#> .
@prefix WriteAccessSpecification: <http://bacowl.sourceforge.net/2012/bacnet/WriteAccessSpecification#> .
@prefix WriteGroupRequest: <http://bacowl.sourceforge.net/2012/bacnet/WriteGroupRequest#> .
@prefix WritePropertyMultipleError: <http://bacowl.sourceforge.net/2012/bacnet/WritePropertyMultipleError#> .
@prefix WritePropertyMultipleRequest: <http://bacowl.sourceforge.net/2012/bacnet/WritePropertyMultipleRequest#> .
@prefix WritePropertyRequest: <http://bacowl.sourceforge.net/2012/bacnet/WritePropertyRequest#> .
@prefix WriteStatus: <http://bacowl.sourceforge.net/2012/bacnet/WriteStatus#> .
@prefix bacnet: <http://purl.org/wot-catalogue/bacnet#> .
@prefix ble: <http://purl.org/wot-catalogue/ble#> .
@prefix dtype: <http://www.linkedmodel.org/schema/dtype#> .
@prefix fn: <http://www.w3.org/2005/xpath-functions#> .
@prefix hgi: <http://homegatewayinitiative.org/xml/dal/3.0> .
@prefix httpList: <http://plugins.linkedpipes.com/ontology/e-httpGetFiles#> .
@prefix lwm2m: <http://purl.org/wot-catalogue/lwm2m#> .
@prefix ocf: <http://purl.org/wot-catalogue/ocf#> .
@prefix ontolex: <http://www.w3.org/ns/lemon/ontolex#> .
@prefix owl: <http://www.w3.org/2002/07/owl#> .
@prefix prov: <http://www.w3.org/ns/prov#> .
@prefix rdf: <http://www.w3.org/1999/02/22-rdf-syntax-ns#> .
@prefix rdfs: <http://www.w3.org/2000/01/rdf-schema#> .
@prefix sdt: <http://purl.org/wot-catalogue/sdt#> .
@prefix skos: <http://www.w3.org/2004/02/skos/core#> .
@prefix xs: <http://www.w3.org/2001/XMLSchema> .
@prefix xsd: <http://www.w3.org/2001/XMLSchema#> .

<http://purl.org/wot-catalogue/lwm2m/ipso#> a skos:Collection;
  skos:member lwm2m:2048, lwm2m:2050, lwm2m:2052, lwm2m:2053, lwm2m:2055, lwm2m:2057,
    lwm2m:3200, lwm2m:3201, lwm2m:3202, lwm2m:3203, lwm2m:3300, lwm2m:3301, lwm2m:3303,
    lwm2m:3304, lwm2m:3305, lwm2m:3308, lwm2m:2056, lwm2m:3310, lwm2m:3312, lwm2m:3315,
    lwm2m:3317, lwm2m:3318, lwm2m:2049, lwm2m:3319, lwm2m:3320, lwm2m:3306, lwm2m:3321,
    lwm2m:3322, lwm2m:3323, lwm2m:3324, lwm2m:3325, lwm2m:3316, lwm2m:3326, lwm2m:3327,
    lwm2m:3314, lwm2m:3328, lwm2m:3329, lwm2m:3311, lwm2m:3313, lwm2m:3330, lwm2m:2051,
    lwm2m:3331, lwm2m:3332, lwm2m:3333, lwm2m:3334, lwm2m:3335, lwm2m:3336, lwm2m:2054,
    lwm2m:3337, lwm2m:3338, lwm2m:3339, lwm2m:3302, lwm2m:3340;
  skos:definition "Objects registered by 3rd party standards organisations or alliances";
  skos:altLabel "External";
  skos:member lwm2m:3341, lwm2m:3342, lwm2m:3343, lwm2m:3344, lwm2m:3345, lwm2m:3346,
    lwm2m:3347, lwm2m:3348, lwm2m:3349, lwm2m:3350, lwm2m:3351, lwm2m:3352, lwm2m:3353,
    lwm2m:3354, lwm2m:3355, lwm2m:3356, lwm2m:3357, lwm2m:3358, lwm2m:3359, lwm2m:3360,
    lwm2m:3361, lwm2m:3362, lwm2m:3363, lwm2m:3364, lwm2m:3365, lwm2m:3366, lwm2m:3367,
    lwm2m:3368, lwm2m:3369, lwm2m:3370, lwm2m:3371, lwm2m:3372, lwm2m:3373, lwm2m:3374,
    lwm2m:3375, lwm2m:3376, lwm2m:3377, lwm2m:3378, lwm2m:3379, lwm2m:3380, lwm2m:3381,
    lwm2m:3382, lwm2m:3383, lwm2m:3384, lwm2m:3385, lwm2m:3386, lwm2m:3387, lwm2m:3388,
    lwm2m:3389, lwm2m:3390, lwm2m:3391, lwm2m:3392, lwm2m:3393, lwm2m:3394, lwm2m:3395,
    lwm2m:3396, lwm2m:3397, lwm2m:3398, lwm2m:3399, lwm2m:3400, lwm2m:3401, lwm2m:3402,
    lwm2m:3403, lwm2m:3404, lwm2m:3405, lwm2m:3406, lwm2m:3407, lwm2m:3408, lwm2m:3410,
    lwm2m:3411, lwm2m:3412, lwm2m:3413, lwm2m:3414, lwm2m:3415, lwm2m:3416, lwm2m:3417,
    lwm2m:3418, lwm2m:3419, lwm2m:3420, lwm2m:3421, lwm2m:3423, lwm2m:3424, lwm2m:3425,
    lwm2m:3426, lwm2m:3427, lwm2m:3428, lwm2m:3429, lwm2m:3430, lwm2m:3431, lwm2m:3432,
    lwm2m:3433, lwm2m:3434, lwm2m:3435, lwm2m:3436, lwm2m:3437, lwm2m:3438, lwm2m:3439,
    lwm2m:3441, lwm2m:3442;
  skos:prefLabel "ext-label" .

<http://purl.org/wot-catalogue/lwm2m/ipso#3434> a skos:Concept, ontolex:LexicalConcept;
  skos:altLabel "people counter";
  skos:broader lwm2m:Object;
  skos:definition "The uCIFI people counter provides people counting information using Bluetooth beacon or any other method.";
  skos:inScheme lwm2m:Scheme;
  skos:prefLabel "People counter";
  skos:related lwm2m:r3434-1, lwm2m:r3434-2, lwm2m:r3434-3, lwm2m:r3434-4, lwm2m:r3434-5,
    lwm2m:r3434-6, lwm2m:r3434-7, lwm2m:r3434-8;
  prov:wasDerivedFrom <file:/data/lp/etl/executor/data/1651932849158-23-3c5fa11b-d02c-40e9-9c76-7d268eee1c69/working/working-outputfiles-214/lwm2m-registry-prod/3434.xml> .

<http://purl.org/wot-catalogue/lwm2m/ipso#2052> a skos:Concept, ontolex:LexicalConcept;
  skos:altLabel "cmdh ecdef param values";
  skos:broader lwm2m:Object;
  skos:definition "This Object represents a specific set of default values for the CMDH related parameters Request Expiration Timestamp, Result Expiration Timestamp, Operational Execution Time, Result Persistence and Delivery Aggregation that are applicable for a given Event Category if these parameters are not specified in the message.";
  skos:inScheme lwm2m:Scheme;
  skos:prefLabel "CmdhEcDefParamValues";
  skos:related lwm2m:r2052-0, lwm2m:r2052-1, lwm2m:r2052-2, lwm2m:r2052-3, lwm2m:r2052-4,
    lwm2m:r2052-5;
  prov:wasDerivedFrom <file:/data/lp/etl/executor/data/1651932849158-23-3c5fa11b-d02c-40e9-9c76-7d268eee1c69/working/working-outputfiles-214/lwm2m-registry-prod/2052.xml> .

<http://purl.org/wot-catalogue/lwm2m/ipso#3400> a skos:Concept, ontolex:LexicalConcept;
  skos:altLabel "oa physical presence sensor";
  skos:broader lwm2m:Object;
  skos:definition "The 'oA_Physical_Presence_Sensor' represents the physical part of a presence sensor. All logical presence sensors (object instances of 'oA Presence Sensor') are mapped to one physical presence sensor.";
  skos:inScheme lwm2m:Scheme;
  skos:prefLabel "oA Physical Presence Sensor";
  skos:related lwm2m:r3400-901, lwm2m:r3400-907, lwm2m:r3400-908, lwm2m:r4001;
  prov:wasDerivedFrom <file:/data/lp/etl/executor/data/1651932849158-23-3c5fa11b-d02c-40e9-9c76-7d268eee1c69/working/working-outputfiles-214/lwm2m-registry-prod/3400.xml> .

<http://purl.org/wot-catalogue/lwm2m/ipso#3202> a skos:Concept, ontolex:LexicalConcept;
  skos:altLabel "analog input";
  skos:broader lwm2m:Object;
  skos:definition "Generic analog input for non-specific sensors";
  skos:inScheme lwm2m:Scheme;
  skos:prefLabel "Analog Input";
  skos:related lwm2m:r5518, lwm2m:r5600, lwm2m:r5601, lwm2m:r5602, lwm2m:r5603, lwm2m:r5604,
    lwm2m:r5605, lwm2m:r5750, lwm2m:r5751, lwm2m:r6042, lwm2m:r6049, lwm2m:r6050;
  prov:wasDerivedFrom <file:/data/lp/etl/executor/data/1651932849158-23-3c5fa11b-d02c-40e9-9c76-7d268eee1c69/working/working-outputfiles-214/lwm2m-registry-prod/3202.xml> .

<http://purl.org/wot-catalogue/lwm2m/ipso#3337> a skos:Concept, ontolex:LexicalConcept;
  skos:altLabel "positioner";
  skos:broader lwm2m:Object;
  skos:definition """This IPSO object should be used with a generic position actuator with range from 0 to 100%. This object optionally allows setting the transition time for an operation that changes the position of the actuator, and for reading the remaining time of the currently active transition.
        """;
  skos:inScheme lwm2m:Scheme;
  skos:prefLabel "Positioner";
  skos:related lwm2m:r5518, lwm2m:r5519, lwm2m:r5520, lwm2m:r5536, lwm2m:r5537, lwm2m:r5538,
    lwm2m:r5601, lwm2m:r5602, lwm2m:r5605, lwm2m:r5750, lwm2m:r6050;
  prov:wasDerivedFrom <file:/data/lp/etl/executor/data/1651932849158-23-3c5fa11b-d02c-40e9-9c76-7d268eee1c69/working/working-outputfiles-214/lwm2m-registry-prod/3337.xml> .

<http://purl.org/wot-catalogue/lwm2m/ipso#3392> a skos:Concept, ontolex:LexicalConcept;
  skos:altLabel "oa logical illuminance sensor";
  skos:broader lwm2m:Object;
  skos:definition "The 'oA Logical Illuminance Sensor' represents the logical part of an illuminance sensor. The corresponding physical device is a sensor that detects illuminance in its detection area.";
  skos:inScheme lwm2m:Scheme;
  skos:prefLabel "oA Logical Illuminance Sensor";
  skos:related lwm2m:r3392-400, lwm2m:r3392-401, lwm2m:r3392-402, lwm2m:r3392-403, lwm2m:r3392-404,
    lwm2m:r3392-901, lwm2m:r3392-903, lwm2m:r3392-904, lwm2m:r3392-905, lwm2m:r3392-906,
    lwm2m:r3392-909, lwm2m:r3392-919, lwm2m:r3392-924, lwm2m:r3392-934, lwm2m:r4001;
  prov:wasDerivedFrom <file:/data/lp/etl/executor/data/1651932849158-23-3c5fa11b-d02c-40e9-9c76-7d268eee1c69/working/working-outputfiles-214/lwm2m-registry-prod/3392.xml> .

<http://purl.org/wot-catalogue/lwm2m/ipso#3358> a skos:Concept, ontolex:LexicalConcept;
  skos:altLabel "rrc timer expiry event";
  skos:broader lwm2m:Object;
  skos:definition "RRC timer expiry event information";
  skos:inScheme lwm2m:Scheme;
  skos:prefLabel "rrcTimerExpiryEvent";
  skos:related lwm2m:r3358-0;
  prov:wasDerivedFrom <file:/data/lp/etl/executor/data/1651932849158-23-3c5fa11b-d02c-40e9-9c76-7d268eee1c69/working/working-outputfiles-214/lwm2m-registry-prod/3358.xml> .

<http://purl.org/wot-catalogue/lwm2m/ipso#2057> a skos:Concept, ontolex:LexicalConcept;
  skos:altLabel "cmdh back off parameters set";
  skos:broader lwm2m:Object;
  skos:definition "This Object defines set of parameters which can be referenced by a specific Instance of the CmdhNwAccessRule Object (ID: 2055)";
  skos:inScheme lwm2m:Scheme;
  skos:prefLabel "CmdhBackOffParametersSet";
  skos:related lwm2m:r2057-0, lwm2m:r2057-1, lwm2m:r2057-2, lwm2m:r2057-3, lwm2m:r2057-4;
  prov:wasDerivedFrom <file:/data/lp/etl/executor/data/1651932849158-23-3c5fa11b-d02c-40e9-9c76-7d268eee1c69/working/working-outputfiles-214/lwm2m-registry-prod/2057.xml> .

<http://purl.org/wot-catalogue/lwm2m/ipso#3410> a skos:Concept, ontolex:LexicalConcept;
  skos:altLabel "device extension";
  skos:broader lwm2m:Object;
  skos:definition "The uCIFI device extension is an extension to the standard Lightweight M2M device (object ID 3) using the resource called \"ExtDevInfo\" (resource ID 22).";
  skos:inScheme lwm2m:Scheme;
  skos:prefLabel "Device Extension";
  skos:related lwm2m:r3410-1, lwm2m:r3410-10, lwm2m:r3410-2, lwm2m:r3410-3, lwm2m:r3410-4,
    lwm2m:r3410-5, lwm2m:r3410-6, lwm2m:r3410-7, lwm2m:r3410-8, lwm2m:r3410-9;
  prov:wasDerivedFrom <file:/data/lp/etl/executor/data/1651932849158-23-3c5fa11b-d02c-40e9-9c76-7d268eee1c69/working/working-outputfiles-214/lwm2m-registry-prod/3410.xml> .

<http://purl.org/wot-catalogue/lwm2m/ipso#3430> a skos:Concept, ontolex:LexicalConcept;
  skos:altLabel "global navigation satellite system";
  skos:broader lwm2m:Object;
  skos:definition "More than a positioning object, the uCIFI global navigation satellite system object provides all the information required to calculate a position/location.";
  skos:inScheme lwm2m:Scheme;
  skos:prefLabel "Global Navigation Satellite System";
  skos:related lwm2m:r3430-0, lwm2m:r3430-1, lwm2m:r3430-10, lwm2m:r3430-11, lwm2m:r3430-12,
    lwm2m:r3430-13, lwm2m:r3430-14, lwm2m:r3430-15, lwm2m:r3430-16, lwm2m:r3430-17, lwm2m:r3430-18,
    lwm2m:r3430-19, lwm2m:r3430-2, lwm2m:r3430-20, lwm2m:r3430-21, lwm2m:r3430-22, lwm2m:r3430-23,
    lwm2m:r3430-24, lwm2m:r3430-25, lwm2m:r3430-26, lwm2m:r3430-27, lwm2m:r3430-28, lwm2m:r3430-3,
    lwm2m:r3430-4, lwm2m:r3430-5, lwm2m:r3430-6, lwm2m:r3430-7, lwm2m:r3430-8, lwm2m:r3430-9;
  prov:wasDerivedFrom <file:/data/lp/etl/executor/data/1651932849158-23-3c5fa11b-d02c-40e9-9c76-7d268eee1c69/working/working-outputfiles-214/lwm2m-registry-prod/3430.xml> .

<http://purl.org/wot-catalogue/lwm2m/ipso#3336> a skos:Concept, ontolex:LexicalConcept;
  skos:altLabel "location";
  skos:broader lwm2m:Object;
  skos:definition """This IPSO object represents GPS coordinates. This object is compatible with the LwM2M management object for location, but uses reusable resources.
        """;
  skos:inScheme lwm2m:Scheme;
  skos:prefLabel "Location";
  skos:related lwm2m:r5517, lwm2m:r5518, lwm2m:r5705, lwm2m:r5750, lwm2m:r6042, lwm2m:r6049,
    lwm2m:r6050, lwm2m:r6051, lwm2m:r6052, lwm2m:r6053;
  prov:wasDerivedFrom <file:/data/lp/etl/executor/data/1651932849158-23-3c5fa11b-d02c-40e9-9c76-7d268eee1c69/working/working-outputfiles-214/lwm2m-registry-prod/3336.xml> .

<http://purl.org/wot-catalogue/lwm2m/ipso#3386> a skos:Concept, ontolex:LexicalConcept;
  skos:altLabel "voltertp packet loss";
  skos:broader lwm2m:Object;
  skos:definition "Log is generated at the receiving end of RTP flow when newReceivedSequenceNumber - lastReceivedSequenceNumber > 1";
  skos:inScheme lwm2m:Scheme;
  skos:prefLabel "VoLTErtpPacketLoss";
  skos:related lwm2m:r3386-0, lwm2m:r3386-1;
  prov:wasDerivedFrom <file:/data/lp/etl/executor/data/1651932849158-23-3c5fa11b-d02c-40e9-9c76-7d268eee1c69/working/working-outputfiles-214/lwm2m-registry-prod/3386.xml> .

<http://purl.org/wot-catalogue/lwm2m/ipso#3332> a skos:Concept, ontolex:LexicalConcept;
  skos:altLabel "direction";
  skos:broader lwm2m:Object;
  skos:definition """This IPSO object is used to report the direction indicated by a compass, wind vane, or other directional indicator. The units of measure is plane angle degrees.
        """;
  skos:inScheme lwm2m:Scheme;
  skos:prefLabel "Direction";
  skos:related lwm2m:r5518, lwm2m:r5601, lwm2m:r5602, lwm2m:r5605, lwm2m:r5705, lwm2m:r5750,
    lwm2m:r6042, lwm2m:r6049, lwm2m:r6050;
  prov:wasDerivedFrom <file:/data/lp/etl/executor/data/1651932849158-23-3c5fa11b-d02c-40e9-9c76-7d268eee1c69/working/working-outputfiles-214/lwm2m-registry-prod/3332.xml> .

<http://purl.org/wot-catalogue/lwm2m/ipso#2055> a skos:Concept, ontolex:LexicalConcept;
  skos:altLabel "cmdh nwaccess rule";
  skos:broader lwm2m:Object;
  skos:definition "This Object defines limits in usage of specific underlying networks for forwarding information to other CSEs during processing of CMDH-related requests in a CSE.";
  skos:inScheme lwm2m:Scheme;
  skos:prefLabel "CmdhNwAccessRule";
  skos:related lwm2m:r2055-0, lwm2m:r2055-1, lwm2m:r2055-2, lwm2m:r2055-3, lwm2m:r2055-4,
    lwm2m:r2055-5;
  prov:wasDerivedFrom <file:/data/lp/etl/executor/data/1651932849158-23-3c5fa11b-d02c-40e9-9c76-7d268eee1c69/working/working-outputfiles-214/lwm2m-registry-prod/2055.xml> .

<http://purl.org/wot-catalogue/lwm2m/ipso#2053> a skos:Concept, ontolex:LexicalConcept;
  skos:altLabel "cmdh limits";
  skos:broader lwm2m:Object;
  skos:definition "This Object represents limits for CMDH related parameter values. ";
  skos:inScheme lwm2m:Scheme;
  skos:prefLabel "CmdhLimits";
  skos:related lwm2m:r2053-0, lwm2m:r2053-1, lwm2m:r2053-10, lwm2m:r2053-2, lwm2m:r2053-3,
    lwm2m:r2053-4, lwm2m:r2053-5, lwm2m:r2053-6, lwm2m:r2053-7, lwm2m:r2053-8, lwm2m:r2053-9;
  prov:wasDerivedFrom <file:/data/lp/etl/executor/data/1651932849158-23-3c5fa11b-d02c-40e9-9c76-7d268eee1c69/working/working-outputfiles-214/lwm2m-registry-prod/2053.xml> .

<http://purl.org/wot-catalogue/lwm2m/ipso#3344> a skos:Concept, ontolex:LexicalConcept;
  skos:altLabel "up/down control";
  skos:broader lwm2m:Object;
  skos:definition """This IPSO object is used to report the state of an up/down control element like a pair of push buttons or a rotary encoder. Counters for increase and decrease operations are provided for counting pulses from a quadrature encoder.
        """;
  skos:inScheme lwm2m:Scheme;
  skos:prefLabel "Up/Down Control";
  skos:related lwm2m:r5532, lwm2m:r5533, lwm2m:r5541, lwm2m:r5542, lwm2m:r5750;
  prov:wasDerivedFrom <file:/data/lp/etl/executor/data/1651932849158-23-3c5fa11b-d02c-40e9-9c76-7d268eee1c69/working/working-outputfiles-214/lwm2m-registry-prod/3344.xml> .

<http://purl.org/wot-catalogue/lwm2m/ipso#3435> a skos:Concept, ontolex:LexicalConcept;
  skos:altLabel "filling level";
  skos:broader lwm2m:Object;
  skos:definition "The uCIFI filling level sensor measures how full and/or how empty a container (e.g. waste, fuel) is and reports it either in percentage or in centimeters. The filling level sensor may be complemented with a temperature sensor to compose a waste filling sensor that can also identify waste container fire.";
  skos:inScheme lwm2m:Scheme;
  skos:prefLabel "Filling level";
  skos:related lwm2m:r3435-1, lwm2m:r3435-10, lwm2m:r3435-11, lwm2m:r3435-12, lwm2m:r3435-13,
    lwm2m:r3435-2, lwm2m:r3435-3, lwm2m:r3435-4, lwm2m:r3435-5, lwm2m:r3435-6, lwm2m:r3435-7,
    lwm2m:r3435-8, lwm2m:r3435-9;
  prov:wasDerivedFrom <file:/data/lp/etl/executor/data/1651932849158-23-3c5fa11b-d02c-40e9-9c76-7d268eee1c69/working/working-outputfiles-214/lwm2m-registry-prod/3435.xml> .

<http://purl.org/wot-catalogue/lwm2m/ipso#3385> a skos:Concept, ontolex:LexicalConcept;
  skos:altLabel "volte call state change event";
  skos:broader lwm2m:Object;
  skos:definition "VoLTE call status change";
  skos:inScheme lwm2m:Scheme;
  skos:prefLabel "volteCallStateChangeEvent";
  skos:related lwm2m:r3385-0, lwm2m:r3385-1;
  prov:wasDerivedFrom <file:/data/lp/etl/executor/data/1651932849158-23-3c5fa11b-d02c-40e9-9c76-7d268eee1c69/working/working-outputfiles-214/lwm2m-registry-prod/3385.xml> .

<http://purl.org/wot-catalogue/lwm2m/ipso#3364> a skos:Concept, ontolex:LexicalConcept;
  skos:altLabel "emm failure cause event";
  skos:broader lwm2m:Object;
  skos:definition "Triggered at EMM failure - failure cause is logged";
  skos:inScheme lwm2m:Scheme;
  skos:prefLabel "emmFailureCauseEvent";
  skos:related lwm2m:r3364-0;
  prov:wasDerivedFrom <file:/data/lp/etl/executor/data/1651932849158-23-3c5fa11b-d02c-40e9-9c76-7d268eee1c69/working/working-outputfiles-214/lwm2m-registry-prod/3364.xml> .

<http://purl.org/wot-catalogue/lwm2m/ipso#3201> a skos:Concept, ontolex:LexicalConcept;
  skos:altLabel "digital output";
  skos:broader lwm2m:Object;
  skos:definition "Generic digital output for non-specific actuators";
  skos:inScheme lwm2m:Scheme;
  skos:prefLabel "Digital Output";
  skos:related lwm2m:r5518, lwm2m:r5550, lwm2m:r5551, lwm2m:r5750, lwm2m:r6050;
  prov:wasDerivedFrom <file:/data/lp/etl/executor/data/1651932849158-23-3c5fa11b-d02c-40e9-9c76-7d268eee1c69/working/working-outputfiles-214/lwm2m-registry-prod/3201.xml> .

<http://purl.org/wot-catalogue/lwm2m/ipso#3328> a skos:Concept, ontolex:LexicalConcept;
  skos:altLabel "power";
  skos:broader lwm2m:Object;
  skos:definition """This IPSO object should be used to report power measurements. It also provides resources for minimum and maximum measured values, as well as the minimum and maximum range that can be measured by the sensor. An example measurement unit is Watts. This object may be used for either real power or apparent power measurements.
        """;
  skos:inScheme lwm2m:Scheme;
  skos:prefLabel "Power";
  skos:related lwm2m:r5518, lwm2m:r5601, lwm2m:r5602, lwm2m:r5603, lwm2m:r5604, lwm2m:r5605,
    lwm2m:r5700, lwm2m:r5701, lwm2m:r5750, lwm2m:r5821, lwm2m:r6042, lwm2m:r6049, lwm2m:r6050;
  prov:wasDerivedFrom <file:/data/lp/etl/executor/data/1651932849158-23-3c5fa11b-d02c-40e9-9c76-7d268eee1c69/working/working-outputfiles-214/lwm2m-registry-prod/3328.xml> .

<http://purl.org/wot-catalogue/lwm2m/ipso#3414> a skos:Concept, ontolex:LexicalConcept;
  skos:altLabel "ucifi data bridge";
  skos:broader lwm2m:Object;
  skos:definition "The uCIFI data bridge object may be used to transport data from a 3rd party device, operating a proprietary network or protocol, over a LwM2M compliant network.";
  skos:inScheme lwm2m:Scheme;
  skos:prefLabel "uCIFI data bridge";
  skos:related lwm2m:r3414-1, lwm2m:r3414-2, lwm2m:r3414-3, lwm2m:r3414-4, lwm2m:r3414-5,
    lwm2m:r3414-6;
  prov:wasDerivedFrom <file:/data/lp/etl/executor/data/1651932849158-23-3c5fa11b-d02c-40e9-9c76-7d268eee1c69/working/working-outputfiles-214/lwm2m-registry-prod/3414.xml> .

<http://purl.org/wot-catalogue/lwm2m/ipso#3354> a skos:Concept, ontolex:LexicalConcept;
  skos:altLabel "cell reselection event";
  skos:broader lwm2m:Object;
  skos:definition "cell reselection event information";
  skos:inScheme lwm2m:Scheme;
  skos:prefLabel "cellReselectionEvent";
  skos:related lwm2m:r3354-0, lwm2m:r3354-3, lwm2m:r6032, lwm2m:r6033;
  prov:wasDerivedFrom <file:/data/lp/etl/executor/data/1651932849158-23-3c5fa11b-d02c-40e9-9c76-7d268eee1c69/working/working-outputfiles-214/lwm2m-registry-prod/3354.xml> .

<http://purl.org/wot-catalogue/lwm2m/ipso#3429> a skos:Concept, ontolex:LexicalConcept;
  skos:altLabel "tilt sensor";
  skos:broader lwm2m:Object;
  skos:definition "The uCIFI tilt sensor provides the angle between the object's internal vertical and the perpendicular to the earth.";
  skos:inScheme lwm2m:Scheme;
  skos:prefLabel "Tilt sensor";
  skos:related lwm2m:r3429-1, lwm2m:r3429-2, lwm2m:r3429-3, lwm2m:r3429-4, lwm2m:r3429-5,
    lwm2m:r3429-6;
  prov:wasDerivedFrom <file:/data/lp/etl/executor/data/1651932849158-23-3c5fa11b-d02c-40e9-9c76-7d268eee1c69/working/working-outputfiles-214/lwm2m-registry-prod/3429.xml> .

<http://purl.org/wot-catalogue/lwm2m/ipso#3398> a skos:Concept, ontolex:LexicalConcept;
  skos:altLabel "oa physical illuminance sensor";
  skos:broader lwm2m:Object;
  skos:definition "The 'oA_Physical_Illuminance_Sensor' represents the physical part of an illuminance sensor. All logical illuminance sensors (object instances of 'oA Illuminance Sensor') are mapped to one physical illuminance sensor.";
  skos:inScheme lwm2m:Scheme;
  skos:prefLabel "oA Physical Illuminance Sensor";
  skos:related lwm2m:r3398-407, lwm2m:r3398-408, lwm2m:r3398-901, lwm2m:r3398-907, lwm2m:r3398-908,
    lwm2m:r4001;
  prov:wasDerivedFrom <file:/data/lp/etl/executor/data/1651932849158-23-3c5fa11b-d02c-40e9-9c76-7d268eee1c69/working/working-outputfiles-214/lwm2m-registry-prod/3398.xml> .

<http://purl.org/wot-catalogue/lwm2m/ipso#3383> a skos:Concept, ontolex:LexicalConcept;
  skos:altLabel "sip publish event";
  skos:broader lwm2m:Object;
  skos:definition "SIP Publish status";
  skos:inScheme lwm2m:Scheme;
  skos:prefLabel "sipPublishEvent";
  skos:related lwm2m:r3383-0;
  prov:wasDerivedFrom <file:/data/lp/etl/executor/data/1651932849158-23-3c5fa11b-d02c-40e9-9c76-7d268eee1c69/working/working-outputfiles-214/lwm2m-registry-prod/3383.xml> .

<http://purl.org/wot-catalogue/lwm2m/ipso#3305> a skos:Concept, ontolex:LexicalConcept;
  skos:altLabel "power measurement";
  skos:broader lwm2m:Object;
  skos:definition "This IPSO object should be used over a power measurement sensor to report a remote power measurement. It also provides resources for minimum/maximum measured values and the minimum/maximum range for both active and reactive power. It also provides resources for cumulative energy, calibration, and the power factor.";
  skos:inScheme lwm2m:Scheme;
  skos:prefLabel "Power Measurement";
  skos:related lwm2m:r5518, lwm2m:r5605, lwm2m:r5750, lwm2m:r5800, lwm2m:r5801, lwm2m:r5802,
    lwm2m:r5803, lwm2m:r5804, lwm2m:r5805, lwm2m:r5806, lwm2m:r5810, lwm2m:r5811, lwm2m:r5812,
    lwm2m:r5813, lwm2m:r5814, lwm2m:r5815, lwm2m:r5816, lwm2m:r5820, lwm2m:r5821, lwm2m:r5822,
    lwm2m:r6042, lwm2m:r6049, lwm2m:r6050;
  prov:wasDerivedFrom <file:/data/lp/etl/executor/data/1651932849158-23-3c5fa11b-d02c-40e9-9c76-7d268eee1c69/working/working-outputfiles-214/lwm2m-registry-prod/3305.xml> .

<http://purl.org/wot-catalogue/lwm2m/ipso#3387> a skos:Concept, ontolex:LexicalConcept;
  skos:altLabel "oa basic control";
  skos:broader lwm2m:Object;
  skos:definition "The 'oA Basic Control' represents a common basic interface for a Control Function. This allows to have vendor specific (executing) control functions using diverse object numbers to be interfaced for the basic functionality in a common way. The object provides the basic functionality required for an OpenAIS control object.";
  skos:inScheme lwm2m:Scheme;
  skos:prefLabel "oA Basic Control";
  skos:related lwm2m:r3387-800, lwm2m:r3387-801, lwm2m:r3387-802, lwm2m:r3387-803, lwm2m:r3387-805,
    lwm2m:r3387-806, lwm2m:r3387-807, lwm2m:r3387-811, lwm2m:r3387-812, lwm2m:r3387-813,
    lwm2m:r3387-901, lwm2m:r3387-905, lwm2m:r3387-906, lwm2m:r3387-909, lwm2m:r3387-924,
    lwm2m:r3387-934, lwm2m:r4001;
  prov:wasDerivedFrom <file:/data/lp/etl/executor/data/1651932849158-23-3c5fa11b-d02c-40e9-9c76-7d268eee1c69/working/working-outputfiles-214/lwm2m-registry-prod/3387.xml> .

<http://purl.org/wot-catalogue/lwm2m/ipso#3380> a skos:Concept, ontolex:LexicalConcept;
  skos:altLabel "prach report";
  skos:broader lwm2m:Object;
  skos:definition "PRACH report information";
  skos:inScheme lwm2m:Scheme;
  skos:prefLabel "PrachReport";
  skos:related lwm2m:r3380-10, lwm2m:r3380-11, lwm2m:r3380-12, lwm2m:r3380-2, lwm2m:r3380-3,
    lwm2m:r3380-4, lwm2m:r3380-5, lwm2m:r3380-6, lwm2m:r3380-7, lwm2m:r3380-8, lwm2m:r3380-9,
    lwm2m:r6037, lwm2m:r6038;
  prov:wasDerivedFrom <file:/data/lp/etl/executor/data/1651932849158-23-3c5fa11b-d02c-40e9-9c76-7d268eee1c69/working/working-outputfiles-214/lwm2m-registry-prod/3380.xml> .

<http://purl.org/wot-catalogue/lwm2m/ipso#3312> a skos:Concept, ontolex:LexicalConcept;
  skos:altLabel "power control";
  skos:broader lwm2m:Object;
  skos:definition "This Object is used to control a power source, such as a Smart Plug.  It allows a power relay to be turned on or off and its dimmer setting to be control as a % between 0 and 100.";
  skos:inScheme lwm2m:Scheme;
  skos:prefLabel "Power Control";
  skos:related lwm2m:r5518, lwm2m:r5750, lwm2m:r5805, lwm2m:r5820, lwm2m:r5850, lwm2m:r5851,
    lwm2m:r5852, lwm2m:r6050;
  prov:wasDerivedFrom <file:/data/lp/etl/executor/data/1651932849158-23-3c5fa11b-d02c-40e9-9c76-7d268eee1c69/working/working-outputfiles-214/lwm2m-registry-prod/3312.xml> .

<http://purl.org/wot-catalogue/lwm2m/ipso#3436> a skos:Concept, ontolex:LexicalConcept;
  skos:altLabel "edge computing manager";
  skos:broader lwm2m:Object;
  skos:definition "The uCIFI edge computing manager object defines the capability of a device to run scripts on the device itself.";
  skos:inScheme lwm2m:Scheme;
  skos:prefLabel "Edge computing manager";
  skos:related lwm2m:r3436-1, lwm2m:r3436-2, lwm2m:r3436-3, lwm2m:r3436-4, lwm2m:r3436-5;
  prov:wasDerivedFrom <file:/data/lp/etl/executor/data/1651932849158-23-3c5fa11b-d02c-40e9-9c76-7d268eee1c69/working/working-outputfiles-214/lwm2m-registry-prod/3436.xml> .

<http://purl.org/wot-catalogue/lwm2m/ipso#3413> a skos:Concept, ontolex:LexicalConcept;
  skos:altLabel "ucifi generic actuator";
  skos:broader lwm2m:Object;
  skos:definition "The uCIFI generic actuator may be used for any actuator but not to replace Outdoor Lamp Controllers nor for an Irrigation Valves which have a specific device type in the uCIFI data model.";
  skos:inScheme lwm2m:Scheme;
  skos:prefLabel "uCIFI Generic Actuator";
  skos:related lwm2m:r3413-1, lwm2m:r3413-2, lwm2m:r3413-3, lwm2m:r3413-4, lwm2m:r3413-5,
    lwm2m:r3413-6;
  prov:wasDerivedFrom <file:/data/lp/etl/executor/data/1651932849158-23-3c5fa11b-d02c-40e9-9c76-7d268eee1c69/working/working-outputfiles-214/lwm2m-registry-prod/3413.xml> .

<http://purl.org/wot-catalogue/lwm2m/ipso#3301> a skos:Concept, ontolex:LexicalConcept;
  skos:altLabel "illuminance";
  skos:broader lwm2m:Object;
  skos:definition "Illuminance sensor, example units = lx";
  skos:inScheme lwm2m:Scheme;
  skos:prefLabel "Illuminance";
  skos:related lwm2m:r5518, lwm2m:r5601, lwm2m:r5602, lwm2m:r5603, lwm2m:r5604, lwm2m:r5605,
    lwm2m:r5700, lwm2m:r5701, lwm2m:r5750, lwm2m:r6042, lwm2m:r6049, lwm2m:r6050;
  prov:wasDerivedFrom <file:/data/lp/etl/executor/data/1651932849158-23-3c5fa11b-d02c-40e9-9c76-7d268eee1c69/working/working-outputfiles-214/lwm2m-registry-prod/3301.xml> .

<http://purl.org/wot-catalogue/lwm2m/ipso#3368> a skos:Concept, ontolex:LexicalConcept;
  skos:altLabel "mac timer status event";
  skos:broader lwm2m:Object;
  skos:definition "MAC timer expiry information";
  skos:inScheme lwm2m:Scheme;
  skos:prefLabel "macTimerStatusEvent";
  skos:related lwm2m:r3368-0;
  prov:wasDerivedFrom <file:/data/lp/etl/executor/data/1651932849158-23-3c5fa11b-d02c-40e9-9c76-7d268eee1c69/working/working-outputfiles-214/lwm2m-registry-prod/3368.xml> .

<http://purl.org/wot-catalogue/lwm2m/ipso#3423> a skos:Concept, ontolex:LexicalConcept;
  skos:altLabel "gas meter";
  skos:broader lwm2m:Object;
  skos:definition "The uCIFI gas meter measures the volume of gas that was distributed through the gas meter, in pulse count and/or in m3. It also detects anomalies in the gas meter.";
  skos:inScheme lwm2m:Scheme;
  skos:prefLabel "Gas meter";
  skos:related lwm2m:r3423-1, lwm2m:r3423-10, lwm2m:r3423-11, lwm2m:r3423-2, lwm2m:r3423-3,
    lwm2m:r3423-4, lwm2m:r3423-5, lwm2m:r3423-6, lwm2m:r3423-7, lwm2m:r3423-8, lwm2m:r3423-9;
  prov:wasDerivedFrom <file:/data/lp/etl/executor/data/1651932849158-23-3c5fa11b-d02c-40e9-9c76-7d268eee1c69/working/working-outputfiles-214/lwm2m-registry-prod/3423.xml> .

<http://purl.org/wot-catalogue/lwm2m/ipso#3411> a skos:Concept, ontolex:LexicalConcept;
  skos:altLabel "battery";
  skos:broader lwm2m:Object;
  skos:definition "The uCIFI battery object provides attributes to monitor battery level and activity.";
  skos:inScheme lwm2m:Scheme;
  skos:prefLabel "Battery";
  skos:related lwm2m:r3411-1, lwm2m:r3411-10, lwm2m:r3411-11, lwm2m:r3411-12, lwm2m:r3411-2,
    lwm2m:r3411-3, lwm2m:r3411-4, lwm2m:r3411-5, lwm2m:r3411-6, lwm2m:r3411-7, lwm2m:r3411-8,
    lwm2m:r3411-9;
  prov:wasDerivedFrom <file:/data/lp/etl/executor/data/1651932849158-23-3c5fa11b-d02c-40e9-9c76-7d268eee1c69/working/working-outputfiles-214/lwm2m-registry-prod/3411.xml> .

<http://purl.org/wot-catalogue/lwm2m/ipso#3325> a skos:Concept, ontolex:LexicalConcept;
  skos:altLabel "concentration";
  skos:broader lwm2m:Object;
  skos:definition """This IPSO object should be used to the particle concentration measurement of a medium. It also provides resources for minimum and maximum measured values, as well as the minimum and maximum range that can be measured by the sensor. An example measurement unit is parts per million.
        """;
  skos:inScheme lwm2m:Scheme;
  skos:prefLabel "Concentration";
  skos:related lwm2m:r5518, lwm2m:r5601, lwm2m:r5602, lwm2m:r5603, lwm2m:r5604, lwm2m:r5605,
    lwm2m:r5700, lwm2m:r5701, lwm2m:r5750, lwm2m:r5821, lwm2m:r6042, lwm2m:r6049, lwm2m:r6050;
  prov:wasDerivedFrom <file:/data/lp/etl/executor/data/1651932849158-23-3c5fa11b-d02c-40e9-9c76-7d268eee1c69/working/working-outputfiles-214/lwm2m-registry-prod/3325.xml> .

<http://purl.org/wot-catalogue/lwm2m/ipso#3203> a skos:Concept, ontolex:LexicalConcept;
  skos:altLabel "analog output";
  skos:broader lwm2m:Object;
  skos:definition "This IPSO object is a generic object that can be used with any kind of analog output interface.";
  skos:inScheme lwm2m:Scheme;
  skos:prefLabel "Analog Output";
  skos:related lwm2m:r5518, lwm2m:r5603, lwm2m:r5604, lwm2m:r5650, lwm2m:r5750, lwm2m:r6050;
  prov:wasDerivedFrom <file:/data/lp/etl/executor/data/1651932849158-23-3c5fa11b-d02c-40e9-9c76-7d268eee1c69/working/working-outputfiles-214/lwm2m-registry-prod/3203.xml> .

<http://purl.org/wot-catalogue/lwm2m/ipso#3342> a skos:Concept, ontolex:LexicalConcept;
  skos:altLabel "on/off switch";
  skos:broader lwm2m:Object;
  skos:definition "This IPSO object should be used with an On/Off switch to report the state of the switch.";
  skos:inScheme lwm2m:Scheme;
  skos:prefLabel "On/Off switch";
  skos:related lwm2m:r5500, lwm2m:r5501, lwm2m:r5518, lwm2m:r5750, lwm2m:r5852, lwm2m:r5854,
    lwm2m:r6050;
  prov:wasDerivedFrom <file:/data/lp/etl/executor/data/1651932849158-23-3c5fa11b-d02c-40e9-9c76-7d268eee1c69/working/working-outputfiles-214/lwm2m-registry-prod/3342.xml> .

<http://purl.org/wot-catalogue/lwm2m/ipso#3376> a skos:Concept, ontolex:LexicalConcept;
  skos:altLabel "tx power back off event";
  skos:broader lwm2m:Object;
  skos:definition "TX Power backoff information";
  skos:inScheme lwm2m:Scheme;
  skos:prefLabel "txPowerBackOffEvent";
  skos:related lwm2m:r3376-0;
  prov:wasDerivedFrom <file:/data/lp/etl/executor/data/1651932849158-23-3c5fa11b-d02c-40e9-9c76-7d268eee1c69/working/working-outputfiles-214/lwm2m-registry-prod/3376.xml> .

<http://purl.org/wot-catalogue/lwm2m/ipso#3304> a skos:Concept, ontolex:LexicalConcept;
  skos:altLabel "humidity";
  skos:broader lwm2m:Object;
  skos:definition "This IPSO object should be used with a humidity sensor to report a humidity measurement.  It also provides resources for minimum/maximum measured values and the minimum/maximum range that can be measured by the humidity sensor. An example measurement unit is relative humidity as a percentage.";
  skos:inScheme lwm2m:Scheme;
  skos:prefLabel "Humidity";
  skos:related lwm2m:r5518, lwm2m:r5601, lwm2m:r5602, lwm2m:r5603, lwm2m:r5604, lwm2m:r5605,
    lwm2m:r5700, lwm2m:r5701, lwm2m:r5750, lwm2m:r6042, lwm2m:r6049, lwm2m:r6050;
  prov:wasDerivedFrom <file:/data/lp/etl/executor/data/1651932849158-23-3c5fa11b-d02c-40e9-9c76-7d268eee1c69/working/working-outputfiles-214/lwm2m-registry-prod/3304.xml> .

<http://purl.org/wot-catalogue/lwm2m/ipso#3370> a skos:Concept, ontolex:LexicalConcept;
  skos:altLabel "serving cell measurement";
  skos:broader lwm2m:Object;
  skos:definition "Serving Cell Measurement";
  skos:inScheme lwm2m:Scheme;
  skos:prefLabel "ServingCellMeasurement";
  skos:related lwm2m:r6032, lwm2m:r6034, lwm2m:r6035, lwm2m:r6036, lwm2m:r6037, lwm2m:r6038;
  prov:wasDerivedFrom <file:/data/lp/etl/executor/data/1651932849158-23-3c5fa11b-d02c-40e9-9c76-7d268eee1c69/working/working-outputfiles-214/lwm2m-registry-prod/3370.xml> .

<http://purl.org/wot-catalogue/lwm2m/ipso#3333> a skos:Concept, ontolex:LexicalConcept;
  skos:altLabel "time";
  skos:broader lwm2m:Object;
  skos:definition """This IPSO object is used to report the current time in seconds since January 1, 1970 UTC. There is also a fractional time counter that has a range of less than one second.
        """;
  skos:inScheme lwm2m:Scheme;
  skos:prefLabel "Time";
  skos:related lwm2m:r5506, lwm2m:r5507, lwm2m:r5750, lwm2m:r6042, lwm2m:r6049;
  prov:wasDerivedFrom <file:/data/lp/etl/executor/data/1651932849158-23-3c5fa11b-d02c-40e9-9c76-7d268eee1c69/working/working-outputfiles-214/lwm2m-registry-prod/3333.xml> .

<http://purl.org/wot-catalogue/lwm2m/ipso#3382> a skos:Concept, ontolex:LexicalConcept;
  skos:altLabel "sip registration event";
  skos:broader lwm2m:Object;
  skos:definition "SIP Registration status";
  skos:inScheme lwm2m:Scheme;
  skos:prefLabel "SipRegistrationEvent";
  skos:related lwm2m:r3382-0, lwm2m:r3382-1;
  prov:wasDerivedFrom <file:/data/lp/etl/executor/data/1651932849158-23-3c5fa11b-d02c-40e9-9c76-7d268eee1c69/working/working-outputfiles-214/lwm2m-registry-prod/3382.xml> .

<http://purl.org/wot-catalogue/lwm2m/ipso#3365> a skos:Concept, ontolex:LexicalConcept;
  skos:altLabel "rach latency delay";
  skos:broader lwm2m:Object;
  skos:definition "RACH Latency & delay information";
  skos:inScheme lwm2m:Scheme;
  skos:prefLabel "rachLatency_delay";
  skos:related lwm2m:r3365-2, lwm2m:r3365-3, lwm2m:r6037, lwm2m:r6038;
  prov:wasDerivedFrom <file:/data/lp/etl/executor/data/1651932849158-23-3c5fa11b-d02c-40e9-9c76-7d268eee1c69/working/working-outputfiles-214/lwm2m-registry-prod/3365.xml> .

<http://purl.org/wot-catalogue/lwm2m/ipso#3346> a skos:Concept, ontolex:LexicalConcept;
  skos:altLabel "rate";
  skos:broader lwm2m:Object;
  skos:definition """This object type should be used to report a rate measurement, for example the speed of a vehicle, or the rotational speed of a drive shaft. It also provides resources for minimum and maximum measured values, as well as the minimum and maximum range that can be measured by the sensor. An example measurement unit is meters per second (m/s).
        """;
  skos:inScheme lwm2m:Scheme;
  skos:prefLabel "Rate";
  skos:related lwm2m:r5518, lwm2m:r5601, lwm2m:r5602, lwm2m:r5603, lwm2m:r5604, lwm2m:r5605,
    lwm2m:r5700, lwm2m:r5701, lwm2m:r5750, lwm2m:r5821, lwm2m:r6042, lwm2m:r6049, lwm2m:r6050;
  prov:wasDerivedFrom <file:/data/lp/etl/executor/data/1651932849158-23-3c5fa11b-d02c-40e9-9c76-7d268eee1c69/working/working-outputfiles-214/lwm2m-registry-prod/3346.xml> .

<http://purl.org/wot-catalogue/lwm2m/ipso#3391> a skos:Concept, ontolex:LexicalConcept;
  skos:altLabel "oa logical colour temperature light-point actuator";
  skos:broader lwm2m:Object;
  skos:definition "The 'oA Logical Colour_Temperature Light Point Actuator' represents the logical part of an actuator model for a tunable white light point. The corresponding physical device is a light channel and associated gear (e.g. LED driver).\\nThe Object (module) supports several interactions that include absolute and relative colour temperature setting. Several device configuration parameters are mapped, which relate to behaviour or describe device limitations. Note that the overall intensity is not controlled by this object, it remains controlled by a logical light point object to ease dimming action across tuneable, coloured and non coloured lights. Please note also, that the corresponding executing object does not need to be restricted to tuneable white operation.";
  skos:inScheme lwm2m:Scheme;
  skos:prefLabel "oA Logical Colour Temperature Light-Point Actuator";
  skos:related lwm2m:r3391-139, lwm2m:r3391-140, lwm2m:r3391-141, lwm2m:r3391-142, lwm2m:r3391-143,
    lwm2m:r3391-144, lwm2m:r3391-145, lwm2m:r3391-146, lwm2m:r3391-901, lwm2m:r3391-902,
    lwm2m:r3391-903, lwm2m:r3391-904, lwm2m:r3391-905, lwm2m:r3391-906, lwm2m:r3391-909,
    lwm2m:r3391-919, lwm2m:r3391-921, lwm2m:r3391-922, lwm2m:r3391-924, lwm2m:r3391-934,
    lwm2m:r4001;
  prov:wasDerivedFrom <file:/data/lp/etl/executor/data/1651932849158-23-3c5fa11b-d02c-40e9-9c76-7d268eee1c69/working/working-outputfiles-214/lwm2m-registry-prod/3391.xml> .

<http://purl.org/wot-catalogue/lwm2m/ipso#3360> a skos:Concept, ontolex:LexicalConcept;
  skos:altLabel "esm context info";
  skos:broader lwm2m:Object;
  skos:definition "ESM context information";
  skos:inScheme lwm2m:Scheme;
  skos:prefLabel "esmContextInfo";
  skos:related lwm2m:r3360-0, lwm2m:r3360-1, lwm2m:r3360-2, lwm2m:r3360-3;
  prov:wasDerivedFrom <file:/data/lp/etl/executor/data/1651932849158-23-3c5fa11b-d02c-40e9-9c76-7d268eee1c69/working/working-outputfiles-214/lwm2m-registry-prod/3360.xml> .

<http://purl.org/wot-catalogue/lwm2m/ipso#3373> a skos:Concept, ontolex:LexicalConcept;
  skos:altLabel "tx power headroom event";
  skos:broader lwm2m:Object;
  skos:definition "TX power headroom information";
  skos:inScheme lwm2m:Scheme;
  skos:prefLabel "txPowerHeadroomEvent";
  skos:related lwm2m:r3373-2, lwm2m:r6037, lwm2m:r6038;
  prov:wasDerivedFrom <file:/data/lp/etl/executor/data/1651932849158-23-3c5fa11b-d02c-40e9-9c76-7d268eee1c69/working/working-outputfiles-214/lwm2m-registry-prod/3373.xml> .

<http://purl.org/wot-catalogue/lwm2m/ipso#3315> a skos:Concept, ontolex:LexicalConcept;
  skos:altLabel "barometer";
  skos:broader lwm2m:Object;
  skos:definition "This IPSO object should be used with an air pressure sensor to report a barometer measurement.  It also provides resources for minimum/maximum measured values and the minimum/maximum range that can be measured by the barometer sensor. An example measurement unit is pascals.";
  skos:inScheme lwm2m:Scheme;
  skos:prefLabel "Barometer";
  skos:related lwm2m:r5518, lwm2m:r5601, lwm2m:r5602, lwm2m:r5603, lwm2m:r5604, lwm2m:r5605,
    lwm2m:r5700, lwm2m:r5701, lwm2m:r5750, lwm2m:r6042, lwm2m:r6049, lwm2m:r6050;
  prov:wasDerivedFrom <file:/data/lp/etl/executor/data/1651932849158-23-3c5fa11b-d02c-40e9-9c76-7d268eee1c69/working/working-outputfiles-214/lwm2m-registry-prod/3315.xml> .

<http://purl.org/wot-catalogue/lwm2m/ipso#3408> a skos:Concept, ontolex:LexicalConcept;
  skos:altLabel "manhole cover";
  skos:broader lwm2m:Object;
  skos:definition "Describe the status of a manhole cover.";
  skos:inScheme lwm2m:Scheme;
  skos:prefLabel "Manhole Cover";
  skos:related lwm2m:r3408-1, lwm2m:r3408-2, lwm2m:r3408-3;
  prov:wasDerivedFrom <file:/data/lp/etl/executor/data/1651932849158-23-3c5fa11b-d02c-40e9-9c76-7d268eee1c69/working/working-outputfiles-214/lwm2m-registry-prod/3408.xml> .

<http://purl.org/wot-catalogue/lwm2m/ipso#3415> a skos:Concept, ontolex:LexicalConcept;
  skos:altLabel "time synchronization";
  skos:broader lwm2m:Object;
  skos:definition "The uCIFI time synchronization object enables a device to sync-up its internal clock with a remote NTP server.";
  skos:inScheme lwm2m:Scheme;
  skos:prefLabel "Time synchronization";
  skos:related lwm2m:r3415-1, lwm2m:r3415-2, lwm2m:r3415-3, lwm2m:r3415-4, lwm2m:r3415-5;
  prov:wasDerivedFrom <file:/data/lp/etl/executor/data/1651932849158-23-3c5fa11b-d02c-40e9-9c76-7d268eee1c69/working/working-outputfiles-214/lwm2m-registry-prod/3415.xml> .

<http://purl.org/wot-catalogue/lwm2m/ipso#3335> a skos:Concept, ontolex:LexicalConcept;
  skos:altLabel "colour";
  skos:broader lwm2m:Object;
  skos:definition """This IPSO object should be used to report the measured value of a colour sensor in some colour space described by the units resource.
        """;
  skos:inScheme lwm2m:Scheme;
  skos:prefLabel "Colour";
  skos:related lwm2m:r5518, lwm2m:r5701, lwm2m:r5706, lwm2m:r5750, lwm2m:r6042, lwm2m:r6049,
    lwm2m:r6050;
  prov:wasDerivedFrom <file:/data/lp/etl/executor/data/1651932849158-23-3c5fa11b-d02c-40e9-9c76-7d268eee1c69/working/working-outputfiles-214/lwm2m-registry-prod/3335.xml> .

<http://purl.org/wot-catalogue/lwm2m/ipso#3361> a skos:Concept, ontolex:LexicalConcept;
  skos:altLabel "emm state value";
  skos:broader lwm2m:Object;
  skos:definition "EMM context information";
  skos:inScheme lwm2m:Scheme;
  skos:prefLabel "emmStateValue";
  skos:related lwm2m:r3361-0, lwm2m:r3361-1;
  prov:wasDerivedFrom <file:/data/lp/etl/executor/data/1651932849158-23-3c5fa11b-d02c-40e9-9c76-7d268eee1c69/working/working-outputfiles-214/lwm2m-registry-prod/3361.xml> .

<http://purl.org/wot-catalogue/lwm2m/ipso#3371> a skos:Concept, ontolex:LexicalConcept;
  skos:altLabel "neighbor cell measurements";
  skos:broader lwm2m:Object;
  skos:definition "Neighbor Cell Measurements";
  skos:inScheme lwm2m:Scheme;
  skos:prefLabel "NeighborCellMeasurements";
  skos:related lwm2m:r6032, lwm2m:r6034, lwm2m:r6035, lwm2m:r6036, lwm2m:r6037, lwm2m:r6038;
  prov:wasDerivedFrom <file:/data/lp/etl/executor/data/1651932849158-23-3c5fa11b-d02c-40e9-9c76-7d268eee1c69/working/working-outputfiles-214/lwm2m-registry-prod/3371.xml> .

<http://purl.org/wot-catalogue/lwm2m/ipso#3405> a skos:Concept, ontolex:LexicalConcept;
  skos:altLabel "oa ogc-security";
  skos:broader lwm2m:Object;
  skos:definition "The 'OGC Security' provides the appropriate keying material for a specific OGC Application group in the context of OGC. The keying material will be provided by a key distribution server, and must not be readable by any instance outside the local node.";
  skos:inScheme lwm2m:Scheme;
  skos:prefLabel "oA OGC-Security";
  skos:related lwm2m:r3405-0, lwm2m:r3405-3, lwm2m:r3405-5, lwm2m:r3405-901, lwm2m:r4001;
  prov:wasDerivedFrom <file:/data/lp/etl/executor/data/1651932849158-23-3c5fa11b-d02c-40e9-9c76-7d268eee1c69/working/working-outputfiles-214/lwm2m-registry-prod/3405.xml> .

<http://purl.org/wot-catalogue/lwm2m/ipso#3418> a skos:Concept, ontolex:LexicalConcept;
  skos:altLabel "electrical monitor";
  skos:broader lwm2m:Object;
  skos:definition "The uCIFI electrical monitor object provides attributes related to the analysis of electrical consumption in an outdoor luminaire or in a streetlight cabinet. It also identifies electrical anomalies.";
  skos:inScheme lwm2m:Scheme;
  skos:prefLabel "Electrical monitor";
  skos:related lwm2m:r3418-1, lwm2m:r3418-10, lwm2m:r3418-11, lwm2m:r3418-12, lwm2m:r3418-13,
    lwm2m:r3418-14, lwm2m:r3418-15, lwm2m:r3418-16, lwm2m:r3418-17, lwm2m:r3418-18, lwm2m:r3418-19,
    lwm2m:r3418-2, lwm2m:r3418-20, lwm2m:r3418-21, lwm2m:r3418-22, lwm2m:r3418-23, lwm2m:r3418-24,
    lwm2m:r3418-25, lwm2m:r3418-26, lwm2m:r3418-27, lwm2m:r3418-28, lwm2m:r3418-29, lwm2m:r3418-3,
    lwm2m:r3418-30, lwm2m:r3418-4, lwm2m:r3418-5, lwm2m:r3418-6, lwm2m:r3418-7, lwm2m:r3418-8,
    lwm2m:r3418-9;
  prov:wasDerivedFrom <file:/data/lp/etl/executor/data/1651932849158-23-3c5fa11b-d02c-40e9-9c76-7d268eee1c69/working/working-outputfiles-214/lwm2m-registry-prod/3418.xml> .

<http://purl.org/wot-catalogue/lwm2m/ipso#3377> a skos:Concept, ontolex:LexicalConcept;
  skos:altLabel "message3report";
  skos:broader lwm2m:Object;
  skos:definition "RACH message 3 report information";
  skos:inScheme lwm2m:Scheme;
  skos:prefLabel "Message3Report";
  skos:related lwm2m:r3377-0, lwm2m:r3377-1, lwm2m:r3377-2, lwm2m:r3377-3, lwm2m:r3377-4,
    lwm2m:r3377-5, lwm2m:r3377-6, lwm2m:r3377-7, lwm2m:r3377-8;
  prov:wasDerivedFrom <file:/data/lp/etl/executor/data/1651932849158-23-3c5fa11b-d02c-40e9-9c76-7d268eee1c69/working/working-outputfiles-214/lwm2m-registry-prod/3377.xml> .

<http://purl.org/wot-catalogue/lwm2m/ipso#3330> a skos:Concept, ontolex:LexicalConcept;
  skos:altLabel "distance";
  skos:broader lwm2m:Object;
  skos:definition """This IPSO object should be used to report a distance measurement. It also provides resources for minimum and maximum measured values, as well as the minimum and maximum range that can be measured by the sensor. An example measurement unit is Meters.
        """;
  skos:inScheme lwm2m:Scheme;
  skos:prefLabel "Distance";
  skos:related lwm2m:r5518, lwm2m:r5601, lwm2m:r5602, lwm2m:r5603, lwm2m:r5604, lwm2m:r5605,
    lwm2m:r5700, lwm2m:r5701, lwm2m:r5750, lwm2m:r5821, lwm2m:r6042, lwm2m:r6049, lwm2m:r6050;
  prov:wasDerivedFrom <file:/data/lp/etl/executor/data/1651932849158-23-3c5fa11b-d02c-40e9-9c76-7d268eee1c69/working/working-outputfiles-214/lwm2m-registry-prod/3330.xml> .

<http://purl.org/wot-catalogue/lwm2m/ipso#3323> a skos:Concept, ontolex:LexicalConcept;
  skos:altLabel "pressure";
  skos:broader lwm2m:Object;
  skos:definition """This IPSO object should be used to report pressure measurements. It also provides resources for minimum and maximum measured values, as well as the minimum and maximum range that can be measured by the sensor. An example measurement unit is pascals.
        """;
  skos:inScheme lwm2m:Scheme;
  skos:prefLabel "Pressure";
  skos:related lwm2m:r5518, lwm2m:r5601, lwm2m:r5602, lwm2m:r5603, lwm2m:r5604, lwm2m:r5605,
    lwm2m:r5700, lwm2m:r5701, lwm2m:r5750, lwm2m:r5821, lwm2m:r6042, lwm2m:r6049, lwm2m:r6050;
  prov:wasDerivedFrom <file:/data/lp/etl/executor/data/1651932849158-23-3c5fa11b-d02c-40e9-9c76-7d268eee1c69/working/working-outputfiles-214/lwm2m-registry-prod/3323.xml> .

<http://purl.org/wot-catalogue/lwm2m/ipso#3300> a skos:Concept, ontolex:LexicalConcept;
  skos:altLabel "generic sensor";
  skos:broader lwm2m:Object;
  skos:definition "This IPSO object allows the description of a generic sensor. It is based on the description of a value and a unit according to the SenML specification. Thus, any type of value defined within this specification can be reported using this object. This object may be used as a generic object if a dedicated one does not exist.";
  skos:inScheme lwm2m:Scheme;
  skos:prefLabel "Generic Sensor";
  skos:related lwm2m:r5518, lwm2m:r5601, lwm2m:r5602, lwm2m:r5603, lwm2m:r5604, lwm2m:r5605,
    lwm2m:r5700, lwm2m:r5701, lwm2m:r5750, lwm2m:r5751, lwm2m:r6042, lwm2m:r6049, lwm2m:r6050;
  prov:wasDerivedFrom <file:/data/lp/etl/executor/data/1651932849158-23-3c5fa11b-d02c-40e9-9c76-7d268eee1c69/working/working-outputfiles-214/lwm2m-registry-prod/3300.xml> .

<http://purl.org/wot-catalogue/lwm2m/ipso#3322> a skos:Concept, ontolex:LexicalConcept;
  skos:altLabel "load";
  skos:broader lwm2m:Object;
  skos:definition """This IPSO object should be used with a load sensor (as in a scale) to report the applied weight or force. It also provides resources for minimum and maximum measured values, as well as the minimum and maximum range that can be measured by the sensor. An example measurement unit is kilograms.
        """;
  skos:inScheme lwm2m:Scheme;
  skos:prefLabel "Load";
  skos:related lwm2m:r5518, lwm2m:r5601, lwm2m:r5602, lwm2m:r5603, lwm2m:r5604, lwm2m:r5605,
    lwm2m:r5700, lwm2m:r5701, lwm2m:r5750, lwm2m:r5821, lwm2m:r6042, lwm2m:r6049, lwm2m:r6050;
  prov:wasDerivedFrom <file:/data/lp/etl/executor/data/1651932849158-23-3c5fa11b-d02c-40e9-9c76-7d268eee1c69/working/working-outputfiles-214/lwm2m-registry-prod/3322.xml> .

<http://purl.org/wot-catalogue/lwm2m/ipso#3441> a skos:Concept, ontolex:LexicalConcept;
  skos:altLabel "lwm2m v1.0 test object";
  skos:broader lwm2m:Object;
  skos:definition "This object is for use in interoperability tests of the LwM2M v1.0 technical specification. It contains resources for each available datatype.";
  skos:inScheme lwm2m:Scheme;
  skos:prefLabel "LwM2M v1.0 Test Object";
  skos:related lwm2m:r3441-0, lwm2m:r3441-1, lwm2m:r3441-110, lwm2m:r3441-1110, lwm2m:r3441-1120,
    lwm2m:r3441-1130, lwm2m:r3441-1140, lwm2m:r3441-1150, lwm2m:r3441-1160, lwm2m:r3441-1170,
    lwm2m:r3441-120, lwm2m:r3441-130, lwm2m:r3441-140, lwm2m:r3441-150, lwm2m:r3441-160,
    lwm2m:r3441-170, lwm2m:r3441-2, lwm2m:r3441-3, lwm2m:r3441-4;
  prov:wasDerivedFrom <file:/data/lp/etl/executor/data/1651932849158-23-3c5fa11b-d02c-40e9-9c76-7d268eee1c69/working/working-outputfiles-214/lwm2m-registry-prod/3441.xml> .

<http://purl.org/wot-catalogue/lwm2m/ipso#3425> a skos:Concept, ontolex:LexicalConcept;
  skos:altLabel "irrigation valve";
  skos:broader lwm2m:Object;
  skos:definition "The uCIFI irrigation valve provides a way to control and monitor an irrigation valve.";
  skos:inScheme lwm2m:Scheme;
  skos:prefLabel "Irrigation valve";
  skos:related lwm2m:r3425-1, lwm2m:r3425-2, lwm2m:r3425-3, lwm2m:r3425-4, lwm2m:r3425-5,
    lwm2m:r3425-6;
  prov:wasDerivedFrom <file:/data/lp/etl/executor/data/1651932849158-23-3c5fa11b-d02c-40e9-9c76-7d268eee1c69/working/working-outputfiles-214/lwm2m-registry-prod/3425.xml> .

<http://purl.org/wot-catalogue/lwm2m/ipso#3338> a skos:Concept, ontolex:LexicalConcept;
  skos:altLabel "buzzer";
  skos:broader lwm2m:Object;
  skos:definition """This IPSO object should be used to actuate an audible alarm such as a buzzer, beeper, or vibration alarm. There is a dimmer control for setting the relative level of the alarm, and an optional duration control to limit the length of time the alarm sounds when turned on. Each time \"true\" is written to the On/Off resource, the alarm will sound again for the configured duration. If no duration is programmed or the setting is \"false\", writing a \"true\" to the On/Off resource will result in the alarm sounding continuously until a \"false\" is written to the On/Off resource.
        """;
  skos:inScheme lwm2m:Scheme;
  skos:prefLabel "Buzzer";
  skos:related lwm2m:r5518, lwm2m:r5521, lwm2m:r5525, lwm2m:r5548, lwm2m:r5750, lwm2m:r5850,
    lwm2m:r6050;
  prov:wasDerivedFrom <file:/data/lp/etl/executor/data/1651932849158-23-3c5fa11b-d02c-40e9-9c76-7d268eee1c69/working/working-outputfiles-214/lwm2m-registry-prod/3338.xml> .

<http://purl.org/wot-catalogue/lwm2m/ipso#3428> a skos:Concept, ontolex:LexicalConcept;
  skos:altLabel "air quality";
  skos:broader lwm2m:Object;
  skos:definition "The uCIFI air quality sensor reports measurement required to calculate Air Quality Index (AIQ. It also provides resources for average calculation as per the IQ index calculation.";
  skos:inScheme lwm2m:Scheme;
  skos:prefLabel "Air quality";
  skos:related lwm2m:r3428-1, lwm2m:r3428-10, lwm2m:r3428-11, lwm2m:r3428-12, lwm2m:r3428-13,
    lwm2m:r3428-14, lwm2m:r3428-15, lwm2m:r3428-16, lwm2m:r3428-17, lwm2m:r3428-18, lwm2m:r3428-19,
    lwm2m:r3428-2, lwm2m:r3428-20, lwm2m:r3428-21, lwm2m:r3428-22, lwm2m:r3428-3, lwm2m:r3428-4,
    lwm2m:r3428-5, lwm2m:r3428-6, lwm2m:r3428-7, lwm2m:r3428-8, lwm2m:r3428-9;
  prov:wasDerivedFrom <file:/data/lp/etl/executor/data/1651932849158-23-3c5fa11b-d02c-40e9-9c76-7d268eee1c69/working/working-outputfiles-214/lwm2m-registry-prod/3428.xml> .

<http://purl.org/wot-catalogue/lwm2m/ipso#3310> a skos:Concept, ontolex:LexicalConcept;
  skos:altLabel "load control";
  skos:broader lwm2m:Object;
  skos:definition "This Object is used for demand-response load control and other load control in automation application (not limited to power).";
  skos:inScheme lwm2m:Scheme;
  skos:prefLabel "Load Control";
  skos:related lwm2m:r5518, lwm2m:r5750, lwm2m:r5823, lwm2m:r5824, lwm2m:r5825, lwm2m:r5826,
    lwm2m:r5827, lwm2m:r5828, lwm2m:r6050;
  prov:wasDerivedFrom <file:/data/lp/etl/executor/data/1651932849158-23-3c5fa11b-d02c-40e9-9c76-7d268eee1c69/working/working-outputfiles-214/lwm2m-registry-prod/3310.xml> .

<http://purl.org/wot-catalogue/lwm2m/ipso#3384> a skos:Concept, ontolex:LexicalConcept;
  skos:altLabel "sip subscription event";
  skos:broader lwm2m:Object;
  skos:definition "SIP Subscription status";
  skos:inScheme lwm2m:Scheme;
  skos:prefLabel "sipSubscriptionEvent";
  skos:related lwm2m:r3384-0, lwm2m:r3384-1;
  prov:wasDerivedFrom <file:/data/lp/etl/executor/data/1651932849158-23-3c5fa11b-d02c-40e9-9c76-7d268eee1c69/working/working-outputfiles-214/lwm2m-registry-prod/3384.xml> .

<http://purl.org/wot-catalogue/lwm2m/ipso#3359> a skos:Concept, ontolex:LexicalConcept;
  skos:altLabel "cell blacklist event";
  skos:broader lwm2m:Object;
  skos:definition "Cell blacklist information";
  skos:inScheme lwm2m:Scheme;
  skos:prefLabel "cellBlacklistEvent";
  skos:related lwm2m:r6032, lwm2m:r6033;
  prov:wasDerivedFrom <file:/data/lp/etl/executor/data/1651932849158-23-3c5fa11b-d02c-40e9-9c76-7d268eee1c69/working/working-outputfiles-214/lwm2m-registry-prod/3359.xml> .

<http://purl.org/wot-catalogue/lwm2m/ipso#3320> a skos:Concept, ontolex:LexicalConcept;
  skos:altLabel "percentage";
  skos:broader lwm2m:Object;
  skos:definition """This IPSO object should can be used to report measurements relative to a 0-100% scale. For example it could be used to measure the level of a liquid in a vessel or container in units of %.
        """;
  skos:inScheme lwm2m:Scheme;
  skos:prefLabel "Percentage";
  skos:related lwm2m:r5518, lwm2m:r5601, lwm2m:r5602, lwm2m:r5603, lwm2m:r5604, lwm2m:r5605,
    lwm2m:r5700, lwm2m:r5701, lwm2m:r5750, lwm2m:r5821, lwm2m:r6042, lwm2m:r6049, lwm2m:r6050;
  prov:wasDerivedFrom <file:/data/lp/etl/executor/data/1651932849158-23-3c5fa11b-d02c-40e9-9c76-7d268eee1c69/working/working-outputfiles-214/lwm2m-registry-prod/3320.xml> .

<http://purl.org/wot-catalogue/lwm2m/ipso#2050> a skos:Concept, ontolex:LexicalConcept;
  skos:altLabel "cmdh defaults";
  skos:broader lwm2m:Object;
  skos:definition "Defines which CMDH related parameters will be used by default. ";
  skos:inScheme lwm2m:Scheme;
  skos:prefLabel "CmdhDefaults";
  skos:related lwm2m:r2050-0, lwm2m:r2050-1;
  prov:wasDerivedFrom <file:/data/lp/etl/executor/data/1651932849158-23-3c5fa11b-d02c-40e9-9c76-7d268eee1c69/working/working-outputfiles-214/lwm2m-registry-prod/2050.xml> .

<http://purl.org/wot-catalogue/lwm2m/ipso#3303> a skos:Concept, ontolex:LexicalConcept;
  skos:altLabel "temperature";
  skos:broader lwm2m:Object;
  skos:definition "This IPSO object should be used with a temperature sensor to report a temperature measurement.  It also provides resources for minimum/maximum measured values and the minimum/maximum range that can be measured by the temperature sensor. An example measurement unit is degrees Celsius.";
  skos:inScheme lwm2m:Scheme;
  skos:prefLabel "Temperature";
  skos:related lwm2m:r5518, lwm2m:r5601, lwm2m:r5602, lwm2m:r5603, lwm2m:r5604, lwm2m:r5605,
    lwm2m:r5700, lwm2m:r5701, lwm2m:r5750, lwm2m:r6042, lwm2m:r6049, lwm2m:r6050;
  prov:wasDerivedFrom <file:/data/lp/etl/executor/data/1651932849158-23-3c5fa11b-d02c-40e9-9c76-7d268eee1c69/working/working-outputfiles-214/lwm2m-registry-prod/3303.xml> .

<http://purl.org/wot-catalogue/lwm2m/ipso#3427> a skos:Concept, ontolex:LexicalConcept;
  skos:altLabel "pressure monitoring sensor";
  skos:broader lwm2m:Object;
  skos:definition "The uCIFI water pressure monitoring sensor measures water pressure and help identify water leaks in water distribution pipelines.";
  skos:inScheme lwm2m:Scheme;
  skos:prefLabel "Pressure monitoring sensor";
  skos:related lwm2m:r3427-1, lwm2m:r3427-2, lwm2m:r3427-3, lwm2m:r3427-4, lwm2m:r3427-5,
    lwm2m:r3427-6, lwm2m:r3427-7, lwm2m:r3427-8, lwm2m:r3427-9;
  prov:wasDerivedFrom <file:/data/lp/etl/executor/data/1651932849158-23-3c5fa11b-d02c-40e9-9c76-7d268eee1c69/working/working-outputfiles-214/lwm2m-registry-prod/3427.xml> .

<http://purl.org/wot-catalogue/lwm2m/ipso#3374> a skos:Concept, ontolex:LexicalConcept;
  skos:altLabel "radio link monitoring";
  skos:broader lwm2m:Object;
  skos:definition "Radio Link monitoring information maintained by RRC";
  skos:inScheme lwm2m:Scheme;
  skos:prefLabel "radioLinkMonitoring";
  skos:related lwm2m:r3374-2, lwm2m:r3374-3, lwm2m:r3374-4, lwm2m:r6037, lwm2m:r6038;
  prov:wasDerivedFrom <file:/data/lp/etl/executor/data/1651932849158-23-3c5fa11b-d02c-40e9-9c76-7d268eee1c69/working/working-outputfiles-214/lwm2m-registry-prod/3374.xml> .

<http://purl.org/wot-catalogue/lwm2m/ipso#3339> a skos:Concept, ontolex:LexicalConcept;
  skos:altLabel "audio clip";
  skos:broader lwm2m:Object;
  skos:definition "This IPSO object should be used for a speaker that plays a pre-recorded audio clip or an audio output that is sent elsewhere. For example, an elevator which announces the floor of the building. A resource is provided to store the clip, a dimmer resource controls the relative sound level of the playback, and a duration resource limits the maximum playback time. After the duration time is reached, any remaining samples in the clip are ignored, and the clip player will be ready to play another clip.";
  skos:inScheme lwm2m:Scheme;
  skos:prefLabel "Audio Clip";
  skos:related lwm2m:r5522, lwm2m:r5523, lwm2m:r5524, lwm2m:r5548, lwm2m:r5750;
  prov:wasDerivedFrom <file:/data/lp/etl/executor/data/1651932849158-23-3c5fa11b-d02c-40e9-9c76-7d268eee1c69/working/working-outputfiles-214/lwm2m-registry-prod/3339.xml> .

<http://purl.org/wot-catalogue/lwm2m/ipso#2048> a skos:Concept, ontolex:LexicalConcept;
  skos:altLabel "cmdh policy";
  skos:broader lwm2m:Object;
  skos:definition "This Object provides links to a set of rules associated with a specific CSE that governs the behavior of that CSE regarding rejecting, buffering and sending request or response messages via the Mcc reference point.";
  skos:inScheme lwm2m:Scheme;
  skos:prefLabel "CmdhPolicy";
  skos:related lwm2m:r2048-0, lwm2m:r2048-1, lwm2m:r2048-2, lwm2m:r2048-3, lwm2m:r2048-4;
  prov:wasDerivedFrom <file:/data/lp/etl/executor/data/1651932849158-23-3c5fa11b-d02c-40e9-9c76-7d268eee1c69/working/working-outputfiles-214/lwm2m-registry-prod/2048.xml> .

<http://purl.org/wot-catalogue/lwm2m/ipso#3343> a skos:Concept, ontolex:LexicalConcept;
  skos:altLabel "dimmer";
  skos:broader lwm2m:Object;
  skos:definition """This IPSO object should be used with a dimmer or level control to report the state of the control.
        """;
  skos:inScheme lwm2m:Scheme;
  skos:prefLabel "Dimmer";
  skos:related lwm2m:r5548, lwm2m:r5750, lwm2m:r5852, lwm2m:r5854;
  prov:wasDerivedFrom <file:/data/lp/etl/executor/data/1651932849158-23-3c5fa11b-d02c-40e9-9c76-7d268eee1c69/working/working-outputfiles-214/lwm2m-registry-prod/3343.xml> .

<http://purl.org/wot-catalogue/lwm2m/ipso#3381> a skos:Concept, ontolex:LexicalConcept;
  skos:altLabel "volte call event";
  skos:broader lwm2m:Object;
  skos:definition "VoLTE call status";
  skos:inScheme lwm2m:Scheme;
  skos:prefLabel "VolteCallEvent";
  skos:related lwm2m:r3381-0, lwm2m:r3381-1;
  prov:wasDerivedFrom <file:/data/lp/etl/executor/data/1651932849158-23-3c5fa11b-d02c-40e9-9c76-7d268eee1c69/working/working-outputfiles-214/lwm2m-registry-prod/3381.xml> .

<http://purl.org/wot-catalogue/lwm2m/ipso#3348> a skos:Concept, ontolex:LexicalConcept;
  skos:altLabel "multi-state selector";
  skos:broader lwm2m:Object;
  skos:definition """This IPSO object is used to represent the state of a Multi-state selector switch with a number of fixed positions.
        """;
  skos:inScheme lwm2m:Scheme;
  skos:prefLabel "Multi-state Selector";
  skos:related lwm2m:r5518, lwm2m:r5547, lwm2m:r5750, lwm2m:r6050;
  prov:wasDerivedFrom <file:/data/lp/etl/executor/data/1651932849158-23-3c5fa11b-d02c-40e9-9c76-7d268eee1c69/working/working-outputfiles-214/lwm2m-registry-prod/3348.xml> .

<http://purl.org/wot-catalogue/lwm2m/ipso#3438> a skos:Concept, ontolex:LexicalConcept;
  skos:altLabel "edge computing time condition";
  skos:broader lwm2m:Object;
  skos:definition "The uCIFI edge computing time condition object defines the day/time (defined as a CRON rule) at which a particular script should be executed by a device.";
  skos:inScheme lwm2m:Scheme;
  skos:prefLabel "Edge computing time condition";
  skos:related lwm2m:r3438-1, lwm2m:r3438-2, lwm2m:r3438-3;
  prov:wasDerivedFrom <file:/data/lp/etl/executor/data/1651932849158-23-3c5fa11b-d02c-40e9-9c76-7d268eee1c69/working/working-outputfiles-214/lwm2m-registry-prod/3438.xml> .

<http://purl.org/wot-catalogue/lwm2m/ipso#3327> a skos:Concept, ontolex:LexicalConcept;
  skos:altLabel "conductivity";
  skos:broader lwm2m:Object;
  skos:definition """This IPSO object should be used to report a measurement of the electric conductivity of a medium or sample. It also provides resources for minimum and maximum measured values, as well as the minimum and maximum range that can be measured by the sensor. An example measurement unit is Siemens.
        """;
  skos:inScheme lwm2m:Scheme;
  skos:prefLabel "Conductivity";
  skos:related lwm2m:r5518, lwm2m:r5601, lwm2m:r5602, lwm2m:r5603, lwm2m:r5604, lwm2m:r5605,
    lwm2m:r5700, lwm2m:r5701, lwm2m:r5750, lwm2m:r5821, lwm2m:r6042, lwm2m:r6049, lwm2m:r6050;
  prov:wasDerivedFrom <file:/data/lp/etl/executor/data/1651932849158-23-3c5fa11b-d02c-40e9-9c76-7d268eee1c69/working/working-outputfiles-214/lwm2m-registry-prod/3327.xml> .

<http://purl.org/wot-catalogue/lwm2m/ipso#3321> a skos:Concept, ontolex:LexicalConcept;
  skos:altLabel "altitude";
  skos:broader lwm2m:Object;
  skos:definition """This IPSO object should be used with an altitude sensor to report altitude above sea level in meters. Note that Altitude can be calculated from the measured pressure given the local sea level pressure.  It also provides resources for minimum and maximum measured values, as well as the minimum and maximum range that can be measured by the sensor. An example measurement unit is meters.
        """;
  skos:inScheme lwm2m:Scheme;
  skos:prefLabel "Altitude";
  skos:related lwm2m:r5518, lwm2m:r5601, lwm2m:r5602, lwm2m:r5603, lwm2m:r5604, lwm2m:r5605,
    lwm2m:r5700, lwm2m:r5701, lwm2m:r5750, lwm2m:r5821, lwm2m:r6042, lwm2m:r6049, lwm2m:r6050;
  prov:wasDerivedFrom <file:/data/lp/etl/executor/data/1651932849158-23-3c5fa11b-d02c-40e9-9c76-7d268eee1c69/working/working-outputfiles-214/lwm2m-registry-prod/3321.xml> .

<http://purl.org/wot-catalogue/lwm2m/ipso#3350> a skos:Concept, ontolex:LexicalConcept;
  skos:altLabel "stopwatch";
  skos:broader lwm2m:Object;
  skos:definition "An ascending timer that counts how long time has passed since the timer was started after reset.";
  skos:inScheme lwm2m:Scheme;
  skos:prefLabel "Stopwatch";
  skos:related lwm2m:r5501, lwm2m:r5518, lwm2m:r5544, lwm2m:r5750, lwm2m:r5850, lwm2m:r6042,
    lwm2m:r6049, lwm2m:r6050;
  prov:wasDerivedFrom <file:/data/lp/etl/executor/data/1651932849158-23-3c5fa11b-d02c-40e9-9c76-7d268eee1c69/working/working-outputfiles-214/lwm2m-registry-prod/3350.xml> .

<http://purl.org/wot-catalogue/lwm2m/ipso#3401> a skos:Concept, ontolex:LexicalConcept;
  skos:altLabel "oa physical push-button sensor";
  skos:broader lwm2m:Object;
  skos:definition "The 'oA_Physical_Push-Button_Sensor' represents the physical part of a push-button sensor. All logical push-button sensors (object instances of 'oA Push-Button Sensor') are mapped to one physical push-button sensor.";
  skos:inScheme lwm2m:Scheme;
  skos:prefLabel "oA Physical Push-Button Sensor";
  skos:related lwm2m:r3401-201, lwm2m:r3401-901, lwm2m:r3401-907, lwm2m:r3401-908, lwm2m:r4001,
    lwm2m:r5502, lwm2m:r5503;
  prov:wasDerivedFrom <file:/data/lp/etl/executor/data/1651932849158-23-3c5fa11b-d02c-40e9-9c76-7d268eee1c69/working/working-outputfiles-214/lwm2m-registry-prod/3401.xml> .

<http://purl.org/wot-catalogue/lwm2m/ipso#3351> a skos:Concept, ontolex:LexicalConcept;
  skos:altLabel "powerup log";
  skos:broader lwm2m:Object;
  skos:definition "One time event sent by the device at power up.";
  skos:inScheme lwm2m:Scheme;
  skos:prefLabel "powerupLog";
  skos:related lwm2m:r3351-0, lwm2m:r3351-1, lwm2m:r3351-2, lwm2m:r3351-3, lwm2m:r3351-4;
  prov:wasDerivedFrom <file:/data/lp/etl/executor/data/1651932849158-23-3c5fa11b-d02c-40e9-9c76-7d268eee1c69/working/working-outputfiles-214/lwm2m-registry-prod/3351.xml> .

<http://purl.org/wot-catalogue/lwm2m/ipso#3345> a skos:Concept, ontolex:LexicalConcept;
  skos:altLabel "multiple axis joystick";
  skos:broader lwm2m:Object;
  skos:definition """This IPSO object can be used to report the position of a shuttle or joystick control. A digital input is provided to report the state of an associated push button.
        """;
  skos:inScheme lwm2m:Scheme;
  skos:prefLabel "Multiple Axis Joystick";
  skos:related lwm2m:r5500, lwm2m:r5501, lwm2m:r5702, lwm2m:r5703, lwm2m:r5704, lwm2m:r5750;
  prov:wasDerivedFrom <file:/data/lp/etl/executor/data/1651932849158-23-3c5fa11b-d02c-40e9-9c76-7d268eee1c69/working/working-outputfiles-214/lwm2m-registry-prod/3345.xml> .

<http://purl.org/wot-catalogue/lwm2m/ipso#3355> a skos:Concept, ontolex:LexicalConcept;
  skos:altLabel "handover event";
  skos:broader lwm2m:Object;
  skos:definition "handover event information";
  skos:inScheme lwm2m:Scheme;
  skos:prefLabel "handoverEvent";
  skos:related lwm2m:r3355-0, lwm2m:r3355-3, lwm2m:r3355-4, lwm2m:r3355-5, lwm2m:r3355-6,
    lwm2m:r6032, lwm2m:r6033;
  prov:wasDerivedFrom <file:/data/lp/etl/executor/data/1651932849158-23-3c5fa11b-d02c-40e9-9c76-7d268eee1c69/working/working-outputfiles-214/lwm2m-registry-prod/3355.xml> .

<http://purl.org/wot-catalogue/lwm2m/ipso#3367> a skos:Concept, ontolex:LexicalConcept;
  skos:altLabel "mac rach attempt reason event";
  skos:broader lwm2m:Object;
  skos:definition "RACH Information - reason for initiating RACH";
  skos:inScheme lwm2m:Scheme;
  skos:prefLabel "macRachAttemptReasonEvent";
  skos:related lwm2m:r3367-0, lwm2m:r3367-1, lwm2m:r3367-2, lwm2m:r3367-3, lwm2m:r3367-4;
  prov:wasDerivedFrom <file:/data/lp/etl/executor/data/1651932849158-23-3c5fa11b-d02c-40e9-9c76-7d268eee1c69/working/working-outputfiles-214/lwm2m-registry-prod/3367.xml> .

<http://purl.org/wot-catalogue/lwm2m/ipso#3442> a skos:Concept, ontolex:LexicalConcept;
  skos:altLabel "lwm2m v1.1 test object";
  skos:broader lwm2m:Object;
  skos:definition "This object aims to make easier to do interoperability tests about LWM2M v1.1. It contains resources for each available datatype.";
  skos:inScheme lwm2m:Scheme;
  skos:prefLabel "LwM2M v1.1 Test Object";
  skos:related lwm2m:r3442-0, lwm2m:r3442-1, lwm2m:r3442-110, lwm2m:r3442-1110, lwm2m:r3442-1120,
    lwm2m:r3442-1125, lwm2m:r3442-1130, lwm2m:r3442-1140, lwm2m:r3442-1150, lwm2m:r3442-1160,
    lwm2m:r3442-1170, lwm2m:r3442-1180, lwm2m:r3442-120, lwm2m:r3442-125, lwm2m:r3442-130,
    lwm2m:r3442-140, lwm2m:r3442-150, lwm2m:r3442-160, lwm2m:r3442-170, lwm2m:r3442-180,
    lwm2m:r3442-2, lwm2m:r3442-3, lwm2m:r3442-4, lwm2m:r3442-5, lwm2m:r3442-6;
  prov:wasDerivedFrom <file:/data/lp/etl/executor/data/1651932849158-23-3c5fa11b-d02c-40e9-9c76-7d268eee1c69/working/working-outputfiles-214/lwm2m-registry-prod/3442.xml> .

<http://purl.org/wot-catalogue/lwm2m/ipso#3352> a skos:Concept, ontolex:LexicalConcept;
  skos:altLabel "plmn search event";
  skos:broader lwm2m:Object;
  skos:definition "List of all PLMNs found during the initial search/scan";
  skos:inScheme lwm2m:Scheme;
  skos:prefLabel "plmnSearchEvent";
  skos:related lwm2m:r3352-0, lwm2m:r6030, lwm2m:r6031, lwm2m:r6032;
  prov:wasDerivedFrom <file:/data/lp/etl/executor/data/1651932849158-23-3c5fa11b-d02c-40e9-9c76-7d268eee1c69/working/working-outputfiles-214/lwm2m-registry-prod/3352.xml> .

<http://purl.org/wot-catalogue/lwm2m/ipso#3200> a skos:Concept, ontolex:LexicalConcept;
  skos:altLabel "digital input";
  skos:broader lwm2m:Object;
  skos:definition "Generic digital input for non-specific sensors";
  skos:inScheme lwm2m:Scheme;
  skos:prefLabel "Digital Input";
  skos:related lwm2m:r5500, lwm2m:r5501, lwm2m:r5502, lwm2m:r5503, lwm2m:r5504, lwm2m:r5505,
    lwm2m:r5518, lwm2m:r5750, lwm2m:r5751, lwm2m:r6050;
  prov:wasDerivedFrom <file:/data/lp/etl/executor/data/1651932849158-23-3c5fa11b-d02c-40e9-9c76-7d268eee1c69/working/working-outputfiles-214/lwm2m-registry-prod/3200.xml> .

<http://purl.org/wot-catalogue/lwm2m/ipso#3397> a skos:Concept, ontolex:LexicalConcept;
  skos:altLabel "oa physical colour temperature light-point actuator";
  skos:broader lwm2m:Object;
  skos:definition "The 'oA_Physical_Colour_Temperature_Light-Point_Actuator' represents a physical tunable white light-point actuator. It is necessary to map at least on Logical Light Point Actuator to control the intensity and one Logical Colour Temperature Light-Point to control the colour temperature to the Physical Colour Temperature Light Point.";
  skos:inScheme lwm2m:Scheme;
  skos:prefLabel "oA Physical Colour Temperature Light-Point Actuator";
  skos:related lwm2m:r3397-100, lwm2m:r3397-102, lwm2m:r3397-103, lwm2m:r3397-104, lwm2m:r3397-105,
    lwm2m:r3397-110, lwm2m:r3397-111, lwm2m:r3397-114, lwm2m:r3397-115, lwm2m:r3397-137,
    lwm2m:r3397-138, lwm2m:r3397-155, lwm2m:r3397-156, lwm2m:r3397-157, lwm2m:r3397-158,
    lwm2m:r3397-901, lwm2m:r3397-907, lwm2m:r3397-908, lwm2m:r3397-910, lwm2m:r3397-911,
    lwm2m:r3397-912, lwm2m:r3397-930, lwm2m:r3397-931, lwm2m:r4001, lwm2m:r5850;
  prov:wasDerivedFrom <file:/data/lp/etl/executor/data/1651932849158-23-3c5fa11b-d02c-40e9-9c76-7d268eee1c69/working/working-outputfiles-214/lwm2m-registry-prod/3397.xml> .

<http://purl.org/wot-catalogue/lwm2m/ipso#3334> a skos:Concept, ontolex:LexicalConcept;
  skos:altLabel "gyrometer";
  skos:broader lwm2m:Object;
  skos:definition """This IPSO Object is used to report the current reading of a gyrometer sensor in 3 axes. It provides tracking of the minimum and maximum angular rate in all 3 axes. An example unit of measure is radians per second.
        """;
  skos:inScheme lwm2m:Scheme;
  skos:prefLabel "Gyrometer";
  skos:related lwm2m:r5508, lwm2m:r5509, lwm2m:r5510, lwm2m:r5511, lwm2m:r5512, lwm2m:r5513,
    lwm2m:r5518, lwm2m:r5603, lwm2m:r5604, lwm2m:r5605, lwm2m:r5701, lwm2m:r5702, lwm2m:r5703,
    lwm2m:r5704, lwm2m:r5750, lwm2m:r6042, lwm2m:r6049, lwm2m:r6050;
  prov:wasDerivedFrom <file:/data/lp/etl/executor/data/1651932849158-23-3c5fa11b-d02c-40e9-9c76-7d268eee1c69/working/working-outputfiles-214/lwm2m-registry-prod/3334.xml> .

<http://purl.org/wot-catalogue/lwm2m/ipso#3433> a skos:Concept, ontolex:LexicalConcept;
  skos:altLabel "noise sensor";
  skos:broader lwm2m:Object;
  skos:definition "The uCIFI noise sensor reports a noise measurement in decibel. It also provides resources for minimum/maximum measured values and the minimum/maximum range that can be measured by the noise sensor and some specific alarms resulting from noise analysis by the device.";
  skos:inScheme lwm2m:Scheme;
  skos:prefLabel "Noise sensor";
  skos:related lwm2m:r3433-1, lwm2m:r3433-2, lwm2m:r3433-3, lwm2m:r3433-4, lwm2m:r3433-5,
    lwm2m:r3433-6, lwm2m:r3433-7, lwm2m:r3433-8;
  prov:wasDerivedFrom <file:/data/lp/etl/executor/data/1651932849158-23-3c5fa11b-d02c-40e9-9c76-7d268eee1c69/working/working-outputfiles-214/lwm2m-registry-prod/3433.xml> .

<http://purl.org/wot-catalogue/lwm2m/ipso#3419> a skos:Concept, ontolex:LexicalConcept;
  skos:altLabel "photocell";
  skos:broader lwm2m:Object;
  skos:definition "A uCIFI photocell object is used for lighting control, particularly to identify when light should be switched ON/OFF.";
  skos:inScheme lwm2m:Scheme;
  skos:prefLabel "Photocell";
  skos:related lwm2m:r3419-1, lwm2m:r3419-2, lwm2m:r3419-3;
  prov:wasDerivedFrom <file:/data/lp/etl/executor/data/1651932849158-23-3c5fa11b-d02c-40e9-9c76-7d268eee1c69/working/working-outputfiles-214/lwm2m-registry-prod/3419.xml> .

<http://purl.org/wot-catalogue/lwm2m/ipso#3347> a skos:Concept, ontolex:LexicalConcept;
  skos:altLabel "push button";
  skos:broader lwm2m:Object;
  skos:definition """This IPSO object is used to report the state of a momentary action push button control and to count the number of times the control has been operated since the last observation.
        """;
  skos:inScheme lwm2m:Scheme;
  skos:prefLabel "Push button";
  skos:related lwm2m:r5500, lwm2m:r5501, lwm2m:r5518, lwm2m:r5750, lwm2m:r6050;
  prov:wasDerivedFrom <file:/data/lp/etl/executor/data/1651932849158-23-3c5fa11b-d02c-40e9-9c76-7d268eee1c69/working/working-outputfiles-214/lwm2m-registry-prod/3347.xml> .

<http://purl.org/wot-catalogue/lwm2m/ipso#3326> a skos:Concept, ontolex:LexicalConcept;
  skos:altLabel "acidity";
  skos:broader lwm2m:Object;
  skos:definition """This IPSO object should be used to report an acidity measurement of a liquid. It also provides resources for minimum and maximum measured values, as well as the minimum and maximum range that can be measured by the sensor. An example measurement unit is pH.
        """;
  skos:inScheme lwm2m:Scheme;
  skos:prefLabel "Acidity";
  skos:related lwm2m:r5518, lwm2m:r5601, lwm2m:r5602, lwm2m:r5603, lwm2m:r5604, lwm2m:r5605,
    lwm2m:r5700, lwm2m:r5701, lwm2m:r5750, lwm2m:r5821, lwm2m:r6042, lwm2m:r6049, lwm2m:r6050;
  prov:wasDerivedFrom <file:/data/lp/etl/executor/data/1651932849158-23-3c5fa11b-d02c-40e9-9c76-7d268eee1c69/working/working-outputfiles-214/lwm2m-registry-prod/3326.xml> .

<http://purl.org/wot-catalogue/lwm2m/ipso#3329> a skos:Concept, ontolex:LexicalConcept;
  skos:altLabel "power factor";
  skos:broader lwm2m:Object;
  skos:definition """This IPSO object should be used to report a measurement or calculation of the power factor of a reactive electrical load. Power Factor is normally the ratio of non-reactive power to total power. This object also provides resources for minimum and maximum measured values, as well as the minimum and maximum range that can be measured by the sensor.
        """;
  skos:inScheme lwm2m:Scheme;
  skos:prefLabel "Power Factor";
  skos:related lwm2m:r5518, lwm2m:r5601, lwm2m:r5602, lwm2m:r5603, lwm2m:r5604, lwm2m:r5605,
    lwm2m:r5700, lwm2m:r5701, lwm2m:r5750, lwm2m:r5821, lwm2m:r6042, lwm2m:r6049, lwm2m:r6050;
  prov:wasDerivedFrom <file:/data/lp/etl/executor/data/1651932849158-23-3c5fa11b-d02c-40e9-9c76-7d268eee1c69/working/working-outputfiles-214/lwm2m-registry-prod/3329.xml> .

<http://purl.org/wot-catalogue/lwm2m/ipso#3319> a skos:Concept, ontolex:LexicalConcept;
  skos:altLabel "depth";
  skos:broader lwm2m:Object;
  skos:definition """This IPSO object should be used to report depth measurements. It can, for example, be used to describe a generic rain gauge that measures the accumulated rainfall in millimetres (mm).
        """;
  skos:inScheme lwm2m:Scheme;
  skos:prefLabel "Depth";
  skos:related lwm2m:r5518, lwm2m:r5601, lwm2m:r5602, lwm2m:r5603, lwm2m:r5604, lwm2m:r5605,
    lwm2m:r5700, lwm2m:r5701, lwm2m:r5750, lwm2m:r5821, lwm2m:r6042, lwm2m:r6049, lwm2m:r6050;
  prov:wasDerivedFrom <file:/data/lp/etl/executor/data/1651932849158-23-3c5fa11b-d02c-40e9-9c76-7d268eee1c69/working/working-outputfiles-214/lwm2m-registry-prod/3319.xml> .

<http://purl.org/wot-catalogue/lwm2m/ipso#3317> a skos:Concept, ontolex:LexicalConcept;
  skos:altLabel "current";
  skos:broader lwm2m:Object;
  skos:definition """This IPSO object should be used with an ammeter to report measured electric current in amperes. It also provides resources for minimum and maximum measured values, as well as the minimum and maximum range that can be measured by the sensor. An example measurement unit is ampere.
        """;
  skos:inScheme lwm2m:Scheme;
  skos:prefLabel "Current";
  skos:related lwm2m:r5518, lwm2m:r5601, lwm2m:r5602, lwm2m:r5603, lwm2m:r5604, lwm2m:r5605,
    lwm2m:r5700, lwm2m:r5701, lwm2m:r5750, lwm2m:r5821, lwm2m:r6042, lwm2m:r6049, lwm2m:r6050;
  prov:wasDerivedFrom <file:/data/lp/etl/executor/data/1651932849158-23-3c5fa11b-d02c-40e9-9c76-7d268eee1c69/working/working-outputfiles-214/lwm2m-registry-prod/3317.xml> .

<http://purl.org/wot-catalogue/lwm2m/ipso#3318> a skos:Concept, ontolex:LexicalConcept;
  skos:altLabel "frequency";
  skos:broader lwm2m:Object;
  skos:definition """This IPSO object should be used to report frequency measurements. It also provides resources for minimum and maximum measured values, as well as the minimum and maximum range that can be measured by the sensor. An example measurement unit is hertz.
        """;
  skos:inScheme lwm2m:Scheme;
  skos:prefLabel "Frequency";
  skos:related lwm2m:r5518, lwm2m:r5601, lwm2m:r5602, lwm2m:r5603, lwm2m:r5604, lwm2m:r5605,
    lwm2m:r5700, lwm2m:r5701, lwm2m:r5750, lwm2m:r5821, lwm2m:r6042, lwm2m:r6049, lwm2m:r6050;
  prov:wasDerivedFrom <file:/data/lp/etl/executor/data/1651932849158-23-3c5fa11b-d02c-40e9-9c76-7d268eee1c69/working/working-outputfiles-214/lwm2m-registry-prod/3318.xml> .

<http://purl.org/wot-catalogue/lwm2m/ipso#3417> a skos:Concept, ontolex:LexicalConcept;
  skos:altLabel "luminaire asset";
  skos:broader lwm2m:Object;
  skos:definition "The uCIFI luminaire asset is an object that enables outdoor lighting control software to configure outdoor lamp controllers. It also enables outdoor lamp controllers to send Zhaga D4i or DALI attributes read from the control gears, to centrally managed outdoor lighting control software or asset management systems.";
  skos:inScheme lwm2m:Scheme;
  skos:prefLabel "Luminaire asset";
  skos:related lwm2m:r3417-1, lwm2m:r3417-10, lwm2m:r3417-11, lwm2m:r3417-12, lwm2m:r3417-13,
    lwm2m:r3417-14, lwm2m:r3417-2, lwm2m:r3417-3, lwm2m:r3417-4, lwm2m:r3417-5, lwm2m:r3417-6,
    lwm2m:r3417-7, lwm2m:r3417-8, lwm2m:r3417-9;
  prov:wasDerivedFrom <file:/data/lp/etl/executor/data/1651932849158-23-3c5fa11b-d02c-40e9-9c76-7d268eee1c69/working/working-outputfiles-214/lwm2m-registry-prod/3417.xml> .

<http://purl.org/wot-catalogue/lwm2m/ipso#3393> a skos:Concept, ontolex:LexicalConcept;
  skos:altLabel "oa logical light-point actuator";
  skos:broader lwm2m:Object;
  skos:definition "The 'oA Logical Light Point Actuator' represents the logical part of an actuator model for a dimmable light point. The corresponding physical device is a light channel and associated gear (e.g. LED driver).\\nThe Object (module) supports several interactions that include basic On/Off as well as Up/Down dimming. Several device configuration parameters are mapped, which relate to behaviour or describe device limitations. For multi-channel luminaires where the configuration per channel may vary significantly (e.g. different max/min values), multiple instances of this Object should be used.";
  skos:inScheme lwm2m:Scheme;
  skos:prefLabel "oA Logical Light-Point Actuator";
  skos:related lwm2m:r3393-100, lwm2m:r3393-101, lwm2m:r3393-106, lwm2m:r3393-108, lwm2m:r3393-109,
    lwm2m:r3393-117, lwm2m:r3393-118, lwm2m:r3393-119, lwm2m:r3393-120, lwm2m:r3393-901,
    lwm2m:r3393-902, lwm2m:r3393-903, lwm2m:r3393-904, lwm2m:r3393-905, lwm2m:r3393-906,
    lwm2m:r3393-909, lwm2m:r3393-919, lwm2m:r3393-921, lwm2m:r3393-922, lwm2m:r3393-924,
    lwm2m:r3393-934, lwm2m:r4001;
  prov:wasDerivedFrom <file:/data/lp/etl/executor/data/1651932849158-23-3c5fa11b-d02c-40e9-9c76-7d268eee1c69/working/working-outputfiles-214/lwm2m-registry-prod/3393.xml> .

<http://purl.org/wot-catalogue/lwm2m/ipso#3378> a skos:Concept, ontolex:LexicalConcept;
  skos:altLabel "pbch decoding results";
  skos:broader lwm2m:Object;
  skos:definition "Serving cell PBCH decoding information";
  skos:inScheme lwm2m:Scheme;
  skos:prefLabel "PbchDecodingResults";
  skos:related lwm2m:r3378-0, lwm2m:r3378-1, lwm2m:r6037;
  prov:wasDerivedFrom <file:/data/lp/etl/executor/data/1651932849158-23-3c5fa11b-d02c-40e9-9c76-7d268eee1c69/working/working-outputfiles-214/lwm2m-registry-prod/3378.xml> .

<http://purl.org/wot-catalogue/lwm2m/ipso#3439> a skos:Concept, ontolex:LexicalConcept;
  skos:altLabel "edge computing generic condition";
  skos:broader lwm2m:Object;
  skos:definition "The uCIFI edge computing generic condition object defines a vendor-specific condition (e.g. when a resource or an object is equal to a particular value) at which a particular script should be executed by the device.";
  skos:inScheme lwm2m:Scheme;
  skos:prefLabel "Edge computing generic condition";
  skos:related lwm2m:r3439-1, lwm2m:r3439-2, lwm2m:r3439-3;
  prov:wasDerivedFrom <file:/data/lp/etl/executor/data/1651932849158-23-3c5fa11b-d02c-40e9-9c76-7d268eee1c69/working/working-outputfiles-214/lwm2m-registry-prod/3439.xml> .

<http://purl.org/wot-catalogue/lwm2m/ipso#3424> a skos:Concept, ontolex:LexicalConcept;
  skos:altLabel "water meter";
  skos:broader lwm2m:Object;
  skos:definition "The uCIFI water meter measures water volume that was distributed through a water meter, in pulse count as well as in m3. It also detects anomalies in the water meter.";
  skos:inScheme lwm2m:Scheme;
  skos:prefLabel "Water meter";
  skos:related lwm2m:r3424-1, lwm2m:r3424-10, lwm2m:r3424-11, lwm2m:r3424-12, lwm2m:r3424-13,
    lwm2m:r3424-2, lwm2m:r3424-3, lwm2m:r3424-4, lwm2m:r3424-5, lwm2m:r3424-6, lwm2m:r3424-7,
    lwm2m:r3424-8, lwm2m:r3424-9;
  prov:wasDerivedFrom <file:/data/lp/etl/executor/data/1651932849158-23-3c5fa11b-d02c-40e9-9c76-7d268eee1c69/working/working-outputfiles-214/lwm2m-registry-prod/3424.xml> .

<http://purl.org/wot-catalogue/lwm2m/ipso#3406> a skos:Concept, ontolex:LexicalConcept;
  skos:altLabel "oa status report structure";
  skos:broader lwm2m:Object;
  skos:definition "The 'oA Status_Report_Structure' describes the content of the status reports. Its ID is always the first byte, the following bytes are defined by Keys.";
  skos:inScheme lwm2m:Scheme;
  skos:prefLabel "oA Status Report Structure";
  skos:related lwm2m:r3406-850, lwm2m:r3406-851, lwm2m:r3406-901, lwm2m:r4001;
  prov:wasDerivedFrom <file:/data/lp/etl/executor/data/1651932849158-23-3c5fa11b-d02c-40e9-9c76-7d268eee1c69/working/working-outputfiles-214/lwm2m-registry-prod/3406.xml> .

<http://purl.org/wot-catalogue/lwm2m/ipso#3394> a skos:Concept, ontolex:LexicalConcept;
  skos:altLabel "oa logical presence sensor";
  skos:broader lwm2m:Object;
  skos:definition "The 'oA Logical Presence Sensor' represents the logical part of a presence sensor. The corresponding physical device is a sensor that detects presence in its detection area. \\nThe Object supports two states 'presence' and 'absence'.";
  skos:inScheme lwm2m:Scheme;
  skos:prefLabel "oA Logical Presence Sensor";
  skos:related lwm2m:r3394-901, lwm2m:r3394-903, lwm2m:r3394-904, lwm2m:r3394-905, lwm2m:r3394-906,
    lwm2m:r3394-909, lwm2m:r3394-919, lwm2m:r3394-924, lwm2m:r3394-934, lwm2m:r4001, lwm2m:r5500,
    lwm2m:r5903, lwm2m:r5904;
  prov:wasDerivedFrom <file:/data/lp/etl/executor/data/1651932849158-23-3c5fa11b-d02c-40e9-9c76-7d268eee1c69/working/working-outputfiles-214/lwm2m-registry-prod/3394.xml> .

<http://purl.org/wot-catalogue/lwm2m/ipso#3402> a skos:Concept, ontolex:LexicalConcept;
  skos:altLabel "oa receiving object";
  skos:broader lwm2m:Object;
  skos:definition "The 'oA Receiving Object' provides a resource for sensors/actuators to report their status message to. It is used with control objects as logical object that forwards the sensor and status data to the executing object.\\nIt is also used to receive the 'go bootstrap' message, using the Struct-ID 255, in OOTB mode.";
  skos:inScheme lwm2m:Scheme;
  skos:prefLabel "oA Receiving Object";
  skos:related lwm2m:r3402-901, lwm2m:r3402-909, lwm2m:r3402-923, lwm2m:r4001;
  prov:wasDerivedFrom <file:/data/lp/etl/executor/data/1651932849158-23-3c5fa11b-d02c-40e9-9c76-7d268eee1c69/working/working-outputfiles-214/lwm2m-registry-prod/3402.xml> .

<http://purl.org/wot-catalogue/lwm2m/ipso#3399> a skos:Concept, ontolex:LexicalConcept;
  skos:altLabel "oa physical light-point actuator";
  skos:broader lwm2m:Object;
  skos:definition "The 'oA_Physical_Light-Point_Actuator' represents a physical light-point actuator. All logical light-point actuators (object instances of 'oA Light-Point Actuator') are mapped to one physical light-point actuator.";
  skos:inScheme lwm2m:Scheme;
  skos:prefLabel "oA Physical Light-Point Actuator";
  skos:related lwm2m:r3399-100, lwm2m:r3399-102, lwm2m:r3399-103, lwm2m:r3399-104, lwm2m:r3399-105,
    lwm2m:r3399-110, lwm2m:r3399-111, lwm2m:r3399-114, lwm2m:r3399-115, lwm2m:r3399-901,
    lwm2m:r3399-907, lwm2m:r3399-908, lwm2m:r3399-910, lwm2m:r3399-911, lwm2m:r3399-912,
    lwm2m:r3399-930, lwm2m:r3399-931, lwm2m:r4001, lwm2m:r5850;
  prov:wasDerivedFrom <file:/data/lp/etl/executor/data/1651932849158-23-3c5fa11b-d02c-40e9-9c76-7d268eee1c69/working/working-outputfiles-214/lwm2m-registry-prod/3399.xml> .

<http://purl.org/wot-catalogue/lwm2m/ipso#3308> a skos:Concept, ontolex:LexicalConcept;
  skos:altLabel "set point";
  skos:broader lwm2m:Object;
  skos:definition "This IPSO object should be used to set a desired value to a controller, such as a thermostat. A special resource is added to set the colour of an object.";
  skos:inScheme lwm2m:Scheme;
  skos:prefLabel "Set Point";
  skos:related lwm2m:r5518, lwm2m:r5701, lwm2m:r5706, lwm2m:r5750, lwm2m:r5900, lwm2m:r6050;
  prov:wasDerivedFrom <file:/data/lp/etl/executor/data/1651932849158-23-3c5fa11b-d02c-40e9-9c76-7d268eee1c69/working/working-outputfiles-214/lwm2m-registry-prod/3308.xml> .

<http://purl.org/wot-catalogue/lwm2m/ipso#3403> a skos:Concept, ontolex:LexicalConcept;
  skos:altLabel "oa reporting object";
  skos:broader lwm2m:Object;
  skos:definition "The 'oA Reporting Object' packs several status messages available at the node into a single, size optimized message, as e.g. used with data collect or BMS interfacing.";
  skos:inScheme lwm2m:Scheme;
  skos:prefLabel "oA Reporting Object";
  skos:related lwm2m:r3403-901, lwm2m:r3403-903, lwm2m:r3403-904, lwm2m:r3403-919, lwm2m:r3403-932,
    lwm2m:r3403-933, lwm2m:r4001;
  prov:wasDerivedFrom <file:/data/lp/etl/executor/data/1651932849158-23-3c5fa11b-d02c-40e9-9c76-7d268eee1c69/working/working-outputfiles-214/lwm2m-registry-prod/3403.xml> .

<http://purl.org/wot-catalogue/lwm2m/ipso#3421> a skos:Concept, ontolex:LexicalConcept;
  skos:altLabel "single-phase electrical meter";
  skos:broader lwm2m:Object;
  skos:definition "The uCIFI single-phase electrical meter measures the electrical consumption of loads on one electrical line, such as electrical cabinets in city infrastructures, street lighting networks, homes and buildings.";
  skos:inScheme lwm2m:Scheme;
  skos:prefLabel "Single-phase electrical meter";
  skos:related lwm2m:r3421-1, lwm2m:r3421-10, lwm2m:r3421-11, lwm2m:r3421-12, lwm2m:r3421-13,
    lwm2m:r3421-14, lwm2m:r3421-15, lwm2m:r3421-16, lwm2m:r3421-17, lwm2m:r3421-18, lwm2m:r3421-19,
    lwm2m:r3421-2, lwm2m:r3421-20, lwm2m:r3421-21, lwm2m:r3421-22, lwm2m:r3421-23, lwm2m:r3421-24,
    lwm2m:r3421-25, lwm2m:r3421-26, lwm2m:r3421-27, lwm2m:r3421-28, lwm2m:r3421-29, lwm2m:r3421-3,
    lwm2m:r3421-30, lwm2m:r3421-31, lwm2m:r3421-32, lwm2m:r3421-33, lwm2m:r3421-34, lwm2m:r3421-35,
    lwm2m:r3421-36, lwm2m:r3421-37, lwm2m:r3421-38, lwm2m:r3421-39, lwm2m:r3421-4, lwm2m:r3421-40,
    lwm2m:r3421-41, lwm2m:r3421-42, lwm2m:r3421-43, lwm2m:r3421-44, lwm2m:r3421-45, lwm2m:r3421-46,
    lwm2m:r3421-47, lwm2m:r3421-48, lwm2m:r3421-49, lwm2m:r3421-5, lwm2m:r3421-50, lwm2m:r3421-51,
    lwm2m:r3421-52, lwm2m:r3421-53, lwm2m:r3421-54, lwm2m:r3421-55, lwm2m:r3421-56, lwm2m:r3421-57,
    lwm2m:r3421-6, lwm2m:r3421-7, lwm2m:r3421-8, lwm2m:r3421-9;
  prov:wasDerivedFrom <file:/data/lp/etl/executor/data/1651932849158-23-3c5fa11b-d02c-40e9-9c76-7d268eee1c69/working/working-outputfiles-214/lwm2m-registry-prod/3421.xml> .

<http://purl.org/wot-catalogue/lwm2m/ipso#3407> a skos:Concept, ontolex:LexicalConcept;
  skos:altLabel "smoke alarm";
  skos:broader lwm2m:Object;
  skos:definition "This is an alarm that should be raised if the meter detects CO2 concentration above a pre-configured threshold.";
  skos:inScheme lwm2m:Scheme;
  skos:prefLabel "Smoke Alarm";
  skos:related lwm2m:r6044, lwm2m:r6045, lwm2m:r6046, lwm2m:r6047, lwm2m:r6048;
  prov:wasDerivedFrom <file:/data/lp/etl/executor/data/1651932849158-23-3c5fa11b-d02c-40e9-9c76-7d268eee1c69/working/working-outputfiles-214/lwm2m-registry-prod/3407.xml> .

<http://purl.org/wot-catalogue/lwm2m/ipso#3353> a skos:Concept, ontolex:LexicalConcept;
  skos:altLabel "scell id";
  skos:broader lwm2m:Object;
  skos:definition "serving cell information that the RRC decides to camp on";
  skos:inScheme lwm2m:Scheme;
  skos:prefLabel "scellID";
  skos:related lwm2m:r3353-2, lwm2m:r6030, lwm2m:r6031, lwm2m:r6033;
  prov:wasDerivedFrom <file:/data/lp/etl/executor/data/1651932849158-23-3c5fa11b-d02c-40e9-9c76-7d268eee1c69/working/working-outputfiles-214/lwm2m-registry-prod/3353.xml> .

<http://purl.org/wot-catalogue/lwm2m/ipso#3404> a skos:Concept, ontolex:LexicalConcept;
  skos:altLabel "oa scene";
  skos:broader lwm2m:Object;
  skos:definition "The 'oA Scene' represents a scene model. The scene holds defined values for each actuator in one group.";
  skos:inScheme lwm2m:Scheme;
  skos:prefLabel "oA Scene";
  skos:related lwm2m:r3404-650, lwm2m:r3404-651, lwm2m:r3404-652, lwm2m:r3404-653, lwm2m:r3404-655,
    lwm2m:r3404-901, lwm2m:r4001;
  prov:wasDerivedFrom <file:/data/lp/etl/executor/data/1651932849158-23-3c5fa11b-d02c-40e9-9c76-7d268eee1c69/working/working-outputfiles-214/lwm2m-registry-prod/3404.xml> .

<http://purl.org/wot-catalogue/lwm2m/ipso#2056> a skos:Concept, ontolex:LexicalConcept;
  skos:altLabel "cmdh buffer";
  skos:broader lwm2m:Object;
  skos:definition "This Object defines limits in usage of buffers for temporarily storing information that needs to be forwarded to other CSEs during processing of CMDH-related requests in a CSE.";
  skos:inScheme lwm2m:Scheme;
  skos:prefLabel "CmdhBuffer";
  skos:related lwm2m:r2056-0, lwm2m:r2056-1, lwm2m:r2056-2;
  prov:wasDerivedFrom <file:/data/lp/etl/executor/data/1651932849158-23-3c5fa11b-d02c-40e9-9c76-7d268eee1c69/working/working-outputfiles-214/lwm2m-registry-prod/2056.xml> .

<http://purl.org/wot-catalogue/lwm2m/ipso#3389> a skos:Concept, ontolex:LexicalConcept;
  skos:altLabel "oa group";
  skos:broader lwm2m:Object;
  skos:definition "The 'oA Group' represents a group. It contains an application group ID, a security group ID and a list of multicast and unicast IP addresses that are used in the group. \\nAdditionally it contains a list of all members of the group.";
  skos:inScheme lwm2m:Scheme;
  skos:prefLabel "oA Group";
  skos:related lwm2m:r3389-600, lwm2m:r3389-601, lwm2m:r3389-602, lwm2m:r3389-603, lwm2m:r3389-901,
    lwm2m:r4001;
  prov:wasDerivedFrom <file:/data/lp/etl/executor/data/1651932849158-23-3c5fa11b-d02c-40e9-9c76-7d268eee1c69/working/working-outputfiles-214/lwm2m-registry-prod/3389.xml> .

<http://purl.org/wot-catalogue/lwm2m/ipso#3366> a skos:Concept, ontolex:LexicalConcept;
  skos:altLabel "mac rach attempt event";
  skos:broader lwm2m:Object;
  skos:definition "RACH information. Logged at RACH TX";
  skos:inScheme lwm2m:Scheme;
  skos:prefLabel "macRachAttemptEvent";
  skos:related lwm2m:r3366-0, lwm2m:r3366-1, lwm2m:r3366-2, lwm2m:r3366-3, lwm2m:r3366-4,
    lwm2m:r3366-5, lwm2m:r3366-6, lwm2m:r3366-7, lwm2m:r3366-8;
  prov:wasDerivedFrom <file:/data/lp/etl/executor/data/1651932849158-23-3c5fa11b-d02c-40e9-9c76-7d268eee1c69/working/working-outputfiles-214/lwm2m-registry-prod/3366.xml> .

<http://purl.org/wot-catalogue/lwm2m/ipso#3357> a skos:Concept, ontolex:LexicalConcept;
  skos:altLabel "rrc state change event";
  skos:broader lwm2m:Object;
  skos:definition "Current RRC state change information, including the event that triggered the state change";
  skos:inScheme lwm2m:Scheme;
  skos:prefLabel "rrcStateChangeEvent";
  skos:related lwm2m:r3357-0, lwm2m:r3357-1;
  prov:wasDerivedFrom <file:/data/lp/etl/executor/data/1651932849158-23-3c5fa11b-d02c-40e9-9c76-7d268eee1c69/working/working-outputfiles-214/lwm2m-registry-prod/3357.xml> .

<http://purl.org/wot-catalogue/lwm2m/ipso#3390> a skos:Concept, ontolex:LexicalConcept;
  skos:altLabel "oa logical colour light-point actuator";
  skos:broader lwm2m:Object;
  skos:definition "The 'oA Logical Colour Light Point Actuator' represents the logical part of an actuator model for a colour light point. The corresponding physical device is a light channel and associated gear (e.g. LED driver).\\nThe Object (module) supports several interactions that include absolute and relative colour setting. Several device configuration parameters are mapped, which relate to behaviour or describe device limitations.";
  skos:inScheme lwm2m:Scheme;
  skos:prefLabel "oA Logical Colour Light-Point Actuator";
  skos:related lwm2m:r3390-125, lwm2m:r3390-126, lwm2m:r3390-127, lwm2m:r3390-128, lwm2m:r3390-129,
    lwm2m:r3390-130, lwm2m:r3390-131, lwm2m:r3390-132, lwm2m:r3390-133, lwm2m:r3390-134,
    lwm2m:r3390-135, lwm2m:r3390-136, lwm2m:r3390-901, lwm2m:r3390-902, lwm2m:r3390-903,
    lwm2m:r3390-904, lwm2m:r3390-905, lwm2m:r3390-906, lwm2m:r3390-909, lwm2m:r3390-919,
    lwm2m:r3390-921, lwm2m:r3390-922, lwm2m:r3390-924, lwm2m:r3390-934, lwm2m:r4001;
  prov:wasDerivedFrom <file:/data/lp/etl/executor/data/1651932849158-23-3c5fa11b-d02c-40e9-9c76-7d268eee1c69/working/working-outputfiles-214/lwm2m-registry-prod/3390.xml> .

<http://purl.org/wot-catalogue/lwm2m/ipso#3356> a skos:Concept, ontolex:LexicalConcept;
  skos:altLabel "radio link failure event";
  skos:broader lwm2m:Object;
  skos:definition "Radio Link Failure Event";
  skos:inScheme lwm2m:Scheme;
  skos:prefLabel "radioLinkFailureEvent";
  skos:related lwm2m:r3356-0, lwm2m:r3356-1;
  prov:wasDerivedFrom <file:/data/lp/etl/executor/data/1651932849158-23-3c5fa11b-d02c-40e9-9c76-7d268eee1c69/working/working-outputfiles-214/lwm2m-registry-prod/3356.xml> .

<http://purl.org/wot-catalogue/lwm2m/ipso#2049> a skos:Concept, ontolex:LexicalConcept;
  skos:altLabel "active cmdh policy";
  skos:broader lwm2m:Object;
  skos:definition "This Object provides a link to the currently active set of CMDH policies";
  skos:inScheme lwm2m:Scheme;
  skos:prefLabel "ActiveCmdhPolicy";
  skos:related lwm2m:r2049-0;
  prov:wasDerivedFrom <file:/data/lp/etl/executor/data/1651932849158-23-3c5fa11b-d02c-40e9-9c76-7d268eee1c69/working/working-outputfiles-214/lwm2m-registry-prod/2049.xml> .

<http://purl.org/wot-catalogue/lwm2m/ipso#3396> a skos:Concept, ontolex:LexicalConcept;
  skos:altLabel "oa physical colour light-point actuator";
  skos:broader lwm2m:Object;
  skos:definition "The 'oA_Physical_Colour_Light-Point_Actuator' represents a physical colour light-point actuator. It is necessary to map at least on Logical Light Point Actuator to control the intensity and one Logical Colour Light-Point to control the colour to the Physical Colour Light-Point.";
  skos:inScheme lwm2m:Scheme;
  skos:prefLabel "oA Physical Colour Light-Point Actuator";
  skos:related lwm2m:r3396-100, lwm2m:r3396-102, lwm2m:r3396-103, lwm2m:r3396-104, lwm2m:r3396-105,
    lwm2m:r3396-110, lwm2m:r3396-111, lwm2m:r3396-114, lwm2m:r3396-115, lwm2m:r3396-122,
    lwm2m:r3396-123, lwm2m:r3396-124, lwm2m:r3396-901, lwm2m:r3396-907, lwm2m:r3396-908,
    lwm2m:r3396-910, lwm2m:r3396-911, lwm2m:r3396-912, lwm2m:r3396-930, lwm2m:r3396-931,
    lwm2m:r4001, lwm2m:r5850;
  prov:wasDerivedFrom <file:/data/lp/etl/executor/data/1651932849158-23-3c5fa11b-d02c-40e9-9c76-7d268eee1c69/working/working-outputfiles-214/lwm2m-registry-prod/3396.xml> .

<http://purl.org/wot-catalogue/lwm2m/ipso#3340> a skos:Concept, ontolex:LexicalConcept;
  skos:altLabel "timer";
  skos:broader lwm2m:Object;
  skos:definition """This IPSO object is used to time events and actions, using patterns common to industrial timers. A write to the trigger resource or On/Off input state change starts the timing operation, and the timer remaining time shows zero when the operation is complete. The patterns supported are One-Shot (mode 1), On-Time or Interval (mode 2), Time delay on pick-up or TDPU (mode 3), and Time Delay on Drop-Out or TDDO (mode 4). Mode 0 disables the timer, so the output follows the input with no delay. A counter is provided to count occurrences of the timer output changing from 0 to 1. Writing a value of zero resets the counter. The Digital Input State resource reports the state of the timer output.
        """;
  skos:inScheme lwm2m:Scheme;
  skos:prefLabel "Timer";
  skos:related lwm2m:r5501, lwm2m:r5521, lwm2m:r5523, lwm2m:r5525, lwm2m:r5526, lwm2m:r5534,
    lwm2m:r5538, lwm2m:r5543, lwm2m:r5544, lwm2m:r5750, lwm2m:r5850;
  prov:wasDerivedFrom <file:/data/lp/etl/executor/data/1651932849158-23-3c5fa11b-d02c-40e9-9c76-7d268eee1c69/working/working-outputfiles-214/lwm2m-registry-prod/3340.xml> .

<http://purl.org/wot-catalogue/lwm2m/ipso#3306> a skos:Concept, ontolex:LexicalConcept;
  skos:altLabel "actuation";
  skos:broader lwm2m:Object;
  skos:definition "This IPSO object is dedicated to remote actuation such as ON/OFF action or dimming. A multi-state output can also be described as a string. This is useful to send pilot wire orders for instance. It also provides a resource to reflect the time that the device has been switched on.";
  skos:inScheme lwm2m:Scheme;
  skos:prefLabel "Actuation";
  skos:related lwm2m:r5518, lwm2m:r5750, lwm2m:r5850, lwm2m:r5851, lwm2m:r5852, lwm2m:r5853,
    lwm2m:r6050;
  prov:wasDerivedFrom <file:/data/lp/etl/executor/data/1651932849158-23-3c5fa11b-d02c-40e9-9c76-7d268eee1c69/working/working-outputfiles-214/lwm2m-registry-prod/3306.xml> .

<http://purl.org/wot-catalogue/lwm2m/ipso#3331> a skos:Concept, ontolex:LexicalConcept;
  skos:altLabel "energy";
  skos:broader lwm2m:Object;
  skos:definition """This IPSO object should be used to report energy consumption (Cumulative Power) of an electrical load. An example measurement unit is Watt Hours.
        """;
  skos:inScheme lwm2m:Scheme;
  skos:prefLabel "Energy";
  skos:related lwm2m:r5518, lwm2m:r5700, lwm2m:r5701, lwm2m:r5750, lwm2m:r5822, lwm2m:r6042,
    lwm2m:r6049, lwm2m:r6050;
  prov:wasDerivedFrom <file:/data/lp/etl/executor/data/1651932849158-23-3c5fa11b-d02c-40e9-9c76-7d268eee1c69/working/working-outputfiles-214/lwm2m-registry-prod/3331.xml> .

<http://purl.org/wot-catalogue/lwm2m/ipso#3379> a skos:Concept, ontolex:LexicalConcept;
  skos:altLabel "pucch power control";
  skos:broader lwm2m:Object;
  skos:definition "PUCCH TX power control information";
  skos:inScheme lwm2m:Scheme;
  skos:prefLabel "pucchPowerControl";
  skos:related lwm2m:r3379-2, lwm2m:r3379-3, lwm2m:r6037, lwm2m:r6038;
  prov:wasDerivedFrom <file:/data/lp/etl/executor/data/1651932849158-23-3c5fa11b-d02c-40e9-9c76-7d268eee1c69/working/working-outputfiles-214/lwm2m-registry-prod/3379.xml> .

<http://purl.org/wot-catalogue/lwm2m/ipso#3324> a skos:Concept, ontolex:LexicalConcept;
  skos:altLabel "loudness";
  skos:broader lwm2m:Object;
  skos:definition """This IPSO object should be used to report loudness or noise level measurements. It also provides resources for minimum and maximum measured values, as well as the minimum and maximum range that can be measured by the sensor. An example measurement unit is decibels.
        """;
  skos:inScheme lwm2m:Scheme;
  skos:prefLabel "Loudness";
  skos:related lwm2m:r5518, lwm2m:r5601, lwm2m:r5602, lwm2m:r5603, lwm2m:r5604, lwm2m:r5605,
    lwm2m:r5700, lwm2m:r5701, lwm2m:r5750, lwm2m:r5821, lwm2m:r6042, lwm2m:r6049, lwm2m:r6050;
  prov:wasDerivedFrom <file:/data/lp/etl/executor/data/1651932849158-23-3c5fa11b-d02c-40e9-9c76-7d268eee1c69/working/working-outputfiles-214/lwm2m-registry-prod/3324.xml> .

<http://purl.org/wot-catalogue/lwm2m/ipso#3349> a skos:Concept, ontolex:LexicalConcept;
  skos:altLabel "bitmap";
  skos:broader lwm2m:Object;
  skos:definition "Summarize several digital inputs to one value by mapping each bit to a digital input.";
  skos:inScheme lwm2m:Scheme;
  skos:prefLabel "Bitmap";
  skos:related lwm2m:r5518, lwm2m:r5750, lwm2m:r5910, lwm2m:r5911, lwm2m:r5912, lwm2m:r6050;
  prov:wasDerivedFrom <file:/data/lp/etl/executor/data/1651932849158-23-3c5fa11b-d02c-40e9-9c76-7d268eee1c69/working/working-outputfiles-214/lwm2m-registry-prod/3349.xml> .

<http://purl.org/wot-catalogue/lwm2m/ipso#3426> a skos:Concept, ontolex:LexicalConcept;
  skos:altLabel "water quality sensor";
  skos:broader lwm2m:Object;
  skos:definition "The uCIFI water quality sensor measures the quality of the water in the drinkable water distribution network, in water tanks or in lakes and rivers.";
  skos:inScheme lwm2m:Scheme;
  skos:prefLabel "Water quality sensor";
  skos:related lwm2m:r3426-1, lwm2m:r3426-10, lwm2m:r3426-11, lwm2m:r3426-12, lwm2m:r3426-13,
    lwm2m:r3426-14, lwm2m:r3426-2, lwm2m:r3426-3, lwm2m:r3426-4, lwm2m:r3426-5, lwm2m:r3426-6,
    lwm2m:r3426-7, lwm2m:r3426-8, lwm2m:r3426-9;
  prov:wasDerivedFrom <file:/data/lp/etl/executor/data/1651932849158-23-3c5fa11b-d02c-40e9-9c76-7d268eee1c69/working/working-outputfiles-214/lwm2m-registry-prod/3426.xml> .

<http://purl.org/wot-catalogue/lwm2m/ipso#3316> a skos:Concept, ontolex:LexicalConcept;
  skos:altLabel "voltage";
  skos:broader lwm2m:Object;
  skos:definition """This IPSO object should be used with voltmeter sensor to report measured voltage between two points.  It also provides resources for minimum and maximum measured values, as well as the minimum and maximum range that can be measured by the sensor. An example measurement unit is volts.
        """;
  skos:inScheme lwm2m:Scheme;
  skos:prefLabel "Voltage";
  skos:related lwm2m:r5518, lwm2m:r5601, lwm2m:r5602, lwm2m:r5603, lwm2m:r5604, lwm2m:r5605,
    lwm2m:r5700, lwm2m:r5701, lwm2m:r5750, lwm2m:r5821, lwm2m:r6042, lwm2m:r6049, lwm2m:r6050;
  prov:wasDerivedFrom <file:/data/lp/etl/executor/data/1651932849158-23-3c5fa11b-d02c-40e9-9c76-7d268eee1c69/working/working-outputfiles-214/lwm2m-registry-prod/3316.xml> .

<http://purl.org/wot-catalogue/lwm2m/ipso#3395> a skos:Concept, ontolex:LexicalConcept;
  skos:altLabel "oa logical push-button sensor";
  skos:broader lwm2m:Object;
  skos:definition "The 'oA Logical Push-Button Sensor' represents the logical part of a standard, normally open, push-button input. The corresponding physical device is a button with a spring that returns the button to the un-pushed state once it is released.\\nThe Object supports several events such as 'click', 'hold', 'double-click' and 'release'. It also indicates if the button is 'stuck'. For physical devices with multiple push-button inputs, an instance of this Object is required to map each input.";
  skos:inScheme lwm2m:Scheme;
  skos:prefLabel "oA Logical Push-Button Sensor";
  skos:related lwm2m:r3395-202, lwm2m:r3395-203, lwm2m:r3395-204, lwm2m:r3395-901, lwm2m:r3395-903,
    lwm2m:r3395-904, lwm2m:r3395-905, lwm2m:r3395-906, lwm2m:r3395-909, lwm2m:r3395-919,
    lwm2m:r3395-924, lwm2m:r3395-934, lwm2m:r4001;
  prov:wasDerivedFrom <file:/data/lp/etl/executor/data/1651932849158-23-3c5fa11b-d02c-40e9-9c76-7d268eee1c69/working/working-outputfiles-214/lwm2m-registry-prod/3395.xml> .

<http://purl.org/wot-catalogue/lwm2m/ipso#3432> a skos:Concept, ontolex:LexicalConcept;
  skos:altLabel "traffic counter";
  skos:broader lwm2m:Object;
  skos:definition "The uCIFI traffic counter provides vehicle counting and traffic analysis data. A traffic counting device may implement multiple instances of this traffic counter object, each of them being in charge of counting different categories of vehicles (e.g. bikes, cars, trucks).";
  skos:inScheme lwm2m:Scheme;
  skos:prefLabel "Traffic Counter";
  skos:related lwm2m:r3432-1, lwm2m:r3432-10, lwm2m:r3432-11, lwm2m:r3432-12, lwm2m:r3432-13,
    lwm2m:r3432-14, lwm2m:r3432-15, lwm2m:r3432-16, lwm2m:r3432-17, lwm2m:r3432-2, lwm2m:r3432-3,
    lwm2m:r3432-4, lwm2m:r3432-5, lwm2m:r3432-6, lwm2m:r3432-7, lwm2m:r3432-8, lwm2m:r3432-9;
  prov:wasDerivedFrom <file:/data/lp/etl/executor/data/1651932849158-23-3c5fa11b-d02c-40e9-9c76-7d268eee1c69/working/working-outputfiles-214/lwm2m-registry-prod/3432.xml> .

<http://purl.org/wot-catalogue/lwm2m/ipso#3314> a skos:Concept, ontolex:LexicalConcept;
  skos:altLabel "magnetometer";
  skos:broader lwm2m:Object;
  skos:definition "This IPSO object can be used to represent a 1-3 axis magnetometer with optional compass direction.";
  skos:inScheme lwm2m:Scheme;
  skos:prefLabel "Magnetometer";
  skos:related lwm2m:r5518, lwm2m:r5701, lwm2m:r5702, lwm2m:r5703, lwm2m:r5704, lwm2m:r5705,
    lwm2m:r5750, lwm2m:r6042, lwm2m:r6049, lwm2m:r6050;
  prov:wasDerivedFrom <file:/data/lp/etl/executor/data/1651932849158-23-3c5fa11b-d02c-40e9-9c76-7d268eee1c69/working/working-outputfiles-214/lwm2m-registry-prod/3314.xml> .

<http://purl.org/wot-catalogue/lwm2m/ipso#3375> a skos:Concept, ontolex:LexicalConcept;
  skos:altLabel "paging drx";
  skos:broader lwm2m:Object;
  skos:definition "Paging DRX information";
  skos:inScheme lwm2m:Scheme;
  skos:prefLabel "PagingDRX";
  skos:related lwm2m:r3375-2, lwm2m:r3375-3, lwm2m:r3375-4, lwm2m:r3375-5, lwm2m:r3375-6,
    lwm2m:r6032, lwm2m:r6034;
  prov:wasDerivedFrom <file:/data/lp/etl/executor/data/1651932849158-23-3c5fa11b-d02c-40e9-9c76-7d268eee1c69/working/working-outputfiles-214/lwm2m-registry-prod/3375.xml> .

<http://purl.org/wot-catalogue/lwm2m/ipso#3412> a skos:Concept, ontolex:LexicalConcept;
  skos:altLabel "lpwan communication";
  skos:broader lwm2m:Object;
  skos:definition "The uCIFI communication object provides attributes related to the communication on the LPWAN network, including multicast grouping.";
  skos:inScheme lwm2m:Scheme;
  skos:prefLabel "LPWAN Communication";
  skos:related lwm2m:r3412-1, lwm2m:r3412-10, lwm2m:r3412-11, lwm2m:r3412-12, lwm2m:r3412-13,
    lwm2m:r3412-14, lwm2m:r3412-15, lwm2m:r3412-16, lwm2m:r3412-17, lwm2m:r3412-18, lwm2m:r3412-19,
    lwm2m:r3412-2, lwm2m:r3412-20, lwm2m:r3412-21, lwm2m:r3412-22, lwm2m:r3412-23, lwm2m:r3412-24,
    lwm2m:r3412-3, lwm2m:r3412-4, lwm2m:r3412-5, lwm2m:r3412-6, lwm2m:r3412-7, lwm2m:r3412-8,
    lwm2m:r3412-9;
  prov:wasDerivedFrom <file:/data/lp/etl/executor/data/1651932849158-23-3c5fa11b-d02c-40e9-9c76-7d268eee1c69/working/working-outputfiles-214/lwm2m-registry-prod/3412.xml> .

<http://purl.org/wot-catalogue/lwm2m/ipso#3311> a skos:Concept, ontolex:LexicalConcept;
  skos:altLabel "light control";
  skos:broader lwm2m:Object;
  skos:definition "This Object is used to control a light source, such as a LED or other light.  It allows a light to be turned on or off and its dimmer setting to be control as a % between 0 and 100. An optional colour setting enables a string to be used to indicate the desired colour.";
  skos:inScheme lwm2m:Scheme;
  skos:prefLabel "Light Control";
  skos:related lwm2m:r5701, lwm2m:r5706, lwm2m:r5750, lwm2m:r5805, lwm2m:r5820, lwm2m:r5850,
    lwm2m:r5851, lwm2m:r5852;
  prov:wasDerivedFrom <file:/data/lp/etl/executor/data/1651932849158-23-3c5fa11b-d02c-40e9-9c76-7d268eee1c69/working/working-outputfiles-214/lwm2m-registry-prod/3311.xml> .

<http://purl.org/wot-catalogue/lwm2m/ipso#3313> a skos:Concept, ontolex:LexicalConcept;
  skos:altLabel "accelerometer";
  skos:broader lwm2m:Object;
  skos:definition "This IPSO object can be used to represent a 1-3 axis accelerometer.";
  skos:inScheme lwm2m:Scheme;
  skos:prefLabel "Accelerometer";
  skos:related lwm2m:r5518, lwm2m:r5603, lwm2m:r5604, lwm2m:r5701, lwm2m:r5702, lwm2m:r5703,
    lwm2m:r5704, lwm2m:r5750, lwm2m:r6042, lwm2m:r6049, lwm2m:r6050;
  prov:wasDerivedFrom <file:/data/lp/etl/executor/data/1651932849158-23-3c5fa11b-d02c-40e9-9c76-7d268eee1c69/working/working-outputfiles-214/lwm2m-registry-prod/3313.xml> .

<http://purl.org/wot-catalogue/lwm2m/ipso#3388> a skos:Concept, ontolex:LexicalConcept;
  skos:altLabel "oa device";
  skos:broader lwm2m:Object;
  skos:definition "The 'oA Device' represents the OpenAIS specific parameters of a Device that are necessary in addition to the LWM2M Device.";
  skos:inScheme lwm2m:Scheme;
  skos:prefLabel "oA Device";
  skos:related lwm2m:r3388-500, lwm2m:r3388-501, lwm2m:r3388-503, lwm2m:r3388-504, lwm2m:r3388-505,
    lwm2m:r3388-901, lwm2m:r3388-907, lwm2m:r3388-908, lwm2m:r3388-910, lwm2m:r3388-911,
    lwm2m:r3388-912, lwm2m:r3388-929, lwm2m:r4001;
  prov:wasDerivedFrom <file:/data/lp/etl/executor/data/1651932849158-23-3c5fa11b-d02c-40e9-9c76-7d268eee1c69/working/working-outputfiles-214/lwm2m-registry-prod/3388.xml> .

<http://purl.org/wot-catalogue/lwm2m/ipso#2051> a skos:Concept, ontolex:LexicalConcept;
  skos:altLabel "cmdh def ecvalues";
  skos:broader lwm2m:Object;
  skos:definition "This Object represents default set of values for the Event Category parameter of an incoming request or response message.";
  skos:inScheme lwm2m:Scheme;
  skos:prefLabel "CmdhDefEcValues";
  skos:related lwm2m:r2051-0, lwm2m:r2051-1, lwm2m:r2051-2, lwm2m:r2051-3, lwm2m:r2051-4,
    lwm2m:r2051-5;
  prov:wasDerivedFrom <file:/data/lp/etl/executor/data/1651932849158-23-3c5fa11b-d02c-40e9-9c76-7d268eee1c69/working/working-outputfiles-214/lwm2m-registry-prod/2051.xml> .

<http://purl.org/wot-catalogue/lwm2m/ipso#3431> a skos:Concept, ontolex:LexicalConcept;
  skos:altLabel "parking sensor";
  skos:broader lwm2m:Object;
  skos:definition "The uCIFI parking sensor provides actual and cumulated occupancy duration as well as forbidden parking detection.";
  skos:inScheme lwm2m:Scheme;
  skos:prefLabel "Parking Sensor";
  skos:related lwm2m:r3431-1, lwm2m:r3431-2, lwm2m:r3431-3, lwm2m:r3431-4, lwm2m:r3431-5;
  prov:wasDerivedFrom <file:/data/lp/etl/executor/data/1651932849158-23-3c5fa11b-d02c-40e9-9c76-7d268eee1c69/working/working-outputfiles-214/lwm2m-registry-prod/3431.xml> .

<http://purl.org/wot-catalogue/lwm2m/ipso#3420> a skos:Concept, ontolex:LexicalConcept;
  skos:altLabel "led color light";
  skos:broader lwm2m:Object;
  skos:definition "The uCIFI LED color light enables to control light colors of a LED luminaire.";
  skos:inScheme lwm2m:Scheme;
  skos:prefLabel "LED color light";
  skos:related lwm2m:r3420-1;
  prov:wasDerivedFrom <file:/data/lp/etl/executor/data/1651932849158-23-3c5fa11b-d02c-40e9-9c76-7d268eee1c69/working/working-outputfiles-214/lwm2m-registry-prod/3420.xml> .

<http://purl.org/wot-catalogue/lwm2m/ipso#3416> a skos:Concept, ontolex:LexicalConcept;
  skos:altLabel "outdoor lamp controller";
  skos:broader lwm2m:Object;
  skos:definition "The uCIFI outdoor lamp controller object provides attributes to control, command and monitor outdoor luminaires in streets, in tunnels, on roads and for illumination of park and gardens.";
  skos:inScheme lwm2m:Scheme;
  skos:prefLabel "Outdoor lamp controller";
  skos:related lwm2m:r3416-1, lwm2m:r3416-10, lwm2m:r3416-11, lwm2m:r3416-12, lwm2m:r3416-13,
    lwm2m:r3416-14, lwm2m:r3416-15, lwm2m:r3416-16, lwm2m:r3416-17, lwm2m:r3416-18, lwm2m:r3416-19,
    lwm2m:r3416-2, lwm2m:r3416-20, lwm2m:r3416-21, lwm2m:r3416-22, lwm2m:r3416-23, lwm2m:r3416-24,
    lwm2m:r3416-25, lwm2m:r3416-26, lwm2m:r3416-27, lwm2m:r3416-28, lwm2m:r3416-29, lwm2m:r3416-3,
    lwm2m:r3416-30, lwm2m:r3416-31, lwm2m:r3416-32, lwm2m:r3416-33, lwm2m:r3416-34, lwm2m:r3416-35,
    lwm2m:r3416-36, lwm2m:r3416-37, lwm2m:r3416-38, lwm2m:r3416-39, lwm2m:r3416-4, lwm2m:r3416-40,
    lwm2m:r3416-41, lwm2m:r3416-42, lwm2m:r3416-43, lwm2m:r3416-44, lwm2m:r3416-45, lwm2m:r3416-46,
    lwm2m:r3416-47, lwm2m:r3416-5, lwm2m:r3416-6, lwm2m:r3416-7, lwm2m:r3416-8, lwm2m:r3416-9;
  prov:wasDerivedFrom <file:/data/lp/etl/executor/data/1651932849158-23-3c5fa11b-d02c-40e9-9c76-7d268eee1c69/working/working-outputfiles-214/lwm2m-registry-prod/3416.xml> .

<http://purl.org/wot-catalogue/lwm2m/ipso#3362> a skos:Concept, ontolex:LexicalConcept;
  skos:altLabel "nas emm timer expiry event";
  skos:broader lwm2m:Object;
  skos:definition "NAS EMM timer expiry information";
  skos:inScheme lwm2m:Scheme;
  skos:prefLabel "nasEmmTimerExpiryEvent";
  skos:related lwm2m:r3362-0;
  prov:wasDerivedFrom <file:/data/lp/etl/executor/data/1651932849158-23-3c5fa11b-d02c-40e9-9c76-7d268eee1c69/working/working-outputfiles-214/lwm2m-registry-prod/3362.xml> .

<http://purl.org/wot-catalogue/lwm2m/ipso#3437> a skos:Concept, ontolex:LexicalConcept;
  skos:altLabel "edge computing script";
  skos:broader lwm2m:Object;
  skos:definition "The uCIFI edge computing scripts object defines a particular script to be executed by a device under a time or any other condition set by a \"Edge Computing Time Condition\" or \"Edge Computing Generic Condition\" object.";
  skos:inScheme lwm2m:Scheme;
  skos:prefLabel "Edge computing script";
  skos:related lwm2m:r3437-1, lwm2m:r3437-2, lwm2m:r3437-3, lwm2m:r3437-4, lwm2m:r3437-5,
    lwm2m:r3437-6, lwm2m:r3437-7;
  prov:wasDerivedFrom <file:/data/lp/etl/executor/data/1651932849158-23-3c5fa11b-d02c-40e9-9c76-7d268eee1c69/working/working-outputfiles-214/lwm2m-registry-prod/3437.xml> .

<http://purl.org/wot-catalogue/lwm2m/ipso#3341> a skos:Concept, ontolex:LexicalConcept;
  skos:altLabel "addressable text display";
  skos:broader lwm2m:Object;
  skos:definition """This IPSO object is used to send text to a text-only or text mode graphics display. Writing a string of text to the text resource causes it to be displayed at the selected X and Y locations on the display. If X or Y are set to a value greater than the size of the display, the position \"wraps around\" to the modulus of the setting and the display size. Likewise, if the text string overflows the display size, the text \"wraps around\" and displays on the next line down or, if the last line has been written, wraps around to the top of the display. Brightness and Contrast controls are provided to allow control of various display types including STN and DSTN type LCD character displays. Writing an empty payload to the Clear Display resource causes the display to be erased.
        """;
  skos:inScheme lwm2m:Scheme;
  skos:prefLabel "Addressable Text Display";
  skos:related lwm2m:r5527, lwm2m:r5528, lwm2m:r5529, lwm2m:r5530, lwm2m:r5531, lwm2m:r5545,
    lwm2m:r5546, lwm2m:r5548, lwm2m:r5750;
  prov:wasDerivedFrom <file:/data/lp/etl/executor/data/1651932849158-23-3c5fa11b-d02c-40e9-9c76-7d268eee1c69/working/working-outputfiles-214/lwm2m-registry-prod/3341.xml> .

<http://purl.org/wot-catalogue/lwm2m/ipso#2054> a skos:Concept, ontolex:LexicalConcept;
  skos:altLabel "cmdh network access rules";
  skos:broader lwm2m:Object;
  skos:definition "This Object defines the usage of underlying networks for forwarding information to other CSEs during processing of CMDH-related requests in a CSE.";
  skos:inScheme lwm2m:Scheme;
  skos:prefLabel "CmdhNetworkAccessRules";
  skos:related lwm2m:r2054-0, lwm2m:r2054-1;
  prov:wasDerivedFrom <file:/data/lp/etl/executor/data/1651932849158-23-3c5fa11b-d02c-40e9-9c76-7d268eee1c69/working/working-outputfiles-214/lwm2m-registry-prod/2054.xml> .

<http://purl.org/wot-catalogue/lwm2m/ipso#3369> a skos:Concept, ontolex:LexicalConcept;
  skos:altLabel "mac timing advance event";
  skos:broader lwm2m:Object;
  skos:definition "Timing advance information";
  skos:inScheme lwm2m:Scheme;
  skos:prefLabel "macTimingAdvanceEvent";
  skos:related lwm2m:r3369-0, lwm2m:r3369-1;
  prov:wasDerivedFrom <file:/data/lp/etl/executor/data/1651932849158-23-3c5fa11b-d02c-40e9-9c76-7d268eee1c69/working/working-outputfiles-214/lwm2m-registry-prod/3369.xml> .

<http://purl.org/wot-catalogue/lwm2m/ipso#3363> a skos:Concept, ontolex:LexicalConcept;
  skos:altLabel "nas esm expiry event";
  skos:broader lwm2m:Object;
  skos:definition "NAS ESM timer expiry information";
  skos:inScheme lwm2m:Scheme;
  skos:prefLabel "nasEsmExpiryEvent";
  skos:related lwm2m:r3363-0;
  prov:wasDerivedFrom <file:/data/lp/etl/executor/data/1651932849158-23-3c5fa11b-d02c-40e9-9c76-7d268eee1c69/working/working-outputfiles-214/lwm2m-registry-prod/3363.xml> .

<http://purl.org/wot-catalogue/lwm2m/ipso#3372> a skos:Concept, ontolex:LexicalConcept;
  skos:altLabel "timing advance";
  skos:broader lwm2m:Object;
  skos:definition "Timing Advance Information";
  skos:inScheme lwm2m:Scheme;
  skos:prefLabel "TimingAdvance";
  skos:related lwm2m:r3372-2, lwm2m:r6037, lwm2m:r6038;
  prov:wasDerivedFrom <file:/data/lp/etl/executor/data/1651932849158-23-3c5fa11b-d02c-40e9-9c76-7d268eee1c69/working/working-outputfiles-214/lwm2m-registry-prod/3372.xml> .

<http://purl.org/wot-catalogue/lwm2m/ipso#3302> a skos:Concept, ontolex:LexicalConcept;
  skos:altLabel "presence";
  skos:broader lwm2m:Object;
  skos:definition "Presence sensor with digital sensing, optional delay parameters";
  skos:inScheme lwm2m:Scheme;
  skos:prefLabel "Presence";
  skos:related lwm2m:r5500, lwm2m:r5501, lwm2m:r5505, lwm2m:r5518, lwm2m:r5750, lwm2m:r5751,
    lwm2m:r5903, lwm2m:r5904, lwm2m:r6042, lwm2m:r6049, lwm2m:r6050;
  prov:wasDerivedFrom <file:/data/lp/etl/executor/data/1651932849158-23-3c5fa11b-d02c-40e9-9c76-7d268eee1c69/working/working-outputfiles-214/lwm2m-registry-prod/3302.xml> .
