@prefix APDU: <http://bacowl.sourceforge.net/2012/bacnet/APDU#> .
@prefix AbortPDU: <http://bacowl.sourceforge.net/2012/bacnet/AbortPDU#> .
@prefix AbortReason: <http://bacowl.sourceforge.net/2012/bacnet/AbortReason#> .
@prefix AccessAuthenticationFactorDisable: <http://bacowl.sourceforge.net/2012/bacnet/AccessAuthenticationFactorDisable#> .
@prefix AccessCredentialDisable: <http://bacowl.sourceforge.net/2012/bacnet/AccessCredentialDisable#> .
@prefix AccessCredentialDisableReason: <http://bacowl.sourceforge.net/2012/bacnet/AccessCredentialDisableReason#> .
@prefix AccessCredentialObject: <http://bacowl.sourceforge.net/2012/bacnet/AccessCredentialObject#> .
@prefix AccessDoorObject: <http://bacowl.sourceforge.net/2012/bacnet/AccessDoorObject#> .
@prefix AccessEvent: <http://bacowl.sourceforge.net/2012/bacnet/AccessEvent#> .
@prefix AccessPassbackMode: <http://bacowl.sourceforge.net/2012/bacnet/AccessPassbackMode#> .
@prefix AccessPointObject: <http://bacowl.sourceforge.net/2012/bacnet/AccessPointObject#> .
@prefix AccessRightsObject: <http://bacowl.sourceforge.net/2012/bacnet/AccessRightsObject#> .
@prefix AccessRule: <http://bacowl.sourceforge.net/2012/bacnet/AccessRule#> .
@prefix AccessRuleLocationSpecifier: <http://bacowl.sourceforge.net/2012/bacnet/AccessRuleLocationSpecifier#> .
@prefix AccessRuleTimeRangeSpecifier: <http://bacowl.sourceforge.net/2012/bacnet/AccessRuleTimeRangeSpecifier#> .
@prefix AccessUserObject: <http://bacowl.sourceforge.net/2012/bacnet/AccessUserObject#> .
@prefix AccessUserType: <http://bacowl.sourceforge.net/2012/bacnet/AccessUserType#> .
@prefix AccessZoneObject: <http://bacowl.sourceforge.net/2012/bacnet/AccessZoneObject#> .
@prefix AccessZoneOccupancyState: <http://bacowl.sourceforge.net/2012/bacnet/AccessZoneOccupancyState#> .
@prefix AccumulatorObject: <http://bacowl.sourceforge.net/2012/bacnet/AccumulatorObject#> .
@prefix AccumulatorRecord: <http://bacowl.sourceforge.net/2012/bacnet/AccumulatorRecord#> .
@prefix AccumulatorRecordAccumulatorStatus: <http://bacowl.sourceforge.net/2012/bacnet/AccumulatorRecordAccumulatorStatus#> .
@prefix AcknowledgeAlarmRequest: <http://bacowl.sourceforge.net/2012/bacnet/AcknowledgeAlarmRequest#> .
@prefix Action: <http://bacowl.sourceforge.net/2012/bacnet/Action#> .
@prefix ActionCommand: <http://bacowl.sourceforge.net/2012/bacnet/ActionCommand#> .
@prefix ActionList: <http://bacowl.sourceforge.net/2012/bacnet/ActionList#> .
@prefix AddListElementRequest: <http://bacowl.sourceforge.net/2012/bacnet/AddListElementRequest#> .
@prefix Address: <http://bacowl.sourceforge.net/2012/bacnet/Address#> .
@prefix AddressBinding: <http://bacowl.sourceforge.net/2012/bacnet/AddressBinding#> .
@prefix AnalogInputObject: <http://bacowl.sourceforge.net/2012/bacnet/AnalogInputObject#> .
@prefix AnalogOutputObject: <http://bacowl.sourceforge.net/2012/bacnet/AnalogOutputObject#> .
@prefix AnalogValueObject: <http://bacowl.sourceforge.net/2012/bacnet/AnalogValueObject#> .
@prefix AssignedAccessRights: <http://bacowl.sourceforge.net/2012/bacnet/AssignedAccessRights#> .
@prefix AtomicReadFileACK: <http://bacowl.sourceforge.net/2012/bacnet/AtomicReadFileACK#> .
@prefix AtomicReadFileACKAccessMethodChoice: <http://bacowl.sourceforge.net/2012/bacnet/AtomicReadFileACKAccessMethodChoice#> .
@prefix AtomicReadFileACKAccessMethodRecordAccess: <http://bacowl.sourceforge.net/2012/bacnet/AtomicReadFileACKAccessMethodRecordAccess#> .
@prefix AtomicReadFileACKAccessMethodStreamAccess: <http://bacowl.sourceforge.net/2012/bacnet/AtomicReadFileACKAccessMethodStreamAccess#> .
@prefix AtomicReadFileRequest: <http://bacowl.sourceforge.net/2012/bacnet/AtomicReadFileRequest#> .
@prefix AtomicReadFileRequestAccessMethodChoice: <http://bacowl.sourceforge.net/2012/bacnet/AtomicReadFileRequestAccessMethodChoice#> .
@prefix AtomicReadFileRequestAccessMethodChoiceRecordAccess: <http://bacowl.sourceforge.net/2012/bacnet/AtomicReadFileRequestAccessMethodChoiceRecordAccess#> .
@prefix AtomicReadFileRequestAccessMethodChoiceStreamAccess: <http://bacowl.sourceforge.net/2012/bacnet/AtomicReadFileRequestAccessMethodChoiceStreamAccess#> .
@prefix AtomicWriteFileACK: <http://bacowl.sourceforge.net/2012/bacnet/AtomicWriteFileACK#> .
@prefix AtomicWriteFileRequest: <http://bacowl.sourceforge.net/2012/bacnet/AtomicWriteFileRequest#> .
@prefix AtomicWriteFileRequestAccessMethodChoice: <http://bacowl.sourceforge.net/2012/bacnet/AtomicWriteFileRequestAccessMethodChoice#> .
@prefix AtomicWriteFileRequestAccessMethodChoiceRecordAccess: <http://bacowl.sourceforge.net/2012/bacnet/AtomicWriteFileRequestAccessMethodChoiceRecordAccess#> .
@prefix AtomicWriteFileRequestAccessMethodChoiceStreamAccess: <http://bacowl.sourceforge.net/2012/bacnet/AtomicWriteFileRequestAccessMethodChoiceStreamAccess#> .
@prefix AuthenticateACK: <http://bacowl.sourceforge.net/2012/bacnet/AuthenticateACK#> .
@prefix AuthenticateRequest: <http://bacowl.sourceforge.net/2012/bacnet/AuthenticateRequest#> .
@prefix AuthenticationFactor: <http://bacowl.sourceforge.net/2012/bacnet/AuthenticationFactor#> .
@prefix AuthenticationFactorFormat: <http://bacowl.sourceforge.net/2012/bacnet/AuthenticationFactorFormat#> .
@prefix AuthenticationFactorType: <http://bacowl.sourceforge.net/2012/bacnet/AuthenticationFactorType#> .
@prefix AuthenticationPolicy: <http://bacowl.sourceforge.net/2012/bacnet/AuthenticationPolicy#> .
@prefix AuthenticationPolicyPolicy: <http://bacowl.sourceforge.net/2012/bacnet/AuthenticationPolicyPolicy#> .
@prefix AuthenticationStatus: <http://bacowl.sourceforge.net/2012/bacnet/AuthenticationStatus#> .
@prefix AuthorizationException: <http://bacowl.sourceforge.net/2012/bacnet/AuthorizationException#> .
@prefix AuthorizationMode: <http://bacowl.sourceforge.net/2012/bacnet/AuthorizationMode#> .
@prefix AveragingObject: <http://bacowl.sourceforge.net/2012/bacnet/AveragingObject#> .
@prefix BACnet: <http://bacowl.sourceforge.net/2012/bacnet#> .
@prefix BackupState: <http://bacowl.sourceforge.net/2012/bacnet/BackupState#> .
@prefix BinaryInputObject: <http://bacowl.sourceforge.net/2012/bacnet/BinaryInputObject#> .
@prefix BinaryOutputObject: <http://bacowl.sourceforge.net/2012/bacnet/BinaryOutputObject#> .
@prefix BinaryPV: <http://bacowl.sourceforge.net/2012/bacnet/BinaryPV#> .
@prefix BinaryValueObject: <http://bacowl.sourceforge.net/2012/bacnet/BinaryValueObject#> .
@prefix Bit: <http://bacowl.sourceforge.net/2012/bacnet/Bit#> .
@prefix BitStringValueObject: <http://bacowl.sourceforge.net/2012/bacnet/BitStringValueObject#> .
@prefix COVNotificationParameters: <http://bacowl.sourceforge.net/2012/bacnet/COVNotificationParameters#> .
@prefix COVSubscription: <http://bacowl.sourceforge.net/2012/bacnet/COVSubscription#> .
@prefix CalendarEntry: <http://bacowl.sourceforge.net/2012/bacnet/CalendarEntry#> .
@prefix CalendarObject: <http://bacowl.sourceforge.net/2012/bacnet/CalendarObject#> .
@prefix ChangeListError: <http://bacowl.sourceforge.net/2012/bacnet/ChangeListError#> .
@prefix ChannelValue: <http://bacowl.sourceforge.net/2012/bacnet/ChannelValue#> .
@prefix CharacterStringValueObject: <http://bacowl.sourceforge.net/2012/bacnet/CharacterStringValueObject#> .
@prefix ClientCOV: <http://bacowl.sourceforge.net/2012/bacnet/ClientCOV#> .
@prefix CommandObject: <http://bacowl.sourceforge.net/2012/bacnet/CommandObject#> .
@prefix ConfirmedCOVNotificationRequest: <http://bacowl.sourceforge.net/2012/bacnet/ConfirmedCOVNotificationRequest#> .
@prefix ConfirmedEventNotificationRequest: <http://bacowl.sourceforge.net/2012/bacnet/ConfirmedEventNotificationRequest#> .
@prefix ConfirmedPrivateTransferACK: <http://bacowl.sourceforge.net/2012/bacnet/ConfirmedPrivateTransferACK#> .
@prefix ConfirmedPrivateTransferError: <http://bacowl.sourceforge.net/2012/bacnet/ConfirmedPrivateTransferError#> .
@prefix ConfirmedPrivateTransferRequest: <http://bacowl.sourceforge.net/2012/bacnet/ConfirmedPrivateTransferRequest#> .
@prefix ConfirmedServiceChoice: <http://bacowl.sourceforge.net/2012/bacnet/ConfirmedServiceChoice#> .
@prefix ConfirmedTextMessageRequest: <http://bacowl.sourceforge.net/2012/bacnet/ConfirmedTextMessageRequest#> .
@prefix ConfirmedTextMessageRequestMessageClass: <http://bacowl.sourceforge.net/2012/bacnet/ConfirmedTextMessageRequestMessageClass#> .
@prefix ConfirmedTextMessageRequestMessagePriority: <http://bacowl.sourceforge.net/2012/bacnet/ConfirmedTextMessageRequestMessagePriority#> .
@prefix CreateObjectACK: <http://bacowl.sourceforge.net/2012/bacnet/CreateObjectACK#> .
@prefix CreateObjectError: <http://bacowl.sourceforge.net/2012/bacnet/CreateObjectError#> .
@prefix CreateObjectRequest: <http://bacowl.sourceforge.net/2012/bacnet/CreateObjectRequest#> .
@prefix CreateObjectRequestObjectSpecifier: <http://bacowl.sourceforge.net/2012/bacnet/CreateObjectRequestObjectSpecifier#> .
@prefix CredentialAuthenticationFactor: <http://bacowl.sourceforge.net/2012/bacnet/CredentialAuthenticationFactor#> .
@prefix CredentialDataInputObject: <http://bacowl.sourceforge.net/2012/bacnet/CredentialDataInputObject#> .
@prefix DailySchedule: <http://bacowl.sourceforge.net/2012/bacnet/DailySchedule#> .
@prefix DatePatternValueObject: <http://bacowl.sourceforge.net/2012/bacnet/DatePatternValueObject#> .
@prefix DateRange: <http://bacowl.sourceforge.net/2012/bacnet/DateRange#> .
@prefix DateTime: <http://bacowl.sourceforge.net/2012/bacnet/DateTime#> .
@prefix DateTimePatternValueObject: <http://bacowl.sourceforge.net/2012/bacnet/DateTimePatternValueObject#> .
@prefix DateTimeValueObject: <http://bacowl.sourceforge.net/2012/bacnet/DateTimeValueObject#> .
@prefix DateValueObject: <http://bacowl.sourceforge.net/2012/bacnet/DateValueObject#> .
@prefix DaysOfWeek: <http://bacowl.sourceforge.net/2012/bacnet/DaysOfWeek#> .
@prefix DeleteObjectRequest: <http://bacowl.sourceforge.net/2012/bacnet/DeleteObjectRequest#> .
@prefix Destination: <http://bacowl.sourceforge.net/2012/bacnet/Destination#> .
@prefix DeviceAddress: <http://bacowl.sourceforge.net/2012/bacnet/DeviceAddress#> .
@prefix DeviceCommunicationControlRequest: <http://bacowl.sourceforge.net/2012/bacnet/DeviceCommunicationControlRequest#> .
@prefix DeviceCommunicationControlRequestEnableDisable: <http://bacowl.sourceforge.net/2012/bacnet/DeviceCommunicationControlRequestEnableDisable#> .
@prefix DeviceObject: <http://bacowl.sourceforge.net/2012/bacnet/DeviceObject#> .
@prefix DeviceObjectPropertyReference: <http://bacowl.sourceforge.net/2012/bacnet/DeviceObjectPropertyReference#> .
@prefix DeviceObjectPropertyValue: <http://bacowl.sourceforge.net/2012/bacnet/DeviceObjectPropertyValue#> .
@prefix DeviceObjectReference: <http://bacowl.sourceforge.net/2012/bacnet/DeviceObjectReference#> .
@prefix DeviceStatus: <http://bacowl.sourceforge.net/2012/bacnet/DeviceStatus#> .
@prefix DoorAlarmState: <http://bacowl.sourceforge.net/2012/bacnet/DoorAlarmState#> .
@prefix DoorSecuredStatus: <http://bacowl.sourceforge.net/2012/bacnet/DoorSecuredStatus#> .
@prefix DoorStatus: <http://bacowl.sourceforge.net/2012/bacnet/DoorStatus#> .
@prefix DoorValue: <http://bacowl.sourceforge.net/2012/bacnet/DoorValue#> .
@prefix Element: <http://bacowl.sourceforge.net/2012/bacnet/Element#> .
@prefix EngineeringUnits: <http://bacowl.sourceforge.net/2012/bacnet/EngineeringUnits#> .
@prefix Enumerated: <http://bacowl.sourceforge.net/2012/bacnet/Enumerated#> .
@prefix Error: <http://bacowl.sourceforge.net/2012/bacnet/Error#> .
@prefix ErrorClass: <http://bacowl.sourceforge.net/2012/bacnet/ErrorClass#> .
@prefix ErrorCode: <http://bacowl.sourceforge.net/2012/bacnet/ErrorCode#> .
@prefix ErrorType: <http://bacowl.sourceforge.net/2012/bacnet/ErrorType#> .
@prefix EventEnrollmentObject: <http://bacowl.sourceforge.net/2012/bacnet/EventEnrollmentObject#> .
@prefix EventLogObject: <http://bacowl.sourceforge.net/2012/bacnet/EventLogObject#> .
@prefix EventLogRecord: <http://bacowl.sourceforge.net/2012/bacnet/EventLogRecord#> .
@prefix EventLogRecordLogDatum: <http://bacowl.sourceforge.net/2012/bacnet/EventLogRecordLogDatum#> .
@prefix EventNotificationParameters: <http://bacowl.sourceforge.net/2012/bacnet/EventNotificationParameters#> .
@prefix EventParameter: <http://bacowl.sourceforge.net/2012/bacnet/EventParameter#> .
@prefix EventParameterAccessEvent: <http://bacowl.sourceforge.net/2012/bacnet/EventParameterAccessEvent#> .
@prefix EventParameterAccessEventAccessEvent: <http://bacowl.sourceforge.net/2012/bacnet/EventParameterAccessEventAccessEvent#> .
@prefix EventParameterBufferReady: <http://bacowl.sourceforge.net/2012/bacnet/EventParameterBufferReady#> .
@prefix EventParameterChangeOfBitstring: <http://bacowl.sourceforge.net/2012/bacnet/EventParameterChangeOfBitstring#> .
@prefix EventParameterChangeOfCharacterString: <http://bacowl.sourceforge.net/2012/bacnet/EventParameterChangeOfCharacterString#> .
@prefix EventParameterChangeOfLifeSafety: <http://bacowl.sourceforge.net/2012/bacnet/EventParameterChangeOfLifeSafety#> .
@prefix EventParameterChangeOfState: <http://bacowl.sourceforge.net/2012/bacnet/EventParameterChangeOfState#> .
@prefix EventParameterChangeOfStatusFlags: <http://bacowl.sourceforge.net/2012/bacnet/EventParameterChangeOfStatusFlags#> .
@prefix EventParameterChangeOfValue: <http://bacowl.sourceforge.net/2012/bacnet/EventParameterChangeOfValue#> .
@prefix EventParameterChangeOfValueCOVCriteria: <http://bacowl.sourceforge.net/2012/bacnet/EventParameterChangeOfValueCOVCriteria#> .
@prefix EventParameterCommandFailure: <http://bacowl.sourceforge.net/2012/bacnet/EventParameterCommandFailure#> .
@prefix EventParameterDoubleOutOfRange: <http://bacowl.sourceforge.net/2012/bacnet/EventParameterDoubleOutOfRange#> .
@prefix EventParameterExtended: <http://bacowl.sourceforge.net/2012/bacnet/EventParameterExtended#> .
@prefix EventParameterExtendedParameters: <http://bacowl.sourceforge.net/2012/bacnet/EventParameterExtendedParameters#> .
@prefix EventParameterFloatingLimit: <http://bacowl.sourceforge.net/2012/bacnet/EventParameterFloatingLimit#> .
@prefix EventParameterOutOfRange: <http://bacowl.sourceforge.net/2012/bacnet/EventParameterOutOfRange#> .
@prefix EventParameterSignedOutOfRange: <http://bacowl.sourceforge.net/2012/bacnet/EventParameterSignedOutOfRange#> .
@prefix EventParameterUnsignedOutOfRange: <http://bacowl.sourceforge.net/2012/bacnet/EventParameterUnsignedOutOfRange#> .
@prefix EventParameterUnsignedRange: <http://bacowl.sourceforge.net/2012/bacnet/EventParameterUnsignedRange#> .
@prefix EventState: <http://bacowl.sourceforge.net/2012/bacnet/EventState#> .
@prefix EventTransitionBits: <http://bacowl.sourceforge.net/2012/bacnet/EventTransitionBits#> .
@prefix EventType: <http://bacowl.sourceforge.net/2012/bacnet/EventType#> .
@prefix FileAccessMethod: <http://bacowl.sourceforge.net/2012/bacnet/FileAccessMethod#> .
@prefix FileObject: <http://bacowl.sourceforge.net/2012/bacnet/FileObject#> .
@prefix GetAlarmSummaryACK: <http://bacowl.sourceforge.net/2012/bacnet/GetAlarmSummaryACK#> .
@prefix GetAlarmSummaryAlarmSummary: <http://bacowl.sourceforge.net/2012/bacnet/GetAlarmSummaryAlarmSummary#> .
@prefix GetAlarmSummaryRequest: <http://bacowl.sourceforge.net/2012/bacnet/GetAlarmSummaryRequest#> .
@prefix GetEnrollmentSummaryACK: <http://bacowl.sourceforge.net/2012/bacnet/GetEnrollmentSummaryACK#> .
@prefix GetEnrollmentSummaryEnrollmentSummary: <http://bacowl.sourceforge.net/2012/bacnet/GetEnrollmentSummaryEnrollmentSummary#> .
@prefix GetEnrollmentSummaryRequest: <http://bacowl.sourceforge.net/2012/bacnet/GetEnrollmentSummaryRequest#> .
@prefix GetEnrollmentSummaryRequestAcknowledgmentFilterType: <http://bacowl.sourceforge.net/2012/bacnet/GetEnrollmentSummaryRequestAcknowledgmentFilterType#> .
@prefix GetEnrollmentSummaryRequestEventStateFilterType: <http://bacowl.sourceforge.net/2012/bacnet/GetEnrollmentSummaryRequestEventStateFilterType#> .
@prefix GetEventInformationACK: <http://bacowl.sourceforge.net/2012/bacnet/GetEventInformationACK#> .
@prefix GetEventInformationEventSummary: <http://bacowl.sourceforge.net/2012/bacnet/GetEventInformationEventSummary#> .
@prefix GetEventInformationRequest: <http://bacowl.sourceforge.net/2012/bacnet/GetEventInformationRequest#> .
@prefix GlobalGroupObject: <http://bacowl.sourceforge.net/2012/bacnet/GlobalGroupObject#> .
@prefix GroupChannelValue: <http://bacowl.sourceforge.net/2012/bacnet/GroupChannelValue#> .
@prefix GroupObject: <http://bacowl.sourceforge.net/2012/bacnet/GroupObject#> .
@prefix IAmRequest: <http://bacowl.sourceforge.net/2012/bacnet/IAmRequest#> .
@prefix IHaveRequest: <http://bacowl.sourceforge.net/2012/bacnet/IHaveRequest#> .
@prefix IntegerValueObject: <http://bacowl.sourceforge.net/2012/bacnet/IntegerValueObject#> .
@prefix KeyIdentifier: <http://bacowl.sourceforge.net/2012/bacnet/KeyIdentifier#> .
@prefix LargeAnalogValueObject: <http://bacowl.sourceforge.net/2012/bacnet/LargeAnalogValueObject#> .
@prefix LifeSafetyMode: <http://bacowl.sourceforge.net/2012/bacnet/LifeSafetyMode#> .
@prefix LifeSafetyOperation: <http://bacowl.sourceforge.net/2012/bacnet/LifeSafetyOperation#> .
@prefix LifeSafetyOperationRequest: <http://bacowl.sourceforge.net/2012/bacnet/LifeSafetyOperationRequest#> .
@prefix LifeSafetyPointObject: <http://bacowl.sourceforge.net/2012/bacnet/LifeSafetyPointObject#> .
@prefix LifeSafetyState: <http://bacowl.sourceforge.net/2012/bacnet/LifeSafetyState#> .
@prefix LifeSafetyZoneObject: <http://bacowl.sourceforge.net/2012/bacnet/LifeSafetyZoneObject#> .
@prefix LightingInProgress: <http://bacowl.sourceforge.net/2012/bacnet/LightingInProgress#> .
@prefix LightingOperation: <http://bacowl.sourceforge.net/2012/bacnet/LightingOperation#> .
@prefix LightingTransition: <http://bacowl.sourceforge.net/2012/bacnet/LightingTransition#> .
@prefix LimitEnable: <http://bacowl.sourceforge.net/2012/bacnet/LimitEnable#> .
@prefix LoadControlObject: <http://bacowl.sourceforge.net/2012/bacnet/LoadControlObject#> .
@prefix LockStatus: <http://bacowl.sourceforge.net/2012/bacnet/LockStatus#> .
@prefix LogData: <http://bacowl.sourceforge.net/2012/bacnet/LogData#> .
@prefix LogDataLogData: <http://bacowl.sourceforge.net/2012/bacnet/LogDataLogData#> .
@prefix LogMultipleRecord: <http://bacowl.sourceforge.net/2012/bacnet/LogMultipleRecord#> .
@prefix LogRecord: <http://bacowl.sourceforge.net/2012/bacnet/LogRecord#> .
@prefix LogRecordLogDatum: <http://bacowl.sourceforge.net/2012/bacnet/LogRecordLogDatum#> .
@prefix LogStatus: <http://bacowl.sourceforge.net/2012/bacnet/LogStatus#> .
@prefix LoggingType: <http://bacowl.sourceforge.net/2012/bacnet/LoggingType#> .
@prefix LoopObject: <http://bacowl.sourceforge.net/2012/bacnet/LoopObject#> .
@prefix Maintenance: <http://bacowl.sourceforge.net/2012/bacnet/Maintenance#> .
@prefix MultiStateInputObject: <http://bacowl.sourceforge.net/2012/bacnet/MultiStateInputObject#> .
@prefix MultiStateOutputObject: <http://bacowl.sourceforge.net/2012/bacnet/MultiStateOutputObject#> .
@prefix MultiStateValueObject: <http://bacowl.sourceforge.net/2012/bacnet/MultiStateValueObject#> .
@prefix NetworkSecurityObject: <http://bacowl.sourceforge.net/2012/bacnet/NetworkSecurityObject#> .
@prefix NetworkSecurityPolicy: <http://bacowl.sourceforge.net/2012/bacnet/NetworkSecurityPolicy#> .
@prefix NodeType: <http://bacowl.sourceforge.net/2012/bacnet/NodeType#> .
@prefix NotificationClassObject: <http://bacowl.sourceforge.net/2012/bacnet/NotificationClassObject#> .
@prefix NotificationParameters: <http://bacowl.sourceforge.net/2012/bacnet/NotificationParameters#> .
@prefix NotificationParametersAccessEventType: <http://bacowl.sourceforge.net/2012/bacnet/NotificationParametersAccessEventType#> .
@prefix NotificationParametersBufferReady: <http://bacowl.sourceforge.net/2012/bacnet/NotificationParametersBufferReady#> .
@prefix NotificationParametersChangeOfBitstring: <http://bacowl.sourceforge.net/2012/bacnet/NotificationParametersChangeOfBitstring#> .
@prefix NotificationParametersChangeOfCharacterStringType: <http://bacowl.sourceforge.net/2012/bacnet/NotificationParametersChangeOfCharacterStringType#> .
@prefix NotificationParametersChangeOfLifeSafety: <http://bacowl.sourceforge.net/2012/bacnet/NotificationParametersChangeOfLifeSafety#> .
@prefix NotificationParametersChangeOfState: <http://bacowl.sourceforge.net/2012/bacnet/NotificationParametersChangeOfState#> .
@prefix NotificationParametersChangeOfStatusFlagsType: <http://bacowl.sourceforge.net/2012/bacnet/NotificationParametersChangeOfStatusFlagsType#> .
@prefix NotificationParametersChangeOfValue: <http://bacowl.sourceforge.net/2012/bacnet/NotificationParametersChangeOfValue#> .
@prefix NotificationParametersChangeOfValueNewValue: <http://bacowl.sourceforge.net/2012/bacnet/NotificationParametersChangeOfValueNewValue#> .
@prefix NotificationParametersCommandFailure: <http://bacowl.sourceforge.net/2012/bacnet/NotificationParametersCommandFailure#> .
@prefix NotificationParametersComplexEventType: <http://bacowl.sourceforge.net/2012/bacnet/NotificationParametersComplexEventType#> .
@prefix NotificationParametersDoubleOutOfRangeType: <http://bacowl.sourceforge.net/2012/bacnet/NotificationParametersDoubleOutOfRangeType#> .
@prefix NotificationParametersExtended: <http://bacowl.sourceforge.net/2012/bacnet/NotificationParametersExtended#> .
@prefix NotificationParametersExtendedParametersType: <http://bacowl.sourceforge.net/2012/bacnet/NotificationParametersExtendedParametersType#> .
@prefix NotificationParametersFloatingLimit: <http://bacowl.sourceforge.net/2012/bacnet/NotificationParametersFloatingLimit#> .
@prefix NotificationParametersOutOfRange: <http://bacowl.sourceforge.net/2012/bacnet/NotificationParametersOutOfRange#> .
@prefix NotificationParametersSignedOutOfRangeType: <http://bacowl.sourceforge.net/2012/bacnet/NotificationParametersSignedOutOfRangeType#> .
@prefix NotificationParametersUnsignedOutOfRangeType: <http://bacowl.sourceforge.net/2012/bacnet/NotificationParametersUnsignedOutOfRangeType#> .
@prefix NotificationParametersUnsignedRange: <http://bacowl.sourceforge.net/2012/bacnet/NotificationParametersUnsignedRange#> .
@prefix NotifyType: <http://bacowl.sourceforge.net/2012/bacnet/NotifyType#> .
@prefix Null: <http://bacowl.sourceforge.net/2012/bacnet/Null#> .
@prefix Object: <http://bacowl.sourceforge.net/2012/bacnet/Object#> .
@prefix ObjectIdentifier: <http://bacowl.sourceforge.net/2012/bacnet/ObjectIdentifier#> .
@prefix ObjectPropertyReference: <http://bacowl.sourceforge.net/2012/bacnet/ObjectPropertyReference#> .
@prefix ObjectPropertyValue: <http://bacowl.sourceforge.net/2012/bacnet/ObjectPropertyValue#> .
@prefix ObjectType: <http://bacowl.sourceforge.net/2012/bacnet/ObjectType#> .
@prefix ObjectTypesSupported: <http://bacowl.sourceforge.net/2012/bacnet/ObjectTypesSupported#> .
@prefix OctetStringValueObject: <http://bacowl.sourceforge.net/2012/bacnet/OctetStringValueObject#> .
@prefix OptionalCharacterString: <http://bacowl.sourceforge.net/2012/bacnet/OptionalCharacterString#> .
@prefix Polarity: <http://bacowl.sourceforge.net/2012/bacnet/Polarity#> .
@prefix PositiveIntegerValueObject: <http://bacowl.sourceforge.net/2012/bacnet/PositiveIntegerValueObject#> .
@prefix Prescale: <http://bacowl.sourceforge.net/2012/bacnet/Prescale#> .
@prefix PriorityValue: <http://bacowl.sourceforge.net/2012/bacnet/PriorityValue#> .
@prefix ProgramError: <http://bacowl.sourceforge.net/2012/bacnet/ProgramError#> .
@prefix ProgramObject: <http://bacowl.sourceforge.net/2012/bacnet/ProgramObject#> .
@prefix ProgramRequest: <http://bacowl.sourceforge.net/2012/bacnet/ProgramRequest#> .
@prefix ProgramState: <http://bacowl.sourceforge.net/2012/bacnet/ProgramState#> .
@prefix Property: <http://bacowl.sourceforge.net/2012/bacnet/Property#> .
@prefix PropertyAccessResult: <http://bacowl.sourceforge.net/2012/bacnet/PropertyAccessResult#> .
@prefix PropertyAccessResultAccessResult: <http://bacowl.sourceforge.net/2012/bacnet/PropertyAccessResultAccessResult#> .
@prefix PropertyIdentifier: <http://bacowl.sourceforge.net/2012/bacnet/PropertyIdentifier#> .
@prefix PropertyReference: <http://bacowl.sourceforge.net/2012/bacnet/PropertyReference#> .
@prefix PropertyStates: <http://bacowl.sourceforge.net/2012/bacnet/PropertyStates#> .
@prefix PropertyValue: <http://bacowl.sourceforge.net/2012/bacnet/PropertyValue#> .
@prefix PulseConverterObject: <http://bacowl.sourceforge.net/2012/bacnet/PulseConverterObject#> .
@prefix Range: <http://bacowl.sourceforge.net/2012/bacnet/Range#> .
@prefix RangeByPosition: <http://bacowl.sourceforge.net/2012/bacnet/RangeByPosition#> .
@prefix RangeBySequenceNumber: <http://bacowl.sourceforge.net/2012/bacnet/RangeBySequenceNumber#> .
@prefix RangeByTime: <http://bacowl.sourceforge.net/2012/bacnet/RangeByTime#> .
@prefix ReadAccessResult: <http://bacowl.sourceforge.net/2012/bacnet/ReadAccessResult#> .
@prefix ReadAccessResultElement: <http://bacowl.sourceforge.net/2012/bacnet/ReadAccessResultElement#> .
@prefix ReadAccessResultElementChoice: <http://bacowl.sourceforge.net/2012/bacnet/ReadAccessResultElementChoice#> .
@prefix ReadAccessSpecification: <http://bacowl.sourceforge.net/2012/bacnet/ReadAccessSpecification#> .
@prefix ReadPropertyACK: <http://bacowl.sourceforge.net/2012/bacnet/ReadPropertyACK#> .
@prefix ReadPropertyMultipleACK: <http://bacowl.sourceforge.net/2012/bacnet/ReadPropertyMultipleACK#> .
@prefix ReadPropertyMultipleRequest: <http://bacowl.sourceforge.net/2012/bacnet/ReadPropertyMultipleRequest#> .
@prefix ReadPropertyRequest: <http://bacowl.sourceforge.net/2012/bacnet/ReadPropertyRequest#> .
@prefix ReadRangeACK: <http://bacowl.sourceforge.net/2012/bacnet/ReadRangeACK#> .
@prefix ReadRangeRequest: <http://bacowl.sourceforge.net/2012/bacnet/ReadRangeRequest#> .
@prefix Recipient: <http://bacowl.sourceforge.net/2012/bacnet/Recipient#> .
@prefix RecipientProcess: <http://bacowl.sourceforge.net/2012/bacnet/RecipientProcess#> .
@prefix ReinitializeDeviceRequest: <http://bacowl.sourceforge.net/2012/bacnet/ReinitializeDeviceRequest#> .
@prefix ReinitializeDeviceRequestReinitializedStateOfDevice: <http://bacowl.sourceforge.net/2012/bacnet/ReinitializeDeviceRequestReinitializedStateOfDevice#> .
@prefix RejectPDU: <http://bacowl.sourceforge.net/2012/bacnet/RejectPDU#> .
@prefix RejectReason: <http://bacowl.sourceforge.net/2012/bacnet/RejectReason#> .
@prefix Reliability: <http://bacowl.sourceforge.net/2012/bacnet/Reliability#> .
@prefix RemoveListElementRequest: <http://bacowl.sourceforge.net/2012/bacnet/RemoveListElementRequest#> .
@prefix RequestKeyRequest: <http://bacowl.sourceforge.net/2012/bacnet/RequestKeyRequest#> .
@prefix RestartReason: <http://bacowl.sourceforge.net/2012/bacnet/RestartReason#> .
@prefix ResultFlags: <http://bacowl.sourceforge.net/2012/bacnet/ResultFlags#> .
@prefix Scale: <http://bacowl.sourceforge.net/2012/bacnet/Scale#> .
@prefix ScheduleObject: <http://bacowl.sourceforge.net/2012/bacnet/ScheduleObject#> .
@prefix SecurityKeySet: <http://bacowl.sourceforge.net/2012/bacnet/SecurityKeySet#> .
@prefix SecurityLevel: <http://bacowl.sourceforge.net/2012/bacnet/SecurityLevel#> .
@prefix SecurityPolicy: <http://bacowl.sourceforge.net/2012/bacnet/SecurityPolicy#> .
@prefix Segmentation: <http://bacowl.sourceforge.net/2012/bacnet/Segmentation#> .
@prefix Sequence: <http://bacowl.sourceforge.net/2012/bacnet/Sequence#> .
@prefix SequenceElement: <http://bacowl.sourceforge.net/2012/bacnet/SequenceElement#> .
@prefix SequenceOf: <http://bacowl.sourceforge.net/2012/bacnet/SequenceOf#> .
@prefix ServicesSupported: <http://bacowl.sourceforge.net/2012/bacnet/ServicesSupported#> .
@prefix SetpointReference: <http://bacowl.sourceforge.net/2012/bacnet/SetpointReference#> .
@prefix ShedLevel: <http://bacowl.sourceforge.net/2012/bacnet/ShedLevel#> .
@prefix ShedState: <http://bacowl.sourceforge.net/2012/bacnet/ShedState#> .
@prefix SilencedState: <http://bacowl.sourceforge.net/2012/bacnet/SilencedState#> .
@prefix SpecialEvent: <http://bacowl.sourceforge.net/2012/bacnet/SpecialEvent#> .
@prefix SpecialEventPeriod: <http://bacowl.sourceforge.net/2012/bacnet/SpecialEventPeriod#> .
@prefix StatusFlags: <http://bacowl.sourceforge.net/2012/bacnet/StatusFlags#> .
@prefix StructuredViewObject: <http://bacowl.sourceforge.net/2012/bacnet/StructuredViewObject#> .
@prefix SubscribeCOVPropertyRequest: <http://bacowl.sourceforge.net/2012/bacnet/SubscribeCOVPropertyRequest#> .
@prefix SubscribeCOVRequest: <http://bacowl.sourceforge.net/2012/bacnet/SubscribeCOVRequest#> .
@prefix TimePatternValueObject: <http://bacowl.sourceforge.net/2012/bacnet/TimePatternValueObject#> .
@prefix TimeStamp: <http://bacowl.sourceforge.net/2012/bacnet/TimeStamp#> .
@prefix TimeSynchronizationRequest: <http://bacowl.sourceforge.net/2012/bacnet/TimeSynchronizationRequest#> .
@prefix TimeValue: <http://bacowl.sourceforge.net/2012/bacnet/TimeValue#> .
@prefix TimeValueObject: <http://bacowl.sourceforge.net/2012/bacnet/TimeValueObject#> .
@prefix TrendLogMultipleObject: <http://bacowl.sourceforge.net/2012/bacnet/TrendLogMultipleObject#> .
@prefix TrendLogObject: <http://bacowl.sourceforge.net/2012/bacnet/TrendLogObject#> .
@prefix UTCTimeSynchronizationRequest: <http://bacowl.sourceforge.net/2012/bacnet/UTCTimeSynchronizationRequest#> .
@prefix UnconfirmedCOVNotificationRequest: <http://bacowl.sourceforge.net/2012/bacnet/UnconfirmedCOVNotificationRequest#> .
@prefix UnconfirmedEventNotificationRequest: <http://bacowl.sourceforge.net/2012/bacnet/UnconfirmedEventNotificationRequest#> .
@prefix UnconfirmedPrivateTransferRequest: <http://bacowl.sourceforge.net/2012/bacnet/UnconfirmedPrivateTransferRequest#> .
@prefix UnconfirmedServiceChoice: <http://bacowl.sourceforge.net/2012/bacnet/UnconfirmedServiceChoice#> .
@prefix UnconfirmedTextMessageRequest: <http://bacowl.sourceforge.net/2012/bacnet/UnconfirmedTextMessageRequest#> .
@prefix UnconfirmedTextMessageRequestMessageClass: <http://bacowl.sourceforge.net/2012/bacnet/UnconfirmedTextMessageRequestMessageClass#> .
@prefix UnconfirmedTextMessageRequestMessagePriority: <http://bacowl.sourceforge.net/2012/bacnet/UnconfirmedTextMessageRequestMessagePriority#> .
@prefix VTClass: <http://bacowl.sourceforge.net/2012/bacnet/VTClass#> .
@prefix VTCloseError: <http://bacowl.sourceforge.net/2012/bacnet/VTCloseError#> .
@prefix VTCloseRequest: <http://bacowl.sourceforge.net/2012/bacnet/VTCloseRequest#> .
@prefix VTDataACK: <http://bacowl.sourceforge.net/2012/bacnet/VTDataACK#> .
@prefix VTDataRequest: <http://bacowl.sourceforge.net/2012/bacnet/VTDataRequest#> .
@prefix VTOpenACK: <http://bacowl.sourceforge.net/2012/bacnet/VTOpenACK#> .
@prefix VTOpenRequest: <http://bacowl.sourceforge.net/2012/bacnet/VTOpenRequest#> .
@prefix VTSession: <http://bacowl.sourceforge.net/2012/bacnet/VTSession#> .
@prefix Vendor: <http://bacowl.sourceforge.net/2012/bacnet/Vendor#> .
@prefix WhoHasLimits: <http://bacowl.sourceforge.net/2012/bacnet/WhoHasLimits#> .
@prefix WhoHasObject: <http://bacowl.sourceforge.net/2012/bacnet/WhoHasObject#> .
@prefix WhoHasRequest: <http://bacowl.sourceforge.net/2012/bacnet/WhoHasRequest#> .
@prefix WhoIsRequest: <http://bacowl.sourceforge.net/2012/bacnet/WhoIsRequest#> .
@prefix WriteAccessSpecification: <http://bacowl.sourceforge.net/2012/bacnet/WriteAccessSpecification#> .
@prefix WriteGroupRequest: <http://bacowl.sourceforge.net/2012/bacnet/WriteGroupRequest#> .
@prefix WritePropertyMultipleError: <http://bacowl.sourceforge.net/2012/bacnet/WritePropertyMultipleError#> .
@prefix WritePropertyMultipleRequest: <http://bacowl.sourceforge.net/2012/bacnet/WritePropertyMultipleRequest#> .
@prefix WritePropertyRequest: <http://bacowl.sourceforge.net/2012/bacnet/WritePropertyRequest#> .
@prefix WriteStatus: <http://bacowl.sourceforge.net/2012/bacnet/WriteStatus#> .
@prefix bacnet: <http://purl.org/wot-catalogue/bacnet#> .
@prefix ble: <http://purl.org/wot-catalogue/ble#> .
@prefix dtype: <http://www.linkedmodel.org/schema/dtype#> .
@prefix fn: <http://www.w3.org/2005/xpath-functions#> .
@prefix hgi: <http://homegatewayinitiative.org/xml/dal/3.0> .
@prefix httpList: <http://plugins.linkedpipes.com/ontology/e-httpGetFiles#> .
@prefix lwm2m: <http://purl.org/wot-catalogue/lwm2m#> .
@prefix ocf: <http://purl.org/wot-catalogue/ocf#> .
@prefix ontolex: <http://www.w3.org/ns/lemon/ontolex#> .
@prefix owl: <http://www.w3.org/2002/07/owl#> .
@prefix prov: <http://www.w3.org/ns/prov#> .
@prefix rdf: <http://www.w3.org/1999/02/22-rdf-syntax-ns#> .
@prefix rdfs: <http://www.w3.org/2000/01/rdf-schema#> .
@prefix sdt: <http://purl.org/wot-catalogue/sdt#> .
@prefix skos: <http://www.w3.org/2004/02/skos/core#> .
@prefix xs: <http://www.w3.org/2001/XMLSchema> .
@prefix xsd: <http://www.w3.org/2001/XMLSchema#> .

<http://purl.org/wot-catalogue/ble/gatt#> a skos:Collection;
  skos:member <http://purl.org/wot-catalogue/ble/gatt#180E>, <http://purl.org/wot-catalogue/ble/gatt#180F>,
    <http://purl.org/wot-catalogue/ble/gatt#1814>, <http://purl.org/wot-catalogue/ble/gatt#1823>,
    <http://purl.org/wot-catalogue/ble/gatt#1825>, <http://purl.org/wot-catalogue/ble/gatt#AnaerobicHeartRateUpperLimit>,
    <http://purl.org/wot-catalogue/ble/gatt#AnalogInput>, <http://purl.org/wot-catalogue/ble/gatt#AveragePower>,
    <http://purl.org/wot-catalogue/ble/gatt#AverageSpeed>, <http://purl.org/wot-catalogue/ble/gatt#AverageStepRate>,
    <http://purl.org/wot-catalogue/ble/gatt#CGMStatus>, <http://purl.org/wot-catalogue/ble/gatt#E2E-CRC>,
    <http://purl.org/wot-catalogue/ble/gatt#ElapsedTime>, <http://purl.org/wot-catalogue/ble/gatt#1806>,
    <http://purl.org/wot-catalogue/ble/gatt#Elevation>, <http://purl.org/wot-catalogue/ble/gatt#EnergyPerHour>,
    <http://purl.org/wot-catalogue/ble/gatt#EnergyPerMinute>, <http://purl.org/wot-catalogue/ble/gatt#FatBurnHeartRateLowerLimit>,
    <http://purl.org/wot-catalogue/ble/gatt#FirmwareRevision>, <http://purl.org/wot-catalogue/ble/gatt#DeviceandSensorStatusSupport>,
    <http://purl.org/wot-catalogue/ble/gatt#FiveZoneHeartRateLimits-Hard/MaximumLimit>,
    <http://purl.org/wot-catalogue/ble/gatt#CategoryID>, <http://purl.org/wot-catalogue/ble/gatt#1821>,
    <http://purl.org/wot-catalogue/ble/gatt#FiveZoneHeartRateLimits-Light/ModerateLimit>,
    <http://purl.org/wot-catalogue/ble/gatt#FiveZoneHeartRateLimits-Moderate/HardLimit>,
    <http://purl.org/wot-catalogue/ble/gatt#FiveZoneHeartRateLimits-Verylight/LightLimit>,
    <http://purl.org/wot-catalogue/ble/gatt#Flags>, <http://purl.org/wot-catalogue/ble/gatt#HeartRate>,
    <http://purl.org/wot-catalogue/ble/gatt#HeartRateControlPoint>, <http://purl.org/wot-catalogue/ble/gatt#HipCircumference>,
    <http://purl.org/wot-catalogue/ble/gatt#Inclination>, <http://purl.org/wot-catalogue/ble/gatt#Indicate>,
    <http://purl.org/wot-catalogue/ble/gatt#InputBits>, <http://purl.org/wot-catalogue/ble/gatt#CyclingPowerFeature>,
    <http://purl.org/wot-catalogue/ble/gatt#CurrentSize>, <http://purl.org/wot-catalogue/ble/gatt#AllocatedSize>,
    <http://purl.org/wot-catalogue/ble/gatt#InstantaneousPower>, <http://purl.org/wot-catalogue/ble/gatt#InstantaneousSpeed>,
    <http://purl.org/wot-catalogue/ble/gatt#181E>, <http://purl.org/wot-catalogue/ble/gatt#IntermediateTemperature>,
    <http://purl.org/wot-catalogue/ble/gatt#Irradiance>, <http://purl.org/wot-catalogue/ble/gatt#LNFeature>,
    <http://purl.org/wot-catalogue/ble/gatt#1805>, <http://purl.org/wot-catalogue/ble/gatt#ManufacturerIdentifier>,
    <http://purl.org/wot-catalogue/ble/gatt#MaximumSpeed>, <http://purl.org/wot-catalogue/ble/gatt#MeasurementInterval>,
    <http://purl.org/wot-catalogue/ble/gatt#MeasurementStatusSupport>, <http://purl.org/wot-catalogue/ble/gatt#MetabolicEquivalent>,
    <http://purl.org/wot-catalogue/ble/gatt#MinimumIncrement>, <http://purl.org/wot-catalogue/ble/gatt#MinimumSpeed>,
    <http://purl.org/wot-catalogue/ble/gatt#MeasurementStatus>, <http://purl.org/wot-catalogue/ble/gatt#DeviceandSensorStatus>,
    <http://purl.org/wot-catalogue/ble/gatt#NegativeElevationGain>, <http://purl.org/wot-catalogue/ble/gatt#1824>,
    <http://purl.org/wot-catalogue/ble/gatt#Notify>, <http://purl.org/wot-catalogue/ble/gatt#CumulativeValue>,
    <http://purl.org/wot-catalogue/ble/gatt#ObjectFirst-Created>, <http://purl.org/wot-catalogue/ble/gatt#OpCode>,
    <http://purl.org/wot-catalogue/ble/gatt#Operand>, <http://purl.org/wot-catalogue/ble/gatt#Operator>,
    <http://purl.org/wot-catalogue/ble/gatt#OrganizationallyUniqueIdentifier>, <http://purl.org/wot-catalogue/ble/gatt#PositiveElevationGain>,
    <http://purl.org/wot-catalogue/ble/gatt#PulseAmplitudeIndex>, <http://purl.org/wot-catalogue/ble/gatt#GlucoseFeature>,
    <http://purl.org/wot-catalogue/ble/gatt#RSCFeature>, <http://purl.org/wot-catalogue/ble/gatt#Rainfall>,
    <http://purl.org/wot-catalogue/ble/gatt#AerobicThreshold>, <http://purl.org/wot-catalogue/ble/gatt#RampAngleSetting>,
    <http://purl.org/wot-catalogue/ble/gatt#CGMFeature>, <http://purl.org/wot-catalogue/ble/gatt#CGMType>,
    <http://purl.org/wot-catalogue/ble/gatt#CGMSampleLocation>, <http://purl.org/wot-catalogue/ble/gatt#Read>,
    <http://purl.org/wot-catalogue/ble/gatt#ModelNumber>, <http://purl.org/wot-catalogue/ble/gatt#ReliableWrite>,
    <http://purl.org/wot-catalogue/ble/gatt#Analog>, <http://purl.org/wot-catalogue/ble/gatt#1826>,
    <http://purl.org/wot-catalogue/ble/gatt#RemainingTime>, <http://purl.org/wot-catalogue/ble/gatt#RequestOpCode>,
    <http://purl.org/wot-catalogue/ble/gatt#ResistanceLevel>, <http://purl.org/wot-catalogue/ble/gatt#ResolvablePrivateAddress>,
    <http://purl.org/wot-catalogue/ble/gatt#ResponseParameter>, <http://purl.org/wot-catalogue/ble/gatt#ResponseValue>,
    <http://purl.org/wot-catalogue/ble/gatt#RingerSetting>, <http://purl.org/wot-catalogue/ble/gatt#SensorLocationValue>,
    <http://purl.org/wot-catalogue/ble/gatt#SpO2PR-Spot-Check-PR>, <http://purl.org/wot-catalogue/ble/gatt#SpO2PR-Spot-Check-SpO2>,
    <http://purl.org/wot-catalogue/ble/gatt#SportTypeforAerobicandAnaerobicThresholds>,
    <http://purl.org/wot-catalogue/ble/gatt#StepPerMinute>, <http://purl.org/wot-catalogue/ble/gatt#StrideCount>,
    <http://purl.org/wot-catalogue/ble/gatt#ApparentWindSpeed>, <http://purl.org/wot-catalogue/ble/gatt#LocationName>,
    <http://purl.org/wot-catalogue/ble/gatt#SupportedFeatures>, <http://purl.org/wot-catalogue/ble/gatt#CSCFeature>,
    <http://purl.org/wot-catalogue/ble/gatt#TimeOffset>, <http://purl.org/wot-catalogue/ble/gatt#TimeSource>,
    <http://purl.org/wot-catalogue/ble/gatt#Timestamp>, <http://purl.org/wot-catalogue/ble/gatt#FirstName>,
    <http://purl.org/wot-catalogue/ble/gatt#HTTPEntityBody>, <http://purl.org/wot-catalogue/ble/gatt#TotalDistance>,
    <http://purl.org/wot-catalogue/ble/gatt#TimeZone>, <http://purl.org/wot-catalogue/ble/gatt#TotalEnergy>,
    <http://purl.org/wot-catalogue/ble/gatt#OpCode-ResponseCodes>, <http://purl.org/wot-catalogue/ble/gatt#CalibrationValue-GlucoseConcentrationofCalibration>,
    <http://purl.org/wot-catalogue/ble/gatt#CalibrationValue-CalibrationTime>, <http://purl.org/wot-catalogue/ble/gatt#CalibrationValue-CalibrationType>,
    <http://purl.org/wot-catalogue/ble/gatt#CalibrationValue-CalibrationSampleLocation>,
    <http://purl.org/wot-catalogue/ble/gatt#CalibrationValue-NextCalibrationTime>, <http://purl.org/wot-catalogue/ble/gatt#CalibrationValue-CalibrationDataRecordNumber>,
    <http://purl.org/wot-catalogue/ble/gatt#CalibrationValue-CalibrationStatus>, <http://purl.org/wot-catalogue/ble/gatt#TrueWindSpeed>,
    <http://purl.org/wot-catalogue/ble/gatt#DewPoint>, <http://purl.org/wot-catalogue/ble/gatt#1813>,
    <http://purl.org/wot-catalogue/ble/gatt#URI>, <http://purl.org/wot-catalogue/ble/gatt#UVIndex>,
    <http://purl.org/wot-catalogue/ble/gatt#VO2Max>, <http://purl.org/wot-catalogue/ble/gatt#TwozoneHeartRateLimit-Fatburn/FitnessLimit>,
    <http://purl.org/wot-catalogue/ble/gatt#1820>, <http://purl.org/wot-catalogue/ble/gatt#WindChill>,
    <http://purl.org/wot-catalogue/ble/gatt#ProtocolModeValue>, <http://purl.org/wot-catalogue/ble/gatt#Write>,
    <http://purl.org/wot-catalogue/ble/gatt#AerobicHeartRateLowerLimit>, <http://purl.org/wot-catalogue/ble/gatt#LE_Scan_Interval>,
    <http://purl.org/wot-catalogue/ble/gatt#LE_Scan_Window>, <http://purl.org/wot-catalogue/ble/gatt#1800>,
    <http://purl.org/wot-catalogue/ble/gatt#HTTPHeaders>, <http://purl.org/wot-catalogue/ble/gatt#org.bluetooth.characteristic.aerobic_heart_rate_lower_limit>,
    <http://purl.org/wot-catalogue/ble/gatt#ManufacturerName>, <http://purl.org/wot-catalogue/ble/gatt#AlertStatus>,
    <http://purl.org/wot-catalogue/ble/gatt#org.bluetooth.characteristic.aerobic_threshold>,
    <http://purl.org/wot-catalogue/ble/gatt#Language>, <http://purl.org/wot-catalogue/ble/gatt#org.bluetooth.characteristic.aggregate>,
    <http://purl.org/wot-catalogue/ble/gatt#SpO2PR-Normal-SpO2>, <http://purl.org/wot-catalogue/ble/gatt#SpO2PR-Normal-PR>,
    <http://purl.org/wot-catalogue/ble/gatt#SpO2PR-Fast-SpO2>, <http://purl.org/wot-catalogue/ble/gatt#SpO2PR-Fast-PR>,
    <http://purl.org/wot-catalogue/ble/gatt#SpO2PR-Slow-SpO2>, <http://purl.org/wot-catalogue/ble/gatt#SpO2PR-Slow-PR>,
    <http://purl.org/wot-catalogue/ble/gatt#org.bluetooth.characteristic.alert_category_id>,
    <http://purl.org/wot-catalogue/ble/gatt#SoftwareRevision>, <http://purl.org/wot-catalogue/ble/gatt#org.bluetooth.characteristic.alert_status>,
    <http://purl.org/wot-catalogue/ble/gatt#LastName>, <http://purl.org/wot-catalogue/ble/gatt#org.bluetooth.characteristic.altitude>,
    <http://purl.org/wot-catalogue/ble/gatt#TxPower>, <http://purl.org/wot-catalogue/ble/gatt#Altitude>,
    <http://purl.org/wot-catalogue/ble/gatt#org.bluetooth.characteristic.anaerobic_heart_rate_upper_limit>,
    <http://purl.org/wot-catalogue/ble/gatt#CrankRevolutionData-CumulativeCrankRevolutions>,
    <http://purl.org/wot-catalogue/ble/gatt#CrankRevolutionData-LastCrankEventTime>, <http://purl.org/wot-catalogue/ble/gatt#FirstCrankMeasurementAngle>,
    <http://purl.org/wot-catalogue/ble/gatt#InstantaneousForceMagnitudeArray>, <http://purl.org/wot-catalogue/ble/gatt#InstantaneousTorqueMagnitudeArray>,
    <http://purl.org/wot-catalogue/ble/gatt#org.bluetooth.characteristic.analog>, <http://purl.org/wot-catalogue/ble/gatt#CGMSessionRunTime>,
    <http://purl.org/wot-catalogue/ble/gatt#InstantaneousCadence>, <http://purl.org/wot-catalogue/ble/gatt#AverageCadence>,
    <http://purl.org/wot-catalogue/ble/gatt#StrokeRate>, <http://purl.org/wot-catalogue/ble/gatt#StrokeCount>,
    <http://purl.org/wot-catalogue/ble/gatt#AverageStrokeRate>, <http://purl.org/wot-catalogue/ble/gatt#InstantaneousPace>,
    <http://purl.org/wot-catalogue/ble/gatt#AveragePace>, <http://purl.org/wot-catalogue/ble/gatt#1809>,
    <http://purl.org/wot-catalogue/ble/gatt#org.bluetooth.characteristic.apparent_wind_speed>,
    <http://purl.org/wot-catalogue/ble/gatt#org.bluetooth.characteristic.battery_level>,
    <http://purl.org/wot-catalogue/ble/gatt#org.bluetooth.characteristic.bond_management_control_point>,
    <http://purl.org/wot-catalogue/ble/gatt#BootMouseInputReportValue>, <http://purl.org/wot-catalogue/ble/gatt#org.bluetooth.characteristic.bond_management_feature>,
    <http://purl.org/wot-catalogue/ble/gatt#OpCodes>, <http://purl.org/wot-catalogue/ble/gatt#ParameterValue>,
    <http://purl.org/wot-catalogue/ble/gatt#org.bluetooth.characteristic.boot_keyboard_input_report>,
    <http://purl.org/wot-catalogue/ble/gatt#BootKeyboardInputReportValue>, <http://purl.org/wot-catalogue/ble/gatt#org.bluetooth.characteristic.boot_mouse_input_report>,
    <http://purl.org/wot-catalogue/ble/gatt#IntermediateCuffPressure>, <http://purl.org/wot-catalogue/ble/gatt#1818>,
    <http://purl.org/wot-catalogue/ble/gatt#org.bluetooth.characteristic.cgm_feature>,
    <http://purl.org/wot-catalogue/ble/gatt#org.bluetooth.characteristic.blood_pressure_measurement>,
    <http://purl.org/wot-catalogue/ble/gatt#BloodPressureMeasurementCompoundValue-Systolic(mmHg)>,
    <http://purl.org/wot-catalogue/ble/gatt#BloodPressureMeasurementCompoundValue-Diastolic(mmHg)>,
    <http://purl.org/wot-catalogue/ble/gatt#BloodPressureMeasurementCompoundValue-MeanArterialPressure(mmHg)>,
    <http://purl.org/wot-catalogue/ble/gatt#BloodPressureMeasurementCompoundValue-Systolic(kPa)>,
    <http://purl.org/wot-catalogue/ble/gatt#BloodPressureMeasurementCompoundValue-Diastolic(kPa)>,
    <http://purl.org/wot-catalogue/ble/gatt#BloodPressureMeasurementCompoundValue-MeanArterialPressure(kPa)>,
    <http://purl.org/wot-catalogue/ble/gatt#TimeStamp>, <http://purl.org/wot-catalogue/ble/gatt#PulseRate>,
    <http://purl.org/wot-catalogue/ble/gatt#UserID>, <http://purl.org/wot-catalogue/ble/gatt#org.bluetooth.characteristic.cgm_session_run_time>,
    <http://purl.org/wot-catalogue/ble/gatt#1807>, <http://purl.org/wot-catalogue/ble/gatt#org.bluetooth.characteristic.cgm_specific_ops_control_point>,
    <http://purl.org/wot-catalogue/ble/gatt#1812>, <http://purl.org/wot-catalogue/ble/gatt#org.bluetooth.characteristic.cgm_status>,
    <http://purl.org/wot-catalogue/ble/gatt#org.bluetooth.characteristic.cross_trainer_data>,
    <http://purl.org/wot-catalogue/ble/gatt#org.bluetooth.characteristic.boot_keyboard_output_report>,
    <http://purl.org/wot-catalogue/ble/gatt#org.bluetooth.characteristic.csc_feature>,
    <http://purl.org/wot-catalogue/ble/gatt#org.bluetooth.characteristic.current_time>,
    <http://purl.org/wot-catalogue/ble/gatt#org.bluetooth.characteristic.cycling_power_control_point>,
    <http://purl.org/wot-catalogue/ble/gatt#org.bluetooth.characteristic.alert_notification_control_point>,
    <http://purl.org/wot-catalogue/ble/gatt#CommandID>, <http://purl.org/wot-catalogue/ble/gatt#181D>,
    <http://purl.org/wot-catalogue/ble/gatt#org.bluetooth.characteristic.cycling_power_feature>,
    <http://purl.org/wot-catalogue/ble/gatt#org.bluetooth.characteristic.cycling_power_measurement>,
    <http://purl.org/wot-catalogue/ble/gatt#org.bluetooth.characteristic.cycling_power_vector>,
    <http://purl.org/wot-catalogue/ble/gatt#Digital>, <http://purl.org/wot-catalogue/ble/gatt#org.bluetooth.characteristic.descriptor_value_changed>,
    <http://purl.org/wot-catalogue/ble/gatt#SequenceNumber>, <http://purl.org/wot-catalogue/ble/gatt#BaseTime>,
    <http://purl.org/wot-catalogue/ble/gatt#GlucoseConcentration-unitsofkg/L>, <http://purl.org/wot-catalogue/ble/gatt#GlucoseConcentration-unitsofmol/L>,
    <http://purl.org/wot-catalogue/ble/gatt#Type>, <http://purl.org/wot-catalogue/ble/gatt#SampleLocation>,
    <http://purl.org/wot-catalogue/ble/gatt#SensorStatusAnnunciation>, <http://purl.org/wot-catalogue/ble/gatt#1803>,
    <http://purl.org/wot-catalogue/ble/gatt#org.bluetooth.characteristic.alert_level>,
    <http://purl.org/wot-catalogue/ble/gatt#Level>, <http://purl.org/wot-catalogue/ble/gatt#ReportMapValue>,
    <http://purl.org/wot-catalogue/ble/gatt#org.bluetooth.characteristic.dew_point>, <http://purl.org/wot-catalogue/ble/gatt#MagneticDeclination>,
    <http://purl.org/wot-catalogue/ble/gatt#1802>, <http://purl.org/wot-catalogue/ble/gatt#181B>,
    <http://purl.org/wot-catalogue/ble/gatt#org.bluetooth.characteristic.body_composition_feature>,
    <http://purl.org/wot-catalogue/ble/gatt#org.bluetooth.characteristic.body_composition_measurement>,
    <http://purl.org/wot-catalogue/ble/gatt#MinimumHeartRate>, <http://purl.org/wot-catalogue/ble/gatt#MaximumHeartRate>,
    <http://purl.org/wot-catalogue/ble/gatt#181F>, <http://purl.org/wot-catalogue/ble/gatt#org.bluetooth.characteristic.cgm_measurement>,
    <http://purl.org/wot-catalogue/ble/gatt#org.bluetooth.characteristic.cgm_session_start_time>,
    <http://purl.org/wot-catalogue/ble/gatt#SessionStartTime>, <http://purl.org/wot-catalogue/ble/gatt#DST-Offset>,
    <http://purl.org/wot-catalogue/ble/gatt#BootKeyboardOutputReportValue>, <http://purl.org/wot-catalogue/ble/gatt#org.bluetooth.characteristic.database_change_increment>,
    <http://purl.org/wot-catalogue/ble/gatt#DatabaseChangeIncrement>, <http://purl.org/wot-catalogue/ble/gatt#org.bluetooth.characteristic.digital>,
    <http://purl.org/wot-catalogue/ble/gatt#RestingHeartRate>, <http://purl.org/wot-catalogue/ble/gatt#MinimumInclination>,
    <http://purl.org/wot-catalogue/ble/gatt#MaximumInclination>, <http://purl.org/wot-catalogue/ble/gatt#Source>,
    <http://purl.org/wot-catalogue/ble/gatt#Accuracy>, <http://purl.org/wot-catalogue/ble/gatt#DaysSinceUpdate>,
    <http://purl.org/wot-catalogue/ble/gatt#HoursSinceUpdate>, <http://purl.org/wot-catalogue/ble/gatt#PedalPowerBalance>,
    <http://purl.org/wot-catalogue/ble/gatt#AccumulatedTorque>, <http://purl.org/wot-catalogue/ble/gatt#WheelRevolutionData-CumulativeWheelRevolutions>,
    <http://purl.org/wot-catalogue/ble/gatt#WheelRevolutionData-LastWheelEventTime>, <http://purl.org/wot-catalogue/ble/gatt#ExtremeForceMagnitudes-MaximumForceMagnitude>,
    <http://purl.org/wot-catalogue/ble/gatt#ExtremeForceMagnitudes-MinimumForceMagnitude>,
    <http://purl.org/wot-catalogue/ble/gatt#ExtremeTorqueMagnitudes-MaximumTorqueMagnitude>,
    <http://purl.org/wot-catalogue/ble/gatt#ExtremeTorqueMagnitudes-MinimumTorqueMagnitude>,
    <http://purl.org/wot-catalogue/ble/gatt#ExtremeAngles-MaximumAngle>, <http://purl.org/wot-catalogue/ble/gatt#ExtremeAngles-MinimumAngle>,
    <http://purl.org/wot-catalogue/ble/gatt#TopDeadSpotAngle>, <http://purl.org/wot-catalogue/ble/gatt#BottomDeadSpotAngle>,
    <http://purl.org/wot-catalogue/ble/gatt#AccumulatedEnergy>, <http://purl.org/wot-catalogue/ble/gatt#TimeUpdateControlPoint>,
    <http://purl.org/wot-catalogue/ble/gatt#Latitude>, <http://purl.org/wot-catalogue/ble/gatt#SensorLocation>,
    <http://purl.org/wot-catalogue/ble/gatt#AlertLevel>, <http://purl.org/wot-catalogue/ble/gatt#BodyFatPercentage>,
    <http://purl.org/wot-catalogue/ble/gatt#BasalMetabolism>, <http://purl.org/wot-catalogue/ble/gatt#MusclePercentage>,
    <http://purl.org/wot-catalogue/ble/gatt#MuscleMass-Kilograms>, <http://purl.org/wot-catalogue/ble/gatt#MuscleMass-Pounds>,
    <http://purl.org/wot-catalogue/ble/gatt#FatFreeMass-Kilograms>, <http://purl.org/wot-catalogue/ble/gatt#FatFreeMass-Pounds>,
    <http://purl.org/wot-catalogue/ble/gatt#SoftLeanMass-Kilograms>, <http://purl.org/wot-catalogue/ble/gatt#SoftLeanMass-Pounds>,
    <http://purl.org/wot-catalogue/ble/gatt#BodyWaterMass-Kilograms>, <http://purl.org/wot-catalogue/ble/gatt#BodyWaterMass-Pounds>,
    <http://purl.org/wot-catalogue/ble/gatt#Impedance>, <http://purl.org/wot-catalogue/ble/gatt#Weight-Kilograms>,
    <http://purl.org/wot-catalogue/ble/gatt#Weight-Pounds>, <http://purl.org/wot-catalogue/ble/gatt#Height-Meters>,
    <http://purl.org/wot-catalogue/ble/gatt#Height-Inches>, <http://purl.org/wot-catalogue/ble/gatt#Weight-SI>,
    <http://purl.org/wot-catalogue/ble/gatt#Weight-Imperial>, <http://purl.org/wot-catalogue/ble/gatt#BMI>,
    <http://purl.org/wot-catalogue/ble/gatt#Height-SI>, <http://purl.org/wot-catalogue/ble/gatt#Height-Imperial>,
    <http://purl.org/wot-catalogue/ble/gatt#org.bluetooth.characteristic.elevation>, <http://purl.org/wot-catalogue/ble/gatt#Bearing>,
    <http://purl.org/wot-catalogue/ble/gatt#Heading>, <http://purl.org/wot-catalogue/ble/gatt#RemainingDistance>,
    <http://purl.org/wot-catalogue/ble/gatt#RemainingVerticalDistance>, <http://purl.org/wot-catalogue/ble/gatt#EstimatedTimeofArrival>,
    <http://purl.org/wot-catalogue/ble/gatt#org.bluetooth.characteristic.fat_burn_heart_rate_lower_limit>,
    <http://purl.org/wot-catalogue/ble/gatt#WaistCircumference>, <http://purl.org/wot-catalogue/ble/gatt#ObjectName>,
    <http://purl.org/wot-catalogue/ble/gatt#org.bluetooth.characteristic.Longitude>, <http://purl.org/wot-catalogue/ble/gatt#Longitude>,
    <http://purl.org/wot-catalogue/ble/gatt#181C>, <http://purl.org/wot-catalogue/ble/gatt#org.bluetooth.characteristic.email_address>,
    <http://purl.org/wot-catalogue/ble/gatt#org.bluetooth.characteristic.age>, <http://purl.org/wot-catalogue/ble/gatt#org.bluetooth.characteristic.date_of_birth>,
    <http://purl.org/wot-catalogue/ble/gatt#org.bluetooth.characteristic.firmware_revision_string>,
    <http://purl.org/wot-catalogue/ble/gatt#org.bluetooth.characteristic.first_name>,
    <http://purl.org/wot-catalogue/ble/gatt#org.bluetooth.characteristic.fitness_machine_control_point>,
    <http://purl.org/wot-catalogue/ble/gatt#org.bluetooth.characteristic.fitness_machine_feature>,
    <http://purl.org/wot-catalogue/ble/gatt#org.bluetooth.characteristic.fitness_machine_status>,
    <http://purl.org/wot-catalogue/ble/gatt#org.bluetooth.characteristic.anaerobic_threshold>,
    <http://purl.org/wot-catalogue/ble/gatt#org.bluetooth.characteristic.date_of_threshold_assessment>,
    <http://purl.org/wot-catalogue/ble/gatt#org.bluetooth.characteristic.fat_burn_heart_rate_upper_limit>,
    <http://purl.org/wot-catalogue/ble/gatt#org.bluetooth.characteristic.aerobic_heart_rate_upper_limit>,
    <http://purl.org/wot-catalogue/ble/gatt#org.bluetooth.characteristic.anaerobic_heart_rate_lower_limit>,
    <http://purl.org/wot-catalogue/ble/gatt#org.bluetooth.characteristic.five_zone_heart_rate_limits>,
    <http://purl.org/wot-catalogue/ble/gatt#org.bluetooth.characteristic.floor_number>,
    <http://purl.org/wot-catalogue/ble/gatt#org.bluetooth.characteristic.gender>, <http://purl.org/wot-catalogue/ble/gatt#LocalNorthCoordinate>,
    <http://purl.org/wot-catalogue/ble/gatt#180A>, <http://purl.org/wot-catalogue/ble/gatt#org.bluetooth.characteristic.glucose_feature>,
    <http://purl.org/wot-catalogue/ble/gatt#org.bluetooth.characteristic.glucose_measurement>,
    <http://purl.org/wot-catalogue/ble/gatt#org.bluetooth.characteristic.hardware_revision_string>,
    <http://purl.org/wot-catalogue/ble/gatt#org.bluetooth.characteristic.Magnetic_flux_density_2D>,
    <http://purl.org/wot-catalogue/ble/gatt#MagneticFluxDensity:X-Axis>, <http://purl.org/wot-catalogue/ble/gatt#MagneticFluxDensity:Y-Axis>,
    <http://purl.org/wot-catalogue/ble/gatt#org.bluetooth.characteristic.gust_factor>,
    <http://purl.org/wot-catalogue/ble/gatt#GustFactor>, <http://purl.org/wot-catalogue/ble/gatt#org.bluetooth.characteristic.heart_rate_control_point>,
    <http://purl.org/wot-catalogue/ble/gatt#Temperature>, <http://purl.org/wot-catalogue/ble/gatt#org.bluetooth.characteristic.heart_rate_max>,
    <http://purl.org/wot-catalogue/ble/gatt#HeatIndex>, <http://purl.org/wot-catalogue/ble/gatt#ExactTime256>,
    <http://purl.org/wot-catalogue/ble/gatt#AdjustReason>, <http://purl.org/wot-catalogue/ble/gatt#Floors>,
    <http://purl.org/wot-catalogue/ble/gatt#ObjectID>, <http://purl.org/wot-catalogue/ble/gatt#BodyCompositionFeature>,
    <http://purl.org/wot-catalogue/ble/gatt#org.bluetooth.characteristic.day_date_time>,
    <http://purl.org/wot-catalogue/ble/gatt#DateTime>, <http://purl.org/wot-catalogue/ble/gatt#DayofWeek>,
    <http://purl.org/wot-catalogue/ble/gatt#org.bluetooth.characteristic.date_time>, <http://purl.org/wot-catalogue/ble/gatt#Year>,
    <http://purl.org/wot-catalogue/ble/gatt#Month>, <http://purl.org/wot-catalogue/ble/gatt#Day>,
    <http://purl.org/wot-catalogue/ble/gatt#Hours>, <http://purl.org/wot-catalogue/ble/gatt#Minutes>,
    <http://purl.org/wot-catalogue/ble/gatt#Seconds>, <http://purl.org/wot-catalogue/ble/gatt#org.bluetooth.characteristic.heat_index>,
    <http://purl.org/wot-catalogue/ble/gatt#NumberofNewAlert>, <http://purl.org/wot-catalogue/ble/gatt#TextStringInformation>,
    <http://purl.org/wot-catalogue/ble/gatt#1819>, <http://purl.org/wot-catalogue/ble/gatt#org.bluetooth.characteristic.height>,
    <http://purl.org/wot-catalogue/ble/gatt#org.bluetooth.characteristic.hid_control_point>,
    <http://purl.org/wot-catalogue/ble/gatt#DaylightSavingTime>, <http://purl.org/wot-catalogue/ble/gatt#EmailAddress>,
    <http://purl.org/wot-catalogue/ble/gatt#MinimumResistanceLevel>, <http://purl.org/wot-catalogue/ble/gatt#MaximumResistanceLevel>,
    <http://purl.org/wot-catalogue/ble/gatt#1822>, <http://purl.org/wot-catalogue/ble/gatt#org.bluetooth.characteristic.hid_information>,
    <http://purl.org/wot-catalogue/ble/gatt#AerobicHeartRateUpperLimit>, <http://purl.org/wot-catalogue/ble/gatt#InstantaneousStrideLength>,
    <http://purl.org/wot-catalogue/ble/gatt#ScanRefreshValue>, <http://purl.org/wot-catalogue/ble/gatt#org.bluetooth.characteristic.apparent_wind_direction>,
    <http://purl.org/wot-catalogue/ble/gatt#ApparentWindDirection>, <http://purl.org/wot-catalogue/ble/gatt#UserIndex>,
    <http://purl.org/wot-catalogue/ble/gatt#org.bluetooth.characteristic.Magnetic_flux_density_3D>,
    <http://purl.org/wot-catalogue/ble/gatt#MagneticFluxDensity:Z-Axis>, <http://purl.org/wot-catalogue/ble/gatt#Weight>,
    <http://purl.org/wot-catalogue/ble/gatt#HeartRateMax>, <http://purl.org/wot-catalogue/ble/gatt#TemperatureTextDescription>,
    <http://purl.org/wot-catalogue/ble/gatt#RingerControlPoint>, <http://purl.org/wot-catalogue/ble/gatt#1808>,
    <http://purl.org/wot-catalogue/ble/gatt#org.bluetooth.characteristic.glucose_measurement_context>,
    <http://purl.org/wot-catalogue/ble/gatt#org.bluetooth.characteristic.hip_circumference>,
    <http://purl.org/wot-catalogue/ble/gatt#Unreadcount>, <http://purl.org/wot-catalogue/ble/gatt#Gender>,
    <http://purl.org/wot-catalogue/ble/gatt#1804>, <http://purl.org/wot-catalogue/ble/gatt#MaximumRecommendedHeartRate>,
    <http://purl.org/wot-catalogue/ble/gatt#CurrentState>, <http://purl.org/wot-catalogue/ble/gatt#Result>,
    <http://purl.org/wot-catalogue/ble/gatt#org.bluetooth.characteristic.http_control_point>,
    <http://purl.org/wot-catalogue/ble/gatt#PollenConcentration>, <http://purl.org/wot-catalogue/ble/gatt#HIDControlPointCommand>,
    <http://purl.org/wot-catalogue/ble/gatt#StepCount>, <http://purl.org/wot-catalogue/ble/gatt#1815>,
    <http://purl.org/wot-catalogue/ble/gatt#AnaerobicHeartRateLowerLimit>, <http://purl.org/wot-catalogue/ble/gatt#org.bluetooth.characteristic.body_sensor_location>,
    <http://purl.org/wot-catalogue/ble/gatt#BodySensorLocation>, <http://purl.org/wot-catalogue/ble/gatt#org.bluetooth.characteristic.http_entity_body>,
    <http://purl.org/wot-catalogue/ble/gatt#CategoryIDBitMask>, <http://purl.org/wot-catalogue/ble/gatt#ExtendedFlags>,
    <http://purl.org/wot-catalogue/ble/gatt#CarbohydrateID>, <http://purl.org/wot-catalogue/ble/gatt#Carbohydrate-unitsofkilograms>,
    <http://purl.org/wot-catalogue/ble/gatt#Meal>, <http://purl.org/wot-catalogue/ble/gatt#Tester>,
    <http://purl.org/wot-catalogue/ble/gatt#Health>, <http://purl.org/wot-catalogue/ble/gatt#ExerciseDuration>,
    <http://purl.org/wot-catalogue/ble/gatt#ExerciseIntensity>, <http://purl.org/wot-catalogue/ble/gatt#MedicationID>,
    <http://purl.org/wot-catalogue/ble/gatt#Medication-unitsofkilograms>, <http://purl.org/wot-catalogue/ble/gatt#Medication-unitsofliters>,
    <http://purl.org/wot-catalogue/ble/gatt#HbA1c>, <http://purl.org/wot-catalogue/ble/gatt#org.bluetooth.characteristic.csc_measurement>,
    <http://purl.org/wot-catalogue/ble/gatt#CumulativeWheelRevolutions>, <http://purl.org/wot-catalogue/ble/gatt#LastWheelEventTime>,
    <http://purl.org/wot-catalogue/ble/gatt#CumulativeCrankRevolutions>, <http://purl.org/wot-catalogue/ble/gatt#LastCrankEventTime>,
    <http://purl.org/wot-catalogue/ble/gatt#Height>, <http://purl.org/wot-catalogue/ble/gatt#org.bluetooth.characteristic.day_of_week>,
    <http://purl.org/wot-catalogue/ble/gatt#NumberofBeaconsinSolution>, <http://purl.org/wot-catalogue/ble/gatt#NumberofBeaconsinView>,
    <http://purl.org/wot-catalogue/ble/gatt#TimetoFirstFix>, <http://purl.org/wot-catalogue/ble/gatt#EHPE>,
    <http://purl.org/wot-catalogue/ble/gatt#EVPE>, <http://purl.org/wot-catalogue/ble/gatt#HDOP>,
    <http://purl.org/wot-catalogue/ble/gatt#VDOP>, <http://purl.org/wot-catalogue/ble/gatt#org.bluetooth.characteristic.http_headers>,
    <http://purl.org/wot-catalogue/ble/gatt#Humidity>, <http://purl.org/wot-catalogue/ble/gatt#1816>,
    <http://purl.org/wot-catalogue/ble/gatt#org.bluetooth.characteristic.http_status_code>,
    <http://purl.org/wot-catalogue/ble/gatt#org.bluetooth.characteristic.https_security>,
    <http://purl.org/wot-catalogue/ble/gatt#Pressure>, <http://purl.org/wot-catalogue/ble/gatt#HTTPSSecurity>,
    <http://purl.org/wot-catalogue/ble/gatt#1810>, <http://purl.org/wot-catalogue/ble/gatt#org.bluetooth.characteristic.blood_pressure_feature>,
    <http://purl.org/wot-catalogue/ble/gatt#ReportValue>, <http://purl.org/wot-catalogue/ble/gatt#TemperatureMeasurementValue(Celsius)>,
    <http://purl.org/wot-catalogue/ble/gatt#TemperatureMeasurementValue(Fahrenheit)>,
    <http://purl.org/wot-catalogue/ble/gatt#TemperatureType>, <http://purl.org/wot-catalogue/ble/gatt#ThreezoneHeartRateLimits-Light(Fatburn)/Moderate(Aerobic)Limit>,
    <http://purl.org/wot-catalogue/ble/gatt#ThreezoneHeartRateLimits-Moderate(Aerobic)/Hard(Anaerobic)Limit>,
    <http://purl.org/wot-catalogue/ble/gatt#org.bluetooth.characteristic.dst_offset>,
    <http://purl.org/wot-catalogue/ble/gatt#DSTOffset>, <http://purl.org/wot-catalogue/ble/gatt#180D>,
    <http://purl.org/wot-catalogue/ble/gatt#org.bluetooth.characteristic.heart_rate_measurement>,
    <http://purl.org/wot-catalogue/ble/gatt#bcdHID>, <http://purl.org/wot-catalogue/ble/gatt#bCountryCode>,
    <http://purl.org/wot-catalogue/ble/gatt#1801>, <http://purl.org/wot-catalogue/ble/gatt#181A>,
    <http://purl.org/wot-catalogue/ble/gatt#org.bluetooth.characteristic.humidity>, <http://purl.org/wot-catalogue/ble/gatt#org.bluetooth.characteristic.barometric_pressure_trend>,
    <http://purl.org/wot-catalogue/ble/gatt#HardwareRevision>, <http://purl.org/wot-catalogue/ble/gatt#ObjectType>,
    <http://purl.org/wot-catalogue/ble/gatt#WeightScaleFeature>, <http://purl.org/wot-catalogue/ble/gatt#MinimumPower>,
    <http://purl.org/wot-catalogue/ble/gatt#MaximumPower>, <http://purl.org/wot-catalogue/ble/gatt#ForceonBelt>,
    <http://purl.org/wot-catalogue/ble/gatt#PowerOutput>, <http://purl.org/wot-catalogue/ble/gatt#LocalEastCoordinate>,
    <http://purl.org/wot-catalogue/ble/gatt#StatusCode>, <http://purl.org/wot-catalogue/ble/gatt#DataStatus>,
    <http://purl.org/wot-catalogue/ble/gatt#Age>, <http://purl.org/wot-catalogue/ble/gatt#Location-Latitude>,
    <http://purl.org/wot-catalogue/ble/gatt#Location-Longitude>, <http://purl.org/wot-catalogue/ble/gatt#RollingTime>,
    <http://purl.org/wot-catalogue/ble/gatt#UTCTime>, <http://purl.org/wot-catalogue/ble/gatt#org.bluetooth.characteristic.alert_category_id_bit_mask>,
    <http://purl.org/wot-catalogue/ble/gatt#CategoryIDBitMask0>, <http://purl.org/wot-catalogue/ble/gatt#CategoryIDBitMask1>,
    <http://purl.org/wot-catalogue/ble/gatt#BloodPressureFeature>, <http://purl.org/wot-catalogue/ble/gatt#VendorIDSource>,
    <http://purl.org/wot-catalogue/ble/gatt#VendorID>, <http://purl.org/wot-catalogue/ble/gatt#ProductID>,
    <http://purl.org/wot-catalogue/ble/gatt#ProductVersion>, <http://purl.org/wot-catalogue/ble/gatt#AnaerobicThreshold>,
    <http://purl.org/wot-catalogue/ble/gatt#Uncertainty>, <http://purl.org/wot-catalogue/ble/gatt#ObjectLast-Modified>,
    <http://purl.org/wot-catalogue/ble/gatt#Size>, <http://purl.org/wot-catalogue/ble/gatt#CGMGlucoseConcentration>,
    <http://purl.org/wot-catalogue/ble/gatt#CGMTrendInformation>, <http://purl.org/wot-catalogue/ble/gatt#CGMQuality>,
    <http://purl.org/wot-catalogue/ble/gatt#1811>, <http://purl.org/wot-catalogue/ble/gatt#FatBurnHeartRateUpperLimit>,
    <http://purl.org/wot-catalogue/ble/gatt#IndoorPositioningConfiguration>, <http://purl.org/wot-catalogue/ble/gatt#SerialNumber>,
    <http://purl.org/wot-catalogue/ble/gatt#FloorNumber>, <http://purl.org/wot-catalogue/ble/gatt#HeartRateMeasurementValue(uint8)>,
    <http://purl.org/wot-catalogue/ble/gatt#HeartRateMeasurementValue(uint16)>, <http://purl.org/wot-catalogue/ble/gatt#EnergyExpended>,
    <http://purl.org/wot-catalogue/ble/gatt#RR-Interval>, <http://purl.org/wot-catalogue/ble/gatt#org.bluetooth.characteristic.exact_time_256>,
    <http://purl.org/wot-catalogue/ble/gatt#DayDateTime>, <http://purl.org/wot-catalogue/ble/gatt#Fractions256>,
    <http://purl.org/wot-catalogue/ble/gatt#BondManagementFeatures>, <http://purl.org/wot-catalogue/ble/gatt#BarometricPressureTrend>,
    <http://purl.org/wot-catalogue/ble/gatt#TrueWindDirection>, <http://purl.org/wot-catalogue/ble/gatt#WritewithoutResponse>,
    <http://purl.org/wot-catalogue/ble/gatt#ReadLong>, <http://purl.org/wot-catalogue/ble/gatt#DeviceInformationService>,
    <http://purl.org/wot-catalogue/ble/gatt#SystemID>, <http://purl.org/wot-catalogue/ble/gatt#IEEE11073-20601RegulatoryCertificationDataList>,
    <http://purl.org/wot-catalogue/ble/gatt#PnPID>, <http://purl.org/wot-catalogue/ble/gatt#BondManagementService>,
    <http://purl.org/wot-catalogue/ble/gatt#BondManagementControlPoint>, <http://purl.org/wot-catalogue/ble/gatt#BondManagementFeature>,
    <http://purl.org/wot-catalogue/ble/gatt#BatteryService>, <http://purl.org/wot-catalogue/ble/gatt#BatteryLevel>,
    <http://purl.org/wot-catalogue/ble/gatt#CurrentTimeService>, <http://purl.org/wot-catalogue/ble/gatt#CurrentTime>,
    <http://purl.org/wot-catalogue/ble/gatt#LocalTimeInformation>, <http://purl.org/wot-catalogue/ble/gatt#ReferenceTimeInformation>,
    <http://purl.org/wot-catalogue/ble/gatt#ScanParametersService>, <http://purl.org/wot-catalogue/ble/gatt#ScanIntervalWindow>,
    <http://purl.org/wot-catalogue/ble/gatt#ScanRefresh>, <http://purl.org/wot-catalogue/ble/gatt#UserDataService>,
    <http://purl.org/wot-catalogue/ble/gatt#UDSCharacteristic>, <http://purl.org/wot-catalogue/ble/gatt#UserControlPoint>,
    <http://purl.org/wot-catalogue/ble/gatt#RecordAccessControlPoint>, <http://purl.org/wot-catalogue/ble/gatt#SCControlPoint>,
    <http://purl.org/wot-catalogue/ble/gatt#ImmediateAlertService>, <http://purl.org/wot-catalogue/ble/gatt#VendorIDSourceField>,
    <http://purl.org/wot-catalogue/ble/gatt#VendorIDField>, <http://purl.org/wot-catalogue/ble/gatt#ProductIDField>,
    <http://purl.org/wot-catalogue/ble/gatt#ProductVersionField>, <http://purl.org/wot-catalogue/ble/gatt#BluetoothSIG>,
    <http://purl.org/wot-catalogue/ble/gatt#USBImplementerForum>, <http://purl.org/wot-catalogue/ble/gatt#Serverrequiresrefresh>,
    <http://purl.org/wot-catalogue/ble/gatt#UDSCharacteristicValue>, <http://purl.org/wot-catalogue/ble/gatt#DatabaseChangeIncrementValue>,
    <http://purl.org/wot-catalogue/ble/gatt#TimeStampField>, <http://purl.org/wot-catalogue/ble/gatt#UserIDField>,
    <http://purl.org/wot-catalogue/ble/gatt#InstantaneousPowerField>, <http://purl.org/wot-catalogue/ble/gatt#InstantaneousSpeedField>,
    <http://purl.org/wot-catalogue/ble/gatt#org.bluetooth.characteristic.indoor_bike_data>,
    <http://purl.org/wot-catalogue/ble/gatt#org.bluetooth.characteristic.indoor_positioning_configuration>,
    <http://purl.org/wot-catalogue/ble/gatt#org.bluetooth.characteristic.intermediate_cuff_pressure>,
    <http://purl.org/wot-catalogue/ble/gatt#org.bluetooth.characteristic.intermediate_temperature>,
    <http://purl.org/wot-catalogue/ble/gatt#org.bluetooth.characteristic.irradiance>,
    <http://purl.org/wot-catalogue/ble/gatt#org.bluetooth.characteristic.language>, <http://purl.org/wot-catalogue/ble/gatt#org.bluetooth.characteristic.last_name>,
    <http://purl.org/wot-catalogue/ble/gatt#org.bluetooth.characteristic.latitude>, <http://purl.org/wot-catalogue/ble/gatt#org.bluetooth.characteristic.ln_control_point>,
    <http://purl.org/wot-catalogue/ble/gatt#org.bluetooth.characteristic.ln_feature>,
    <http://purl.org/wot-catalogue/ble/gatt#org.bluetooth.characteristic.local_east_coordinate>,
    <http://purl.org/wot-catalogue/ble/gatt#org.bluetooth.characteristic.local_north_coordinate>,
    <http://purl.org/wot-catalogue/ble/gatt#org.bluetooth.characteristic.local_time_information>,
    <http://purl.org/wot-catalogue/ble/gatt#org.bluetooth.characteristic.location_and_speed>,
    <http://purl.org/wot-catalogue/ble/gatt#org.bluetooth.characteristic.location_name>,
    <http://purl.org/wot-catalogue/ble/gatt#org.bluetooth.characteristic.magnetic_declination>,
    <http://purl.org/wot-catalogue/ble/gatt#org.bluetooth.characteristic.manufacturer_name_string>,
    <http://purl.org/wot-catalogue/ble/gatt#org.bluetooth.characteristic.maximum_recommended_heart_rate>,
    <http://purl.org/wot-catalogue/ble/gatt#org.bluetooth.characteristic.measurement_interval>,
    <http://purl.org/wot-catalogue/ble/gatt#org.bluetooth.characteristic.model_number_string>,
    <http://purl.org/wot-catalogue/ble/gatt#org.bluetooth.characteristic.navigation>,
    <http://purl.org/wot-catalogue/ble/gatt#org.bluetooth.characteristic.new_alert>, <http://purl.org/wot-catalogue/ble/gatt#org.bluetooth.characteristic.object_action_control_point>,
    <http://purl.org/wot-catalogue/ble/gatt#org.bluetooth.characteristic.object_changed>,
    <http://purl.org/wot-catalogue/ble/gatt#org.bluetooth.characteristic.object_first_created>,
    <http://purl.org/wot-catalogue/ble/gatt#org.bluetooth.characteristic.object_id>, <http://purl.org/wot-catalogue/ble/gatt#org.bluetooth.characteristic.object_last_modified>,
    <http://purl.org/wot-catalogue/ble/gatt#org.bluetooth.characteristic.object_list_control_point>,
    <http://purl.org/wot-catalogue/ble/gatt#org.bluetooth.characteristic.object_list_filter>,
    <http://purl.org/wot-catalogue/ble/gatt#org.bluetooth.characteristic.object_name>,
    <http://purl.org/wot-catalogue/ble/gatt#org.bluetooth.characteristic.object_properties>,
    <http://purl.org/wot-catalogue/ble/gatt#org.bluetooth.characteristic.object_size>,
    <http://purl.org/wot-catalogue/ble/gatt#org.bluetooth.characteristic.object_type>,
    <http://purl.org/wot-catalogue/ble/gatt#org.bluetooth.characteristic.ots_feature>,
    <http://purl.org/wot-catalogue/ble/gatt#org.bluetooth.characteristic.plx_continuous_measurement>,
    <http://purl.org/wot-catalogue/ble/gatt#org.bluetooth.characteristic.plx_features>,
    <http://purl.org/wot-catalogue/ble/gatt#org.bluetooth.characteristic.plx_spot_check_measurement>,
    <http://purl.org/wot-catalogue/ble/gatt#org.bluetooth.characteristic.pnp_id>, <http://purl.org/wot-catalogue/ble/gatt#org.bluetooth.characteristic.pollen_concentration>,
    <http://purl.org/wot-catalogue/ble/gatt#org.bluetooth.characteristic.position_quality>,
    <http://purl.org/wot-catalogue/ble/gatt#org.bluetooth.characteristic.pressure>, <http://purl.org/wot-catalogue/ble/gatt#org.bluetooth.characteristic.protocol_mode>,
    <http://purl.org/wot-catalogue/ble/gatt#org.bluetooth.characteristic.rainfall>, <http://purl.org/wot-catalogue/ble/gatt#org.bluetooth.characteristic.record_access_control_point>,
    <http://purl.org/wot-catalogue/ble/gatt#org.bluetooth.characteristic.reference_time_information>,
    <http://purl.org/wot-catalogue/ble/gatt#org.bluetooth.characteristic.report>, <http://purl.org/wot-catalogue/ble/gatt#org.bluetooth.characteristic.report_map>,
    <http://purl.org/wot-catalogue/ble/gatt#org.bluetooth.characteristic.resolvable_private_address_only>,
    <http://purl.org/wot-catalogue/ble/gatt#org.bluetooth.characteristic.resting_heart_rate>,
    <http://purl.org/wot-catalogue/ble/gatt#org.bluetooth.characteristic.ringer_control_point>,
    <http://purl.org/wot-catalogue/ble/gatt#org.bluetooth.characteristic.ringer_setting>,
    <http://purl.org/wot-catalogue/ble/gatt#org.bluetooth.characteristic.rower_data>,
    <http://purl.org/wot-catalogue/ble/gatt#org.bluetooth.characteristic.rsc_feature>,
    <http://purl.org/wot-catalogue/ble/gatt#org.bluetooth.characteristic.rsc_measurement>,
    <http://purl.org/wot-catalogue/ble/gatt#org.bluetooth.characteristic.sc_control_point>,
    <http://purl.org/wot-catalogue/ble/gatt#org.bluetooth.characteristic.scan_interval_window>,
    <http://purl.org/wot-catalogue/ble/gatt#org.bluetooth.characteristic.scan_refresh>,
    <http://purl.org/wot-catalogue/ble/gatt#org.bluetooth.characteristic.sensor_location>,
    <http://purl.org/wot-catalogue/ble/gatt#org.bluetooth.characteristic.serial_number_string>,
    <http://purl.org/wot-catalogue/ble/gatt#org.bluetooth.characteristic.software_revision_string>,
    <http://purl.org/wot-catalogue/ble/gatt#org.bluetooth.characteristic.sport_type_for_aerobic_and_anaerobic_thresholds>,
    <http://purl.org/wot-catalogue/ble/gatt#org.bluetooth.characteristic.stair_climber_data>,
    <http://purl.org/wot-catalogue/ble/gatt#org.bluetooth.characteristic.step_climber_data>,
    <http://purl.org/wot-catalogue/ble/gatt#org.bluetooth.characteristic.supported_heart_rate_range>,
    <http://purl.org/wot-catalogue/ble/gatt#org.bluetooth.characteristic.supported_inclination_range>,
    <http://purl.org/wot-catalogue/ble/gatt#org.bluetooth.characteristic.supported_new_alert_category>,
    <http://purl.org/wot-catalogue/ble/gatt#org.bluetooth.characteristic.supported_power_range>,
    <http://purl.org/wot-catalogue/ble/gatt#org.bluetooth.characteristic.supported_resistance_level_range>,
    <http://purl.org/wot-catalogue/ble/gatt#org.bluetooth.characteristic.supported_speed_range>,
    <http://purl.org/wot-catalogue/ble/gatt#org.bluetooth.characteristic.supported_unread_alert_category>,
    <http://purl.org/wot-catalogue/ble/gatt#org.bluetooth.characteristic.system_id>, <http://purl.org/wot-catalogue/ble/gatt#org.bluetooth.characteristic.tds_control_point>,
    <http://purl.org/wot-catalogue/ble/gatt#org.bluetooth.characteristic.temperature>,
    <http://purl.org/wot-catalogue/ble/gatt#org.bluetooth.characteristic.temperature_measurement>,
    <http://purl.org/wot-catalogue/ble/gatt#org.bluetooth.characteristic.temperature_type>,
    <http://purl.org/wot-catalogue/ble/gatt#org.bluetooth.characteristic.three_zone_heart_rate_limits>,
    <http://purl.org/wot-catalogue/ble/gatt#org.bluetooth.characteristic.time_accuracy>,
    <http://purl.org/wot-catalogue/ble/gatt#org.bluetooth.characteristic.time_source>,
    <http://purl.org/wot-catalogue/ble/gatt#org.bluetooth.characteristic.time_update_control_point>,
    <http://purl.org/wot-catalogue/ble/gatt#org.bluetooth.characteristic.time_update_state>,
    <http://purl.org/wot-catalogue/ble/gatt#org.bluetooth.characteristic.time_with_dst>,
    <http://purl.org/wot-catalogue/ble/gatt#org.bluetooth.characteristic.time_zone>, <http://purl.org/wot-catalogue/ble/gatt#org.bluetooth.characteristic.training_status>,
    <http://purl.org/wot-catalogue/ble/gatt#org.bluetooth.characteristic.treadmill_data>,
    <http://purl.org/wot-catalogue/ble/gatt#org.bluetooth.characteristic.true_wind_direction>,
    <http://purl.org/wot-catalogue/ble/gatt#org.bluetooth.characteristic.true_wind_speed>,
    <http://purl.org/wot-catalogue/ble/gatt#org.bluetooth.characteristic.two_zone_heart_rate_limit>,
    <http://purl.org/wot-catalogue/ble/gatt#org.bluetooth.characteristic.tx_power_level>,
    <http://purl.org/wot-catalogue/ble/gatt#org.bluetooth.characteristic.uncertainty>,
    <http://purl.org/wot-catalogue/ble/gatt#org.bluetooth.characteristic.unread_alert_status>,
    <http://purl.org/wot-catalogue/ble/gatt#org.bluetooth.characteristic.uri>, <http://purl.org/wot-catalogue/ble/gatt#org.bluetooth.characteristic.user_control_point>,
    <http://purl.org/wot-catalogue/ble/gatt#org.bluetooth.characteristic.user_index>,
    <http://purl.org/wot-catalogue/ble/gatt#org.bluetooth.characteristic.uv_index>, <http://purl.org/wot-catalogue/ble/gatt#org.bluetooth.characteristic.vo2_max>,
    <http://purl.org/wot-catalogue/ble/gatt#org.bluetooth.characteristic.waist_circumference>,
    <http://purl.org/wot-catalogue/ble/gatt#org.bluetooth.characteristic.weight>, <http://purl.org/wot-catalogue/ble/gatt#org.bluetooth.characteristic.weight_measurement>,
    <http://purl.org/wot-catalogue/ble/gatt#org.bluetooth.characteristic.weight_scale_feature>,
    <http://purl.org/wot-catalogue/ble/gatt#org.bluetooth.characteristic.wind_chill> .

<http://purl.org/wot-catalogue/ble/gatt#org.bluetooth.characteristic.ln_feature> a
    skos:Concept, ontolex:LexicalConcept, prov:Entity;
  skos:altLabel "ln feature";
  skos:broader ble:Characteristic;
  skos:definition """The LN Feature characteristic is used to report a list
    of features supported by the device.""";
  skos:inScheme ble:Scheme;
  skos:prefLabel "LN Feature";
  skos:related ble:LNFeature, ble:Read;
  prov:wasDerivedFrom <file:/data/lp/etl/executor/data/1651932367716-22-f5b1c2e0-1947-4a2e-a814-6ce401f2a604/working/working-outputfiles-33/gatt-xml-master/org.bluetooth.characteristic.ln_feature.xml> .

<http://purl.org/wot-catalogue/ble/gatt#LNFeature> a skos:Concept, ontolex:LexicalConcept,
    prov:Entity;
  skos:altLabel "ln feature";
  skos:broader ble:Value;
  skos:inScheme ble:Scheme;
  skos:prefLabel "LN Feature";
  prov:wasDerivedFrom <file:/data/lp/etl/executor/data/1651932367716-22-f5b1c2e0-1947-4a2e-a814-6ce401f2a604/working/working-outputfiles-33/gatt-xml-master/org.bluetooth.characteristic.ln_feature.xml> .

<http://purl.org/wot-catalogue/ble/gatt#org.bluetooth.characteristic.intermediate_temperature>
  a skos:Concept, ontolex:LexicalConcept, prov:Entity;
  skos:altLabel "intermediate temperature";
  skos:broader ble:Characteristic;
  skos:definition """The Intermediate Temperature characteristic has the
    same format as the Temperature Measurement characteristic.
    However, due to a different context, the Value field is
    referred to as the Intermediate Temperature Value
    field.""";
  skos:inScheme ble:Scheme;
  skos:prefLabel "Intermediate Temperature";
  skos:related ble:IntermediateTemperature, ble:Notify;
  prov:wasDerivedFrom <file:/data/lp/etl/executor/data/1651932367716-22-f5b1c2e0-1947-4a2e-a814-6ce401f2a604/working/working-outputfiles-33/gatt-xml-master/org.bluetooth.characteristic.intermediate_temperature.xml> .

<http://purl.org/wot-catalogue/ble/gatt#IntermediateTemperature> a skos:Concept, ontolex:LexicalConcept,
    prov:Entity;
  skos:altLabel "intermediate temperature";
  skos:broader ble:Value;
  skos:inScheme ble:Scheme;
  skos:prefLabel "Intermediate Temperature";
  prov:wasDerivedFrom <file:/data/lp/etl/executor/data/1651932367716-22-f5b1c2e0-1947-4a2e-a814-6ce401f2a604/working/working-outputfiles-33/gatt-xml-master/org.bluetooth.characteristic.intermediate_temperature.xml> .

<http://purl.org/wot-catalogue/ble/gatt#org.bluetooth.characteristic.true_wind_speed>
  a skos:Concept, ontolex:LexicalConcept, prov:Entity;
  skos:altLabel "true wind speed";
  skos:broader ble:Characteristic;
  skos:inScheme ble:Scheme;
  skos:prefLabel "True Wind Speed";
  skos:related ble:ExtendedProperties, ble:Notify, ble:Read, ble:TrueWindSpeed, ble:WritableAuxiliaries;
  prov:wasDerivedFrom <file:/data/lp/etl/executor/data/1651932367716-22-f5b1c2e0-1947-4a2e-a814-6ce401f2a604/working/working-outputfiles-33/gatt-xml-master/org.bluetooth.characteristic.true_wind_speed.xml> .

<http://purl.org/wot-catalogue/ble/gatt#TrueWindSpeed> a skos:Concept, ontolex:LexicalConcept,
    prov:Entity;
  skos:altLabel "true wind speed";
  skos:broader ble:Value;
  skos:definition """Unit is in meters per second with a
      resolution of 0.01 m/s""";
  skos:inScheme ble:Scheme;
  skos:prefLabel "True Wind Speed";
  prov:wasDerivedFrom <file:/data/lp/etl/executor/data/1651932367716-22-f5b1c2e0-1947-4a2e-a814-6ce401f2a604/working/working-outputfiles-33/gatt-xml-master/org.bluetooth.characteristic.true_wind_speed.xml> .

<http://purl.org/wot-catalogue/ble/gatt#1823> a skos:Concept, ontolex:LexicalConcept,
    prov:Entity;
  skos:altLabel "http proxy";
  skos:broader ble:Service;
  skos:definition """The HTTP Proxy Service (HPS) allows a device to expose
    HTTP Web Services to a client. This enables an HPS client
    device to program a set of characteristics that configures a
    Hyper Text Transfer Protocol (HTTP) request, initiate this,
    request, and then read the response.""";
  skos:inScheme ble:Scheme;
  skos:prefLabel "HTTP Proxy";
  skos:related ble:org.bluetooth.characteristic.http_control_point, ble:org.bluetooth.characteristic.http_entity_body,
    ble:org.bluetooth.characteristic.http_headers, ble:org.bluetooth.characteristic.http_status_code,
    ble:org.bluetooth.characteristic.https_security, ble:org.bluetooth.characteristic.uri;
  prov:wasDerivedFrom <file:/data/lp/etl/executor/data/1651932367716-22-f5b1c2e0-1947-4a2e-a814-6ce401f2a604/working/working-outputfiles-33/gatt-xml-master/org.bluetooth.service.http_proxy.xml> .

<http://purl.org/wot-catalogue/ble/gatt#org.bluetooth.characteristic.uri> a skos:Concept,
    ontolex:LexicalConcept, prov:Entity;
  skos:altLabel "uri";
  skos:broader ble:Characteristic;
  skos:definition """The Uniform Resource Identifier (URI) Characteristic
    is used to configure the URI for a subsequent
    request.""";
  skos:inScheme ble:Scheme;
  skos:prefLabel "URI";
  skos:related ble:URI, ble:Write;
  prov:wasDerivedFrom <file:/data/lp/etl/executor/data/1651932367716-22-f5b1c2e0-1947-4a2e-a814-6ce401f2a604/working/working-outputfiles-33/gatt-xml-master/org.bluetooth.characteristic.uri.xml> .

<http://purl.org/wot-catalogue/ble/gatt#org.bluetooth.characteristic.http_headers>
  a skos:Concept, ontolex:LexicalConcept, prov:Entity;
  skos:altLabel "http headers";
  skos:broader ble:Characteristic;
  skos:definition """The HTTP Headers Characteristic is used to hold the
    headers that would be sent to the HTTP Request or the headers
    contained within an HTTP response message from the HTTP
    Server.""";
  skos:inScheme ble:Scheme;
  skos:prefLabel "HTTP Headers";
  skos:related ble:HTTPHeaders, ble:Read, ble:Write;
  prov:wasDerivedFrom <file:/data/lp/etl/executor/data/1651932367716-22-f5b1c2e0-1947-4a2e-a814-6ce401f2a604/working/working-outputfiles-33/gatt-xml-master/org.bluetooth.characteristic.http_headers.xml> .

<http://purl.org/wot-catalogue/ble/gatt#org.bluetooth.characteristic.http_entity_body>
  a skos:Concept, ontolex:LexicalConcept, prov:Entity;
  skos:altLabel "http entity body";
  skos:broader ble:Characteristic;
  skos:definition """The HTTP Entity Body Characteristic contains the
    contents of the message body after any Transfer Encoding has
    been applied.""";
  skos:inScheme ble:Scheme;
  skos:prefLabel "HTTP Entity Body";
  skos:related ble:HTTPEntityBody, ble:Read, ble:Write;
  prov:wasDerivedFrom <file:/data/lp/etl/executor/data/1651932367716-22-f5b1c2e0-1947-4a2e-a814-6ce401f2a604/working/working-outputfiles-33/gatt-xml-master/org.bluetooth.characteristic.http_entity_body.xml> .

<http://purl.org/wot-catalogue/ble/gatt#org.bluetooth.characteristic.http_control_point>
  a skos:Concept, ontolex:LexicalConcept, prov:Entity;
  skos:altLabel "http control point";
  skos:broader ble:Characteristic;
  skos:definition """The HTTP Control Point is used to initiate a request
    to send an HTTP request message from the device contgaining the
    HTTP Proxy Service, acting as an HTTP Client, and an HTTP
    Server.""";
  skos:inScheme ble:Scheme;
  skos:prefLabel "HTTP Control Point";
  skos:related ble:OpCode, ble:Write;
  prov:wasDerivedFrom <file:/data/lp/etl/executor/data/1651932367716-22-f5b1c2e0-1947-4a2e-a814-6ce401f2a604/working/working-outputfiles-33/gatt-xml-master/org.bluetooth.characteristic.http_control_point.xml> .

<http://purl.org/wot-catalogue/ble/gatt#org.bluetooth.characteristic.http_status_code>
  a skos:Concept, ontolex:LexicalConcept, prov:Entity;
  skos:altLabel "http status code";
  skos:broader ble:Characteristic;
  skos:definition """The HTTP Status Code characteristic contains the
    Status-Code from the Status-Line of the first line of the HTTP
    Response Message, followed by one octet indicating the Data
    Status Bit Field indicating the status of the data
    received.""";
  skos:inScheme ble:Scheme;
  skos:prefLabel "HTTP Status Code";
  skos:related ble:DataStatus, ble:Notify, ble:StatusCode;
  prov:wasDerivedFrom <file:/data/lp/etl/executor/data/1651932367716-22-f5b1c2e0-1947-4a2e-a814-6ce401f2a604/working/working-outputfiles-33/gatt-xml-master/org.bluetooth.characteristic.http_status_code.xml> .

<http://purl.org/wot-catalogue/ble/gatt#org.bluetooth.characteristic.https_security>
  a skos:Concept, ontolex:LexicalConcept, prov:Entity;
  skos:altLabel "https security";
  skos:broader ble:Characteristic;
  skos:definition """The HTTPS Security characteristic contains the known
    authenticity of the HTTPS Server certificate for the
    URI.""";
  skos:inScheme ble:Scheme;
  skos:prefLabel "HTTPS Security";
  skos:related ble:HTTPSSecurity, ble:Read;
  prov:wasDerivedFrom <file:/data/lp/etl/executor/data/1651932367716-22-f5b1c2e0-1947-4a2e-a814-6ce401f2a604/working/working-outputfiles-33/gatt-xml-master/org.bluetooth.characteristic.https_security.xml> .

<http://purl.org/wot-catalogue/ble/gatt#Write> a skos:Concept;
  skos:altLabel "write";
  skos:definition "A Characteristic Value is writen to a server when the client knows the Characteristic Value Handle";
  skos:inScheme ble:Scheme;
  skos:prefLabel "Write" .

<http://purl.org/wot-catalogue/ble/gatt#Read> a skos:Concept;
  skos:altLabel "read";
  skos:definition "A Characteristic Value is read from a server when the client knows the Characteristic Value Handle";
  skos:inScheme ble:Scheme;
  skos:prefLabel "Read" .

<http://purl.org/wot-catalogue/ble/gatt#Notify> a skos:Concept;
  skos:altLabel "notify";
  skos:definition "A server is configured to notify a Characteristic Value to a client without expecting any Attribute Protocol layer acknowledgment that the notification was successfully received";
  skos:inScheme ble:Scheme;
  skos:prefLabel "Notify" .

<http://purl.org/wot-catalogue/ble/gatt#180F> a skos:Concept, ontolex:LexicalConcept,
    prov:Entity;
  skos:altLabel "battery service";
  skos:broader ble:Service;
  skos:definition """The Battery Service exposes the Battery State and
    Battery Level of a single battery or set of batteries in a
    device.""";
  skos:inScheme ble:Scheme;
  skos:prefLabel "Battery Service";
  skos:related ble:org.bluetooth.characteristic.battery_level;
  prov:wasDerivedFrom <file:/data/lp/etl/executor/data/1651932367716-22-f5b1c2e0-1947-4a2e-a814-6ce401f2a604/working/working-outputfiles-33/gatt-xml-master/org.bluetooth.service.battery_service.xml> .

<http://purl.org/wot-catalogue/ble/gatt#org.bluetooth.characteristic.battery_level>
  a skos:Concept, ontolex:LexicalConcept, prov:Entity;
  skos:altLabel "battery level";
  skos:broader ble:Characteristic;
  skos:definition """The current charge level of a battery. 100%
    represents fully charged while 0% represents fully
    discharged.""";
  skos:inScheme ble:Scheme;
  skos:prefLabel "Battery Level";
  skos:related ble:Level, ble:Notify, ble:Read;
  prov:wasDerivedFrom <file:/data/lp/etl/executor/data/1651932367716-22-f5b1c2e0-1947-4a2e-a814-6ce401f2a604/working/working-outputfiles-33/gatt-xml-master/org.bluetooth.characteristic.battery_level.xml> .

<http://purl.org/wot-catalogue/ble/gatt#org.bluetooth.characteristic.record_access_control_point>
  a skos:Concept, ontolex:LexicalConcept, prov:Entity;
  skos:altLabel "record access control point";
  skos:broader ble:Characteristic;
  skos:definition """This control point is used with a service to provide
    basic management functionality for the Glucose Sensor patient
    record database. This enables functions including counting
    records, transmitting records and clearing records based on
    filter criterion. The filter criterion in the Operand field is
    defined by the service that references this characteristic as
    is the format of a record (which may be comprised of one or
    more characteristics) and the sequence of transferred
    records.""";
  skos:inScheme ble:Scheme;
  skos:prefLabel "Record Access Control Point";
  skos:related ble:Indicate, ble:InformationText, ble:OpCode, ble:Operand, ble:Operator,
    ble:Write;
  prov:wasDerivedFrom <file:/data/lp/etl/executor/data/1651932367716-22-f5b1c2e0-1947-4a2e-a814-6ce401f2a604/working/working-outputfiles-33/gatt-xml-master/org.bluetooth.characteristic.record_access_control_point.xml> .

<http://purl.org/wot-catalogue/ble/gatt#OpCode> a skos:Concept, ontolex:LexicalConcept,
    prov:Entity;
  skos:altLabel "op code";
  skos:broader ble:Value;
  skos:inScheme ble:Scheme;
  skos:prefLabel "Op Code";
  prov:wasDerivedFrom <file:/data/lp/etl/executor/data/1651932367716-22-f5b1c2e0-1947-4a2e-a814-6ce401f2a604/working/working-outputfiles-33/gatt-xml-master/org.bluetooth.characteristic.bond_management_control_point.xml>,
    <file:/data/lp/etl/executor/data/1651932367716-22-f5b1c2e0-1947-4a2e-a814-6ce401f2a604/working/working-outputfiles-33/gatt-xml-master/org.bluetooth.characteristic.cgm_specific_ops_control_point.xml>,
    <file:/data/lp/etl/executor/data/1651932367716-22-f5b1c2e0-1947-4a2e-a814-6ce401f2a604/working/working-outputfiles-33/gatt-xml-master/org.bluetooth.characteristic.http_control_point.xml>,
    <file:/data/lp/etl/executor/data/1651932367716-22-f5b1c2e0-1947-4a2e-a814-6ce401f2a604/working/working-outputfiles-33/gatt-xml-master/org.bluetooth.characteristic.record_access_control_point.xml>,
    <file:/data/lp/etl/executor/data/1651932367716-22-f5b1c2e0-1947-4a2e-a814-6ce401f2a604/working/working-outputfiles-33/gatt-xml-master/org.bluetooth.characteristic.sc_control_point.xml> .

<http://purl.org/wot-catalogue/ble/gatt#Operator> a skos:Concept, ontolex:LexicalConcept,
    prov:Entity;
  skos:altLabel "operator";
  skos:broader ble:Value;
  skos:inScheme ble:Scheme;
  skos:prefLabel "Operator";
  prov:wasDerivedFrom <file:/data/lp/etl/executor/data/1651932367716-22-f5b1c2e0-1947-4a2e-a814-6ce401f2a604/working/working-outputfiles-33/gatt-xml-master/org.bluetooth.characteristic.record_access_control_point.xml> .

<http://purl.org/wot-catalogue/ble/gatt#Operand> a skos:Concept, ontolex:LexicalConcept,
    prov:Entity;
  skos:altLabel "operand";
  skos:broader ble:Value;
  skos:definition "Octet Order - LSO-MSO", """The operands correspond to the Op Code
      values (Keys 0 to 255) defined in the Op Code Field
      above""",
    "Value defined per Service";
  skos:inScheme ble:Scheme;
  skos:prefLabel "Operand";
  prov:wasDerivedFrom <file:/data/lp/etl/executor/data/1651932367716-22-f5b1c2e0-1947-4a2e-a814-6ce401f2a604/working/working-outputfiles-33/gatt-xml-master/org.bluetooth.characteristic.bond_management_control_point.xml>,
    <file:/data/lp/etl/executor/data/1651932367716-22-f5b1c2e0-1947-4a2e-a814-6ce401f2a604/working/working-outputfiles-33/gatt-xml-master/org.bluetooth.characteristic.cgm_specific_ops_control_point.xml>,
    <file:/data/lp/etl/executor/data/1651932367716-22-f5b1c2e0-1947-4a2e-a814-6ce401f2a604/working/working-outputfiles-33/gatt-xml-master/org.bluetooth.characteristic.record_access_control_point.xml> .

<http://purl.org/wot-catalogue/ble/gatt#org.bluetooth.characteristic.system_id> a
    skos:Concept, ontolex:LexicalConcept, prov:Entity;
  skos:altLabel "system id";
  skos:broader ble:Characteristic;
  skos:definition """The SYSTEM ID characteristic consists of a structure with
      two fields. The first field are the LSOs and the second field
      contains the MSOs. This is a 64-bit structure which consists
      of a 40-bit manufacturer-defined identifier concatenated with
      a 24 bit unique Organizationally Unique Identifier (OUI). The
      OUI is issued by the IEEE Registration Authority
      (http://standards.ieee.org/regauth/index.html) and is
      required to be used in accordance with IEEE Standard
      802-2001.6 while the least significant 40 bits are
      manufacturer defined.If System ID generated based on a Bluetooth Device
      Address, it is required to be done as follows. System ID and
      the Bluetooth Device Address have a very similar structure: a
      Bluetooth Device Address is 48 bits in length and consists of
      a 24 bit Company Assigned Identifier (manufacturer defined
      identifier) concatenated with a 24 bit Company Identifier
      (OUI). In order to encapsulate a Bluetooth Device Address as
      System ID, the Company Identifier is concatenated with 0xFFFE
      followed by the Company Assigned Identifier of the Bluetooth
      Address. For more guidelines related to EUI-64, refer to
      http://standards.ieee.org/develop/regauth/tut/eui64.pdf.""";
  skos:inScheme ble:Scheme;
  skos:prefLabel "System ID";
  skos:related ble:ManufacturerIdentifier, ble:OrganizationallyUniqueIdentifier, ble:Read;
  prov:wasDerivedFrom <file:/data/lp/etl/executor/data/1651932367716-22-f5b1c2e0-1947-4a2e-a814-6ce401f2a604/working/working-outputfiles-33/gatt-xml-master/org.bluetooth.characteristic.system_id.xml> .

<http://purl.org/wot-catalogue/ble/gatt#ManufacturerIdentifier> a skos:Concept, ontolex:LexicalConcept,
    prov:Entity;
  skos:altLabel "manufacturer identifier";
  skos:broader ble:Value;
  skos:definition "The System ID characteristic shall represent a structure containing a manufacturer-defined identifier following an Organizationally Unique Identifier (OUI) and is unique for each individual instance of the product.";
  skos:inScheme ble:Scheme;
  skos:prefLabel "Manufacturer Identifier";
  skos:related xsd:unsignedInt;
  prov:wasDerivedFrom <file:/data/lp/etl/executor/data/1651932367716-22-f5b1c2e0-1947-4a2e-a814-6ce401f2a604/working/working-outputfiles-33/gatt-xml-master/org.bluetooth.characteristic.system_id.xml> .

<http://purl.org/wot-catalogue/ble/gatt#OrganizationallyUniqueIdentifier> a skos:Concept,
    ontolex:LexicalConcept, prov:Entity;
  skos:altLabel "organizationally unique identifier";
  skos:broader ble:Value;
  skos:definition "The System ID characteristic shall represent a structure containing an Organizationally Unique Identifier (OUI)  is unique for each individual instance of the product.";
  skos:inScheme ble:Scheme;
  skos:prefLabel "Organizationally Unique Identifier";
  skos:related xsd:unsignedInt;
  prov:wasDerivedFrom <file:/data/lp/etl/executor/data/1651932367716-22-f5b1c2e0-1947-4a2e-a814-6ce401f2a604/working/working-outputfiles-33/gatt-xml-master/org.bluetooth.characteristic.system_id.xml> .

<http://purl.org/wot-catalogue/ble/gatt#org.bluetooth.characteristic.elevation> a
    skos:Concept, ontolex:LexicalConcept, prov:Entity;
  skos:altLabel "elevation";
  skos:broader ble:Characteristic;
  skos:inScheme ble:Scheme;
  skos:prefLabel "Elevation";
  skos:related ble:Elevation, ble:ExtendedProperties, ble:Notify, ble:Read, ble:WritableAuxiliaries;
  prov:wasDerivedFrom <file:/data/lp/etl/executor/data/1651932367716-22-f5b1c2e0-1947-4a2e-a814-6ce401f2a604/working/working-outputfiles-33/gatt-xml-master/org.bluetooth.characteristic.elevation.xml> .

<http://purl.org/wot-catalogue/ble/gatt#Elevation> a skos:Concept, ontolex:LexicalConcept,
    prov:Entity;
  skos:altLabel "elevation";
  skos:broader ble:Value;
  skos:definition """Unit is in meters with a resolution of
      1/100""", """Unit is in meters with a resolution of 0.01
      m""";
  skos:inScheme ble:Scheme;
  skos:prefLabel "Elevation";
  prov:wasDerivedFrom <file:/data/lp/etl/executor/data/1651932367716-22-f5b1c2e0-1947-4a2e-a814-6ce401f2a604/working/working-outputfiles-33/gatt-xml-master/org.bluetooth.characteristic.elevation.xml>,
    <file:/data/lp/etl/executor/data/1651932367716-22-f5b1c2e0-1947-4a2e-a814-6ce401f2a604/working/working-outputfiles-33/gatt-xml-master/org.bluetooth.characteristic.location_and_speed.xml> .

<http://purl.org/wot-catalogue/ble/gatt#org.bluetooth.characteristic.object_first_created>
  a skos:Concept, ontolex:LexicalConcept, prov:Entity;
  skos:altLabel "object first-created";
  skos:broader ble:Characteristic;
  skos:inScheme ble:Scheme;
  skos:prefLabel "Object First-Created";
  skos:related ble:ObjectFirst-Created, ble:Read, ble:Write;
  prov:wasDerivedFrom <file:/data/lp/etl/executor/data/1651932367716-22-f5b1c2e0-1947-4a2e-a814-6ce401f2a604/working/working-outputfiles-33/gatt-xml-master/org.bluetooth.characteristic.object_first_created.xml> .

<http://purl.org/wot-catalogue/ble/gatt#ObjectFirst-Created> a skos:Concept, ontolex:LexicalConcept,
    prov:Entity;
  skos:altLabel "object first-created";
  skos:broader ble:Value;
  skos:inScheme ble:Scheme;
  skos:prefLabel "Object First-Created";
  prov:wasDerivedFrom <file:/data/lp/etl/executor/data/1651932367716-22-f5b1c2e0-1947-4a2e-a814-6ce401f2a604/working/working-outputfiles-33/gatt-xml-master/org.bluetooth.characteristic.object_first_created.xml> .

<http://purl.org/wot-catalogue/ble/gatt#org.bluetooth.characteristic.rsc_feature>
  a skos:Concept, ontolex:LexicalConcept, prov:Entity;
  skos:altLabel "rsc feature";
  skos:broader ble:Characteristic;
  skos:definition """The RSC (Running Speed and Cadence) Feature
    characteristic is used to describe the supported features of
    the Server.""";
  skos:inScheme ble:Scheme;
  skos:prefLabel "RSC Feature";
  skos:related ble:RSCFeature, ble:Read;
  prov:wasDerivedFrom <file:/data/lp/etl/executor/data/1651932367716-22-f5b1c2e0-1947-4a2e-a814-6ce401f2a604/working/working-outputfiles-33/gatt-xml-master/org.bluetooth.characteristic.rsc_feature.xml> .

<http://purl.org/wot-catalogue/ble/gatt#RSCFeature> a skos:Concept, ontolex:LexicalConcept,
    prov:Entity;
  skos:altLabel "rsc feature";
  skos:broader ble:Value;
  skos:inScheme ble:Scheme;
  skos:prefLabel "RSC Feature";
  prov:wasDerivedFrom <file:/data/lp/etl/executor/data/1651932367716-22-f5b1c2e0-1947-4a2e-a814-6ce401f2a604/working/working-outputfiles-33/gatt-xml-master/org.bluetooth.characteristic.rsc_feature.xml> .

<http://purl.org/wot-catalogue/ble/gatt#org.bluetooth.characteristic.vo2_max> a skos:Concept,
    ontolex:LexicalConcept, prov:Entity;
  skos:altLabel "vo2 max";
  skos:broader ble:Characteristic;
  skos:definition "Maximal Oxygen uptake of a user";
  skos:inScheme ble:Scheme;
  skos:prefLabel "VO2 Max";
  skos:related ble:Read, ble:VO2Max, ble:Write;
  prov:wasDerivedFrom <file:/data/lp/etl/executor/data/1651932367716-22-f5b1c2e0-1947-4a2e-a814-6ce401f2a604/working/working-outputfiles-33/gatt-xml-master/org.bluetooth.characteristic.vo2_max.xml> .

<http://purl.org/wot-catalogue/ble/gatt#VO2Max> a skos:Concept, ontolex:LexicalConcept,
    prov:Entity;
  skos:altLabel "vo2 max";
  skos:broader ble:Value;
  skos:definition """Unit is in Milliliter per kilogram per
      minutes with a resolution of 1 .""";
  skos:inScheme ble:Scheme;
  skos:prefLabel "VO2 Max";
  prov:wasDerivedFrom <file:/data/lp/etl/executor/data/1651932367716-22-f5b1c2e0-1947-4a2e-a814-6ce401f2a604/working/working-outputfiles-33/gatt-xml-master/org.bluetooth.characteristic.vo2_max.xml> .

<http://purl.org/wot-catalogue/ble/gatt#org.bluetooth.characteristic.anaerobic_heart_rate_upper_limit>
  a skos:Concept, ontolex:LexicalConcept, prov:Entity;
  skos:altLabel "anaerobic heart rate upper limit";
  skos:broader ble:Characteristic;
  skos:definition """Upper limit of the heart rate where the user enhances
    his anaerobic tolerance while exercising.""";
  skos:inScheme ble:Scheme;
  skos:prefLabel "Anaerobic Heart Rate Upper Limit";
  skos:related ble:AnaerobicHeartRateUpperLimit, ble:Read, ble:Write;
  prov:wasDerivedFrom <file:/data/lp/etl/executor/data/1651932367716-22-f5b1c2e0-1947-4a2e-a814-6ce401f2a604/working/working-outputfiles-33/gatt-xml-master/org.bluetooth.characteristic.anaerobic_heart_rate_upper_limit.xml> .

<http://purl.org/wot-catalogue/ble/gatt#AnaerobicHeartRateUpperLimit> a skos:Concept,
    ontolex:LexicalConcept, prov:Entity;
  skos:altLabel "anaerobic heart rate upper limit";
  skos:broader ble:Value;
  skos:definition """Unit is in beats per minute with a
      resolution of 1""";
  skos:inScheme ble:Scheme;
  skos:prefLabel "Anaerobic Heart Rate Upper Limit";
  prov:wasDerivedFrom <file:/data/lp/etl/executor/data/1651932367716-22-f5b1c2e0-1947-4a2e-a814-6ce401f2a604/working/working-outputfiles-33/gatt-xml-master/org.bluetooth.characteristic.anaerobic_heart_rate_upper_limit.xml> .

<http://purl.org/wot-catalogue/ble/gatt#org.bluetooth.characteristic.irradiance> a
    skos:Concept, ontolex:LexicalConcept, prov:Entity;
  skos:altLabel "irradiance";
  skos:broader ble:Characteristic;
  skos:inScheme ble:Scheme;
  skos:prefLabel "Irradiance";
  skos:related ble:ExtendedProperties, ble:Irradiance, ble:Notify, ble:Read, ble:WritableAuxiliaries;
  prov:wasDerivedFrom <file:/data/lp/etl/executor/data/1651932367716-22-f5b1c2e0-1947-4a2e-a814-6ce401f2a604/working/working-outputfiles-33/gatt-xml-master/org.bluetooth.characteristic.irradiance.xml> .

<http://purl.org/wot-catalogue/ble/gatt#Irradiance> a skos:Concept, ontolex:LexicalConcept,
    prov:Entity;
  skos:altLabel "irradiance";
  skos:broader ble:Value;
  skos:definition """Unit is in watt per square meter with a
      resolution of 0.1 W/m^2""";
  skos:inScheme ble:Scheme;
  skos:prefLabel "Irradiance";
  prov:wasDerivedFrom <file:/data/lp/etl/executor/data/1651932367716-22-f5b1c2e0-1947-4a2e-a814-6ce401f2a604/working/working-outputfiles-33/gatt-xml-master/org.bluetooth.characteristic.irradiance.xml> .

<http://purl.org/wot-catalogue/ble/gatt#org.bluetooth.characteristic.cross_trainer_data>
  a skos:Concept, ontolex:LexicalConcept, prov:Entity;
  skos:altLabel "cross trainer data";
  skos:broader ble:Characteristic;
  skos:definition """The Cross Trainer Data characteristic is used to send
    training-related data to the Client from a cross trainer
    (Server).""";
  skos:inScheme ble:Scheme;
  skos:prefLabel "Cross Trainer Data";
  skos:related ble:AveragePower, ble:AverageSpeed, ble:AverageStepRate, ble:ElapsedTime,
    ble:EnergyPerHour, ble:EnergyPerMinute, ble:Flags, ble:HeartRate, ble:Inclination,
    ble:InstantaneousPower, ble:InstantaneousSpeed, ble:MetabolicEquivalent, ble:NegativeElevationGain,
    ble:Notify, ble:PositiveElevationGain, ble:RampAngleSetting, ble:RemainingTime, ble:ResistanceLevel,
    ble:StepPerMinute, ble:StrideCount, ble:TotalDistance, ble:TotalEnergy;
  prov:wasDerivedFrom <file:/data/lp/etl/executor/data/1651932367716-22-f5b1c2e0-1947-4a2e-a814-6ce401f2a604/working/working-outputfiles-33/gatt-xml-master/org.bluetooth.characteristic.cross_trainer_data.xml> .

<http://purl.org/wot-catalogue/ble/gatt#Flags> a skos:Concept, ontolex:LexicalConcept,
    prov:Entity;
  skos:altLabel "flags";
  skos:broader ble:Value;
  skos:definition """These flags define which data fields are
      present in the Characteristic value""",
    """These flags define which data fields are
      present in the Characteristic value.""";
  skos:inScheme ble:Scheme;
  skos:prefLabel "Flags";
  prov:wasDerivedFrom <file:/data/lp/etl/executor/data/1651932367716-22-f5b1c2e0-1947-4a2e-a814-6ce401f2a604/working/working-outputfiles-33/gatt-xml-master/org.bluetooth.characteristic.blood_pressure_measurement.xml>,
    <file:/data/lp/etl/executor/data/1651932367716-22-f5b1c2e0-1947-4a2e-a814-6ce401f2a604/working/working-outputfiles-33/gatt-xml-master/org.bluetooth.characteristic.body_composition_measurement.xml>,
    <file:/data/lp/etl/executor/data/1651932367716-22-f5b1c2e0-1947-4a2e-a814-6ce401f2a604/working/working-outputfiles-33/gatt-xml-master/org.bluetooth.characteristic.cgm_measurement.xml>,
    <file:/data/lp/etl/executor/data/1651932367716-22-f5b1c2e0-1947-4a2e-a814-6ce401f2a604/working/working-outputfiles-33/gatt-xml-master/org.bluetooth.characteristic.cross_trainer_data.xml>,
    <file:/data/lp/etl/executor/data/1651932367716-22-f5b1c2e0-1947-4a2e-a814-6ce401f2a604/working/working-outputfiles-33/gatt-xml-master/org.bluetooth.characteristic.csc_measurement.xml>,
    <file:/data/lp/etl/executor/data/1651932367716-22-f5b1c2e0-1947-4a2e-a814-6ce401f2a604/working/working-outputfiles-33/gatt-xml-master/org.bluetooth.characteristic.cycling_power_measurement.xml>,
    <file:/data/lp/etl/executor/data/1651932367716-22-f5b1c2e0-1947-4a2e-a814-6ce401f2a604/working/working-outputfiles-33/gatt-xml-master/org.bluetooth.characteristic.cycling_power_vector.xml>,
    <file:/data/lp/etl/executor/data/1651932367716-22-f5b1c2e0-1947-4a2e-a814-6ce401f2a604/working/working-outputfiles-33/gatt-xml-master/org.bluetooth.characteristic.glucose_measurement.xml>,
    <file:/data/lp/etl/executor/data/1651932367716-22-f5b1c2e0-1947-4a2e-a814-6ce401f2a604/working/working-outputfiles-33/gatt-xml-master/org.bluetooth.characteristic.glucose_measurement_context.xml>,
    <file:/data/lp/etl/executor/data/1651932367716-22-f5b1c2e0-1947-4a2e-a814-6ce401f2a604/working/working-outputfiles-33/gatt-xml-master/org.bluetooth.characteristic.heart_rate_measurement.xml>,
    <file:/data/lp/etl/executor/data/1651932367716-22-f5b1c2e0-1947-4a2e-a814-6ce401f2a604/working/working-outputfiles-33/gatt-xml-master/org.bluetooth.characteristic.hid_information.xml>,
    <file:/data/lp/etl/executor/data/1651932367716-22-f5b1c2e0-1947-4a2e-a814-6ce401f2a604/working/working-outputfiles-33/gatt-xml-master/org.bluetooth.characteristic.indoor_bike_data.xml>,
    <file:/data/lp/etl/executor/data/1651932367716-22-f5b1c2e0-1947-4a2e-a814-6ce401f2a604/working/working-outputfiles-33/gatt-xml-master/org.bluetooth.characteristic.location_and_speed.xml>,
    <file:/data/lp/etl/executor/data/1651932367716-22-f5b1c2e0-1947-4a2e-a814-6ce401f2a604/working/working-outputfiles-33/gatt-xml-master/org.bluetooth.characteristic.navigation.xml>,
    <file:/data/lp/etl/executor/data/1651932367716-22-f5b1c2e0-1947-4a2e-a814-6ce401f2a604/working/working-outputfiles-33/gatt-xml-master/org.bluetooth.characteristic.plx_continuous_measurement.xml>,
    <file:/data/lp/etl/executor/data/1651932367716-22-f5b1c2e0-1947-4a2e-a814-6ce401f2a604/working/working-outputfiles-33/gatt-xml-master/org.bluetooth.characteristic.plx_spot_check_measurement.xml>,
    <file:/data/lp/etl/executor/data/1651932367716-22-f5b1c2e0-1947-4a2e-a814-6ce401f2a604/working/working-outputfiles-33/gatt-xml-master/org.bluetooth.characteristic.position_quality.xml>,
    <file:/data/lp/etl/executor/data/1651932367716-22-f5b1c2e0-1947-4a2e-a814-6ce401f2a604/working/working-outputfiles-33/gatt-xml-master/org.bluetooth.characteristic.rower_data.xml>,
    <file:/data/lp/etl/executor/data/1651932367716-22-f5b1c2e0-1947-4a2e-a814-6ce401f2a604/working/working-outputfiles-33/gatt-xml-master/org.bluetooth.characteristic.rsc_measurement.xml>,
    <file:/data/lp/etl/executor/data/1651932367716-22-f5b1c2e0-1947-4a2e-a814-6ce401f2a604/working/working-outputfiles-33/gatt-xml-master/org.bluetooth.characteristic.stair_climber_data.xml>,
    <file:/data/lp/etl/executor/data/1651932367716-22-f5b1c2e0-1947-4a2e-a814-6ce401f2a604/working/working-outputfiles-33/gatt-xml-master/org.bluetooth.characteristic.step_climber_data.xml>,
    <file:/data/lp/etl/executor/data/1651932367716-22-f5b1c2e0-1947-4a2e-a814-6ce401f2a604/working/working-outputfiles-33/gatt-xml-master/org.bluetooth.characteristic.temperature_measurement.xml>,
    <file:/data/lp/etl/executor/data/1651932367716-22-f5b1c2e0-1947-4a2e-a814-6ce401f2a604/working/working-outputfiles-33/gatt-xml-master/org.bluetooth.characteristic.treadmill_data.xml>,
    <file:/data/lp/etl/executor/data/1651932367716-22-f5b1c2e0-1947-4a2e-a814-6ce401f2a604/working/working-outputfiles-33/gatt-xml-master/org.bluetooth.characteristic.weight_measurement.xml> .

<http://purl.org/wot-catalogue/ble/gatt#InstantaneousSpeed> a skos:Concept, ontolex:LexicalConcept,
    prov:Entity;
  skos:altLabel "instantaneous speed";
  skos:broader ble:Value;
  skos:definition """Kilometer per hour with a resolution of
      0.01""", """Unit is in m/s with a resolution of 1/256
      s""",
    """Unit is in meters per second with a
      resolution of 1/100""";
  skos:inScheme ble:Scheme;
  skos:prefLabel "Instantaneous Speed";
  prov:wasDerivedFrom <file:/data/lp/etl/executor/data/1651932367716-22-f5b1c2e0-1947-4a2e-a814-6ce401f2a604/working/working-outputfiles-33/gatt-xml-master/org.bluetooth.characteristic.cross_trainer_data.xml>,
    <file:/data/lp/etl/executor/data/1651932367716-22-f5b1c2e0-1947-4a2e-a814-6ce401f2a604/working/working-outputfiles-33/gatt-xml-master/org.bluetooth.characteristic.indoor_bike_data.xml>,
    <file:/data/lp/etl/executor/data/1651932367716-22-f5b1c2e0-1947-4a2e-a814-6ce401f2a604/working/working-outputfiles-33/gatt-xml-master/org.bluetooth.characteristic.location_and_speed.xml>,
    <file:/data/lp/etl/executor/data/1651932367716-22-f5b1c2e0-1947-4a2e-a814-6ce401f2a604/working/working-outputfiles-33/gatt-xml-master/org.bluetooth.characteristic.rsc_measurement.xml>,
    <file:/data/lp/etl/executor/data/1651932367716-22-f5b1c2e0-1947-4a2e-a814-6ce401f2a604/working/working-outputfiles-33/gatt-xml-master/org.bluetooth.characteristic.treadmill_data.xml> .

<http://purl.org/wot-catalogue/ble/gatt#AverageSpeed> a skos:Concept, ontolex:LexicalConcept,
    prov:Entity;
  skos:altLabel "average speed";
  skos:broader ble:Value;
  skos:definition """Kilometer per hour with a resolution of
      0.01""";
  skos:inScheme ble:Scheme;
  skos:prefLabel "Average Speed";
  prov:wasDerivedFrom <file:/data/lp/etl/executor/data/1651932367716-22-f5b1c2e0-1947-4a2e-a814-6ce401f2a604/working/working-outputfiles-33/gatt-xml-master/org.bluetooth.characteristic.cross_trainer_data.xml>,
    <file:/data/lp/etl/executor/data/1651932367716-22-f5b1c2e0-1947-4a2e-a814-6ce401f2a604/working/working-outputfiles-33/gatt-xml-master/org.bluetooth.characteristic.indoor_bike_data.xml>,
    <file:/data/lp/etl/executor/data/1651932367716-22-f5b1c2e0-1947-4a2e-a814-6ce401f2a604/working/working-outputfiles-33/gatt-xml-master/org.bluetooth.characteristic.treadmill_data.xml> .

<http://purl.org/wot-catalogue/ble/gatt#TotalDistance> a skos:Concept, ontolex:LexicalConcept,
    prov:Entity;
  skos:altLabel "total distance";
  skos:broader ble:Value;
  skos:definition """C2: Field exists if the key of bit 1 of the Flags field
        is set to 1.- Unit is in meter with a resolution of 1/10 m (or
        decimeter).""",
    """Meters with a resolution of
      1""", """Unit is in meters with a resolution of
      1/10""";
  skos:inScheme ble:Scheme;
  skos:prefLabel "Total Distance";
  prov:wasDerivedFrom <file:/data/lp/etl/executor/data/1651932367716-22-f5b1c2e0-1947-4a2e-a814-6ce401f2a604/working/working-outputfiles-33/gatt-xml-master/org.bluetooth.characteristic.cross_trainer_data.xml>,
    <file:/data/lp/etl/executor/data/1651932367716-22-f5b1c2e0-1947-4a2e-a814-6ce401f2a604/working/working-outputfiles-33/gatt-xml-master/org.bluetooth.characteristic.indoor_bike_data.xml>,
    <file:/data/lp/etl/executor/data/1651932367716-22-f5b1c2e0-1947-4a2e-a814-6ce401f2a604/working/working-outputfiles-33/gatt-xml-master/org.bluetooth.characteristic.location_and_speed.xml>,
    <file:/data/lp/etl/executor/data/1651932367716-22-f5b1c2e0-1947-4a2e-a814-6ce401f2a604/working/working-outputfiles-33/gatt-xml-master/org.bluetooth.characteristic.rower_data.xml>,
    <file:/data/lp/etl/executor/data/1651932367716-22-f5b1c2e0-1947-4a2e-a814-6ce401f2a604/working/working-outputfiles-33/gatt-xml-master/org.bluetooth.characteristic.rsc_measurement.xml>,
    <file:/data/lp/etl/executor/data/1651932367716-22-f5b1c2e0-1947-4a2e-a814-6ce401f2a604/working/working-outputfiles-33/gatt-xml-master/org.bluetooth.characteristic.treadmill_data.xml> .

<http://purl.org/wot-catalogue/ble/gatt#StepPerMinute> a skos:Concept, ontolex:LexicalConcept,
    prov:Entity;
  skos:altLabel "step per minute";
  skos:broader ble:Value;
  skos:definition """Step/minute with a resolution of
      1""";
  skos:inScheme ble:Scheme;
  skos:prefLabel "Step Per Minute";
  prov:wasDerivedFrom <file:/data/lp/etl/executor/data/1651932367716-22-f5b1c2e0-1947-4a2e-a814-6ce401f2a604/working/working-outputfiles-33/gatt-xml-master/org.bluetooth.characteristic.cross_trainer_data.xml>,
    <file:/data/lp/etl/executor/data/1651932367716-22-f5b1c2e0-1947-4a2e-a814-6ce401f2a604/working/working-outputfiles-33/gatt-xml-master/org.bluetooth.characteristic.stair_climber_data.xml>,
    <file:/data/lp/etl/executor/data/1651932367716-22-f5b1c2e0-1947-4a2e-a814-6ce401f2a604/working/working-outputfiles-33/gatt-xml-master/org.bluetooth.characteristic.step_climber_data.xml> .

<http://purl.org/wot-catalogue/ble/gatt#AverageStepRate> a skos:Concept, ontolex:LexicalConcept,
    prov:Entity;
  skos:altLabel "average step rate";
  skos:broader ble:Value;
  skos:definition """Step/minute with a resolution of
      1""";
  skos:inScheme ble:Scheme;
  skos:prefLabel "Average Step Rate";
  prov:wasDerivedFrom <file:/data/lp/etl/executor/data/1651932367716-22-f5b1c2e0-1947-4a2e-a814-6ce401f2a604/working/working-outputfiles-33/gatt-xml-master/org.bluetooth.characteristic.cross_trainer_data.xml>,
    <file:/data/lp/etl/executor/data/1651932367716-22-f5b1c2e0-1947-4a2e-a814-6ce401f2a604/working/working-outputfiles-33/gatt-xml-master/org.bluetooth.characteristic.stair_climber_data.xml>,
    <file:/data/lp/etl/executor/data/1651932367716-22-f5b1c2e0-1947-4a2e-a814-6ce401f2a604/working/working-outputfiles-33/gatt-xml-master/org.bluetooth.characteristic.step_climber_data.xml> .

<http://purl.org/wot-catalogue/ble/gatt#StrideCount> a skos:Concept, ontolex:LexicalConcept,
    prov:Entity;
  skos:altLabel "stride count";
  skos:broader ble:Value;
  skos:definition """Unitless with a resolution of
      0.1""", """Unitless with a resolution of
      1""";
  skos:inScheme ble:Scheme;
  skos:prefLabel "Stride Count";
  prov:wasDerivedFrom <file:/data/lp/etl/executor/data/1651932367716-22-f5b1c2e0-1947-4a2e-a814-6ce401f2a604/working/working-outputfiles-33/gatt-xml-master/org.bluetooth.characteristic.cross_trainer_data.xml>,
    <file:/data/lp/etl/executor/data/1651932367716-22-f5b1c2e0-1947-4a2e-a814-6ce401f2a604/working/working-outputfiles-33/gatt-xml-master/org.bluetooth.characteristic.stair_climber_data.xml> .

<http://purl.org/wot-catalogue/ble/gatt#PositiveElevationGain> a skos:Concept, ontolex:LexicalConcept,
    prov:Entity;
  skos:altLabel "positive elevation gain";
  skos:broader ble:Value;
  skos:definition """Meters with a resolution of
      0.1""", """Meters with a resolution of
      1""";
  skos:inScheme ble:Scheme;
  skos:prefLabel "Positive Elevation Gain";
  prov:wasDerivedFrom <file:/data/lp/etl/executor/data/1651932367716-22-f5b1c2e0-1947-4a2e-a814-6ce401f2a604/working/working-outputfiles-33/gatt-xml-master/org.bluetooth.characteristic.cross_trainer_data.xml>,
    <file:/data/lp/etl/executor/data/1651932367716-22-f5b1c2e0-1947-4a2e-a814-6ce401f2a604/working/working-outputfiles-33/gatt-xml-master/org.bluetooth.characteristic.stair_climber_data.xml>,
    <file:/data/lp/etl/executor/data/1651932367716-22-f5b1c2e0-1947-4a2e-a814-6ce401f2a604/working/working-outputfiles-33/gatt-xml-master/org.bluetooth.characteristic.step_climber_data.xml>,
    <file:/data/lp/etl/executor/data/1651932367716-22-f5b1c2e0-1947-4a2e-a814-6ce401f2a604/working/working-outputfiles-33/gatt-xml-master/org.bluetooth.characteristic.treadmill_data.xml> .

<http://purl.org/wot-catalogue/ble/gatt#NegativeElevationGain> a skos:Concept, ontolex:LexicalConcept,
    prov:Entity;
  skos:altLabel "negative elevation gain";
  skos:broader ble:Value;
  skos:definition """Meters with a resolution of
      0.1""", """Meters with a resolution of
      1""";
  skos:inScheme ble:Scheme;
  skos:prefLabel "Negative Elevation Gain";
  prov:wasDerivedFrom <file:/data/lp/etl/executor/data/1651932367716-22-f5b1c2e0-1947-4a2e-a814-6ce401f2a604/working/working-outputfiles-33/gatt-xml-master/org.bluetooth.characteristic.cross_trainer_data.xml>,
    <file:/data/lp/etl/executor/data/1651932367716-22-f5b1c2e0-1947-4a2e-a814-6ce401f2a604/working/working-outputfiles-33/gatt-xml-master/org.bluetooth.characteristic.treadmill_data.xml> .

<http://purl.org/wot-catalogue/ble/gatt#Inclination> a skos:Concept, ontolex:LexicalConcept,
    prov:Entity;
  skos:altLabel "inclination";
  skos:broader ble:Value;
  skos:definition """Percent with a resolution of
      0.1""";
  skos:inScheme ble:Scheme;
  skos:prefLabel "Inclination";
  prov:wasDerivedFrom <file:/data/lp/etl/executor/data/1651932367716-22-f5b1c2e0-1947-4a2e-a814-6ce401f2a604/working/working-outputfiles-33/gatt-xml-master/org.bluetooth.characteristic.cross_trainer_data.xml>,
    <file:/data/lp/etl/executor/data/1651932367716-22-f5b1c2e0-1947-4a2e-a814-6ce401f2a604/working/working-outputfiles-33/gatt-xml-master/org.bluetooth.characteristic.treadmill_data.xml> .

<http://purl.org/wot-catalogue/ble/gatt#RampAngleSetting> a skos:Concept, ontolex:LexicalConcept,
    prov:Entity;
  skos:altLabel "ramp angle setting";
  skos:broader ble:Value;
  skos:definition """Degree with a resolution of
      0.1""";
  skos:inScheme ble:Scheme;
  skos:prefLabel "Ramp Angle Setting";
  prov:wasDerivedFrom <file:/data/lp/etl/executor/data/1651932367716-22-f5b1c2e0-1947-4a2e-a814-6ce401f2a604/working/working-outputfiles-33/gatt-xml-master/org.bluetooth.characteristic.cross_trainer_data.xml>,
    <file:/data/lp/etl/executor/data/1651932367716-22-f5b1c2e0-1947-4a2e-a814-6ce401f2a604/working/working-outputfiles-33/gatt-xml-master/org.bluetooth.characteristic.treadmill_data.xml> .

<http://purl.org/wot-catalogue/ble/gatt#ResistanceLevel> a skos:Concept, ontolex:LexicalConcept,
    prov:Entity;
  skos:altLabel "resistance level";
  skos:broader ble:Value;
  skos:definition """Unitless with a resolution of
      0.1""", """Unitless with a resolution of
      1""";
  skos:inScheme ble:Scheme;
  skos:prefLabel "Resistance Level";
  prov:wasDerivedFrom <file:/data/lp/etl/executor/data/1651932367716-22-f5b1c2e0-1947-4a2e-a814-6ce401f2a604/working/working-outputfiles-33/gatt-xml-master/org.bluetooth.characteristic.cross_trainer_data.xml>,
    <file:/data/lp/etl/executor/data/1651932367716-22-f5b1c2e0-1947-4a2e-a814-6ce401f2a604/working/working-outputfiles-33/gatt-xml-master/org.bluetooth.characteristic.indoor_bike_data.xml>,
    <file:/data/lp/etl/executor/data/1651932367716-22-f5b1c2e0-1947-4a2e-a814-6ce401f2a604/working/working-outputfiles-33/gatt-xml-master/org.bluetooth.characteristic.rower_data.xml> .

<http://purl.org/wot-catalogue/ble/gatt#InstantaneousPower> a skos:Concept, ontolex:LexicalConcept,
    prov:Entity;
  skos:altLabel "instantaneous power";
  skos:broader ble:Value;
  skos:definition """Unit is in watts with a resolution of
      1.""", """Watts with a resolution of
      1""";
  skos:inScheme ble:Scheme;
  skos:prefLabel "Instantaneous Power";
  prov:wasDerivedFrom <file:/data/lp/etl/executor/data/1651932367716-22-f5b1c2e0-1947-4a2e-a814-6ce401f2a604/working/working-outputfiles-33/gatt-xml-master/org.bluetooth.characteristic.cross_trainer_data.xml>,
    <file:/data/lp/etl/executor/data/1651932367716-22-f5b1c2e0-1947-4a2e-a814-6ce401f2a604/working/working-outputfiles-33/gatt-xml-master/org.bluetooth.characteristic.cycling_power_measurement.xml>,
    <file:/data/lp/etl/executor/data/1651932367716-22-f5b1c2e0-1947-4a2e-a814-6ce401f2a604/working/working-outputfiles-33/gatt-xml-master/org.bluetooth.characteristic.indoor_bike_data.xml>,
    <file:/data/lp/etl/executor/data/1651932367716-22-f5b1c2e0-1947-4a2e-a814-6ce401f2a604/working/working-outputfiles-33/gatt-xml-master/org.bluetooth.characteristic.rower_data.xml> .

<http://purl.org/wot-catalogue/ble/gatt#AveragePower> a skos:Concept, ontolex:LexicalConcept,
    prov:Entity;
  skos:altLabel "average power";
  skos:broader ble:Value;
  skos:definition """Watts with a resolution of
      1""";
  skos:inScheme ble:Scheme;
  skos:prefLabel "Average Power";
  prov:wasDerivedFrom <file:/data/lp/etl/executor/data/1651932367716-22-f5b1c2e0-1947-4a2e-a814-6ce401f2a604/working/working-outputfiles-33/gatt-xml-master/org.bluetooth.characteristic.cross_trainer_data.xml>,
    <file:/data/lp/etl/executor/data/1651932367716-22-f5b1c2e0-1947-4a2e-a814-6ce401f2a604/working/working-outputfiles-33/gatt-xml-master/org.bluetooth.characteristic.indoor_bike_data.xml>,
    <file:/data/lp/etl/executor/data/1651932367716-22-f5b1c2e0-1947-4a2e-a814-6ce401f2a604/working/working-outputfiles-33/gatt-xml-master/org.bluetooth.characteristic.rower_data.xml> .

<http://purl.org/wot-catalogue/ble/gatt#TotalEnergy> a skos:Concept, ontolex:LexicalConcept,
    prov:Entity;
  skos:altLabel "total energy";
  skos:broader ble:Value;
  skos:definition """Kilo Calorie with a resolution of
      1""";
  skos:inScheme ble:Scheme;
  skos:prefLabel "Total Energy";
  prov:wasDerivedFrom <file:/data/lp/etl/executor/data/1651932367716-22-f5b1c2e0-1947-4a2e-a814-6ce401f2a604/working/working-outputfiles-33/gatt-xml-master/org.bluetooth.characteristic.cross_trainer_data.xml>,
    <file:/data/lp/etl/executor/data/1651932367716-22-f5b1c2e0-1947-4a2e-a814-6ce401f2a604/working/working-outputfiles-33/gatt-xml-master/org.bluetooth.characteristic.indoor_bike_data.xml>,
    <file:/data/lp/etl/executor/data/1651932367716-22-f5b1c2e0-1947-4a2e-a814-6ce401f2a604/working/working-outputfiles-33/gatt-xml-master/org.bluetooth.characteristic.rower_data.xml>,
    <file:/data/lp/etl/executor/data/1651932367716-22-f5b1c2e0-1947-4a2e-a814-6ce401f2a604/working/working-outputfiles-33/gatt-xml-master/org.bluetooth.characteristic.stair_climber_data.xml>,
    <file:/data/lp/etl/executor/data/1651932367716-22-f5b1c2e0-1947-4a2e-a814-6ce401f2a604/working/working-outputfiles-33/gatt-xml-master/org.bluetooth.characteristic.step_climber_data.xml>,
    <file:/data/lp/etl/executor/data/1651932367716-22-f5b1c2e0-1947-4a2e-a814-6ce401f2a604/working/working-outputfiles-33/gatt-xml-master/org.bluetooth.characteristic.treadmill_data.xml> .

<http://purl.org/wot-catalogue/ble/gatt#EnergyPerHour> a skos:Concept, ontolex:LexicalConcept,
    prov:Entity;
  skos:altLabel "energy per hour";
  skos:broader ble:Value;
  skos:definition """Kilo Calorie with a resolution of
      1""";
  skos:inScheme ble:Scheme;
  skos:prefLabel "Energy Per Hour";
  prov:wasDerivedFrom <file:/data/lp/etl/executor/data/1651932367716-22-f5b1c2e0-1947-4a2e-a814-6ce401f2a604/working/working-outputfiles-33/gatt-xml-master/org.bluetooth.characteristic.cross_trainer_data.xml>,
    <file:/data/lp/etl/executor/data/1651932367716-22-f5b1c2e0-1947-4a2e-a814-6ce401f2a604/working/working-outputfiles-33/gatt-xml-master/org.bluetooth.characteristic.indoor_bike_data.xml>,
    <file:/data/lp/etl/executor/data/1651932367716-22-f5b1c2e0-1947-4a2e-a814-6ce401f2a604/working/working-outputfiles-33/gatt-xml-master/org.bluetooth.characteristic.rower_data.xml>,
    <file:/data/lp/etl/executor/data/1651932367716-22-f5b1c2e0-1947-4a2e-a814-6ce401f2a604/working/working-outputfiles-33/gatt-xml-master/org.bluetooth.characteristic.stair_climber_data.xml>,
    <file:/data/lp/etl/executor/data/1651932367716-22-f5b1c2e0-1947-4a2e-a814-6ce401f2a604/working/working-outputfiles-33/gatt-xml-master/org.bluetooth.characteristic.step_climber_data.xml>,
    <file:/data/lp/etl/executor/data/1651932367716-22-f5b1c2e0-1947-4a2e-a814-6ce401f2a604/working/working-outputfiles-33/gatt-xml-master/org.bluetooth.characteristic.treadmill_data.xml> .

<http://purl.org/wot-catalogue/ble/gatt#EnergyPerMinute> a skos:Concept, ontolex:LexicalConcept,
    prov:Entity;
  skos:altLabel "energy per minute";
  skos:broader ble:Value;
  skos:definition """Kilo Calorie with a resolution of
      1""";
  skos:inScheme ble:Scheme;
  skos:prefLabel "Energy Per Minute";
  prov:wasDerivedFrom <file:/data/lp/etl/executor/data/1651932367716-22-f5b1c2e0-1947-4a2e-a814-6ce401f2a604/working/working-outputfiles-33/gatt-xml-master/org.bluetooth.characteristic.cross_trainer_data.xml>,
    <file:/data/lp/etl/executor/data/1651932367716-22-f5b1c2e0-1947-4a2e-a814-6ce401f2a604/working/working-outputfiles-33/gatt-xml-master/org.bluetooth.characteristic.indoor_bike_data.xml>,
    <file:/data/lp/etl/executor/data/1651932367716-22-f5b1c2e0-1947-4a2e-a814-6ce401f2a604/working/working-outputfiles-33/gatt-xml-master/org.bluetooth.characteristic.rower_data.xml>,
    <file:/data/lp/etl/executor/data/1651932367716-22-f5b1c2e0-1947-4a2e-a814-6ce401f2a604/working/working-outputfiles-33/gatt-xml-master/org.bluetooth.characteristic.stair_climber_data.xml>,
    <file:/data/lp/etl/executor/data/1651932367716-22-f5b1c2e0-1947-4a2e-a814-6ce401f2a604/working/working-outputfiles-33/gatt-xml-master/org.bluetooth.characteristic.step_climber_data.xml>,
    <file:/data/lp/etl/executor/data/1651932367716-22-f5b1c2e0-1947-4a2e-a814-6ce401f2a604/working/working-outputfiles-33/gatt-xml-master/org.bluetooth.characteristic.treadmill_data.xml> .

<http://purl.org/wot-catalogue/ble/gatt#HeartRate> a skos:Concept, ontolex:LexicalConcept,
    prov:Entity;
  skos:altLabel "heart rate";
  skos:broader ble:Value;
  skos:definition """Beats per minute with a resolution of
      1""";
  skos:inScheme ble:Scheme;
  skos:prefLabel "Heart Rate";
  prov:wasDerivedFrom <file:/data/lp/etl/executor/data/1651932367716-22-f5b1c2e0-1947-4a2e-a814-6ce401f2a604/working/working-outputfiles-33/gatt-xml-master/org.bluetooth.characteristic.cross_trainer_data.xml>,
    <file:/data/lp/etl/executor/data/1651932367716-22-f5b1c2e0-1947-4a2e-a814-6ce401f2a604/working/working-outputfiles-33/gatt-xml-master/org.bluetooth.characteristic.indoor_bike_data.xml>,
    <file:/data/lp/etl/executor/data/1651932367716-22-f5b1c2e0-1947-4a2e-a814-6ce401f2a604/working/working-outputfiles-33/gatt-xml-master/org.bluetooth.characteristic.rower_data.xml>,
    <file:/data/lp/etl/executor/data/1651932367716-22-f5b1c2e0-1947-4a2e-a814-6ce401f2a604/working/working-outputfiles-33/gatt-xml-master/org.bluetooth.characteristic.stair_climber_data.xml>,
    <file:/data/lp/etl/executor/data/1651932367716-22-f5b1c2e0-1947-4a2e-a814-6ce401f2a604/working/working-outputfiles-33/gatt-xml-master/org.bluetooth.characteristic.step_climber_data.xml>,
    <file:/data/lp/etl/executor/data/1651932367716-22-f5b1c2e0-1947-4a2e-a814-6ce401f2a604/working/working-outputfiles-33/gatt-xml-master/org.bluetooth.characteristic.treadmill_data.xml> .

<http://purl.org/wot-catalogue/ble/gatt#MetabolicEquivalent> a skos:Concept, ontolex:LexicalConcept,
    prov:Entity;
  skos:altLabel "metabolic equivalent";
  skos:broader ble:Value;
  skos:definition """Metabolic Equivalent with a resolution of
      0.1""";
  skos:inScheme ble:Scheme;
  skos:prefLabel "Metabolic Equivalent";
  prov:wasDerivedFrom <file:/data/lp/etl/executor/data/1651932367716-22-f5b1c2e0-1947-4a2e-a814-6ce401f2a604/working/working-outputfiles-33/gatt-xml-master/org.bluetooth.characteristic.cross_trainer_data.xml>,
    <file:/data/lp/etl/executor/data/1651932367716-22-f5b1c2e0-1947-4a2e-a814-6ce401f2a604/working/working-outputfiles-33/gatt-xml-master/org.bluetooth.characteristic.indoor_bike_data.xml>,
    <file:/data/lp/etl/executor/data/1651932367716-22-f5b1c2e0-1947-4a2e-a814-6ce401f2a604/working/working-outputfiles-33/gatt-xml-master/org.bluetooth.characteristic.rower_data.xml>,
    <file:/data/lp/etl/executor/data/1651932367716-22-f5b1c2e0-1947-4a2e-a814-6ce401f2a604/working/working-outputfiles-33/gatt-xml-master/org.bluetooth.characteristic.stair_climber_data.xml>,
    <file:/data/lp/etl/executor/data/1651932367716-22-f5b1c2e0-1947-4a2e-a814-6ce401f2a604/working/working-outputfiles-33/gatt-xml-master/org.bluetooth.characteristic.step_climber_data.xml>,
    <file:/data/lp/etl/executor/data/1651932367716-22-f5b1c2e0-1947-4a2e-a814-6ce401f2a604/working/working-outputfiles-33/gatt-xml-master/org.bluetooth.characteristic.treadmill_data.xml> .

<http://purl.org/wot-catalogue/ble/gatt#ElapsedTime> a skos:Concept, ontolex:LexicalConcept,
    prov:Entity;
  skos:altLabel "elapsed time";
  skos:broader ble:Value;
  skos:definition """Second with a resolution of
      1""";
  skos:inScheme ble:Scheme;
  skos:prefLabel "Elapsed Time";
  prov:wasDerivedFrom <file:/data/lp/etl/executor/data/1651932367716-22-f5b1c2e0-1947-4a2e-a814-6ce401f2a604/working/working-outputfiles-33/gatt-xml-master/org.bluetooth.characteristic.cross_trainer_data.xml>,
    <file:/data/lp/etl/executor/data/1651932367716-22-f5b1c2e0-1947-4a2e-a814-6ce401f2a604/working/working-outputfiles-33/gatt-xml-master/org.bluetooth.characteristic.indoor_bike_data.xml>,
    <file:/data/lp/etl/executor/data/1651932367716-22-f5b1c2e0-1947-4a2e-a814-6ce401f2a604/working/working-outputfiles-33/gatt-xml-master/org.bluetooth.characteristic.rower_data.xml>,
    <file:/data/lp/etl/executor/data/1651932367716-22-f5b1c2e0-1947-4a2e-a814-6ce401f2a604/working/working-outputfiles-33/gatt-xml-master/org.bluetooth.characteristic.stair_climber_data.xml>,
    <file:/data/lp/etl/executor/data/1651932367716-22-f5b1c2e0-1947-4a2e-a814-6ce401f2a604/working/working-outputfiles-33/gatt-xml-master/org.bluetooth.characteristic.step_climber_data.xml>,
    <file:/data/lp/etl/executor/data/1651932367716-22-f5b1c2e0-1947-4a2e-a814-6ce401f2a604/working/working-outputfiles-33/gatt-xml-master/org.bluetooth.characteristic.treadmill_data.xml> .

<http://purl.org/wot-catalogue/ble/gatt#RemainingTime> a skos:Concept, ontolex:LexicalConcept,
    prov:Entity;
  skos:altLabel "remaining time";
  skos:broader ble:Value;
  skos:definition """Second with a resolution of
      1""";
  skos:inScheme ble:Scheme;
  skos:prefLabel "Remaining Time";
  prov:wasDerivedFrom <file:/data/lp/etl/executor/data/1651932367716-22-f5b1c2e0-1947-4a2e-a814-6ce401f2a604/working/working-outputfiles-33/gatt-xml-master/org.bluetooth.characteristic.cross_trainer_data.xml>,
    <file:/data/lp/etl/executor/data/1651932367716-22-f5b1c2e0-1947-4a2e-a814-6ce401f2a604/working/working-outputfiles-33/gatt-xml-master/org.bluetooth.characteristic.indoor_bike_data.xml>,
    <file:/data/lp/etl/executor/data/1651932367716-22-f5b1c2e0-1947-4a2e-a814-6ce401f2a604/working/working-outputfiles-33/gatt-xml-master/org.bluetooth.characteristic.rower_data.xml>,
    <file:/data/lp/etl/executor/data/1651932367716-22-f5b1c2e0-1947-4a2e-a814-6ce401f2a604/working/working-outputfiles-33/gatt-xml-master/org.bluetooth.characteristic.stair_climber_data.xml>,
    <file:/data/lp/etl/executor/data/1651932367716-22-f5b1c2e0-1947-4a2e-a814-6ce401f2a604/working/working-outputfiles-33/gatt-xml-master/org.bluetooth.characteristic.step_climber_data.xml>,
    <file:/data/lp/etl/executor/data/1651932367716-22-f5b1c2e0-1947-4a2e-a814-6ce401f2a604/working/working-outputfiles-33/gatt-xml-master/org.bluetooth.characteristic.treadmill_data.xml> .

<http://purl.org/wot-catalogue/ble/gatt#org.bluetooth.characteristic.cgm_status> a
    skos:Concept, ontolex:LexicalConcept, prov:Entity;
  skos:altLabel "cgm status";
  skos:broader ble:Characteristic;
  skos:definition """The CGM Status allows the Collector to actively
    request the current status from the CGM Sensor, particularly
    when the CGM measurement is not running and the status cannot
    be given in the measurement result in the Status
    Annunciation.""";
  skos:inScheme ble:Scheme;
  skos:prefLabel "CGM Status";
  skos:related ble:CGMStatus, ble:E2E-CRC, ble:Read, ble:TimeOffset;
  prov:wasDerivedFrom <file:/data/lp/etl/executor/data/1651932367716-22-f5b1c2e0-1947-4a2e-a814-6ce401f2a604/working/working-outputfiles-33/gatt-xml-master/org.bluetooth.characteristic.cgm_status.xml> .

<http://purl.org/wot-catalogue/ble/gatt#TimeOffset> a skos:Concept, ontolex:LexicalConcept,
    prov:Entity;
  skos:altLabel "time offset";
  skos:broader ble:Value;
  skos:definition """C1: Field exists if the key of bit 0 of the
      Flags field is set to 1""",
    """The Time Offset Field specifies the actual
      relative time difference to the session start
      time.""",
    """The following values are defined for the
      Time Offset Field, specifying the relative time difference of
      the single CGM values to the session start time. Value:
      (0x0000 - 0xFFFF), Description: (Time offset in minutes as
      offset to the Session Start Time).""";
  skos:inScheme ble:Scheme;
  skos:prefLabel "Time Offset";
  prov:wasDerivedFrom <file:/data/lp/etl/executor/data/1651932367716-22-f5b1c2e0-1947-4a2e-a814-6ce401f2a604/working/working-outputfiles-33/gatt-xml-master/org.bluetooth.characteristic.cgm_measurement.xml>,
    <file:/data/lp/etl/executor/data/1651932367716-22-f5b1c2e0-1947-4a2e-a814-6ce401f2a604/working/working-outputfiles-33/gatt-xml-master/org.bluetooth.characteristic.cgm_status.xml>,
    <file:/data/lp/etl/executor/data/1651932367716-22-f5b1c2e0-1947-4a2e-a814-6ce401f2a604/working/working-outputfiles-33/gatt-xml-master/org.bluetooth.characteristic.glucose_measurement.xml> .

<http://purl.org/wot-catalogue/ble/gatt#CGMStatus> a skos:Concept, ontolex:LexicalConcept,
    prov:Entity;
  skos:altLabel "cgm status";
  skos:broader ble:Value;
  skos:definition """The structure of the CGM Status Field shall
      be identical to the structure of the Status Annunciation
      Field, as defined in the CGM Measurement Characteristic
      \"Sensor Status Annunciation Field\". It always consists of
      three octets regardless the value.""";
  skos:inScheme ble:Scheme;
  skos:prefLabel "CGM Status";
  prov:wasDerivedFrom <file:/data/lp/etl/executor/data/1651932367716-22-f5b1c2e0-1947-4a2e-a814-6ce401f2a604/working/working-outputfiles-33/gatt-xml-master/org.bluetooth.characteristic.cgm_status.xml> .

<http://purl.org/wot-catalogue/ble/gatt#E2E-CRC> a skos:Concept, ontolex:LexicalConcept,
    prov:Entity;
  skos:altLabel "e2e-crc";
  skos:broader ble:Value;
  skos:definition """If the device supports E2E-safety
      (E2E-CRC-Supported bit is set in CGM Feature), the session
      run time is secured by a CRC calculated over all
      fields.""",
    """If the device supports E2E-safety
      (E2E-CRC-Supported bit is set in CGM Feature), the session
      start time is secured by a CRC calculated over all
      fields.""",
    """If the device supports E2E-safety
      (E2E-CRC-Supported bit is set in CGM Feature), the specific
      ops control point is secured by a CRC calculated over all
      fields. Refer to CGM Service specification.""",
    """If the device supports E2E-safety (E2E-CRC
      Supported bit is set in CGM Feature), the feature are secured
      by a CRC calculated over all data. This field is mandatory in
      this characteristic. If the device doesn?t support E2E-safety
      the value of the field shall be set to
      0xFFFF.""",
    """If the device supports E2E-safety (E2E-CRC
      Supported bit is set in CGM Feature), the measurement is
      secured by a CRC calculated over all fields. The computation
      of the CRC is done using a CRC-CCITT generator polynomial
      g(D)=D16+D12+D5+1 (i.e.210041 in octal representation) with a
      seed of 0xFFFF. This field is mandatory if the device
      supports E2E-CRC (Bit 12 in CGM Feature is set to 1)
      otherwise excluded.""",
    """If the device supports E2E-safety (E2E-CRC
      Supported bit is set in CGM Feature), the status is secured
      by a CRC calculated over all fields.""";
  skos:inScheme ble:Scheme;
  skos:prefLabel "E2E-CRC";
  prov:wasDerivedFrom <file:/data/lp/etl/executor/data/1651932367716-22-f5b1c2e0-1947-4a2e-a814-6ce401f2a604/working/working-outputfiles-33/gatt-xml-master/org.bluetooth.characteristic.cgm_feature.xml>,
    <file:/data/lp/etl/executor/data/1651932367716-22-f5b1c2e0-1947-4a2e-a814-6ce401f2a604/working/working-outputfiles-33/gatt-xml-master/org.bluetooth.characteristic.cgm_measurement.xml>,
    <file:/data/lp/etl/executor/data/1651932367716-22-f5b1c2e0-1947-4a2e-a814-6ce401f2a604/working/working-outputfiles-33/gatt-xml-master/org.bluetooth.characteristic.cgm_session_run_time.xml>,
    <file:/data/lp/etl/executor/data/1651932367716-22-f5b1c2e0-1947-4a2e-a814-6ce401f2a604/working/working-outputfiles-33/gatt-xml-master/org.bluetooth.characteristic.cgm_session_start_time.xml>,
    <file:/data/lp/etl/executor/data/1651932367716-22-f5b1c2e0-1947-4a2e-a814-6ce401f2a604/working/working-outputfiles-33/gatt-xml-master/org.bluetooth.characteristic.cgm_specific_ops_control_point.xml>,
    <file:/data/lp/etl/executor/data/1651932367716-22-f5b1c2e0-1947-4a2e-a814-6ce401f2a604/working/working-outputfiles-33/gatt-xml-master/org.bluetooth.characteristic.cgm_status.xml> .

<http://purl.org/wot-catalogue/ble/gatt#org.bluetooth.characteristic.aggregate> a
    skos:Concept, ontolex:LexicalConcept, prov:Entity;
  skos:altLabel "aggregate";
  skos:broader ble:Characteristic;
  skos:definition """The Aggregate Input is an aggregate of the Digital
    Input Characteristic value (if available) and ALL Analog Inputs
    available.""";
  skos:inScheme ble:Scheme;
  skos:prefLabel "Aggregate";
  skos:related ble:AnalogInput, ble:Indicate, ble:InputBits, ble:Notify, ble:Read;
  prov:wasDerivedFrom <file:/data/lp/etl/executor/data/1651932367716-22-f5b1c2e0-1947-4a2e-a814-6ce401f2a604/working/working-outputfiles-33/gatt-xml-master/org.bluetooth.characteristic.aggregate.xml> .

<http://purl.org/wot-catalogue/ble/gatt#InputBits> a skos:Concept, ontolex:LexicalConcept,
    prov:Entity;
  skos:altLabel "input bits";
  skos:broader ble:Value;
  skos:inScheme ble:Scheme;
  skos:prefLabel "Input Bits";
  prov:wasDerivedFrom <file:/data/lp/etl/executor/data/1651932367716-22-f5b1c2e0-1947-4a2e-a814-6ce401f2a604/working/working-outputfiles-33/gatt-xml-master/org.bluetooth.characteristic.aggregate.xml> .

<http://purl.org/wot-catalogue/ble/gatt#AnalogInput> a skos:Concept, ontolex:LexicalConcept,
    prov:Entity;
  skos:altLabel "analog input";
  skos:broader ble:Value;
  skos:inScheme ble:Scheme;
  skos:prefLabel "Analog Input";
  prov:wasDerivedFrom <file:/data/lp/etl/executor/data/1651932367716-22-f5b1c2e0-1947-4a2e-a814-6ce401f2a604/working/working-outputfiles-33/gatt-xml-master/org.bluetooth.characteristic.aggregate.xml> .

<http://purl.org/wot-catalogue/ble/gatt#org.bluetooth.characteristic.supported_speed_range>
  a skos:Concept, ontolex:LexicalConcept, prov:Entity;
  skos:altLabel "supported speed range";
  skos:broader ble:Characteristic;
  skos:definition """The Supported Speed Range characteristic is used to
    send the supported speed range as well as the minimum speed
    increment supported by the Server.""";
  skos:inScheme ble:Scheme;
  skos:prefLabel "Supported Speed Range";
  skos:related ble:InformationText, ble:MaximumSpeed, ble:MinimumIncrement, ble:MinimumSpeed,
    ble:Read;
  prov:wasDerivedFrom <file:/data/lp/etl/executor/data/1651932367716-22-f5b1c2e0-1947-4a2e-a814-6ce401f2a604/working/working-outputfiles-33/gatt-xml-master/org.bluetooth.characteristic.supported_speed_range.xml> .

<http://purl.org/wot-catalogue/ble/gatt#MinimumSpeed> a skos:Concept, ontolex:LexicalConcept,
    prov:Entity;
  skos:altLabel "minimum speed";
  skos:broader ble:Value;
  skos:definition """Kilometer per hour with a resolution of
      0.01""";
  skos:inScheme ble:Scheme;
  skos:prefLabel "Minimum Speed";
  prov:wasDerivedFrom <file:/data/lp/etl/executor/data/1651932367716-22-f5b1c2e0-1947-4a2e-a814-6ce401f2a604/working/working-outputfiles-33/gatt-xml-master/org.bluetooth.characteristic.supported_speed_range.xml> .

<http://purl.org/wot-catalogue/ble/gatt#MaximumSpeed> a skos:Concept, ontolex:LexicalConcept,
    prov:Entity;
  skos:altLabel "maximum speed";
  skos:broader ble:Value;
  skos:definition """Kilometer per hour with a resolution of
      0.01""";
  skos:inScheme ble:Scheme;
  skos:prefLabel "Maximum Speed";
  prov:wasDerivedFrom <file:/data/lp/etl/executor/data/1651932367716-22-f5b1c2e0-1947-4a2e-a814-6ce401f2a604/working/working-outputfiles-33/gatt-xml-master/org.bluetooth.characteristic.supported_speed_range.xml> .

<http://purl.org/wot-catalogue/ble/gatt#MinimumIncrement> a skos:Concept, ontolex:LexicalConcept,
    prov:Entity;
  skos:altLabel "minimum increment";
  skos:broader ble:Value;
  skos:definition """Beats per minute with a resolution of
      1""", """Meters per second with a resolution of
      0.01""",
    """Percent with a resolution of
      0.1""", """Unitless with a resolution of
      0.1""",
    """Watt with a resolution of
      1""";
  skos:inScheme ble:Scheme;
  skos:prefLabel "Minimum Increment";
  prov:wasDerivedFrom <file:/data/lp/etl/executor/data/1651932367716-22-f5b1c2e0-1947-4a2e-a814-6ce401f2a604/working/working-outputfiles-33/gatt-xml-master/org.bluetooth.characteristic.supported_heart_rate_range.xml>,
    <file:/data/lp/etl/executor/data/1651932367716-22-f5b1c2e0-1947-4a2e-a814-6ce401f2a604/working/working-outputfiles-33/gatt-xml-master/org.bluetooth.characteristic.supported_inclination_range.xml>,
    <file:/data/lp/etl/executor/data/1651932367716-22-f5b1c2e0-1947-4a2e-a814-6ce401f2a604/working/working-outputfiles-33/gatt-xml-master/org.bluetooth.characteristic.supported_power_range.xml>,
    <file:/data/lp/etl/executor/data/1651932367716-22-f5b1c2e0-1947-4a2e-a814-6ce401f2a604/working/working-outputfiles-33/gatt-xml-master/org.bluetooth.characteristic.supported_resistance_level_range.xml>,
    <file:/data/lp/etl/executor/data/1651932367716-22-f5b1c2e0-1947-4a2e-a814-6ce401f2a604/working/working-outputfiles-33/gatt-xml-master/org.bluetooth.characteristic.supported_speed_range.xml> .

<http://purl.org/wot-catalogue/ble/gatt#org.bluetooth.characteristic.five_zone_heart_rate_limits>
  a skos:Concept, ontolex:LexicalConcept, prov:Entity;
  skos:altLabel "five zone heart rate limits";
  skos:broader ble:Characteristic;
  skos:definition """Data structure containing the limits between the
    heart rate zones for the 5-zone heart rate definition (Maximum,
    Hard, Moderate, Light and Very Light).""";
  skos:inScheme ble:Scheme;
  skos:prefLabel "Five Zone Heart Rate Limits";
  skos:related <http://purl.org/wot-catalogue/ble#FiveZoneHeartRateLimits-Hard/MaximumLimit>,
    <http://purl.org/wot-catalogue/ble#FiveZoneHeartRateLimits-Light/ModerateLimit>, <http://purl.org/wot-catalogue/ble#FiveZoneHeartRateLimits-Moderate/HardLimit>,
    <http://purl.org/wot-catalogue/ble#FiveZoneHeartRateLimits-Verylight/LightLimit>,
    ble:Read, ble:Write;
  prov:wasDerivedFrom <file:/data/lp/etl/executor/data/1651932367716-22-f5b1c2e0-1947-4a2e-a814-6ce401f2a604/working/working-outputfiles-33/gatt-xml-master/org.bluetooth.characteristic.five_zone_heart_rate_limits.xml> .

<http://purl.org/wot-catalogue/ble/gatt#FiveZoneHeartRateLimits-Verylight/LightLimit>
  a skos:Concept, ontolex:LexicalConcept, prov:Entity;
  skos:altLabel "five zone heart rate limits - very light / light limit";
  skos:broader ble:Value;
  skos:definition """Unit is in beats per minute with a
      resolution of 1""";
  skos:inScheme ble:Scheme;
  skos:prefLabel "Five Zone Heart Rate Limits - Very light / Light Limit";
  prov:wasDerivedFrom <file:/data/lp/etl/executor/data/1651932367716-22-f5b1c2e0-1947-4a2e-a814-6ce401f2a604/working/working-outputfiles-33/gatt-xml-master/org.bluetooth.characteristic.five_zone_heart_rate_limits.xml> .

<http://purl.org/wot-catalogue/ble/gatt#FiveZoneHeartRateLimits-Light/ModerateLimit>
  a skos:Concept, ontolex:LexicalConcept, prov:Entity;
  skos:altLabel "five zone heart rate limits - light / moderate limit";
  skos:broader ble:Value;
  skos:definition """Unit is in beats per minute with a
      resolution of 1""";
  skos:inScheme ble:Scheme;
  skos:prefLabel "Five Zone Heart Rate Limits - Light / Moderate Limit";
  prov:wasDerivedFrom <file:/data/lp/etl/executor/data/1651932367716-22-f5b1c2e0-1947-4a2e-a814-6ce401f2a604/working/working-outputfiles-33/gatt-xml-master/org.bluetooth.characteristic.five_zone_heart_rate_limits.xml> .

<http://purl.org/wot-catalogue/ble/gatt#FiveZoneHeartRateLimits-Moderate/HardLimit>
  a skos:Concept, ontolex:LexicalConcept, prov:Entity;
  skos:altLabel "five zone heart rate limits - moderate / hard limit";
  skos:broader ble:Value;
  skos:definition """Unit is in beats per minute with a
      resolution of 1""";
  skos:inScheme ble:Scheme;
  skos:prefLabel "Five Zone Heart Rate Limits - Moderate / Hard Limit";
  prov:wasDerivedFrom <file:/data/lp/etl/executor/data/1651932367716-22-f5b1c2e0-1947-4a2e-a814-6ce401f2a604/working/working-outputfiles-33/gatt-xml-master/org.bluetooth.characteristic.five_zone_heart_rate_limits.xml> .

<http://purl.org/wot-catalogue/ble/gatt#FiveZoneHeartRateLimits-Hard/MaximumLimit>
  a skos:Concept, ontolex:LexicalConcept, prov:Entity;
  skos:altLabel "five zone heart rate limits - hard / maximum limit";
  skos:broader ble:Value;
  skos:definition """Unit is in beats per minute with a
      resolution of 1""";
  skos:inScheme ble:Scheme;
  skos:prefLabel "Five Zone Heart Rate Limits - Hard / Maximum Limit";
  prov:wasDerivedFrom <file:/data/lp/etl/executor/data/1651932367716-22-f5b1c2e0-1947-4a2e-a814-6ce401f2a604/working/working-outputfiles-33/gatt-xml-master/org.bluetooth.characteristic.five_zone_heart_rate_limits.xml> .

<http://purl.org/wot-catalogue/ble/gatt#1825> a skos:Concept, ontolex:LexicalConcept,
    prov:Entity;
  skos:altLabel "object transfer service";
  skos:broader ble:Service;
  skos:definition ".";
  skos:inScheme ble:Scheme;
  skos:prefLabel "Object Transfer Service";
  skos:related ble:org.bluetooth.characteristic.object_action_control_point, ble:org.bluetooth.characteristic.object_changed,
    ble:org.bluetooth.characteristic.object_first_created, ble:org.bluetooth.characteristic.object_id,
    ble:org.bluetooth.characteristic.object_last_modified, ble:org.bluetooth.characteristic.object_list_control_point,
    ble:org.bluetooth.characteristic.object_list_filter, ble:org.bluetooth.characteristic.object_name,
    ble:org.bluetooth.characteristic.object_properties, ble:org.bluetooth.characteristic.object_size,
    ble:org.bluetooth.characteristic.object_type, ble:org.bluetooth.characteristic.ots_feature;
  prov:wasDerivedFrom <file:/data/lp/etl/executor/data/1651932367716-22-f5b1c2e0-1947-4a2e-a814-6ce401f2a604/working/working-outputfiles-33/gatt-xml-master/org.bluetooth.service.object_transfer.xml> .

<http://purl.org/wot-catalogue/ble/gatt#org.bluetooth.characteristic.ots_feature>
  a skos:Concept, ontolex:LexicalConcept, prov:Entity;
  skos:altLabel "ots feature";
  skos:broader ble:Characteristic;
  skos:inScheme ble:Scheme;
  skos:prefLabel "OTS Feature";
  skos:related ble:Read;
  prov:wasDerivedFrom <file:/data/lp/etl/executor/data/1651932367716-22-f5b1c2e0-1947-4a2e-a814-6ce401f2a604/working/working-outputfiles-33/gatt-xml-master/org.bluetooth.characteristic.ots_feature.xml> .

<http://purl.org/wot-catalogue/ble/gatt#org.bluetooth.characteristic.object_name>
  a skos:Concept, ontolex:LexicalConcept, prov:Entity;
  skos:altLabel "object name";
  skos:broader ble:Characteristic;
  skos:inScheme ble:Scheme;
  skos:prefLabel "Object Name";
  skos:related ble:ObjectName, ble:Read, ble:Write;
  prov:wasDerivedFrom <file:/data/lp/etl/executor/data/1651932367716-22-f5b1c2e0-1947-4a2e-a814-6ce401f2a604/working/working-outputfiles-33/gatt-xml-master/org.bluetooth.characteristic.object_name.xml> .

<http://purl.org/wot-catalogue/ble/gatt#org.bluetooth.characteristic.object_type>
  a skos:Concept, ontolex:LexicalConcept, prov:Entity;
  skos:altLabel "object type";
  skos:broader ble:Characteristic;
  skos:inScheme ble:Scheme;
  skos:prefLabel "Object Type";
  skos:related ble:ObjectType, ble:Read;
  prov:wasDerivedFrom <file:/data/lp/etl/executor/data/1651932367716-22-f5b1c2e0-1947-4a2e-a814-6ce401f2a604/working/working-outputfiles-33/gatt-xml-master/org.bluetooth.characteristic.object_type.xml> .

<http://purl.org/wot-catalogue/ble/gatt#org.bluetooth.characteristic.object_size>
  a skos:Concept, ontolex:LexicalConcept, prov:Entity;
  skos:altLabel "object size";
  skos:broader ble:Characteristic;
  skos:inScheme ble:Scheme;
  skos:prefLabel "Object Size";
  skos:related ble:AllocatedSize, ble:CurrentSize, ble:Read;
  prov:wasDerivedFrom <file:/data/lp/etl/executor/data/1651932367716-22-f5b1c2e0-1947-4a2e-a814-6ce401f2a604/working/working-outputfiles-33/gatt-xml-master/org.bluetooth.characteristic.object_size.xml> .

<http://purl.org/wot-catalogue/ble/gatt#org.bluetooth.characteristic.object_last_modified>
  a skos:Concept, ontolex:LexicalConcept, prov:Entity;
  skos:altLabel "object last-modified";
  skos:broader ble:Characteristic;
  skos:inScheme ble:Scheme;
  skos:prefLabel "Object Last-Modified";
  skos:related ble:ObjectLast-Modified, ble:Read, ble:Write;
  prov:wasDerivedFrom <file:/data/lp/etl/executor/data/1651932367716-22-f5b1c2e0-1947-4a2e-a814-6ce401f2a604/working/working-outputfiles-33/gatt-xml-master/org.bluetooth.characteristic.object_last_modified.xml> .

<http://purl.org/wot-catalogue/ble/gatt#org.bluetooth.characteristic.object_id> a
    skos:Concept, ontolex:LexicalConcept, prov:Entity;
  skos:altLabel "object id";
  skos:broader ble:Characteristic;
  skos:inScheme ble:Scheme;
  skos:prefLabel "Object ID";
  skos:related ble:ObjectID, ble:Read;
  prov:wasDerivedFrom <file:/data/lp/etl/executor/data/1651932367716-22-f5b1c2e0-1947-4a2e-a814-6ce401f2a604/working/working-outputfiles-33/gatt-xml-master/org.bluetooth.characteristic.object_id.xml> .

<http://purl.org/wot-catalogue/ble/gatt#org.bluetooth.characteristic.object_properties>
  a skos:Concept, ontolex:LexicalConcept, prov:Entity;
  skos:altLabel "object properties";
  skos:broader ble:Characteristic;
  skos:inScheme ble:Scheme;
  skos:prefLabel "Object Properties";
  skos:related ble:Read, ble:Write;
  prov:wasDerivedFrom <file:/data/lp/etl/executor/data/1651932367716-22-f5b1c2e0-1947-4a2e-a814-6ce401f2a604/working/working-outputfiles-33/gatt-xml-master/org.bluetooth.characteristic.object_properties.xml> .

<http://purl.org/wot-catalogue/ble/gatt#org.bluetooth.characteristic.object_action_control_point>
  a skos:Concept, ontolex:LexicalConcept, prov:Entity;
  skos:altLabel "object action control point";
  skos:broader ble:Characteristic;
  skos:inScheme ble:Scheme;
  skos:prefLabel "Object Action Control Point";
  skos:related ble:Indicate, ble:Write;
  prov:wasDerivedFrom <file:/data/lp/etl/executor/data/1651932367716-22-f5b1c2e0-1947-4a2e-a814-6ce401f2a604/working/working-outputfiles-33/gatt-xml-master/org.bluetooth.characteristic.object_action_control_point.xml> .

<http://purl.org/wot-catalogue/ble/gatt#org.bluetooth.characteristic.object_list_control_point>
  a skos:Concept, ontolex:LexicalConcept, prov:Entity;
  skos:altLabel "object list control point";
  skos:broader ble:Characteristic;
  skos:inScheme ble:Scheme;
  skos:prefLabel "Object List Control Point";
  skos:related ble:Indicate, ble:Write;
  prov:wasDerivedFrom <file:/data/lp/etl/executor/data/1651932367716-22-f5b1c2e0-1947-4a2e-a814-6ce401f2a604/working/working-outputfiles-33/gatt-xml-master/org.bluetooth.characteristic.object_list_control_point.xml> .

<http://purl.org/wot-catalogue/ble/gatt#org.bluetooth.characteristic.object_list_filter>
  a skos:Concept, ontolex:LexicalConcept, prov:Entity;
  skos:altLabel "object list filter";
  skos:broader ble:Characteristic;
  skos:inScheme ble:Scheme;
  skos:prefLabel "Object List Filter";
  skos:related ble:Read, ble:Write;
  prov:wasDerivedFrom <file:/data/lp/etl/executor/data/1651932367716-22-f5b1c2e0-1947-4a2e-a814-6ce401f2a604/working/working-outputfiles-33/gatt-xml-master/org.bluetooth.characteristic.object_list_filter.xml> .

<http://purl.org/wot-catalogue/ble/gatt#org.bluetooth.characteristic.object_changed>
  a skos:Concept, ontolex:LexicalConcept, prov:Entity;
  skos:altLabel "object changed";
  skos:broader ble:Characteristic;
  skos:inScheme ble:Scheme;
  skos:prefLabel "Object Changed";
  skos:related ble:Indicate;
  prov:wasDerivedFrom <file:/data/lp/etl/executor/data/1651932367716-22-f5b1c2e0-1947-4a2e-a814-6ce401f2a604/working/working-outputfiles-33/gatt-xml-master/org.bluetooth.characteristic.object_changed.xml> .

<http://purl.org/wot-catalogue/ble/gatt#Indicate> a skos:Concept;
  skos:altLabel "indicate";
  skos:definition "A server is configured to indicate a Characteristic Value to a client and expects an Attribute Protocol layer acknowledgment that the indication was successfully received";
  skos:inScheme ble:Scheme;
  skos:prefLabel "Indicate" .

<http://purl.org/wot-catalogue/ble/gatt#org.bluetooth.characteristic.heart_rate_control_point>
  a skos:Concept, ontolex:LexicalConcept, prov:Entity;
  skos:altLabel "heart rate control point";
  skos:broader ble:Characteristic;
  skos:inScheme ble:Scheme;
  skos:prefLabel "Heart Rate Control Point";
  skos:related ble:HeartRateControlPoint, ble:Write;
  prov:wasDerivedFrom <file:/data/lp/etl/executor/data/1651932367716-22-f5b1c2e0-1947-4a2e-a814-6ce401f2a604/working/working-outputfiles-33/gatt-xml-master/org.bluetooth.characteristic.heart_rate_control_point.xml> .

<http://purl.org/wot-catalogue/ble/gatt#HeartRateControlPoint> a skos:Concept, ontolex:LexicalConcept,
    prov:Entity;
  skos:altLabel "heart rate control point";
  skos:broader ble:Value;
  skos:inScheme ble:Scheme;
  skos:prefLabel "Heart Rate Control Point";
  prov:wasDerivedFrom <file:/data/lp/etl/executor/data/1651932367716-22-f5b1c2e0-1947-4a2e-a814-6ce401f2a604/working/working-outputfiles-33/gatt-xml-master/org.bluetooth.characteristic.heart_rate_control_point.xml> .

<http://purl.org/wot-catalogue/ble/gatt#1814> a skos:Concept, ontolex:LexicalConcept,
    prov:Entity;
  skos:altLabel "running speed and cadence";
  skos:broader ble:Service;
  skos:definition """The Running Speed and Cadence (RSC) Service exposes
    speed, cadence and other data related to fitness applications
    such as the stride length and the total distance the user has
    traveled while using the Speed and Cadence Sensor
    (Server).""";
  skos:inScheme ble:Scheme;
  skos:prefLabel "Running Speed and Cadence";
  skos:related ble:org.bluetooth.characteristic.rsc_feature, ble:org.bluetooth.characteristic.rsc_measurement,
    ble:org.bluetooth.characteristic.sc_control_point, ble:org.bluetooth.characteristic.sensor_location;
  prov:wasDerivedFrom <file:/data/lp/etl/executor/data/1651932367716-22-f5b1c2e0-1947-4a2e-a814-6ce401f2a604/working/working-outputfiles-33/gatt-xml-master/org.bluetooth.service.running_speed_and_cadence.xml> .

<http://purl.org/wot-catalogue/ble/gatt#org.bluetooth.characteristic.rsc_measurement>
  a skos:Concept, ontolex:LexicalConcept, prov:Entity;
  skos:altLabel "rsc measurement";
  skos:broader ble:Characteristic;
  skos:definition """The RSC Measurement characteristic (RSC refers to
    Running Speed and Cadence) is a variable length structure
    containing a Flags field, an Instantaneous Speed field and an
    Instantaneous Cadence field and, based on the contents of the
    Flags field, may contain a Stride Length field and a Total
    Distance field.""";
  skos:inScheme ble:Scheme;
  skos:prefLabel "RSC Measurement";
  skos:related ble:Flags, ble:InstantaneousCadence, ble:InstantaneousSpeed, ble:InstantaneousStrideLength,
    ble:Notify, ble:TotalDistance;
  prov:wasDerivedFrom <file:/data/lp/etl/executor/data/1651932367716-22-f5b1c2e0-1947-4a2e-a814-6ce401f2a604/working/working-outputfiles-33/gatt-xml-master/org.bluetooth.characteristic.rsc_measurement.xml> .

<http://purl.org/wot-catalogue/ble/gatt#org.bluetooth.characteristic.sensor_location>
  a skos:Concept, ontolex:LexicalConcept, prov:Entity;
  skos:altLabel "sensor location";
  skos:broader ble:Characteristic;
  skos:definition """The Sensor Location characteristic is used to expose
    the location of the sensor.""";
  skos:inScheme ble:Scheme;
  skos:prefLabel "Sensor Location";
  skos:related ble:Read, ble:SensorLocation;
  prov:wasDerivedFrom <file:/data/lp/etl/executor/data/1651932367716-22-f5b1c2e0-1947-4a2e-a814-6ce401f2a604/working/working-outputfiles-33/gatt-xml-master/org.bluetooth.characteristic.sensor_location.xml> .

<http://purl.org/wot-catalogue/ble/gatt#org.bluetooth.characteristic.sc_control_point>
  a skos:Concept, ontolex:LexicalConcept, prov:Entity;
  skos:altLabel "sc control point";
  skos:broader ble:Characteristic;
  skos:definition """The SC Control Point characteristic is used to request
    a specific function to be executed on the receiving
    device.""";
  skos:inScheme ble:Scheme;
  skos:prefLabel "SC Control Point";
  skos:related ble:CumulativeValue, ble:Indicate, ble:OpCode, ble:RequestOpCode, ble:ResponseParameter,
    ble:ResponseValue, ble:SensorLocationValue, ble:Write;
  prov:wasDerivedFrom <file:/data/lp/etl/executor/data/1651932367716-22-f5b1c2e0-1947-4a2e-a814-6ce401f2a604/working/working-outputfiles-33/gatt-xml-master/org.bluetooth.characteristic.sc_control_point.xml> .

<http://purl.org/wot-catalogue/ble/gatt#org.bluetooth.characteristic.hip_circumference>
  a skos:Concept, ontolex:LexicalConcept, prov:Entity;
  skos:altLabel "hip circumference";
  skos:broader ble:Characteristic;
  skos:definition """Used with the Waist Circumference value to calculate
    the Waist to Hip Ratio (WHR)""";
  skos:inScheme ble:Scheme;
  skos:prefLabel "Hip Circumference";
  skos:related ble:HipCircumference, ble:Read, ble:Write;
  prov:wasDerivedFrom <file:/data/lp/etl/executor/data/1651932367716-22-f5b1c2e0-1947-4a2e-a814-6ce401f2a604/working/working-outputfiles-33/gatt-xml-master/org.bluetooth.characteristic.hip_circumference.xml> .

<http://purl.org/wot-catalogue/ble/gatt#HipCircumference> a skos:Concept, ontolex:LexicalConcept,
    prov:Entity;
  skos:altLabel "hip circumference";
  skos:broader ble:Value;
  skos:definition """Unit is in meters with a resoluton of
      0.01""";
  skos:inScheme ble:Scheme;
  skos:prefLabel "Hip Circumference";
  prov:wasDerivedFrom <file:/data/lp/etl/executor/data/1651932367716-22-f5b1c2e0-1947-4a2e-a814-6ce401f2a604/working/working-outputfiles-33/gatt-xml-master/org.bluetooth.characteristic.hip_circumference.xml> .

<http://purl.org/wot-catalogue/ble/gatt#org.bluetooth.characteristic.sport_type_for_aerobic_and_anaerobic_thresholds>
  a skos:Concept, ontolex:LexicalConcept, prov:Entity;
  skos:altLabel "sport type for aerobic and anaerobic thresholds";
  skos:broader ble:Characteristic;
  skos:definition """Sport type enumeration(See note below). The values of
    the Sport Type for Aerobic and Anaerobic Thresholds
    characteristic are defined below""";
  skos:inScheme ble:Scheme;
  skos:prefLabel "Sport Type for Aerobic and Anaerobic Thresholds";
  skos:related ble:Read, ble:SportTypeforAerobicandAnaerobicThresholds, ble:Write;
  prov:wasDerivedFrom <file:/data/lp/etl/executor/data/1651932367716-22-f5b1c2e0-1947-4a2e-a814-6ce401f2a604/working/working-outputfiles-33/gatt-xml-master/org.bluetooth.characteristic.sport_type_for_aerobic_and_anaerobic_thresholds.xml> .

<http://purl.org/wot-catalogue/ble/gatt#SportTypeforAerobicandAnaerobicThresholds>
  a skos:Concept, ontolex:LexicalConcept, prov:Entity;
  skos:altLabel "sport type for aerobic and anaerobic thresholds";
  skos:broader ble:Value;
  skos:inScheme ble:Scheme;
  skos:prefLabel "Sport Type for Aerobic and Anaerobic Thresholds";
  prov:wasDerivedFrom <file:/data/lp/etl/executor/data/1651932367716-22-f5b1c2e0-1947-4a2e-a814-6ce401f2a604/working/working-outputfiles-33/gatt-xml-master/org.bluetooth.characteristic.sport_type_for_aerobic_and_anaerobic_thresholds.xml> .

<http://purl.org/wot-catalogue/ble/gatt#180E> a skos:Concept, ontolex:LexicalConcept,
    prov:Entity;
  skos:altLabel "phone alert status service";
  skos:broader ble:Service;
  skos:definition """The Phone Alert Status service uses the Alert Status
    characteristic, Ringer Setting characteristic to expose the
    phone alert status and Ringer Control Point characteristic to
    control phone into mute or enable.""";
  skos:inScheme ble:Scheme;
  skos:prefLabel "Phone Alert Status Service";
  skos:related ble:org.bluetooth.characteristic.alert_status, ble:org.bluetooth.characteristic.ringer_control_point,
    ble:org.bluetooth.characteristic.ringer_setting;
  prov:wasDerivedFrom <file:/data/lp/etl/executor/data/1651932367716-22-f5b1c2e0-1947-4a2e-a814-6ce401f2a604/working/working-outputfiles-33/gatt-xml-master/org.bluetooth.service.phone_alert_status.xml> .

<http://purl.org/wot-catalogue/ble/gatt#org.bluetooth.characteristic.alert_status>
  a skos:Concept, ontolex:LexicalConcept, prov:Entity;
  skos:altLabel "alert status";
  skos:broader ble:Characteristic;
  skos:definition """The Alert Status characteristic defines the Status of
    alert. 
    Bit 0, meaning ?Ringer State?Bit 1, meaning ?Vibrator State?Bit 2, meaning \"Display Alert Status\"""";
  skos:inScheme ble:Scheme;
  skos:prefLabel "Alert Status";
  skos:related ble:AlertStatus, ble:Notify, ble:Read;
  prov:wasDerivedFrom <file:/data/lp/etl/executor/data/1651932367716-22-f5b1c2e0-1947-4a2e-a814-6ce401f2a604/working/working-outputfiles-33/gatt-xml-master/org.bluetooth.characteristic.alert_status.xml> .

<http://purl.org/wot-catalogue/ble/gatt#org.bluetooth.characteristic.ringer_setting>
  a skos:Concept, ontolex:LexicalConcept, prov:Entity;
  skos:altLabel "ringer setting";
  skos:broader ble:Characteristic;
  skos:definition """The Ringer Setting characteristic defines the Setting
    of the Ringer. 
    Value 0, meaning ?Ringer Silent\"Value 1, meaning ?Ringer Normal?""";
  skos:inScheme ble:Scheme;
  skos:prefLabel "Ringer Setting";
  skos:related ble:Notify, ble:Read, ble:RingerSetting;
  prov:wasDerivedFrom <file:/data/lp/etl/executor/data/1651932367716-22-f5b1c2e0-1947-4a2e-a814-6ce401f2a604/working/working-outputfiles-33/gatt-xml-master/org.bluetooth.characteristic.ringer_setting.xml> .

<http://purl.org/wot-catalogue/ble/gatt#org.bluetooth.characteristic.ringer_control_point>
  a skos:Concept, ontolex:LexicalConcept, prov:Entity;
  skos:altLabel "ringer control point";
  skos:broader ble:Characteristic;
  skos:definition """The Ringer Control Point characteristic defines the
    Control Point of Ringer. 
    Value 1, meaning ?Silent Mode\"Value 2, meaning ?Mute Once?Value 3, meaning ?Cancel Silent Mode?""";
  skos:inScheme ble:Scheme;
  skos:prefLabel "Ringer Control point";
  skos:related ble:RingerControlPoint, ble:WriteWithoutResponse;
  prov:wasDerivedFrom <file:/data/lp/etl/executor/data/1651932367716-22-f5b1c2e0-1947-4a2e-a814-6ce401f2a604/working/working-outputfiles-33/gatt-xml-master/org.bluetooth.characteristic.ringer_control_point.xml> .

<http://purl.org/wot-catalogue/ble/gatt#org.bluetooth.characteristic.fat_burn_heart_rate_lower_limit>
  a skos:Concept, ontolex:LexicalConcept, prov:Entity;
  skos:altLabel "fat burn heart rate lower limit";
  skos:broader ble:Characteristic;
  skos:definition """Lower limit of the heart rate where the user
    maximizes the fat burn while exersizing""";
  skos:inScheme ble:Scheme;
  skos:prefLabel "Fat Burn Heart Rate Lower Limit";
  skos:related ble:FatBurnHeartRateLowerLimit, ble:Read, ble:Write;
  prov:wasDerivedFrom <file:/data/lp/etl/executor/data/1651932367716-22-f5b1c2e0-1947-4a2e-a814-6ce401f2a604/working/working-outputfiles-33/gatt-xml-master/org.bluetooth.characteristic.fat_burn_heart_rate_lower_limit.xml> .

<http://purl.org/wot-catalogue/ble/gatt#FatBurnHeartRateLowerLimit> a skos:Concept,
    ontolex:LexicalConcept, prov:Entity;
  skos:altLabel "fat burn heart rate lower limit";
  skos:broader ble:Value;
  skos:definition """Unit is in beats per minute with a
      resolution of 1""";
  skos:inScheme ble:Scheme;
  skos:prefLabel "Fat Burn Heart Rate Lower Limit";
  prov:wasDerivedFrom <file:/data/lp/etl/executor/data/1651932367716-22-f5b1c2e0-1947-4a2e-a814-6ce401f2a604/working/working-outputfiles-33/gatt-xml-master/org.bluetooth.characteristic.fat_burn_heart_rate_lower_limit.xml> .

<http://purl.org/wot-catalogue/ble/gatt#URI> a skos:Concept, ontolex:LexicalConcept,
    prov:Entity;
  skos:altLabel "uri";
  skos:broader ble:Value;
  skos:definition """The URI to be used in the HTTP
      request.""";
  skos:inScheme ble:Scheme;
  skos:prefLabel "URI";
  prov:wasDerivedFrom <file:/data/lp/etl/executor/data/1651932367716-22-f5b1c2e0-1947-4a2e-a814-6ce401f2a604/working/working-outputfiles-33/gatt-xml-master/org.bluetooth.characteristic.uri.xml> .

<http://purl.org/wot-catalogue/ble/gatt#org.bluetooth.characteristic.rainfall> a skos:Concept,
    ontolex:LexicalConcept, prov:Entity;
  skos:altLabel "rainfall";
  skos:broader ble:Characteristic;
  skos:inScheme ble:Scheme;
  skos:prefLabel "Rainfall";
  skos:related ble:ExtendedProperties, ble:Notify, ble:Rainfall, ble:Read, ble:WritableAuxiliaries;
  prov:wasDerivedFrom <file:/data/lp/etl/executor/data/1651932367716-22-f5b1c2e0-1947-4a2e-a814-6ce401f2a604/working/working-outputfiles-33/gatt-xml-master/org.bluetooth.characteristic.rainfall.xml> .

<http://purl.org/wot-catalogue/ble/gatt#Rainfall> a skos:Concept, ontolex:LexicalConcept,
    prov:Entity;
  skos:altLabel "rainfall";
  skos:broader ble:Value;
  skos:definition """Unit is in meters with a resolution of
      1mm""";
  skos:inScheme ble:Scheme;
  skos:prefLabel "Rainfall";
  prov:wasDerivedFrom <file:/data/lp/etl/executor/data/1651932367716-22-f5b1c2e0-1947-4a2e-a814-6ce401f2a604/working/working-outputfiles-33/gatt-xml-master/org.bluetooth.characteristic.rainfall.xml> .

<http://purl.org/wot-catalogue/ble/gatt#org.bluetooth.characteristic.firmware_revision_string>
  a skos:Concept, ontolex:LexicalConcept, prov:Entity;
  skos:altLabel "firmware revision string";
  skos:broader ble:Characteristic;
  skos:definition """The value of this characteristic is a UTF-8 string
    representing the firmware revision for the firmware within the
    device.""";
  skos:inScheme ble:Scheme;
  skos:prefLabel "Firmware Revision String";
  skos:related ble:FirmwareRevision, ble:Read;
  prov:wasDerivedFrom <file:/data/lp/etl/executor/data/1651932367716-22-f5b1c2e0-1947-4a2e-a814-6ce401f2a604/working/working-outputfiles-33/gatt-xml-master/org.bluetooth.characteristic.firmware_revision_string.xml> .

<http://purl.org/wot-catalogue/ble/gatt#FirmwareRevision> a skos:Concept, ontolex:LexicalConcept,
    prov:Entity;
  skos:altLabel "firmware revision";
  skos:broader ble:Value;
  skos:definition "The Firmware Revision String characteristic shall represent the firmware revision for the firmware within the device.";
  skos:inScheme ble:Scheme;
  skos:prefLabel "Firmware Revision";
  skos:related ble:Read, xsd:string;
  prov:wasDerivedFrom <file:/data/lp/etl/executor/data/1651932367716-22-f5b1c2e0-1947-4a2e-a814-6ce401f2a604/working/working-outputfiles-33/gatt-xml-master/org.bluetooth.characteristic.firmware_revision_string.xml> .

<http://purl.org/wot-catalogue/ble/gatt#org.bluetooth.characteristic.wind_chill> a
    skos:Concept, ontolex:LexicalConcept, prov:Entity;
  skos:altLabel "wind chill";
  skos:broader ble:Characteristic;
  skos:inScheme ble:Scheme;
  skos:prefLabel "Wind Chill";
  skos:related ble:ExtendedProperties, ble:Notify, ble:Read, ble:WindChill, ble:WritableAuxiliaries;
  prov:wasDerivedFrom <file:/data/lp/etl/executor/data/1651932367716-22-f5b1c2e0-1947-4a2e-a814-6ce401f2a604/working/working-outputfiles-33/gatt-xml-master/org.bluetooth.characteristic.wind_chill.xml> .

<http://purl.org/wot-catalogue/ble/gatt#WindChill> a skos:Concept, ontolex:LexicalConcept,
    prov:Entity;
  skos:altLabel "wind chill";
  skos:broader ble:Value;
  skos:definition """Unit is in degrees Celsius with a resolution
      of 1 degree Celsius""";
  skos:inScheme ble:Scheme;
  skos:prefLabel "Wind Chill";
  prov:wasDerivedFrom <file:/data/lp/etl/executor/data/1651932367716-22-f5b1c2e0-1947-4a2e-a814-6ce401f2a604/working/working-outputfiles-33/gatt-xml-master/org.bluetooth.characteristic.wind_chill.xml> .

<http://purl.org/wot-catalogue/ble/gatt#org.bluetooth.characteristic.time_source>
  a skos:Concept, ontolex:LexicalConcept, prov:Entity;
  skos:altLabel "time source";
  skos:broader ble:Characteristic;
  skos:inScheme ble:Scheme;
  skos:prefLabel "Time Source";
  skos:related ble:TimeSource;
  prov:wasDerivedFrom <file:/data/lp/etl/executor/data/1651932367716-22-f5b1c2e0-1947-4a2e-a814-6ce401f2a604/working/working-outputfiles-33/gatt-xml-master/org.bluetooth.characteristic.time_source.xml> .

<http://purl.org/wot-catalogue/ble/gatt#TimeSource> a skos:Concept, ontolex:LexicalConcept,
    prov:Entity;
  skos:altLabel "time source";
  skos:broader ble:Value;
  skos:inScheme ble:Scheme;
  skos:prefLabel "Time Source";
  prov:wasDerivedFrom <file:/data/lp/etl/executor/data/1651932367716-22-f5b1c2e0-1947-4a2e-a814-6ce401f2a604/working/working-outputfiles-33/gatt-xml-master/org.bluetooth.characteristic.time_source.xml> .

<http://purl.org/wot-catalogue/ble/gatt#1806> a skos:Concept, ontolex:LexicalConcept,
    prov:Entity;
  skos:altLabel "reference time update service";
  skos:broader ble:Service;
  skos:definition """This service enables a Bluetooth device that can
    update the system time using reference time such as GPS to
    expose the control point and the accuracy (drift) of the local
    system time compared to the reference time source.""";
  skos:inScheme ble:Scheme;
  skos:prefLabel "Reference Time Update Service";
  skos:related ble:org.bluetooth.characteristic.time_update_control_point, ble:org.bluetooth.characteristic.time_update_state;
  prov:wasDerivedFrom <file:/data/lp/etl/executor/data/1651932367716-22-f5b1c2e0-1947-4a2e-a814-6ce401f2a604/working/working-outputfiles-33/gatt-xml-master/org.bluetooth.service.reference_time_update.xml> .

<http://purl.org/wot-catalogue/ble/gatt#org.bluetooth.characteristic.time_update_control_point>
  a skos:Concept, ontolex:LexicalConcept, prov:Entity;
  skos:altLabel "time update control point";
  skos:broader ble:Characteristic;
  skos:inScheme ble:Scheme;
  skos:prefLabel "Time Update Control Point";
  skos:related ble:TimeUpdateControlPoint, ble:WriteWithoutResponse;
  prov:wasDerivedFrom <file:/data/lp/etl/executor/data/1651932367716-22-f5b1c2e0-1947-4a2e-a814-6ce401f2a604/working/working-outputfiles-33/gatt-xml-master/org.bluetooth.characteristic.time_update_control_point.xml> .

<http://purl.org/wot-catalogue/ble/gatt#org.bluetooth.characteristic.time_update_state>
  a skos:Concept, ontolex:LexicalConcept, prov:Entity;
  skos:altLabel "time update state";
  skos:broader ble:Characteristic;
  skos:inScheme ble:Scheme;
  skos:prefLabel "Time Update State";
  skos:related ble:CurrentState, ble:Read, ble:Result;
  prov:wasDerivedFrom <file:/data/lp/etl/executor/data/1651932367716-22-f5b1c2e0-1947-4a2e-a814-6ce401f2a604/working/working-outputfiles-33/gatt-xml-master/org.bluetooth.characteristic.time_update_state.xml> .

<http://purl.org/wot-catalogue/ble/gatt#org.bluetooth.characteristic.plx_features>
  a skos:Concept, ontolex:LexicalConcept, prov:Entity;
  skos:altLabel "plx features";
  skos:broader ble:Characteristic;
  skos:definition """The PLX Features characteristic is used to describe
    the supported features of the Server. Included in the
    characteristic is a PLX Features field, and, depending on the
    contents of the PLX Features field, the Measurement Status
    Support field, and the Device and Sensor Status Support
    field.""";
  skos:inScheme ble:Scheme;
  skos:prefLabel "PLX Features";
  skos:related ble:DeviceandSensorStatusSupport, ble:MeasurementStatusSupport, ble:Read,
    ble:SupportedFeatures;
  prov:wasDerivedFrom <file:/data/lp/etl/executor/data/1651932367716-22-f5b1c2e0-1947-4a2e-a814-6ce401f2a604/working/working-outputfiles-33/gatt-xml-master/org.bluetooth.characteristic.plx_features.xml> .

<http://purl.org/wot-catalogue/ble/gatt#SupportedFeatures> a skos:Concept, ontolex:LexicalConcept,
    prov:Entity;
  skos:altLabel "supported features";
  skos:broader ble:Value;
  skos:inScheme ble:Scheme;
  skos:prefLabel "Supported Features";
  prov:wasDerivedFrom <file:/data/lp/etl/executor/data/1651932367716-22-f5b1c2e0-1947-4a2e-a814-6ce401f2a604/working/working-outputfiles-33/gatt-xml-master/org.bluetooth.characteristic.plx_features.xml> .

<http://purl.org/wot-catalogue/ble/gatt#MeasurementStatusSupport> a skos:Concept,
    ontolex:LexicalConcept, prov:Entity;
  skos:altLabel "measurement status support";
  skos:broader ble:Value;
  skos:inScheme ble:Scheme;
  skos:prefLabel "Measurement Status Support";
  prov:wasDerivedFrom <file:/data/lp/etl/executor/data/1651932367716-22-f5b1c2e0-1947-4a2e-a814-6ce401f2a604/working/working-outputfiles-33/gatt-xml-master/org.bluetooth.characteristic.plx_features.xml> .

<http://purl.org/wot-catalogue/ble/gatt#DeviceandSensorStatusSupport> a skos:Concept,
    ontolex:LexicalConcept, prov:Entity;
  skos:altLabel "device and sensor status support";
  skos:broader ble:Value;
  skos:inScheme ble:Scheme;
  skos:prefLabel "Device and Sensor Status Support";
  prov:wasDerivedFrom <file:/data/lp/etl/executor/data/1651932367716-22-f5b1c2e0-1947-4a2e-a814-6ce401f2a604/working/working-outputfiles-33/gatt-xml-master/org.bluetooth.characteristic.plx_features.xml> .

<http://purl.org/wot-catalogue/ble/gatt#org.bluetooth.characteristic.alert_category_id>
  a skos:Concept, ontolex:LexicalConcept, prov:Entity;
  skos:altLabel "alert category id";
  skos:broader ble:Characteristic;
  skos:definition """The value of the characteristic is an unsigned 8 bit
    integer that has a fixed point exponent of 0. The Alert
    Category ID characteristic defines the predefined categories of
    messages as an enumeration.""";
  skos:inScheme ble:Scheme;
  skos:prefLabel "Alert Category ID";
  skos:related ble:CategoryID;
  prov:wasDerivedFrom <file:/data/lp/etl/executor/data/1651932367716-22-f5b1c2e0-1947-4a2e-a814-6ce401f2a604/working/working-outputfiles-33/gatt-xml-master/org.bluetooth.characteristic.alert_category_id.xml> .

<http://purl.org/wot-catalogue/ble/gatt#CategoryID> a skos:Concept, ontolex:LexicalConcept,
    prov:Entity;
  skos:altLabel "category id";
  skos:broader ble:Value;
  skos:definition """Target category that the command applies
      to.""", """The value shows the category for unread
      alert count""",
    """This field shows the category of the new
      alert.""";
  skos:inScheme ble:Scheme;
  skos:prefLabel "Category ID";
  prov:wasDerivedFrom <file:/data/lp/etl/executor/data/1651932367716-22-f5b1c2e0-1947-4a2e-a814-6ce401f2a604/working/working-outputfiles-33/gatt-xml-master/org.bluetooth.characteristic.alert_category_id.xml>,
    <file:/data/lp/etl/executor/data/1651932367716-22-f5b1c2e0-1947-4a2e-a814-6ce401f2a604/working/working-outputfiles-33/gatt-xml-master/org.bluetooth.characteristic.alert_notification_control_point.xml>,
    <file:/data/lp/etl/executor/data/1651932367716-22-f5b1c2e0-1947-4a2e-a814-6ce401f2a604/working/working-outputfiles-33/gatt-xml-master/org.bluetooth.characteristic.new_alert.xml>,
    <file:/data/lp/etl/executor/data/1651932367716-22-f5b1c2e0-1947-4a2e-a814-6ce401f2a604/working/working-outputfiles-33/gatt-xml-master/org.bluetooth.characteristic.unread_alert_status.xml> .

<http://purl.org/wot-catalogue/ble/gatt#1821> a skos:Concept, ontolex:LexicalConcept,
    prov:Entity;
  skos:altLabel "indoor positioning";
  skos:broader ble:Service;
  skos:definition """The service shall be either a Primary Service or
    Secondary Service and the service UUID set to Indoor
    Positioning Service.""";
  skos:inScheme ble:Scheme;
  skos:prefLabel "Indoor Positioning";
  skos:related ble:org.bluetooth.characteristic.altitude, ble:org.bluetooth.characteristic.floor_number,
    ble:org.bluetooth.characteristic.indoor_positioning_configuration, ble:org.bluetooth.characteristic.latitude,
    ble:org.bluetooth.characteristic.local_east_coordinate, ble:org.bluetooth.characteristic.local_north_coordinate,
    ble:org.bluetooth.characteristic.location_name, ble:org.bluetooth.characteristic.longitude,
    ble:org.bluetooth.characteristic.uncertainty;
  prov:wasDerivedFrom <file:/data/lp/etl/executor/data/1651932367716-22-f5b1c2e0-1947-4a2e-a814-6ce401f2a604/working/working-outputfiles-33/gatt-xml-master/org.bluetooth.service.indoor_positioning.xml> .

<http://purl.org/wot-catalogue/ble/gatt#org.bluetooth.characteristic.indoor_positioning_configuration>
  a skos:Concept, ontolex:LexicalConcept, prov:Entity;
  skos:altLabel "indoor positioning configuration";
  skos:broader ble:Characteristic;
  skos:definition """The Indoor Positioning Configuration describes the
    set of characteristic values included in the Indoor Positioning
    Service AD type.""";
  skos:inScheme ble:Scheme;
  skos:prefLabel "Indoor Positioning Configuration";
  skos:related ble:IndoorPositioningConfiguration, ble:Read, ble:ReliableWrite, ble:Write,
    ble:WriteWithoutResponse;
  prov:wasDerivedFrom <file:/data/lp/etl/executor/data/1651932367716-22-f5b1c2e0-1947-4a2e-a814-6ce401f2a604/working/working-outputfiles-33/gatt-xml-master/org.bluetooth.characteristic.indoor_positioning_configuration.xml> .

<http://purl.org/wot-catalogue/ble/gatt#org.bluetooth.characteristic.latitude> a skos:Concept,
    ontolex:LexicalConcept, prov:Entity;
  skos:altLabel "latitude";
  skos:broader ble:Characteristic;
  skos:definition """The Latitude characteristic describes the WGS84 North
    coordinate of the device.""";
  skos:inScheme ble:Scheme;
  skos:prefLabel "Latitude";
  skos:related ble:Broadcast, ble:Latitude, ble:Read, ble:ReliableWrite, ble:Write,
    ble:WriteWithoutResponse;
  prov:wasDerivedFrom <file:/data/lp/etl/executor/data/1651932367716-22-f5b1c2e0-1947-4a2e-a814-6ce401f2a604/working/working-outputfiles-33/gatt-xml-master/org.bluetooth.characteristic.latitude.xml> .

<http://purl.org/wot-catalogue/ble/gatt#org.bluetooth.characteristic.local_north_coordinate>
  a skos:Concept, ontolex:LexicalConcept, prov:Entity;
  skos:altLabel "local north coordinate";
  skos:broader ble:Characteristic;
  skos:definition """The Local North characteristic describes the North
    coordinate of the device using local coordinate
    system.""";
  skos:inScheme ble:Scheme;
  skos:prefLabel "Local North Coordinate";
  skos:related ble:Broadcast, ble:LocalNorthCoordinate, ble:Read, ble:ReliableWrite,
    ble:Write, ble:WriteWithoutResponse;
  prov:wasDerivedFrom <file:/data/lp/etl/executor/data/1651932367716-22-f5b1c2e0-1947-4a2e-a814-6ce401f2a604/working/working-outputfiles-33/gatt-xml-master/org.bluetooth.characteristic.local_north_coordinate.xml> .

<http://purl.org/wot-catalogue/ble/gatt#org.bluetooth.characteristic.local_east_coordinate>
  a skos:Concept, ontolex:LexicalConcept, prov:Entity;
  skos:altLabel "local east coordinate";
  skos:broader ble:Characteristic;
  skos:definition """The Local East characteristic describes the East
    coordinate of the device using local coordinate
    system.""";
  skos:inScheme ble:Scheme;
  skos:prefLabel "Local East Coordinate";
  skos:related ble:Broadcast, ble:LocalEastCoordinate, ble:Read, ble:ReliableWrite,
    ble:Write, ble:WriteWithoutResponse;
  prov:wasDerivedFrom <file:/data/lp/etl/executor/data/1651932367716-22-f5b1c2e0-1947-4a2e-a814-6ce401f2a604/working/working-outputfiles-33/gatt-xml-master/org.bluetooth.characteristic.local_east_coordinate.xml> .

<http://purl.org/wot-catalogue/ble/gatt#org.bluetooth.characteristic.floor_number>
  a skos:Concept, ontolex:LexicalConcept, prov:Entity;
  skos:altLabel "floor number";
  skos:broader ble:Characteristic;
  skos:definition """The Floor Number characteristic describes in which
    floor the device is installed.""";
  skos:inScheme ble:Scheme;
  skos:prefLabel "Floor Number";
  skos:related ble:Broadcast, ble:FloorNumber, ble:Read, ble:ReliableWrite, ble:Write,
    ble:WriteWithoutResponse;
  prov:wasDerivedFrom <file:/data/lp/etl/executor/data/1651932367716-22-f5b1c2e0-1947-4a2e-a814-6ce401f2a604/working/working-outputfiles-33/gatt-xml-master/org.bluetooth.characteristic.floor_number.xml> .

<http://purl.org/wot-catalogue/ble/gatt#org.bluetooth.characteristic.altitude> a skos:Concept,
    ontolex:LexicalConcept, prov:Entity;
  skos:altLabel "altitude";
  skos:broader ble:Characteristic;
  skos:definition """The Altitude characteristic describes the altitude of
    the device.""";
  skos:inScheme ble:Scheme;
  skos:prefLabel "Altitude";
  skos:related ble:Altitude, ble:Broadcast, ble:Read, ble:ReliableWrite, ble:Write,
    ble:WriteWithoutResponse;
  prov:wasDerivedFrom <file:/data/lp/etl/executor/data/1651932367716-22-f5b1c2e0-1947-4a2e-a814-6ce401f2a604/working/working-outputfiles-33/gatt-xml-master/org.bluetooth.characteristic.altitude.xml> .

<http://purl.org/wot-catalogue/ble/gatt#org.bluetooth.characteristic.uncertainty>
  a skos:Concept, ontolex:LexicalConcept, prov:Entity;
  skos:altLabel "uncertainty";
  skos:broader ble:Characteristic;
  skos:definition """The Uncertainty characteristic describes the
    uncertainty of the location information the device
    exposes.""";
  skos:inScheme ble:Scheme;
  skos:prefLabel "Uncertainty";
  skos:related ble:Broadcast, ble:Read, ble:ReliableWrite, ble:Uncertainty, ble:Write,
    ble:WriteWithoutResponse;
  prov:wasDerivedFrom <file:/data/lp/etl/executor/data/1651932367716-22-f5b1c2e0-1947-4a2e-a814-6ce401f2a604/working/working-outputfiles-33/gatt-xml-master/org.bluetooth.characteristic.uncertainty.xml> .

<http://purl.org/wot-catalogue/ble/gatt#org.bluetooth.characteristic.location_name>
  a skos:Concept, ontolex:LexicalConcept, prov:Entity;
  skos:altLabel "location name";
  skos:broader ble:Characteristic;
  skos:definition """The Location Name characteristic describes the name
    of the location the device is installed in.""";
  skos:inScheme ble:Scheme;
  skos:prefLabel "Location Name";
  skos:related ble:Broadcast, ble:LocationName, ble:Read, ble:ReliableWrite, ble:Write,
    ble:WriteWithoutResponse;
  prov:wasDerivedFrom <file:/data/lp/etl/executor/data/1651932367716-22-f5b1c2e0-1947-4a2e-a814-6ce401f2a604/working/working-outputfiles-33/gatt-xml-master/org.bluetooth.characteristic.location_name.xml> .

<http://purl.org/wot-catalogue/ble/gatt#ReliableWrite> a skos:Concept;
  skos:altLabel "reliable write";
  skos:definition "Characteristic Value is written to a server when the client knows the Characteristic Value Handle, and assurance is required that the correct Characteristic Value is going to be written by transferring the Characteristic Value to be written in both directions before the write is performed.";
  skos:inScheme ble:Scheme;
  skos:prefLabel "Reliable Write" .

<http://purl.org/wot-catalogue/ble/gatt#org.bluetooth.characteristic.cycling_power_feature>
  a skos:Concept, ontolex:LexicalConcept, prov:Entity;
  skos:altLabel "cycling power feature";
  skos:broader ble:Characteristic;
  skos:definition """The CP Feature characteristic is used to report a list
    of features supported by the device.""";
  skos:inScheme ble:Scheme;
  skos:prefLabel "Cycling Power Feature";
  skos:related ble:CyclingPowerFeature, ble:Read;
  prov:wasDerivedFrom <file:/data/lp/etl/executor/data/1651932367716-22-f5b1c2e0-1947-4a2e-a814-6ce401f2a604/working/working-outputfiles-33/gatt-xml-master/org.bluetooth.characteristic.cycling_power_feature.xml> .

<http://purl.org/wot-catalogue/ble/gatt#CyclingPowerFeature> a skos:Concept, ontolex:LexicalConcept,
    prov:Entity;
  skos:altLabel "cycling power feature";
  skos:broader ble:Value;
  skos:inScheme ble:Scheme;
  skos:prefLabel "Cycling Power Feature";
  prov:wasDerivedFrom <file:/data/lp/etl/executor/data/1651932367716-22-f5b1c2e0-1947-4a2e-a814-6ce401f2a604/working/working-outputfiles-33/gatt-xml-master/org.bluetooth.characteristic.cycling_power_feature.xml> .

<http://purl.org/wot-catalogue/ble/gatt#CurrentSize> a skos:Concept, ontolex:LexicalConcept,
    prov:Entity;
  skos:altLabel "current size";
  skos:broader ble:Value;
  skos:inScheme ble:Scheme;
  skos:prefLabel "Current Size";
  prov:wasDerivedFrom <file:/data/lp/etl/executor/data/1651932367716-22-f5b1c2e0-1947-4a2e-a814-6ce401f2a604/working/working-outputfiles-33/gatt-xml-master/org.bluetooth.characteristic.object_size.xml> .

<http://purl.org/wot-catalogue/ble/gatt#AllocatedSize> a skos:Concept, ontolex:LexicalConcept,
    prov:Entity;
  skos:altLabel "allocated size";
  skos:broader ble:Value;
  skos:inScheme ble:Scheme;
  skos:prefLabel "Allocated Size";
  prov:wasDerivedFrom <file:/data/lp/etl/executor/data/1651932367716-22-f5b1c2e0-1947-4a2e-a814-6ce401f2a604/working/working-outputfiles-33/gatt-xml-master/org.bluetooth.characteristic.object_size.xml> .

<http://purl.org/wot-catalogue/ble/gatt#org.bluetooth.characteristic.measurement_interval>
  a skos:Concept, ontolex:LexicalConcept, prov:Entity;
  skos:altLabel "measurement interval";
  skos:broader ble:Characteristic;
  skos:definition """This characteristic is capable of representing values
    from 1 second to 65535 seconds which is equal to 18 hours, 12
    minutes and 15 seconds.""";
  skos:inScheme ble:Scheme;
  skos:prefLabel "Measurement Interval";
  skos:related ble:Indicate, ble:MeasurementInterval, ble:Read, ble:Write;
  prov:wasDerivedFrom <file:/data/lp/etl/executor/data/1651932367716-22-f5b1c2e0-1947-4a2e-a814-6ce401f2a604/working/working-outputfiles-33/gatt-xml-master/org.bluetooth.characteristic.measurement_interval.xml> .

<http://purl.org/wot-catalogue/ble/gatt#MeasurementInterval> a skos:Concept, ontolex:LexicalConcept,
    prov:Entity;
  skos:altLabel "measurement interval";
  skos:broader ble:Value;
  skos:inScheme ble:Scheme;
  skos:prefLabel "Measurement Interval";
  prov:wasDerivedFrom <file:/data/lp/etl/executor/data/1651932367716-22-f5b1c2e0-1947-4a2e-a814-6ce401f2a604/working/working-outputfiles-33/gatt-xml-master/org.bluetooth.characteristic.measurement_interval.xml> .

<http://purl.org/wot-catalogue/ble/gatt#181E> a skos:Concept, ontolex:LexicalConcept,
    prov:Entity;
  skos:altLabel "bond management service";
  skos:broader ble:Service;
  skos:definition """This service defines how a peer Bluetooth device can
    manage the storage of bond information, especially the deletion
    of it, on the Bluetooth device supporting this
    service.""";
  skos:inScheme ble:Scheme;
  skos:prefLabel "Bond Management Service";
  skos:related ble:org.bluetooth.characteristic.bond_management_control_point, ble:org.bluetooth.characteristic.bond_management_feature;
  prov:wasDerivedFrom <file:/data/lp/etl/executor/data/1651932367716-22-f5b1c2e0-1947-4a2e-a814-6ce401f2a604/working/working-outputfiles-33/gatt-xml-master/org.bluetooth.service.bond_management.xml> .

<http://purl.org/wot-catalogue/ble/gatt#org.bluetooth.characteristic.bond_management_control_point>
  a skos:Concept, ontolex:LexicalConcept, prov:Entity;
  skos:altLabel "bond management control point";
  skos:broader ble:Characteristic;
  skos:definition """This control point is used with a service to provide
    BMS specific functionality and the ability to manage bonds on
    the device. This includes functions like delete the bond
    information of the current connection or deletion of the whole
    bond information. The criterion in the Operand field is defined
    by the service that references this characteristic""";
  skos:inScheme ble:Scheme;
  skos:prefLabel "Bond Management Control Point";
  skos:related ble:OpCode, ble:Operand, ble:ReliableWrite, ble:Write;
  prov:wasDerivedFrom <file:/data/lp/etl/executor/data/1651932367716-22-f5b1c2e0-1947-4a2e-a814-6ce401f2a604/working/working-outputfiles-33/gatt-xml-master/org.bluetooth.characteristic.bond_management_control_point.xml> .

<http://purl.org/wot-catalogue/ble/gatt#org.bluetooth.characteristic.bond_management_feature>
  a skos:Concept, ontolex:LexicalConcept, prov:Entity;
  skos:altLabel "bond management features";
  skos:broader ble:Characteristic;
  skos:inScheme ble:Scheme;
  skos:prefLabel "Bond Management Features";
  skos:related ble:BondManagementFeatures, ble:Read;
  prov:wasDerivedFrom <file:/data/lp/etl/executor/data/1651932367716-22-f5b1c2e0-1947-4a2e-a814-6ce401f2a604/working/working-outputfiles-33/gatt-xml-master/org.bluetooth.characteristic.bond_management_feature.xml> .

<http://purl.org/wot-catalogue/ble/gatt#org.bluetooth.characteristic.fitness_machine_control_point>
  a skos:Concept, ontolex:LexicalConcept, prov:Entity;
  skos:altLabel "fitness machine control point";
  skos:broader ble:Characteristic;
  skos:definition """The Fitness Machine Control Point characteristic is
    defined in the Fitness Machine Service Specification.""";
  skos:inScheme ble:Scheme;
  skos:prefLabel "Fitness Machine Control Point";
  skos:related ble:Indicate, ble:Write;
  prov:wasDerivedFrom <file:/data/lp/etl/executor/data/1651932367716-22-f5b1c2e0-1947-4a2e-a814-6ce401f2a604/working/working-outputfiles-33/gatt-xml-master/org.bluetooth.characteristic.fitness_machine_control_point.xml> .

<http://purl.org/wot-catalogue/ble/gatt#1805> a skos:Concept, ontolex:LexicalConcept,
    prov:Entity;
  skos:altLabel "current time service";
  skos:broader ble:Service;
  skos:definition """Many Bluetooth devices have the ability to store and
    show time information. This service defines how a Bluetooth
    device can expose time information to other Bluetooth
    devices.""";
  skos:inScheme ble:Scheme;
  skos:prefLabel "Current Time Service";
  skos:related ble:org.bluetooth.characteristic.current_time, ble:org.bluetooth.characteristic.local_time_information,
    ble:org.bluetooth.characteristic.reference_time_information;
  prov:wasDerivedFrom <file:/data/lp/etl/executor/data/1651932367716-22-f5b1c2e0-1947-4a2e-a814-6ce401f2a604/working/working-outputfiles-33/gatt-xml-master/org.bluetooth.service.current_time.xml> .

<http://purl.org/wot-catalogue/ble/gatt#org.bluetooth.characteristic.current_time>
  a skos:Concept, ontolex:LexicalConcept, prov:Entity;
  skos:altLabel "current time";
  skos:broader ble:Characteristic;
  skos:inScheme ble:Scheme;
  skos:prefLabel "Current Time";
  skos:related ble:AdjustReason, ble:ExactTime256, ble:Notify, ble:Read, ble:Write;
  prov:wasDerivedFrom <file:/data/lp/etl/executor/data/1651932367716-22-f5b1c2e0-1947-4a2e-a814-6ce401f2a604/working/working-outputfiles-33/gatt-xml-master/org.bluetooth.characteristic.current_time.xml> .

<http://purl.org/wot-catalogue/ble/gatt#org.bluetooth.characteristic.local_time_information>
  a skos:Concept, ontolex:LexicalConcept, prov:Entity;
  skos:altLabel "local time information";
  skos:broader ble:Characteristic;
  skos:inScheme ble:Scheme;
  skos:prefLabel "Local Time Information";
  skos:related ble:DaylightSavingTime, ble:Read, ble:TimeZone, ble:Write;
  prov:wasDerivedFrom <file:/data/lp/etl/executor/data/1651932367716-22-f5b1c2e0-1947-4a2e-a814-6ce401f2a604/working/working-outputfiles-33/gatt-xml-master/org.bluetooth.characteristic.local_time_information.xml> .

<http://purl.org/wot-catalogue/ble/gatt#org.bluetooth.characteristic.reference_time_information>
  a skos:Concept, ontolex:LexicalConcept, prov:Entity;
  skos:altLabel "reference time information";
  skos:broader ble:Characteristic;
  skos:inScheme ble:Scheme;
  skos:prefLabel "Reference Time Information";
  skos:related ble:Accuracy, ble:DaysSinceUpdate, ble:HoursSinceUpdate, ble:Read, ble:Source;
  prov:wasDerivedFrom <file:/data/lp/etl/executor/data/1651932367716-22-f5b1c2e0-1947-4a2e-a814-6ce401f2a604/working/working-outputfiles-33/gatt-xml-master/org.bluetooth.characteristic.reference_time_information.xml> .

<http://purl.org/wot-catalogue/ble/gatt#org.bluetooth.characteristic.plx_spot_check_measurement>
  a skos:Concept, ontolex:LexicalConcept, prov:Entity;
  skos:altLabel "plx spot-check measurement";
  skos:broader ble:Characteristic;
  skos:definition """The PLX Spot-check Measurement characteristic, if
    supported, is used to send Spot-check measurements of SpO2
    (Percent oxygen saturation of hemoglobin) and PR (pulse rate).
    This characteristic is a variable length structure containing
    the Flags field, the SpO2PR-Spot-Check field, and depending on
    the contents of the Flags field, the Timestamp field, the
    Measurement Status field, the Device and Sensor Status field,
    and/or the Pulse Amplitude Index field.""";
  skos:inScheme ble:Scheme;
  skos:prefLabel "PLX Spot-Check Measurement";
  skos:related ble:DeviceandSensorStatus, ble:Flags, ble:Indicate, ble:InformationText,
    ble:MeasurementStatus, ble:PulseAmplitudeIndex, ble:SpO2PR-Spot-Check-PR, ble:SpO2PR-Spot-Check-SpO2,
    ble:Timestamp;
  prov:wasDerivedFrom <file:/data/lp/etl/executor/data/1651932367716-22-f5b1c2e0-1947-4a2e-a814-6ce401f2a604/working/working-outputfiles-33/gatt-xml-master/org.bluetooth.characteristic.plx_spot_check_measurement.xml> .

<http://purl.org/wot-catalogue/ble/gatt#SpO2PR-Spot-Check-SpO2> a skos:Concept, ontolex:LexicalConcept,
    prov:Entity;
  skos:altLabel "spo2pr-spot-check - spo2";
  skos:broader ble:Value;
  skos:definition """Unit is percentage with a resolution of
      1""";
  skos:inScheme ble:Scheme;
  skos:prefLabel "SpO2PR-Spot-Check - SpO2";
  prov:wasDerivedFrom <file:/data/lp/etl/executor/data/1651932367716-22-f5b1c2e0-1947-4a2e-a814-6ce401f2a604/working/working-outputfiles-33/gatt-xml-master/org.bluetooth.characteristic.plx_spot_check_measurement.xml> .

<http://purl.org/wot-catalogue/ble/gatt#SpO2PR-Spot-Check-PR> a skos:Concept, ontolex:LexicalConcept,
    prov:Entity;
  skos:altLabel "spo2pr-spot-check - pr";
  skos:broader ble:Value;
  skos:definition """Unit is beats per minute with a resolution
      of 1""";
  skos:inScheme ble:Scheme;
  skos:prefLabel "SpO2PR-Spot-Check - PR";
  prov:wasDerivedFrom <file:/data/lp/etl/executor/data/1651932367716-22-f5b1c2e0-1947-4a2e-a814-6ce401f2a604/working/working-outputfiles-33/gatt-xml-master/org.bluetooth.characteristic.plx_spot_check_measurement.xml> .

<http://purl.org/wot-catalogue/ble/gatt#Timestamp> a skos:Concept, ontolex:LexicalConcept,
    prov:Entity;
  skos:altLabel "timestamp";
  skos:broader ble:Value;
  skos:definition """Unit is smallest unit in seconds with a
      resolution of 1""";
  skos:inScheme ble:Scheme;
  skos:prefLabel "Timestamp";
  prov:wasDerivedFrom <file:/data/lp/etl/executor/data/1651932367716-22-f5b1c2e0-1947-4a2e-a814-6ce401f2a604/working/working-outputfiles-33/gatt-xml-master/org.bluetooth.characteristic.plx_spot_check_measurement.xml> .

<http://purl.org/wot-catalogue/ble/gatt#MeasurementStatus> a skos:Concept, ontolex:LexicalConcept,
    prov:Entity;
  skos:altLabel "measurement status";
  skos:broader ble:Value;
  skos:definition """C6: Field exists if the key of bit 4 of the
      Flags field is set to 1""";
  skos:inScheme ble:Scheme;
  skos:prefLabel "Measurement Status";
  prov:wasDerivedFrom <file:/data/lp/etl/executor/data/1651932367716-22-f5b1c2e0-1947-4a2e-a814-6ce401f2a604/working/working-outputfiles-33/gatt-xml-master/org.bluetooth.characteristic.blood_pressure_measurement.xml>,
    <file:/data/lp/etl/executor/data/1651932367716-22-f5b1c2e0-1947-4a2e-a814-6ce401f2a604/working/working-outputfiles-33/gatt-xml-master/org.bluetooth.characteristic.plx_continuous_measurement.xml>,
    <file:/data/lp/etl/executor/data/1651932367716-22-f5b1c2e0-1947-4a2e-a814-6ce401f2a604/working/working-outputfiles-33/gatt-xml-master/org.bluetooth.characteristic.plx_spot_check_measurement.xml> .

<http://purl.org/wot-catalogue/ble/gatt#DeviceandSensorStatus> a skos:Concept, ontolex:LexicalConcept,
    prov:Entity;
  skos:altLabel "device and sensor status";
  skos:broader ble:Value;
  skos:inScheme ble:Scheme;
  skos:prefLabel "Device and Sensor Status";
  prov:wasDerivedFrom <file:/data/lp/etl/executor/data/1651932367716-22-f5b1c2e0-1947-4a2e-a814-6ce401f2a604/working/working-outputfiles-33/gatt-xml-master/org.bluetooth.characteristic.plx_continuous_measurement.xml>,
    <file:/data/lp/etl/executor/data/1651932367716-22-f5b1c2e0-1947-4a2e-a814-6ce401f2a604/working/working-outputfiles-33/gatt-xml-master/org.bluetooth.characteristic.plx_spot_check_measurement.xml> .

<http://purl.org/wot-catalogue/ble/gatt#PulseAmplitudeIndex> a skos:Concept, ontolex:LexicalConcept,
    prov:Entity;
  skos:altLabel "pulse amplitude index";
  skos:broader ble:Value;
  skos:definition """Unit is percentage with a resolution of
      1""";
  skos:inScheme ble:Scheme;
  skos:prefLabel "Pulse Amplitude Index";
  prov:wasDerivedFrom <file:/data/lp/etl/executor/data/1651932367716-22-f5b1c2e0-1947-4a2e-a814-6ce401f2a604/working/working-outputfiles-33/gatt-xml-master/org.bluetooth.characteristic.plx_continuous_measurement.xml>,
    <file:/data/lp/etl/executor/data/1651932367716-22-f5b1c2e0-1947-4a2e-a814-6ce401f2a604/working/working-outputfiles-33/gatt-xml-master/org.bluetooth.characteristic.plx_spot_check_measurement.xml> .

<http://purl.org/wot-catalogue/ble/gatt#1824> a skos:Concept, ontolex:LexicalConcept,
    prov:Entity;
  skos:altLabel "transport discovery";
  skos:broader ble:Service;
  skos:definition """The Transport Discovery Service (TDS) enables a device
    using Bluetooth low energy wireless technology to expose
    services that are available on a transport other than Bluetooth
    low energy.""";
  skos:inScheme ble:Scheme;
  skos:prefLabel "Transport Discovery";
  skos:related ble:org.bluetooth.characteristic.tds_control_point;
  prov:wasDerivedFrom <file:/data/lp/etl/executor/data/1651932367716-22-f5b1c2e0-1947-4a2e-a814-6ce401f2a604/working/working-outputfiles-33/gatt-xml-master/org.bluetooth.service.transport_discovery.xml> .

<http://purl.org/wot-catalogue/ble/gatt#org.bluetooth.characteristic.tds_control_point>
  a skos:Concept, ontolex:LexicalConcept, prov:Entity;
  skos:altLabel "tds control point";
  skos:broader ble:Characteristic;
  skos:definition """The TDS Control Point characteristic is defined in the
    Transport Discovery Service, Section 4.1 and its
    sub-sections.""";
  skos:inScheme ble:Scheme;
  skos:prefLabel "TDS Control Point";
  skos:related ble:Indicate, ble:Write;
  prov:wasDerivedFrom <file:/data/lp/etl/executor/data/1651932367716-22-f5b1c2e0-1947-4a2e-a814-6ce401f2a604/working/working-outputfiles-33/gatt-xml-master/org.bluetooth.characteristic.tds_control_point.xml> .

<http://purl.org/wot-catalogue/ble/gatt#CumulativeValue> a skos:Concept, ontolex:LexicalConcept,
    prov:Entity;
  skos:altLabel "cumulative value";
  skos:broader ble:Value;
  skos:definition """Parameter Value for \"Set Cumulative Value\"
      Op Code""";
  skos:inScheme ble:Scheme;
  skos:prefLabel "Cumulative Value";
  prov:wasDerivedFrom <file:/data/lp/etl/executor/data/1651932367716-22-f5b1c2e0-1947-4a2e-a814-6ce401f2a604/working/working-outputfiles-33/gatt-xml-master/org.bluetooth.characteristic.sc_control_point.xml> .

<http://purl.org/wot-catalogue/ble/gatt#SensorLocationValue> a skos:Concept, ontolex:LexicalConcept,
    prov:Entity;
  skos:altLabel "sensor location value";
  skos:broader ble:Value;
  skos:definition """Parameter Value for \"Update Sensor Location\"
      Op Code""";
  skos:inScheme ble:Scheme;
  skos:prefLabel "Sensor Location Value";
  prov:wasDerivedFrom <file:/data/lp/etl/executor/data/1651932367716-22-f5b1c2e0-1947-4a2e-a814-6ce401f2a604/working/working-outputfiles-33/gatt-xml-master/org.bluetooth.characteristic.sc_control_point.xml> .

<http://purl.org/wot-catalogue/ble/gatt#RequestOpCode> a skos:Concept, ontolex:LexicalConcept,
    prov:Entity;
  skos:altLabel "request op code";
  skos:broader ble:Value;
  skos:definition """Parameter Value for \"Response Code\" Op
      Code""", """The Request Op Code is a sub field of the
      Parameter Value for \"Response Code\" Op Code. 
      C1: This Field is Mandatory for \"Response Code\" Op Code,
      otherwise this field is Excluded.""";
  skos:inScheme ble:Scheme;
  skos:prefLabel "Request Op Code";
  prov:wasDerivedFrom <file:/data/lp/etl/executor/data/1651932367716-22-f5b1c2e0-1947-4a2e-a814-6ce401f2a604/working/working-outputfiles-33/gatt-xml-master/org.bluetooth.characteristic.cycling_power_control_point.xml>,
    <file:/data/lp/etl/executor/data/1651932367716-22-f5b1c2e0-1947-4a2e-a814-6ce401f2a604/working/working-outputfiles-33/gatt-xml-master/org.bluetooth.characteristic.ln_control_point.xml>,
    <file:/data/lp/etl/executor/data/1651932367716-22-f5b1c2e0-1947-4a2e-a814-6ce401f2a604/working/working-outputfiles-33/gatt-xml-master/org.bluetooth.characteristic.sc_control_point.xml> .

<http://purl.org/wot-catalogue/ble/gatt#ResponseValue> a skos:Concept, ontolex:LexicalConcept,
    prov:Entity;
  skos:altLabel "response value";
  skos:broader ble:Value;
  skos:definition """Parameter Value for \"Response Code\" Op
      Code""", """The Response Value is a sub field of the
      Parameter Value for \"Response Code\" Op Code 
      C1: This Field is Mandatory for \"Response Code\" Op Code,
      otherwise this field is Excluded.""";
  skos:inScheme ble:Scheme;
  skos:prefLabel "Response Value";
  prov:wasDerivedFrom <file:/data/lp/etl/executor/data/1651932367716-22-f5b1c2e0-1947-4a2e-a814-6ce401f2a604/working/working-outputfiles-33/gatt-xml-master/org.bluetooth.characteristic.cycling_power_control_point.xml>,
    <file:/data/lp/etl/executor/data/1651932367716-22-f5b1c2e0-1947-4a2e-a814-6ce401f2a604/working/working-outputfiles-33/gatt-xml-master/org.bluetooth.characteristic.ln_control_point.xml>,
    <file:/data/lp/etl/executor/data/1651932367716-22-f5b1c2e0-1947-4a2e-a814-6ce401f2a604/working/working-outputfiles-33/gatt-xml-master/org.bluetooth.characteristic.sc_control_point.xml> .

<http://purl.org/wot-catalogue/ble/gatt#ResponseParameter> a skos:Concept, ontolex:LexicalConcept,
    prov:Entity;
  skos:altLabel "response parameter";
  skos:broader ble:Value;
  skos:definition """Parameter Value for \"Response Code\" Op
      Code""", """The Response Parameter is a sub field of the
      Parameter Value for \"Response Code\" Op Code. 
      C2:This Field is Optional for \"Response Code\" Op Code,
      otherwise this field is Excluded.""";
  skos:inScheme ble:Scheme;
  skos:prefLabel "Response Parameter";
  prov:wasDerivedFrom <file:/data/lp/etl/executor/data/1651932367716-22-f5b1c2e0-1947-4a2e-a814-6ce401f2a604/working/working-outputfiles-33/gatt-xml-master/org.bluetooth.characteristic.cycling_power_control_point.xml>,
    <file:/data/lp/etl/executor/data/1651932367716-22-f5b1c2e0-1947-4a2e-a814-6ce401f2a604/working/working-outputfiles-33/gatt-xml-master/org.bluetooth.characteristic.ln_control_point.xml>,
    <file:/data/lp/etl/executor/data/1651932367716-22-f5b1c2e0-1947-4a2e-a814-6ce401f2a604/working/working-outputfiles-33/gatt-xml-master/org.bluetooth.characteristic.sc_control_point.xml> .

<http://purl.org/wot-catalogue/ble/gatt#org.bluetooth.characteristic.resolvable_private_address_only>
  a skos:Concept, ontolex:LexicalConcept, prov:Entity;
  skos:altLabel "resolvable private address only";
  skos:broader ble:Characteristic;
  skos:definition """The Resolvable Private Address Only characteristic
    defines whether the device will only use Resolvable Private
    Addresses (RPAs) as local addresses.""";
  skos:inScheme ble:Scheme;
  skos:prefLabel "Resolvable Private Address Only";
  skos:related ble:ResolvablePrivateAddress;
  prov:wasDerivedFrom <file:/data/lp/etl/executor/data/1651932367716-22-f5b1c2e0-1947-4a2e-a814-6ce401f2a604/working/working-outputfiles-33/gatt-xml-master/org.bluetooth.characteristic.resolvable_private_address_only.xml> .

<http://purl.org/wot-catalogue/ble/gatt#ResolvablePrivateAddress> a skos:Concept,
    ontolex:LexicalConcept, prov:Entity;
  skos:altLabel "resolvable private address";
  skos:broader ble:Value;
  skos:inScheme ble:Scheme;
  skos:prefLabel "Resolvable Private Address";
  prov:wasDerivedFrom <file:/data/lp/etl/executor/data/1651932367716-22-f5b1c2e0-1947-4a2e-a814-6ce401f2a604/working/working-outputfiles-33/gatt-xml-master/org.bluetooth.characteristic.resolvable_private_address_only.xml> .

<http://purl.org/wot-catalogue/ble/gatt#org.bluetooth.characteristic.glucose_feature>
  a skos:Concept, ontolex:LexicalConcept, prov:Entity;
  skos:altLabel "glucose feature";
  skos:broader ble:Characteristic;
  skos:definition """The Glucose Feature characteristic is used to describe
    the supported features of the Server. When read, the Glucose
    Feature characteristic returns a value that is used by a Client
    to determine the supported features of the Server.""";
  skos:inScheme ble:Scheme;
  skos:prefLabel "Glucose Feature";
  skos:related ble:GlucoseFeature, ble:Read;
  prov:wasDerivedFrom <file:/data/lp/etl/executor/data/1651932367716-22-f5b1c2e0-1947-4a2e-a814-6ce401f2a604/working/working-outputfiles-33/gatt-xml-master/org.bluetooth.characteristic.glucose_feature.xml> .

<http://purl.org/wot-catalogue/ble/gatt#GlucoseFeature> a skos:Concept, ontolex:LexicalConcept,
    prov:Entity;
  skos:altLabel "glucose feature";
  skos:broader ble:Value;
  skos:inScheme ble:Scheme;
  skos:prefLabel "Glucose Feature";
  prov:wasDerivedFrom <file:/data/lp/etl/executor/data/1651932367716-22-f5b1c2e0-1947-4a2e-a814-6ce401f2a604/working/working-outputfiles-33/gatt-xml-master/org.bluetooth.characteristic.glucose_feature.xml> .

<http://purl.org/wot-catalogue/ble/gatt#RingerSetting> a skos:Concept, ontolex:LexicalConcept,
    prov:Entity;
  skos:altLabel "ringer setting";
  skos:broader ble:Value;
  skos:inScheme ble:Scheme;
  skos:prefLabel "Ringer Setting";
  prov:wasDerivedFrom <file:/data/lp/etl/executor/data/1651932367716-22-f5b1c2e0-1947-4a2e-a814-6ce401f2a604/working/working-outputfiles-33/gatt-xml-master/org.bluetooth.characteristic.ringer_setting.xml> .

<http://purl.org/wot-catalogue/ble/gatt#org.bluetooth.characteristic.aerobic_threshold>
  a skos:Concept, ontolex:LexicalConcept, prov:Entity;
  skos:altLabel "aerobic threshold";
  skos:broader ble:Characteristic;
  skos:definition "First metabolic threshold.";
  skos:inScheme ble:Scheme;
  skos:prefLabel "Aerobic Threshold";
  skos:related ble:AerobicThreshold, ble:Read, ble:Write;
  prov:wasDerivedFrom <file:/data/lp/etl/executor/data/1651932367716-22-f5b1c2e0-1947-4a2e-a814-6ce401f2a604/working/working-outputfiles-33/gatt-xml-master/org.bluetooth.characteristic.aerobic_threshold.xml> .

<http://purl.org/wot-catalogue/ble/gatt#AerobicThreshold> a skos:Concept, ontolex:LexicalConcept,
    prov:Entity;
  skos:altLabel "aerobic threshold";
  skos:broader ble:Value;
  skos:definition """The Unit is beats per minute with a
      resolution of 1""";
  skos:inScheme ble:Scheme;
  skos:prefLabel "Aerobic Threshold";
  prov:wasDerivedFrom <file:/data/lp/etl/executor/data/1651932367716-22-f5b1c2e0-1947-4a2e-a814-6ce401f2a604/working/working-outputfiles-33/gatt-xml-master/org.bluetooth.characteristic.aerobic_threshold.xml> .

<http://purl.org/wot-catalogue/ble/gatt#org.bluetooth.characteristic.cgm_feature>
  a skos:Concept, ontolex:LexicalConcept, prov:Entity;
  skos:altLabel "cgm feature";
  skos:broader ble:Characteristic;
  skos:inScheme ble:Scheme;
  skos:prefLabel "CGM Feature";
  skos:related ble:CGMFeature, ble:CGMSampleLocation, ble:CGMType, ble:E2E-CRC, ble:Read;
  prov:wasDerivedFrom <file:/data/lp/etl/executor/data/1651932367716-22-f5b1c2e0-1947-4a2e-a814-6ce401f2a604/working/working-outputfiles-33/gatt-xml-master/org.bluetooth.characteristic.cgm_feature.xml> .

<http://purl.org/wot-catalogue/ble/gatt#CGMFeature> a skos:Concept, ontolex:LexicalConcept,
    prov:Entity;
  skos:altLabel "cgm feature";
  skos:broader ble:Value;
  skos:definition "Byte Order - LSO...MSO";
  skos:inScheme ble:Scheme;
  skos:prefLabel "CGM Feature";
  prov:wasDerivedFrom <file:/data/lp/etl/executor/data/1651932367716-22-f5b1c2e0-1947-4a2e-a814-6ce401f2a604/working/working-outputfiles-33/gatt-xml-master/org.bluetooth.characteristic.cgm_feature.xml> .

<http://purl.org/wot-catalogue/ble/gatt#CGMType> a skos:Concept, ontolex:LexicalConcept,
    prov:Entity;
  skos:altLabel "cgm type";
  skos:broader ble:Value;
  skos:definition "See Note number 2 below.";
  skos:inScheme ble:Scheme;
  skos:prefLabel "CGM Type";
  prov:wasDerivedFrom <file:/data/lp/etl/executor/data/1651932367716-22-f5b1c2e0-1947-4a2e-a814-6ce401f2a604/working/working-outputfiles-33/gatt-xml-master/org.bluetooth.characteristic.cgm_feature.xml> .

<http://purl.org/wot-catalogue/ble/gatt#CGMSampleLocation> a skos:Concept, ontolex:LexicalConcept,
    prov:Entity;
  skos:altLabel "cgm sample location";
  skos:broader ble:Value;
  skos:definition "See Note number 2 below.";
  skos:inScheme ble:Scheme;
  skos:prefLabel "CGM Sample Location";
  prov:wasDerivedFrom <file:/data/lp/etl/executor/data/1651932367716-22-f5b1c2e0-1947-4a2e-a814-6ce401f2a604/working/working-outputfiles-33/gatt-xml-master/org.bluetooth.characteristic.cgm_feature.xml> .

<http://purl.org/wot-catalogue/ble/gatt#org.bluetooth.characteristic.model_number_string>
  a skos:Concept, ontolex:LexicalConcept, prov:Entity;
  skos:altLabel "model number string";
  skos:broader ble:Characteristic;
  skos:definition """The value of this characteristic is a UTF-8 string
    representing the model number assigned by the device
    vendor.""";
  skos:inScheme ble:Scheme;
  skos:prefLabel "Model Number String";
  skos:related ble:ModelNumber, ble:Read;
  prov:wasDerivedFrom <file:/data/lp/etl/executor/data/1651932367716-22-f5b1c2e0-1947-4a2e-a814-6ce401f2a604/working/working-outputfiles-33/gatt-xml-master/org.bluetooth.characteristic.model_number_string.xml> .

<http://purl.org/wot-catalogue/ble/gatt#ModelNumber> a skos:Concept, ontolex:LexicalConcept,
    prov:Entity;
  skos:altLabel "model number";
  skos:broader ble:Value;
  skos:definition "The Model Number String characteristic shall represent the model number that is assigned by the device vendor.";
  skos:inScheme ble:Scheme;
  skos:prefLabel "Model Number";
  skos:related ble:Read, xsd:string;
  prov:wasDerivedFrom <file:/data/lp/etl/executor/data/1651932367716-22-f5b1c2e0-1947-4a2e-a814-6ce401f2a604/working/working-outputfiles-33/gatt-xml-master/org.bluetooth.characteristic.model_number_string.xml> .

<http://purl.org/wot-catalogue/ble/gatt#org.bluetooth.characteristic.analog> a skos:Concept,
    ontolex:LexicalConcept, prov:Entity;
  skos:altLabel "analog";
  skos:broader ble:Characteristic;
  skos:definition """The Analog characteristic is used to read or write the
    value of one of the IO Module?s analog signals.""";
  skos:inScheme ble:Scheme;
  skos:prefLabel "Analog";
  skos:related ble:Analog, ble:Indicate, ble:Notify, ble:Read, ble:Write, ble:WriteWithoutResponse;
  prov:wasDerivedFrom <file:/data/lp/etl/executor/data/1651932367716-22-f5b1c2e0-1947-4a2e-a814-6ce401f2a604/working/working-outputfiles-33/gatt-xml-master/org.bluetooth.characteristic.analog.xml> .

<http://purl.org/wot-catalogue/ble/gatt#Analog> a skos:Concept, ontolex:LexicalConcept,
    prov:Entity;
  skos:altLabel "analog";
  skos:broader ble:Value;
  skos:inScheme ble:Scheme;
  skos:prefLabel "Analog";
  prov:wasDerivedFrom <file:/data/lp/etl/executor/data/1651932367716-22-f5b1c2e0-1947-4a2e-a814-6ce401f2a604/working/working-outputfiles-33/gatt-xml-master/org.bluetooth.characteristic.analog.xml> .

<http://purl.org/wot-catalogue/ble/gatt#1826> a skos:Concept, ontolex:LexicalConcept,
    prov:Entity;
  skos:altLabel "fitness machine";
  skos:broader ble:Service;
  skos:definition """The Fitness Machine Service (FTMS) exposes
    training-related data in the sports and fitness environment,
    which allows a Client to collect training data while a user is
    exercising with a fitness machine (Server).""";
  skos:inScheme ble:Scheme;
  skos:prefLabel "Fitness Machine";
  skos:related ble:org.bluetooth.characteristic.cross_trainer_data, ble:org.bluetooth.characteristic.fitness_machine_control_point,
    ble:org.bluetooth.characteristic.fitness_machine_feature, ble:org.bluetooth.characteristic.fitness_machine_status,
    ble:org.bluetooth.characteristic.indoor_bike_data, ble:org.bluetooth.characteristic.rower_data,
    ble:org.bluetooth.characteristic.stair_climber_data, ble:org.bluetooth.characteristic.step_climber_data,
    ble:org.bluetooth.characteristic.supported_heart_rate_range, ble:org.bluetooth.characteristic.supported_inclination_range,
    ble:org.bluetooth.characteristic.supported_power_range, ble:org.bluetooth.characteristic.supported_resistance_level_range,
    ble:org.bluetooth.characteristic.supported_speed_range, ble:org.bluetooth.characteristic.training_status,
    ble:org.bluetooth.characteristic.treadmill_data;
  prov:wasDerivedFrom <file:/data/lp/etl/executor/data/1651932367716-22-f5b1c2e0-1947-4a2e-a814-6ce401f2a604/working/working-outputfiles-33/gatt-xml-master/org.bluetooth.service.fitness_machine.xml> .

<http://purl.org/wot-catalogue/ble/gatt#org.bluetooth.characteristic.fitness_machine_feature>
  a skos:Concept, ontolex:LexicalConcept, prov:Entity;
  skos:altLabel "fitness machine feature";
  skos:broader ble:Characteristic;
  skos:definition """The Fitness Machine Feature characteristic is defined
    in the Fitness Machine Service Specification.""";
  skos:inScheme ble:Scheme;
  skos:prefLabel "Fitness Machine Feature";
  skos:related ble:Read;
  prov:wasDerivedFrom <file:/data/lp/etl/executor/data/1651932367716-22-f5b1c2e0-1947-4a2e-a814-6ce401f2a604/working/working-outputfiles-33/gatt-xml-master/org.bluetooth.characteristic.fitness_machine_feature.xml> .

<http://purl.org/wot-catalogue/ble/gatt#org.bluetooth.characteristic.treadmill_data>
  a skos:Concept, ontolex:LexicalConcept, prov:Entity;
  skos:altLabel "treadmill data";
  skos:broader ble:Characteristic;
  skos:definition """The Treadmill Data characteristic is used to send
    training-related data to the Client from a treadmill
    (Server).""";
  skos:inScheme ble:Scheme;
  skos:prefLabel "Treadmill Data";
  skos:related ble:AveragePace, ble:AverageSpeed, ble:ElapsedTime, ble:EnergyPerHour,
    ble:EnergyPerMinute, ble:Flags, ble:ForceonBelt, ble:HeartRate, ble:Inclination, ble:InstantaneousPace,
    ble:InstantaneousSpeed, ble:MetabolicEquivalent, ble:NegativeElevationGain, ble:Notify,
    ble:PositiveElevationGain, ble:PowerOutput, ble:RampAngleSetting, ble:RemainingTime,
    ble:TotalDistance, ble:TotalEnergy;
  prov:wasDerivedFrom <file:/data/lp/etl/executor/data/1651932367716-22-f5b1c2e0-1947-4a2e-a814-6ce401f2a604/working/working-outputfiles-33/gatt-xml-master/org.bluetooth.characteristic.treadmill_data.xml> .

<http://purl.org/wot-catalogue/ble/gatt#org.bluetooth.characteristic.step_climber_data>
  a skos:Concept, ontolex:LexicalConcept, prov:Entity;
  skos:altLabel "step climber data";
  skos:broader ble:Characteristic;
  skos:definition """The Step Climber Data characteristic is used to send
    training-related data to the Client from a step climber
    (Server).""";
  skos:inScheme ble:Scheme;
  skos:prefLabel "Step Climber Data";
  skos:related ble:AverageStepRate, ble:ElapsedTime, ble:EnergyPerHour, ble:EnergyPerMinute,
    ble:Flags, ble:Floors, ble:HeartRate, ble:MetabolicEquivalent, ble:Notify, ble:PositiveElevationGain,
    ble:RemainingTime, ble:StepCount, ble:StepPerMinute, ble:TotalEnergy;
  prov:wasDerivedFrom <file:/data/lp/etl/executor/data/1651932367716-22-f5b1c2e0-1947-4a2e-a814-6ce401f2a604/working/working-outputfiles-33/gatt-xml-master/org.bluetooth.characteristic.step_climber_data.xml> .

<http://purl.org/wot-catalogue/ble/gatt#org.bluetooth.characteristic.stair_climber_data>
  a skos:Concept, ontolex:LexicalConcept, prov:Entity;
  skos:altLabel "stair climber data";
  skos:broader ble:Characteristic;
  skos:definition """The Stair Climber Data characteristic is used to send
    training-related data to the Client from a stair climber
    (Server).""";
  skos:inScheme ble:Scheme;
  skos:prefLabel "Stair Climber Data";
  skos:related ble:AverageStepRate, ble:ElapsedTime, ble:EnergyPerHour, ble:EnergyPerMinute,
    ble:Flags, ble:Floors, ble:HeartRate, ble:MetabolicEquivalent, ble:Notify, ble:PositiveElevationGain,
    ble:RemainingTime, ble:StepPerMinute, ble:StrideCount, ble:TotalEnergy;
  prov:wasDerivedFrom <file:/data/lp/etl/executor/data/1651932367716-22-f5b1c2e0-1947-4a2e-a814-6ce401f2a604/working/working-outputfiles-33/gatt-xml-master/org.bluetooth.characteristic.stair_climber_data.xml> .

<http://purl.org/wot-catalogue/ble/gatt#org.bluetooth.characteristic.rower_data> a
    skos:Concept, ontolex:LexicalConcept, prov:Entity;
  skos:altLabel "rower data";
  skos:broader ble:Characteristic;
  skos:definition """The Rower Data characteristic is used to send
    training-related data to the Client from a rower
    (Server).""";
  skos:inScheme ble:Scheme;
  skos:prefLabel "Rower Data";
  skos:related ble:AveragePace, ble:AveragePower, ble:AverageStrokeRate, ble:ElapsedTime,
    ble:EnergyPerHour, ble:EnergyPerMinute, ble:Flags, ble:HeartRate, ble:InstantaneousPace,
    ble:InstantaneousPower, ble:MetabolicEquivalent, ble:Notify, ble:RemainingTime, ble:ResistanceLevel,
    ble:StrokeCount, ble:StrokeRate, ble:TotalDistance, ble:TotalEnergy;
  prov:wasDerivedFrom <file:/data/lp/etl/executor/data/1651932367716-22-f5b1c2e0-1947-4a2e-a814-6ce401f2a604/working/working-outputfiles-33/gatt-xml-master/org.bluetooth.characteristic.rower_data.xml> .

<http://purl.org/wot-catalogue/ble/gatt#org.bluetooth.characteristic.indoor_bike_data>
  a skos:Concept, ontolex:LexicalConcept, prov:Entity;
  skos:altLabel "indoor bike data";
  skos:broader ble:Characteristic;
  skos:definition """The Indoor Bike Data characteristic is used to send
    training-related data to the Client from an indoor bike
    (Server).""";
  skos:inScheme ble:Scheme;
  skos:prefLabel "Indoor Bike Data";
  skos:related ble:AverageCadence, ble:AveragePower, ble:AverageSpeed, ble:ElapsedTime,
    ble:EnergyPerHour, ble:EnergyPerMinute, ble:Flags, ble:HeartRate, ble:InstantaneousCadence,
    ble:InstantaneousPower, ble:InstantaneousSpeed, ble:MetabolicEquivalent, ble:Notify,
    ble:RemainingTime, ble:ResistanceLevel, ble:TotalDistance, ble:TotalEnergy;
  prov:wasDerivedFrom <file:/data/lp/etl/executor/data/1651932367716-22-f5b1c2e0-1947-4a2e-a814-6ce401f2a604/working/working-outputfiles-33/gatt-xml-master/org.bluetooth.characteristic.indoor_bike_data.xml> .

<http://purl.org/wot-catalogue/ble/gatt#org.bluetooth.characteristic.training_status>
  a skos:Concept, ontolex:LexicalConcept, prov:Entity;
  skos:altLabel "training status";
  skos:broader ble:Characteristic;
  skos:definition """The Training Status characteristic is defined in the
    Fitness Machine Service Specification.""";
  skos:inScheme ble:Scheme;
  skos:prefLabel "Training Status";
  skos:related ble:Notify, ble:Read;
  prov:wasDerivedFrom <file:/data/lp/etl/executor/data/1651932367716-22-f5b1c2e0-1947-4a2e-a814-6ce401f2a604/working/working-outputfiles-33/gatt-xml-master/org.bluetooth.characteristic.training_status.xml> .

<http://purl.org/wot-catalogue/ble/gatt#org.bluetooth.characteristic.supported_inclination_range>
  a skos:Concept, ontolex:LexicalConcept, prov:Entity;
  skos:altLabel "supported inclination range";
  skos:broader ble:Characteristic;
  skos:definition """The Supported Inclination Range characteristic is used
    to send the supported inclination range as well as the minimum
    inclination increment supported by the Server.""";
  skos:inScheme ble:Scheme;
  skos:prefLabel "Supported Inclination Range";
  skos:related ble:InformationText, ble:MaximumInclination, ble:MinimumInclination,
    ble:MinimumIncrement, ble:Read;
  prov:wasDerivedFrom <file:/data/lp/etl/executor/data/1651932367716-22-f5b1c2e0-1947-4a2e-a814-6ce401f2a604/working/working-outputfiles-33/gatt-xml-master/org.bluetooth.characteristic.supported_inclination_range.xml> .

<http://purl.org/wot-catalogue/ble/gatt#org.bluetooth.characteristic.supported_resistance_level_range>
  a skos:Concept, ontolex:LexicalConcept, prov:Entity;
  skos:altLabel "supported resistance level range";
  skos:broader ble:Characteristic;
  skos:definition """The Supported Resistance Level Range characteristic is
    used to send the supported resistance level range as well as
    the minimum resistance increment supported by the
    Server.""";
  skos:inScheme ble:Scheme;
  skos:prefLabel "Supported Resistance Level Range";
  skos:related ble:InformationText, ble:MaximumResistanceLevel, ble:MinimumIncrement,
    ble:MinimumResistanceLevel, ble:Read;
  prov:wasDerivedFrom <file:/data/lp/etl/executor/data/1651932367716-22-f5b1c2e0-1947-4a2e-a814-6ce401f2a604/working/working-outputfiles-33/gatt-xml-master/org.bluetooth.characteristic.supported_resistance_level_range.xml> .

<http://purl.org/wot-catalogue/ble/gatt#org.bluetooth.characteristic.supported_power_range>
  a skos:Concept, ontolex:LexicalConcept, prov:Entity;
  skos:altLabel "supported power range";
  skos:broader ble:Characteristic;
  skos:definition """The Supported Power Range characteristic is used to
    send the supported power range as well as the minimum power
    increment supported by the Server.""";
  skos:inScheme ble:Scheme;
  skos:prefLabel "Supported Power Range";
  skos:related ble:InformationText, ble:MaximumPower, ble:MinimumIncrement, ble:MinimumPower,
    ble:Read;
  prov:wasDerivedFrom <file:/data/lp/etl/executor/data/1651932367716-22-f5b1c2e0-1947-4a2e-a814-6ce401f2a604/working/working-outputfiles-33/gatt-xml-master/org.bluetooth.characteristic.supported_power_range.xml> .

<http://purl.org/wot-catalogue/ble/gatt#org.bluetooth.characteristic.supported_heart_rate_range>
  a skos:Concept, ontolex:LexicalConcept, prov:Entity;
  skos:altLabel "supported heart rate range";
  skos:broader ble:Characteristic;
  skos:definition """The Supported Heart Rate Range characteristic is used
    to send the supported Heart Rate range as well as the minimum
    Heart Rate increment supported by the Server.""";
  skos:inScheme ble:Scheme;
  skos:prefLabel "Supported Heart Rate Range";
  skos:related ble:InformationText, ble:MaximumHeartRate, ble:MinimumHeartRate, ble:MinimumIncrement,
    ble:Read;
  prov:wasDerivedFrom <file:/data/lp/etl/executor/data/1651932367716-22-f5b1c2e0-1947-4a2e-a814-6ce401f2a604/working/working-outputfiles-33/gatt-xml-master/org.bluetooth.characteristic.supported_heart_rate_range.xml> .

<http://purl.org/wot-catalogue/ble/gatt#org.bluetooth.characteristic.fitness_machine_status>
  a skos:Concept, ontolex:LexicalConcept, prov:Entity;
  skos:altLabel "fitness machine status";
  skos:broader ble:Characteristic;
  skos:definition """The Fitness Machine Status characteristic is defined
    in the Fitness Machine Service Specification.""";
  skos:inScheme ble:Scheme;
  skos:prefLabel "Fitness Machine Status";
  skos:related ble:InformationText, ble:Notify;
  prov:wasDerivedFrom <file:/data/lp/etl/executor/data/1651932367716-22-f5b1c2e0-1947-4a2e-a814-6ce401f2a604/working/working-outputfiles-33/gatt-xml-master/org.bluetooth.characteristic.fitness_machine_status.xml> .

<http://purl.org/wot-catalogue/ble/gatt#org.bluetooth.characteristic.apparent_wind_speed>
  a skos:Concept, ontolex:LexicalConcept, prov:Entity;
  skos:altLabel "apparent wind speed";
  skos:broader ble:Characteristic;
  skos:inScheme ble:Scheme;
  skos:prefLabel "Apparent Wind Speed";
  skos:related ble:ApparentWindSpeed, ble:ExtendedProperties, ble:Notify, ble:Read,
    ble:WritableAuxiliaries;
  prov:wasDerivedFrom <file:/data/lp/etl/executor/data/1651932367716-22-f5b1c2e0-1947-4a2e-a814-6ce401f2a604/working/working-outputfiles-33/gatt-xml-master/org.bluetooth.characteristic.apparent_wind_speed.xml> .

<http://purl.org/wot-catalogue/ble/gatt#ApparentWindSpeed> a skos:Concept, ontolex:LexicalConcept,
    prov:Entity;
  skos:altLabel "apparent wind speed";
  skos:broader ble:Value;
  skos:definition """Unit is in meters per second with a
      resolution of 0.01 m/s""";
  skos:inScheme ble:Scheme;
  skos:prefLabel "Apparent Wind Speed";
  prov:wasDerivedFrom <file:/data/lp/etl/executor/data/1651932367716-22-f5b1c2e0-1947-4a2e-a814-6ce401f2a604/working/working-outputfiles-33/gatt-xml-master/org.bluetooth.characteristic.apparent_wind_speed.xml> .

<http://purl.org/wot-catalogue/ble/gatt#LocationName> a skos:Concept, ontolex:LexicalConcept,
    prov:Entity;
  skos:altLabel "location name";
  skos:broader ble:Value;
  skos:inScheme ble:Scheme;
  skos:prefLabel "Location Name";
  prov:wasDerivedFrom <file:/data/lp/etl/executor/data/1651932367716-22-f5b1c2e0-1947-4a2e-a814-6ce401f2a604/working/working-outputfiles-33/gatt-xml-master/org.bluetooth.characteristic.location_name.xml> .

<http://purl.org/wot-catalogue/ble/gatt#org.bluetooth.characteristic.csc_feature>
  a skos:Concept, ontolex:LexicalConcept, prov:Entity;
  skos:altLabel "csc feature";
  skos:broader ble:Characteristic;
  skos:definition """The CSC (Cycling Speed and Cadence) Feature
    characteristic is used to describe the supported features of
    the Server.""";
  skos:inScheme ble:Scheme;
  skos:prefLabel "CSC Feature";
  skos:related ble:CSCFeature, ble:Read;
  prov:wasDerivedFrom <file:/data/lp/etl/executor/data/1651932367716-22-f5b1c2e0-1947-4a2e-a814-6ce401f2a604/working/working-outputfiles-33/gatt-xml-master/org.bluetooth.characteristic.csc_feature.xml> .

<http://purl.org/wot-catalogue/ble/gatt#CSCFeature> a skos:Concept, ontolex:LexicalConcept,
    prov:Entity;
  skos:altLabel "csc feature";
  skos:broader ble:Value;
  skos:inScheme ble:Scheme;
  skos:prefLabel "CSC Feature";
  prov:wasDerivedFrom <file:/data/lp/etl/executor/data/1651932367716-22-f5b1c2e0-1947-4a2e-a814-6ce401f2a604/working/working-outputfiles-33/gatt-xml-master/org.bluetooth.characteristic.csc_feature.xml> .

<http://purl.org/wot-catalogue/ble/gatt#org.bluetooth.characteristic.uv_index> a skos:Concept,
    ontolex:LexicalConcept, prov:Entity;
  skos:altLabel "uv index";
  skos:broader ble:Characteristic;
  skos:inScheme ble:Scheme;
  skos:prefLabel "UV Index";
  skos:related ble:ExtendedProperties, ble:Notify, ble:Read, ble:UVIndex, ble:WritableAuxiliaries;
  prov:wasDerivedFrom <file:/data/lp/etl/executor/data/1651932367716-22-f5b1c2e0-1947-4a2e-a814-6ce401f2a604/working/working-outputfiles-33/gatt-xml-master/org.bluetooth.characteristic.uv_index.xml> .

<http://purl.org/wot-catalogue/ble/gatt#UVIndex> a skos:Concept, ontolex:LexicalConcept,
    prov:Entity;
  skos:altLabel "uv index";
  skos:broader ble:Value;
  skos:inScheme ble:Scheme;
  skos:prefLabel "UV Index";
  prov:wasDerivedFrom <file:/data/lp/etl/executor/data/1651932367716-22-f5b1c2e0-1947-4a2e-a814-6ce401f2a604/working/working-outputfiles-33/gatt-xml-master/org.bluetooth.characteristic.uv_index.xml> .

<http://purl.org/wot-catalogue/ble/gatt#org.bluetooth.characteristic.first_name> a
    skos:Concept, ontolex:LexicalConcept, prov:Entity;
  skos:altLabel "first name";
  skos:broader ble:Characteristic;
  skos:definition "First name of the user. See Note below.";
  skos:inScheme ble:Scheme;
  skos:prefLabel "First Name";
  skos:related ble:FirstName, ble:Read, ble:Write;
  prov:wasDerivedFrom <file:/data/lp/etl/executor/data/1651932367716-22-f5b1c2e0-1947-4a2e-a814-6ce401f2a604/working/working-outputfiles-33/gatt-xml-master/org.bluetooth.characteristic.first_name.xml> .

<http://purl.org/wot-catalogue/ble/gatt#FirstName> a skos:Concept, ontolex:LexicalConcept,
    prov:Entity;
  skos:altLabel "first name";
  skos:broader ble:Value;
  skos:inScheme ble:Scheme;
  skos:prefLabel "First Name";
  prov:wasDerivedFrom <file:/data/lp/etl/executor/data/1651932367716-22-f5b1c2e0-1947-4a2e-a814-6ce401f2a604/working/working-outputfiles-33/gatt-xml-master/org.bluetooth.characteristic.first_name.xml> .

<http://purl.org/wot-catalogue/ble/gatt#HTTPEntityBody> a skos:Concept, ontolex:LexicalConcept,
    prov:Entity;
  skos:altLabel "http entity body";
  skos:broader ble:Value;
  skos:definition """The HTTP entity body used in the HTTP
      request.""";
  skos:inScheme ble:Scheme;
  skos:prefLabel "HTTP Entity Body";
  prov:wasDerivedFrom <file:/data/lp/etl/executor/data/1651932367716-22-f5b1c2e0-1947-4a2e-a814-6ce401f2a604/working/working-outputfiles-33/gatt-xml-master/org.bluetooth.characteristic.http_entity_body.xml> .

<http://purl.org/wot-catalogue/ble/gatt#org.bluetooth.characteristic.time_zone> a
    skos:Concept, ontolex:LexicalConcept, prov:Entity;
  skos:altLabel "time zone";
  skos:broader ble:Characteristic;
  skos:inScheme ble:Scheme;
  skos:prefLabel "Time Zone";
  skos:related ble:TimeZone;
  prov:wasDerivedFrom <file:/data/lp/etl/executor/data/1651932367716-22-f5b1c2e0-1947-4a2e-a814-6ce401f2a604/working/working-outputfiles-33/gatt-xml-master/org.bluetooth.characteristic.time_zone.xml> .

<http://purl.org/wot-catalogue/ble/gatt#TimeZone> a skos:Concept, ontolex:LexicalConcept,
    prov:Entity;
  skos:altLabel "time zone";
  skos:broader ble:Value;
  skos:definition """Same format as the Time Zone
      Characteristic""";
  skos:inScheme ble:Scheme;
  skos:prefLabel "Time Zone";
  prov:wasDerivedFrom <file:/data/lp/etl/executor/data/1651932367716-22-f5b1c2e0-1947-4a2e-a814-6ce401f2a604/working/working-outputfiles-33/gatt-xml-master/org.bluetooth.characteristic.cgm_session_start_time.xml>,
    <file:/data/lp/etl/executor/data/1651932367716-22-f5b1c2e0-1947-4a2e-a814-6ce401f2a604/working/working-outputfiles-33/gatt-xml-master/org.bluetooth.characteristic.local_time_information.xml>,
    <file:/data/lp/etl/executor/data/1651932367716-22-f5b1c2e0-1947-4a2e-a814-6ce401f2a604/working/working-outputfiles-33/gatt-xml-master/org.bluetooth.characteristic.time_zone.xml> .

<http://purl.org/wot-catalogue/ble/gatt#org.bluetooth.characteristic.cgm_specific_ops_control_point>
  a skos:Concept, ontolex:LexicalConcept, prov:Entity;
  skos:altLabel "cgm specific ops control point";
  skos:broader ble:Characteristic;
  skos:definition """The CGM Specific Ops Control Point encapsulates all
    functionality and mechanisms that are unique to a CGM-device.
    This control point is used with a service to provide CGM
    specific functionality and the ability to change CGM specific
    settings of the device. This includes functions like setting
    the CGM Communication Interval or the sending a calibration
    value to the device. The criterion in the Operand field is
    defined by the service that references this
    characteristic""";
  skos:inScheme ble:Scheme;
  skos:prefLabel "CGM Specific Ops Control Point";
  skos:related ble:CalibrationValue-CalibrationDataRecordNumber, ble:CalibrationValue-CalibrationSampleLocation,
    ble:CalibrationValue-CalibrationStatus, ble:CalibrationValue-CalibrationTime, ble:CalibrationValue-CalibrationType,
    ble:CalibrationValue-GlucoseConcentrationofCalibration, ble:CalibrationValue-NextCalibrationTime,
    ble:E2E-CRC, ble:Indicate, ble:OpCode, ble:OpCode-ResponseCodes, ble:Operand, ble:Write;
  prov:wasDerivedFrom <file:/data/lp/etl/executor/data/1651932367716-22-f5b1c2e0-1947-4a2e-a814-6ce401f2a604/working/working-outputfiles-33/gatt-xml-master/org.bluetooth.characteristic.cgm_specific_ops_control_point.xml> .

<http://purl.org/wot-catalogue/ble/gatt#OpCode-ResponseCodes> a skos:Concept, ontolex:LexicalConcept,
    prov:Entity;
  skos:altLabel "op code - response codes";
  skos:broader ble:Value;
  skos:inScheme ble:Scheme;
  skos:prefLabel "Op Code - Response Codes";
  prov:wasDerivedFrom <file:/data/lp/etl/executor/data/1651932367716-22-f5b1c2e0-1947-4a2e-a814-6ce401f2a604/working/working-outputfiles-33/gatt-xml-master/org.bluetooth.characteristic.cgm_specific_ops_control_point.xml> .

<http://purl.org/wot-catalogue/ble/gatt#CalibrationValue-GlucoseConcentrationofCalibration>
  a skos:Concept, ontolex:LexicalConcept, prov:Entity;
  skos:altLabel "calibration value - glucose concentration of calibration";
  skos:broader ble:Value;
  skos:definition "See Note number 2 below.";
  skos:inScheme ble:Scheme;
  skos:prefLabel "Calibration Value - Glucose Concentration of Calibration";
  prov:wasDerivedFrom <file:/data/lp/etl/executor/data/1651932367716-22-f5b1c2e0-1947-4a2e-a814-6ce401f2a604/working/working-outputfiles-33/gatt-xml-master/org.bluetooth.characteristic.cgm_specific_ops_control_point.xml> .

<http://purl.org/wot-catalogue/ble/gatt#CalibrationValue-CalibrationTime> a skos:Concept,
    ontolex:LexicalConcept, prov:Entity;
  skos:altLabel "calibration value - calibration time";
  skos:broader ble:Value;
  skos:definition "See Note number 2 below.";
  skos:inScheme ble:Scheme;
  skos:prefLabel "Calibration Value - Calibration Time";
  prov:wasDerivedFrom <file:/data/lp/etl/executor/data/1651932367716-22-f5b1c2e0-1947-4a2e-a814-6ce401f2a604/working/working-outputfiles-33/gatt-xml-master/org.bluetooth.characteristic.cgm_specific_ops_control_point.xml> .

<http://purl.org/wot-catalogue/ble/gatt#CalibrationValue-CalibrationType> a skos:Concept,
    ontolex:LexicalConcept, prov:Entity;
  skos:altLabel "calibration value - calibration type";
  skos:broader ble:Value;
  skos:definition "See Note number 2 below.";
  skos:inScheme ble:Scheme;
  skos:prefLabel "Calibration Value - Calibration Type";
  prov:wasDerivedFrom <file:/data/lp/etl/executor/data/1651932367716-22-f5b1c2e0-1947-4a2e-a814-6ce401f2a604/working/working-outputfiles-33/gatt-xml-master/org.bluetooth.characteristic.cgm_specific_ops_control_point.xml> .

<http://purl.org/wot-catalogue/ble/gatt#CalibrationValue-CalibrationSampleLocation>
  a skos:Concept, ontolex:LexicalConcept, prov:Entity;
  skos:altLabel "calibration value - calibration sample location";
  skos:broader ble:Value;
  skos:definition "See Note number 2 below.";
  skos:inScheme ble:Scheme;
  skos:prefLabel "Calibration Value - Calibration Sample Location";
  prov:wasDerivedFrom <file:/data/lp/etl/executor/data/1651932367716-22-f5b1c2e0-1947-4a2e-a814-6ce401f2a604/working/working-outputfiles-33/gatt-xml-master/org.bluetooth.characteristic.cgm_specific_ops_control_point.xml> .

<http://purl.org/wot-catalogue/ble/gatt#CalibrationValue-NextCalibrationTime> a skos:Concept,
    ontolex:LexicalConcept, prov:Entity;
  skos:altLabel "calibration value - next calibration time";
  skos:broader ble:Value;
  skos:definition "See Note number 2 below.";
  skos:inScheme ble:Scheme;
  skos:prefLabel "Calibration Value - Next Calibration Time";
  prov:wasDerivedFrom <file:/data/lp/etl/executor/data/1651932367716-22-f5b1c2e0-1947-4a2e-a814-6ce401f2a604/working/working-outputfiles-33/gatt-xml-master/org.bluetooth.characteristic.cgm_specific_ops_control_point.xml> .

<http://purl.org/wot-catalogue/ble/gatt#CalibrationValue-CalibrationDataRecordNumber>
  a skos:Concept, ontolex:LexicalConcept, prov:Entity;
  skos:altLabel "calibration value - calibration data record number";
  skos:broader ble:Value;
  skos:definition "See Note number 2 below.";
  skos:inScheme ble:Scheme;
  skos:prefLabel "Calibration Value - Calibration Data Record Number";
  prov:wasDerivedFrom <file:/data/lp/etl/executor/data/1651932367716-22-f5b1c2e0-1947-4a2e-a814-6ce401f2a604/working/working-outputfiles-33/gatt-xml-master/org.bluetooth.characteristic.cgm_specific_ops_control_point.xml> .

<http://purl.org/wot-catalogue/ble/gatt#CalibrationValue-CalibrationStatus> a skos:Concept,
    ontolex:LexicalConcept, prov:Entity;
  skos:altLabel "calibration value - calibration status";
  skos:broader ble:Value;
  skos:definition "See Note number 2 below.";
  skos:inScheme ble:Scheme;
  skos:prefLabel "Calibration Value - Calibration Status";
  prov:wasDerivedFrom <file:/data/lp/etl/executor/data/1651932367716-22-f5b1c2e0-1947-4a2e-a814-6ce401f2a604/working/working-outputfiles-33/gatt-xml-master/org.bluetooth.characteristic.cgm_specific_ops_control_point.xml> .

<http://purl.org/wot-catalogue/ble/gatt#org.bluetooth.characteristic.dew_point> a
    skos:Concept, ontolex:LexicalConcept, prov:Entity;
  skos:altLabel "dew point";
  skos:broader ble:Characteristic;
  skos:inScheme ble:Scheme;
  skos:prefLabel "Dew Point";
  skos:related ble:DewPoint, ble:ExtendedProperties, ble:Notify, ble:Read, ble:WritableAuxiliaries;
  prov:wasDerivedFrom <file:/data/lp/etl/executor/data/1651932367716-22-f5b1c2e0-1947-4a2e-a814-6ce401f2a604/working/working-outputfiles-33/gatt-xml-master/org.bluetooth.characteristic.dew_point.xml> .

<http://purl.org/wot-catalogue/ble/gatt#DewPoint> a skos:Concept, ontolex:LexicalConcept,
    prov:Entity;
  skos:altLabel "dew point";
  skos:broader ble:Value;
  skos:definition """Unit is in degrees celsius with a resolution
      of 1 degree Celsius""";
  skos:inScheme ble:Scheme;
  skos:prefLabel "Dew Point";
  prov:wasDerivedFrom <file:/data/lp/etl/executor/data/1651932367716-22-f5b1c2e0-1947-4a2e-a814-6ce401f2a604/working/working-outputfiles-33/gatt-xml-master/org.bluetooth.characteristic.dew_point.xml> .

<http://purl.org/wot-catalogue/ble/gatt#1813> a skos:Concept, ontolex:LexicalConcept,
    prov:Entity;
  skos:altLabel "scan parameters";
  skos:broader ble:Service;
  skos:definition """The Scan Parameters Service enables a GATT Server
    device to expose a characteristic for the GATT Client to write
    its scan interval and scan window on the GATT Server
    device.""";
  skos:inScheme ble:Scheme;
  skos:prefLabel "Scan Parameters";
  skos:related ble:org.bluetooth.characteristic.scan_interval_window, ble:org.bluetooth.characteristic.scan_refresh;
  prov:wasDerivedFrom <file:/data/lp/etl/executor/data/1651932367716-22-f5b1c2e0-1947-4a2e-a814-6ce401f2a604/working/working-outputfiles-33/gatt-xml-master/org.bluetooth.service.scan_parameters.xml> .

<http://purl.org/wot-catalogue/ble/gatt#org.bluetooth.characteristic.scan_interval_window>
  a skos:Concept, ontolex:LexicalConcept, prov:Entity;
  skos:altLabel "scan interval window";
  skos:broader ble:Characteristic;
  skos:definition """The Scan Interval Window characteristic is used to
    store the scan parameters of the GATT Client. The GATT Server
    can use these values to optimize its own advertisement rate and
    to minimize the rate of its own advertisements while also
    minimizing the latency of reconnections.""";
  skos:inScheme ble:Scheme;
  skos:prefLabel "Scan Interval Window";
  skos:related ble:LE_Scan_Interval, ble:LE_Scan_Window, ble:WriteWithoutResponse;
  prov:wasDerivedFrom <file:/data/lp/etl/executor/data/1651932367716-22-f5b1c2e0-1947-4a2e-a814-6ce401f2a604/working/working-outputfiles-33/gatt-xml-master/org.bluetooth.characteristic.scan_interval_window.xml> .

<http://purl.org/wot-catalogue/ble/gatt#org.bluetooth.characteristic.scan_refresh>
  a skos:Concept, ontolex:LexicalConcept, prov:Entity;
  skos:altLabel "scan refresh";
  skos:broader ble:Characteristic;
  skos:definition """The Scan Refresh characteristic is used to notify the
    Client that the Server requires the Scan Interval Window
    characteristic to be written with the latest values upon
    notification.""";
  skos:inScheme ble:Scheme;
  skos:prefLabel "Scan Refresh";
  skos:related ble:Notify, ble:ScanRefreshValue;
  prov:wasDerivedFrom <file:/data/lp/etl/executor/data/1651932367716-22-f5b1c2e0-1947-4a2e-a814-6ce401f2a604/working/working-outputfiles-33/gatt-xml-master/org.bluetooth.characteristic.scan_refresh.xml> .

<http://purl.org/wot-catalogue/ble/gatt#org.bluetooth.characteristic.two_zone_heart_rate_limit>
  a skos:Concept, ontolex:LexicalConcept, prov:Entity;
  skos:altLabel "two zone heart rate limit";
  skos:broader ble:Characteristic;
  skos:definition """Heart rate limit between the heart rate zones for the
    2-zone heart rate definition (Fitness and Fat Burn).""";
  skos:inScheme ble:Scheme;
  skos:prefLabel "Two Zone Heart Rate Limit";
  skos:related ble:Read, <http://purl.org/wot-catalogue/ble#TwozoneHeartRateLimit-Fatburn/FitnessLimit>,
    ble:Write;
  prov:wasDerivedFrom <file:/data/lp/etl/executor/data/1651932367716-22-f5b1c2e0-1947-4a2e-a814-6ce401f2a604/working/working-outputfiles-33/gatt-xml-master/org.bluetooth.characteristic.two_zone_heart_rate_limit.xml> .

<http://purl.org/wot-catalogue/ble/gatt#TwozoneHeartRateLimit-Fatburn/FitnessLimit>
  a skos:Concept, ontolex:LexicalConcept, prov:Entity;
  skos:altLabel "two zone heart rate limit - fat burn / fitness limit";
  skos:broader ble:Value;
  skos:definition """Unit is in beats per minute with a
      resolution of 1""";
  skos:inScheme ble:Scheme;
  skos:prefLabel "Two zone Heart Rate Limit - Fat burn / Fitness Limit";
  prov:wasDerivedFrom <file:/data/lp/etl/executor/data/1651932367716-22-f5b1c2e0-1947-4a2e-a814-6ce401f2a604/working/working-outputfiles-33/gatt-xml-master/org.bluetooth.characteristic.two_zone_heart_rate_limit.xml> .

<http://purl.org/wot-catalogue/ble/gatt#1820> a skos:Concept, ontolex:LexicalConcept,
    prov:Entity;
  skos:altLabel "internet protocol support service";
  skos:broader ble:Service;
  skos:definition """This service does not define any
    characteristics""";
  skos:inScheme ble:Scheme;
  skos:prefLabel "Internet Protocol Support Service";
  prov:wasDerivedFrom <file:/data/lp/etl/executor/data/1651932367716-22-f5b1c2e0-1947-4a2e-a814-6ce401f2a604/working/working-outputfiles-33/gatt-xml-master/org.bluetooth.service.internet_protocol_support.xml> .

<http://purl.org/wot-catalogue/ble/gatt#org.bluetooth.characteristic.protocol_mode>
  a skos:Concept, ontolex:LexicalConcept, prov:Entity;
  skos:altLabel "protocol mode";
  skos:broader ble:Characteristic;
  skos:definition """The Protocol Mode characteristic is used to expose the
    current protocol mode of the HID Service with which it is
    associated, or to set the desired protocol mode of the HID
    Service.""";
  skos:inScheme ble:Scheme;
  skos:prefLabel "Protocol Mode";
  skos:related ble:ProtocolModeValue, ble:Read, ble:WriteWithoutResponse;
  prov:wasDerivedFrom <file:/data/lp/etl/executor/data/1651932367716-22-f5b1c2e0-1947-4a2e-a814-6ce401f2a604/working/working-outputfiles-33/gatt-xml-master/org.bluetooth.characteristic.protocol_mode.xml> .

<http://purl.org/wot-catalogue/ble/gatt#ProtocolModeValue> a skos:Concept, ontolex:LexicalConcept,
    prov:Entity;
  skos:altLabel "protocol mode value";
  skos:broader ble:Value;
  skos:inScheme ble:Scheme;
  skos:prefLabel "Protocol Mode Value";
  prov:wasDerivedFrom <file:/data/lp/etl/executor/data/1651932367716-22-f5b1c2e0-1947-4a2e-a814-6ce401f2a604/working/working-outputfiles-33/gatt-xml-master/org.bluetooth.characteristic.protocol_mode.xml> .

<http://purl.org/wot-catalogue/ble/gatt#org.bluetooth.characteristic.aerobic_heart_rate_lower_limit>
  a skos:Concept, ontolex:LexicalConcept, prov:Entity;
  skos:altLabel "aerobic heart rate lower limit";
  skos:broader ble:Characteristic;
  skos:definition """Lower limit of the heart rate where the user enhances
    his endurance while exercising""";
  skos:inScheme ble:Scheme;
  skos:prefLabel "Aerobic Heart Rate Lower Limit";
  skos:related ble:AerobicHeartRateLowerLimit, ble:Read, ble:Write;
  prov:wasDerivedFrom <file:/data/lp/etl/executor/data/1651932367716-22-f5b1c2e0-1947-4a2e-a814-6ce401f2a604/working/working-outputfiles-33/gatt-xml-master/org.bluetooth.characteristic.aerobic_heart_rate_lower_limit.xml> .

<http://purl.org/wot-catalogue/ble/gatt#AerobicHeartRateLowerLimit> a skos:Concept,
    ontolex:LexicalConcept, prov:Entity;
  skos:altLabel "aerobic heart rate lower limit";
  skos:broader ble:Value;
  skos:definition """Unit is in beats per minute with a
      resolution of 1""";
  skos:inScheme ble:Scheme;
  skos:prefLabel "Aerobic Heart Rate Lower Limit";
  prov:wasDerivedFrom <file:/data/lp/etl/executor/data/1651932367716-22-f5b1c2e0-1947-4a2e-a814-6ce401f2a604/working/working-outputfiles-33/gatt-xml-master/org.bluetooth.characteristic.aerobic_heart_rate_lower_limit.xml> .

<http://purl.org/wot-catalogue/ble/gatt#LE_Scan_Interval> a skos:Concept, ontolex:LexicalConcept,
    prov:Entity;
  skos:altLabel "le_scan_interval", "low energy_scan_window";
  skos:broader ble:Value;
  skos:definition "The minimum LE_Scan_Window of the Client corresponding to the LE_Scan_Interval.";
  skos:inScheme ble:Scheme;
  skos:prefLabel "LE_Scan_Interval", "Low Energy_Scan_Window";
  skos:related xsd:unsignedShort;
  prov:wasDerivedFrom <file:/data/lp/etl/executor/data/1651932367716-22-f5b1c2e0-1947-4a2e-a814-6ce401f2a604/working/working-outputfiles-33/gatt-xml-master/org.bluetooth.characteristic.scan_interval_window.xml> .

<http://purl.org/wot-catalogue/ble/gatt#LE_Scan_Window> a skos:Concept, ontolex:LexicalConcept,
    prov:Entity;
  skos:altLabel "le_scan_window", "low energy_scan_interval";
  skos:broader ble:Value;
  skos:definition "The maximum LE_Scan_Interval of the Clien.";
  skos:inScheme ble:Scheme;
  skos:prefLabel "LE_Scan_Window", "Low Energy_Scan_Interval";
  skos:related xsd:unsignedShort;
  prov:wasDerivedFrom <file:/data/lp/etl/executor/data/1651932367716-22-f5b1c2e0-1947-4a2e-a814-6ce401f2a604/working/working-outputfiles-33/gatt-xml-master/org.bluetooth.characteristic.scan_interval_window.xml> .

<http://purl.org/wot-catalogue/ble/gatt#1800> a skos:Concept, ontolex:LexicalConcept,
    prov:Entity;
  skos:altLabel " generic access";
  skos:broader ble:Service;
  skos:definition """The generic_access service contains generic
    information about the device. All available Characteristics are
    readonly.""";
  skos:inScheme ble:Scheme;
  skos:prefLabel " Generic Access";
  skos:related ble:org.bluetooth.characteristic.gap.appearance, ble:org.bluetooth.characteristic.gap.device_name,
    ble:org.bluetooth.characteristic.gap.peripheral_preferred_connection_parameters, ble:org.bluetooth.characteristic.gap.peripheral_privacy_flag,
    ble:org.bluetooth.characteristic.gap.reconnection_address;
  prov:wasDerivedFrom <file:/data/lp/etl/executor/data/1651932367716-22-f5b1c2e0-1947-4a2e-a814-6ce401f2a604/working/working-outputfiles-33/gatt-xml-master/org.bluetooth.service.generic_access.xml> .

<http://purl.org/wot-catalogue/ble/gatt#HTTPHeaders> a skos:Concept, ontolex:LexicalConcept,
    prov:Entity;
  skos:altLabel "http headers";
  skos:broader ble:Value;
  skos:definition """The HTTP headers to be used in the HTTP
      request.""";
  skos:inScheme ble:Scheme;
  skos:prefLabel "HTTP Headers";
  prov:wasDerivedFrom <file:/data/lp/etl/executor/data/1651932367716-22-f5b1c2e0-1947-4a2e-a814-6ce401f2a604/working/working-outputfiles-33/gatt-xml-master/org.bluetooth.characteristic.http_headers.xml> .

<http://purl.org/wot-catalogue/ble/gatt#org.bluetooth.characteristic.manufacturer_name_string>
  a skos:Concept, ontolex:LexicalConcept, prov:Entity;
  skos:altLabel "manufacturer name string";
  skos:broader ble:Characteristic;
  skos:definition """The value of this characteristic is a UTF-8 string
    representing the name of the manufacturer of the
    device.""";
  skos:inScheme ble:Scheme;
  skos:prefLabel "Manufacturer Name String";
  skos:related ble:ManufacturerName, ble:Read;
  prov:wasDerivedFrom <file:/data/lp/etl/executor/data/1651932367716-22-f5b1c2e0-1947-4a2e-a814-6ce401f2a604/working/working-outputfiles-33/gatt-xml-master/org.bluetooth.characteristic.manufacturer_name_string.xml> .

<http://purl.org/wot-catalogue/ble/gatt#ManufacturerName> a skos:Concept, ontolex:LexicalConcept,
    prov:Entity;
  skos:altLabel "manufacturer name";
  skos:broader ble:Value;
  skos:definition "The Manufacturer Name String characteristic shall represent the name of the manufacturer of the device.";
  skos:inScheme ble:Scheme;
  skos:prefLabel "Manufacturer Name";
  skos:related ble:Read, xsd:string;
  prov:wasDerivedFrom <file:/data/lp/etl/executor/data/1651932367716-22-f5b1c2e0-1947-4a2e-a814-6ce401f2a604/working/working-outputfiles-33/gatt-xml-master/org.bluetooth.characteristic.manufacturer_name_string.xml> .

<http://purl.org/wot-catalogue/ble/gatt#AlertStatus> a skos:Concept, ontolex:LexicalConcept,
    prov:Entity;
  skos:altLabel "alert status";
  skos:broader ble:Value;
  skos:inScheme ble:Scheme;
  skos:prefLabel "Alert Status";
  prov:wasDerivedFrom <file:/data/lp/etl/executor/data/1651932367716-22-f5b1c2e0-1947-4a2e-a814-6ce401f2a604/working/working-outputfiles-33/gatt-xml-master/org.bluetooth.characteristic.alert_status.xml> .

<http://purl.org/wot-catalogue/ble/gatt#org.bluetooth.characteristic.language> a skos:Concept,
    ontolex:LexicalConcept, prov:Entity;
  skos:altLabel "language";
  skos:broader ble:Characteristic;
  skos:inScheme ble:Scheme;
  skos:prefLabel "Language";
  skos:related ble:Language, ble:Read, ble:Write;
  prov:wasDerivedFrom <file:/data/lp/etl/executor/data/1651932367716-22-f5b1c2e0-1947-4a2e-a814-6ce401f2a604/working/working-outputfiles-33/gatt-xml-master/org.bluetooth.characteristic.language.xml> .

<http://purl.org/wot-catalogue/ble/gatt#Language> a skos:Concept, ontolex:LexicalConcept,
    prov:Entity;
  skos:altLabel "language";
  skos:broader ble:Value;
  skos:definition """The Language definition is based on
      ISO639-1.""";
  skos:inScheme ble:Scheme;
  skos:prefLabel "Language";
  prov:wasDerivedFrom <file:/data/lp/etl/executor/data/1651932367716-22-f5b1c2e0-1947-4a2e-a814-6ce401f2a604/working/working-outputfiles-33/gatt-xml-master/org.bluetooth.characteristic.language.xml> .

<http://purl.org/wot-catalogue/ble/gatt#org.bluetooth.characteristic.plx_continuous_measurement>
  a skos:Concept, ontolex:LexicalConcept, prov:Entity;
  skos:altLabel "plx continuous measurement characteristic";
  skos:broader ble:Characteristic;
  skos:definition """The PLX Continuous Measurement characteristic, if
    supported, is used to send periodic pulse oximetry
    measurements. This characteristic is a variable length
    structure containing the Flags field (to indicate presence of
    optional fields), the SpO2PR-Normal field, and depending on the
    contents of the Flags field, the SpO2PR-Fast field, the
    SpO2PR-Slow field, the Measurement Status field, the Device and
    Sensor Status field, and/or the Pulse Amplitude Index
    field.""";
  skos:inScheme ble:Scheme;
  skos:prefLabel "PLX Continuous Measurement Characteristic";
  skos:related ble:DeviceandSensorStatus, ble:Flags, ble:InformationText, ble:MeasurementStatus,
    ble:Notify, ble:PulseAmplitudeIndex, ble:SpO2PR-Fast-PR, ble:SpO2PR-Fast-SpO2, ble:SpO2PR-Normal-PR,
    ble:SpO2PR-Normal-SpO2, ble:SpO2PR-Slow-PR, ble:SpO2PR-Slow-SpO2;
  prov:wasDerivedFrom <file:/data/lp/etl/executor/data/1651932367716-22-f5b1c2e0-1947-4a2e-a814-6ce401f2a604/working/working-outputfiles-33/gatt-xml-master/org.bluetooth.characteristic.plx_continuous_measurement.xml> .

<http://purl.org/wot-catalogue/ble/gatt#SpO2PR-Normal-SpO2> a skos:Concept, ontolex:LexicalConcept,
    prov:Entity;
  skos:altLabel "spo2pr-normal - spo2";
  skos:broader ble:Value;
  skos:definition """Unit is percentage with a resolution of
      1""";
  skos:inScheme ble:Scheme;
  skos:prefLabel "SpO2PR-Normal - SpO2";
  prov:wasDerivedFrom <file:/data/lp/etl/executor/data/1651932367716-22-f5b1c2e0-1947-4a2e-a814-6ce401f2a604/working/working-outputfiles-33/gatt-xml-master/org.bluetooth.characteristic.plx_continuous_measurement.xml> .

<http://purl.org/wot-catalogue/ble/gatt#SpO2PR-Normal-PR> a skos:Concept, ontolex:LexicalConcept,
    prov:Entity;
  skos:altLabel "spo2pr-normal - pr";
  skos:broader ble:Value;
  skos:definition """Unit is beats per minute with a resolution
      of 1""";
  skos:inScheme ble:Scheme;
  skos:prefLabel "SpO2PR-Normal - PR";
  prov:wasDerivedFrom <file:/data/lp/etl/executor/data/1651932367716-22-f5b1c2e0-1947-4a2e-a814-6ce401f2a604/working/working-outputfiles-33/gatt-xml-master/org.bluetooth.characteristic.plx_continuous_measurement.xml> .

<http://purl.org/wot-catalogue/ble/gatt#SpO2PR-Fast-SpO2> a skos:Concept, ontolex:LexicalConcept,
    prov:Entity;
  skos:altLabel "spo2pr-fast - spo2";
  skos:broader ble:Value;
  skos:definition """Unit is percentage with a resolution of
      1""";
  skos:inScheme ble:Scheme;
  skos:prefLabel "SpO2PR-Fast - SpO2";
  prov:wasDerivedFrom <file:/data/lp/etl/executor/data/1651932367716-22-f5b1c2e0-1947-4a2e-a814-6ce401f2a604/working/working-outputfiles-33/gatt-xml-master/org.bluetooth.characteristic.plx_continuous_measurement.xml> .

<http://purl.org/wot-catalogue/ble/gatt#SpO2PR-Fast-PR> a skos:Concept, ontolex:LexicalConcept,
    prov:Entity;
  skos:altLabel "spo2pr-fast - pr";
  skos:broader ble:Value;
  skos:definition """Unit is beats per minute with a resolution
      of 1""";
  skos:inScheme ble:Scheme;
  skos:prefLabel "SpO2PR-Fast - PR";
  prov:wasDerivedFrom <file:/data/lp/etl/executor/data/1651932367716-22-f5b1c2e0-1947-4a2e-a814-6ce401f2a604/working/working-outputfiles-33/gatt-xml-master/org.bluetooth.characteristic.plx_continuous_measurement.xml> .

<http://purl.org/wot-catalogue/ble/gatt#SpO2PR-Slow-SpO2> a skos:Concept, ontolex:LexicalConcept,
    prov:Entity;
  skos:altLabel "spo2pr-slow - spo2";
  skos:broader ble:Value;
  skos:definition """Unit is percentage with a resolution of
      1""";
  skos:inScheme ble:Scheme;
  skos:prefLabel "SpO2PR-Slow - SpO2";
  prov:wasDerivedFrom <file:/data/lp/etl/executor/data/1651932367716-22-f5b1c2e0-1947-4a2e-a814-6ce401f2a604/working/working-outputfiles-33/gatt-xml-master/org.bluetooth.characteristic.plx_continuous_measurement.xml> .

<http://purl.org/wot-catalogue/ble/gatt#SpO2PR-Slow-PR> a skos:Concept, ontolex:LexicalConcept,
    prov:Entity;
  skos:altLabel "spo2pr-slow - pr";
  skos:broader ble:Value;
  skos:definition """Unit is beats per minute with a resolution
      of 1""";
  skos:inScheme ble:Scheme;
  skos:prefLabel "SpO2PR-Slow - PR";
  prov:wasDerivedFrom <file:/data/lp/etl/executor/data/1651932367716-22-f5b1c2e0-1947-4a2e-a814-6ce401f2a604/working/working-outputfiles-33/gatt-xml-master/org.bluetooth.characteristic.plx_continuous_measurement.xml> .

<http://purl.org/wot-catalogue/ble/gatt#org.bluetooth.characteristic.software_revision_string>
  a skos:Concept, ontolex:LexicalConcept, prov:Entity;
  skos:altLabel "software revision string";
  skos:broader ble:Characteristic;
  skos:definition """The value of this characteristic is a UTF-8 string
    representing the software revision for the software within the
    device.""";
  skos:inScheme ble:Scheme;
  skos:prefLabel "Software Revision String";
  skos:related ble:Read, ble:SoftwareRevision;
  prov:wasDerivedFrom <file:/data/lp/etl/executor/data/1651932367716-22-f5b1c2e0-1947-4a2e-a814-6ce401f2a604/working/working-outputfiles-33/gatt-xml-master/org.bluetooth.characteristic.software_revision_string.xml> .

<http://purl.org/wot-catalogue/ble/gatt#SoftwareRevision> a skos:Concept, ontolex:LexicalConcept,
    prov:Entity;
  skos:altLabel "software revision", "softwarerevision";
  skos:broader ble:Value;
  skos:definition "The Software Revision String characteristic shall represent the software revision for the software within the device.";
  skos:inScheme ble:Scheme;
  skos:prefLabel "Software Revision", "SoftwareRevision";
  skos:related ble:Read, xsd:string;
  prov:wasDerivedFrom <file:/data/lp/etl/executor/data/1651932367716-22-f5b1c2e0-1947-4a2e-a814-6ce401f2a604/working/working-outputfiles-33/gatt-xml-master/org.bluetooth.characteristic.software_revision_string.xml> .

<http://purl.org/wot-catalogue/ble/gatt#org.bluetooth.characteristic.last_name> a
    skos:Concept, ontolex:LexicalConcept, prov:Entity;
  skos:altLabel "last name";
  skos:broader ble:Characteristic;
  skos:definition "Last name of the user. See Note below.";
  skos:inScheme ble:Scheme;
  skos:prefLabel "Last Name";
  skos:related ble:LastName, ble:Read, ble:Write;
  prov:wasDerivedFrom <file:/data/lp/etl/executor/data/1651932367716-22-f5b1c2e0-1947-4a2e-a814-6ce401f2a604/working/working-outputfiles-33/gatt-xml-master/org.bluetooth.characteristic.last_name.xml> .

<http://purl.org/wot-catalogue/ble/gatt#LastName> a skos:Concept, ontolex:LexicalConcept,
    prov:Entity;
  skos:altLabel "last name";
  skos:broader ble:Value;
  skos:inScheme ble:Scheme;
  skos:prefLabel "Last Name";
  prov:wasDerivedFrom <file:/data/lp/etl/executor/data/1651932367716-22-f5b1c2e0-1947-4a2e-a814-6ce401f2a604/working/working-outputfiles-33/gatt-xml-master/org.bluetooth.characteristic.last_name.xml> .

<http://purl.org/wot-catalogue/ble/gatt#org.bluetooth.characteristic.tx_power_level>
  a skos:Concept, ontolex:LexicalConcept, prov:Entity;
  skos:altLabel "tx power level";
  skos:broader ble:Characteristic;
  skos:definition """The value of the characteristic is a signed 8 bit
    integer that has a fixed point exponent of 0.""";
  skos:inScheme ble:Scheme;
  skos:prefLabel "Tx Power Level";
  skos:related ble:Read, ble:TxPower;
  prov:wasDerivedFrom <file:/data/lp/etl/executor/data/1651932367716-22-f5b1c2e0-1947-4a2e-a814-6ce401f2a604/working/working-outputfiles-33/gatt-xml-master/org.bluetooth.characteristic.tx_power_level.xml> .

<http://purl.org/wot-catalogue/ble/gatt#TxPower> a skos:Concept, ontolex:LexicalConcept,
    prov:Entity;
  skos:altLabel "tx power";
  skos:broader ble:Value;
  skos:inScheme ble:Scheme;
  skos:prefLabel "Tx Power";
  prov:wasDerivedFrom <file:/data/lp/etl/executor/data/1651932367716-22-f5b1c2e0-1947-4a2e-a814-6ce401f2a604/working/working-outputfiles-33/gatt-xml-master/org.bluetooth.characteristic.tx_power_level.xml> .

<http://purl.org/wot-catalogue/ble/gatt#Altitude> a skos:Concept, ontolex:LexicalConcept,
    prov:Entity;
  skos:altLabel "altitude";
  skos:broader ble:Value;
  skos:inScheme ble:Scheme;
  skos:prefLabel "Altitude";
  prov:wasDerivedFrom <file:/data/lp/etl/executor/data/1651932367716-22-f5b1c2e0-1947-4a2e-a814-6ce401f2a604/working/working-outputfiles-33/gatt-xml-master/org.bluetooth.characteristic.altitude.xml> .

<http://purl.org/wot-catalogue/ble/gatt#org.bluetooth.characteristic.cycling_power_vector>
  a skos:Concept, ontolex:LexicalConcept, prov:Entity;
  skos:altLabel "cycling power vector";
  skos:broader ble:Characteristic;
  skos:definition """The Cycling Power Vector characteristic is a variable
    length structure containing a Flags fieldand based on the
    contents of the Flags field, may contain one or more additional
    fields as shown in the table below.""";
  skos:inScheme ble:Scheme;
  skos:prefLabel "Cycling Power Vector";
  skos:related ble:CrankRevolutionData-CumulativeCrankRevolutions, ble:CrankRevolutionData-LastCrankEventTime,
    ble:FirstCrankMeasurementAngle, ble:Flags, ble:InstantaneousForceMagnitudeArray, ble:InstantaneousTorqueMagnitudeArray,
    ble:Notify;
  prov:wasDerivedFrom <file:/data/lp/etl/executor/data/1651932367716-22-f5b1c2e0-1947-4a2e-a814-6ce401f2a604/working/working-outputfiles-33/gatt-xml-master/org.bluetooth.characteristic.cycling_power_vector.xml> .

<http://purl.org/wot-catalogue/ble/gatt#CrankRevolutionData-CumulativeCrankRevolutions>
  a skos:Concept, ontolex:LexicalConcept, prov:Entity;
  skos:altLabel "crank revolution data - cumulative crank revolutions", "crank revolution data- cumulative crank revolutions";
  skos:broader ble:Value;
  skos:definition """Unitless 
      C1:When present, these fields are always present as a
      pair.""",
    """Unitless 
      C2:When present, these fields are always present as a
      pair.""";
  skos:inScheme ble:Scheme;
  skos:prefLabel "Crank Revolution Data - Cumulative Crank Revolutions", "Crank Revolution Data- Cumulative Crank Revolutions";
  prov:wasDerivedFrom <file:/data/lp/etl/executor/data/1651932367716-22-f5b1c2e0-1947-4a2e-a814-6ce401f2a604/working/working-outputfiles-33/gatt-xml-master/org.bluetooth.characteristic.cycling_power_measurement.xml>,
    <file:/data/lp/etl/executor/data/1651932367716-22-f5b1c2e0-1947-4a2e-a814-6ce401f2a604/working/working-outputfiles-33/gatt-xml-master/org.bluetooth.characteristic.cycling_power_vector.xml> .

<http://purl.org/wot-catalogue/ble/gatt#CrankRevolutionData-LastCrankEventTime> a
    skos:Concept, ontolex:LexicalConcept, prov:Entity;
  skos:altLabel "crank revolution data - last crank event time", "crank revolution data- last crank event time";
  skos:broader ble:Value;
  skos:definition """Unit is in seconds with a resolution of
      1/1024. 
      C1:When present, these fields are always present as a
      pair.""",
    """Unit is in seconds with a resolution of
      1/1024. 
      C2:When present, these fields are always present as a
      pair.""";
  skos:inScheme ble:Scheme;
  skos:prefLabel "Crank Revolution Data - Last Crank Event Time", "Crank Revolution Data- Last Crank Event Time";
  prov:wasDerivedFrom <file:/data/lp/etl/executor/data/1651932367716-22-f5b1c2e0-1947-4a2e-a814-6ce401f2a604/working/working-outputfiles-33/gatt-xml-master/org.bluetooth.characteristic.cycling_power_measurement.xml>,
    <file:/data/lp/etl/executor/data/1651932367716-22-f5b1c2e0-1947-4a2e-a814-6ce401f2a604/working/working-outputfiles-33/gatt-xml-master/org.bluetooth.characteristic.cycling_power_vector.xml> .

<http://purl.org/wot-catalogue/ble/gatt#FirstCrankMeasurementAngle> a skos:Concept,
    ontolex:LexicalConcept, prov:Entity;
  skos:altLabel "first crank measurement angle";
  skos:broader ble:Value;
  skos:definition """Unit is in degrees with a resolution of
      1.""";
  skos:inScheme ble:Scheme;
  skos:prefLabel "First Crank Measurement Angle";
  prov:wasDerivedFrom <file:/data/lp/etl/executor/data/1651932367716-22-f5b1c2e0-1947-4a2e-a814-6ce401f2a604/working/working-outputfiles-33/gatt-xml-master/org.bluetooth.characteristic.cycling_power_vector.xml> .

<http://purl.org/wot-catalogue/ble/gatt#InstantaneousForceMagnitudeArray> a skos:Concept,
    ontolex:LexicalConcept, prov:Entity;
  skos:altLabel "instantaneous force magnitude array";
  skos:broader ble:Value;
  skos:definition """The unit is in newtons with a resolution of
      1 
      Array Order - Older is towards the LSO and Newer is
      towards the MSOC2: These fields are mutually exclusive. When this field
      is present, the presence of the Instantaneous Torque
      Magnitude Array is excluded.""";
  skos:inScheme ble:Scheme;
  skos:prefLabel "Instantaneous Force Magnitude Array";
  prov:wasDerivedFrom <file:/data/lp/etl/executor/data/1651932367716-22-f5b1c2e0-1947-4a2e-a814-6ce401f2a604/working/working-outputfiles-33/gatt-xml-master/org.bluetooth.characteristic.cycling_power_vector.xml> .

<http://purl.org/wot-catalogue/ble/gatt#InstantaneousTorqueMagnitudeArray> a skos:Concept,
    ontolex:LexicalConcept, prov:Entity;
  skos:altLabel "instantaneous torque magnitude array";
  skos:broader ble:Value;
  skos:definition """Unit is in newton/meter with a resolution of
      1/32 
      Array Order - Older is towards the LSO and Newer is
      towards the MSOC2: These fields are mutually exclusive. When this field
      is present, the presence of the Instantaneous Force Magnitude
      Array is excluded.""";
  skos:inScheme ble:Scheme;
  skos:prefLabel "Instantaneous Torque Magnitude Array";
  prov:wasDerivedFrom <file:/data/lp/etl/executor/data/1651932367716-22-f5b1c2e0-1947-4a2e-a814-6ce401f2a604/working/working-outputfiles-33/gatt-xml-master/org.bluetooth.characteristic.cycling_power_vector.xml> .

<http://purl.org/wot-catalogue/ble/gatt#org.bluetooth.characteristic.cgm_session_run_time>
  a skos:Concept, ontolex:LexicalConcept, prov:Entity;
  skos:altLabel "cgm session run time";
  skos:broader ble:Characteristic;
  skos:inScheme ble:Scheme;
  skos:prefLabel "CGM Session Run Time";
  skos:related ble:CGMSessionRunTime, ble:E2E-CRC, ble:Read;
  prov:wasDerivedFrom <file:/data/lp/etl/executor/data/1651932367716-22-f5b1c2e0-1947-4a2e-a814-6ce401f2a604/working/working-outputfiles-33/gatt-xml-master/org.bluetooth.characteristic.cgm_session_run_time.xml> .

<http://purl.org/wot-catalogue/ble/gatt#CGMSessionRunTime> a skos:Concept, ontolex:LexicalConcept,
    prov:Entity;
  skos:altLabel "cgm session run time";
  skos:broader ble:Value;
  skos:definition """Typically the CGM Sensors have a limited run
      time where they are approved for by regulatory bodies.
      However this characteristic should enable a prediction of the
      run time depending on physiological effects in future
      devices.""";
  skos:inScheme ble:Scheme;
  skos:prefLabel "CGM Session Run Time";
  prov:wasDerivedFrom <file:/data/lp/etl/executor/data/1651932367716-22-f5b1c2e0-1947-4a2e-a814-6ce401f2a604/working/working-outputfiles-33/gatt-xml-master/org.bluetooth.characteristic.cgm_session_run_time.xml> .

<http://purl.org/wot-catalogue/ble/gatt#InstantaneousCadence> a skos:Concept, ontolex:LexicalConcept,
    prov:Entity;
  skos:altLabel "instantaneous cadence";
  skos:broader ble:Value;
  skos:definition """1/minute with a resolution of
      0.5""", """Unit is in 1/minute (or RPM) with a
      resolutions of 1 1/min (or 1 RPM)""";
  skos:inScheme ble:Scheme;
  skos:prefLabel "Instantaneous Cadence";
  prov:wasDerivedFrom <file:/data/lp/etl/executor/data/1651932367716-22-f5b1c2e0-1947-4a2e-a814-6ce401f2a604/working/working-outputfiles-33/gatt-xml-master/org.bluetooth.characteristic.indoor_bike_data.xml>,
    <file:/data/lp/etl/executor/data/1651932367716-22-f5b1c2e0-1947-4a2e-a814-6ce401f2a604/working/working-outputfiles-33/gatt-xml-master/org.bluetooth.characteristic.rsc_measurement.xml> .

<http://purl.org/wot-catalogue/ble/gatt#AverageCadence> a skos:Concept, ontolex:LexicalConcept,
    prov:Entity;
  skos:altLabel "average cadence";
  skos:broader ble:Value;
  skos:definition """1/minute with a resolution of
      0.5""";
  skos:inScheme ble:Scheme;
  skos:prefLabel "Average Cadence";
  prov:wasDerivedFrom <file:/data/lp/etl/executor/data/1651932367716-22-f5b1c2e0-1947-4a2e-a814-6ce401f2a604/working/working-outputfiles-33/gatt-xml-master/org.bluetooth.characteristic.indoor_bike_data.xml> .

<http://purl.org/wot-catalogue/ble/gatt#StrokeRate> a skos:Concept, ontolex:LexicalConcept,
    prov:Entity;
  skos:altLabel "stroke rate";
  skos:broader ble:Value;
  skos:definition """stroke/minute with a resolution of
      0.5""";
  skos:inScheme ble:Scheme;
  skos:prefLabel "Stroke Rate";
  prov:wasDerivedFrom <file:/data/lp/etl/executor/data/1651932367716-22-f5b1c2e0-1947-4a2e-a814-6ce401f2a604/working/working-outputfiles-33/gatt-xml-master/org.bluetooth.characteristic.rower_data.xml> .

<http://purl.org/wot-catalogue/ble/gatt#StrokeCount> a skos:Concept, ontolex:LexicalConcept,
    prov:Entity;
  skos:altLabel "stroke count";
  skos:broader ble:Value;
  skos:definition """Unitless with a resolution of
      1""";
  skos:inScheme ble:Scheme;
  skos:prefLabel "Stroke Count";
  prov:wasDerivedFrom <file:/data/lp/etl/executor/data/1651932367716-22-f5b1c2e0-1947-4a2e-a814-6ce401f2a604/working/working-outputfiles-33/gatt-xml-master/org.bluetooth.characteristic.rower_data.xml> .

<http://purl.org/wot-catalogue/ble/gatt#AverageStrokeRate> a skos:Concept, ontolex:LexicalConcept,
    prov:Entity;
  skos:altLabel "average stroke rate";
  skos:broader ble:Value;
  skos:definition """1/minute with a resolution of
      0.5""";
  skos:inScheme ble:Scheme;
  skos:prefLabel "Average Stroke Rate";
  prov:wasDerivedFrom <file:/data/lp/etl/executor/data/1651932367716-22-f5b1c2e0-1947-4a2e-a814-6ce401f2a604/working/working-outputfiles-33/gatt-xml-master/org.bluetooth.characteristic.rower_data.xml> .

<http://purl.org/wot-catalogue/ble/gatt#InstantaneousPace> a skos:Concept, ontolex:LexicalConcept,
    prov:Entity;
  skos:altLabel "instantaneous pace";
  skos:broader ble:Value;
  skos:definition """Kilometer per minute with a resolution of
      0.1""", """Second with a resolution of
      1""";
  skos:inScheme ble:Scheme;
  skos:prefLabel "Instantaneous Pace";
  prov:wasDerivedFrom <file:/data/lp/etl/executor/data/1651932367716-22-f5b1c2e0-1947-4a2e-a814-6ce401f2a604/working/working-outputfiles-33/gatt-xml-master/org.bluetooth.characteristic.rower_data.xml>,
    <file:/data/lp/etl/executor/data/1651932367716-22-f5b1c2e0-1947-4a2e-a814-6ce401f2a604/working/working-outputfiles-33/gatt-xml-master/org.bluetooth.characteristic.treadmill_data.xml> .

<http://purl.org/wot-catalogue/ble/gatt#AveragePace> a skos:Concept, ontolex:LexicalConcept,
    prov:Entity;
  skos:altLabel "average pace";
  skos:broader ble:Value;
  skos:definition """Kilometer per minute with a resolution of
      0.1""", """Second with a resolution of
      1""";
  skos:inScheme ble:Scheme;
  skos:prefLabel "Average Pace";
  prov:wasDerivedFrom <file:/data/lp/etl/executor/data/1651932367716-22-f5b1c2e0-1947-4a2e-a814-6ce401f2a604/working/working-outputfiles-33/gatt-xml-master/org.bluetooth.characteristic.rower_data.xml>,
    <file:/data/lp/etl/executor/data/1651932367716-22-f5b1c2e0-1947-4a2e-a814-6ce401f2a604/working/working-outputfiles-33/gatt-xml-master/org.bluetooth.characteristic.treadmill_data.xml> .

<http://purl.org/wot-catalogue/ble/gatt#1809> a skos:Concept, ontolex:LexicalConcept,
    prov:Entity;
  skos:altLabel "health thermometer";
  skos:broader ble:Service;
  skos:definition """The Health Thermometer service is instantiated as a
    Primary Service. There are one or more instantiations of the
    Health Thermometer service per device claiming conformance with
    this specification.""";
  skos:inScheme ble:Scheme;
  skos:prefLabel "Health Thermometer";
  skos:related ble:org.bluetooth.characteristic.intermediate_temperature, ble:org.bluetooth.characteristic.measurement_interval,
    ble:org.bluetooth.characteristic.temperature_measurement, ble:org.bluetooth.characteristic.temperature_type;
  prov:wasDerivedFrom <file:/data/lp/etl/executor/data/1651932367716-22-f5b1c2e0-1947-4a2e-a814-6ce401f2a604/working/working-outputfiles-33/gatt-xml-master/org.bluetooth.service.health_thermometer.xml> .

<http://purl.org/wot-catalogue/ble/gatt#org.bluetooth.characteristic.temperature_measurement>
  a skos:Concept, ontolex:LexicalConcept, prov:Entity;
  skos:altLabel "temperature measurement";
  skos:broader ble:Characteristic;
  skos:definition """The flags is the first field sent followed by the
    Temperature Measurement Value.""";
  skos:inScheme ble:Scheme;
  skos:prefLabel "Temperature Measurement";
  skos:related ble:Flags, ble:Indicate, <http://purl.org/wot-catalogue/ble#TemperatureMeasurementValue(Celsius)>,
    <http://purl.org/wot-catalogue/ble#TemperatureMeasurementValue(Fahrenheit)>, ble:TemperatureType,
    ble:TimeStamp;
  prov:wasDerivedFrom <file:/data/lp/etl/executor/data/1651932367716-22-f5b1c2e0-1947-4a2e-a814-6ce401f2a604/working/working-outputfiles-33/gatt-xml-master/org.bluetooth.characteristic.temperature_measurement.xml> .

<http://purl.org/wot-catalogue/ble/gatt#org.bluetooth.characteristic.temperature_type>
  a skos:Concept, ontolex:LexicalConcept, prov:Entity;
  skos:altLabel "temperature type";
  skos:broader ble:Characteristic;
  skos:definition """These Temperature Type values correspond to the
    Temperature Type descriptions used in ISO/IEEE
    11073-10408-2008.""";
  skos:inScheme ble:Scheme;
  skos:prefLabel "Temperature Type";
  skos:related ble:Read, ble:TemperatureTextDescription;
  prov:wasDerivedFrom <file:/data/lp/etl/executor/data/1651932367716-22-f5b1c2e0-1947-4a2e-a814-6ce401f2a604/working/working-outputfiles-33/gatt-xml-master/org.bluetooth.characteristic.temperature_type.xml> .

<http://purl.org/wot-catalogue/ble/gatt#org.bluetooth.characteristic.boot_mouse_input_report>
  a skos:Concept, ontolex:LexicalConcept, prov:Entity;
  skos:altLabel "boot mouse input report";
  skos:broader ble:Characteristic;
  skos:definition """The Boot Mouse Input Report characteristic is used to
    transfer fixed format and length Input Report data between a
    HID Host operating in Boot Protocol Mode and a HID Service
    corresponding to a boot mouse.""";
  skos:inScheme ble:Scheme;
  skos:prefLabel "Boot Mouse Input Report";
  skos:related ble:BootMouseInputReportValue, ble:Notify, ble:Read, ble:Write;
  prov:wasDerivedFrom <file:/data/lp/etl/executor/data/1651932367716-22-f5b1c2e0-1947-4a2e-a814-6ce401f2a604/working/working-outputfiles-33/gatt-xml-master/org.bluetooth.characteristic.boot_mouse_input_report.xml> .

<http://purl.org/wot-catalogue/ble/gatt#BootMouseInputReportValue> a skos:Concept,
    ontolex:LexicalConcept, prov:Entity;
  skos:altLabel "boot mouse input report value";
  skos:broader ble:Value;
  skos:inScheme ble:Scheme;
  skos:prefLabel "Boot Mouse Input Report Value";
  prov:wasDerivedFrom <file:/data/lp/etl/executor/data/1651932367716-22-f5b1c2e0-1947-4a2e-a814-6ce401f2a604/working/working-outputfiles-33/gatt-xml-master/org.bluetooth.characteristic.boot_mouse_input_report.xml> .

<http://purl.org/wot-catalogue/ble/gatt#org.bluetooth.characteristic.cycling_power_control_point>
  a skos:Concept, ontolex:LexicalConcept, prov:Entity;
  skos:altLabel "cycling power control point";
  skos:broader ble:Characteristic;
  skos:definition """The Cycling Power Control Point characteristic is used
    to request a specific function to be executed on the receiving
    device.""";
  skos:inScheme ble:Scheme;
  skos:prefLabel "Cycling Power Control Point";
  skos:related ble:Indicate, ble:OpCodes, ble:ParameterValue, ble:RequestOpCode, ble:ResponseParameter,
    ble:ResponseValue, ble:Write;
  prov:wasDerivedFrom <file:/data/lp/etl/executor/data/1651932367716-22-f5b1c2e0-1947-4a2e-a814-6ce401f2a604/working/working-outputfiles-33/gatt-xml-master/org.bluetooth.characteristic.cycling_power_control_point.xml> .

<http://purl.org/wot-catalogue/ble/gatt#OpCodes> a skos:Concept, ontolex:LexicalConcept,
    prov:Entity;
  skos:altLabel "op codes";
  skos:broader ble:Value;
  skos:inScheme ble:Scheme;
  skos:prefLabel "Op Codes";
  prov:wasDerivedFrom <file:/data/lp/etl/executor/data/1651932367716-22-f5b1c2e0-1947-4a2e-a814-6ce401f2a604/working/working-outputfiles-33/gatt-xml-master/org.bluetooth.characteristic.cycling_power_control_point.xml>,
    <file:/data/lp/etl/executor/data/1651932367716-22-f5b1c2e0-1947-4a2e-a814-6ce401f2a604/working/working-outputfiles-33/gatt-xml-master/org.bluetooth.characteristic.ln_control_point.xml> .

<http://purl.org/wot-catalogue/ble/gatt#ParameterValue> a skos:Concept, ontolex:LexicalConcept,
    prov:Entity;
  skos:altLabel "parameter value";
  skos:broader ble:Value;
  skos:inScheme ble:Scheme;
  skos:prefLabel "Parameter Value";
  prov:wasDerivedFrom <file:/data/lp/etl/executor/data/1651932367716-22-f5b1c2e0-1947-4a2e-a814-6ce401f2a604/working/working-outputfiles-33/gatt-xml-master/org.bluetooth.characteristic.cycling_power_control_point.xml>,
    <file:/data/lp/etl/executor/data/1651932367716-22-f5b1c2e0-1947-4a2e-a814-6ce401f2a604/working/working-outputfiles-33/gatt-xml-master/org.bluetooth.characteristic.ln_control_point.xml> .

<http://purl.org/wot-catalogue/ble/gatt#org.bluetooth.characteristic.boot_keyboard_input_report>
  a skos:Concept, ontolex:LexicalConcept, prov:Entity;
  skos:altLabel "boot keyboard input report";
  skos:broader ble:Characteristic;
  skos:definition """The Boot Keyboard Input Report characteristic is used
    to transfer fixed format and length Input Report data between a
    HID Host operating in Boot Protocol Mode and a HID Service
    corresponding to a boot keyboard.""";
  skos:inScheme ble:Scheme;
  skos:prefLabel "Boot Keyboard Input Report";
  skos:related ble:BootKeyboardInputReportValue, ble:Notify, ble:Read, ble:Write;
  prov:wasDerivedFrom <file:/data/lp/etl/executor/data/1651932367716-22-f5b1c2e0-1947-4a2e-a814-6ce401f2a604/working/working-outputfiles-33/gatt-xml-master/org.bluetooth.characteristic.boot_keyboard_input_report.xml> .

<http://purl.org/wot-catalogue/ble/gatt#BootKeyboardInputReportValue> a skos:Concept,
    ontolex:LexicalConcept, prov:Entity;
  skos:altLabel "boot keyboard input report value";
  skos:broader ble:Value;
  skos:inScheme ble:Scheme;
  skos:prefLabel "Boot Keyboard Input Report Value";
  prov:wasDerivedFrom <file:/data/lp/etl/executor/data/1651932367716-22-f5b1c2e0-1947-4a2e-a814-6ce401f2a604/working/working-outputfiles-33/gatt-xml-master/org.bluetooth.characteristic.boot_keyboard_input_report.xml> .

<http://purl.org/wot-catalogue/ble/gatt#org.bluetooth.characteristic.intermediate_cuff_pressure>
  a skos:Concept, ontolex:LexicalConcept, prov:Entity;
  skos:altLabel "intermediate cuff pressure";
  skos:broader ble:Characteristic;
  skos:inScheme ble:Scheme;
  skos:prefLabel "Intermediate Cuff Pressure";
  skos:related ble:IntermediateCuffPressure, ble:Notify;
  prov:wasDerivedFrom <file:/data/lp/etl/executor/data/1651932367716-22-f5b1c2e0-1947-4a2e-a814-6ce401f2a604/working/working-outputfiles-33/gatt-xml-master/org.bluetooth.characteristic.intermediate_cuff_pressure.xml> .

<http://purl.org/wot-catalogue/ble/gatt#IntermediateCuffPressure> a skos:Concept,
    ontolex:LexicalConcept, prov:Entity;
  skos:altLabel "intermediate cuff pressure";
  skos:broader ble:Value;
  skos:inScheme ble:Scheme;
  skos:prefLabel "Intermediate Cuff Pressure";
  prov:wasDerivedFrom <file:/data/lp/etl/executor/data/1651932367716-22-f5b1c2e0-1947-4a2e-a814-6ce401f2a604/working/working-outputfiles-33/gatt-xml-master/org.bluetooth.characteristic.intermediate_cuff_pressure.xml> .

<http://purl.org/wot-catalogue/ble/gatt#1818> a skos:Concept, ontolex:LexicalConcept,
    prov:Entity;
  skos:altLabel "cycling power";
  skos:broader ble:Service;
  skos:definition """The Cycling Power (CP) Service exposes power- and
    force-related data and optionally speed- and cadence-related
    data from a Cycling Power sensor (Server) intended for sports
    and fitness applications.""";
  skos:inScheme ble:Scheme;
  skos:prefLabel "Cycling Power";
  skos:related ble:org.bluetooth.characteristic.cycling_power_control_point, ble:org.bluetooth.characteristic.cycling_power_feature,
    ble:org.bluetooth.characteristic.cycling_power_measurement, ble:org.bluetooth.characteristic.cycling_power_vector,
    ble:org.bluetooth.characteristic.sensor_location;
  prov:wasDerivedFrom <file:/data/lp/etl/executor/data/1651932367716-22-f5b1c2e0-1947-4a2e-a814-6ce401f2a604/working/working-outputfiles-33/gatt-xml-master/org.bluetooth.service.cycling_power.xml> .

<http://purl.org/wot-catalogue/ble/gatt#org.bluetooth.characteristic.cycling_power_measurement>
  a skos:Concept, ontolex:LexicalConcept, prov:Entity;
  skos:altLabel "cycling power measurement";
  skos:broader ble:Characteristic;
  skos:definition """The Cycling Power Measurement characteristic is a
    variable length structure containing a Flags field, an
    Instantaneous Power field and, based on the contents of the
    Flags field, may contain one or more additional fields as shown
    in the table below.""";
  skos:inScheme ble:Scheme;
  skos:prefLabel "Cycling Power Measurement";
  skos:related ble:AccumulatedEnergy, ble:AccumulatedTorque, ble:BottomDeadSpotAngle,
    ble:Broadcast, ble:CrankRevolutionData-CumulativeCrankRevolutions, ble:CrankRevolutionData-LastCrankEventTime,
    ble:ExtremeAngles-MaximumAngle, ble:ExtremeAngles-MinimumAngle, ble:ExtremeForceMagnitudes-MaximumForceMagnitude,
    ble:ExtremeForceMagnitudes-MinimumForceMagnitude, ble:ExtremeTorqueMagnitudes-MaximumTorqueMagnitude,
    ble:ExtremeTorqueMagnitudes-MinimumTorqueMagnitude, ble:Flags, ble:InstantaneousPower,
    ble:Notify, ble:PedalPowerBalance, ble:TopDeadSpotAngle, ble:WheelRevolutionData-CumulativeWheelRevolutions,
    ble:WheelRevolutionData-LastWheelEventTime;
  prov:wasDerivedFrom <file:/data/lp/etl/executor/data/1651932367716-22-f5b1c2e0-1947-4a2e-a814-6ce401f2a604/working/working-outputfiles-33/gatt-xml-master/org.bluetooth.characteristic.cycling_power_measurement.xml> .

<http://purl.org/wot-catalogue/ble/gatt#org.bluetooth.characteristic.blood_pressure_measurement>
  a skos:Concept, ontolex:LexicalConcept, prov:Entity;
  skos:altLabel "blood pressure measurement";
  skos:broader ble:Characteristic;
  skos:definition """The Blood Pressure Measurement characteristic is a
    variable length structure containing a Flags field, a Blood
    Pressure Measurement Compound Value field, and contains
    additional fields such as Time Stamp, Pulse Rate and User ID as
    determined by the contents of the Flags field.""";
  skos:inScheme ble:Scheme;
  skos:prefLabel "Blood Pressure Measurement";
  skos:related <http://purl.org/wot-catalogue/ble#BloodPressureMeasurementCompoundValue-Diastolic(kPa)>,
    <http://purl.org/wot-catalogue/ble#BloodPressureMeasurementCompoundValue-Diastolic(mmHg)>,
    <http://purl.org/wot-catalogue/ble#BloodPressureMeasurementCompoundValue-MeanArterialPressure(kPa)>,
    <http://purl.org/wot-catalogue/ble#BloodPressureMeasurementCompoundValue-MeanArterialPressure(mmHg)>,
    <http://purl.org/wot-catalogue/ble#BloodPressureMeasurementCompoundValue-Systolic(kPa)>,
    <http://purl.org/wot-catalogue/ble#BloodPressureMeasurementCompoundValue-Systolic(mmHg)>,
    ble:Flags, ble:Indicate, ble:MeasurementStatus, ble:PulseRate, ble:TimeStamp, ble:UserID;
  prov:wasDerivedFrom <file:/data/lp/etl/executor/data/1651932367716-22-f5b1c2e0-1947-4a2e-a814-6ce401f2a604/working/working-outputfiles-33/gatt-xml-master/org.bluetooth.characteristic.blood_pressure_measurement.xml> .

<http://purl.org/wot-catalogue/ble/gatt#BloodPressureMeasurementCompoundValue-Systolic(mmHg)>
  a skos:Concept, ontolex:LexicalConcept, prov:Entity;
  skos:altLabel "blood pressure measurement compound value - systolic (mmhg)";
  skos:broader ble:Value;
  skos:definition """C1: Field exists if the key of bit 0 of the
      Flags field is set to 0""";
  skos:inScheme ble:Scheme;
  skos:prefLabel "Blood Pressure Measurement Compound Value - Systolic (mmHg)";
  prov:wasDerivedFrom <file:/data/lp/etl/executor/data/1651932367716-22-f5b1c2e0-1947-4a2e-a814-6ce401f2a604/working/working-outputfiles-33/gatt-xml-master/org.bluetooth.characteristic.blood_pressure_measurement.xml> .

<http://purl.org/wot-catalogue/ble/gatt#BloodPressureMeasurementCompoundValue-Diastolic(mmHg)>
  a skos:Concept, ontolex:LexicalConcept, prov:Entity;
  skos:altLabel "blood pressure measurement compound value - diastolic (mmhg)";
  skos:broader ble:Value;
  skos:definition """C1: Field exists if the key of bit 0 of the
      Flags field is set to 0""";
  skos:inScheme ble:Scheme;
  skos:prefLabel "Blood Pressure Measurement Compound Value - Diastolic (mmHg)";
  prov:wasDerivedFrom <file:/data/lp/etl/executor/data/1651932367716-22-f5b1c2e0-1947-4a2e-a814-6ce401f2a604/working/working-outputfiles-33/gatt-xml-master/org.bluetooth.characteristic.blood_pressure_measurement.xml> .

<http://purl.org/wot-catalogue/ble/gatt#BloodPressureMeasurementCompoundValue-MeanArterialPressure(mmHg)>
  a skos:Concept, ontolex:LexicalConcept, prov:Entity;
  skos:altLabel "blood pressure measurement compound value - mean arterial pressure (mmhg)";
  skos:broader ble:Value;
  skos:definition """C1: Field exists if the key of bit 0 of the
      Flags field is set to 0""";
  skos:inScheme ble:Scheme;
  skos:prefLabel "Blood Pressure Measurement Compound Value - Mean Arterial Pressure (mmHg)";
  prov:wasDerivedFrom <file:/data/lp/etl/executor/data/1651932367716-22-f5b1c2e0-1947-4a2e-a814-6ce401f2a604/working/working-outputfiles-33/gatt-xml-master/org.bluetooth.characteristic.blood_pressure_measurement.xml> .

<http://purl.org/wot-catalogue/ble/gatt#BloodPressureMeasurementCompoundValue-Systolic(kPa)>
  a skos:Concept, ontolex:LexicalConcept, prov:Entity;
  skos:altLabel "blood pressure measurement compound value - systolic (kpa)";
  skos:broader ble:Value;
  skos:definition """C2: Field exists if the key of bit 0 of the
      Flags field is set to 1""";
  skos:inScheme ble:Scheme;
  skos:prefLabel "Blood Pressure Measurement Compound Value - Systolic (kPa)";
  prov:wasDerivedFrom <file:/data/lp/etl/executor/data/1651932367716-22-f5b1c2e0-1947-4a2e-a814-6ce401f2a604/working/working-outputfiles-33/gatt-xml-master/org.bluetooth.characteristic.blood_pressure_measurement.xml> .

<http://purl.org/wot-catalogue/ble/gatt#BloodPressureMeasurementCompoundValue-Diastolic(kPa)>
  a skos:Concept, ontolex:LexicalConcept, prov:Entity;
  skos:altLabel "blood pressure measurement compound value - diastolic (kpa)";
  skos:broader ble:Value;
  skos:definition """C2: Field exists if the key of bit 0 of the
      Flags field is set to 1""";
  skos:inScheme ble:Scheme;
  skos:prefLabel "Blood Pressure Measurement Compound Value - Diastolic (kPa)";
  prov:wasDerivedFrom <file:/data/lp/etl/executor/data/1651932367716-22-f5b1c2e0-1947-4a2e-a814-6ce401f2a604/working/working-outputfiles-33/gatt-xml-master/org.bluetooth.characteristic.blood_pressure_measurement.xml> .

<http://purl.org/wot-catalogue/ble/gatt#BloodPressureMeasurementCompoundValue-MeanArterialPressure(kPa)>
  a skos:Concept, ontolex:LexicalConcept, prov:Entity;
  skos:altLabel "blood pressure measurement compound value - mean arterial pressure (kpa)";
  skos:broader ble:Value;
  skos:definition """C2: Field exists if the key of bit 0 of the
      Flags field is set to 1""";
  skos:inScheme ble:Scheme;
  skos:prefLabel "Blood Pressure Measurement Compound Value - Mean Arterial Pressure (kPa)";
  prov:wasDerivedFrom <file:/data/lp/etl/executor/data/1651932367716-22-f5b1c2e0-1947-4a2e-a814-6ce401f2a604/working/working-outputfiles-33/gatt-xml-master/org.bluetooth.characteristic.blood_pressure_measurement.xml> .

<http://purl.org/wot-catalogue/ble/gatt#TimeStamp> a skos:Concept, ontolex:LexicalConcept,
    prov:Entity;
  skos:altLabel "time stamp";
  skos:broader ble:Value;
  skos:definition """C3: Field exists if the key of bit 1 of the
      Flags field is set to 1""",
    """If the flags bit 1 is 1 this field is
      included. If it is 0, this field is not
      included""",
    "Smallest unit in seconds";
  skos:inScheme ble:Scheme;
  skos:prefLabel "Time Stamp";
  prov:wasDerivedFrom <file:/data/lp/etl/executor/data/1651932367716-22-f5b1c2e0-1947-4a2e-a814-6ce401f2a604/working/working-outputfiles-33/gatt-xml-master/org.bluetooth.characteristic.blood_pressure_measurement.xml>,
    <file:/data/lp/etl/executor/data/1651932367716-22-f5b1c2e0-1947-4a2e-a814-6ce401f2a604/working/working-outputfiles-33/gatt-xml-master/org.bluetooth.characteristic.body_composition_measurement.xml>,
    <file:/data/lp/etl/executor/data/1651932367716-22-f5b1c2e0-1947-4a2e-a814-6ce401f2a604/working/working-outputfiles-33/gatt-xml-master/org.bluetooth.characteristic.temperature_measurement.xml>,
    <file:/data/lp/etl/executor/data/1651932367716-22-f5b1c2e0-1947-4a2e-a814-6ce401f2a604/working/working-outputfiles-33/gatt-xml-master/org.bluetooth.characteristic.weight_measurement.xml> .

<http://purl.org/wot-catalogue/ble/gatt#PulseRate> a skos:Concept, ontolex:LexicalConcept,
    prov:Entity;
  skos:altLabel "pulse rate";
  skos:broader ble:Value;
  skos:definition """C4: Field exists if the key of bit 2 of the
      Flags field is set to 1""";
  skos:inScheme ble:Scheme;
  skos:prefLabel "Pulse Rate";
  prov:wasDerivedFrom <file:/data/lp/etl/executor/data/1651932367716-22-f5b1c2e0-1947-4a2e-a814-6ce401f2a604/working/working-outputfiles-33/gatt-xml-master/org.bluetooth.characteristic.blood_pressure_measurement.xml> .

<http://purl.org/wot-catalogue/ble/gatt#UserID> a skos:Concept, ontolex:LexicalConcept,
    prov:Entity;
  skos:altLabel "user id";
  skos:broader ble:Value;
  skos:definition """C5: Field exists if the key of bit 3 of the
      Flags field is set to 1""",
    """Unit is unitless with a resolution of
      1""", """Unit is unitless with a resoluton of
      1""";
  skos:inScheme ble:Scheme;
  skos:prefLabel "User ID";
  prov:wasDerivedFrom <file:/data/lp/etl/executor/data/1651932367716-22-f5b1c2e0-1947-4a2e-a814-6ce401f2a604/working/working-outputfiles-33/gatt-xml-master/org.bluetooth.characteristic.blood_pressure_measurement.xml>,
    <file:/data/lp/etl/executor/data/1651932367716-22-f5b1c2e0-1947-4a2e-a814-6ce401f2a604/working/working-outputfiles-33/gatt-xml-master/org.bluetooth.characteristic.body_composition_measurement.xml>,
    <file:/data/lp/etl/executor/data/1651932367716-22-f5b1c2e0-1947-4a2e-a814-6ce401f2a604/working/working-outputfiles-33/gatt-xml-master/org.bluetooth.characteristic.weight_measurement.xml> .

<http://purl.org/wot-catalogue/ble/gatt#org.bluetooth.characteristic.descriptor_value_changed>
  a skos:Concept, ontolex:LexicalConcept, prov:Entity;
  skos:altLabel "descriptor value changed";
  skos:broader ble:Characteristic;
  skos:inScheme ble:Scheme;
  skos:prefLabel "Descriptor Value Changed";
  skos:related ble:ExtendedProperties, ble:Indicate, ble:WritableAuxiliaries;
  prov:wasDerivedFrom <file:/data/lp/etl/executor/data/1651932367716-22-f5b1c2e0-1947-4a2e-a814-6ce401f2a604/working/working-outputfiles-33/gatt-xml-master/org.bluetooth.characteristic.descriptor_value_changed.xml> .

<http://purl.org/wot-catalogue/ble/gatt#1807> a skos:Concept, ontolex:LexicalConcept,
    prov:Entity;
  skos:altLabel "next dst change service";
  skos:broader ble:Service;
  skos:definition """This service enables a Bluetooth device that has
    knowledge about the next occurrence of a DST change to expose
    this information to another Bluetooth device.""";
  skos:inScheme ble:Scheme;
  skos:prefLabel "Next DST Change Service";
  skos:related ble:org.bluetooth.characteristic.time_with_dst;
  prov:wasDerivedFrom <file:/data/lp/etl/executor/data/1651932367716-22-f5b1c2e0-1947-4a2e-a814-6ce401f2a604/working/working-outputfiles-33/gatt-xml-master/org.bluetooth.service.next_dst_change.xml> .

<http://purl.org/wot-catalogue/ble/gatt#org.bluetooth.characteristic.time_with_dst>
  a skos:Concept, ontolex:LexicalConcept, prov:Entity;
  skos:altLabel "time with dst";
  skos:broader ble:Characteristic;
  skos:inScheme ble:Scheme;
  skos:prefLabel "Time with DST";
  skos:related ble:DSTOffset, ble:DateTime, ble:Read;
  prov:wasDerivedFrom <file:/data/lp/etl/executor/data/1651932367716-22-f5b1c2e0-1947-4a2e-a814-6ce401f2a604/working/working-outputfiles-33/gatt-xml-master/org.bluetooth.characteristic.time_with_dst.xml> .

<http://purl.org/wot-catalogue/ble/gatt#1812> a skos:Concept, ontolex:LexicalConcept,
    prov:Entity;
  skos:altLabel "human interface device";
  skos:broader ble:Service;
  skos:definition """The HID Service exposes characteristics required for a
    HID Device to transfer HID report descriptors and reports to a
    HID Host. This also exposes the characteristics for a HID Host
    to write to a Device. The Human Interface Device Service is
    instantiated as a Primary Service.""";
  skos:inScheme ble:Scheme;
  skos:prefLabel "Human Interface Device";
  skos:related ble:org.bluetooth.characteristic.boot_keyboard_input_report, ble:org.bluetooth.characteristic.boot_keyboard_output_report,
    ble:org.bluetooth.characteristic.boot_mouse_input_report, ble:org.bluetooth.characteristic.hid_control_point,
    ble:org.bluetooth.characteristic.hid_information, ble:org.bluetooth.characteristic.protocol_mode,
    ble:org.bluetooth.characteristic.report, ble:org.bluetooth.characteristic.report_map;
  prov:wasDerivedFrom <file:/data/lp/etl/executor/data/1651932367716-22-f5b1c2e0-1947-4a2e-a814-6ce401f2a604/working/working-outputfiles-33/gatt-xml-master/org.bluetooth.service.human_interface_device.xml> .

<http://purl.org/wot-catalogue/ble/gatt#org.bluetooth.characteristic.report> a skos:Concept,
    ontolex:LexicalConcept, prov:Entity;
  skos:altLabel "report";
  skos:broader ble:Characteristic;
  skos:definition """The Report characteristic value contains Input Report,
    Output Report or Feature Report data to be transferred between
    the HID Device and HID Host.""";
  skos:inScheme ble:Scheme;
  skos:prefLabel "Report";
  skos:related ble:InformationText, ble:Notify, ble:Read, ble:ReportValue, ble:Write,
    ble:WriteWithoutResponse;
  prov:wasDerivedFrom <file:/data/lp/etl/executor/data/1651932367716-22-f5b1c2e0-1947-4a2e-a814-6ce401f2a604/working/working-outputfiles-33/gatt-xml-master/org.bluetooth.characteristic.report.xml> .

<http://purl.org/wot-catalogue/ble/gatt#org.bluetooth.characteristic.report_map> a
    skos:Concept, ontolex:LexicalConcept, prov:Entity;
  skos:altLabel "report map";
  skos:broader ble:Characteristic;
  skos:definition """The Report Map characteristic is used to define
    formatting information for Input Report, Output Report, and
    Feature Report data transferred between a HID Device and HID
    Host, information on how this data can be used, and other
    information regarding physical aspects of the device (i.e. that
    the device functions as a keyboard, for example, or has
    multiple functions such as a keyboard and volume controls). 
    Only a single instance of this characteristic exists as part
    of a HID Service.""";
  skos:inScheme ble:Scheme;
  skos:prefLabel "Report Map";
  skos:related ble:Read, ble:ReportMapValue;
  prov:wasDerivedFrom <file:/data/lp/etl/executor/data/1651932367716-22-f5b1c2e0-1947-4a2e-a814-6ce401f2a604/working/working-outputfiles-33/gatt-xml-master/org.bluetooth.characteristic.report_map.xml> .

<http://purl.org/wot-catalogue/ble/gatt#org.bluetooth.characteristic.boot_keyboard_output_report>
  a skos:Concept, ontolex:LexicalConcept, prov:Entity;
  skos:altLabel "boot keyboard output report";
  skos:broader ble:Characteristic;
  skos:definition """The Boot Keyboard Output Report characteristic is used
    to transfer fixed format and length Output Report data between
    a HID Host operating in Boot Protocol Mode and a HID Service
    corresponding to a boot keyboard.""";
  skos:inScheme ble:Scheme;
  skos:prefLabel "Boot Keyboard Output Report";
  skos:related ble:BootKeyboardOutputReportValue, ble:Read, ble:Write, ble:WriteWithoutResponse;
  prov:wasDerivedFrom <file:/data/lp/etl/executor/data/1651932367716-22-f5b1c2e0-1947-4a2e-a814-6ce401f2a604/working/working-outputfiles-33/gatt-xml-master/org.bluetooth.characteristic.boot_keyboard_output_report.xml> .

<http://purl.org/wot-catalogue/ble/gatt#org.bluetooth.characteristic.hid_information>
  a skos:Concept, ontolex:LexicalConcept, prov:Entity;
  skos:altLabel "hid information";
  skos:broader ble:Characteristic;
  skos:definition """The HID Information Characteristic contains the HID
    attributes. The value of this Characteristic is static and can
    be cached for the lifetime of the bond between the HID device
    and the HID host.""";
  skos:inScheme ble:Scheme;
  skos:prefLabel "HID Information";
  skos:related ble:Flags, ble:Read, ble:bCountryCode, ble:bcdHID;
  prov:wasDerivedFrom <file:/data/lp/etl/executor/data/1651932367716-22-f5b1c2e0-1947-4a2e-a814-6ce401f2a604/working/working-outputfiles-33/gatt-xml-master/org.bluetooth.characteristic.hid_information.xml> .

<http://purl.org/wot-catalogue/ble/gatt#org.bluetooth.characteristic.hid_control_point>
  a skos:Concept, ontolex:LexicalConcept, prov:Entity;
  skos:altLabel "hid control point";
  skos:broader ble:Characteristic;
  skos:definition """The HID Control Point characteristic is a
    control-point attribute that defines the following HID Commands
    when written: 
    ? Suspend ( Refer to Section 7.4.2, Bluetooth HID Profile
    Specification 1.0? Exit Suspend (Refer to Section 7.4.2, Bluetooth HID
    Profile Specification 1.0""";
  skos:inScheme ble:Scheme;
  skos:prefLabel "HID Control Point";
  skos:related ble:HIDControlPointCommand, ble:WriteWithoutResponse;
  prov:wasDerivedFrom <file:/data/lp/etl/executor/data/1651932367716-22-f5b1c2e0-1947-4a2e-a814-6ce401f2a604/working/working-outputfiles-33/gatt-xml-master/org.bluetooth.characteristic.hid_control_point.xml> .

<http://purl.org/wot-catalogue/ble/gatt#org.bluetooth.characteristic.ln_control_point>
  a skos:Concept, ontolex:LexicalConcept, prov:Entity;
  skos:altLabel "ln control point";
  skos:broader ble:Characteristic;
  skos:definition """The LN Control Point characteristic is used to request
    a specific function to be executed on the receiving
    device.""";
  skos:inScheme ble:Scheme;
  skos:prefLabel "LN Control Point";
  skos:related ble:Indicate, ble:OpCodes, ble:ParameterValue, ble:RequestOpCode, ble:ResponseParameter,
    ble:ResponseValue, ble:Write;
  prov:wasDerivedFrom <file:/data/lp/etl/executor/data/1651932367716-22-f5b1c2e0-1947-4a2e-a814-6ce401f2a604/working/working-outputfiles-33/gatt-xml-master/org.bluetooth.characteristic.ln_control_point.xml> .

<http://purl.org/wot-catalogue/ble/gatt#org.bluetooth.characteristic.alert_notification_control_point>
  a skos:Concept, ontolex:LexicalConcept, prov:Entity;
  skos:altLabel "alert notification control point";
  skos:broader ble:Characteristic;
  skos:definition """The 1st octet value of the characteristic is an
    unsigned 8 bit integer that has a fixed point exponent of 0.
    The 1st octet value expresses the command ID that defines the
    server?s actions. 
    The 2nd octet value of the characteristic is an ?Alert
    Category ID? format. This octet shows the target category that
    the command ID applies for.""";
  skos:inScheme ble:Scheme;
  skos:prefLabel "Alert Notification Control Point";
  skos:related ble:CategoryID, ble:CommandID, ble:Write;
  prov:wasDerivedFrom <file:/data/lp/etl/executor/data/1651932367716-22-f5b1c2e0-1947-4a2e-a814-6ce401f2a604/working/working-outputfiles-33/gatt-xml-master/org.bluetooth.characteristic.alert_notification_control_point.xml> .

<http://purl.org/wot-catalogue/ble/gatt#CommandID> a skos:Concept, ontolex:LexicalConcept,
    prov:Entity;
  skos:altLabel "command id";
  skos:broader ble:Value;
  skos:inScheme ble:Scheme;
  skos:prefLabel "Command ID";
  prov:wasDerivedFrom <file:/data/lp/etl/executor/data/1651932367716-22-f5b1c2e0-1947-4a2e-a814-6ce401f2a604/working/working-outputfiles-33/gatt-xml-master/org.bluetooth.characteristic.alert_notification_control_point.xml> .

<http://purl.org/wot-catalogue/ble/gatt#181D> a skos:Concept, ontolex:LexicalConcept,
    prov:Entity;
  skos:altLabel "weight scale";
  skos:broader ble:Service;
  skos:definition """The Weight Scale (WS) Service exposes weight and
    related data from a weight scale (Server) intended for consumer
    healthcare as well as sports/fitness applications.""";
  skos:inScheme ble:Scheme;
  skos:prefLabel "Weight Scale";
  skos:related ble:org.bluetooth.characteristic.weight_measurement, ble:org.bluetooth.characteristic.weight_scale_feature;
  prov:wasDerivedFrom <file:/data/lp/etl/executor/data/1651932367716-22-f5b1c2e0-1947-4a2e-a814-6ce401f2a604/working/working-outputfiles-33/gatt-xml-master/org.bluetooth.service.weight_scale.xml> .

<http://purl.org/wot-catalogue/ble/gatt#org.bluetooth.characteristic.weight_scale_feature>
  a skos:Concept, ontolex:LexicalConcept, prov:Entity;
  skos:altLabel "weight scale feature";
  skos:broader ble:Characteristic;
  skos:inScheme ble:Scheme;
  skos:prefLabel "Weight Scale Feature";
  skos:related ble:Read, ble:WeightScaleFeature;
  prov:wasDerivedFrom <file:/data/lp/etl/executor/data/1651932367716-22-f5b1c2e0-1947-4a2e-a814-6ce401f2a604/working/working-outputfiles-33/gatt-xml-master/org.bluetooth.characteristic.weight_scale_feature.xml> .

<http://purl.org/wot-catalogue/ble/gatt#org.bluetooth.characteristic.weight_measurement>
  a skos:Concept, ontolex:LexicalConcept, prov:Entity;
  skos:altLabel "weight measurement";
  skos:broader ble:Characteristic;
  skos:inScheme ble:Scheme;
  skos:prefLabel "Weight Measurement";
  skos:related ble:BMI, ble:Flags, ble:Height-Imperial, ble:Height-SI, ble:Indicate,
    ble:TimeStamp, ble:UserID, ble:Weight-Imperial, ble:Weight-SI;
  prov:wasDerivedFrom <file:/data/lp/etl/executor/data/1651932367716-22-f5b1c2e0-1947-4a2e-a814-6ce401f2a604/working/working-outputfiles-33/gatt-xml-master/org.bluetooth.characteristic.weight_measurement.xml> .

<http://purl.org/wot-catalogue/ble/gatt#org.bluetooth.characteristic.digital> a skos:Concept,
    ontolex:LexicalConcept, prov:Entity;
  skos:altLabel "digital";
  skos:broader ble:Characteristic;
  skos:definition """The Digital characteristic is used to expose and
    change the state of an IO Module?s digital signals.""";
  skos:inScheme ble:Scheme;
  skos:prefLabel "Digital";
  skos:related ble:Digital, ble:Indicate, ble:Notify, ble:Read, ble:Write, ble:WriteWithoutResponse;
  prov:wasDerivedFrom <file:/data/lp/etl/executor/data/1651932367716-22-f5b1c2e0-1947-4a2e-a814-6ce401f2a604/working/working-outputfiles-33/gatt-xml-master/org.bluetooth.characteristic.digital.xml> .

<http://purl.org/wot-catalogue/ble/gatt#Digital> a skos:Concept, ontolex:LexicalConcept,
    prov:Entity;
  skos:altLabel "digital";
  skos:broader ble:Value;
  skos:definition """The Digital characteristic is an array of n
      2-bit values in a bit field""";
  skos:inScheme ble:Scheme;
  skos:prefLabel "Digital";
  prov:wasDerivedFrom <file:/data/lp/etl/executor/data/1651932367716-22-f5b1c2e0-1947-4a2e-a814-6ce401f2a604/working/working-outputfiles-33/gatt-xml-master/org.bluetooth.characteristic.digital.xml> .

<http://purl.org/wot-catalogue/ble/gatt#org.bluetooth.characteristic.glucose_measurement>
  a skos:Concept, ontolex:LexicalConcept, prov:Entity;
  skos:altLabel "glucose measurement";
  skos:broader ble:Characteristic;
  skos:definition """The Glucose Measurement characteristic is a variable
    length structure containing a Flags field, a Sequence Number
    field, a Base Time field and, based upon the contents of the
    Flags field, may contain a Time Offset field, Glucose
    Concentration field, Type-Sample Location field and a Sensor
    Status Annunciation field.""";
  skos:inScheme ble:Scheme;
  skos:prefLabel "Glucose Measurement";
  skos:related ble:BaseTime, ble:Flags, <http://purl.org/wot-catalogue/ble#GlucoseConcentration-unitsofkg/L>,
    <http://purl.org/wot-catalogue/ble#GlucoseConcentration-unitsofmol/L>, ble:Notify,
    ble:SampleLocation, ble:SensorStatusAnnunciation, ble:SequenceNumber, ble:TimeOffset,
    ble:Type;
  prov:wasDerivedFrom <file:/data/lp/etl/executor/data/1651932367716-22-f5b1c2e0-1947-4a2e-a814-6ce401f2a604/working/working-outputfiles-33/gatt-xml-master/org.bluetooth.characteristic.glucose_measurement.xml> .

<http://purl.org/wot-catalogue/ble/gatt#SequenceNumber> a skos:Concept, ontolex:LexicalConcept,
    prov:Entity;
  skos:altLabel "sequence number";
  skos:broader ble:Value;
  skos:inScheme ble:Scheme;
  skos:prefLabel "Sequence Number";
  prov:wasDerivedFrom <file:/data/lp/etl/executor/data/1651932367716-22-f5b1c2e0-1947-4a2e-a814-6ce401f2a604/working/working-outputfiles-33/gatt-xml-master/org.bluetooth.characteristic.glucose_measurement.xml>,
    <file:/data/lp/etl/executor/data/1651932367716-22-f5b1c2e0-1947-4a2e-a814-6ce401f2a604/working/working-outputfiles-33/gatt-xml-master/org.bluetooth.characteristic.glucose_measurement_context.xml> .

<http://purl.org/wot-catalogue/ble/gatt#BaseTime> a skos:Concept, ontolex:LexicalConcept,
    prov:Entity;
  skos:altLabel "base time";
  skos:broader ble:Value;
  skos:inScheme ble:Scheme;
  skos:prefLabel "Base Time";
  prov:wasDerivedFrom <file:/data/lp/etl/executor/data/1651932367716-22-f5b1c2e0-1947-4a2e-a814-6ce401f2a604/working/working-outputfiles-33/gatt-xml-master/org.bluetooth.characteristic.glucose_measurement.xml> .

<http://purl.org/wot-catalogue/ble/gatt#GlucoseConcentration-unitsofkg/L> a skos:Concept,
    ontolex:LexicalConcept, prov:Entity;
  skos:altLabel "glucose concentration - units of kg/l";
  skos:broader ble:Value;
  skos:definition """C2: Field exists if the key of bit 1 of the
      Flags field is set to 1, C3: Field exists if the key of bit 2
      of the Flags field is set to 0""";
  skos:inScheme ble:Scheme;
  skos:prefLabel "Glucose Concentration - units of kg/L";
  prov:wasDerivedFrom <file:/data/lp/etl/executor/data/1651932367716-22-f5b1c2e0-1947-4a2e-a814-6ce401f2a604/working/working-outputfiles-33/gatt-xml-master/org.bluetooth.characteristic.glucose_measurement.xml> .

<http://purl.org/wot-catalogue/ble/gatt#GlucoseConcentration-unitsofmol/L> a skos:Concept,
    ontolex:LexicalConcept, prov:Entity;
  skos:altLabel "glucose concentration - units of mol/l";
  skos:broader ble:Value;
  skos:definition """C2: Field exists if the key of bit 1 of the
      Flags field is set to 1, C4: Field exists if the key of bit 2
      of the Flags field is set to 1""";
  skos:inScheme ble:Scheme;
  skos:prefLabel "Glucose Concentration - units of mol/L";
  prov:wasDerivedFrom <file:/data/lp/etl/executor/data/1651932367716-22-f5b1c2e0-1947-4a2e-a814-6ce401f2a604/working/working-outputfiles-33/gatt-xml-master/org.bluetooth.characteristic.glucose_measurement.xml> .

<http://purl.org/wot-catalogue/ble/gatt#Type> a skos:Concept, ontolex:LexicalConcept,
    prov:Entity;
  skos:altLabel "type";
  skos:broader ble:Value;
  skos:definition """C2: Field exists if the key of bit 1 of the
      Flags field is set to 1""";
  skos:inScheme ble:Scheme;
  skos:prefLabel "Type";
  prov:wasDerivedFrom <file:/data/lp/etl/executor/data/1651932367716-22-f5b1c2e0-1947-4a2e-a814-6ce401f2a604/working/working-outputfiles-33/gatt-xml-master/org.bluetooth.characteristic.glucose_measurement.xml> .

<http://purl.org/wot-catalogue/ble/gatt#SampleLocation> a skos:Concept, ontolex:LexicalConcept,
    prov:Entity;
  skos:altLabel "sample location";
  skos:broader ble:Value;
  skos:definition """C2: Field exists if the key of bit 1 of the
      Flags field is set to 1""";
  skos:inScheme ble:Scheme;
  skos:prefLabel "Sample Location";
  prov:wasDerivedFrom <file:/data/lp/etl/executor/data/1651932367716-22-f5b1c2e0-1947-4a2e-a814-6ce401f2a604/working/working-outputfiles-33/gatt-xml-master/org.bluetooth.characteristic.glucose_measurement.xml> .

<http://purl.org/wot-catalogue/ble/gatt#SensorStatusAnnunciation> a skos:Concept,
    ontolex:LexicalConcept, prov:Entity;
  skos:altLabel "sensor status annunciation";
  skos:broader ble:Value;
  skos:definition """C5: Field exists if the key of bit 3 of the
      Flags field is set to 1""",
    """The Sensor Status Annunciation Field is an
      optional field comprising up to three octets. It is only
      attached if one or more bits are set to ?1?. Only the
      affected octet(s) shall be added and indicated by the Flags
      Field. The Sensor Status Annunciation Field shall be attached
      to every CGM Measurement Record to which the status
      applies.""";
  skos:inScheme ble:Scheme;
  skos:prefLabel "Sensor Status Annunciation";
  prov:wasDerivedFrom <file:/data/lp/etl/executor/data/1651932367716-22-f5b1c2e0-1947-4a2e-a814-6ce401f2a604/working/working-outputfiles-33/gatt-xml-master/org.bluetooth.characteristic.cgm_measurement.xml>,
    <file:/data/lp/etl/executor/data/1651932367716-22-f5b1c2e0-1947-4a2e-a814-6ce401f2a604/working/working-outputfiles-33/gatt-xml-master/org.bluetooth.characteristic.glucose_measurement.xml> .

<http://purl.org/wot-catalogue/ble/gatt#1803> a skos:Concept, ontolex:LexicalConcept,
    prov:Entity;
  skos:altLabel "link loss";
  skos:broader ble:Service;
  skos:definition """The LINK LOSS Service is instantiated as a Primary
    Service. There is only one instance of the Link Loss Service on
    a device. There is only one instance of the Alert Level
    characteristic in a Link Loss Service. This alert continues
    until one of following conditions occurs: ? An implementation
    specific timeout ? User interaction on this device ? A new
    alert level is written ? The physical link is
    disconnected""";
  skos:inScheme ble:Scheme;
  skos:prefLabel "Link Loss";
  skos:related ble:org.bluetooth.characteristic.alert_level;
  prov:wasDerivedFrom <file:/data/lp/etl/executor/data/1651932367716-22-f5b1c2e0-1947-4a2e-a814-6ce401f2a604/working/working-outputfiles-33/gatt-xml-master/org.bluetooth.service.link_loss.xml> .

<http://purl.org/wot-catalogue/ble/gatt#org.bluetooth.characteristic.alert_level>
  a skos:Concept, ontolex:LexicalConcept, prov:Entity;
  skos:altLabel "alert level";
  skos:broader ble:Characteristic;
  skos:definition """The value of the characteristic shall be an unsigned 8
    bit integer that has a fixed point exponent of 0. The Alert
    Level characteristic defines the level of alert, and is one of
    the following three values: 
    ? Value 0, meaning ?No Alert?? Value 1, meaning ?Mild Alert?? Value 2, meaning ?High Alert?""";
  skos:inScheme ble:Scheme;
  skos:prefLabel "Alert Level";
  skos:related ble:AlertLevel, ble:Read, ble:Write, ble:WriteWithoutResponse;
  prov:wasDerivedFrom <file:/data/lp/etl/executor/data/1651932367716-22-f5b1c2e0-1947-4a2e-a814-6ce401f2a604/working/working-outputfiles-33/gatt-xml-master/org.bluetooth.characteristic.alert_level.xml> .

<http://purl.org/wot-catalogue/ble/gatt#Level> a skos:Concept, ontolex:LexicalConcept,
    prov:Entity;
  skos:altLabel "level";
  skos:broader ble:Value;
  skos:inScheme ble:Scheme;
  skos:prefLabel "Level";
  prov:wasDerivedFrom <file:/data/lp/etl/executor/data/1651932367716-22-f5b1c2e0-1947-4a2e-a814-6ce401f2a604/working/working-outputfiles-33/gatt-xml-master/org.bluetooth.characteristic.battery_level.xml> .

<http://purl.org/wot-catalogue/ble/gatt#ReportMapValue> a skos:Concept, ontolex:LexicalConcept,
    prov:Entity;
  skos:altLabel "report map value";
  skos:broader ble:Value;
  skos:inScheme ble:Scheme;
  skos:prefLabel "Report Map Value";
  prov:wasDerivedFrom <file:/data/lp/etl/executor/data/1651932367716-22-f5b1c2e0-1947-4a2e-a814-6ce401f2a604/working/working-outputfiles-33/gatt-xml-master/org.bluetooth.characteristic.report_map.xml> .

<http://purl.org/wot-catalogue/ble/gatt#org.bluetooth.characteristic.magnetic_declination>
  a skos:Concept, ontolex:LexicalConcept, prov:Entity;
  skos:altLabel "magnetic declination";
  skos:broader ble:Characteristic;
  skos:inScheme ble:Scheme;
  skos:prefLabel "Magnetic Declination";
  skos:related ble:ExtendedProperties, ble:MagneticDeclination, ble:Notify, ble:Read,
    ble:WritableAuxiliaries;
  prov:wasDerivedFrom <file:/data/lp/etl/executor/data/1651932367716-22-f5b1c2e0-1947-4a2e-a814-6ce401f2a604/working/working-outputfiles-33/gatt-xml-master/org.bluetooth.characteristic.magnetic_declination.xml> .

<http://purl.org/wot-catalogue/ble/gatt#MagneticDeclination> a skos:Concept, ontolex:LexicalConcept,
    prov:Entity;
  skos:altLabel "magnetic declination";
  skos:broader ble:Value;
  skos:definition """Unit is in degrees with a resolution of 0.01
      degrees""";
  skos:inScheme ble:Scheme;
  skos:prefLabel "Magnetic Declination";
  prov:wasDerivedFrom <file:/data/lp/etl/executor/data/1651932367716-22-f5b1c2e0-1947-4a2e-a814-6ce401f2a604/working/working-outputfiles-33/gatt-xml-master/org.bluetooth.characteristic.magnetic_declination.xml> .

<http://purl.org/wot-catalogue/ble/gatt#1802> a skos:Concept, ontolex:LexicalConcept,
    prov:Entity;
  skos:altLabel "immediate alert";
  skos:broader ble:Service;
  skos:definition """The Immediate Alert service is instantiated as a
    Primary Service. There is only one instance of the Immediate
    Alert service on a device. There is only one instance of the
    Alert Level characteristic in an Immediate Alert service. This
    alert continues until one of following conditions occurs: ? An
    implementation specific timeout ? User interaction on this
    device ? A new alert level is written ? The physical link is
    disconnected""";
  skos:inScheme ble:Scheme;
  skos:prefLabel "Immediate Alert";
  skos:related ble:org.bluetooth.characteristic.alert_level;
  prov:wasDerivedFrom <file:/data/lp/etl/executor/data/1651932367716-22-f5b1c2e0-1947-4a2e-a814-6ce401f2a604/working/working-outputfiles-33/gatt-xml-master/org.bluetooth.service.immediate_alert.xml> .

<http://purl.org/wot-catalogue/ble/gatt#181B> a skos:Concept, ontolex:LexicalConcept,
    prov:Entity;
  skos:altLabel "body composition";
  skos:broader ble:Service;
  skos:definition """The Body Composition Service (BCS) exposes data
    related to body composition from a body composition analyzer
    (Server) intended for consumer healthcare as well as
    sports/fitness applications.""";
  skos:inScheme ble:Scheme;
  skos:prefLabel "Body Composition";
  skos:related ble:org.bluetooth.characteristic.body_composition_feature, ble:org.bluetooth.characteristic.body_composition_measurement;
  prov:wasDerivedFrom <file:/data/lp/etl/executor/data/1651932367716-22-f5b1c2e0-1947-4a2e-a814-6ce401f2a604/working/working-outputfiles-33/gatt-xml-master/org.bluetooth.service.body_composition.xml> .

<http://purl.org/wot-catalogue/ble/gatt#org.bluetooth.characteristic.body_composition_feature>
  a skos:Concept, ontolex:LexicalConcept, prov:Entity;
  skos:altLabel "body composition feature";
  skos:broader ble:Characteristic;
  skos:inScheme ble:Scheme;
  skos:prefLabel "Body Composition Feature";
  skos:related ble:BodyCompositionFeature, ble:Read;
  prov:wasDerivedFrom <file:/data/lp/etl/executor/data/1651932367716-22-f5b1c2e0-1947-4a2e-a814-6ce401f2a604/working/working-outputfiles-33/gatt-xml-master/org.bluetooth.characteristic.body_composition_feature.xml> .

<http://purl.org/wot-catalogue/ble/gatt#org.bluetooth.characteristic.body_composition_measurement>
  a skos:Concept, ontolex:LexicalConcept, prov:Entity;
  skos:altLabel "body composition measurement";
  skos:broader ble:Characteristic;
  skos:inScheme ble:Scheme;
  skos:prefLabel "Body Composition Measurement";
  skos:related ble:BasalMetabolism, ble:BodyFatPercentage, ble:BodyWaterMass-Kilograms,
    ble:BodyWaterMass-Pounds, ble:FatFreeMass-Kilograms, ble:FatFreeMass-Pounds, ble:Flags,
    ble:Height-Inches, ble:Height-Meters, ble:Impedance, ble:Indicate, ble:MuscleMass-Kilograms,
    ble:MuscleMass-Pounds, ble:MusclePercentage, ble:SoftLeanMass-Kilograms, ble:SoftLeanMass-Pounds,
    ble:TimeStamp, ble:UserID, ble:Weight-Kilograms, ble:Weight-Pounds;
  prov:wasDerivedFrom <file:/data/lp/etl/executor/data/1651932367716-22-f5b1c2e0-1947-4a2e-a814-6ce401f2a604/working/working-outputfiles-33/gatt-xml-master/org.bluetooth.characteristic.body_composition_measurement.xml> .

<http://purl.org/wot-catalogue/ble/gatt#MinimumHeartRate> a skos:Concept, ontolex:LexicalConcept,
    prov:Entity;
  skos:altLabel "minimum heart rate";
  skos:broader ble:Value;
  skos:definition """Beats per minute with a resolution of
      1""";
  skos:inScheme ble:Scheme;
  skos:prefLabel "Minimum Heart Rate";
  prov:wasDerivedFrom <file:/data/lp/etl/executor/data/1651932367716-22-f5b1c2e0-1947-4a2e-a814-6ce401f2a604/working/working-outputfiles-33/gatt-xml-master/org.bluetooth.characteristic.supported_heart_rate_range.xml> .

<http://purl.org/wot-catalogue/ble/gatt#MaximumHeartRate> a skos:Concept, ontolex:LexicalConcept,
    prov:Entity;
  skos:altLabel "maximum heart rate";
  skos:broader ble:Value;
  skos:definition """Beats per minute with a resolution of
      1""";
  skos:inScheme ble:Scheme;
  skos:prefLabel "Maximum Heart Rate";
  prov:wasDerivedFrom <file:/data/lp/etl/executor/data/1651932367716-22-f5b1c2e0-1947-4a2e-a814-6ce401f2a604/working/working-outputfiles-33/gatt-xml-master/org.bluetooth.characteristic.supported_heart_rate_range.xml> .

<http://purl.org/wot-catalogue/ble/gatt#181F> a skos:Concept, ontolex:LexicalConcept,
    prov:Entity;
  skos:altLabel "continuous glucose monitoring";
  skos:broader ble:Service;
  skos:definition """The Continuous Glucose Monitoring (CGM) Service
    exposes glucose measurement and other data related to a
    personal CGM sensor for healthcare applications.""";
  skos:inScheme ble:Scheme;
  skos:prefLabel "Continuous Glucose Monitoring";
  skos:related ble:org.bluetooth.characteristic.cgm_feature, ble:org.bluetooth.characteristic.cgm_measurement,
    ble:org.bluetooth.characteristic.cgm_session_run_time, ble:org.bluetooth.characteristic.cgm_session_start_time,
    ble:org.bluetooth.characteristic.cgm_specific_ops_control_point, ble:org.bluetooth.characteristic.cgm_status,
    ble:org.bluetooth.characteristic.record_access_control_point;
  prov:wasDerivedFrom <file:/data/lp/etl/executor/data/1651932367716-22-f5b1c2e0-1947-4a2e-a814-6ce401f2a604/working/working-outputfiles-33/gatt-xml-master/org.bluetooth.service.continuous_glucose_monitoring.xml> .

<http://purl.org/wot-catalogue/ble/gatt#org.bluetooth.characteristic.cgm_measurement>
  a skos:Concept, ontolex:LexicalConcept, prov:Entity;
  skos:altLabel "cgm measurement";
  skos:broader ble:Characteristic;
  skos:definition """The CGM Measurement characteristic is a variable
    length structure containing one or more CGM Measurement
    records, each comprising a Size field, a Flags Field, a Glucose
    Concentration field, a Time Offset field, a Sensor Status
    Annunciation field (optional), a CGM Trend Information Field
    (optional), a CGM Quality Field (optional), and an E2E-CRC
    Field (mandatory if this feature is supported).""";
  skos:inScheme ble:Scheme;
  skos:prefLabel "CGM Measurement";
  skos:related ble:CGMGlucoseConcentration, ble:CGMQuality, ble:CGMTrendInformation,
    ble:E2E-CRC, ble:Flags, ble:Notify, ble:SensorStatusAnnunciation, ble:Size, ble:TimeOffset;
  prov:wasDerivedFrom <file:/data/lp/etl/executor/data/1651932367716-22-f5b1c2e0-1947-4a2e-a814-6ce401f2a604/working/working-outputfiles-33/gatt-xml-master/org.bluetooth.characteristic.cgm_measurement.xml> .

<http://purl.org/wot-catalogue/ble/gatt#org.bluetooth.characteristic.cgm_session_start_time>
  a skos:Concept, ontolex:LexicalConcept, prov:Entity;
  skos:altLabel "cgm session start time";
  skos:broader ble:Characteristic;
  skos:inScheme ble:Scheme;
  skos:prefLabel "CGM Session Start Time";
  skos:related ble:DST-Offset, ble:E2E-CRC, ble:Read, ble:SessionStartTime, ble:TimeZone,
    ble:Write;
  prov:wasDerivedFrom <file:/data/lp/etl/executor/data/1651932367716-22-f5b1c2e0-1947-4a2e-a814-6ce401f2a604/working/working-outputfiles-33/gatt-xml-master/org.bluetooth.characteristic.cgm_session_start_time.xml> .

<http://purl.org/wot-catalogue/ble/gatt#SessionStartTime> a skos:Concept, ontolex:LexicalConcept,
    prov:Entity;
  skos:altLabel "session start time";
  skos:broader ble:Value;
  skos:definition """Same format as the Date Time Characteristic,
      smallest unit in seconds""";
  skos:inScheme ble:Scheme;
  skos:prefLabel "Session Start Time";
  prov:wasDerivedFrom <file:/data/lp/etl/executor/data/1651932367716-22-f5b1c2e0-1947-4a2e-a814-6ce401f2a604/working/working-outputfiles-33/gatt-xml-master/org.bluetooth.characteristic.cgm_session_start_time.xml> .

<http://purl.org/wot-catalogue/ble/gatt#DST-Offset> a skos:Concept, ontolex:LexicalConcept,
    prov:Entity;
  skos:altLabel "dst-offset";
  skos:broader ble:Value;
  skos:definition """Same format as the DST Offset
      Characteristic""";
  skos:inScheme ble:Scheme;
  skos:prefLabel "DST-Offset";
  prov:wasDerivedFrom <file:/data/lp/etl/executor/data/1651932367716-22-f5b1c2e0-1947-4a2e-a814-6ce401f2a604/working/working-outputfiles-33/gatt-xml-master/org.bluetooth.characteristic.cgm_session_start_time.xml> .

<http://purl.org/wot-catalogue/ble/gatt#BootKeyboardOutputReportValue> a skos:Concept,
    ontolex:LexicalConcept, prov:Entity;
  skos:altLabel "boot keyboard output report value";
  skos:broader ble:Value;
  skos:inScheme ble:Scheme;
  skos:prefLabel "Boot Keyboard Output Report Value";
  prov:wasDerivedFrom <file:/data/lp/etl/executor/data/1651932367716-22-f5b1c2e0-1947-4a2e-a814-6ce401f2a604/working/working-outputfiles-33/gatt-xml-master/org.bluetooth.characteristic.boot_keyboard_output_report.xml> .

<http://purl.org/wot-catalogue/ble/gatt#org.bluetooth.characteristic.database_change_increment>
  a skos:Concept, ontolex:LexicalConcept, prov:Entity;
  skos:altLabel "database change increment";
  skos:broader ble:Characteristic;
  skos:inScheme ble:Scheme;
  skos:prefLabel "Database Change Increment";
  skos:related ble:DatabaseChangeIncrement, ble:Notify, ble:Read, ble:Write;
  prov:wasDerivedFrom <file:/data/lp/etl/executor/data/1651932367716-22-f5b1c2e0-1947-4a2e-a814-6ce401f2a604/working/working-outputfiles-33/gatt-xml-master/org.bluetooth.characteristic.database_change_increment.xml> .

<http://purl.org/wot-catalogue/ble/gatt#DatabaseChangeIncrement> a skos:Concept, ontolex:LexicalConcept,
    prov:Entity;
  skos:altLabel "database change increment";
  skos:broader ble:Value;
  skos:definition "When read or notified, the Database Change Increment characteristic returns a value that is used by a Client to determine whether or not the UDS Characteristics need to be synchronized between the Server and the Client.";
  skos:inScheme ble:Scheme;
  skos:prefLabel "Database Change Increment";
  skos:related ble:DatabaseChangeIncrementValue, ble:Read, ble:Write;
  prov:wasDerivedFrom <file:/data/lp/etl/executor/data/1651932367716-22-f5b1c2e0-1947-4a2e-a814-6ce401f2a604/working/working-outputfiles-33/gatt-xml-master/org.bluetooth.characteristic.database_change_increment.xml> .

<http://purl.org/wot-catalogue/ble/gatt#org.bluetooth.characteristic.resting_heart_rate>
  a skos:Concept, ontolex:LexicalConcept, prov:Entity;
  skos:altLabel "resting heart rate";
  skos:broader ble:Characteristic;
  skos:definition "Lowest Heart Rate a user can reach";
  skos:inScheme ble:Scheme;
  skos:prefLabel "Resting Heart Rate";
  skos:related ble:Read, ble:RestingHeartRate, ble:Write;
  prov:wasDerivedFrom <file:/data/lp/etl/executor/data/1651932367716-22-f5b1c2e0-1947-4a2e-a814-6ce401f2a604/working/working-outputfiles-33/gatt-xml-master/org.bluetooth.characteristic.resting_heart_rate.xml> .

<http://purl.org/wot-catalogue/ble/gatt#RestingHeartRate> a skos:Concept, ontolex:LexicalConcept,
    prov:Entity;
  skos:altLabel "resting heart rate";
  skos:broader ble:Value;
  skos:definition """Unit is in beats per minute with a
      resolution of 1""";
  skos:inScheme ble:Scheme;
  skos:prefLabel "Resting Heart Rate";
  prov:wasDerivedFrom <file:/data/lp/etl/executor/data/1651932367716-22-f5b1c2e0-1947-4a2e-a814-6ce401f2a604/working/working-outputfiles-33/gatt-xml-master/org.bluetooth.characteristic.resting_heart_rate.xml> .

<http://purl.org/wot-catalogue/ble/gatt#MinimumInclination> a skos:Concept, ontolex:LexicalConcept,
    prov:Entity;
  skos:altLabel "minimum inclination";
  skos:broader ble:Value;
  skos:definition """Percent with a resolution of
      0.1""";
  skos:inScheme ble:Scheme;
  skos:prefLabel "Minimum Inclination";
  prov:wasDerivedFrom <file:/data/lp/etl/executor/data/1651932367716-22-f5b1c2e0-1947-4a2e-a814-6ce401f2a604/working/working-outputfiles-33/gatt-xml-master/org.bluetooth.characteristic.supported_inclination_range.xml> .

<http://purl.org/wot-catalogue/ble/gatt#MaximumInclination> a skos:Concept, ontolex:LexicalConcept,
    prov:Entity;
  skos:altLabel "maximum inclination";
  skos:broader ble:Value;
  skos:definition """Percent with a resolution of
      0.1""";
  skos:inScheme ble:Scheme;
  skos:prefLabel "Maximum Inclination";
  prov:wasDerivedFrom <file:/data/lp/etl/executor/data/1651932367716-22-f5b1c2e0-1947-4a2e-a814-6ce401f2a604/working/working-outputfiles-33/gatt-xml-master/org.bluetooth.characteristic.supported_inclination_range.xml> .

<http://purl.org/wot-catalogue/ble/gatt#Source> a skos:Concept, ontolex:LexicalConcept,
    prov:Entity;
  skos:altLabel "source";
  skos:broader ble:Value;
  skos:inScheme ble:Scheme;
  skos:prefLabel "Source";
  prov:wasDerivedFrom <file:/data/lp/etl/executor/data/1651932367716-22-f5b1c2e0-1947-4a2e-a814-6ce401f2a604/working/working-outputfiles-33/gatt-xml-master/org.bluetooth.characteristic.reference_time_information.xml> .

<http://purl.org/wot-catalogue/ble/gatt#Accuracy> a skos:Concept, ontolex:LexicalConcept,
    prov:Entity;
  skos:altLabel "accuracy";
  skos:broader ble:Value;
  skos:definition """Accuracy (drift) of time information in
      steps of 1/8 of a second (125ms) compared to a reference time
      source. Valid range from 0 to 253 (0s to 31.5s). A value of
      254 means Accuracy is out of range (> 31.5s). A value of
      255 means Accuracy is unknown.""";
  skos:inScheme ble:Scheme;
  skos:prefLabel "Accuracy";
  prov:wasDerivedFrom <file:/data/lp/etl/executor/data/1651932367716-22-f5b1c2e0-1947-4a2e-a814-6ce401f2a604/working/working-outputfiles-33/gatt-xml-master/org.bluetooth.characteristic.reference_time_information.xml>,
    <file:/data/lp/etl/executor/data/1651932367716-22-f5b1c2e0-1947-4a2e-a814-6ce401f2a604/working/working-outputfiles-33/gatt-xml-master/org.bluetooth.characteristic.time_accuracy.xml> .

<http://purl.org/wot-catalogue/ble/gatt#DaysSinceUpdate> a skos:Concept, ontolex:LexicalConcept,
    prov:Entity;
  skos:altLabel "days since update";
  skos:broader ble:Value;
  skos:inScheme ble:Scheme;
  skos:prefLabel "Days Since Update";
  prov:wasDerivedFrom <file:/data/lp/etl/executor/data/1651932367716-22-f5b1c2e0-1947-4a2e-a814-6ce401f2a604/working/working-outputfiles-33/gatt-xml-master/org.bluetooth.characteristic.reference_time_information.xml> .

<http://purl.org/wot-catalogue/ble/gatt#HoursSinceUpdate> a skos:Concept, ontolex:LexicalConcept,
    prov:Entity;
  skos:altLabel "hours since update";
  skos:broader ble:Value;
  skos:definition """If Days Since Update = 255, then Hours Since
      Update shall also be set to 255""";
  skos:inScheme ble:Scheme;
  skos:prefLabel "Hours Since Update";
  prov:wasDerivedFrom <file:/data/lp/etl/executor/data/1651932367716-22-f5b1c2e0-1947-4a2e-a814-6ce401f2a604/working/working-outputfiles-33/gatt-xml-master/org.bluetooth.characteristic.reference_time_information.xml> .

<http://purl.org/wot-catalogue/ble/gatt#PedalPowerBalance> a skos:Concept, ontolex:LexicalConcept,
    prov:Entity;
  skos:altLabel "pedal power balance";
  skos:broader ble:Value;
  skos:definition """Unit is in percentage with a resolution of
      1/2.""";
  skos:inScheme ble:Scheme;
  skos:prefLabel "Pedal Power Balance";
  prov:wasDerivedFrom <file:/data/lp/etl/executor/data/1651932367716-22-f5b1c2e0-1947-4a2e-a814-6ce401f2a604/working/working-outputfiles-33/gatt-xml-master/org.bluetooth.characteristic.cycling_power_measurement.xml> .

<http://purl.org/wot-catalogue/ble/gatt#AccumulatedTorque> a skos:Concept, ontolex:LexicalConcept,
    prov:Entity;
  skos:altLabel "accumulated torque";
  skos:broader ble:Value;
  skos:definition """Unit is in newton metres with a resolution
      of 1/32.""";
  skos:inScheme ble:Scheme;
  skos:prefLabel "Accumulated Torque";
  prov:wasDerivedFrom <file:/data/lp/etl/executor/data/1651932367716-22-f5b1c2e0-1947-4a2e-a814-6ce401f2a604/working/working-outputfiles-33/gatt-xml-master/org.bluetooth.characteristic.cycling_power_measurement.xml> .

<http://purl.org/wot-catalogue/ble/gatt#WheelRevolutionData-CumulativeWheelRevolutions>
  a skos:Concept, ontolex:LexicalConcept, prov:Entity;
  skos:altLabel "wheel revolution data - cumulative wheel revolutions";
  skos:broader ble:Value;
  skos:definition """Unitless 
      C1:When present, these fields are always present as a
      pair.""";
  skos:inScheme ble:Scheme;
  skos:prefLabel "Wheel Revolution Data - Cumulative Wheel Revolutions";
  prov:wasDerivedFrom <file:/data/lp/etl/executor/data/1651932367716-22-f5b1c2e0-1947-4a2e-a814-6ce401f2a604/working/working-outputfiles-33/gatt-xml-master/org.bluetooth.characteristic.cycling_power_measurement.xml> .

<http://purl.org/wot-catalogue/ble/gatt#WheelRevolutionData-LastWheelEventTime> a
    skos:Concept, ontolex:LexicalConcept, prov:Entity;
  skos:altLabel "wheel revolution data - last wheel event time";
  skos:broader ble:Value;
  skos:definition """Unit is in seconds with a resolution of
      1/2048. 
      C1:When present, these fields are always present as a
      pair.""";
  skos:inScheme ble:Scheme;
  skos:prefLabel "Wheel Revolution Data - Last Wheel Event Time";
  prov:wasDerivedFrom <file:/data/lp/etl/executor/data/1651932367716-22-f5b1c2e0-1947-4a2e-a814-6ce401f2a604/working/working-outputfiles-33/gatt-xml-master/org.bluetooth.characteristic.cycling_power_measurement.xml> .

<http://purl.org/wot-catalogue/ble/gatt#ExtremeForceMagnitudes-MaximumForceMagnitude>
  a skos:Concept, ontolex:LexicalConcept, prov:Entity;
  skos:altLabel "extreme force magnitudes - maximum force magnitude";
  skos:broader ble:Value;
  skos:definition """Unit is in newtons with a resolution of 1. 
      C3:When present, these fields are always present as a
      pair.""";
  skos:inScheme ble:Scheme;
  skos:prefLabel "Extreme Force Magnitudes - Maximum Force Magnitude";
  prov:wasDerivedFrom <file:/data/lp/etl/executor/data/1651932367716-22-f5b1c2e0-1947-4a2e-a814-6ce401f2a604/working/working-outputfiles-33/gatt-xml-master/org.bluetooth.characteristic.cycling_power_measurement.xml> .

<http://purl.org/wot-catalogue/ble/gatt#ExtremeForceMagnitudes-MinimumForceMagnitude>
  a skos:Concept, ontolex:LexicalConcept, prov:Entity;
  skos:altLabel "extreme force magnitudes - minimum force magnitude";
  skos:broader ble:Value;
  skos:definition """Unit is in newtons with a resolution of 1. 
      C3:When present, these fields are always present as a
      pair.""";
  skos:inScheme ble:Scheme;
  skos:prefLabel "Extreme Force Magnitudes - Minimum Force Magnitude";
  prov:wasDerivedFrom <file:/data/lp/etl/executor/data/1651932367716-22-f5b1c2e0-1947-4a2e-a814-6ce401f2a604/working/working-outputfiles-33/gatt-xml-master/org.bluetooth.characteristic.cycling_power_measurement.xml> .

<http://purl.org/wot-catalogue/ble/gatt#ExtremeTorqueMagnitudes-MaximumTorqueMagnitude>
  a skos:Concept, ontolex:LexicalConcept, prov:Entity;
  skos:altLabel "extreme torque magnitudes- maximum torque magnitude";
  skos:broader ble:Value;
  skos:definition """Unit is in newton metres with a resolution
      of 1/32. 
      C4:When present, these fields are always present as a
      pair.""";
  skos:inScheme ble:Scheme;
  skos:prefLabel "Extreme Torque Magnitudes- Maximum Torque Magnitude";
  prov:wasDerivedFrom <file:/data/lp/etl/executor/data/1651932367716-22-f5b1c2e0-1947-4a2e-a814-6ce401f2a604/working/working-outputfiles-33/gatt-xml-master/org.bluetooth.characteristic.cycling_power_measurement.xml> .

<http://purl.org/wot-catalogue/ble/gatt#ExtremeTorqueMagnitudes-MinimumTorqueMagnitude>
  a skos:Concept, ontolex:LexicalConcept, prov:Entity;
  skos:altLabel "extreme torque magnitudes- minimum torque magnitude";
  skos:broader ble:Value;
  skos:definition """Unit is in newton metres with a resolution
      of 1/32. 
      C4:When present, these fields are always present as a
      pair.""";
  skos:inScheme ble:Scheme;
  skos:prefLabel "Extreme Torque Magnitudes- Minimum Torque Magnitude";
  prov:wasDerivedFrom <file:/data/lp/etl/executor/data/1651932367716-22-f5b1c2e0-1947-4a2e-a814-6ce401f2a604/working/working-outputfiles-33/gatt-xml-master/org.bluetooth.characteristic.cycling_power_measurement.xml> .

<http://purl.org/wot-catalogue/ble/gatt#ExtremeAngles-MaximumAngle> a skos:Concept,
    ontolex:LexicalConcept, prov:Entity;
  skos:altLabel "extreme angles - maximum angle";
  skos:broader ble:Value;
  skos:definition """Unit is in degrees with a resolution of 1 
      C5: When present, this field and the \"Extreme Angles -
      Minimum Angle\" field are always present as a pair and are
      concatenated into a UINT24 value (3 octets). As an example,
      if the Maximum Angle is 0xABC and the Minimum Angle is 0x123,
      the transmitted value is 0x123ABC.""";
  skos:inScheme ble:Scheme;
  skos:prefLabel "Extreme Angles - Maximum Angle";
  prov:wasDerivedFrom <file:/data/lp/etl/executor/data/1651932367716-22-f5b1c2e0-1947-4a2e-a814-6ce401f2a604/working/working-outputfiles-33/gatt-xml-master/org.bluetooth.characteristic.cycling_power_measurement.xml> .

<http://purl.org/wot-catalogue/ble/gatt#ExtremeAngles-MinimumAngle> a skos:Concept,
    ontolex:LexicalConcept, prov:Entity;
  skos:altLabel "extreme angles - minimum angle";
  skos:broader ble:Value;
  skos:definition """Unit is in degrees with a resolution of 1. 
      C5: When present, this field and the \"Extreme Angles -
      Maximum Angle\" field are always present as a pair and are
      concatenated into a UINT24 value (3 octets). As an example,
      if the Maximum Angle is 0xABC and the Minimum Angle is 0x123,
      the transmitted value is 0x123ABC.""";
  skos:inScheme ble:Scheme;
  skos:prefLabel "Extreme Angles - Minimum Angle";
  prov:wasDerivedFrom <file:/data/lp/etl/executor/data/1651932367716-22-f5b1c2e0-1947-4a2e-a814-6ce401f2a604/working/working-outputfiles-33/gatt-xml-master/org.bluetooth.characteristic.cycling_power_measurement.xml> .

<http://purl.org/wot-catalogue/ble/gatt#TopDeadSpotAngle> a skos:Concept, ontolex:LexicalConcept,
    prov:Entity;
  skos:altLabel "top dead spot angle";
  skos:broader ble:Value;
  skos:definition """Unit is in degrees with a resolution of
      1.""";
  skos:inScheme ble:Scheme;
  skos:prefLabel "Top Dead Spot Angle";
  prov:wasDerivedFrom <file:/data/lp/etl/executor/data/1651932367716-22-f5b1c2e0-1947-4a2e-a814-6ce401f2a604/working/working-outputfiles-33/gatt-xml-master/org.bluetooth.characteristic.cycling_power_measurement.xml> .

<http://purl.org/wot-catalogue/ble/gatt#BottomDeadSpotAngle> a skos:Concept, ontolex:LexicalConcept,
    prov:Entity;
  skos:altLabel "bottom dead spot angle";
  skos:broader ble:Value;
  skos:definition """Unit is in degrees with a resolution of
      1.""";
  skos:inScheme ble:Scheme;
  skos:prefLabel "Bottom Dead Spot Angle";
  prov:wasDerivedFrom <file:/data/lp/etl/executor/data/1651932367716-22-f5b1c2e0-1947-4a2e-a814-6ce401f2a604/working/working-outputfiles-33/gatt-xml-master/org.bluetooth.characteristic.cycling_power_measurement.xml> .

<http://purl.org/wot-catalogue/ble/gatt#AccumulatedEnergy> a skos:Concept, ontolex:LexicalConcept,
    prov:Entity;
  skos:altLabel "accumulated energy";
  skos:broader ble:Value;
  skos:definition """Unit is in kilojoules with a resolution of
      1.""";
  skos:inScheme ble:Scheme;
  skos:prefLabel "Accumulated Energy";
  prov:wasDerivedFrom <file:/data/lp/etl/executor/data/1651932367716-22-f5b1c2e0-1947-4a2e-a814-6ce401f2a604/working/working-outputfiles-33/gatt-xml-master/org.bluetooth.characteristic.cycling_power_measurement.xml> .

<http://purl.org/wot-catalogue/ble/gatt#TimeUpdateControlPoint> a skos:Concept, ontolex:LexicalConcept,
    prov:Entity;
  skos:altLabel "time update control point";
  skos:broader ble:Value;
  skos:inScheme ble:Scheme;
  skos:prefLabel "Time Update Control Point";
  prov:wasDerivedFrom <file:/data/lp/etl/executor/data/1651932367716-22-f5b1c2e0-1947-4a2e-a814-6ce401f2a604/working/working-outputfiles-33/gatt-xml-master/org.bluetooth.characteristic.time_update_control_point.xml> .

<http://purl.org/wot-catalogue/ble/gatt#Latitude> a skos:Concept, ontolex:LexicalConcept,
    prov:Entity;
  skos:altLabel "latitude";
  skos:broader ble:Value;
  skos:inScheme ble:Scheme;
  skos:prefLabel "Latitude";
  prov:wasDerivedFrom <file:/data/lp/etl/executor/data/1651932367716-22-f5b1c2e0-1947-4a2e-a814-6ce401f2a604/working/working-outputfiles-33/gatt-xml-master/org.bluetooth.characteristic.latitude.xml> .

<http://purl.org/wot-catalogue/ble/gatt#SensorLocation> a skos:Concept, ontolex:LexicalConcept,
    prov:Entity;
  skos:altLabel "sensor location";
  skos:broader ble:Value;
  skos:definition "The Sensor Location characteristic of the device is used to describe the physical location of the Server when correctly fitted.";
  skos:inScheme ble:Scheme;
  skos:prefLabel "Sensor Location";
  skos:related ble:Read, xsd:unsignedByte;
  prov:wasDerivedFrom <file:/data/lp/etl/executor/data/1651932367716-22-f5b1c2e0-1947-4a2e-a814-6ce401f2a604/working/working-outputfiles-33/gatt-xml-master/org.bluetooth.characteristic.sensor_location.xml> .

<http://purl.org/wot-catalogue/ble/gatt#AlertLevel> a skos:Concept, ontolex:LexicalConcept,
    prov:Entity;
  skos:altLabel "alert level";
  skos:broader ble:Value;
  skos:definition "The Alert Level characteristic is a control point that allows a peer to command this device to alert to a given level.";
  skos:inScheme ble:Scheme;
  skos:prefLabel "Alert Level";
  skos:related ble:WritewithoutResponse;
  prov:wasDerivedFrom <file:/data/lp/etl/executor/data/1651932367716-22-f5b1c2e0-1947-4a2e-a814-6ce401f2a604/working/working-outputfiles-33/gatt-xml-master/org.bluetooth.characteristic.alert_level.xml> .

<http://purl.org/wot-catalogue/ble/gatt#BodyFatPercentage> a skos:Concept, ontolex:LexicalConcept,
    prov:Entity;
  skos:altLabel "body fat percentage";
  skos:broader ble:Value;
  skos:definition """Unit is in percent with a resolution of
      0.1""";
  skos:inScheme ble:Scheme;
  skos:prefLabel "Body Fat Percentage";
  prov:wasDerivedFrom <file:/data/lp/etl/executor/data/1651932367716-22-f5b1c2e0-1947-4a2e-a814-6ce401f2a604/working/working-outputfiles-33/gatt-xml-master/org.bluetooth.characteristic.body_composition_measurement.xml> .

<http://purl.org/wot-catalogue/ble/gatt#BasalMetabolism> a skos:Concept, ontolex:LexicalConcept,
    prov:Entity;
  skos:altLabel "basal metabolism";
  skos:broader ble:Value;
  skos:definition """Unit is in kilo Joules with a resolution of
      1""";
  skos:inScheme ble:Scheme;
  skos:prefLabel "Basal Metabolism";
  prov:wasDerivedFrom <file:/data/lp/etl/executor/data/1651932367716-22-f5b1c2e0-1947-4a2e-a814-6ce401f2a604/working/working-outputfiles-33/gatt-xml-master/org.bluetooth.characteristic.body_composition_measurement.xml> .

<http://purl.org/wot-catalogue/ble/gatt#MusclePercentage> a skos:Concept, ontolex:LexicalConcept,
    prov:Entity;
  skos:altLabel "muscle percentage";
  skos:broader ble:Value;
  skos:definition """Unit is in percentage with a resolution of
      0.1""";
  skos:inScheme ble:Scheme;
  skos:prefLabel "Muscle Percentage";
  prov:wasDerivedFrom <file:/data/lp/etl/executor/data/1651932367716-22-f5b1c2e0-1947-4a2e-a814-6ce401f2a604/working/working-outputfiles-33/gatt-xml-master/org.bluetooth.characteristic.body_composition_measurement.xml> .

<http://purl.org/wot-catalogue/ble/gatt#MuscleMass-Kilograms> a skos:Concept, ontolex:LexicalConcept,
    prov:Entity;
  skos:altLabel "muscle mass - kilograms";
  skos:broader ble:Value;
  skos:definition """Unit is in kilograms with resolution 0.005.
      Note: Determined when bit 0 of the Flags field is set to
      0.""";
  skos:inScheme ble:Scheme;
  skos:prefLabel "Muscle Mass - Kilograms";
  prov:wasDerivedFrom <file:/data/lp/etl/executor/data/1651932367716-22-f5b1c2e0-1947-4a2e-a814-6ce401f2a604/working/working-outputfiles-33/gatt-xml-master/org.bluetooth.characteristic.body_composition_measurement.xml> .

<http://purl.org/wot-catalogue/ble/gatt#MuscleMass-Pounds> a skos:Concept, ontolex:LexicalConcept,
    prov:Entity;
  skos:altLabel "muscle mass - pounds";
  skos:broader ble:Value;
  skos:definition """Unit is in pounds with resolution 0.01.
      Note: Determined when bit 0 of the Flags field is set to
      1.""";
  skos:inScheme ble:Scheme;
  skos:prefLabel "Muscle Mass - Pounds";
  prov:wasDerivedFrom <file:/data/lp/etl/executor/data/1651932367716-22-f5b1c2e0-1947-4a2e-a814-6ce401f2a604/working/working-outputfiles-33/gatt-xml-master/org.bluetooth.characteristic.body_composition_measurement.xml> .

<http://purl.org/wot-catalogue/ble/gatt#FatFreeMass-Kilograms> a skos:Concept, ontolex:LexicalConcept,
    prov:Entity;
  skos:altLabel "fat free mass - kilograms";
  skos:broader ble:Value;
  skos:definition """Unit is in kilograms with resolution 0.005.
      Note: Determined when bit 0 of the Flags field is set to
      0.""";
  skos:inScheme ble:Scheme;
  skos:prefLabel "Fat Free Mass - Kilograms";
  prov:wasDerivedFrom <file:/data/lp/etl/executor/data/1651932367716-22-f5b1c2e0-1947-4a2e-a814-6ce401f2a604/working/working-outputfiles-33/gatt-xml-master/org.bluetooth.characteristic.body_composition_measurement.xml> .

<http://purl.org/wot-catalogue/ble/gatt#FatFreeMass-Pounds> a skos:Concept, ontolex:LexicalConcept,
    prov:Entity;
  skos:altLabel "fat free mass - pounds";
  skos:broader ble:Value;
  skos:definition """Unit is in pounds with a resolution of 0.01.
      Note: Determined when bit 0 of the Flags field is set to
      1.""";
  skos:inScheme ble:Scheme;
  skos:prefLabel "Fat Free Mass - Pounds";
  prov:wasDerivedFrom <file:/data/lp/etl/executor/data/1651932367716-22-f5b1c2e0-1947-4a2e-a814-6ce401f2a604/working/working-outputfiles-33/gatt-xml-master/org.bluetooth.characteristic.body_composition_measurement.xml> .

<http://purl.org/wot-catalogue/ble/gatt#SoftLeanMass-Kilograms> a skos:Concept, ontolex:LexicalConcept,
    prov:Entity;
  skos:altLabel "soft lean mass - kilograms";
  skos:broader ble:Value;
  skos:definition """Unit is in kilograms with a resolution of
      0.005. Note: Determined when bit 0 of the Flags field is set
      to 0.""";
  skos:inScheme ble:Scheme;
  skos:prefLabel "Soft Lean Mass - Kilograms";
  prov:wasDerivedFrom <file:/data/lp/etl/executor/data/1651932367716-22-f5b1c2e0-1947-4a2e-a814-6ce401f2a604/working/working-outputfiles-33/gatt-xml-master/org.bluetooth.characteristic.body_composition_measurement.xml> .

<http://purl.org/wot-catalogue/ble/gatt#SoftLeanMass-Pounds> a skos:Concept, ontolex:LexicalConcept,
    prov:Entity;
  skos:altLabel "soft lean mass - pounds";
  skos:broader ble:Value;
  skos:definition """Unit is in pounds with a resolution of 0.01.
      Note: Determined when bit 0 of the Flags field is set to
      1.""";
  skos:inScheme ble:Scheme;
  skos:prefLabel "Soft Lean Mass - Pounds";
  prov:wasDerivedFrom <file:/data/lp/etl/executor/data/1651932367716-22-f5b1c2e0-1947-4a2e-a814-6ce401f2a604/working/working-outputfiles-33/gatt-xml-master/org.bluetooth.characteristic.body_composition_measurement.xml> .

<http://purl.org/wot-catalogue/ble/gatt#BodyWaterMass-Kilograms> a skos:Concept, ontolex:LexicalConcept,
    prov:Entity;
  skos:altLabel "body water mass - kilograms";
  skos:broader ble:Value;
  skos:definition """Unit is in kilograms with a resolution of
      0.005. Note: Determined when bit 0 of the Flags field is set
      to 0.""";
  skos:inScheme ble:Scheme;
  skos:prefLabel "Body Water Mass - Kilograms";
  prov:wasDerivedFrom <file:/data/lp/etl/executor/data/1651932367716-22-f5b1c2e0-1947-4a2e-a814-6ce401f2a604/working/working-outputfiles-33/gatt-xml-master/org.bluetooth.characteristic.body_composition_measurement.xml> .

<http://purl.org/wot-catalogue/ble/gatt#BodyWaterMass-Pounds> a skos:Concept, ontolex:LexicalConcept,
    prov:Entity;
  skos:altLabel "body water mass - pounds";
  skos:broader ble:Value;
  skos:definition """Unit is in pounds with a resolution of 0.01.
      Note: Determined when bit 0 of the Flags field is set to
      1.""";
  skos:inScheme ble:Scheme;
  skos:prefLabel "Body Water Mass - Pounds";
  prov:wasDerivedFrom <file:/data/lp/etl/executor/data/1651932367716-22-f5b1c2e0-1947-4a2e-a814-6ce401f2a604/working/working-outputfiles-33/gatt-xml-master/org.bluetooth.characteristic.body_composition_measurement.xml> .

<http://purl.org/wot-catalogue/ble/gatt#Impedance> a skos:Concept, ontolex:LexicalConcept,
    prov:Entity;
  skos:altLabel "impedance";
  skos:broader ble:Value;
  skos:definition """Unit is in Ohms with a resolution of
      0.1""";
  skos:inScheme ble:Scheme;
  skos:prefLabel "Impedance";
  prov:wasDerivedFrom <file:/data/lp/etl/executor/data/1651932367716-22-f5b1c2e0-1947-4a2e-a814-6ce401f2a604/working/working-outputfiles-33/gatt-xml-master/org.bluetooth.characteristic.body_composition_measurement.xml> .

<http://purl.org/wot-catalogue/ble/gatt#Weight-Kilograms> a skos:Concept, ontolex:LexicalConcept,
    prov:Entity;
  skos:altLabel "weight - kilograms";
  skos:broader ble:Value;
  skos:definition """Unit is in kilograms with a resolution of
      0.005. Note: Determined when bit 0 of the Flags field is set
      to 0.""";
  skos:inScheme ble:Scheme;
  skos:prefLabel "Weight - Kilograms";
  prov:wasDerivedFrom <file:/data/lp/etl/executor/data/1651932367716-22-f5b1c2e0-1947-4a2e-a814-6ce401f2a604/working/working-outputfiles-33/gatt-xml-master/org.bluetooth.characteristic.body_composition_measurement.xml> .

<http://purl.org/wot-catalogue/ble/gatt#Weight-Pounds> a skos:Concept, ontolex:LexicalConcept,
    prov:Entity;
  skos:altLabel "weight - pounds";
  skos:broader ble:Value;
  skos:definition """Unit is in pounds with a resolution of 0.01.
      Note: Determined when bit 0 of the Flags field is set to
      1.""";
  skos:inScheme ble:Scheme;
  skos:prefLabel "Weight - Pounds";
  prov:wasDerivedFrom <file:/data/lp/etl/executor/data/1651932367716-22-f5b1c2e0-1947-4a2e-a814-6ce401f2a604/working/working-outputfiles-33/gatt-xml-master/org.bluetooth.characteristic.body_composition_measurement.xml> .

<http://purl.org/wot-catalogue/ble/gatt#Height-Meters> a skos:Concept, ontolex:LexicalConcept,
    prov:Entity;
  skos:altLabel "height - meters";
  skos:broader ble:Value;
  skos:definition """Unit is in meters with a resolution of
      0.001. Note: Determined when bit 0 of the Flags field is set
      to 0.""";
  skos:inScheme ble:Scheme;
  skos:prefLabel "Height - Meters";
  prov:wasDerivedFrom <file:/data/lp/etl/executor/data/1651932367716-22-f5b1c2e0-1947-4a2e-a814-6ce401f2a604/working/working-outputfiles-33/gatt-xml-master/org.bluetooth.characteristic.body_composition_measurement.xml> .

<http://purl.org/wot-catalogue/ble/gatt#Height-Inches> a skos:Concept, ontolex:LexicalConcept,
    prov:Entity;
  skos:altLabel "height - inches";
  skos:broader ble:Value;
  skos:definition """Unit is in meters with a resolution of 0.1.
      Note: Determined when bit 0 of the Flags field is set to
      1.""";
  skos:inScheme ble:Scheme;
  skos:prefLabel "Height - Inches";
  prov:wasDerivedFrom <file:/data/lp/etl/executor/data/1651932367716-22-f5b1c2e0-1947-4a2e-a814-6ce401f2a604/working/working-outputfiles-33/gatt-xml-master/org.bluetooth.characteristic.body_composition_measurement.xml> .

<http://purl.org/wot-catalogue/ble/gatt#Weight-SI> a skos:Concept, ontolex:LexicalConcept,
    prov:Entity;
  skos:altLabel "weight - si";
  skos:broader ble:Value;
  skos:definition """Unit is in kilograms with a resolution of
      0.005, and determined when bit 0 of the Flags field is set to
      0.""";
  skos:inScheme ble:Scheme;
  skos:prefLabel "Weight - SI";
  prov:wasDerivedFrom <file:/data/lp/etl/executor/data/1651932367716-22-f5b1c2e0-1947-4a2e-a814-6ce401f2a604/working/working-outputfiles-33/gatt-xml-master/org.bluetooth.characteristic.weight_measurement.xml> .

<http://purl.org/wot-catalogue/ble/gatt#Weight-Imperial> a skos:Concept, ontolex:LexicalConcept,
    prov:Entity;
  skos:altLabel "weight - imperial";
  skos:broader ble:Value;
  skos:definition """Unit is in pounds with a resolution of 0.01,
      and determined when bit 0 of the Flags field is set to
      1.""";
  skos:inScheme ble:Scheme;
  skos:prefLabel "Weight - Imperial";
  prov:wasDerivedFrom <file:/data/lp/etl/executor/data/1651932367716-22-f5b1c2e0-1947-4a2e-a814-6ce401f2a604/working/working-outputfiles-33/gatt-xml-master/org.bluetooth.characteristic.weight_measurement.xml> .

<http://purl.org/wot-catalogue/ble/gatt#BMI> a skos:Concept, ontolex:LexicalConcept,
    prov:Entity;
  skos:altLabel "bmi";
  skos:broader ble:Value;
  skos:definition """Unit is unitless with a resolution of
      0.1""";
  skos:inScheme ble:Scheme;
  skos:prefLabel "BMI";
  prov:wasDerivedFrom <file:/data/lp/etl/executor/data/1651932367716-22-f5b1c2e0-1947-4a2e-a814-6ce401f2a604/working/working-outputfiles-33/gatt-xml-master/org.bluetooth.characteristic.weight_measurement.xml> .

<http://purl.org/wot-catalogue/ble/gatt#Height-SI> a skos:Concept, ontolex:LexicalConcept,
    prov:Entity;
  skos:altLabel "height - si";
  skos:broader ble:Value;
  skos:definition """Unit is in meters with a resolution of
      0.001, and determined when bit 0 of the Flags field is set to
      0.""";
  skos:inScheme ble:Scheme;
  skos:prefLabel "Height - SI";
  prov:wasDerivedFrom <file:/data/lp/etl/executor/data/1651932367716-22-f5b1c2e0-1947-4a2e-a814-6ce401f2a604/working/working-outputfiles-33/gatt-xml-master/org.bluetooth.characteristic.weight_measurement.xml> .

<http://purl.org/wot-catalogue/ble/gatt#Height-Imperial> a skos:Concept, ontolex:LexicalConcept,
    prov:Entity;
  skos:altLabel "height - imperial";
  skos:broader ble:Value;
  skos:definition """Unit is in inches with a resolution of 0.1,
      and determined when bit 0 of the Flags field is set to
      1""";
  skos:inScheme ble:Scheme;
  skos:prefLabel "Height - Imperial";
  prov:wasDerivedFrom <file:/data/lp/etl/executor/data/1651932367716-22-f5b1c2e0-1947-4a2e-a814-6ce401f2a604/working/working-outputfiles-33/gatt-xml-master/org.bluetooth.characteristic.weight_measurement.xml> .

<http://purl.org/wot-catalogue/ble/gatt#org.bluetooth.characteristic.navigation> a
    skos:Concept, ontolex:LexicalConcept, prov:Entity;
  skos:altLabel "navigation";
  skos:broader ble:Characteristic;
  skos:definition """The Navigation characteristic is a variable length
    structure containing a Flags field, a Bearing field, a Heading
    field and, based on the contents of the Flags field, may
    contain a combination of data fields listed below.""";
  skos:inScheme ble:Scheme;
  skos:prefLabel "Navigation";
  skos:related ble:Bearing, ble:EstimatedTimeofArrival, ble:Flags, ble:Heading, ble:Notify,
    ble:RemainingDistance, ble:RemainingVerticalDistance;
  prov:wasDerivedFrom <file:/data/lp/etl/executor/data/1651932367716-22-f5b1c2e0-1947-4a2e-a814-6ce401f2a604/working/working-outputfiles-33/gatt-xml-master/org.bluetooth.characteristic.navigation.xml> .

<http://purl.org/wot-catalogue/ble/gatt#Bearing> a skos:Concept, ontolex:LexicalConcept,
    prov:Entity;
  skos:altLabel "bearing";
  skos:broader ble:Value;
  skos:definition """Unit is in degrees with a resolution of
      1/100""";
  skos:inScheme ble:Scheme;
  skos:prefLabel "Bearing";
  prov:wasDerivedFrom <file:/data/lp/etl/executor/data/1651932367716-22-f5b1c2e0-1947-4a2e-a814-6ce401f2a604/working/working-outputfiles-33/gatt-xml-master/org.bluetooth.characteristic.navigation.xml> .

<http://purl.org/wot-catalogue/ble/gatt#Heading> a skos:Concept, ontolex:LexicalConcept,
    prov:Entity;
  skos:altLabel "heading";
  skos:broader ble:Value;
  skos:definition """Unit is in degrees with a resolution of
      1/100""";
  skos:inScheme ble:Scheme;
  skos:prefLabel "Heading";
  prov:wasDerivedFrom <file:/data/lp/etl/executor/data/1651932367716-22-f5b1c2e0-1947-4a2e-a814-6ce401f2a604/working/working-outputfiles-33/gatt-xml-master/org.bluetooth.characteristic.location_and_speed.xml>,
    <file:/data/lp/etl/executor/data/1651932367716-22-f5b1c2e0-1947-4a2e-a814-6ce401f2a604/working/working-outputfiles-33/gatt-xml-master/org.bluetooth.characteristic.navigation.xml> .

<http://purl.org/wot-catalogue/ble/gatt#RemainingDistance> a skos:Concept, ontolex:LexicalConcept,
    prov:Entity;
  skos:altLabel "remaining distance";
  skos:broader ble:Value;
  skos:definition """Unit is in meters with a resolution of
      1/10""";
  skos:inScheme ble:Scheme;
  skos:prefLabel "Remaining Distance";
  prov:wasDerivedFrom <file:/data/lp/etl/executor/data/1651932367716-22-f5b1c2e0-1947-4a2e-a814-6ce401f2a604/working/working-outputfiles-33/gatt-xml-master/org.bluetooth.characteristic.navigation.xml> .

<http://purl.org/wot-catalogue/ble/gatt#RemainingVerticalDistance> a skos:Concept,
    ontolex:LexicalConcept, prov:Entity;
  skos:altLabel "remaining vertical distance";
  skos:broader ble:Value;
  skos:definition """Unit is in meters with a resolution of
      1/100""";
  skos:inScheme ble:Scheme;
  skos:prefLabel "Remaining Vertical Distance";
  prov:wasDerivedFrom <file:/data/lp/etl/executor/data/1651932367716-22-f5b1c2e0-1947-4a2e-a814-6ce401f2a604/working/working-outputfiles-33/gatt-xml-master/org.bluetooth.characteristic.navigation.xml> .

<http://purl.org/wot-catalogue/ble/gatt#EstimatedTimeofArrival> a skos:Concept, ontolex:LexicalConcept,
    prov:Entity;
  skos:altLabel "estimated time of arrival";
  skos:broader ble:Value;
  skos:definition "Smallest units in seconds";
  skos:inScheme ble:Scheme;
  skos:prefLabel "Estimated Time of Arrival";
  prov:wasDerivedFrom <file:/data/lp/etl/executor/data/1651932367716-22-f5b1c2e0-1947-4a2e-a814-6ce401f2a604/working/working-outputfiles-33/gatt-xml-master/org.bluetooth.characteristic.navigation.xml> .

<http://purl.org/wot-catalogue/ble/gatt#org.bluetooth.characteristic.waist_circumference>
  a skos:Concept, ontolex:LexicalConcept, prov:Entity;
  skos:altLabel "waist circumference";
  skos:broader ble:Characteristic;
  skos:definition """Used with the Hip Circumference value to calculate
    the Waist to Hip Ratio (WHR)""";
  skos:inScheme ble:Scheme;
  skos:prefLabel "Waist Circumference";
  skos:related ble:Read, ble:WaistCircumference, ble:Write;
  prov:wasDerivedFrom <file:/data/lp/etl/executor/data/1651932367716-22-f5b1c2e0-1947-4a2e-a814-6ce401f2a604/working/working-outputfiles-33/gatt-xml-master/org.bluetooth.characteristic.waist_circumference.xml> .

<http://purl.org/wot-catalogue/ble/gatt#WaistCircumference> a skos:Concept, ontolex:LexicalConcept,
    prov:Entity;
  skos:altLabel "waist circumference";
  skos:broader ble:Value;
  skos:definition """Unit is in meters with a resolution of
      0.01""";
  skos:inScheme ble:Scheme;
  skos:prefLabel "Waist Circumference";
  prov:wasDerivedFrom <file:/data/lp/etl/executor/data/1651932367716-22-f5b1c2e0-1947-4a2e-a814-6ce401f2a604/working/working-outputfiles-33/gatt-xml-master/org.bluetooth.characteristic.waist_circumference.xml> .

<http://purl.org/wot-catalogue/ble/gatt#ObjectName> a skos:Concept, ontolex:LexicalConcept,
    prov:Entity;
  skos:altLabel "object name";
  skos:broader ble:Value;
  skos:definition """The length of the field value is variable
      from 0 octets to 120 octets.""";
  skos:inScheme ble:Scheme;
  skos:prefLabel "Object Name";
  prov:wasDerivedFrom <file:/data/lp/etl/executor/data/1651932367716-22-f5b1c2e0-1947-4a2e-a814-6ce401f2a604/working/working-outputfiles-33/gatt-xml-master/org.bluetooth.characteristic.object_name.xml> .

<http://purl.org/wot-catalogue/ble/gatt#org.bluetooth.characteristic.Longitude> a
    skos:Concept, ontolex:LexicalConcept, prov:Entity;
  skos:altLabel "longitude";
  skos:broader ble:Characteristic;
  skos:definition """The Longitude characteristic describes the WGS84 East
    coordinate of the device.""";
  skos:inScheme ble:Scheme;
  skos:prefLabel "Longitude";
  skos:related ble:Longitude;
  prov:wasDerivedFrom <file:/data/lp/etl/executor/data/1651932367716-22-f5b1c2e0-1947-4a2e-a814-6ce401f2a604/working/working-outputfiles-33/gatt-xml-master/org.bluetooth.characteristic.longitude.xml> .

<http://purl.org/wot-catalogue/ble/gatt#Longitude> a skos:Concept, ontolex:LexicalConcept,
    prov:Entity;
  skos:altLabel "longitude";
  skos:broader ble:Value;
  skos:inScheme ble:Scheme;
  skos:prefLabel "Longitude";
  prov:wasDerivedFrom <file:/data/lp/etl/executor/data/1651932367716-22-f5b1c2e0-1947-4a2e-a814-6ce401f2a604/working/working-outputfiles-33/gatt-xml-master/org.bluetooth.characteristic.longitude.xml> .

<http://purl.org/wot-catalogue/ble/gatt#181C> a skos:Concept, ontolex:LexicalConcept,
    prov:Entity;
  skos:altLabel "user data";
  skos:broader ble:Service;
  skos:definition """The User Data Service (UDS) exposes user-related data
    in the sports and fitness environment. This allows remote
    access and update of user data by a Client as well as the
    synchronization of user data between a Server and a
    Client.""";
  skos:inScheme ble:Scheme;
  skos:prefLabel "User Data";
  skos:related ble:org.bluetooth.characteristic.aerobic_heart_rate_lower_limit, ble:org.bluetooth.characteristic.aerobic_heart_rate_upper_limit,
    ble:org.bluetooth.characteristic.aerobic_threshold, ble:org.bluetooth.characteristic.age,
    ble:org.bluetooth.characteristic.anaerobic_heart_rate_lower_limit, ble:org.bluetooth.characteristic.anaerobic_heart_rate_upper_limit,
    ble:org.bluetooth.characteristic.anaerobic_threshold, ble:org.bluetooth.characteristic.database_change_increment,
    ble:org.bluetooth.characteristic.date_of_birth, ble:org.bluetooth.characteristic.date_of_threshold_assessment,
    ble:org.bluetooth.characteristic.email_address, ble:org.bluetooth.characteristic.fat_burn_heart_rate_lower_limit,
    ble:org.bluetooth.characteristic.fat_burn_heart_rate_upper_limit, ble:org.bluetooth.characteristic.first_name,
    ble:org.bluetooth.characteristic.five_zone_heart_rate_limits, ble:org.bluetooth.characteristic.gender,
    ble:org.bluetooth.characteristic.heart_rate_max, ble:org.bluetooth.characteristic.height,
    ble:org.bluetooth.characteristic.hip_circumference, ble:org.bluetooth.characteristic.language,
    ble:org.bluetooth.characteristic.last_name, ble:org.bluetooth.characteristic.maximum_recommended_heart_rate,
    ble:org.bluetooth.characteristic.resting_heart_rate, ble:org.bluetooth.characteristic.sport_type_for_aerobic_and_anaerobic_thresholds,
    ble:org.bluetooth.characteristic.three_zone_heart_rate_limits, ble:org.bluetooth.characteristic.two_zone_heart_rate_limit,
    ble:org.bluetooth.characteristic.user_control_point, ble:org.bluetooth.characteristic.user_index,
    ble:org.bluetooth.characteristic.vo2_max, ble:org.bluetooth.characteristic.waist_circumference,
    ble:org.bluetooth.characteristic.weight;
  prov:wasDerivedFrom <file:/data/lp/etl/executor/data/1651932367716-22-f5b1c2e0-1947-4a2e-a814-6ce401f2a604/working/working-outputfiles-33/gatt-xml-master/org.bluetooth.service.user_data.xml> .

<http://purl.org/wot-catalogue/ble/gatt#org.bluetooth.characteristic.email_address>
  a skos:Concept, ontolex:LexicalConcept, prov:Entity;
  skos:altLabel "email address";
  skos:broader ble:Characteristic;
  skos:definition "Email address of the user. See Note below.";
  skos:inScheme ble:Scheme;
  skos:prefLabel "Email Address";
  skos:related ble:EmailAddress, ble:Read, ble:Write;
  prov:wasDerivedFrom <file:/data/lp/etl/executor/data/1651932367716-22-f5b1c2e0-1947-4a2e-a814-6ce401f2a604/working/working-outputfiles-33/gatt-xml-master/org.bluetooth.characteristic.email_address.xml> .

<http://purl.org/wot-catalogue/ble/gatt#org.bluetooth.characteristic.age> a skos:Concept,
    ontolex:LexicalConcept, prov:Entity;
  skos:altLabel "age";
  skos:broader ble:Characteristic;
  skos:definition "Age of the User.";
  skos:inScheme ble:Scheme;
  skos:prefLabel "Age";
  skos:related ble:Age, ble:Read, ble:Write;
  prov:wasDerivedFrom <file:/data/lp/etl/executor/data/1651932367716-22-f5b1c2e0-1947-4a2e-a814-6ce401f2a604/working/working-outputfiles-33/gatt-xml-master/org.bluetooth.characteristic.age.xml> .

<http://purl.org/wot-catalogue/ble/gatt#org.bluetooth.characteristic.date_of_birth>
  a skos:Concept, ontolex:LexicalConcept, prov:Entity;
  skos:altLabel "date of birth";
  skos:broader ble:Characteristic;
  skos:inScheme ble:Scheme;
  skos:prefLabel "Date of Birth";
  skos:related ble:Day, ble:Month, ble:Read, ble:Write, ble:Year;
  prov:wasDerivedFrom <file:/data/lp/etl/executor/data/1651932367716-22-f5b1c2e0-1947-4a2e-a814-6ce401f2a604/working/working-outputfiles-33/gatt-xml-master/org.bluetooth.characteristic.date_of_birth.xml> .

<http://purl.org/wot-catalogue/ble/gatt#org.bluetooth.characteristic.gender> a skos:Concept,
    ontolex:LexicalConcept, prov:Entity;
  skos:altLabel "gender";
  skos:broader ble:Characteristic;
  skos:definition """Gender of the user. The value of the Gender
    characteristic are defined below: 0:male,1:female,
    2:Unspecified,3-225: RFU""";
  skos:inScheme ble:Scheme;
  skos:prefLabel "Gender";
  skos:related ble:Gender, ble:Read, ble:Write;
  prov:wasDerivedFrom <file:/data/lp/etl/executor/data/1651932367716-22-f5b1c2e0-1947-4a2e-a814-6ce401f2a604/working/working-outputfiles-33/gatt-xml-master/org.bluetooth.characteristic.gender.xml> .

<http://purl.org/wot-catalogue/ble/gatt#org.bluetooth.characteristic.weight> a skos:Concept,
    ontolex:LexicalConcept, prov:Entity;
  skos:altLabel "weight";
  skos:broader ble:Characteristic;
  skos:definition "Weight of the User";
  skos:inScheme ble:Scheme;
  skos:prefLabel "Weight";
  skos:related ble:Read, ble:Weight, ble:Write;
  prov:wasDerivedFrom <file:/data/lp/etl/executor/data/1651932367716-22-f5b1c2e0-1947-4a2e-a814-6ce401f2a604/working/working-outputfiles-33/gatt-xml-master/org.bluetooth.characteristic.weight.xml> .

<http://purl.org/wot-catalogue/ble/gatt#org.bluetooth.characteristic.height> a skos:Concept,
    ontolex:LexicalConcept, prov:Entity;
  skos:altLabel "height";
  skos:broader ble:Characteristic;
  skos:definition "Height of the User";
  skos:inScheme ble:Scheme;
  skos:prefLabel "Height";
  skos:related ble:Height, ble:Read, ble:Write;
  prov:wasDerivedFrom <file:/data/lp/etl/executor/data/1651932367716-22-f5b1c2e0-1947-4a2e-a814-6ce401f2a604/working/working-outputfiles-33/gatt-xml-master/org.bluetooth.characteristic.height.xml> .

<http://purl.org/wot-catalogue/ble/gatt#org.bluetooth.characteristic.heart_rate_max>
  a skos:Concept, ontolex:LexicalConcept, prov:Entity;
  skos:altLabel "heart rate max";
  skos:broader ble:Characteristic;
  skos:definition "Maximum heart rate a user can reach.";
  skos:inScheme ble:Scheme;
  skos:prefLabel "Heart Rate Max";
  skos:related ble:HeartRateMax, ble:Read, ble:Write;
  prov:wasDerivedFrom <file:/data/lp/etl/executor/data/1651932367716-22-f5b1c2e0-1947-4a2e-a814-6ce401f2a604/working/working-outputfiles-33/gatt-xml-master/org.bluetooth.characteristic.heart_rate_max.xml> .

<http://purl.org/wot-catalogue/ble/gatt#org.bluetooth.characteristic.maximum_recommended_heart_rate>
  a skos:Concept, ontolex:LexicalConcept, prov:Entity;
  skos:altLabel "maximum recommended heart rate";
  skos:broader ble:Characteristic;
  skos:definition """Maximum recommended heart rate is a threshold that
    may be set to limit exertion. The maximum recommended heart
    rate is smaller or equal to the maximal heart rate a user can
    reach.""";
  skos:inScheme ble:Scheme;
  skos:prefLabel "Maximum Recommended Heart Rate";
  skos:related ble:MaximumRecommendedHeartRate, ble:Read, ble:Write;
  prov:wasDerivedFrom <file:/data/lp/etl/executor/data/1651932367716-22-f5b1c2e0-1947-4a2e-a814-6ce401f2a604/working/working-outputfiles-33/gatt-xml-master/org.bluetooth.characteristic.maximum_recommended_heart_rate.xml> .

<http://purl.org/wot-catalogue/ble/gatt#org.bluetooth.characteristic.anaerobic_threshold>
  a skos:Concept, ontolex:LexicalConcept, prov:Entity;
  skos:altLabel "anaerobic threshold";
  skos:broader ble:Characteristic;
  skos:definition "Second metabolic threshold";
  skos:inScheme ble:Scheme;
  skos:prefLabel "Anaerobic Threshold";
  skos:related ble:AnaerobicThreshold, ble:Read, ble:Write;
  prov:wasDerivedFrom <file:/data/lp/etl/executor/data/1651932367716-22-f5b1c2e0-1947-4a2e-a814-6ce401f2a604/working/working-outputfiles-33/gatt-xml-master/org.bluetooth.characteristic.anaerobic_threshold.xml> .

<http://purl.org/wot-catalogue/ble/gatt#org.bluetooth.characteristic.date_of_threshold_assessment>
  a skos:Concept, ontolex:LexicalConcept, prov:Entity;
  skos:altLabel "date of threshold assessment";
  skos:broader ble:Characteristic;
  skos:inScheme ble:Scheme;
  skos:prefLabel "Date of Threshold Assessment";
  skos:related ble:Day, ble:Month, ble:Read, ble:Write, ble:Year;
  prov:wasDerivedFrom <file:/data/lp/etl/executor/data/1651932367716-22-f5b1c2e0-1947-4a2e-a814-6ce401f2a604/working/working-outputfiles-33/gatt-xml-master/org.bluetooth.characteristic.date_of_threshold_assessment.xml> .

<http://purl.org/wot-catalogue/ble/gatt#org.bluetooth.characteristic.fat_burn_heart_rate_upper_limit>
  a skos:Concept, ontolex:LexicalConcept, prov:Entity;
  skos:altLabel "fat burn heart rate upper limit";
  skos:broader ble:Characteristic;
  skos:definition """Upper limit of the heart rate where the user
    maximizes the fat burn while exersizing""";
  skos:inScheme ble:Scheme;
  skos:prefLabel "Fat Burn Heart Rate Upper Limit";
  skos:related ble:FatBurnHeartRateUpperLimit, ble:Read, ble:Write;
  prov:wasDerivedFrom <file:/data/lp/etl/executor/data/1651932367716-22-f5b1c2e0-1947-4a2e-a814-6ce401f2a604/working/working-outputfiles-33/gatt-xml-master/org.bluetooth.characteristic.fat_burn_heart_rate_upper_limit.xml> .

<http://purl.org/wot-catalogue/ble/gatt#org.bluetooth.characteristic.aerobic_heart_rate_upper_limit>
  a skos:Concept, ontolex:LexicalConcept, prov:Entity;
  skos:altLabel "aerobic heart rate upper limit";
  skos:broader ble:Characteristic;
  skos:definition """Upper limit of the heart rate where the user enhances
    his endurance while exercising""";
  skos:inScheme ble:Scheme;
  skos:prefLabel "Aerobic Heart Rate Upper Limit";
  skos:related ble:AerobicHeartRateUpperLimit, ble:Read, ble:Write;
  prov:wasDerivedFrom <file:/data/lp/etl/executor/data/1651932367716-22-f5b1c2e0-1947-4a2e-a814-6ce401f2a604/working/working-outputfiles-33/gatt-xml-master/org.bluetooth.characteristic.aerobic_heart_rate_upper_limit.xml> .

<http://purl.org/wot-catalogue/ble/gatt#org.bluetooth.characteristic.anaerobic_heart_rate_lower_limit>
  a skos:Concept, ontolex:LexicalConcept, prov:Entity;
  skos:altLabel "anaerobic heart rate lower limit";
  skos:broader ble:Characteristic;
  skos:definition """Lower limit of the heart rate where the user enhances
    his anaerobic tolerance while exercising.""";
  skos:inScheme ble:Scheme;
  skos:prefLabel "Anaerobic Heart Rate Lower Limit";
  skos:related ble:AnaerobicHeartRateLowerLimit, ble:Read, ble:Write;
  prov:wasDerivedFrom <file:/data/lp/etl/executor/data/1651932367716-22-f5b1c2e0-1947-4a2e-a814-6ce401f2a604/working/working-outputfiles-33/gatt-xml-master/org.bluetooth.characteristic.anaerobic_heart_rate_lower_limit.xml> .

<http://purl.org/wot-catalogue/ble/gatt#org.bluetooth.characteristic.three_zone_heart_rate_limits>
  a skos:Concept, ontolex:LexicalConcept, prov:Entity;
  skos:altLabel "three zone heart rate limits";
  skos:broader ble:Characteristic;
  skos:definition """Data structure containing the limits between the
    heart rate zones for the 3-zone heart rate definition (Hard,
    Moderate and Light).""";
  skos:inScheme ble:Scheme;
  skos:prefLabel "Three Zone Heart Rate Limits";
  skos:related ble:Read, <http://purl.org/wot-catalogue/ble#ThreezoneHeartRateLimits-Light(Fatburn)/Moderate(Aerobic)Limit>,
    <http://purl.org/wot-catalogue/ble#ThreezoneHeartRateLimits-Moderate(Aerobic)/Hard(Anaerobic)Limit>,
    ble:Write;
  prov:wasDerivedFrom <file:/data/lp/etl/executor/data/1651932367716-22-f5b1c2e0-1947-4a2e-a814-6ce401f2a604/working/working-outputfiles-33/gatt-xml-master/org.bluetooth.characteristic.three_zone_heart_rate_limits.xml> .

<http://purl.org/wot-catalogue/ble/gatt#org.bluetooth.characteristic.user_index> a
    skos:Concept, ontolex:LexicalConcept, prov:Entity;
  skos:altLabel "user index";
  skos:broader ble:Characteristic;
  skos:inScheme ble:Scheme;
  skos:prefLabel "User Index";
  skos:related ble:Read, ble:UserIndex;
  prov:wasDerivedFrom <file:/data/lp/etl/executor/data/1651932367716-22-f5b1c2e0-1947-4a2e-a814-6ce401f2a604/working/working-outputfiles-33/gatt-xml-master/org.bluetooth.characteristic.user_index.xml> .

<http://purl.org/wot-catalogue/ble/gatt#org.bluetooth.characteristic.user_control_point>
  a skos:Concept, ontolex:LexicalConcept, prov:Entity;
  skos:altLabel "user control point";
  skos:broader ble:Characteristic;
  skos:inScheme ble:Scheme;
  skos:prefLabel "User Control Point";
  skos:related ble:Indicate, ble:Write;
  prov:wasDerivedFrom <file:/data/lp/etl/executor/data/1651932367716-22-f5b1c2e0-1947-4a2e-a814-6ce401f2a604/working/working-outputfiles-33/gatt-xml-master/org.bluetooth.characteristic.user_control_point.xml> .

<http://purl.org/wot-catalogue/ble/gatt#LocalNorthCoordinate> a skos:Concept, ontolex:LexicalConcept,
    prov:Entity;
  skos:altLabel "local north coordinate";
  skos:broader ble:Value;
  skos:inScheme ble:Scheme;
  skos:prefLabel "Local North Coordinate";
  prov:wasDerivedFrom <file:/data/lp/etl/executor/data/1651932367716-22-f5b1c2e0-1947-4a2e-a814-6ce401f2a604/working/working-outputfiles-33/gatt-xml-master/org.bluetooth.characteristic.local_north_coordinate.xml> .

<http://purl.org/wot-catalogue/ble/gatt#180A> a skos:Concept, ontolex:LexicalConcept,
    prov:Entity;
  skos:altLabel "device information";
  skos:broader ble:Service;
  skos:definition """This service exposes manufacturer information about a
    device. The Device Information Service is instantiated as a
    Primary Service. Only one instance of the Device Information
    Service is exposed on a device.""";
  skos:inScheme ble:Scheme;
  skos:prefLabel "Device Information";
  skos:related ble:org.bluetooth.characteristic.firmware_revision_string, ble:org.bluetooth.characteristic.hardware_revision_string,
    ble:org.bluetooth.characteristic.ieee_11073-20601_regulatory_certification_data_list,
    ble:org.bluetooth.characteristic.manufacturer_name_string, ble:org.bluetooth.characteristic.model_number_string,
    ble:org.bluetooth.characteristic.pnp_id, ble:org.bluetooth.characteristic.serial_number_string,
    ble:org.bluetooth.characteristic.software_revision_string, ble:org.bluetooth.characteristic.system_id;
  prov:wasDerivedFrom <file:/data/lp/etl/executor/data/1651932367716-22-f5b1c2e0-1947-4a2e-a814-6ce401f2a604/working/working-outputfiles-33/gatt-xml-master/org.bluetooth.service.device_information.xml> .

<http://purl.org/wot-catalogue/ble/gatt#org.bluetooth.characteristic.serial_number_string>
  a skos:Concept, ontolex:LexicalConcept, prov:Entity;
  skos:altLabel "serial number string";
  skos:broader ble:Characteristic;
  skos:definition """The value of this characteristic is a variable-length
    UTF-8 string representing the serial number for a particular
    instance of the device.""";
  skos:inScheme ble:Scheme;
  skos:prefLabel "Serial Number String";
  skos:related ble:Read, ble:SerialNumber;
  prov:wasDerivedFrom <file:/data/lp/etl/executor/data/1651932367716-22-f5b1c2e0-1947-4a2e-a814-6ce401f2a604/working/working-outputfiles-33/gatt-xml-master/org.bluetooth.characteristic.serial_number_string.xml> .

<http://purl.org/wot-catalogue/ble/gatt#org.bluetooth.characteristic.hardware_revision_string>
  a skos:Concept, ontolex:LexicalConcept, prov:Entity;
  skos:altLabel "hardware revision string";
  skos:broader ble:Characteristic;
  skos:definition """The value of this characteristic is a UTF-8 string
    representing the hardware revision for the hardware within the
    device.""";
  skos:inScheme ble:Scheme;
  skos:prefLabel "Hardware Revision String";
  skos:related ble:HardwareRevision, ble:Read;
  prov:wasDerivedFrom <file:/data/lp/etl/executor/data/1651932367716-22-f5b1c2e0-1947-4a2e-a814-6ce401f2a604/working/working-outputfiles-33/gatt-xml-master/org.bluetooth.characteristic.hardware_revision_string.xml> .

<http://purl.org/wot-catalogue/ble/gatt#org.bluetooth.characteristic.pnp_id> a skos:Concept,
    ontolex:LexicalConcept, prov:Entity;
  skos:altLabel "pnp id";
  skos:broader ble:Characteristic;
  skos:definition """The PnP_ID characteristic is a set of values that used
    to create a device ID value that is unique for this device.
    Included in the characteristic is a Vendor ID Source field, a
    Vendor ID field, a Product ID field and a Product Version
    field. These values are used to identify all devices of a given
    type/model/version using numbers.""";
  skos:inScheme ble:Scheme;
  skos:prefLabel "PnP ID";
  skos:related ble:ProductID, ble:ProductVersion, ble:Read, ble:VendorID, ble:VendorIDSource;
  prov:wasDerivedFrom <file:/data/lp/etl/executor/data/1651932367716-22-f5b1c2e0-1947-4a2e-a814-6ce401f2a604/working/working-outputfiles-33/gatt-xml-master/org.bluetooth.characteristic.pnp_id.xml> .

<http://purl.org/wot-catalogue/ble/gatt#org.bluetooth.characteristic.Magnetic_flux_density_2D>
  a skos:Concept, ontolex:LexicalConcept, prov:Entity;
  skos:altLabel "magnetic flux density - 2d";
  skos:broader ble:Characteristic;
  skos:inScheme ble:Scheme;
  skos:prefLabel "Magnetic Flux Density - 2D";
  skos:related ble:MagneticFluxDensity:X-Axis, ble:MagneticFluxDensity:Y-Axis;
  prov:wasDerivedFrom <file:/data/lp/etl/executor/data/1651932367716-22-f5b1c2e0-1947-4a2e-a814-6ce401f2a604/working/working-outputfiles-33/gatt-xml-master/org.bluetooth.characteristic.Magnetic_flux_density_2D.xml> .

<http://purl.org/wot-catalogue/ble/gatt#MagneticFluxDensity:X-Axis> a skos:Concept,
    ontolex:LexicalConcept, prov:Entity;
  skos:altLabel "magnetic flux density: x-axis";
  skos:broader ble:Value;
  skos:inScheme ble:Scheme;
  skos:prefLabel "Magnetic Flux Density: X-Axis";
  prov:wasDerivedFrom <file:/data/lp/etl/executor/data/1651932367716-22-f5b1c2e0-1947-4a2e-a814-6ce401f2a604/working/working-outputfiles-33/gatt-xml-master/org.bluetooth.characteristic.Magnetic_flux_density_2D.xml>,
    <file:/data/lp/etl/executor/data/1651932367716-22-f5b1c2e0-1947-4a2e-a814-6ce401f2a604/working/working-outputfiles-33/gatt-xml-master/org.bluetooth.characteristic.Magnetic_flux_density_3D.xml> .

<http://purl.org/wot-catalogue/ble/gatt#MagneticFluxDensity:Y-Axis> a skos:Concept,
    ontolex:LexicalConcept, prov:Entity;
  skos:altLabel "magnetic flux density: y-axis";
  skos:broader ble:Value;
  skos:inScheme ble:Scheme;
  skos:prefLabel "Magnetic Flux Density: Y-Axis";
  prov:wasDerivedFrom <file:/data/lp/etl/executor/data/1651932367716-22-f5b1c2e0-1947-4a2e-a814-6ce401f2a604/working/working-outputfiles-33/gatt-xml-master/org.bluetooth.characteristic.Magnetic_flux_density_2D.xml>,
    <file:/data/lp/etl/executor/data/1651932367716-22-f5b1c2e0-1947-4a2e-a814-6ce401f2a604/working/working-outputfiles-33/gatt-xml-master/org.bluetooth.characteristic.Magnetic_flux_density_3D.xml> .

<http://purl.org/wot-catalogue/ble/gatt#org.bluetooth.characteristic.gust_factor>
  a skos:Concept, ontolex:LexicalConcept, prov:Entity;
  skos:altLabel "gust factor";
  skos:broader ble:Characteristic;
  skos:inScheme ble:Scheme;
  skos:prefLabel "Gust Factor";
  skos:related ble:ExtendedProperties, ble:GustFactor, ble:Notify, ble:Read, ble:WritableAuxiliaries;
  prov:wasDerivedFrom <file:/data/lp/etl/executor/data/1651932367716-22-f5b1c2e0-1947-4a2e-a814-6ce401f2a604/working/working-outputfiles-33/gatt-xml-master/org.bluetooth.characteristic.gust_factor.xml> .

<http://purl.org/wot-catalogue/ble/gatt#GustFactor> a skos:Concept, ontolex:LexicalConcept,
    prov:Entity;
  skos:altLabel "gust factor";
  skos:broader ble:Value;
  skos:definition """The factor has a fixed-point representation,
      where the actual factor is (attribute value *
      0.1)""";
  skos:inScheme ble:Scheme;
  skos:prefLabel "Gust Factor";
  prov:wasDerivedFrom <file:/data/lp/etl/executor/data/1651932367716-22-f5b1c2e0-1947-4a2e-a814-6ce401f2a604/working/working-outputfiles-33/gatt-xml-master/org.bluetooth.characteristic.gust_factor.xml> .

<http://purl.org/wot-catalogue/ble/gatt#org.bluetooth.characteristic.temperature>
  a skos:Concept, ontolex:LexicalConcept, prov:Entity;
  skos:altLabel "temperature";
  skos:broader ble:Characteristic;
  skos:inScheme ble:Scheme;
  skos:prefLabel "Temperature";
  skos:related ble:ExtendedProperties, ble:Notify, ble:Read, ble:Temperature, ble:WritableAuxiliaries;
  prov:wasDerivedFrom <file:/data/lp/etl/executor/data/1651932367716-22-f5b1c2e0-1947-4a2e-a814-6ce401f2a604/working/working-outputfiles-33/gatt-xml-master/org.bluetooth.characteristic.temperature.xml> .

<http://purl.org/wot-catalogue/ble/gatt#Temperature> a skos:Concept, ontolex:LexicalConcept,
    prov:Entity;
  skos:altLabel "temperature";
  skos:broader ble:Value;
  skos:definition """Unit is in degrees Celsius with a resolution
      of 0.01 degrees Celsius""";
  skos:inScheme ble:Scheme;
  skos:prefLabel "Temperature";
  prov:wasDerivedFrom <file:/data/lp/etl/executor/data/1651932367716-22-f5b1c2e0-1947-4a2e-a814-6ce401f2a604/working/working-outputfiles-33/gatt-xml-master/org.bluetooth.characteristic.temperature.xml> .

<http://purl.org/wot-catalogue/ble/gatt#org.bluetooth.characteristic.heat_index> a
    skos:Concept, ontolex:LexicalConcept, prov:Entity;
  skos:altLabel "heat index";
  skos:broader ble:Characteristic;
  skos:inScheme ble:Scheme;
  skos:prefLabel "Heat Index";
  skos:related ble:ExtendedProperties, ble:HeatIndex, ble:Notify, ble:Read, ble:WritableAuxiliaries;
  prov:wasDerivedFrom <file:/data/lp/etl/executor/data/1651932367716-22-f5b1c2e0-1947-4a2e-a814-6ce401f2a604/working/working-outputfiles-33/gatt-xml-master/org.bluetooth.characteristic.heat_index.xml> .

<http://purl.org/wot-catalogue/ble/gatt#HeatIndex> a skos:Concept, ontolex:LexicalConcept,
    prov:Entity;
  skos:altLabel "heat index";
  skos:broader ble:Value;
  skos:definition """Unit is in degrees celsius with a resolution
      of 1 degree Celsius""";
  skos:inScheme ble:Scheme;
  skos:prefLabel "Heat Index";
  prov:wasDerivedFrom <file:/data/lp/etl/executor/data/1651932367716-22-f5b1c2e0-1947-4a2e-a814-6ce401f2a604/working/working-outputfiles-33/gatt-xml-master/org.bluetooth.characteristic.heat_index.xml> .

<http://purl.org/wot-catalogue/ble/gatt#ExactTime256> a skos:Concept, ontolex:LexicalConcept,
    prov:Entity;
  skos:altLabel "exact time 256";
  skos:broader ble:Value;
  skos:inScheme ble:Scheme;
  skos:prefLabel "Exact Time 256";
  prov:wasDerivedFrom <file:/data/lp/etl/executor/data/1651932367716-22-f5b1c2e0-1947-4a2e-a814-6ce401f2a604/working/working-outputfiles-33/gatt-xml-master/org.bluetooth.characteristic.current_time.xml> .

<http://purl.org/wot-catalogue/ble/gatt#AdjustReason> a skos:Concept, ontolex:LexicalConcept,
    prov:Entity;
  skos:altLabel "adjust reason";
  skos:broader ble:Value;
  skos:inScheme ble:Scheme;
  skos:prefLabel "Adjust Reason";
  prov:wasDerivedFrom <file:/data/lp/etl/executor/data/1651932367716-22-f5b1c2e0-1947-4a2e-a814-6ce401f2a604/working/working-outputfiles-33/gatt-xml-master/org.bluetooth.characteristic.current_time.xml> .

<http://purl.org/wot-catalogue/ble/gatt#Floors> a skos:Concept, ontolex:LexicalConcept,
    prov:Entity;
  skos:altLabel "floors";
  skos:broader ble:Value;
  skos:definition """Unitless with a resolution of
      1""";
  skos:inScheme ble:Scheme;
  skos:prefLabel "Floors";
  prov:wasDerivedFrom <file:/data/lp/etl/executor/data/1651932367716-22-f5b1c2e0-1947-4a2e-a814-6ce401f2a604/working/working-outputfiles-33/gatt-xml-master/org.bluetooth.characteristic.stair_climber_data.xml>,
    <file:/data/lp/etl/executor/data/1651932367716-22-f5b1c2e0-1947-4a2e-a814-6ce401f2a604/working/working-outputfiles-33/gatt-xml-master/org.bluetooth.characteristic.step_climber_data.xml> .

<http://purl.org/wot-catalogue/ble/gatt#ObjectID> a skos:Concept, ontolex:LexicalConcept,
    prov:Entity;
  skos:altLabel "object id";
  skos:broader ble:Value;
  skos:inScheme ble:Scheme;
  skos:prefLabel "Object ID";
  prov:wasDerivedFrom <file:/data/lp/etl/executor/data/1651932367716-22-f5b1c2e0-1947-4a2e-a814-6ce401f2a604/working/working-outputfiles-33/gatt-xml-master/org.bluetooth.characteristic.object_id.xml> .

<http://purl.org/wot-catalogue/ble/gatt#BodyCompositionFeature> a skos:Concept, ontolex:LexicalConcept,
    prov:Entity;
  skos:altLabel "body composition feature";
  skos:broader ble:Value;
  skos:inScheme ble:Scheme;
  skos:prefLabel "Body Composition Feature";
  prov:wasDerivedFrom <file:/data/lp/etl/executor/data/1651932367716-22-f5b1c2e0-1947-4a2e-a814-6ce401f2a604/working/working-outputfiles-33/gatt-xml-master/org.bluetooth.characteristic.body_composition_feature.xml> .

<http://purl.org/wot-catalogue/ble/gatt#org.bluetooth.characteristic.day_date_time>
  a skos:Concept, ontolex:LexicalConcept, prov:Entity;
  skos:altLabel "day date time";
  skos:broader ble:Characteristic;
  skos:inScheme ble:Scheme;
  skos:prefLabel "Day Date Time";
  skos:related ble:DateTime, ble:DayofWeek;
  prov:wasDerivedFrom <file:/data/lp/etl/executor/data/1651932367716-22-f5b1c2e0-1947-4a2e-a814-6ce401f2a604/working/working-outputfiles-33/gatt-xml-master/org.bluetooth.characteristic.day_date_time.xml> .

<http://purl.org/wot-catalogue/ble/gatt#DateTime> a skos:Concept, ontolex:LexicalConcept,
    prov:Entity;
  skos:altLabel "date time";
  skos:broader ble:Value;
  skos:inScheme ble:Scheme;
  skos:prefLabel "Date Time";
  prov:wasDerivedFrom <file:/data/lp/etl/executor/data/1651932367716-22-f5b1c2e0-1947-4a2e-a814-6ce401f2a604/working/working-outputfiles-33/gatt-xml-master/org.bluetooth.characteristic.day_date_time.xml>,
    <file:/data/lp/etl/executor/data/1651932367716-22-f5b1c2e0-1947-4a2e-a814-6ce401f2a604/working/working-outputfiles-33/gatt-xml-master/org.bluetooth.characteristic.time_with_dst.xml> .

<http://purl.org/wot-catalogue/ble/gatt#DayofWeek> a skos:Concept, ontolex:LexicalConcept,
    prov:Entity;
  skos:altLabel "day of week";
  skos:broader ble:Value;
  skos:inScheme ble:Scheme;
  skos:prefLabel "Day of Week";
  prov:wasDerivedFrom <file:/data/lp/etl/executor/data/1651932367716-22-f5b1c2e0-1947-4a2e-a814-6ce401f2a604/working/working-outputfiles-33/gatt-xml-master/org.bluetooth.characteristic.day_date_time.xml>,
    <file:/data/lp/etl/executor/data/1651932367716-22-f5b1c2e0-1947-4a2e-a814-6ce401f2a604/working/working-outputfiles-33/gatt-xml-master/org.bluetooth.characteristic.day_of_week.xml> .

<http://purl.org/wot-catalogue/ble/gatt#org.bluetooth.characteristic.date_time> a
    skos:Concept, ontolex:LexicalConcept, prov:Entity;
  skos:altLabel "date time";
  skos:broader ble:Characteristic;
  skos:definition """The Date Time characteristic contains fields for year,
    month, day, hours, minutes and seconds. Calendar days in Date
    Time are represented using Gregorian calendar. Hours in Date
    Time are represented in the 24h system.""";
  skos:inScheme ble:Scheme;
  skos:prefLabel "Date Time";
  skos:related ble:Day, ble:Hours, ble:Minutes, ble:Month, ble:Seconds, ble:Year;
  prov:wasDerivedFrom <file:/data/lp/etl/executor/data/1651932367716-22-f5b1c2e0-1947-4a2e-a814-6ce401f2a604/working/working-outputfiles-33/gatt-xml-master/org.bluetooth.characteristic.date_time.xml> .

<http://purl.org/wot-catalogue/ble/gatt#Year> a skos:Concept, ontolex:LexicalConcept,
    prov:Entity;
  skos:altLabel "year";
  skos:broader ble:Value;
  skos:definition """Year as defined by the Gregorian
      calendar.""";
  skos:inScheme ble:Scheme;
  skos:prefLabel "Year";
  prov:wasDerivedFrom <file:/data/lp/etl/executor/data/1651932367716-22-f5b1c2e0-1947-4a2e-a814-6ce401f2a604/working/working-outputfiles-33/gatt-xml-master/org.bluetooth.characteristic.date_of_birth.xml>,
    <file:/data/lp/etl/executor/data/1651932367716-22-f5b1c2e0-1947-4a2e-a814-6ce401f2a604/working/working-outputfiles-33/gatt-xml-master/org.bluetooth.characteristic.date_of_threshold_assessment.xml>,
    <file:/data/lp/etl/executor/data/1651932367716-22-f5b1c2e0-1947-4a2e-a814-6ce401f2a604/working/working-outputfiles-33/gatt-xml-master/org.bluetooth.characteristic.date_time.xml> .

<http://purl.org/wot-catalogue/ble/gatt#Month> a skos:Concept, ontolex:LexicalConcept,
    prov:Entity;
  skos:altLabel "month";
  skos:broader ble:Value;
  skos:definition """Month of the year as defined by the
      Gregorian calendar.""";
  skos:inScheme ble:Scheme;
  skos:prefLabel "Month";
  prov:wasDerivedFrom <file:/data/lp/etl/executor/data/1651932367716-22-f5b1c2e0-1947-4a2e-a814-6ce401f2a604/working/working-outputfiles-33/gatt-xml-master/org.bluetooth.characteristic.date_of_birth.xml>,
    <file:/data/lp/etl/executor/data/1651932367716-22-f5b1c2e0-1947-4a2e-a814-6ce401f2a604/working/working-outputfiles-33/gatt-xml-master/org.bluetooth.characteristic.date_of_threshold_assessment.xml>,
    <file:/data/lp/etl/executor/data/1651932367716-22-f5b1c2e0-1947-4a2e-a814-6ce401f2a604/working/working-outputfiles-33/gatt-xml-master/org.bluetooth.characteristic.date_time.xml> .

<http://purl.org/wot-catalogue/ble/gatt#Day> a skos:Concept, ontolex:LexicalConcept,
    prov:Entity;
  skos:altLabel "day";
  skos:broader ble:Value;
  skos:definition """Day of the month as defined by the Gregorian
      calendar.""";
  skos:inScheme ble:Scheme;
  skos:prefLabel "Day";
  prov:wasDerivedFrom <file:/data/lp/etl/executor/data/1651932367716-22-f5b1c2e0-1947-4a2e-a814-6ce401f2a604/working/working-outputfiles-33/gatt-xml-master/org.bluetooth.characteristic.date_of_birth.xml>,
    <file:/data/lp/etl/executor/data/1651932367716-22-f5b1c2e0-1947-4a2e-a814-6ce401f2a604/working/working-outputfiles-33/gatt-xml-master/org.bluetooth.characteristic.date_of_threshold_assessment.xml>,
    <file:/data/lp/etl/executor/data/1651932367716-22-f5b1c2e0-1947-4a2e-a814-6ce401f2a604/working/working-outputfiles-33/gatt-xml-master/org.bluetooth.characteristic.date_time.xml> .

<http://purl.org/wot-catalogue/ble/gatt#Hours> a skos:Concept, ontolex:LexicalConcept,
    prov:Entity;
  skos:altLabel "hours";
  skos:broader ble:Value;
  skos:definition """Number of hours past
      midnight.""";
  skos:inScheme ble:Scheme;
  skos:prefLabel "Hours";
  prov:wasDerivedFrom <file:/data/lp/etl/executor/data/1651932367716-22-f5b1c2e0-1947-4a2e-a814-6ce401f2a604/working/working-outputfiles-33/gatt-xml-master/org.bluetooth.characteristic.date_time.xml> .

<http://purl.org/wot-catalogue/ble/gatt#Minutes> a skos:Concept, ontolex:LexicalConcept,
    prov:Entity;
  skos:altLabel "minutes";
  skos:broader ble:Value;
  skos:definition """Number of minutes since the start of the
      hour.""";
  skos:inScheme ble:Scheme;
  skos:prefLabel "Minutes";
  prov:wasDerivedFrom <file:/data/lp/etl/executor/data/1651932367716-22-f5b1c2e0-1947-4a2e-a814-6ce401f2a604/working/working-outputfiles-33/gatt-xml-master/org.bluetooth.characteristic.date_time.xml> .

<http://purl.org/wot-catalogue/ble/gatt#Seconds> a skos:Concept, ontolex:LexicalConcept,
    prov:Entity;
  skos:altLabel "seconds";
  skos:broader ble:Value;
  skos:definition """Number of seconds since the start of the
      minute.""";
  skos:inScheme ble:Scheme;
  skos:prefLabel "Seconds";
  prov:wasDerivedFrom <file:/data/lp/etl/executor/data/1651932367716-22-f5b1c2e0-1947-4a2e-a814-6ce401f2a604/working/working-outputfiles-33/gatt-xml-master/org.bluetooth.characteristic.date_time.xml> .

<http://purl.org/wot-catalogue/ble/gatt#org.bluetooth.characteristic.new_alert> a
    skos:Concept, ontolex:LexicalConcept, prov:Entity;
  skos:altLabel "new alert";
  skos:broader ble:Characteristic;
  skos:definition """This characteristic consists of ?Category ID?,
    ?uint8?, and ?UTF-8 string? fields. The size of this
    characteristic is dynamic because of the variable length text
    (?UTF-8?) field. The minimum length of ?UTF-8 string? is 0
    octets and maximum length of ?UTF-8 string? is 18
    octets.""";
  skos:inScheme ble:Scheme;
  skos:prefLabel "New Alert";
  skos:related ble:CategoryID, ble:Notify, ble:NumberofNewAlert, ble:TextStringInformation;
  prov:wasDerivedFrom <file:/data/lp/etl/executor/data/1651932367716-22-f5b1c2e0-1947-4a2e-a814-6ce401f2a604/working/working-outputfiles-33/gatt-xml-master/org.bluetooth.characteristic.new_alert.xml> .

<http://purl.org/wot-catalogue/ble/gatt#NumberofNewAlert> a skos:Concept, ontolex:LexicalConcept,
    prov:Entity;
  skos:altLabel "number of new alert";
  skos:broader ble:Value;
  skos:definition """This field provides the number of new alerts
      in the server.""";
  skos:inScheme ble:Scheme;
  skos:prefLabel "Number of New Alert";
  prov:wasDerivedFrom <file:/data/lp/etl/executor/data/1651932367716-22-f5b1c2e0-1947-4a2e-a814-6ce401f2a604/working/working-outputfiles-33/gatt-xml-master/org.bluetooth.characteristic.new_alert.xml> .

<http://purl.org/wot-catalogue/ble/gatt#TextStringInformation> a skos:Concept, ontolex:LexicalConcept,
    prov:Entity;
  skos:altLabel "text string information";
  skos:broader ble:Value;
  skos:definition """The field provides brief text information
      for the last alert.""";
  skos:inScheme ble:Scheme;
  skos:prefLabel "Text String Information";
  prov:wasDerivedFrom <file:/data/lp/etl/executor/data/1651932367716-22-f5b1c2e0-1947-4a2e-a814-6ce401f2a604/working/working-outputfiles-33/gatt-xml-master/org.bluetooth.characteristic.new_alert.xml> .

<http://purl.org/wot-catalogue/ble/gatt#1819> a skos:Concept, ontolex:LexicalConcept,
    prov:Entity;
  skos:altLabel "location and navigation";
  skos:broader ble:Service;
  skos:definition """The Location and Navigation Service (LN Service)
    exposes location and navigation-related data from a Location
    and Navigation sensor (Server) intended for outdoor activity
    applications.""";
  skos:inScheme ble:Scheme;
  skos:prefLabel "Location and Navigation";
  skos:related ble:org.bluetooth.characteristic.ln_control_point, ble:org.bluetooth.characteristic.ln_feature,
    ble:org.bluetooth.characteristic.location_and_speed, ble:org.bluetooth.characteristic.navigation,
    ble:org.bluetooth.characteristic.position_quality;
  prov:wasDerivedFrom <file:/data/lp/etl/executor/data/1651932367716-22-f5b1c2e0-1947-4a2e-a814-6ce401f2a604/working/working-outputfiles-33/gatt-xml-master/org.bluetooth.service.location_and_navigation.xml> .

<http://purl.org/wot-catalogue/ble/gatt#org.bluetooth.characteristic.location_and_speed>
  a skos:Concept, ontolex:LexicalConcept, prov:Entity;
  skos:altLabel "location and speed characteristic";
  skos:broader ble:Characteristic;
  skos:definition """The Location and Speed characteristic is a variable
    length structure containing a Flags field and, based on the
    contents of the Flags field, may contain a combination of data
    fields listed below. Note that it is possible for this
    characteristic to exceed the default LE MTU size.""";
  skos:inScheme ble:Scheme;
  skos:prefLabel "Location and Speed Characteristic";
  skos:related ble:Elevation, ble:Flags, ble:Heading, ble:InstantaneousSpeed, ble:Location-Latitude,
    ble:Location-Longitude, ble:Notify, ble:RollingTime, ble:TotalDistance, ble:UTCTime;
  prov:wasDerivedFrom <file:/data/lp/etl/executor/data/1651932367716-22-f5b1c2e0-1947-4a2e-a814-6ce401f2a604/working/working-outputfiles-33/gatt-xml-master/org.bluetooth.characteristic.location_and_speed.xml> .

<http://purl.org/wot-catalogue/ble/gatt#org.bluetooth.characteristic.position_quality>
  a skos:Concept, ontolex:LexicalConcept, prov:Entity;
  skos:altLabel "position quality";
  skos:broader ble:Characteristic;
  skos:definition """The Position Quality characteristic is a variable
    length structure containing a Flags field and at least one of
    the optional data fields listed below""";
  skos:inScheme ble:Scheme;
  skos:prefLabel "Position Quality";
  skos:related ble:EHPE, ble:EVPE, ble:Flags, ble:HDOP, ble:NumberofBeaconsinSolution,
    ble:NumberofBeaconsinView, ble:Read, ble:TimetoFirstFix, ble:VDOP;
  prov:wasDerivedFrom <file:/data/lp/etl/executor/data/1651932367716-22-f5b1c2e0-1947-4a2e-a814-6ce401f2a604/working/working-outputfiles-33/gatt-xml-master/org.bluetooth.characteristic.position_quality.xml> .

<http://purl.org/wot-catalogue/ble/gatt#DaylightSavingTime> a skos:Concept, ontolex:LexicalConcept,
    prov:Entity;
  skos:altLabel "daylight saving time";
  skos:broader ble:Value;
  skos:inScheme ble:Scheme;
  skos:prefLabel "Daylight Saving Time";
  prov:wasDerivedFrom <file:/data/lp/etl/executor/data/1651932367716-22-f5b1c2e0-1947-4a2e-a814-6ce401f2a604/working/working-outputfiles-33/gatt-xml-master/org.bluetooth.characteristic.local_time_information.xml> .

<http://purl.org/wot-catalogue/ble/gatt#EmailAddress> a skos:Concept, ontolex:LexicalConcept,
    prov:Entity;
  skos:altLabel "email address";
  skos:broader ble:Value;
  skos:inScheme ble:Scheme;
  skos:prefLabel "Email Address";
  prov:wasDerivedFrom <file:/data/lp/etl/executor/data/1651932367716-22-f5b1c2e0-1947-4a2e-a814-6ce401f2a604/working/working-outputfiles-33/gatt-xml-master/org.bluetooth.characteristic.email_address.xml> .

<http://purl.org/wot-catalogue/ble/gatt#MinimumResistanceLevel> a skos:Concept, ontolex:LexicalConcept,
    prov:Entity;
  skos:altLabel "minimum resistance level";
  skos:broader ble:Value;
  skos:definition """Unitless with a resolution of
      0.1""";
  skos:inScheme ble:Scheme;
  skos:prefLabel "Minimum Resistance Level";
  prov:wasDerivedFrom <file:/data/lp/etl/executor/data/1651932367716-22-f5b1c2e0-1947-4a2e-a814-6ce401f2a604/working/working-outputfiles-33/gatt-xml-master/org.bluetooth.characteristic.supported_resistance_level_range.xml> .

<http://purl.org/wot-catalogue/ble/gatt#MaximumResistanceLevel> a skos:Concept, ontolex:LexicalConcept,
    prov:Entity;
  skos:altLabel "maximum resistance level";
  skos:broader ble:Value;
  skos:definition """Unitless with a resolution of
      0.1""";
  skos:inScheme ble:Scheme;
  skos:prefLabel "Maximum Resistance Level";
  prov:wasDerivedFrom <file:/data/lp/etl/executor/data/1651932367716-22-f5b1c2e0-1947-4a2e-a814-6ce401f2a604/working/working-outputfiles-33/gatt-xml-master/org.bluetooth.characteristic.supported_resistance_level_range.xml> .

<http://purl.org/wot-catalogue/ble/gatt#1822> a skos:Concept, ontolex:LexicalConcept,
    prov:Entity;
  skos:altLabel "pulse oximeter service";
  skos:broader ble:Service;
  skos:definition """The Pulse Oximeter Service exposes pulse oximetry data
    related to a non-invasive pulse oximetry sensor for consumer
    and professional healthcare applications.""";
  skos:inScheme ble:Scheme;
  skos:prefLabel "Pulse Oximeter Service";
  skos:related ble:org.bluetooth.characteristic.plx_continuous_measurement, ble:org.bluetooth.characteristic.plx_features,
    ble:org.bluetooth.characteristic.plx_spot_check_measurement, ble:org.bluetooth.characteristic.record_access_control_point;
  prov:wasDerivedFrom <file:/data/lp/etl/executor/data/1651932367716-22-f5b1c2e0-1947-4a2e-a814-6ce401f2a604/working/working-outputfiles-33/gatt-xml-master/org.bluetooth.service.pulse_oximeter.xml> .

<http://purl.org/wot-catalogue/ble/gatt#org.bluetooth.characteristic.time_accuracy>
  a skos:Concept, ontolex:LexicalConcept, prov:Entity;
  skos:altLabel "time accuracy";
  skos:broader ble:Characteristic;
  skos:inScheme ble:Scheme;
  skos:prefLabel "Time Accuracy";
  skos:related ble:Accuracy;
  prov:wasDerivedFrom <file:/data/lp/etl/executor/data/1651932367716-22-f5b1c2e0-1947-4a2e-a814-6ce401f2a604/working/working-outputfiles-33/gatt-xml-master/org.bluetooth.characteristic.time_accuracy.xml> .

<http://purl.org/wot-catalogue/ble/gatt#AerobicHeartRateUpperLimit> a skos:Concept,
    ontolex:LexicalConcept, prov:Entity;
  skos:altLabel "aerobic heart rate upper limit";
  skos:broader ble:Value;
  skos:definition """Unit is in beats per minute with a
      resolution of 1""";
  skos:inScheme ble:Scheme;
  skos:prefLabel "Aerobic Heart Rate Upper Limit";
  prov:wasDerivedFrom <file:/data/lp/etl/executor/data/1651932367716-22-f5b1c2e0-1947-4a2e-a814-6ce401f2a604/working/working-outputfiles-33/gatt-xml-master/org.bluetooth.characteristic.aerobic_heart_rate_upper_limit.xml> .

<http://purl.org/wot-catalogue/ble/gatt#InstantaneousStrideLength> a skos:Concept,
    ontolex:LexicalConcept, prov:Entity;
  skos:altLabel "instantaneous stride length";
  skos:broader ble:Value;
  skos:definition """C1: Field exists if the key of bit 0 of the Flags field
        is set to 1.- Unit is in meter with a resolution of 1/100 m (or
        centimeter).""";
  skos:inScheme ble:Scheme;
  skos:prefLabel "Instantaneous Stride Length";
  prov:wasDerivedFrom <file:/data/lp/etl/executor/data/1651932367716-22-f5b1c2e0-1947-4a2e-a814-6ce401f2a604/working/working-outputfiles-33/gatt-xml-master/org.bluetooth.characteristic.rsc_measurement.xml> .

<http://purl.org/wot-catalogue/ble/gatt#ScanRefreshValue> a skos:Concept, ontolex:LexicalConcept,
    prov:Entity;
  skos:altLabel "scan refresh value";
  skos:broader ble:Value;
  skos:inScheme ble:Scheme;
  skos:prefLabel "Scan Refresh Value";
  prov:wasDerivedFrom <file:/data/lp/etl/executor/data/1651932367716-22-f5b1c2e0-1947-4a2e-a814-6ce401f2a604/working/working-outputfiles-33/gatt-xml-master/org.bluetooth.characteristic.scan_refresh.xml> .

<http://purl.org/wot-catalogue/ble/gatt#org.bluetooth.characteristic.apparent_wind_direction>
  a skos:Concept, ontolex:LexicalConcept, prov:Entity;
  skos:altLabel "apparent wind direction";
  skos:broader ble:Characteristic;
  skos:inScheme ble:Scheme;
  skos:prefLabel "Apparent Wind Direction";
  skos:related ble:ApparentWindDirection, ble:ExtendedProperties, ble:Notify, ble:Read,
    ble:WritableAuxiliaries;
  prov:wasDerivedFrom <file:/data/lp/etl/executor/data/1651932367716-22-f5b1c2e0-1947-4a2e-a814-6ce401f2a604/working/working-outputfiles-33/gatt-xml-master/org.bluetooth.characteristic.apparent_wind_direction.xml> .

<http://purl.org/wot-catalogue/ble/gatt#ApparentWindDirection> a skos:Concept, ontolex:LexicalConcept,
    prov:Entity;
  skos:altLabel "apparent wind direction";
  skos:broader ble:Value;
  skos:definition """Unit is in degrees with a resolution of 0.01
      degrees""";
  skos:inScheme ble:Scheme;
  skos:prefLabel "Apparent Wind Direction";
  prov:wasDerivedFrom <file:/data/lp/etl/executor/data/1651932367716-22-f5b1c2e0-1947-4a2e-a814-6ce401f2a604/working/working-outputfiles-33/gatt-xml-master/org.bluetooth.characteristic.apparent_wind_direction.xml> .

<http://purl.org/wot-catalogue/ble/gatt#UserIndex> a skos:Concept, ontolex:LexicalConcept,
    prov:Entity;
  skos:altLabel "user index";
  skos:broader ble:Value;
  skos:definition "When read, the User Index characteristic returns the index of the current user (i.e. the user that has given consent) to access the UDS Characteristics.";
  skos:inScheme ble:Scheme;
  skos:prefLabel "User Index";
  skos:related ble:Read;
  prov:wasDerivedFrom <file:/data/lp/etl/executor/data/1651932367716-22-f5b1c2e0-1947-4a2e-a814-6ce401f2a604/working/working-outputfiles-33/gatt-xml-master/org.bluetooth.characteristic.user_index.xml> .

<http://purl.org/wot-catalogue/ble/gatt#org.bluetooth.characteristic.Magnetic_flux_density_3D>
  a skos:Concept, ontolex:LexicalConcept, prov:Entity;
  skos:altLabel "magnetic flux density - 3d";
  skos:broader ble:Characteristic;
  skos:inScheme ble:Scheme;
  skos:prefLabel "Magnetic Flux Density - 3D";
  skos:related ble:MagneticFluxDensity:X-Axis, ble:MagneticFluxDensity:Y-Axis, ble:MagneticFluxDensity:Z-Axis;
  prov:wasDerivedFrom <file:/data/lp/etl/executor/data/1651932367716-22-f5b1c2e0-1947-4a2e-a814-6ce401f2a604/working/working-outputfiles-33/gatt-xml-master/org.bluetooth.characteristic.Magnetic_flux_density_3D.xml> .

<http://purl.org/wot-catalogue/ble/gatt#MagneticFluxDensity:Z-Axis> a skos:Concept,
    ontolex:LexicalConcept, prov:Entity;
  skos:altLabel "magnetic flux density: z-axis";
  skos:broader ble:Value;
  skos:inScheme ble:Scheme;
  skos:prefLabel "Magnetic Flux Density: Z-Axis";
  prov:wasDerivedFrom <file:/data/lp/etl/executor/data/1651932367716-22-f5b1c2e0-1947-4a2e-a814-6ce401f2a604/working/working-outputfiles-33/gatt-xml-master/org.bluetooth.characteristic.Magnetic_flux_density_3D.xml> .

<http://purl.org/wot-catalogue/ble/gatt#Weight> a skos:Concept, ontolex:LexicalConcept,
    prov:Entity;
  skos:altLabel "weight";
  skos:broader ble:Value;
  skos:definition """Unit is in kilograms with a resolution of
      0.005.""";
  skos:inScheme ble:Scheme;
  skos:prefLabel "Weight";
  prov:wasDerivedFrom <file:/data/lp/etl/executor/data/1651932367716-22-f5b1c2e0-1947-4a2e-a814-6ce401f2a604/working/working-outputfiles-33/gatt-xml-master/org.bluetooth.characteristic.weight.xml> .

<http://purl.org/wot-catalogue/ble/gatt#HeartRateMax> a skos:Concept, ontolex:LexicalConcept,
    prov:Entity;
  skos:altLabel "heart rate max";
  skos:broader ble:Value;
  skos:definition """Unit is in beats per minute with a
      resolution of 1.""";
  skos:inScheme ble:Scheme;
  skos:prefLabel "Heart Rate Max";
  prov:wasDerivedFrom <file:/data/lp/etl/executor/data/1651932367716-22-f5b1c2e0-1947-4a2e-a814-6ce401f2a604/working/working-outputfiles-33/gatt-xml-master/org.bluetooth.characteristic.heart_rate_max.xml> .

<http://purl.org/wot-catalogue/ble/gatt#TemperatureTextDescription> a skos:Concept,
    ontolex:LexicalConcept, prov:Entity;
  skos:altLabel "temperature text description";
  skos:broader ble:Value;
  skos:inScheme ble:Scheme;
  skos:prefLabel "Temperature Text Description";
  prov:wasDerivedFrom <file:/data/lp/etl/executor/data/1651932367716-22-f5b1c2e0-1947-4a2e-a814-6ce401f2a604/working/working-outputfiles-33/gatt-xml-master/org.bluetooth.characteristic.temperature_type.xml> .

<http://purl.org/wot-catalogue/ble/gatt#RingerControlPoint> a skos:Concept, ontolex:LexicalConcept,
    prov:Entity;
  skos:altLabel "ringer control point";
  skos:broader ble:Value;
  skos:inScheme ble:Scheme;
  skos:prefLabel "Ringer Control Point";
  prov:wasDerivedFrom <file:/data/lp/etl/executor/data/1651932367716-22-f5b1c2e0-1947-4a2e-a814-6ce401f2a604/working/working-outputfiles-33/gatt-xml-master/org.bluetooth.characteristic.ringer_control_point.xml> .

<http://purl.org/wot-catalogue/ble/gatt#1808> a skos:Concept, ontolex:LexicalConcept,
    prov:Entity;
  skos:altLabel "glucose";
  skos:broader ble:Service;
  skos:definition """The Glucose Service exposes glucose and other data
    related to a glucose sensor for consumer and professional
    healthcare applications.""";
  skos:inScheme ble:Scheme;
  skos:prefLabel "Glucose";
  skos:related ble:org.bluetooth.characteristic.glucose_feature, ble:org.bluetooth.characteristic.glucose_measurement,
    ble:org.bluetooth.characteristic.glucose_measurement_context, ble:org.bluetooth.characteristic.record_access_control_point;
  prov:wasDerivedFrom <file:/data/lp/etl/executor/data/1651932367716-22-f5b1c2e0-1947-4a2e-a814-6ce401f2a604/working/working-outputfiles-33/gatt-xml-master/org.bluetooth.service.glucose.xml> .

<http://purl.org/wot-catalogue/ble/gatt#org.bluetooth.characteristic.glucose_measurement_context>
  a skos:Concept, ontolex:LexicalConcept, prov:Entity;
  skos:altLabel "glucose measurement context";
  skos:broader ble:Characteristic;
  skos:definition """The Glucose Measurement Context characteristic is a
    variable length structure containing a Flags field, a Sequence
    Number field and, based upon the contents of the Flags field,
    may contain a Carbohydrate ID field, Carbohydrate field, Meal
    field, Tester-Health field, Exercise Duration field, Exercise
    Intensity field, Medication ID field, Medication field and a
    HbA1c field.""";
  skos:inScheme ble:Scheme;
  skos:prefLabel "Glucose Measurement Context";
  skos:related ble:Carbohydrate-unitsofkilograms, ble:CarbohydrateID, ble:ExerciseDuration,
    ble:ExerciseIntensity, ble:ExtendedFlags, ble:Flags, ble:HbA1c, ble:Health, ble:Meal,
    ble:Medication-unitsofkilograms, ble:Medication-unitsofliters, ble:MedicationID, ble:Notify,
    ble:SequenceNumber, ble:Tester;
  prov:wasDerivedFrom <file:/data/lp/etl/executor/data/1651932367716-22-f5b1c2e0-1947-4a2e-a814-6ce401f2a604/working/working-outputfiles-33/gatt-xml-master/org.bluetooth.characteristic.glucose_measurement_context.xml> .

<http://purl.org/wot-catalogue/ble/gatt#org.bluetooth.characteristic.unread_alert_status>
  a skos:Concept, ontolex:LexicalConcept, prov:Entity;
  skos:altLabel "unread alert status";
  skos:broader ble:Characteristic;
  skos:definition """This characteristic consists of ?Category ID? and
    ?uint8? which shows the number of unread
    alerts/messages.""";
  skos:inScheme ble:Scheme;
  skos:prefLabel "Unread Alert Status";
  skos:related ble:CategoryID, ble:Notify, ble:Unreadcount;
  prov:wasDerivedFrom <file:/data/lp/etl/executor/data/1651932367716-22-f5b1c2e0-1947-4a2e-a814-6ce401f2a604/working/working-outputfiles-33/gatt-xml-master/org.bluetooth.characteristic.unread_alert_status.xml> .

<http://purl.org/wot-catalogue/ble/gatt#Unreadcount> a skos:Concept, ontolex:LexicalConcept,
    prov:Entity;
  skos:altLabel "unread count";
  skos:broader ble:Value;
  skos:definition """How many unread alerts exist on the server. 
      If the value is 255, it means Unread count is greater than
      254.""";
  skos:inScheme ble:Scheme;
  skos:prefLabel "Unread count";
  prov:wasDerivedFrom <file:/data/lp/etl/executor/data/1651932367716-22-f5b1c2e0-1947-4a2e-a814-6ce401f2a604/working/working-outputfiles-33/gatt-xml-master/org.bluetooth.characteristic.unread_alert_status.xml> .

<http://purl.org/wot-catalogue/ble/gatt#Gender> a skos:Concept, ontolex:LexicalConcept,
    prov:Entity;
  skos:altLabel "gender";
  skos:broader ble:Value;
  skos:inScheme ble:Scheme;
  skos:prefLabel "Gender";
  prov:wasDerivedFrom <file:/data/lp/etl/executor/data/1651932367716-22-f5b1c2e0-1947-4a2e-a814-6ce401f2a604/working/working-outputfiles-33/gatt-xml-master/org.bluetooth.characteristic.gender.xml> .

<http://purl.org/wot-catalogue/ble/gatt#1804> a skos:Concept, ontolex:LexicalConcept,
    prov:Entity;
  skos:altLabel "tx power";
  skos:broader ble:Service;
  skos:definition """The Tx Power service is instantiated as a Primary
    Service. There is only one instance of the Tx Power service on
    a device. There is exactly one instance of the Tx Power Level
    characteristic""";
  skos:inScheme ble:Scheme;
  skos:prefLabel "Tx Power";
  skos:related ble:org.bluetooth.characteristic.tx_power_level;
  prov:wasDerivedFrom <file:/data/lp/etl/executor/data/1651932367716-22-f5b1c2e0-1947-4a2e-a814-6ce401f2a604/working/working-outputfiles-33/gatt-xml-master/org.bluetooth.service.tx_power.xml> .

<http://purl.org/wot-catalogue/ble/gatt#MaximumRecommendedHeartRate> a skos:Concept,
    ontolex:LexicalConcept, prov:Entity;
  skos:altLabel "maximum recommended heart rate";
  skos:broader ble:Value;
  skos:definition """The Unit is beats per minute with a
      resolution of 1""";
  skos:inScheme ble:Scheme;
  skos:prefLabel "Maximum Recommended Heart Rate";
  prov:wasDerivedFrom <file:/data/lp/etl/executor/data/1651932367716-22-f5b1c2e0-1947-4a2e-a814-6ce401f2a604/working/working-outputfiles-33/gatt-xml-master/org.bluetooth.characteristic.maximum_recommended_heart_rate.xml> .

<http://purl.org/wot-catalogue/ble/gatt#CurrentState> a skos:Concept, ontolex:LexicalConcept,
    prov:Entity;
  skos:altLabel "current state";
  skos:broader ble:Value;
  skos:inScheme ble:Scheme;
  skos:prefLabel "Current State";
  prov:wasDerivedFrom <file:/data/lp/etl/executor/data/1651932367716-22-f5b1c2e0-1947-4a2e-a814-6ce401f2a604/working/working-outputfiles-33/gatt-xml-master/org.bluetooth.characteristic.time_update_state.xml> .

<http://purl.org/wot-catalogue/ble/gatt#Result> a skos:Concept, ontolex:LexicalConcept,
    prov:Entity;
  skos:altLabel "result";
  skos:broader ble:Value;
  skos:inScheme ble:Scheme;
  skos:prefLabel "Result";
  prov:wasDerivedFrom <file:/data/lp/etl/executor/data/1651932367716-22-f5b1c2e0-1947-4a2e-a814-6ce401f2a604/working/working-outputfiles-33/gatt-xml-master/org.bluetooth.characteristic.time_update_state.xml> .

<http://purl.org/wot-catalogue/ble/gatt#org.bluetooth.characteristic.pollen_concentration>
  a skos:Concept, ontolex:LexicalConcept, prov:Entity;
  skos:altLabel "pollen concentration";
  skos:broader ble:Characteristic;
  skos:inScheme ble:Scheme;
  skos:prefLabel "Pollen Concentration";
  skos:related ble:ExtendedProperties, ble:Notify, ble:PollenConcentration, ble:Read,
    ble:WritableAuxiliaries;
  prov:wasDerivedFrom <file:/data/lp/etl/executor/data/1651932367716-22-f5b1c2e0-1947-4a2e-a814-6ce401f2a604/working/working-outputfiles-33/gatt-xml-master/org.bluetooth.characteristic.pollen_concentration.xml> .

<http://purl.org/wot-catalogue/ble/gatt#PollenConcentration> a skos:Concept, ontolex:LexicalConcept,
    prov:Entity;
  skos:altLabel "pollen concentration";
  skos:broader ble:Value;
  skos:definition """Unit is in concentration count per cubic
      meter with a resolution of 1/m^3""";
  skos:inScheme ble:Scheme;
  skos:prefLabel "Pollen Concentration";
  prov:wasDerivedFrom <file:/data/lp/etl/executor/data/1651932367716-22-f5b1c2e0-1947-4a2e-a814-6ce401f2a604/working/working-outputfiles-33/gatt-xml-master/org.bluetooth.characteristic.pollen_concentration.xml> .

<http://purl.org/wot-catalogue/ble/gatt#HIDControlPointCommand> a skos:Concept, ontolex:LexicalConcept,
    prov:Entity;
  skos:altLabel "hid control point command";
  skos:broader ble:Value;
  skos:definition """There are no response codes defined for the
      Suspend and Exit Suspend commands.""";
  skos:inScheme ble:Scheme;
  skos:prefLabel "HID Control Point Command";
  prov:wasDerivedFrom <file:/data/lp/etl/executor/data/1651932367716-22-f5b1c2e0-1947-4a2e-a814-6ce401f2a604/working/working-outputfiles-33/gatt-xml-master/org.bluetooth.characteristic.hid_control_point.xml> .

<http://purl.org/wot-catalogue/ble/gatt#StepCount> a skos:Concept, ontolex:LexicalConcept,
    prov:Entity;
  skos:altLabel "step count";
  skos:broader ble:Value;
  skos:definition """Unitless with a resolution of
      1""";
  skos:inScheme ble:Scheme;
  skos:prefLabel "Step Count";
  prov:wasDerivedFrom <file:/data/lp/etl/executor/data/1651932367716-22-f5b1c2e0-1947-4a2e-a814-6ce401f2a604/working/working-outputfiles-33/gatt-xml-master/org.bluetooth.characteristic.step_climber_data.xml> .

<http://purl.org/wot-catalogue/ble/gatt#1815> a skos:Concept, ontolex:LexicalConcept,
    prov:Entity;
  skos:altLabel "automation io";
  skos:broader ble:Service;
  skos:definition """The Automation IO service is used to expose the
    analog inputs/outputs and digital input/outputs of a generic IO
    module (IOM).""";
  skos:inScheme ble:Scheme;
  skos:prefLabel "Automation IO";
  skos:related ble:org.bluetooth.characteristic.aggregate, ble:org.bluetooth.characteristic.analog,
    ble:org.bluetooth.characteristic.digital;
  prov:wasDerivedFrom <file:/data/lp/etl/executor/data/1651932367716-22-f5b1c2e0-1947-4a2e-a814-6ce401f2a604/working/working-outputfiles-33/gatt-xml-master/org.bluetooth.service.automation_io.xml> .

<http://purl.org/wot-catalogue/ble/gatt#AnaerobicHeartRateLowerLimit> a skos:Concept,
    ontolex:LexicalConcept, prov:Entity;
  skos:altLabel "anaerobic heart rate lower limit";
  skos:broader ble:Value;
  skos:definition """Unit is in beats per minute with a
      resolution of 1""";
  skos:inScheme ble:Scheme;
  skos:prefLabel "Anaerobic Heart Rate Lower Limit";
  prov:wasDerivedFrom <file:/data/lp/etl/executor/data/1651932367716-22-f5b1c2e0-1947-4a2e-a814-6ce401f2a604/working/working-outputfiles-33/gatt-xml-master/org.bluetooth.characteristic.anaerobic_heart_rate_lower_limit.xml> .

<http://purl.org/wot-catalogue/ble/gatt#org.bluetooth.characteristic.body_sensor_location>
  a skos:Concept, ontolex:LexicalConcept, prov:Entity;
  skos:altLabel "body sensor location";
  skos:broader ble:Characteristic;
  skos:inScheme ble:Scheme;
  skos:prefLabel "Body Sensor Location";
  skos:related ble:BodySensorLocation, ble:Read;
  prov:wasDerivedFrom <file:/data/lp/etl/executor/data/1651932367716-22-f5b1c2e0-1947-4a2e-a814-6ce401f2a604/working/working-outputfiles-33/gatt-xml-master/org.bluetooth.characteristic.body_sensor_location.xml> .

<http://purl.org/wot-catalogue/ble/gatt#BodySensorLocation> a skos:Concept, ontolex:LexicalConcept,
    prov:Entity;
  skos:altLabel "body sensor location";
  skos:broader ble:Value;
  skos:inScheme ble:Scheme;
  skos:prefLabel "Body Sensor Location";
  prov:wasDerivedFrom <file:/data/lp/etl/executor/data/1651932367716-22-f5b1c2e0-1947-4a2e-a814-6ce401f2a604/working/working-outputfiles-33/gatt-xml-master/org.bluetooth.characteristic.body_sensor_location.xml> .

<http://purl.org/wot-catalogue/ble/gatt#org.bluetooth.characteristic.supported_new_alert_category>
  a skos:Concept, ontolex:LexicalConcept, prov:Entity;
  skos:altLabel "supported new alert category";
  skos:broader ble:Characteristic;
  skos:definition """This characteristic uses the Alert Category ID Bit
    Mask Characteristic. If bit(s) is/are set, it means the server
    supports the corresponded categories for new incoming
    alert.""";
  skos:inScheme ble:Scheme;
  skos:prefLabel "Supported New Alert Category";
  skos:related ble:CategoryIDBitMask, ble:Read;
  prov:wasDerivedFrom <file:/data/lp/etl/executor/data/1651932367716-22-f5b1c2e0-1947-4a2e-a814-6ce401f2a604/working/working-outputfiles-33/gatt-xml-master/org.bluetooth.characteristic.supported_new_alert_category.xml> .

<http://purl.org/wot-catalogue/ble/gatt#CategoryIDBitMask> a skos:Concept, ontolex:LexicalConcept,
    prov:Entity;
  skos:altLabel "category id bit mask";
  skos:broader ble:Value;
  skos:inScheme ble:Scheme;
  skos:prefLabel "Category ID Bit Mask";
  prov:wasDerivedFrom <file:/data/lp/etl/executor/data/1651932367716-22-f5b1c2e0-1947-4a2e-a814-6ce401f2a604/working/working-outputfiles-33/gatt-xml-master/org.bluetooth.characteristic.supported_new_alert_category.xml>,
    <file:/data/lp/etl/executor/data/1651932367716-22-f5b1c2e0-1947-4a2e-a814-6ce401f2a604/working/working-outputfiles-33/gatt-xml-master/org.bluetooth.characteristic.supported_unread_alert_category.xml> .

<http://purl.org/wot-catalogue/ble/gatt#ExtendedFlags> a skos:Concept, ontolex:LexicalConcept,
    prov:Entity;
  skos:altLabel "extended flags";
  skos:broader ble:Value;
  skos:definition """C1: Field exists if the key of bit 7 of the
      Flags field is set to 1""";
  skos:inScheme ble:Scheme;
  skos:prefLabel "Extended Flags";
  prov:wasDerivedFrom <file:/data/lp/etl/executor/data/1651932367716-22-f5b1c2e0-1947-4a2e-a814-6ce401f2a604/working/working-outputfiles-33/gatt-xml-master/org.bluetooth.characteristic.glucose_measurement_context.xml> .

<http://purl.org/wot-catalogue/ble/gatt#CarbohydrateID> a skos:Concept, ontolex:LexicalConcept,
    prov:Entity;
  skos:altLabel "carbohydrate id";
  skos:broader ble:Value;
  skos:definition """C2: Field exists if the key of bit 0 of the
      Flags field is set to 1""";
  skos:inScheme ble:Scheme;
  skos:prefLabel "Carbohydrate ID";
  prov:wasDerivedFrom <file:/data/lp/etl/executor/data/1651932367716-22-f5b1c2e0-1947-4a2e-a814-6ce401f2a604/working/working-outputfiles-33/gatt-xml-master/org.bluetooth.characteristic.glucose_measurement_context.xml> .

<http://purl.org/wot-catalogue/ble/gatt#Carbohydrate-unitsofkilograms> a skos:Concept,
    ontolex:LexicalConcept, prov:Entity;
  skos:altLabel "carbohydrate - units of kilograms";
  skos:broader ble:Value;
  skos:definition """C2: Field exists if the key of bit 0 of the
      Flags field is set to 1""";
  skos:inScheme ble:Scheme;
  skos:prefLabel "Carbohydrate - units of kilograms";
  prov:wasDerivedFrom <file:/data/lp/etl/executor/data/1651932367716-22-f5b1c2e0-1947-4a2e-a814-6ce401f2a604/working/working-outputfiles-33/gatt-xml-master/org.bluetooth.characteristic.glucose_measurement_context.xml> .

<http://purl.org/wot-catalogue/ble/gatt#Meal> a skos:Concept, ontolex:LexicalConcept,
    prov:Entity;
  skos:altLabel "meal";
  skos:broader ble:Value;
  skos:definition """C3: Field exists if the key of bit 1 of the
      Flags field is set to 1""";
  skos:inScheme ble:Scheme;
  skos:prefLabel "Meal";
  prov:wasDerivedFrom <file:/data/lp/etl/executor/data/1651932367716-22-f5b1c2e0-1947-4a2e-a814-6ce401f2a604/working/working-outputfiles-33/gatt-xml-master/org.bluetooth.characteristic.glucose_measurement_context.xml> .

<http://purl.org/wot-catalogue/ble/gatt#Tester> a skos:Concept, ontolex:LexicalConcept,
    prov:Entity;
  skos:altLabel "tester";
  skos:broader ble:Value;
  skos:definition """C4: Field exists if the key of bit 2 of the
      Flags field is set to 1""";
  skos:inScheme ble:Scheme;
  skos:prefLabel "Tester";
  prov:wasDerivedFrom <file:/data/lp/etl/executor/data/1651932367716-22-f5b1c2e0-1947-4a2e-a814-6ce401f2a604/working/working-outputfiles-33/gatt-xml-master/org.bluetooth.characteristic.glucose_measurement_context.xml> .

<http://purl.org/wot-catalogue/ble/gatt#Health> a skos:Concept, ontolex:LexicalConcept,
    prov:Entity;
  skos:altLabel "health";
  skos:broader ble:Value;
  skos:definition """C4: Field exists if the key of bit 2 of the
      Flags field is set to 1""";
  skos:inScheme ble:Scheme;
  skos:prefLabel "Health";
  prov:wasDerivedFrom <file:/data/lp/etl/executor/data/1651932367716-22-f5b1c2e0-1947-4a2e-a814-6ce401f2a604/working/working-outputfiles-33/gatt-xml-master/org.bluetooth.characteristic.glucose_measurement_context.xml> .

<http://purl.org/wot-catalogue/ble/gatt#ExerciseDuration> a skos:Concept, ontolex:LexicalConcept,
    prov:Entity;
  skos:altLabel "exercise duration";
  skos:broader ble:Value;
  skos:definition """C5: Field exists if the key of bit 3 of the
      Flags field is set to 1""";
  skos:inScheme ble:Scheme;
  skos:prefLabel "Exercise Duration";
  prov:wasDerivedFrom <file:/data/lp/etl/executor/data/1651932367716-22-f5b1c2e0-1947-4a2e-a814-6ce401f2a604/working/working-outputfiles-33/gatt-xml-master/org.bluetooth.characteristic.glucose_measurement_context.xml> .

<http://purl.org/wot-catalogue/ble/gatt#ExerciseIntensity> a skos:Concept, ontolex:LexicalConcept,
    prov:Entity;
  skos:altLabel "exercise intensity";
  skos:broader ble:Value;
  skos:definition """C5: Field exists if the key of bit 3 of the
      Flags field is set to 1""";
  skos:inScheme ble:Scheme;
  skos:prefLabel "Exercise Intensity";
  prov:wasDerivedFrom <file:/data/lp/etl/executor/data/1651932367716-22-f5b1c2e0-1947-4a2e-a814-6ce401f2a604/working/working-outputfiles-33/gatt-xml-master/org.bluetooth.characteristic.glucose_measurement_context.xml> .

<http://purl.org/wot-catalogue/ble/gatt#MedicationID> a skos:Concept, ontolex:LexicalConcept,
    prov:Entity;
  skos:altLabel "medication id";
  skos:broader ble:Value;
  skos:definition """C6: Field exists if the key of bit 4 of the
      Flags field is set to 1""";
  skos:inScheme ble:Scheme;
  skos:prefLabel "Medication ID";
  prov:wasDerivedFrom <file:/data/lp/etl/executor/data/1651932367716-22-f5b1c2e0-1947-4a2e-a814-6ce401f2a604/working/working-outputfiles-33/gatt-xml-master/org.bluetooth.characteristic.glucose_measurement_context.xml> .

<http://purl.org/wot-catalogue/ble/gatt#Medication-unitsofkilograms> a skos:Concept,
    ontolex:LexicalConcept, prov:Entity;
  skos:altLabel "medication - units of kilograms";
  skos:broader ble:Value;
  skos:definition """C6: Field exists if the key of bit 4 of the
      Flags field is set to 1, C8: Field exists if the key of bit 5
      of the Flags field is set to 0""";
  skos:inScheme ble:Scheme;
  skos:prefLabel "Medication - units of kilograms";
  prov:wasDerivedFrom <file:/data/lp/etl/executor/data/1651932367716-22-f5b1c2e0-1947-4a2e-a814-6ce401f2a604/working/working-outputfiles-33/gatt-xml-master/org.bluetooth.characteristic.glucose_measurement_context.xml> .

<http://purl.org/wot-catalogue/ble/gatt#Medication-unitsofliters> a skos:Concept,
    ontolex:LexicalConcept, prov:Entity;
  skos:altLabel "medication - units of liters";
  skos:broader ble:Value;
  skos:definition """C6: Field exists if the key of bit 4 of the
      Flags field is set to 1, C9: Field exists if the key of bit 5
      of the Flags field is set to 1""";
  skos:inScheme ble:Scheme;
  skos:prefLabel "Medication - units of liters";
  prov:wasDerivedFrom <file:/data/lp/etl/executor/data/1651932367716-22-f5b1c2e0-1947-4a2e-a814-6ce401f2a604/working/working-outputfiles-33/gatt-xml-master/org.bluetooth.characteristic.glucose_measurement_context.xml> .

<http://purl.org/wot-catalogue/ble/gatt#HbA1c> a skos:Concept, ontolex:LexicalConcept,
    prov:Entity;
  skos:altLabel "hba1c";
  skos:broader ble:Value;
  skos:definition """C7: Field exists if the key of bit 6 of the
      Flags field is set to 1""";
  skos:inScheme ble:Scheme;
  skos:prefLabel "HbA1c";
  prov:wasDerivedFrom <file:/data/lp/etl/executor/data/1651932367716-22-f5b1c2e0-1947-4a2e-a814-6ce401f2a604/working/working-outputfiles-33/gatt-xml-master/org.bluetooth.characteristic.glucose_measurement_context.xml> .

<http://purl.org/wot-catalogue/ble/gatt#org.bluetooth.characteristic.csc_measurement>
  a skos:Concept, ontolex:LexicalConcept, prov:Entity;
  skos:altLabel "csc measurement";
  skos:broader ble:Characteristic;
  skos:definition """The CSC Measurement characteristic (CSC refers to
    Cycling Speed and Cadence) is a variable length structure
    containing a Flags field and, based on the contents of the
    Flags field, may contain one or more additional fields as shown
    in the tables below.""";
  skos:inScheme ble:Scheme;
  skos:prefLabel "CSC Measurement";
  skos:related ble:CumulativeCrankRevolutions, ble:CumulativeWheelRevolutions, ble:Flags,
    ble:LastCrankEventTime, ble:LastWheelEventTime, ble:Notify;
  prov:wasDerivedFrom <file:/data/lp/etl/executor/data/1651932367716-22-f5b1c2e0-1947-4a2e-a814-6ce401f2a604/working/working-outputfiles-33/gatt-xml-master/org.bluetooth.characteristic.csc_measurement.xml> .

<http://purl.org/wot-catalogue/ble/gatt#CumulativeWheelRevolutions> a skos:Concept,
    ontolex:LexicalConcept, prov:Entity;
  skos:altLabel "cumulative wheel revolutions";
  skos:broader ble:Value;
  skos:definition """C1: Field exists if the key of bit 0 of the
      Flags field is set to 1.""";
  skos:inScheme ble:Scheme;
  skos:prefLabel "Cumulative Wheel Revolutions";
  prov:wasDerivedFrom <file:/data/lp/etl/executor/data/1651932367716-22-f5b1c2e0-1947-4a2e-a814-6ce401f2a604/working/working-outputfiles-33/gatt-xml-master/org.bluetooth.characteristic.csc_measurement.xml> .

<http://purl.org/wot-catalogue/ble/gatt#LastWheelEventTime> a skos:Concept, ontolex:LexicalConcept,
    prov:Entity;
  skos:altLabel "last wheel event time";
  skos:broader ble:Value;
  skos:definition """Unit has a resolution of 1/1024s. 
      C1: Field exists if the key of bit 0 of the Flags field
      is set to 1.""";
  skos:inScheme ble:Scheme;
  skos:prefLabel "Last Wheel Event Time";
  prov:wasDerivedFrom <file:/data/lp/etl/executor/data/1651932367716-22-f5b1c2e0-1947-4a2e-a814-6ce401f2a604/working/working-outputfiles-33/gatt-xml-master/org.bluetooth.characteristic.csc_measurement.xml> .

<http://purl.org/wot-catalogue/ble/gatt#CumulativeCrankRevolutions> a skos:Concept,
    ontolex:LexicalConcept, prov:Entity;
  skos:altLabel "cumulative crank revolutions";
  skos:broader ble:Value;
  skos:definition """C2: Field exists if the key of bit 1 of the
      Flags field is set to 1.""",
    "The Cumulative Crank Revolutions value represents the number of times a crank rotates and is one value of Crank Revolution Data pair.";
  skos:inScheme ble:Scheme;
  skos:prefLabel "Cumulative Crank Revolutions";
  skos:related xsd:unsignedShort;
  prov:wasDerivedFrom <file:/data/lp/etl/executor/data/1651932367716-22-f5b1c2e0-1947-4a2e-a814-6ce401f2a604/working/working-outputfiles-33/gatt-xml-master/org.bluetooth.characteristic.csc_measurement.xml> .

<http://purl.org/wot-catalogue/ble/gatt#LastCrankEventTime> a skos:Concept, ontolex:LexicalConcept,
    prov:Entity;
  skos:altLabel "last crank event time";
  skos:broader ble:Value;
  skos:definition """C2: Field exists if the key of bit 1 of the
      Flags field is set to 1. 
      Unit has a resolution of 1/1024s.""",
    "The Last Crank Event Time is one value of Crank Revolution Data pair and always presents as a pair with Cumulative Crank Revolutions.";
  skos:inScheme ble:Scheme;
  skos:prefLabel "Last Crank Event Time";
  skos:related xsd:unsignedShort;
  prov:wasDerivedFrom <file:/data/lp/etl/executor/data/1651932367716-22-f5b1c2e0-1947-4a2e-a814-6ce401f2a604/working/working-outputfiles-33/gatt-xml-master/org.bluetooth.characteristic.csc_measurement.xml> .

<http://purl.org/wot-catalogue/ble/gatt#Height> a skos:Concept, ontolex:LexicalConcept,
    prov:Entity;
  skos:altLabel "height";
  skos:broader ble:Value;
  skos:definition """Unit is in meters with a resolution of 0.01
      .""";
  skos:inScheme ble:Scheme;
  skos:prefLabel "Height";
  prov:wasDerivedFrom <file:/data/lp/etl/executor/data/1651932367716-22-f5b1c2e0-1947-4a2e-a814-6ce401f2a604/working/working-outputfiles-33/gatt-xml-master/org.bluetooth.characteristic.height.xml> .

<http://purl.org/wot-catalogue/ble/gatt#org.bluetooth.characteristic.day_of_week>
  a skos:Concept, ontolex:LexicalConcept, prov:Entity;
  skos:altLabel "day of week";
  skos:broader ble:Characteristic;
  skos:inScheme ble:Scheme;
  skos:prefLabel "Day of Week";
  skos:related ble:DayofWeek;
  prov:wasDerivedFrom <file:/data/lp/etl/executor/data/1651932367716-22-f5b1c2e0-1947-4a2e-a814-6ce401f2a604/working/working-outputfiles-33/gatt-xml-master/org.bluetooth.characteristic.day_of_week.xml> .

<http://purl.org/wot-catalogue/ble/gatt#NumberofBeaconsinSolution> a skos:Concept,
    ontolex:LexicalConcept, prov:Entity;
  skos:altLabel "number of beacons in solution";
  skos:broader ble:Value;
  skos:definition """Unitless with a resolution of
      1""";
  skos:inScheme ble:Scheme;
  skos:prefLabel "Number of Beacons in Solution";
  prov:wasDerivedFrom <file:/data/lp/etl/executor/data/1651932367716-22-f5b1c2e0-1947-4a2e-a814-6ce401f2a604/working/working-outputfiles-33/gatt-xml-master/org.bluetooth.characteristic.position_quality.xml> .

<http://purl.org/wot-catalogue/ble/gatt#NumberofBeaconsinView> a skos:Concept, ontolex:LexicalConcept,
    prov:Entity;
  skos:altLabel "number of beacons in view";
  skos:broader ble:Value;
  skos:definition """Unitless with a resolution of
      1""";
  skos:inScheme ble:Scheme;
  skos:prefLabel "Number of Beacons in View";
  prov:wasDerivedFrom <file:/data/lp/etl/executor/data/1651932367716-22-f5b1c2e0-1947-4a2e-a814-6ce401f2a604/working/working-outputfiles-33/gatt-xml-master/org.bluetooth.characteristic.position_quality.xml> .

<http://purl.org/wot-catalogue/ble/gatt#TimetoFirstFix> a skos:Concept, ontolex:LexicalConcept,
    prov:Entity;
  skos:altLabel "time to first fix";
  skos:broader ble:Value;
  skos:definition """Unit is in seconds with a resolution of
      1/10""";
  skos:inScheme ble:Scheme;
  skos:prefLabel "Time to First Fix";
  prov:wasDerivedFrom <file:/data/lp/etl/executor/data/1651932367716-22-f5b1c2e0-1947-4a2e-a814-6ce401f2a604/working/working-outputfiles-33/gatt-xml-master/org.bluetooth.characteristic.position_quality.xml> .

<http://purl.org/wot-catalogue/ble/gatt#EHPE> a skos:Concept, ontolex:LexicalConcept,
    prov:Entity;
  skos:altLabel "ehpe";
  skos:broader ble:Value;
  skos:definition """Unit is in meters with a resolution of
      1/100""";
  skos:inScheme ble:Scheme;
  skos:prefLabel "EHPE";
  prov:wasDerivedFrom <file:/data/lp/etl/executor/data/1651932367716-22-f5b1c2e0-1947-4a2e-a814-6ce401f2a604/working/working-outputfiles-33/gatt-xml-master/org.bluetooth.characteristic.position_quality.xml> .

<http://purl.org/wot-catalogue/ble/gatt#EVPE> a skos:Concept, ontolex:LexicalConcept,
    prov:Entity;
  skos:altLabel "evpe";
  skos:broader ble:Value;
  skos:definition """Unit is in meters with a resolution of
      1/100""";
  skos:inScheme ble:Scheme;
  skos:prefLabel "EVPE";
  prov:wasDerivedFrom <file:/data/lp/etl/executor/data/1651932367716-22-f5b1c2e0-1947-4a2e-a814-6ce401f2a604/working/working-outputfiles-33/gatt-xml-master/org.bluetooth.characteristic.position_quality.xml> .

<http://purl.org/wot-catalogue/ble/gatt#HDOP> a skos:Concept, ontolex:LexicalConcept,
    prov:Entity;
  skos:altLabel "hdop";
  skos:broader ble:Value;
  skos:definition """Unitless with a resolution of
      2/10""";
  skos:inScheme ble:Scheme;
  skos:prefLabel "HDOP";
  prov:wasDerivedFrom <file:/data/lp/etl/executor/data/1651932367716-22-f5b1c2e0-1947-4a2e-a814-6ce401f2a604/working/working-outputfiles-33/gatt-xml-master/org.bluetooth.characteristic.position_quality.xml> .

<http://purl.org/wot-catalogue/ble/gatt#VDOP> a skos:Concept, ontolex:LexicalConcept,
    prov:Entity;
  skos:altLabel "vdop";
  skos:broader ble:Value;
  skos:definition """Unitless with a resolution of
      2/10""";
  skos:inScheme ble:Scheme;
  skos:prefLabel "VDOP";
  prov:wasDerivedFrom <file:/data/lp/etl/executor/data/1651932367716-22-f5b1c2e0-1947-4a2e-a814-6ce401f2a604/working/working-outputfiles-33/gatt-xml-master/org.bluetooth.characteristic.position_quality.xml> .

<http://purl.org/wot-catalogue/ble/gatt#org.bluetooth.characteristic.humidity> a skos:Concept,
    ontolex:LexicalConcept, prov:Entity;
  skos:altLabel "humidity";
  skos:broader ble:Characteristic;
  skos:inScheme ble:Scheme;
  skos:prefLabel "Humidity";
  skos:related ble:ExtendedProperties, ble:Humidity, ble:Notify, ble:Read, ble:WritableAuxiliaries;
  prov:wasDerivedFrom <file:/data/lp/etl/executor/data/1651932367716-22-f5b1c2e0-1947-4a2e-a814-6ce401f2a604/working/working-outputfiles-33/gatt-xml-master/org.bluetooth.characteristic.humidity.xml> .

<http://purl.org/wot-catalogue/ble/gatt#Humidity> a skos:Concept, ontolex:LexicalConcept,
    prov:Entity;
  skos:altLabel "humidity";
  skos:broader ble:Value;
  skos:definition """Unit is in percent with a resolution of 0.01
      percent""";
  skos:inScheme ble:Scheme;
  skos:prefLabel "Humidity";
  prov:wasDerivedFrom <file:/data/lp/etl/executor/data/1651932367716-22-f5b1c2e0-1947-4a2e-a814-6ce401f2a604/working/working-outputfiles-33/gatt-xml-master/org.bluetooth.characteristic.humidity.xml> .

<http://purl.org/wot-catalogue/ble/gatt#1816> a skos:Concept, ontolex:LexicalConcept,
    prov:Entity;
  skos:altLabel "cycling speed and cadence";
  skos:broader ble:Service;
  skos:definition """The Cycling Speed and Cadence (CSC) Service exposes
    speed-related data and/or cadence-related data while using the
    Cycling Speed and Cadence sensor (Server).""";
  skos:inScheme ble:Scheme;
  skos:prefLabel "Cycling Speed and Cadence";
  skos:related ble:org.bluetooth.characteristic.csc_feature, ble:org.bluetooth.characteristic.csc_measurement,
    ble:org.bluetooth.characteristic.sc_control_point, ble:org.bluetooth.characteristic.sensor_location;
  prov:wasDerivedFrom <file:/data/lp/etl/executor/data/1651932367716-22-f5b1c2e0-1947-4a2e-a814-6ce401f2a604/working/working-outputfiles-33/gatt-xml-master/org.bluetooth.service.cycling_speed_and_cadence.xml> .

<http://purl.org/wot-catalogue/ble/gatt#org.bluetooth.characteristic.supported_unread_alert_category>
  a skos:Concept, ontolex:LexicalConcept, prov:Entity;
  skos:altLabel "supported unread alert category";
  skos:broader ble:Characteristic;
  skos:definition """This characteristic uses the Alert Category ID Bit
    Mask Characteristic. If bit(s) is/are set, it means the server
    supports the corresponded categories for unread
    alert.""";
  skos:inScheme ble:Scheme;
  skos:prefLabel "Supported Unread Alert Category";
  skos:related ble:CategoryIDBitMask, ble:Read;
  prov:wasDerivedFrom <file:/data/lp/etl/executor/data/1651932367716-22-f5b1c2e0-1947-4a2e-a814-6ce401f2a604/working/working-outputfiles-33/gatt-xml-master/org.bluetooth.characteristic.supported_unread_alert_category.xml> .

<http://purl.org/wot-catalogue/ble/gatt#org.bluetooth.characteristic.pressure> a skos:Concept,
    ontolex:LexicalConcept, prov:Entity;
  skos:altLabel "pressure";
  skos:broader ble:Characteristic;
  skos:inScheme ble:Scheme;
  skos:prefLabel "Pressure";
  skos:related ble:ExtendedProperties, ble:Notify, ble:Pressure, ble:Read, ble:WritableAuxiliaries;
  prov:wasDerivedFrom <file:/data/lp/etl/executor/data/1651932367716-22-f5b1c2e0-1947-4a2e-a814-6ce401f2a604/working/working-outputfiles-33/gatt-xml-master/org.bluetooth.characteristic.pressure.xml> .

<http://purl.org/wot-catalogue/ble/gatt#Pressure> a skos:Concept, ontolex:LexicalConcept,
    prov:Entity;
  skos:altLabel "pressure";
  skos:broader ble:Value;
  skos:definition """Unit is in pascals with a resolution of 0.1
      Pa""";
  skos:inScheme ble:Scheme;
  skos:prefLabel "Pressure";
  prov:wasDerivedFrom <file:/data/lp/etl/executor/data/1651932367716-22-f5b1c2e0-1947-4a2e-a814-6ce401f2a604/working/working-outputfiles-33/gatt-xml-master/org.bluetooth.characteristic.pressure.xml> .

<http://purl.org/wot-catalogue/ble/gatt#HTTPSSecurity> a skos:Concept, ontolex:LexicalConcept,
    prov:Entity;
  skos:altLabel "https security";
  skos:broader ble:Value;
  skos:definition """The known authenticity of the HTTP Server
      certificate for the URI.""";
  skos:inScheme ble:Scheme;
  skos:prefLabel "HTTPS Security";
  prov:wasDerivedFrom <file:/data/lp/etl/executor/data/1651932367716-22-f5b1c2e0-1947-4a2e-a814-6ce401f2a604/working/working-outputfiles-33/gatt-xml-master/org.bluetooth.characteristic.https_security.xml> .

<http://purl.org/wot-catalogue/ble/gatt#1810> a skos:Concept, ontolex:LexicalConcept,
    prov:Entity;
  skos:altLabel "blood pressure";
  skos:broader ble:Service;
  skos:definition """The BLOOD PRESSURE Service exposes blood pressure and
    other data related to a blood pressure monitor.""";
  skos:inScheme ble:Scheme;
  skos:prefLabel "Blood Pressure";
  skos:related ble:org.bluetooth.characteristic.blood_pressure_feature, ble:org.bluetooth.characteristic.blood_pressure_measurement,
    ble:org.bluetooth.characteristic.intermediate_cuff_pressure;
  prov:wasDerivedFrom <file:/data/lp/etl/executor/data/1651932367716-22-f5b1c2e0-1947-4a2e-a814-6ce401f2a604/working/working-outputfiles-33/gatt-xml-master/org.bluetooth.service.blood_pressure.xml> .

<http://purl.org/wot-catalogue/ble/gatt#org.bluetooth.characteristic.blood_pressure_feature>
  a skos:Concept, ontolex:LexicalConcept, prov:Entity;
  skos:altLabel "blood pressure feature";
  skos:broader ble:Characteristic;
  skos:definition """The Blood Pressure Feature characteristic is used to
    describe the supported features of the Blood Pressure
    Sensor.""";
  skos:inScheme ble:Scheme;
  skos:prefLabel "Blood Pressure Feature";
  skos:related ble:BloodPressureFeature, ble:Read;
  prov:wasDerivedFrom <file:/data/lp/etl/executor/data/1651932367716-22-f5b1c2e0-1947-4a2e-a814-6ce401f2a604/working/working-outputfiles-33/gatt-xml-master/org.bluetooth.characteristic.blood_pressure_feature.xml> .

<http://purl.org/wot-catalogue/ble/gatt#ReportValue> a skos:Concept, ontolex:LexicalConcept,
    prov:Entity;
  skos:altLabel "report value";
  skos:broader ble:Value;
  skos:inScheme ble:Scheme;
  skos:prefLabel "Report Value";
  prov:wasDerivedFrom <file:/data/lp/etl/executor/data/1651932367716-22-f5b1c2e0-1947-4a2e-a814-6ce401f2a604/working/working-outputfiles-33/gatt-xml-master/org.bluetooth.characteristic.report.xml> .

<http://purl.org/wot-catalogue/ble/gatt#TemperatureMeasurementValue(Celsius)> a skos:Concept,
    ontolex:LexicalConcept, prov:Entity;
  skos:altLabel "temperature measurement value (celsius)";
  skos:broader ble:Value;
  skos:definition """This field is only included if the flags bit
      0 is 0.""";
  skos:inScheme ble:Scheme;
  skos:prefLabel "Temperature Measurement Value (Celsius)";
  prov:wasDerivedFrom <file:/data/lp/etl/executor/data/1651932367716-22-f5b1c2e0-1947-4a2e-a814-6ce401f2a604/working/working-outputfiles-33/gatt-xml-master/org.bluetooth.characteristic.temperature_measurement.xml> .

<http://purl.org/wot-catalogue/ble/gatt#TemperatureMeasurementValue(Fahrenheit)> a
    skos:Concept, ontolex:LexicalConcept, prov:Entity;
  skos:altLabel "temperature measurement value (fahrenheit)";
  skos:broader ble:Value;
  skos:definition """This field is only included if the flags bit
      0 is 1.""";
  skos:inScheme ble:Scheme;
  skos:prefLabel "Temperature Measurement Value (Fahrenheit)";
  prov:wasDerivedFrom <file:/data/lp/etl/executor/data/1651932367716-22-f5b1c2e0-1947-4a2e-a814-6ce401f2a604/working/working-outputfiles-33/gatt-xml-master/org.bluetooth.characteristic.temperature_measurement.xml> .

<http://purl.org/wot-catalogue/ble/gatt#TemperatureType> a skos:Concept, ontolex:LexicalConcept,
    prov:Entity;
  skos:altLabel "temperature type";
  skos:broader ble:Value;
  skos:definition """If the flags bit 2 is set to 1 this field is
      included. If it is 0, this field is not
      included""";
  skos:inScheme ble:Scheme;
  skos:prefLabel "Temperature Type";
  prov:wasDerivedFrom <file:/data/lp/etl/executor/data/1651932367716-22-f5b1c2e0-1947-4a2e-a814-6ce401f2a604/working/working-outputfiles-33/gatt-xml-master/org.bluetooth.characteristic.temperature_measurement.xml> .

<http://purl.org/wot-catalogue/ble/gatt#ThreezoneHeartRateLimits-Light(Fatburn)/Moderate(Aerobic)Limit>
  a skos:Concept, ontolex:LexicalConcept, prov:Entity;
  skos:altLabel "three zone heart rate limits - light (fat burn) / moderate (aerobic) limit";
  skos:broader ble:Value;
  skos:definition """Unit is in beats per minute with a
      resolution of 1""";
  skos:inScheme ble:Scheme;
  skos:prefLabel "Three zone Heart Rate Limits - Light (Fat burn) / Moderate (Aerobic) Limit";
  prov:wasDerivedFrom <file:/data/lp/etl/executor/data/1651932367716-22-f5b1c2e0-1947-4a2e-a814-6ce401f2a604/working/working-outputfiles-33/gatt-xml-master/org.bluetooth.characteristic.three_zone_heart_rate_limits.xml> .

<http://purl.org/wot-catalogue/ble/gatt#ThreezoneHeartRateLimits-Moderate(Aerobic)/Hard(Anaerobic)Limit>
  a skos:Concept, ontolex:LexicalConcept, prov:Entity;
  skos:altLabel "three zone heart rate limits - moderate (aerobic) / hard (anaerobic) limit";
  skos:broader ble:Value;
  skos:definition """Unit is in beats per minute with a
      resolution of 1""";
  skos:inScheme ble:Scheme;
  skos:prefLabel "Three zone Heart Rate Limits - Moderate (Aerobic) / Hard (Anaerobic) Limit";
  prov:wasDerivedFrom <file:/data/lp/etl/executor/data/1651932367716-22-f5b1c2e0-1947-4a2e-a814-6ce401f2a604/working/working-outputfiles-33/gatt-xml-master/org.bluetooth.characteristic.three_zone_heart_rate_limits.xml> .

<http://purl.org/wot-catalogue/ble/gatt#org.bluetooth.characteristic.dst_offset> a
    skos:Concept, ontolex:LexicalConcept, prov:Entity;
  skos:altLabel "dst offset";
  skos:broader ble:Characteristic;
  skos:inScheme ble:Scheme;
  skos:prefLabel "DST Offset";
  skos:related ble:DSTOffset;
  prov:wasDerivedFrom <file:/data/lp/etl/executor/data/1651932367716-22-f5b1c2e0-1947-4a2e-a814-6ce401f2a604/working/working-outputfiles-33/gatt-xml-master/org.bluetooth.characteristic.dst_offset.xml> .

<http://purl.org/wot-catalogue/ble/gatt#DSTOffset> a skos:Concept, ontolex:LexicalConcept,
    prov:Entity;
  skos:altLabel "dst offset";
  skos:broader ble:Value;
  skos:inScheme ble:Scheme;
  skos:prefLabel "DST Offset";
  prov:wasDerivedFrom <file:/data/lp/etl/executor/data/1651932367716-22-f5b1c2e0-1947-4a2e-a814-6ce401f2a604/working/working-outputfiles-33/gatt-xml-master/org.bluetooth.characteristic.dst_offset.xml>,
    <file:/data/lp/etl/executor/data/1651932367716-22-f5b1c2e0-1947-4a2e-a814-6ce401f2a604/working/working-outputfiles-33/gatt-xml-master/org.bluetooth.characteristic.time_with_dst.xml> .

<http://purl.org/wot-catalogue/ble/gatt#180D> a skos:Concept, ontolex:LexicalConcept,
    prov:Entity;
  skos:altLabel "heart rate";
  skos:broader ble:Service;
  skos:definition """The HEART RATE Service exposes heart rate and other
    data related to a heart rate sensor intended for fitness
    applications.""";
  skos:inScheme ble:Scheme;
  skos:prefLabel "Heart Rate";
  skos:related ble:org.bluetooth.characteristic.body_sensor_location, ble:org.bluetooth.characteristic.heart_rate_control_point,
    ble:org.bluetooth.characteristic.heart_rate_measurement;
  prov:wasDerivedFrom <file:/data/lp/etl/executor/data/1651932367716-22-f5b1c2e0-1947-4a2e-a814-6ce401f2a604/working/working-outputfiles-33/gatt-xml-master/org.bluetooth.service.heart_rate.xml> .

<http://purl.org/wot-catalogue/ble/gatt#org.bluetooth.characteristic.heart_rate_measurement>
  a skos:Concept, ontolex:LexicalConcept, prov:Entity;
  skos:altLabel "heart rate measurement";
  skos:broader ble:Characteristic;
  skos:inScheme ble:Scheme;
  skos:prefLabel "Heart Rate Measurement";
  skos:related ble:EnergyExpended, ble:Flags, <http://purl.org/wot-catalogue/ble#HeartRateMeasurementValue(uint16)>,
    <http://purl.org/wot-catalogue/ble#HeartRateMeasurementValue(uint8)>, ble:Notify,
    ble:RR-Interval;
  prov:wasDerivedFrom <file:/data/lp/etl/executor/data/1651932367716-22-f5b1c2e0-1947-4a2e-a814-6ce401f2a604/working/working-outputfiles-33/gatt-xml-master/org.bluetooth.characteristic.heart_rate_measurement.xml> .

<http://purl.org/wot-catalogue/ble/gatt#bcdHID> a skos:Concept, ontolex:LexicalConcept,
    prov:Entity;
  skos:altLabel "bcdhid";
  skos:broader ble:Value;
  skos:definition """16-bit unsigned integer representing version
      number of base USB HID Specification implemented by HID
      Device""";
  skos:inScheme ble:Scheme;
  skos:prefLabel "bcdHID";
  prov:wasDerivedFrom <file:/data/lp/etl/executor/data/1651932367716-22-f5b1c2e0-1947-4a2e-a814-6ce401f2a604/working/working-outputfiles-33/gatt-xml-master/org.bluetooth.characteristic.hid_information.xml> .

<http://purl.org/wot-catalogue/ble/gatt#bCountryCode> a skos:Concept, ontolex:LexicalConcept,
    prov:Entity;
  skos:altLabel "bcountrycode";
  skos:broader ble:Value;
  skos:definition """Identifies which country the hardware is
      localized for. Most hardware is not localized and thus this
      value would be zero (0).""";
  skos:inScheme ble:Scheme;
  skos:prefLabel "bCountryCode";
  prov:wasDerivedFrom <file:/data/lp/etl/executor/data/1651932367716-22-f5b1c2e0-1947-4a2e-a814-6ce401f2a604/working/working-outputfiles-33/gatt-xml-master/org.bluetooth.characteristic.hid_information.xml> .

<http://purl.org/wot-catalogue/ble/gatt#1801> a skos:Concept, ontolex:LexicalConcept,
    prov:Entity;
  skos:altLabel "generic attribute";
  skos:broader ble:Service;
  skos:inScheme ble:Scheme;
  skos:prefLabel "Generic Attribute";
  skos:related ble:org.bluetooth.characteristic.gatt.service_changed;
  prov:wasDerivedFrom <file:/data/lp/etl/executor/data/1651932367716-22-f5b1c2e0-1947-4a2e-a814-6ce401f2a604/working/working-outputfiles-33/gatt-xml-master/org.bluetooth.service.generic_attribute.xml> .

<http://purl.org/wot-catalogue/ble/gatt#181A> a skos:Concept, ontolex:LexicalConcept,
    prov:Entity;
  skos:altLabel "environmental sensing";
  skos:broader ble:Service;
  skos:definition """The Environmental Sensing Service (ESS) exposes
    measurement data from an environmental sensor intended for
    sports and fitness applications. A wide range of environmental
    parameters is supported.""";
  skos:inScheme ble:Scheme;
  skos:prefLabel "Environmental Sensing";
  skos:related ble:org.bluetooth.characteristic.apparent_wind_direction, ble:org.bluetooth.characteristic.apparent_wind_speed,
    ble:org.bluetooth.characteristic.barometric_pressure_trend, ble:org.bluetooth.characteristic.descriptor_value_changed,
    ble:org.bluetooth.characteristic.dew_point, ble:org.bluetooth.characteristic.elevation,
    ble:org.bluetooth.characteristic.gust_factor, ble:org.bluetooth.characteristic.heat_index,
    ble:org.bluetooth.characteristic.humidity, ble:org.bluetooth.characteristic.irradiance,
    ble:org.bluetooth.characteristic.magnetic_declination, ble:org.bluetooth.characteristic.magnetic_flux_density_2D,
    ble:org.bluetooth.characteristic.magnetic_flux_density_3D, ble:org.bluetooth.characteristic.pollen_concentration,
    ble:org.bluetooth.characteristic.pressure, ble:org.bluetooth.characteristic.rainfall,
    ble:org.bluetooth.characteristic.temperature, ble:org.bluetooth.characteristic.true_wind_direction,
    ble:org.bluetooth.characteristic.true_wind_speed, ble:org.bluetooth.characteristic.uv_index,
    ble:org.bluetooth.characteristic.wind_chill;
  prov:wasDerivedFrom <file:/data/lp/etl/executor/data/1651932367716-22-f5b1c2e0-1947-4a2e-a814-6ce401f2a604/working/working-outputfiles-33/gatt-xml-master/org.bluetooth.service.environmental_sensing.xml> .

<http://purl.org/wot-catalogue/ble/gatt#org.bluetooth.characteristic.true_wind_direction>
  a skos:Concept, ontolex:LexicalConcept, prov:Entity;
  skos:altLabel "true wind direction";
  skos:broader ble:Characteristic;
  skos:inScheme ble:Scheme;
  skos:prefLabel "True Wind Direction";
  skos:related ble:ExtendedProperties, ble:Notify, ble:Read, ble:TrueWindDirection,
    ble:WritableAuxiliaries;
  prov:wasDerivedFrom <file:/data/lp/etl/executor/data/1651932367716-22-f5b1c2e0-1947-4a2e-a814-6ce401f2a604/working/working-outputfiles-33/gatt-xml-master/org.bluetooth.characteristic.true_wind_direction.xml> .

<http://purl.org/wot-catalogue/ble/gatt#org.bluetooth.characteristic.barometric_pressure_trend>
  a skos:Concept, ontolex:LexicalConcept, prov:Entity;
  skos:altLabel "barometric pressure trend";
  skos:broader ble:Characteristic;
  skos:inScheme ble:Scheme;
  skos:prefLabel "Barometric Pressure Trend";
  skos:related ble:BarometricPressureTrend, ble:ExtendedProperties, ble:Notify, ble:Read,
    ble:WritableAuxiliaries;
  prov:wasDerivedFrom <file:/data/lp/etl/executor/data/1651932367716-22-f5b1c2e0-1947-4a2e-a814-6ce401f2a604/working/working-outputfiles-33/gatt-xml-master/org.bluetooth.characteristic.barometric_pressure_trend.xml> .

<http://purl.org/wot-catalogue/ble/gatt#HardwareRevision> a skos:Concept, ontolex:LexicalConcept,
    prov:Entity;
  skos:altLabel "hardware revision";
  skos:broader ble:Value;
  skos:definition "The Hardware Revision String characteristic shall represent the hardware revision for the hardware within the device.";
  skos:inScheme ble:Scheme;
  skos:prefLabel "Hardware Revision";
  skos:related ble:Read, xsd:string;
  prov:wasDerivedFrom <file:/data/lp/etl/executor/data/1651932367716-22-f5b1c2e0-1947-4a2e-a814-6ce401f2a604/working/working-outputfiles-33/gatt-xml-master/org.bluetooth.characteristic.hardware_revision_string.xml> .

<http://purl.org/wot-catalogue/ble/gatt#ObjectType> a skos:Concept, ontolex:LexicalConcept,
    prov:Entity;
  skos:altLabel "object type";
  skos:broader ble:Value;
  skos:definition """Refer to note below for 16-bit
      values""";
  skos:inScheme ble:Scheme;
  skos:prefLabel "Object Type";
  prov:wasDerivedFrom <file:/data/lp/etl/executor/data/1651932367716-22-f5b1c2e0-1947-4a2e-a814-6ce401f2a604/working/working-outputfiles-33/gatt-xml-master/org.bluetooth.characteristic.object_type.xml> .

<http://purl.org/wot-catalogue/ble/gatt#WeightScaleFeature> a skos:Concept, ontolex:LexicalConcept,
    prov:Entity;
  skos:altLabel "weight scale feature";
  skos:broader ble:Value;
  skos:inScheme ble:Scheme;
  skos:prefLabel "Weight Scale Feature";
  prov:wasDerivedFrom <file:/data/lp/etl/executor/data/1651932367716-22-f5b1c2e0-1947-4a2e-a814-6ce401f2a604/working/working-outputfiles-33/gatt-xml-master/org.bluetooth.characteristic.weight_scale_feature.xml> .

<http://purl.org/wot-catalogue/ble/gatt#MinimumPower> a skos:Concept, ontolex:LexicalConcept,
    prov:Entity;
  skos:altLabel "minimum power";
  skos:broader ble:Value;
  skos:definition """Watt with a resolution of
      1""";
  skos:inScheme ble:Scheme;
  skos:prefLabel "Minimum Power";
  prov:wasDerivedFrom <file:/data/lp/etl/executor/data/1651932367716-22-f5b1c2e0-1947-4a2e-a814-6ce401f2a604/working/working-outputfiles-33/gatt-xml-master/org.bluetooth.characteristic.supported_power_range.xml> .

<http://purl.org/wot-catalogue/ble/gatt#MaximumPower> a skos:Concept, ontolex:LexicalConcept,
    prov:Entity;
  skos:altLabel "maximum power";
  skos:broader ble:Value;
  skos:definition """Watt with a resolution of
      1""";
  skos:inScheme ble:Scheme;
  skos:prefLabel "Maximum Power";
  prov:wasDerivedFrom <file:/data/lp/etl/executor/data/1651932367716-22-f5b1c2e0-1947-4a2e-a814-6ce401f2a604/working/working-outputfiles-33/gatt-xml-master/org.bluetooth.characteristic.supported_power_range.xml> .

<http://purl.org/wot-catalogue/ble/gatt#ForceonBelt> a skos:Concept, ontolex:LexicalConcept,
    prov:Entity;
  skos:altLabel "force on belt";
  skos:broader ble:Value;
  skos:definition """Newton with a resolution of
      1""";
  skos:inScheme ble:Scheme;
  skos:prefLabel "Force on Belt";
  prov:wasDerivedFrom <file:/data/lp/etl/executor/data/1651932367716-22-f5b1c2e0-1947-4a2e-a814-6ce401f2a604/working/working-outputfiles-33/gatt-xml-master/org.bluetooth.characteristic.treadmill_data.xml> .

<http://purl.org/wot-catalogue/ble/gatt#PowerOutput> a skos:Concept, ontolex:LexicalConcept,
    prov:Entity;
  skos:altLabel "power output";
  skos:broader ble:Value;
  skos:definition """Watts with a resolution of
      1""";
  skos:inScheme ble:Scheme;
  skos:prefLabel "Power Output";
  prov:wasDerivedFrom <file:/data/lp/etl/executor/data/1651932367716-22-f5b1c2e0-1947-4a2e-a814-6ce401f2a604/working/working-outputfiles-33/gatt-xml-master/org.bluetooth.characteristic.treadmill_data.xml> .

<http://purl.org/wot-catalogue/ble/gatt#LocalEastCoordinate> a skos:Concept, ontolex:LexicalConcept,
    prov:Entity;
  skos:altLabel "local east coordinate";
  skos:broader ble:Value;
  skos:inScheme ble:Scheme;
  skos:prefLabel "Local East Coordinate";
  prov:wasDerivedFrom <file:/data/lp/etl/executor/data/1651932367716-22-f5b1c2e0-1947-4a2e-a814-6ce401f2a604/working/working-outputfiles-33/gatt-xml-master/org.bluetooth.characteristic.local_east_coordinate.xml> .

<http://purl.org/wot-catalogue/ble/gatt#StatusCode> a skos:Concept, ontolex:LexicalConcept,
    prov:Entity;
  skos:altLabel "status code";
  skos:broader ble:Value;
  skos:inScheme ble:Scheme;
  skos:prefLabel "Status Code";
  prov:wasDerivedFrom <file:/data/lp/etl/executor/data/1651932367716-22-f5b1c2e0-1947-4a2e-a814-6ce401f2a604/working/working-outputfiles-33/gatt-xml-master/org.bluetooth.characteristic.http_status_code.xml> .

<http://purl.org/wot-catalogue/ble/gatt#DataStatus> a skos:Concept, ontolex:LexicalConcept,
    prov:Entity;
  skos:altLabel "data status";
  skos:broader ble:Value;
  skos:inScheme ble:Scheme;
  skos:prefLabel "Data Status";
  prov:wasDerivedFrom <file:/data/lp/etl/executor/data/1651932367716-22-f5b1c2e0-1947-4a2e-a814-6ce401f2a604/working/working-outputfiles-33/gatt-xml-master/org.bluetooth.characteristic.http_status_code.xml> .

<http://purl.org/wot-catalogue/ble/gatt#Age> a skos:Concept, ontolex:LexicalConcept,
    prov:Entity;
  skos:altLabel "age";
  skos:broader ble:Value;
  skos:inScheme ble:Scheme;
  skos:prefLabel "Age";
  prov:wasDerivedFrom <file:/data/lp/etl/executor/data/1651932367716-22-f5b1c2e0-1947-4a2e-a814-6ce401f2a604/working/working-outputfiles-33/gatt-xml-master/org.bluetooth.characteristic.age.xml> .

<http://purl.org/wot-catalogue/ble/gatt#Location-Latitude> a skos:Concept, ontolex:LexicalConcept,
    prov:Entity;
  skos:altLabel "location - latitude";
  skos:broader ble:Value;
  skos:definition """Unit is in degrees with a resolution of
      1/(10^7) 
      C1: When present, these fields are always present as a
      pair.""";
  skos:inScheme ble:Scheme;
  skos:prefLabel "Location - Latitude";
  prov:wasDerivedFrom <file:/data/lp/etl/executor/data/1651932367716-22-f5b1c2e0-1947-4a2e-a814-6ce401f2a604/working/working-outputfiles-33/gatt-xml-master/org.bluetooth.characteristic.location_and_speed.xml> .

<http://purl.org/wot-catalogue/ble/gatt#Location-Longitude> a skos:Concept, ontolex:LexicalConcept,
    prov:Entity;
  skos:altLabel "location - longitude";
  skos:broader ble:Value;
  skos:definition """Unit is in degrees with a resolution of
      1/(10^7) 
      C1:When present, these fields are always present as a
      pair.""";
  skos:inScheme ble:Scheme;
  skos:prefLabel "Location - Longitude";
  prov:wasDerivedFrom <file:/data/lp/etl/executor/data/1651932367716-22-f5b1c2e0-1947-4a2e-a814-6ce401f2a604/working/working-outputfiles-33/gatt-xml-master/org.bluetooth.characteristic.location_and_speed.xml> .

<http://purl.org/wot-catalogue/ble/gatt#RollingTime> a skos:Concept, ontolex:LexicalConcept,
    prov:Entity;
  skos:altLabel "rolling time";
  skos:broader ble:Value;
  skos:definition """Unit is in seconds with a resolution of 1
      second""";
  skos:inScheme ble:Scheme;
  skos:prefLabel "Rolling Time";
  prov:wasDerivedFrom <file:/data/lp/etl/executor/data/1651932367716-22-f5b1c2e0-1947-4a2e-a814-6ce401f2a604/working/working-outputfiles-33/gatt-xml-master/org.bluetooth.characteristic.location_and_speed.xml> .

<http://purl.org/wot-catalogue/ble/gatt#UTCTime> a skos:Concept, ontolex:LexicalConcept,
    prov:Entity;
  skos:altLabel "utc time";
  skos:broader ble:Value;
  skos:definition "Smallest units in seconds";
  skos:inScheme ble:Scheme;
  skos:prefLabel "UTC Time";
  prov:wasDerivedFrom <file:/data/lp/etl/executor/data/1651932367716-22-f5b1c2e0-1947-4a2e-a814-6ce401f2a604/working/working-outputfiles-33/gatt-xml-master/org.bluetooth.characteristic.location_and_speed.xml> .

<http://purl.org/wot-catalogue/ble/gatt#org.bluetooth.characteristic.alert_category_id_bit_mask>
  a skos:Concept, ontolex:LexicalConcept, prov:Entity;
  skos:altLabel "alert category id bit mask";
  skos:broader ble:Characteristic;
  skos:definition """The value of the characteristic is a bit mask
    implemented as an array of unsigned 8 bit integers. The Alert
    Category ID Bit Mask characteristic defines one bit for each
    predefined category ID.""";
  skos:inScheme ble:Scheme;
  skos:prefLabel "Alert Category ID Bit Mask";
  skos:related ble:CategoryIDBitMask0, ble:CategoryIDBitMask1;
  prov:wasDerivedFrom <file:/data/lp/etl/executor/data/1651932367716-22-f5b1c2e0-1947-4a2e-a814-6ce401f2a604/working/working-outputfiles-33/gatt-xml-master/org.bluetooth.characteristic.alert_category_id_bit_mask.xml> .

<http://purl.org/wot-catalogue/ble/gatt#CategoryIDBitMask0> a skos:Concept, ontolex:LexicalConcept,
    prov:Entity;
  skos:altLabel "category id bit mask 0";
  skos:broader ble:Value;
  skos:inScheme ble:Scheme;
  skos:prefLabel "Category ID Bit Mask 0";
  prov:wasDerivedFrom <file:/data/lp/etl/executor/data/1651932367716-22-f5b1c2e0-1947-4a2e-a814-6ce401f2a604/working/working-outputfiles-33/gatt-xml-master/org.bluetooth.characteristic.alert_category_id_bit_mask.xml> .

<http://purl.org/wot-catalogue/ble/gatt#CategoryIDBitMask1> a skos:Concept, ontolex:LexicalConcept,
    prov:Entity;
  skos:altLabel "category id bit mask 1";
  skos:broader ble:Value;
  skos:inScheme ble:Scheme;
  skos:prefLabel "Category ID Bit Mask 1";
  prov:wasDerivedFrom <file:/data/lp/etl/executor/data/1651932367716-22-f5b1c2e0-1947-4a2e-a814-6ce401f2a604/working/working-outputfiles-33/gatt-xml-master/org.bluetooth.characteristic.alert_category_id_bit_mask.xml> .

<http://purl.org/wot-catalogue/ble/gatt#BloodPressureFeature> a skos:Concept, ontolex:LexicalConcept,
    prov:Entity;
  skos:altLabel "blood pressure feature";
  skos:broader ble:Value;
  skos:inScheme ble:Scheme;
  skos:prefLabel "Blood Pressure Feature";
  prov:wasDerivedFrom <file:/data/lp/etl/executor/data/1651932367716-22-f5b1c2e0-1947-4a2e-a814-6ce401f2a604/working/working-outputfiles-33/gatt-xml-master/org.bluetooth.characteristic.blood_pressure_feature.xml> .

<http://purl.org/wot-catalogue/ble/gatt#VendorIDSource> a skos:Concept, ontolex:LexicalConcept,
    prov:Entity;
  skos:altLabel "vendor id source";
  skos:broader ble:Value;
  skos:definition """Identifies the source of the Vendor ID
      field""";
  skos:inScheme ble:Scheme;
  skos:prefLabel "Vendor ID Source";
  prov:wasDerivedFrom <file:/data/lp/etl/executor/data/1651932367716-22-f5b1c2e0-1947-4a2e-a814-6ce401f2a604/working/working-outputfiles-33/gatt-xml-master/org.bluetooth.characteristic.pnp_id.xml> .

<http://purl.org/wot-catalogue/ble/gatt#VendorID> a skos:Concept, ontolex:LexicalConcept,
    prov:Entity;
  skos:altLabel "vendor id";
  skos:broader ble:Value;
  skos:definition """Identifies the product vendor from the
      namespace in the Vendor ID Source""";
  skos:inScheme ble:Scheme;
  skos:prefLabel "Vendor ID";
  prov:wasDerivedFrom <file:/data/lp/etl/executor/data/1651932367716-22-f5b1c2e0-1947-4a2e-a814-6ce401f2a604/working/working-outputfiles-33/gatt-xml-master/org.bluetooth.characteristic.pnp_id.xml> .

<http://purl.org/wot-catalogue/ble/gatt#ProductID> a skos:Concept, ontolex:LexicalConcept,
    prov:Entity;
  skos:altLabel "product id";
  skos:broader ble:Value;
  skos:definition """Manufacturer managed identifier for this
      product""";
  skos:inScheme ble:Scheme;
  skos:prefLabel "Product ID";
  prov:wasDerivedFrom <file:/data/lp/etl/executor/data/1651932367716-22-f5b1c2e0-1947-4a2e-a814-6ce401f2a604/working/working-outputfiles-33/gatt-xml-master/org.bluetooth.characteristic.pnp_id.xml> .

<http://purl.org/wot-catalogue/ble/gatt#ProductVersion> a skos:Concept, ontolex:LexicalConcept,
    prov:Entity;
  skos:altLabel "product version";
  skos:broader ble:Value;
  skos:definition """Manufacturer managed version for this
      product""";
  skos:inScheme ble:Scheme;
  skos:prefLabel "Product Version";
  prov:wasDerivedFrom <file:/data/lp/etl/executor/data/1651932367716-22-f5b1c2e0-1947-4a2e-a814-6ce401f2a604/working/working-outputfiles-33/gatt-xml-master/org.bluetooth.characteristic.pnp_id.xml> .

<http://purl.org/wot-catalogue/ble/gatt#AnaerobicThreshold> a skos:Concept, ontolex:LexicalConcept,
    prov:Entity;
  skos:altLabel "anaerobic threshold";
  skos:broader ble:Value;
  skos:definition """The Unit is beats per minute with a
      resolution of 1""";
  skos:inScheme ble:Scheme;
  skos:prefLabel "Anaerobic Threshold";
  prov:wasDerivedFrom <file:/data/lp/etl/executor/data/1651932367716-22-f5b1c2e0-1947-4a2e-a814-6ce401f2a604/working/working-outputfiles-33/gatt-xml-master/org.bluetooth.characteristic.anaerobic_threshold.xml> .

<http://purl.org/wot-catalogue/ble/gatt#Uncertainty> a skos:Concept, ontolex:LexicalConcept,
    prov:Entity;
  skos:altLabel "uncertainty";
  skos:broader ble:Value;
  skos:inScheme ble:Scheme;
  skos:prefLabel "Uncertainty";
  prov:wasDerivedFrom <file:/data/lp/etl/executor/data/1651932367716-22-f5b1c2e0-1947-4a2e-a814-6ce401f2a604/working/working-outputfiles-33/gatt-xml-master/org.bluetooth.characteristic.uncertainty.xml> .

<http://purl.org/wot-catalogue/ble/gatt#ObjectLast-Modified> a skos:Concept, ontolex:LexicalConcept,
    prov:Entity;
  skos:altLabel "object last-modified";
  skos:broader ble:Value;
  skos:inScheme ble:Scheme;
  skos:prefLabel "Object Last-Modified";
  prov:wasDerivedFrom <file:/data/lp/etl/executor/data/1651932367716-22-f5b1c2e0-1947-4a2e-a814-6ce401f2a604/working/working-outputfiles-33/gatt-xml-master/org.bluetooth.characteristic.object_last_modified.xml> .

<http://purl.org/wot-catalogue/ble/gatt#Size> a skos:Concept, ontolex:LexicalConcept,
    prov:Entity;
  skos:altLabel "size";
  skos:broader ble:Value;
  skos:definition """The Size Field represents the size of the
      CGM Measurement record. In minimum the size is 6 octets and
      is enlarged by more octets indicated by the Flags Field
      (Sensor Status Annunciation Field, CGM Trend Information
      Field and CGM Quality Field) and the E2E-CRC Supported bit in
      CGM Feature. The Size Field itself is included in the overall
      length calculation.""";
  skos:inScheme ble:Scheme;
  skos:prefLabel "Size";
  prov:wasDerivedFrom <file:/data/lp/etl/executor/data/1651932367716-22-f5b1c2e0-1947-4a2e-a814-6ce401f2a604/working/working-outputfiles-33/gatt-xml-master/org.bluetooth.characteristic.cgm_measurement.xml> .

<http://purl.org/wot-catalogue/ble/gatt#CGMGlucoseConcentration> a skos:Concept, ontolex:LexicalConcept,
    prov:Entity;
  skos:altLabel "cgm glucose concentration";
  skos:broader ble:Value;
  skos:definition """The CGM Glucose Concetration Field contains
      the CGM glucose concentration in mg/dL as a SFLOAT data type.
      The SFLOAT-Type is a 16-bit word comprising a signed 4-bit
      integer exponent followed by a signed 12-bit Mantissa, each
      in twos-complement form.""";
  skos:inScheme ble:Scheme;
  skos:prefLabel "CGM Glucose Concentration";
  prov:wasDerivedFrom <file:/data/lp/etl/executor/data/1651932367716-22-f5b1c2e0-1947-4a2e-a814-6ce401f2a604/working/working-outputfiles-33/gatt-xml-master/org.bluetooth.characteristic.cgm_measurement.xml> .

<http://purl.org/wot-catalogue/ble/gatt#CGMTrendInformation> a skos:Concept, ontolex:LexicalConcept,
    prov:Entity;
  skos:altLabel "cgm trend information";
  skos:broader ble:Value;
  skos:definition """The CGM Trend Information Field contains the
      CGM Trend information in (mg/dL)/min as an SFLOAT data type.
      This field is optional if the device supports CGM Trend
      information (Bit 15 in CGM Feature is set to 1) otherwise
      excluded.""";
  skos:inScheme ble:Scheme;
  skos:prefLabel "CGM Trend Information";
  prov:wasDerivedFrom <file:/data/lp/etl/executor/data/1651932367716-22-f5b1c2e0-1947-4a2e-a814-6ce401f2a604/working/working-outputfiles-33/gatt-xml-master/org.bluetooth.characteristic.cgm_measurement.xml> .

<http://purl.org/wot-catalogue/ble/gatt#CGMQuality> a skos:Concept, ontolex:LexicalConcept,
    prov:Entity;
  skos:altLabel "cgm quality";
  skos:broader ble:Value;
  skos:definition """This field contains the CGM Quality
      information in % as an SFLOAT data type. The SFLOAT-Type is a
      16-bit word comprising a signed 4-bit integer exponent
      followed by a signed 12-bit Mantissa, each in twos-complement
      form. This field is optional if the device supports CGM
      Quality (Bit 16 in CGM Feature is set to 1) otherwise
      excluded.""";
  skos:inScheme ble:Scheme;
  skos:prefLabel "CGM Quality";
  prov:wasDerivedFrom <file:/data/lp/etl/executor/data/1651932367716-22-f5b1c2e0-1947-4a2e-a814-6ce401f2a604/working/working-outputfiles-33/gatt-xml-master/org.bluetooth.characteristic.cgm_measurement.xml> .

<http://purl.org/wot-catalogue/ble/gatt#1811> a skos:Concept, ontolex:LexicalConcept,
    prov:Entity;
  skos:altLabel "alert notification service";
  skos:broader ble:Service;
  skos:definition """The Alert Notification service exposes alert
    information in a device. This information includes the
    following: 
    - Type of alert occuring in a device.- Additional text information such as caller ID or sender
    ID- Count of new alerts.- Count of unread alert items.""";
  skos:inScheme ble:Scheme;
  skos:prefLabel "Alert Notification Service";
  skos:related ble:org.bluetooth.characteristic.alert_notification_control_point, ble:org.bluetooth.characteristic.new_alert,
    ble:org.bluetooth.characteristic.supported_new_alert_category, ble:org.bluetooth.characteristic.supported_unread_alert_category,
    ble:org.bluetooth.characteristic.unread_alert_status;
  prov:wasDerivedFrom <file:/data/lp/etl/executor/data/1651932367716-22-f5b1c2e0-1947-4a2e-a814-6ce401f2a604/working/working-outputfiles-33/gatt-xml-master/org.bluetooth.service.alert_notification.xml> .

<http://purl.org/wot-catalogue/ble/gatt#FatBurnHeartRateUpperLimit> a skos:Concept,
    ontolex:LexicalConcept, prov:Entity;
  skos:altLabel "fat burn heart rate upper limit";
  skos:broader ble:Value;
  skos:definition """Unit is in beats per minute with a
      resolution of 1""";
  skos:inScheme ble:Scheme;
  skos:prefLabel "Fat Burn Heart Rate Upper Limit";
  prov:wasDerivedFrom <file:/data/lp/etl/executor/data/1651932367716-22-f5b1c2e0-1947-4a2e-a814-6ce401f2a604/working/working-outputfiles-33/gatt-xml-master/org.bluetooth.characteristic.fat_burn_heart_rate_upper_limit.xml> .

<http://purl.org/wot-catalogue/ble/gatt#IndoorPositioningConfiguration> a skos:Concept,
    ontolex:LexicalConcept, prov:Entity;
  skos:altLabel "indoor positioning configuration";
  skos:broader ble:Value;
  skos:inScheme ble:Scheme;
  skos:prefLabel "Indoor Positioning Configuration";
  prov:wasDerivedFrom <file:/data/lp/etl/executor/data/1651932367716-22-f5b1c2e0-1947-4a2e-a814-6ce401f2a604/working/working-outputfiles-33/gatt-xml-master/org.bluetooth.characteristic.indoor_positioning_configuration.xml> .

<http://purl.org/wot-catalogue/ble/gatt#SerialNumber> a skos:Concept, ontolex:LexicalConcept,
    prov:Entity;
  skos:altLabel "serial number";
  skos:broader ble:Value;
  skos:definition "The Serial Number String characteristic shall represent the serial number for a particular instance of the device.";
  skos:inScheme ble:Scheme;
  skos:prefLabel "Serial Number";
  skos:related ble:Read, xsd:string;
  prov:wasDerivedFrom <file:/data/lp/etl/executor/data/1651932367716-22-f5b1c2e0-1947-4a2e-a814-6ce401f2a604/working/working-outputfiles-33/gatt-xml-master/org.bluetooth.characteristic.serial_number_string.xml> .

<http://purl.org/wot-catalogue/ble/gatt#FloorNumber> a skos:Concept, ontolex:LexicalConcept,
    prov:Entity;
  skos:altLabel "floor number";
  skos:broader ble:Value;
  skos:inScheme ble:Scheme;
  skos:prefLabel "Floor Number";
  prov:wasDerivedFrom <file:/data/lp/etl/executor/data/1651932367716-22-f5b1c2e0-1947-4a2e-a814-6ce401f2a604/working/working-outputfiles-33/gatt-xml-master/org.bluetooth.characteristic.floor_number.xml> .

<http://purl.org/wot-catalogue/ble/gatt#HeartRateMeasurementValue(uint8)> a skos:Concept,
    ontolex:LexicalConcept, prov:Entity;
  skos:altLabel "heart rate measurement value (uint8)";
  skos:broader ble:Value;
  skos:definition """Note: The format of the Heart Rate
      Measurement Value field is dependent upon bit 0 of the Flags
      field.""";
  skos:inScheme ble:Scheme;
  skos:prefLabel "Heart Rate Measurement Value (uint8)";
  prov:wasDerivedFrom <file:/data/lp/etl/executor/data/1651932367716-22-f5b1c2e0-1947-4a2e-a814-6ce401f2a604/working/working-outputfiles-33/gatt-xml-master/org.bluetooth.characteristic.heart_rate_measurement.xml> .

<http://purl.org/wot-catalogue/ble/gatt#HeartRateMeasurementValue(uint16)> a skos:Concept,
    ontolex:LexicalConcept, prov:Entity;
  skos:altLabel "heart rate measurement value (uint16)";
  skos:broader ble:Value;
  skos:definition """Note: The format of the Heart Rate
      Measurement Value field is dependent upon bit 0 of the Flags
      field.""";
  skos:inScheme ble:Scheme;
  skos:prefLabel "Heart Rate Measurement Value (uint16)";
  prov:wasDerivedFrom <file:/data/lp/etl/executor/data/1651932367716-22-f5b1c2e0-1947-4a2e-a814-6ce401f2a604/working/working-outputfiles-33/gatt-xml-master/org.bluetooth.characteristic.heart_rate_measurement.xml> .

<http://purl.org/wot-catalogue/ble/gatt#EnergyExpended> a skos:Concept, ontolex:LexicalConcept,
    prov:Entity;
  skos:altLabel "energy expended";
  skos:broader ble:Value;
  skos:definition """The presence of the Energy Expended field is
      dependent upon bit 3 of the Flags field.""";
  skos:inScheme ble:Scheme;
  skos:prefLabel "Energy Expended";
  prov:wasDerivedFrom <file:/data/lp/etl/executor/data/1651932367716-22-f5b1c2e0-1947-4a2e-a814-6ce401f2a604/working/working-outputfiles-33/gatt-xml-master/org.bluetooth.characteristic.heart_rate_measurement.xml> .

<http://purl.org/wot-catalogue/ble/gatt#RR-Interval> a skos:Concept, ontolex:LexicalConcept,
    prov:Entity;
  skos:altLabel "rr-interval";
  skos:broader ble:Value;
  skos:inScheme ble:Scheme;
  skos:prefLabel "RR-Interval";
  prov:wasDerivedFrom <file:/data/lp/etl/executor/data/1651932367716-22-f5b1c2e0-1947-4a2e-a814-6ce401f2a604/working/working-outputfiles-33/gatt-xml-master/org.bluetooth.characteristic.heart_rate_measurement.xml> .

<http://purl.org/wot-catalogue/ble/gatt#org.bluetooth.characteristic.exact_time_256>
  a skos:Concept, ontolex:LexicalConcept, prov:Entity;
  skos:altLabel "exact time 256";
  skos:broader ble:Characteristic;
  skos:inScheme ble:Scheme;
  skos:prefLabel "Exact Time 256";
  skos:related ble:DayDateTime, ble:Fractions256;
  prov:wasDerivedFrom <file:/data/lp/etl/executor/data/1651932367716-22-f5b1c2e0-1947-4a2e-a814-6ce401f2a604/working/working-outputfiles-33/gatt-xml-master/org.bluetooth.characteristic.exact_time_256.xml> .

<http://purl.org/wot-catalogue/ble/gatt#DayDateTime> a skos:Concept, ontolex:LexicalConcept,
    prov:Entity;
  skos:altLabel "day date time";
  skos:broader ble:Value;
  skos:definition """Reference the Time
      Characteristic""";
  skos:inScheme ble:Scheme;
  skos:prefLabel "Day Date Time";
  prov:wasDerivedFrom <file:/data/lp/etl/executor/data/1651932367716-22-f5b1c2e0-1947-4a2e-a814-6ce401f2a604/working/working-outputfiles-33/gatt-xml-master/org.bluetooth.characteristic.exact_time_256.xml> .

<http://purl.org/wot-catalogue/ble/gatt#Fractions256> a skos:Concept, ontolex:LexicalConcept,
    prov:Entity;
  skos:altLabel "fractions256";
  skos:broader ble:Value;
  skos:definition "1/256th of a second";
  skos:inScheme ble:Scheme;
  skos:prefLabel "Fractions256";
  prov:wasDerivedFrom <file:/data/lp/etl/executor/data/1651932367716-22-f5b1c2e0-1947-4a2e-a814-6ce401f2a604/working/working-outputfiles-33/gatt-xml-master/org.bluetooth.characteristic.exact_time_256.xml> .

<http://purl.org/wot-catalogue/ble/gatt#BondManagementFeatures> a skos:Concept, ontolex:LexicalConcept,
    prov:Entity;
  skos:altLabel "bond management features";
  skos:broader ble:Value;
  skos:definition "Byte Order - LSO...MSO";
  skos:inScheme ble:Scheme;
  skos:prefLabel "Bond Management Features";
  prov:wasDerivedFrom <file:/data/lp/etl/executor/data/1651932367716-22-f5b1c2e0-1947-4a2e-a814-6ce401f2a604/working/working-outputfiles-33/gatt-xml-master/org.bluetooth.characteristic.bond_management_feature.xml> .

<http://purl.org/wot-catalogue/ble/gatt#BarometricPressureTrend> a skos:Concept, ontolex:LexicalConcept,
    prov:Entity;
  skos:altLabel "barometric pressure trend";
  skos:broader ble:Value;
  skos:inScheme ble:Scheme;
  skos:prefLabel "Barometric Pressure Trend";
  prov:wasDerivedFrom <file:/data/lp/etl/executor/data/1651932367716-22-f5b1c2e0-1947-4a2e-a814-6ce401f2a604/working/working-outputfiles-33/gatt-xml-master/org.bluetooth.characteristic.barometric_pressure_trend.xml> .

<http://purl.org/wot-catalogue/ble/gatt#TrueWindDirection> a skos:Concept, ontolex:LexicalConcept,
    prov:Entity;
  skos:altLabel "true wind direction";
  skos:broader ble:Value;
  skos:definition """Unit is in degrees with a resolution of 0.01
      degrees""";
  skos:inScheme ble:Scheme;
  skos:prefLabel "True Wind Direction";
  prov:wasDerivedFrom <file:/data/lp/etl/executor/data/1651932367716-22-f5b1c2e0-1947-4a2e-a814-6ce401f2a604/working/working-outputfiles-33/gatt-xml-master/org.bluetooth.characteristic.true_wind_direction.xml> .

<http://purl.org/wot-catalogue/ble/gatt#WritewithoutResponse> a skos:Concept;
  skos:altLabel "write without response";
  skos:definition "A Characteristic Value is writen to a server when the client knows the Characteristic Value Handle and the client does not need an acknowledgment that the write was successfully performed";
  skos:inScheme ble:Scheme;
  skos:prefLabel "Write without Response" .

<http://purl.org/wot-catalogue/ble/gatt#ReadLong> a skos:Concept;
  skos:altLabel "read long";
  skos:definition "Characteristic Value is read from a server when the client knows the Characteristic Value Handle and the length of the Characteristic Value is longer than can be sent in a single Read Response Attribute protocol message.";
  skos:inScheme ble:Scheme;
  skos:prefLabel "Read Long" .

<http://purl.org/wot-catalogue/ble/gatt#DeviceInformationService> a skos:Concept;
  rdfs:seeAlso <https://www.bluetooth.org/docman/handlers/downloaddoc.ashx?doc_id=244369>;
  owl:versionInfo "1.1";
  skos:altLabel "device information service.";
  skos:definition "The Device Information Service exposes manufacturer and/or vendor information about a device.";
  skos:inScheme ble:Scheme;
  skos:prefLabel "Device Information Service.";
  skos:related ble:FirmwareRevision, ble:HardwareRevision, ble:IEEE11073-20601RegulatoryCertificationDataList,
    ble:ManufacturerName, ble:ModelNumber, ble:PnPID, ble:SerialNumber, ble:SoftwareRevision,
    ble:SystemID .

<http://purl.org/wot-catalogue/ble/gatt#SystemID> a skos:Concept;
  skos:altLabel "system id";
  skos:definition "The System ID characteristic shall represent a structure containing an Organizationally Unique Identifier (OUI) followed by a manufacturer-defined identifier and is unique for each individual instance of the product";
  skos:inScheme ble:Scheme;
  skos:prefLabel "System ID";
  skos:related ble:ManufacturerIdentifier, ble:OrganizationallyUniqueIdentifier, ble:Read .

<http://purl.org/wot-catalogue/ble/gatt#IEEE11073-20601RegulatoryCertificationDataList>
  a skos:Concept;
  skos:altLabel "institute of electrical and electronics engineers (ieee) 11073-20601 regulatory certification data list";
  skos:definition "The IEEE 11073-20601 Regulatory Certification Data List characteristic shall represent regulatory and certification information for the product in a list defined in IEEE 11073-20601";
  skos:inScheme ble:Scheme;
  skos:prefLabel "Institute of Electrical and Electronics Engineers (IEEE) 11073-20601 Regulatory Certification Data List";
  skos:related ble:Read, xsd:string .

<http://purl.org/wot-catalogue/ble/gatt#PnPID> a skos:Concept;
  skos:altLabel "plug and play identification";
  skos:definition "The PnP_ID characteristic is a set of values that shall be used to create a device ID value that is unique for this device. Included in the characteristic are a Vendor ID source field, a Vendor ID field, a Product ID field, and a Product Version field";
  skos:inScheme ble:Scheme;
  skos:prefLabel "Plug and Play Identification";
  skos:related ble:ProductIDField, ble:ProductVersionField, ble:Read, ble:VendorIDField,
    ble:VendorIDSourceField .

<http://purl.org/wot-catalogue/ble/gatt#BondManagementService> a skos:Concept;
  rdfs:seeAlso <https://www.bluetooth.org/docman/handlers/downloaddoc.ashx?doc_id=293524>;
  owl:versionInfo "1.0";
  skos:altLabel "bond management service";
  skos:definition "This Specification proposes that this service will enable users to manage their bonds on devices with a limited user interface.";
  skos:inScheme ble:Scheme;
  skos:prefLabel "Bond Management Service";
  skos:related ble:BondManagementControlPoint, ble:BondManagementFeature .

<http://purl.org/wot-catalogue/ble/gatt#BondManagementControlPoint> a skos:Concept;
  skos:altLabel "bond management control point";
  skos:definition "The Server shall evaluate a GATT Characteristic Value Write procedure or a GATT Characteristic Value Reliable Write procedure to the Bond Management Control";
  skos:inScheme ble:Scheme;
  skos:prefLabel "Bond Management Control Point";
  skos:related ble:Write .

<http://purl.org/wot-catalogue/ble/gatt#BondManagementFeature> a skos:Concept;
  skos:altLabel "bond management feature";
  skos:definition "The Bond Management Feature characteristic shall be used to indicate the supported features of the server.";
  skos:inScheme ble:Scheme;
  skos:prefLabel "Bond Management Feature";
  skos:related ble:Read .

<http://purl.org/wot-catalogue/ble/gatt#BatteryService> a skos:Concept;
  rdfs:seeAlso <https://www.bluetooth.org/docman/handlers/downloaddoc.ashx?doc_id=245138>;
  owl:versionInfo "1.0";
  skos:altLabel "battery service";
  skos:definition "The Battery Service exposes the Battery Level of a single battery or set of batteries in a device.";
  skos:inScheme ble:Scheme;
  skos:prefLabel "Battery Service";
  skos:related ble:BatteryLevel .

<http://purl.org/wot-catalogue/ble/gatt#BatteryLevel> a skos:Concept;
  skos:altLabel "battery level";
  skos:definition "The Battery Level characteristic is read using the GATT Read Characteristic Value subprocedure and returns the current battery level as a percentage.";
  skos:inScheme ble:Scheme;
  skos:prefLabel "Battery Level";
  skos:related ble:Notify, ble:Read, xsd:unsignedByte .

<http://purl.org/wot-catalogue/ble/gatt#CurrentTimeService> a skos:Concept;
  rdfs:seeAlso <https://www.bluetooth.org/docman/handlers/downloaddoc.ashx?doc_id=292957>;
  owl:versionInfo "1.1";
  skos:altLabel "current time service";
  skos:definition "This service defines how a Bluetooth device can expose date and time information to other Bluetooth devices.";
  skos:inScheme ble:Scheme;
  skos:prefLabel "Current Time Service";
  skos:related ble:CurrentTime, ble:LocalTimeInformation, ble:ReferenceTimeInformation .

<http://purl.org/wot-catalogue/ble/gatt#CurrentTime> a skos:Concept;
  skos:altLabel "current time";
  skos:definition "The Current Time characteristic returns the current date and time in the server device.";
  skos:inScheme ble:Scheme;
  skos:prefLabel "Current Time";
  skos:related ble:Notify, ble:Read, ble:Write .

<http://purl.org/wot-catalogue/ble/gatt#LocalTimeInformation> a skos:Concept;
  skos:altLabel "local time information";
  skos:definition "The Local Time Information characteristic returns the local time information that includes time zone and DST offset.";
  skos:inScheme ble:Scheme;
  skos:prefLabel "Local Time Information";
  skos:related ble:Read, ble:Write .

<http://purl.org/wot-catalogue/ble/gatt#ReferenceTimeInformation> a skos:Concept;
  skos:altLabel "reference time information";
  skos:definition "The Reference Time Information characteristic returns the information about the reference time source.";
  skos:inScheme ble:Scheme;
  skos:prefLabel "Reference Time Information";
  skos:related ble:Read .

<http://purl.org/wot-catalogue/ble/gatt#ScanParametersService> a skos:Concept;
  rdfs:seeAlso <https://www.bluetooth.org/docman/handlers/downloaddoc.ashx?doc_id=245143>;
  owl:versionInfo "1.0";
  skos:altLabel "scan parameters service";
  skos:definition "The Scan Parameters Service enables a GATT Server device to expose a characteristic for the GATT Client to write its scan interval and scan window on the GATT Server device, and enables a GATT Server to request a refresh of the GATT Client scan interval and scan window.";
  skos:inScheme ble:Scheme;
  skos:prefLabel "Scan Parameters Service";
  skos:related ble:ScanIntervalWindow, ble:ScanRefresh .

<http://purl.org/wot-catalogue/ble/gatt#ScanIntervalWindow> a skos:Concept;
  skos:altLabel "scan interval window";
  skos:definition "The Scan Interval Window characteristic is used to store the scan parameters of the Client.";
  skos:inScheme ble:Scheme;
  skos:prefLabel "Scan Interval Window";
  skos:related ble:LE_Scan_Interval, ble:LE_Scan_Window, ble:WritewithoutResponse .

<http://purl.org/wot-catalogue/ble/gatt#ScanRefresh> a skos:Concept;
  skos:altLabel "scan refresh";
  skos:definition "The Scan Refresh characteristic is used to notify the Client that the Server requires the Scan Interval Window characteristic to be written with the latest values upon notification.";
  skos:inScheme ble:Scheme;
  skos:prefLabel "Scan Refresh";
  skos:related ble:Notify, ble:Serverrequiresrefresh .

<http://purl.org/wot-catalogue/ble/gatt#UserDataService> a skos:Concept;
  rdfs:comment "This allows remote access and update of user data by a Client as well as the synchronization of user data between a Server and a Client.";
  rdfs:seeAlso <https://www.bluetooth.org/docman/handlers/downloaddoc.ashx?doc_id=288352>;
  owl:versionInfo "1.0";
  skos:altLabel "user data service";
  skos:definition "The User Data Service (UDS) exposes user-related data in the sports and fitness environment.";
  skos:inScheme ble:Scheme;
  skos:prefLabel "User Data Service";
  skos:related ble:DatabaseChangeIncrement, ble:UDSCharacteristic, ble:UserControlPoint,
    ble:UserIndex .

<http://purl.org/wot-catalogue/ble/gatt#UDSCharacteristic> a skos:Concept;
  skos:altLabel "user data service characteristic";
  skos:definition "Each UDS Characteristic is defined in the User Data Service Characteristics table";
  skos:inScheme ble:Scheme;
  skos:prefLabel "User Data Service Characteristic";
  skos:related ble:Read, ble:UDSCharacteristicValue, ble:Write .

<http://purl.org/wot-catalogue/ble/gatt#UserControlPoint> a skos:Concept;
  skos:altLabel "user control point";
  skos:definition "The User Control Point characteristic is used to request a specific function to be executed on the receiving device.";
  skos:inScheme ble:Scheme;
  skos:prefLabel "User Control Point";
  skos:related ble:Indicate, ble:Write .

<http://purl.org/wot-catalogue/ble/gatt#RecordAccessControlPoint> a skos:Concept;
  skos:altLabel "record access control point";
  skos:definition "The Record Access Control Point shall be used to control notifications and other data operations.";
  skos:inScheme ble:Scheme;
  skos:prefLabel "Record Access Control Point";
  skos:related ble:Indicate, ble:Write .

<http://purl.org/wot-catalogue/ble/gatt#SCControlPoint> a skos:Concept;
  skos:altLabel "speed and cadence control point";
  skos:definition "The SC Control Point is used by a Client to control certain behaviors of the Server.";
  skos:inScheme ble:Scheme;
  skos:prefLabel "Speed and Cadence Control Point" .

<http://purl.org/wot-catalogue/ble/gatt#ImmediateAlertService> a skos:Concept;
  rdfs:seeAlso <https://www.bluetooth.org/docman/handlers/downloaddoc.ashx?doc_id=239390>;
  owl:versionInfo "1.0";
  skos:altLabel "immediate alert service";
  skos:definition "This service exposes a control point to allow a peer device to cause the device to immediately alert.";
  skos:inScheme ble:Scheme;
  skos:prefLabel "Immediate Alert Service";
  skos:related ble:AlertLevel .

<http://purl.org/wot-catalogue/ble/gatt#VendorIDSourceField> a skos:Concept;
  skos:altLabel "vendor id source field";
  skos:definition "The Vendor ID Source field designates which organization assigned the value used in the Vendor ID field value.";
  skos:inScheme ble:Scheme;
  skos:narrower ble:BluetoothSIG, ble:USBImplementerForum;
  skos:prefLabel "Vendor ID Source Field" .

<http://purl.org/wot-catalogue/ble/gatt#VendorIDField> a skos:Concept;
  skos:altLabel "vendor id field";
  skos:definition "The Vendor ID field is intended to uniquely identify the vendor of the device.";
  skos:inScheme ble:Scheme;
  skos:prefLabel "Vendor ID Field";
  skos:related xsd:unsignedShort .

<http://purl.org/wot-catalogue/ble/gatt#ProductIDField> a skos:Concept;
  skos:altLabel "product id field";
  skos:definition "The Product ID field is intended to distinguish between different products made by the vendor identified with the Vendor ID field.";
  skos:inScheme ble:Scheme;
  skos:prefLabel "Product ID Field";
  skos:related xsd:unsignedShort .

<http://purl.org/wot-catalogue/ble/gatt#ProductVersionField> a skos:Concept;
  skos:altLabel "product version field";
  skos:definition "The Product Version field is a numeric expression identifying the device release number in Binary-Coded Decimal.";
  skos:inScheme ble:Scheme;
  skos:prefLabel "Product Version Field";
  skos:related xsd:unsignedShort .

<http://purl.org/wot-catalogue/ble/gatt#BluetoothSIG> a skos:Concept;
  skos:altLabel "bluetooth special interest group";
  skos:definition "Bluetooth SIG- assigned Device ID Vendor ID value from the Assigned Numbers document.";
  skos:inScheme ble:Scheme;
  skos:prefLabel "Bluetooth Special Interest Group";
  skos:related xsd:unsignedByte .

<http://purl.org/wot-catalogue/ble/gatt#USBImplementerForum> a skos:Concept;
  skos:altLabel "usb implementers forum";
  skos:definition "USB Implementers Forum assigned Vendor ID value.";
  skos:inScheme ble:Scheme;
  skos:prefLabel "USB Implementers Forum";
  skos:related xsd:unsignedByte .

<http://purl.org/wot-catalogue/ble/gatt#Serverrequiresrefresh> a skos:Concept;
  skos:altLabel "server requires refresh";
  skos:definition "Scan Refresh characteristic value  is a single octet.";
  skos:inScheme ble:Scheme;
  skos:prefLabel "Server requires refresh";
  skos:related xsd:unsignedByte .

<http://purl.org/wot-catalogue/ble/gatt#UDSCharacteristicValue> a skos:Concept;
  skos:altLabel "user data service characteristic value";
  skos:definition "A UDS Characteristic returns its associated characteristic value when read.";
  skos:inScheme ble:Scheme;
  skos:prefLabel "User Data Service Characteristic Value" .

<http://purl.org/wot-catalogue/ble/gatt#DatabaseChangeIncrementValue> a skos:Concept;
  skos:altLabel "database change increment value";
  skos:definition "When read or notified, the Database Change Increment characteristic returns a value that is used by a Client to determine whether or not the UDS Characteristics need to be synchronized between the Server and the Client.";
  skos:inScheme ble:Scheme;
  skos:prefLabel "Database Change Increment Value";
  skos:related xsd:unsignedInt .

<http://purl.org/wot-catalogue/ble/gatt#TimeStampField> a skos:Concept;
  skos:altLabel "time stamp field";
  skos:definition "The value of the Time Stamp field is derived from a source of date and time at the time of measurement.";
  skos:inScheme ble:Scheme;
  skos:prefLabel "Time Stamp Field" .

<http://purl.org/wot-catalogue/ble/gatt#UserIDField> a skos:Concept;
  skos:altLabel "user id field";
  skos:definition "The User ID field shall be included in the characteristic if the device supports the Multiple Users feature.";
  skos:inScheme ble:Scheme;
  skos:prefLabel "User ID Field";
  skos:related xsd:unsignedByte .

<http://purl.org/wot-catalogue/ble/gatt#InstantaneousPowerField> a skos:Concept;
  skos:altLabel "instantaneous power field";
  skos:definition "The Instantaneous Power field represents the value of the instantaneous power measured by the Server.";
  skos:inScheme ble:Scheme;
  skos:prefLabel "Instantaneous Power Field";
  skos:related xsd:short .

<http://purl.org/wot-catalogue/ble/gatt#InstantaneousSpeedField> a skos:Concept;
  skos:altLabel "instantaneous speed field";
  skos:definition "The Instantaneous Speed field represents the instantaneous value of the speed measured by the sensor.";
  skos:inScheme ble:Scheme;
  skos:prefLabel "Instantaneous Speed Field";
  skos:related xsd:unsignedShort .
