@prefix : <http://purl.org/wot-catalogue/openhab#> .
@prefix skos: <http://www.w3.org/2004/02/skos/core#> .
@prefix rdfs: <http://www.w3.org/2000/01/rdf-schema#> .

:scheme a skos:ConceptScheme ;
    rdfs:seeAlso <https://www.openhab.org/docs/tutorial/model.html> .

:Location a skos:Concept ;
    skos:prefLabel "Location" ;
    skos:definition "A Location is a Group Item that can contain sub-Locations, Equipment, and Points, and represents a physical location (building, room, etc.)."@en ;
    skos:related :Equipment, :Point ;
    skos:inScheme :scheme .

:Equipment a skos:Concept ;
    skos:prefLabel "Equipment" ;
    skos:definition "An Equipment is normally a Group Item that can contain sub-Equipment, and Points."@en ;
    skos:related :Point ;
    skos:inScheme :scheme .

:Point a skos:Concept ;
    skos:prefLabel "Point" ;
    skos:definition "A Point is not a Group, but represents any other type of Item and is usually linked to a Channel."@en ;
    skos:related :Property ;
    skos:inScheme :scheme .

:Property a skos:Concept ;
    skos:prefLabel "Property" ;
    skos:definition "A Property is an additional tag on a Point Item that indicates what sort of point it is. For example, a thermometer might be a Point of type Measurement with a Property of type Temperature."@en ;
    skos:inScheme :scheme .