@prefix haim: <http://purl.org/wot-catalogue/onem2m/haim#> .
@prefix onem2m: <http://purl.org/wot-catalogue/onem2m#> .
@prefix ontolex: <http://www.w3.org/ns/lemon/ontolex#> .
@prefix prov: <http://www.w3.org/ns/prov#> .
@prefix skos: <http://www.w3.org/2004/02/skos/core#> .

haim:collection skos:member haim:absoluteEnergyConsumption,
        haim:absoluteStartTime,
        haim:absoluteStopTime,
        haim:acousticSensor,
        haim:acousticStatus,
        haim:activateClockTimer,
        haim:adfStates,
        haim:airConJobMode,
        haim:airFlow,
        haim:airPurifierJobMode,
        haim:airQualitySensor,
        haim:alarm,
        haim:alarmSpeaker,
        haim:alarmStatus,
        haim:altitude,
        haim:answer,
        haim:audioVolume,
        haim:autoDocumentFeeder,
        haim:automode,
        haim:availableChannels,
        haim:basalMetabolism,
        haim:bath,
        haim:battery,
        haim:batteryThreshold,
        haim:binaryObject,
        haim:binarySwitch,
        haim:bioElectricalImpedanceAnalysis,
        haim:blue,
        haim:bmi,
        haim:bodyCompositionAnalyser,
        haim:bodyLength,
        haim:boiler,
        haim:bone,
        haim:brewing,
        haim:brightness,
        haim:call,
        haim:callState,
        haim:callerID,
        haim:capacity,
        haim:ch2o,
        haim:channelId,
        haim:channelName,
        haim:charging,
        haim:chargingCapacity,
        haim:clock,
        haim:close,
        haim:clothesDryerJobMode,
        haim:clothesWasherDryerJobMode,
        haim:clothesWasherJobMode,
        haim:clothesWasherJobModeOption,
        haim:co,
        haim:co2,
        haim:coarseness,
        haim:code,
        haim:coldWash,
        haim:colour,
        haim:colourSaturation,
        haim:concentration,
        haim:contextCarbohydratesAmount,
        haim:contextCarbohydratesSource,
        haim:contextExercise,
        haim:contextHealth,
        haim:contextLocation,
        haim:contextMeal,
        haim:contextMedication,
        haim:contextTester,
        haim:cookerHoodJobMode,
        haim:credentials,
        haim:cupsNumber,
        haim:current,
        haim:currentAdfState,
        haim:currentDate,
        haim:currentJobMode,
        haim:currentJobModeName,
        haim:currentJobState,
        haim:currentMachineState,
        haim:currentPlayerMode,
        haim:currentPlayerModeName,
        haim:currentSecurityMode,
        haim:currentTemperature,
        haim:currentTime,
        haim:currentTimeZone,
        haim:currentValue,
        haim:deactivateClockTimer,
        haim:decrementNumberValue,
        haim:defaultValue,
        haim:defrost,
        haim:dehumidifierJobMode,
        haim:description,
        haim:desiredHumidity,
        haim:detectedTime,
        haim:deviceAirConditioner,
        haim:deviceAirPurifier,
        haim:deviceAirQualityMonitor,
        haim:deviceAudioReceiver,
        haim:deviceBloodPressureMonitor,
        haim:deviceCamera,
        haim:deviceClothesDryer,
        haim:deviceClothesWasher,
        haim:deviceClothesWasherDryer,
        haim:deviceCoffeeMachine,
        haim:deviceCookerHood,
        haim:deviceCooktop,
        haim:deviceDehumidifier,
        haim:deviceDishWasher,
        haim:deviceDoor,
        haim:deviceDoorLock,
        haim:deviceElectricVehicleCharger,
        haim:deviceFan,
        haim:deviceFoodProbe,
        haim:deviceFreezer,
        haim:deviceGlucosemeter,
        haim:deviceHeartRateMonitor,
        haim:deviceHomeCCTV,
        haim:deviceHumidifier,
        haim:deviceKettle,
        haim:deviceLight,
        haim:deviceMicrogeneration,
        haim:deviceMultiFunctionPrinter,
        haim:deviceOutdoorLamp,
        haim:deviceOven,
        haim:devicePrinter,
        haim:devicePulseOximeter,
        haim:deviceRefrigerator,
        haim:deviceRobotCleaner,
        haim:deviceScanner,
        haim:deviceSecurityPanel,
        haim:deviceSetTopBox,
        haim:deviceSmartElectricMeter,
        haim:deviceSmartPlug,
        haim:deviceSteamCloset,
        haim:deviceStorageBattery,
        haim:deviceSwitch,
        haim:deviceTelevision,
        haim:deviceThermometer,
        haim:deviceThermostat,
        haim:deviceThreeDPrinter,
        haim:deviceWaterHeater,
        haim:deviceWaterValve,
        haim:deviceWeightScaleAndBodyCompositionAnalyser,
        haim:deviceWindowShade,
        haim:diastolicPressure,
        haim:discharging,
        haim:dischargingCapacity,
        haim:dishWasherJobMode,
        haim:doorState,
        haim:doorStatus,
        haim:downChannel,
        haim:downVolume,
        haim:duration,
        haim:electricEnergy,
        haim:electricVehicleConnector,
        haim:energy,
        haim:energyConsumption,
        haim:energyGeneration,
        haim:estimatedTimeToEnd,
        haim:extraRinse,
        haim:fat,
        haim:fatFreeMass,
        haim:faultDetection,
        haim:filterInfo,
        haim:filterLifetime,
        haim:foaming,
        haim:foamingStrength,
        haim:frequency,
        haim:generationSource,
        haim:geoLocation,
        haim:glucometer,
        haim:grainsRemaining,
        haim:green,
        haim:grinder,
        haim:hangup,
        haim:hash,
        haim:hba1c,
        haim:heading,
        haim:headingAccuracy,
        haim:heatingLevel,
        haim:heatingZone,
        haim:height,
        haim:horizontalAccuracy,
        haim:horizontalDirection,
        haim:hotWaterSupply,
        haim:impactDirectionHorizontal,
        haim:impactDirectionVertical,
        haim:impactLevel,
        haim:impactSensor,
        haim:impactStatus,
        haim:impedance,
        haim:incrementNumberValue,
        haim:jobModes,
        haim:jobStates,
        haim:kcal,
        haim:keepWarm,
        haim:keyNumber,
        haim:keypad,
        haim:latitude,
        haim:level,
        haim:light,
        haim:liquidLevel,
        haim:liquidRemaining,
        haim:lock,
        haim:loginName,
        haim:longitude,
        haim:loudness,
        haim:lowBattery,
        haim:lqi,
        haim:machineStates,
        haim:material,
        haim:maxHeatingLevel,
        haim:maxLength,
        haim:maxLevel,
        haim:maxSpeed,
        haim:maxValue,
        haim:meanPressure,
        haim:measuringScope,
        haim:mediaID,
        haim:mediaName,
        haim:mediaSelect,
        haim:mediaType,
        haim:memorySize,
        haim:messageEncoding,
        haim:minLength,
        haim:minLevel,
        haim:minSpeed,
        haim:minValue,
        haim:modality,
        haim:monitoringEnabled,
        haim:motionSensor,
        haim:multiplyingFactors,
        haim:muscle,
        haim:muscleMass,
        haim:muteEnabled,
        haim:network,
        haim:nextTrack,
        haim:numberValue,
        haim:object,
        haim:objectType,
        haim:open,
        haim:openAlarm,
        haim:openDuration,
        haim:openLevel,
        haim:operationMode,
        haim:overcurrentSensor,
        haim:overcurrentStatus,
        haim:oximeter,
        haim:oxygenSaturation,
        haim:ozoneMeter,
        haim:ozoneStatus,
        haim:ozoneValueMG,
        haim:ozoneValuePPM,
        haim:password,
        haim:phoneCall,
        haim:playerControl,
        haim:power,
        haim:powerGenerationData,
        haim:powerSave,
        haim:powerSaveEnabled,
        haim:powerState,
        haim:preWash,
        haim:previousChannel,
        haim:previousTrack,
        haim:printQueue,
        haim:printSizeX,
        haim:printSizeY,
        haim:printSizeZ,
        haim:printType,
        haim:printingState,
        haim:progressPercentage,
        haim:pulseRate,
        haim:pulsemeter,
        haim:pushButton,
        haim:pushed,
        haim:rapidCool,
        haim:rapidFreeze,
        haim:recipientID,
        haim:recorder,
        haim:red,
        haim:referenceTimer,
        haim:refrigeration,
        haim:relativeHumidity,
        haim:remoteControlEnable,
        haim:remoteControlEnabled,
        haim:resetNumberValue,
        haim:resetTextMessage,
        haim:resistance,
        haim:robotCleanerJobMode,
        haim:roundingEnergyConsumption,
        haim:roundingEnergyGeneration,
        haim:rr,
        haim:rssi,
        haim:runState,
        haim:runningTime,
        haim:sdp,
        haim:securityMode,
        haim:securityModes,
        haim:sensitivity,
        haim:sensorHumidity,
        haim:sensorOdor,
        haim:sensorPM1,
        haim:sensorPM10,
        haim:sensorPM2,
        haim:sessionDescription,
        haim:signalStrength,
        haim:significantDigits,
        haim:silentTime,
        haim:size,
        haim:smokeSensor,
        haim:smokeThreshold,
        haim:softLeanMass,
        haim:soilLevel,
        haim:speed,
        haim:speedFactor,
        haim:speedWash,
        haim:sphygmomanometer,
        haim:spinLevel,
        haim:spinLevelStrength,
        haim:spinSpeed,
        haim:start3Dprint,
        haim:startPause,
        haim:status,
        haim:steamClosetJobMode,
        haim:steamTreat,
        haim:step,
        haim:stepValue,
        haim:stop3Dprint,
        haim:strength,
        haim:subDeviceCuff,
        haim:subDevicePowerOutlet,
        haim:supportedHorizontalDirection,
        haim:supportedMediaSources,
        haim:supportedMessageValues,
        haim:supportedPlayerModes,
        haim:supportedVerticalDirection,
        haim:systolicPressure,
        haim:targetAltitude,
        haim:targetDuration,
        haim:targetLatitude,
        haim:targetLongitude,
        haim:targetTemperature,
        haim:targetTimeToStart,
        haim:targetTimeToStop,
        haim:televisionChannel,
        haim:temperature,
        haim:temperatureAlarm,
        haim:temperatureThreshold,
        haim:textMessage,
        haim:threeDPrinter,
        haim:time,
        haim:timer,
        haim:toggle,
        haim:token,
        haim:tone,
        haim:turbo,
        haim:turboEnabled,
        haim:unit,
        haim:upChannel,
        haim:upVolume,
        haim:uri,
        haim:url,
        haim:useGrinder,
        haim:uvSensor,
        haim:uvStatus,
        haim:uvValue,
        haim:verticalAccuracy,
        haim:verticalDirection,
        haim:visceraFat,
        haim:voc,
        haim:voltage,
        haim:volumePercentage,
        haim:washTemp,
        haim:water,
        haim:waterFlow,
        haim:waterFlowStrength,
        haim:waterSensor,
        haim:weight .

haim:binaryObject a skos:Concept,
        ontolex:LexicalConcept ;
    skos:broader onem2m:Module ;
    skos:definition "This ModuleClass describes the handling of a binary object (blob). "@en ;
    skos:inScheme onem2m:scheme ;
    skos:prefLabel "binaryObject"@en ;
    skos:related haim:hash,
        haim:object,
        haim:objectType,
        haim:size ;
    prov:wasDerivedFrom <https://git.onem2m.org/MAS/Home-Appliances/-/raw/master/3.7.0/SDT-TS0023-ModuleClasses.xml> .

haim:credentials a skos:Concept,
        ontolex:LexicalConcept ;
    skos:broader onem2m:Module ;
    skos:definition "This ModuleClass provides the capability to manage user credentials which allows a user to authenticate on an appliance or a server that is associated with the appliance. The authentication depends on a user login and password, or on a token. An example appliance which may include this ModuleClass is a camera. "@en ;
    skos:inScheme onem2m:scheme ;
    skos:prefLabel "credentials"@en ;
    skos:related haim:loginName,
        haim:password,
        haim:token ;
    prov:wasDerivedFrom <https://git.onem2m.org/MAS/Home-Appliances/-/raw/master/3.7.0/SDT-TS0023-ModuleClasses.xml> .

haim:deviceAirConditioner a skos:Concept,
        ontolex:LexicalConcept ;
    skos:broader onem2m:Device ;
    skos:definition "An air conditioner is a home appliance used to alter the properties of air (primarily temperature and humidity) to more comfortable conditions. This air conditioner information model provides capabilities to control and monitor air conditioner specific functions and resources."@en ;
    skos:inScheme onem2m:scheme ;
    skos:prefLabel "deviceAirConditioner"@en ;
    skos:related haim:airConJobMode,
        haim:airFlow,
        haim:airQualitySensor,
        haim:binarySwitch,
        haim:filterInfo,
        haim:operationMode,
        haim:powerSave,
        haim:runState,
        haim:temperature,
        haim:timer,
        haim:turbo ;
    prov:wasDerivedFrom <https://git.onem2m.org/MAS/Home-Appliances/-/raw/master/3.7.0/SDT-TS0023-Devices.xml> .

haim:deviceAirPurifier a skos:Concept,
        ontolex:LexicalConcept ;
    skos:broader onem2m:Device ;
    skos:definition "An airPurifieris a home appliance is used to prevent dust and other particles from air by filtering, washing or electrostatic precipitation. This airPurifier information model provides capabilities to control and monitor airPurifier specific functions and resources."@en ;
    skos:inScheme onem2m:scheme ;
    skos:prefLabel "deviceAirPurifier"@en ;
    skos:related haim:airPurifierJobMode,
        haim:airQualitySensor,
        haim:binarySwitch,
        haim:filterInfo,
        haim:operationMode,
        haim:powerSave,
        haim:runState,
        haim:timer ;
    prov:wasDerivedFrom <https://git.onem2m.org/MAS/Home-Appliances/-/raw/master/3.7.0/SDT-TS0023-Devices.xml> .

haim:deviceAirQualityMonitor a skos:Concept,
        ontolex:LexicalConcept ;
    skos:broader onem2m:Device ;
    skos:definition "An air quality monitor is a home appliance for monitoring the air quality. This airQualityMonitor information model provides capabilities to monitor the airQualityMonitor functions and resources."@en ;
    skos:inScheme onem2m:scheme ;
    skos:prefLabel "deviceAirQualityMonitor"@en ;
    skos:related haim:airQualitySensor ;
    prov:wasDerivedFrom <https://git.onem2m.org/MAS/Home-Appliances/-/raw/master/3.7.0/SDT-TS0023-Devices.xml> .

haim:deviceAudioReceiver a skos:Concept,
        ontolex:LexicalConcept ;
    skos:broader onem2m:Device ;
    skos:definition "An audio receiver is a device that receives audio signals from a number of sources, processing them to drive speakers."@en ;
    skos:inScheme onem2m:scheme ;
    skos:prefLabel "deviceAudioReceiver"@en ;
    skos:related haim:audioVolume,
        haim:binarySwitch,
        haim:mediaSelect ;
    prov:wasDerivedFrom <https://git.onem2m.org/MAS/Home-Appliances/-/raw/master/3.7.0/SDT-TS0023-Devices.xml> .

haim:deviceBloodPressureMonitor a skos:Concept,
        ontolex:LexicalConcept ;
    skos:broader onem2m:Device ;
    skos:definition "A blood pressure monitor is a device that can be used to monitor the blood pressure and is composed of one or more cuffs and a main montor machine."@en ;
    skos:inScheme onem2m:scheme ;
    skos:prefLabel "deviceBloodPressureMonitor"@en ;
    skos:related haim:battery,
        haim:binarySwitch ;
    prov:wasDerivedFrom <https://git.onem2m.org/MAS/Home-Appliances/-/raw/master/3.7.0/SDT-TS0023-Devices.xml> .

haim:deviceCamera a skos:Concept,
        ontolex:LexicalConcept ;
    skos:broader onem2m:Device ;
    skos:definition "A camera is an optical instrument for recording or capturing images, which may be stored locally or transmitted to another locations."@en ;
    skos:inScheme onem2m:scheme ;
    skos:prefLabel "deviceCamera"@en ;
    skos:related haim:motionSensor,
        haim:playerControl,
        haim:sessionDescription ;
    prov:wasDerivedFrom <https://git.onem2m.org/MAS/Home-Appliances/-/raw/master/3.7.0/SDT-TS0023-Devices.xml> .

haim:deviceClothesDryer a skos:Concept,
        ontolex:LexicalConcept ;
    skos:broader onem2m:Device ;
    skos:definition "A clothes dryer is a home appliance for drying clothes. This clothesDryer information model provides capabilities to control and monitor clothes dryer specific functions and resources."@en ;
    skos:inScheme onem2m:scheme ;
    skos:prefLabel "deviceClothesDryer"@en ;
    skos:related haim:binarySwitch,
        haim:clothesDryerJobMode,
        haim:operationMode,
        haim:runState ;
    prov:wasDerivedFrom <https://git.onem2m.org/MAS/Home-Appliances/-/raw/master/3.7.0/SDT-TS0023-Devices.xml> .

haim:deviceClothesWasher a skos:Concept,
        ontolex:LexicalConcept ;
    skos:broader onem2m:Device ;
    skos:definition "A clothes washer is a home appliance that is used to wash laundry, such as clothing and sheets. This information model provides capabilities to interact with specific functions and resources of clothes washers."@en ;
    skos:inScheme onem2m:scheme ;
    skos:prefLabel "deviceClothesWasher"@en ;
    skos:related haim:binarySwitch,
        haim:clothesWasherJobMode,
        haim:clothesWasherJobModeOption,
        haim:operationMode,
        haim:remoteControlEnable,
        haim:runState,
        haim:timer ;
    prov:wasDerivedFrom <https://git.onem2m.org/MAS/Home-Appliances/-/raw/master/3.7.0/SDT-TS0023-Devices.xml> .

haim:deviceClothesWasherDryer a skos:Concept,
        ontolex:LexicalConcept ;
    skos:broader onem2m:Device ;
    skos:definition "A clothes washer dryer is a home appliance that is a combination of cloth washer and cloth dryer in a single cabinet. This information model provides capabilities to interact with specific functions and resources of clothes washers and dryers."@en ;
    skos:inScheme onem2m:scheme ;
    skos:prefLabel "deviceClothesWasherDryer"@en ;
    skos:related haim:binarySwitch,
        haim:clothesWasherDryerJobMode,
        haim:clothesWasherJobModeOption,
        haim:operationMode,
        haim:remoteControlEnable,
        haim:runState,
        haim:timer ;
    prov:wasDerivedFrom <https://git.onem2m.org/MAS/Home-Appliances/-/raw/master/3.7.0/SDT-TS0023-Devices.xml> .

haim:deviceCoffeeMachine a skos:Concept,
        ontolex:LexicalConcept ;
    skos:broader onem2m:Device ;
    skos:definition "A coffee machine is a device that is used to brew a coffee, may add foamed milk, and may include some variants, for example a grinder."@en ;
    skos:inScheme onem2m:scheme ;
    skos:prefLabel "deviceCoffeeMachine"@en ;
    skos:related haim:binarySwitch,
        haim:brewing,
        haim:clock,
        haim:faultDetection,
        haim:foaming,
        haim:grinder,
        haim:keepWarm,
        haim:liquidLevel,
        haim:liquidRemaining,
        haim:runState ;
    prov:wasDerivedFrom <https://git.onem2m.org/MAS/Home-Appliances/-/raw/master/3.7.0/SDT-TS0023-Devices.xml> .

haim:deviceCookerHood a skos:Concept,
        ontolex:LexicalConcept ;
    skos:broader onem2m:Device ;
    skos:definition "A cooker hood is a device containing a mechanical fan that hangs above the stove or cooktop in the kitchen."@en ;
    skos:inScheme onem2m:scheme ;
    skos:prefLabel "deviceCookerHood"@en ;
    skos:related haim:airFlow,
        haim:binarySwitch,
        haim:cookerHoodJobMode,
        haim:runState ;
    prov:wasDerivedFrom <https://git.onem2m.org/MAS/Home-Appliances/-/raw/master/3.7.0/SDT-TS0023-Devices.xml> .

haim:deviceCooktop a skos:Concept,
        ontolex:LexicalConcept ;
    skos:broader onem2m:Device ;
    skos:definition "A cooktop is a device that is a kitchen appliance designed for the purpose of cooking food."@en ;
    skos:inScheme onem2m:scheme ;
    skos:prefLabel "deviceCooktop"@en ;
    skos:related haim:heatingZone ;
    prov:wasDerivedFrom <https://git.onem2m.org/MAS/Home-Appliances/-/raw/master/3.7.0/SDT-TS0023-Devices.xml> .

haim:deviceDehumidifier a skos:Concept,
        ontolex:LexicalConcept ;
    skos:broader onem2m:Device ;
    skos:definition "A dehumidifier is a device that is used to monitor or control the state of a dehumidifying appliance."@en ;
    skos:inScheme onem2m:scheme ;
    skos:prefLabel "deviceDehumidifier"@en ;
    skos:related haim:binarySwitch,
        haim:dehumidifierJobMode,
        haim:operationMode,
        haim:powerSave,
        haim:relativeHumidity,
        haim:runState,
        haim:timer ;
    prov:wasDerivedFrom <https://git.onem2m.org/MAS/Home-Appliances/-/raw/master/3.7.0/SDT-TS0023-Devices.xml> .

haim:deviceDishWasher a skos:Concept,
        ontolex:LexicalConcept ;
    skos:broader onem2m:Device ;
    skos:definition "A dish washer is a home appliance used to wash dishes. This information model provides capabilities to interact with specific functions and resources of a dish washer."@en ;
    skos:inScheme onem2m:scheme ;
    skos:prefLabel "deviceDishWasher"@en ;
    skos:related haim:binarySwitch,
        haim:dishWasherJobMode,
        haim:runState ;
    prov:wasDerivedFrom <https://git.onem2m.org/MAS/Home-Appliances/-/raw/master/3.7.0/SDT-TS0023-Devices.xml> .

haim:deviceDoor a skos:Concept,
        ontolex:LexicalConcept ;
    skos:broader onem2m:Device ;
    skos:definition "A deviceDoor is a device that is used to open and close a door."@en ;
    skos:inScheme onem2m:scheme ;
    skos:prefLabel "deviceDoor"@en ;
    skos:related haim:doorStatus,
        haim:lock,
        haim:openLevel ;
    prov:wasDerivedFrom <https://git.onem2m.org/MAS/Home-Appliances/-/raw/master/3.7.0/SDT-TS0023-Devices.xml> .

haim:deviceDoorLock a skos:Concept,
        ontolex:LexicalConcept ;
    skos:broader onem2m:Device ;
    skos:definition "A door lock is a device that can be used to lock, for example, a door."@en ;
    skos:inScheme onem2m:scheme ;
    skos:prefLabel "deviceDoorLock"@en ;
    skos:related haim:battery,
        haim:doorStatus,
        haim:lock ;
    prov:wasDerivedFrom <https://git.onem2m.org/MAS/Home-Appliances/-/raw/master/3.7.0/SDT-TS0023-Devices.xml> .

haim:deviceElectricVehicleCharger a skos:Concept,
        ontolex:LexicalConcept ;
    skos:broader onem2m:Device ;
    skos:definition "An electric vehicle charger is a device that is used for charging or discharging electric vehicles."@en ;
    skos:inScheme onem2m:scheme ;
    skos:prefLabel "deviceElectricVehicleCharger"@en ;
    skos:related haim:battery,
        haim:binarySwitch,
        haim:electricVehicleConnector,
        haim:faultDetection,
        haim:runState ;
    prov:wasDerivedFrom <https://git.onem2m.org/MAS/Home-Appliances/-/raw/master/3.7.0/SDT-TS0023-Devices.xml> .

haim:deviceFan a skos:Concept,
        ontolex:LexicalConcept ;
    skos:broader onem2m:Device ;
    skos:definition "A fan is a device that is used to monitor or control the state of a fanning device."@en ;
    skos:inScheme onem2m:scheme ;
    skos:prefLabel "deviceFan"@en ;
    skos:related haim:binarySwitch ;
    prov:wasDerivedFrom <https://git.onem2m.org/MAS/Home-Appliances/-/raw/master/3.7.0/SDT-TS0023-Devices.xml> .

haim:deviceFoodProbe a skos:Concept,
        ontolex:LexicalConcept ;
    skos:broader onem2m:Device ;
    skos:definition "A food probe is a device that is used to measure the internal temperature of food."@en ;
    skos:inScheme onem2m:scheme ;
    skos:prefLabel "deviceFoodProbe"@en ;
    skos:related haim:temperature ;
    prov:wasDerivedFrom <https://git.onem2m.org/MAS/Home-Appliances/-/raw/master/3.7.0/SDT-TS0023-Devices.xml> .

haim:deviceFreezer a skos:Concept,
        ontolex:LexicalConcept ;
    skos:broader onem2m:Device ;
    skos:definition "A freezer is a large container like a fridge in which the temperature is kept below freezing point, so that food can be storeed inside of it for long periods. This freezer information model provides capabilities to monitor freezer specific functions and resources."@en ;
    skos:inScheme onem2m:scheme ;
    skos:prefLabel "deviceFreezer"@en ;
    skos:related haim:temperature ;
    prov:wasDerivedFrom <https://git.onem2m.org/MAS/Home-Appliances/-/raw/master/3.7.0/SDT-TS0023-Devices.xml> .

haim:deviceGlucosemeter a skos:Concept,
        ontolex:LexicalConcept ;
    skos:broader onem2m:Device ;
    skos:definition "A glucometer is a device that can be used to monitor the blood glucose level."@en ;
    skos:inScheme onem2m:scheme ;
    skos:prefLabel "deviceGlucosemeter"@en ;
    skos:related haim:battery,
        haim:glucometer ;
    prov:wasDerivedFrom <https://git.onem2m.org/MAS/Home-Appliances/-/raw/master/3.7.0/SDT-TS0023-Devices.xml> .

haim:deviceHeartRateMonitor a skos:Concept,
        ontolex:LexicalConcept ;
    skos:broader onem2m:Device ;
    skos:definition "A heart rate monitor is a device that can be used to monitor the heart rate."@en ;
    skos:inScheme onem2m:scheme ;
    skos:prefLabel "deviceHeartRateMonitor"@en ;
    skos:related haim:battery,
        haim:pulsemeter ;
    prov:wasDerivedFrom <https://git.onem2m.org/MAS/Home-Appliances/-/raw/master/3.7.0/SDT-TS0023-Devices.xml> .

haim:deviceHomeCCTV a skos:Concept,
        ontolex:LexicalConcept ;
    skos:broader onem2m:Device ;
    skos:definition "A home CCTV is a smart home appliance to provide monitoring capabilities when people stay away from their home or a room, or to monitor the environmental status of their home or room."@en ;
    skos:inScheme onem2m:scheme ;
    skos:prefLabel "deviceHomeCCTV"@en ;
    skos:related haim:acousticSensor,
        haim:airQualitySensor,
        haim:alarmSpeaker,
        haim:binarySwitch,
        haim:faultDetection,
        haim:impactSensor,
        haim:motionSensor,
        haim:ozoneMeter,
        haim:playerControl,
        haim:runState,
        haim:sessionDescription,
        haim:smokeSensor ;
    prov:wasDerivedFrom <https://git.onem2m.org/MAS/Home-Appliances/-/raw/master/3.7.0/SDT-TS0023-Devices.xml> .

haim:deviceHumidifier a skos:Concept,
        ontolex:LexicalConcept ;
    skos:broader onem2m:Device ;
    skos:definition "A humidifier is a device that is used to monitor or control the state of a humidifying appliance."@en ;
    skos:inScheme onem2m:scheme ;
    skos:prefLabel "deviceHumidifier"@en ;
    skos:related haim:binarySwitch ;
    prov:wasDerivedFrom <https://git.onem2m.org/MAS/Home-Appliances/-/raw/master/3.7.0/SDT-TS0023-Devices.xml> .

haim:deviceKettle a skos:Concept,
        ontolex:LexicalConcept ;
    skos:broader onem2m:Device ;
    skos:definition "Kettle is a device used to boil water. It may set a desired temperature for water and may keep water warm for a desired time."@en ;
    skos:inScheme onem2m:scheme ;
    skos:prefLabel "deviceKettle"@en ;
    skos:related haim:binarySwitch,
        haim:faultDetection,
        haim:keepWarm,
        haim:liquidRemaining,
        haim:runState,
        haim:temperature ;
    prov:wasDerivedFrom <https://git.onem2m.org/MAS/Home-Appliances/-/raw/master/3.7.0/SDT-TS0023-Devices.xml> .

haim:deviceLight a skos:Concept,
        ontolex:LexicalConcept ;
    skos:broader onem2m:Device ;
    skos:definition "A light is a device that is used to control the state of an illumination appliance."@en ;
    skos:inScheme onem2m:scheme ;
    skos:prefLabel "deviceLight"@en ;
    skos:related haim:binarySwitch,
        haim:brightness,
        haim:colour,
        haim:colourSaturation,
        haim:faultDetection,
        haim:runState ;
    prov:wasDerivedFrom <https://git.onem2m.org/MAS/Home-Appliances/-/raw/master/3.7.0/SDT-TS0023-Devices.xml> .

haim:deviceMicrogeneration a skos:Concept,
        ontolex:LexicalConcept ;
    skos:broader onem2m:Device ;
    skos:definition "A microgeneration is a Home Energy Management System (HEMS) device that is used to generate energy. Examples of microgeneration devices are photovoltaics device or fuel cells."@en ;
    skos:inScheme onem2m:scheme ;
    skos:prefLabel "deviceMicrogeneration"@en ;
    skos:related haim:binarySwitch,
        haim:energyGeneration,
        haim:faultDetection,
        haim:runState ;
    prov:wasDerivedFrom <https://git.onem2m.org/MAS/Home-Appliances/-/raw/master/3.7.0/SDT-TS0023-Devices.xml> .

haim:deviceMultiFunctionPrinter a skos:Concept,
        ontolex:LexicalConcept ;
    skos:broader onem2m:Device ;
    skos:definition "A Multi Function Printer (MFP) is an office machine which incorporates the functionality of multiple devices in one, so as to have a smaller footprint in home or office. A typical MFP may act as a combination of printer, scanner and more. This MFP information model provides capabilities to control and monitor MFP specific functions and resources."@en ;
    skos:inScheme onem2m:scheme ;
    skos:prefLabel "deviceMultiFunctionPrinter"@en ;
    skos:related haim:autoDocumentFeeder,
        haim:binarySwitch,
        haim:printQueue,
        haim:runState ;
    prov:wasDerivedFrom <https://git.onem2m.org/MAS/Home-Appliances/-/raw/master/3.7.0/SDT-TS0023-Devices.xml> .

haim:deviceOutdoorLamp a skos:Concept,
        ontolex:LexicalConcept ;
    skos:broader onem2m:Device ;
    skos:definition "An outdoor lamp is a smart home appliance to provide lights and information for outside of home with smart sensing capabilities such as ultraviolet sensing."@en ;
    skos:inScheme onem2m:scheme ;
    skos:prefLabel "deviceOutdoorLamp"@en ;
    skos:related haim:airQualitySensor,
        haim:binarySwitch,
        haim:brightness,
        haim:faultDetection,
        haim:motionSensor,
        haim:timer,
        haim:uvSensor ;
    prov:wasDerivedFrom <https://git.onem2m.org/MAS/Home-Appliances/-/raw/master/3.7.0/SDT-TS0023-Devices.xml> .

haim:deviceOven a skos:Concept,
        ontolex:LexicalConcept ;
    skos:broader onem2m:Device ;
    skos:definition "An oven is a home appliance used to roast and heat food in a complete stove. This information model is applicable to different types of ovens: gas ovens, electrical ovens, steam ovens, microwave ovens, etc. This information model provides capabilities to interact with specific functions and resources of ovens."@en ;
    skos:inScheme onem2m:scheme ;
    skos:prefLabel "deviceOven"@en ;
    skos:related haim:binarySwitch,
        haim:runState,
        haim:temperature,
        haim:timer ;
    prov:wasDerivedFrom <https://git.onem2m.org/MAS/Home-Appliances/-/raw/master/3.7.0/SDT-TS0023-Devices.xml> .

haim:devicePrinter a skos:Concept,
        ontolex:LexicalConcept ;
    skos:broader onem2m:Device ;
    skos:definition "A printer is a device that is used to monitor or control the state of a printing appliance."@en ;
    skos:inScheme onem2m:scheme ;
    skos:prefLabel "devicePrinter"@en ;
    skos:related haim:binarySwitch,
        haim:printQueue,
        haim:runState ;
    prov:wasDerivedFrom <https://git.onem2m.org/MAS/Home-Appliances/-/raw/master/3.7.0/SDT-TS0023-Devices.xml> .

haim:devicePulseOximeter a skos:Concept,
        ontolex:LexicalConcept ;
    skos:broader onem2m:Device ;
    skos:definition "A pulseoximeter is a device that can be used to monitor the blood characteristics."@en ;
    skos:inScheme onem2m:scheme ;
    skos:prefLabel "devicePulseOximeter"@en ;
    skos:related haim:battery,
        haim:oximeter,
        haim:pulsemeter ;
    prov:wasDerivedFrom <https://git.onem2m.org/MAS/Home-Appliances/-/raw/master/3.7.0/SDT-TS0023-Devices.xml> .

haim:deviceRefrigerator a skos:Concept,
        ontolex:LexicalConcept ;
    skos:broader onem2m:Device ;
    skos:definition "A refrigerator is a home appliance used to store food at temperatures which are a few degrees above the freezing point of water. This information model provides capabilities to interact with specific functions and resource of refrigerators."@en ;
    skos:inScheme onem2m:scheme ;
    skos:prefLabel "deviceRefrigerator"@en ;
    skos:related haim:binarySwitch,
        haim:doorStatus,
        haim:filterInfo,
        haim:lock,
        haim:powerSave,
        haim:refrigeration,
        haim:temperature ;
    prov:wasDerivedFrom <https://git.onem2m.org/MAS/Home-Appliances/-/raw/master/3.7.0/SDT-TS0023-Devices.xml> .

haim:deviceRobotCleaner a skos:Concept,
        ontolex:LexicalConcept ;
    skos:broader onem2m:Device ;
    skos:definition "A robot cleaner is an autonomous robotic vacuum cleaner that has intelligent programming and a limited vacuum cleaning system. This robot cleaner information model provides capabilities to control and monitor robot cleaner specific functions and resources."@en ;
    skos:inScheme onem2m:scheme ;
    skos:prefLabel "deviceRobotCleaner"@en ;
    skos:related haim:battery,
        haim:binarySwitch,
        haim:operationMode,
        haim:robotCleanerJobMode,
        haim:runState,
        haim:timer ;
    prov:wasDerivedFrom <https://git.onem2m.org/MAS/Home-Appliances/-/raw/master/3.7.0/SDT-TS0023-Devices.xml> .

haim:deviceScanner a skos:Concept,
        ontolex:LexicalConcept ;
    skos:broader onem2m:Device ;
    skos:definition "A scanner is a device that optically scans images, printed text, handwriting or an object, and converts it to a digital image."@en ;
    skos:inScheme onem2m:scheme ;
    skos:prefLabel "deviceScanner"@en ;
    skos:related haim:autoDocumentFeeder,
        haim:binarySwitch,
        haim:runState ;
    prov:wasDerivedFrom <https://git.onem2m.org/MAS/Home-Appliances/-/raw/master/3.7.0/SDT-TS0023-Devices.xml> .

haim:deviceSecurityPanel a skos:Concept,
        ontolex:LexicalConcept ;
    skos:broader onem2m:Device ;
    skos:definition "A security panel is a device that can change the security mode of, for example, an alarm system."@en ;
    skos:inScheme onem2m:scheme ;
    skos:prefLabel "deviceSecurityPanel"@en ;
    skos:related haim:securityMode ;
    prov:wasDerivedFrom <https://git.onem2m.org/MAS/Home-Appliances/-/raw/master/3.7.0/SDT-TS0023-Devices.xml> .

haim:deviceSetTopBox a skos:Concept,
        ontolex:LexicalConcept ;
    skos:broader onem2m:Device ;
    skos:definition "A set top box is a device that in general contains a TV tuner input and displays output to a TV."@en ;
    skos:inScheme onem2m:scheme ;
    skos:prefLabel "deviceSetTopBox"@en ;
    skos:related haim:audioVolume,
        haim:binarySwitch,
        haim:mediaSelect,
        haim:televisionChannel ;
    prov:wasDerivedFrom <https://git.onem2m.org/MAS/Home-Appliances/-/raw/master/3.7.0/SDT-TS0023-Devices.xml> .

haim:deviceSmartElectricMeter a skos:Concept,
        ontolex:LexicalConcept ;
    skos:broader onem2m:Device ;
    skos:definition "A smart electric meter is a metering device that is used to measure consumption data for electricity."@en ;
    skos:inScheme onem2m:scheme ;
    skos:prefLabel "deviceSmartElectricMeter"@en ;
    skos:related haim:binarySwitch,
        haim:clock,
        haim:energyConsumption,
        haim:energyGeneration,
        haim:faultDetection,
        haim:runState ;
    prov:wasDerivedFrom <https://git.onem2m.org/MAS/Home-Appliances/-/raw/master/3.7.0/SDT-TS0023-Devices.xml> .

haim:deviceSmartPlug a skos:Concept,
        ontolex:LexicalConcept ;
    skos:broader onem2m:Device ;
    skos:definition "A smart plug is a device that can turn on and off a connected appliance."@en ;
    skos:inScheme onem2m:scheme ;
    skos:prefLabel "deviceSmartPlug"@en ;
    skos:related haim:binarySwitch,
        haim:faultDetection,
        haim:remoteControlEnable ;
    prov:wasDerivedFrom <https://git.onem2m.org/MAS/Home-Appliances/-/raw/master/3.7.0/SDT-TS0023-Devices.xml> .

haim:deviceSteamCloset a skos:Concept,
        ontolex:LexicalConcept ;
    skos:broader onem2m:Device ;
    skos:definition "A deviceSteamCloset is a home appliance that de-wrinkles, sanitizes and dries to clean fabrics similar to a dry cleaner. This information model provides capabilities to interact with specific functions and resources of the steam closet."@en ;
    skos:inScheme onem2m:scheme ;
    skos:prefLabel "deviceSteamCloset"@en ;
    skos:related haim:binarySwitch,
        haim:operationMode,
        haim:runState,
        haim:steamClosetJobMode ;
    prov:wasDerivedFrom <https://git.onem2m.org/MAS/Home-Appliances/-/raw/master/3.7.0/SDT-TS0023-Devices.xml> .

haim:deviceStorageBattery a skos:Concept,
        ontolex:LexicalConcept ;
    skos:broader onem2m:Device ;
    skos:definition "A storage battery is a Home Energy Management System HEMS device that is used to provide the home with electrical energy."@en ;
    skos:inScheme onem2m:scheme ;
    skos:prefLabel "deviceStorageBattery"@en ;
    skos:related haim:battery,
        haim:binarySwitch,
        haim:faultDetection,
        haim:runState ;
    prov:wasDerivedFrom <https://git.onem2m.org/MAS/Home-Appliances/-/raw/master/3.7.0/SDT-TS0023-Devices.xml> .

haim:deviceSwitch a skos:Concept,
        ontolex:LexicalConcept ;
    skos:broader onem2m:Device ;
    skos:definition "A switch is a device that is used to control and monitor the state of power. Although there is only one module instance in Table 5.5.42-1, the binarySwitch module instance can be extended using different module instance names according to the requirement."@en ;
    skos:inScheme onem2m:scheme ;
    skos:prefLabel "deviceSwitch"@en ;
    skos:related haim:binarySwitch ;
    prov:wasDerivedFrom <https://git.onem2m.org/MAS/Home-Appliances/-/raw/master/3.7.0/SDT-TS0023-Devices.xml> .

haim:deviceTelevision a skos:Concept,
        ontolex:LexicalConcept ;
    skos:broader onem2m:Device ;
    skos:definition "A television (TV) is a home appliance used to show audio and visual content such as broadcasting programs and network streaming. This TV information model provides capabilities to control and monitor TV specific resources."@en ;
    skos:inScheme onem2m:scheme ;
    skos:prefLabel "deviceTelevision"@en ;
    skos:related haim:audioVolume,
        haim:binarySwitch,
        haim:mediaSelect,
        haim:playerControl,
        haim:televisionChannel ;
    prov:wasDerivedFrom <https://git.onem2m.org/MAS/Home-Appliances/-/raw/master/3.7.0/SDT-TS0023-Devices.xml> .

haim:deviceThermometer a skos:Concept,
        ontolex:LexicalConcept ;
    skos:broader onem2m:Device ;
    skos:definition "A thermometer is a device that can be used to check, for example, the body or other temperatures."@en ;
    skos:inScheme onem2m:scheme ;
    skos:prefLabel "deviceThermometer"@en ;
    skos:related haim:battery,
        haim:temperature ;
    prov:wasDerivedFrom <https://git.onem2m.org/MAS/Home-Appliances/-/raw/master/3.7.0/SDT-TS0023-Devices.xml> .

haim:deviceThermostat a skos:Concept,
        ontolex:LexicalConcept ;
    skos:broader onem2m:Device ;
    skos:definition "A thermostat is used to control the ambient temperature of rooms within, for example, a house. This information model provides capabilities to interact with specific functions of thermostats."@en ;
    skos:inScheme onem2m:scheme ;
    skos:prefLabel "deviceThermostat"@en ;
    skos:related haim:runState,
        haim:temperature,
        haim:timer ;
    prov:wasDerivedFrom <https://git.onem2m.org/MAS/Home-Appliances/-/raw/master/3.7.0/SDT-TS0023-Devices.xml> .

haim:deviceThreeDPrinter a skos:Concept,
        ontolex:LexicalConcept ;
    skos:broader onem2m:Device ;
    skos:definition "A 3D printer is a smart home appliance to provide 3D printing capabilities."@en ;
    skos:inScheme onem2m:scheme ;
    skos:prefLabel "deviceThreeDPrinter"@en ;
    skos:related haim:binarySwitch,
        haim:faultDetection,
        haim:printQueue,
        haim:runState,
        haim:temperature,
        haim:threeDPrinter ;
    prov:wasDerivedFrom <https://git.onem2m.org/MAS/Home-Appliances/-/raw/master/3.7.0/SDT-TS0023-Devices.xml> .

haim:deviceWaterHeater a skos:Concept,
        ontolex:LexicalConcept ;
    skos:broader onem2m:Device ;
    skos:definition "A water heater is a device that is used to provide hot water through home facilities."@en ;
    skos:inScheme onem2m:scheme ;
    skos:prefLabel "deviceWaterHeater"@en ;
    skos:related haim:binarySwitch,
        haim:boiler,
        haim:clock,
        haim:faultDetection,
        haim:hotWaterSupply,
        haim:runState ;
    prov:wasDerivedFrom <https://git.onem2m.org/MAS/Home-Appliances/-/raw/master/3.7.0/SDT-TS0023-Devices.xml> .

haim:deviceWaterValve a skos:Concept,
        ontolex:LexicalConcept ;
    skos:broader onem2m:Device ;
    skos:definition "A water valve is a device that is used to turn the water supply ON or OFF remotely."@en ;
    skos:inScheme onem2m:scheme ;
    skos:prefLabel "deviceWaterValve"@en ;
    skos:related haim:openLevel ;
    prov:wasDerivedFrom <https://git.onem2m.org/MAS/Home-Appliances/-/raw/master/3.7.0/SDT-TS0023-Devices.xml> .

haim:deviceWeightScaleAndBodyCompositionAnalyser a skos:Concept,
        ontolex:LexicalConcept ;
    skos:broader onem2m:Device ;
    skos:definition "A weight scale and body composition analyser is a device that can be used to monitor the weight and body composition."@en ;
    skos:inScheme onem2m:scheme ;
    skos:prefLabel "deviceWeightScaleAndBodyCompositionAnalyser"@en ;
    skos:related haim:battery,
        haim:bioElectricalImpedanceAnalysis,
        haim:bodyCompositionAnalyser,
        haim:weight ;
    prov:wasDerivedFrom <https://git.onem2m.org/MAS/Home-Appliances/-/raw/master/3.7.0/SDT-TS0023-Devices.xml> .

haim:deviceWindowShade a skos:Concept,
        ontolex:LexicalConcept ;
    skos:broader onem2m:Device ;
    skos:definition "The window shade is an appliance that provides the ability to cover windows. This device type includes but not limited to roller shades, drapes, and tilt-only blinds."@en ;
    skos:inScheme onem2m:scheme ;
    skos:prefLabel "deviceWindowShade"@en ;
    skos:related haim:battery,
        haim:openLevel ;
    prov:wasDerivedFrom <https://git.onem2m.org/MAS/Home-Appliances/-/raw/master/3.7.0/SDT-TS0023-Devices.xml> .

haim:geoLocation a skos:Concept,
        ontolex:LexicalConcept ;
    skos:broader onem2m:Module ;
    skos:definition "This ModuleClass provides the capability to get or set geo-location information."@en ;
    skos:inScheme onem2m:scheme ;
    skos:prefLabel "geoLocation"@en ;
    skos:related haim:altitude,
        haim:heading,
        haim:headingAccuracy,
        haim:horizontalAccuracy,
        haim:latitude,
        haim:longitude,
        haim:targetAltitude,
        haim:targetLatitude,
        haim:targetLongitude,
        haim:verticalAccuracy ;
    prov:wasDerivedFrom <https://git.onem2m.org/MAS/Home-Appliances/-/raw/master/3.7.0/SDT-TS0023-ModuleClasses.xml> .

haim:keypad a skos:Concept,
        ontolex:LexicalConcept ;
    skos:broader onem2m:Module ;
    skos:definition "This ModuleClass provides the capability to require a user defined service through the key-in number. For example, a user can define key 1 as \"require a takeout from restaurant XXX with combo meal 1\". The IoT service provider or user can define the services."@en ;
    skos:inScheme onem2m:scheme ;
    skos:prefLabel "keypad"@en ;
    skos:related haim:keyNumber ;
    prov:wasDerivedFrom <https://git.onem2m.org/MAS/Home-Appliances/-/raw/master/3.7.0/SDT-TS0023-ModuleClasses.xml> .

haim:phoneCall a skos:Concept,
        ontolex:LexicalConcept ;
    skos:broader onem2m:Module ;
    skos:definition "This ModuleClass provides the capability get or set the caller and recipient IDs as well as to initiate and terminate a call."@en ;
    skos:inScheme onem2m:scheme ;
    skos:prefLabel "phoneCall"@en ;
    skos:related haim:answer,
        haim:call,
        haim:callState,
        haim:callerID,
        haim:hangup,
        haim:recipientID ;
    prov:wasDerivedFrom <https://git.onem2m.org/MAS/Home-Appliances/-/raw/master/3.7.0/SDT-TS0023-ModuleClasses.xml> .

haim:pushButton a skos:Concept,
        ontolex:LexicalConcept ;
    skos:broader onem2m:Module ;
    skos:definition "This ModuleClass provides the capability to indicate the operation of a button style switch. A typical application can be an SOS button."@en ;
    skos:inScheme onem2m:scheme ;
    skos:prefLabel "pushButton"@en ;
    skos:related haim:pushed ;
    prov:wasDerivedFrom <https://git.onem2m.org/MAS/Home-Appliances/-/raw/master/3.7.0/SDT-TS0023-ModuleClasses.xml> .

haim:recorder a skos:Concept,
        ontolex:LexicalConcept ;
    skos:broader onem2m:Module ;
    skos:definition "This ModuleClass provides the capability to record the video/audio for a defined duration."@en ;
    skos:inScheme onem2m:scheme ;
    skos:prefLabel "recorder"@en ;
    skos:related haim:duration ;
    prov:wasDerivedFrom <https://git.onem2m.org/MAS/Home-Appliances/-/raw/master/3.7.0/SDT-TS0023-ModuleClasses.xml> .

haim:signalStrength a skos:Concept,
        ontolex:LexicalConcept ;
    skos:broader onem2m:Module ;
    skos:definition "This ModuleClass provides the capability to monitor the strength of the signal."@en ;
    skos:inScheme onem2m:scheme ;
    skos:prefLabel "signalStrength"@en ;
    skos:related haim:lqi,
        haim:rssi ;
    prov:wasDerivedFrom <https://git.onem2m.org/MAS/Home-Appliances/-/raw/master/3.7.0/SDT-TS0023-ModuleClasses.xml> .

haim:spinLevel a skos:Concept,
        ontolex:LexicalConcept ;
    skos:broader onem2m:Module ;
    skos:definition "This ModuleClass provides capabilities to control and monitor the level of spin. It is intended to be part of devices which use spinning function such as a washing machine and a dryer."@en ;
    skos:inScheme onem2m:scheme ;
    skos:prefLabel "spinLevel"@en ;
    skos:related haim:spinLevelStrength ;
    prov:wasDerivedFrom <https://git.onem2m.org/MAS/Home-Appliances/-/raw/master/3.7.0/SDT-TS0023-ModuleClasses.xml> .

haim:subDeviceCuff a skos:Concept,
        ontolex:LexicalConcept ;
    skos:broader onem2m:Device ;
    skos:definition "A cuff is a subDevice that expresses the attachment device for measuring blood pressure."@en ;
    skos:inScheme onem2m:scheme ;
    skos:prefLabel "subDeviceCuff"@en ;
    skos:related haim:binarySwitch,
        haim:pulsemeter,
        haim:sphygmomanometer .

haim:subDevicePowerOutlet a skos:Concept,
        ontolex:LexicalConcept ;
    skos:broader onem2m:Device ;
    skos:definition "A powerOutlet is a subDevice that specifies the attachment device for deviceSmartPlug."@en ;
    skos:inScheme onem2m:scheme ;
    skos:prefLabel "subDevicePowerOutlet"@en ;
    skos:related haim:binarySwitch,
        haim:dimmingLevel,
        haim:energyConsumption,
        haim:overcurrentSensor .

haim:temperatureAlarm a skos:Concept,
        ontolex:LexicalConcept ;
    skos:broader onem2m:Module ;
    skos:definition "This ModuleClass provides the capabilities to indicate the detection of abnormal temperatures and raises an alarm if the triggering criterion is met."@en ;
    skos:inScheme onem2m:scheme ;
    skos:prefLabel "temperatureAlarm"@en ;
    skos:related haim:alarm,
        haim:temperature,
        haim:temperatureThreshold ;
    prov:wasDerivedFrom <https://git.onem2m.org/MAS/Home-Appliances/-/raw/master/3.7.0/SDT-TS0023-ModuleClasses.xml> .

haim:waterFlow a skos:Concept,
        ontolex:LexicalConcept ;
    skos:broader onem2m:Module ;
    skos:definition "This ModuleClass provides capabilities for controlling the water strength of a device."@en ;
    skos:inScheme onem2m:scheme ;
    skos:prefLabel "waterFlow"@en ;
    skos:related haim:waterFlowStrength ;
    prov:wasDerivedFrom <https://git.onem2m.org/MAS/Home-Appliances/-/raw/master/3.7.0/SDT-TS0023-ModuleClasses.xml> .

haim:waterSensor a skos:Concept,
        ontolex:LexicalConcept ;
    skos:broader onem2m:Module ;
    skos:definition "This ModuleClass provides the capabilities to indicate whether or not water has been sensed, and raising an alarm if the triggering criterion is met."@en ;
    skos:inScheme onem2m:scheme ;
    skos:prefLabel "waterSensor"@en ;
    skos:related haim:alarm ;
    prov:wasDerivedFrom <https://git.onem2m.org/MAS/Home-Appliances/-/raw/master/3.7.0/SDT-TS0023-ModuleClasses.xml> .

haim:absoluteEnergyConsumption a skos:Concept,
        ontolex:LexicalConcept ;
    skos:broader onem2m:DataPoint ;
    skos:definition "The absolute energy consumption, reflecting the real measurement of accumulative energy. The unit of measure is Watt-hour (Wh)."@en ;
    skos:inScheme onem2m:scheme ;
    skos:prefLabel "absoluteEnergyConsumption"@en .

haim:absoluteStartTime a skos:Concept,
        ontolex:LexicalConcept ;
    skos:broader onem2m:DataPoint ;
    skos:definition "An absolute time to specify the start time."@en ;
    skos:inScheme onem2m:scheme ;
    skos:prefLabel "absoluteStartTime"@en .

haim:absoluteStopTime a skos:Concept,
        ontolex:LexicalConcept ;
    skos:broader onem2m:DataPoint ;
    skos:definition "An absolute time to specify the stop time."@en ;
    skos:inScheme onem2m:scheme ;
    skos:prefLabel "absoluteStopTime"@en .

haim:acousticSensor a skos:Concept,
        ontolex:LexicalConcept ;
    skos:broader onem2m:Module ;
    skos:definition "This ModuleClass provides capabilities for an acoustic sensor."@en ;
    skos:inScheme onem2m:scheme ;
    skos:prefLabel "acousticSensor"@en ;
    skos:related haim:acousticStatus,
        haim:loudness ;
    prov:wasDerivedFrom <https://git.onem2m.org/MAS/Home-Appliances/-/raw/master/3.7.0/SDT-TS0023-ModuleClasses.xml> .

haim:acousticStatus a skos:Concept,
        ontolex:LexicalConcept ;
    skos:broader onem2m:DataPoint ;
    skos:definition "The acousticStatus is expressed in percent, whereas a value of 0 means \"no sound\" and a value of 100 means \"most noisy\"."@en ;
    skos:inScheme onem2m:scheme ;
    skos:prefLabel "acousticStatus"@en .

haim:activateClockTimer a skos:Concept,
        ontolex:LexicalConcept ;
    skos:broader onem2m:Action ;
    skos:definition "Activate current clock timer."@en ;
    skos:inScheme onem2m:scheme ;
    skos:prefLabel "activateClockTimer"@en .

haim:adfStates a skos:Concept,
        ontolex:LexicalConcept ;
    skos:broader onem2m:DataPoint ;
    skos:definition "List of possible ADF states that are supported by the device (see clause 5.6.2)."@en ;
    skos:inScheme onem2m:scheme ;
    skos:prefLabel "adfStates"@en .

haim:airConJobMode a skos:Concept,
        ontolex:LexicalConcept ;
    skos:broader onem2m:Module ;
    skos:definition "This ModuleClasses provides capabilities to control and monitor the job modes of an air conditioner."@en ;
    skos:inScheme onem2m:scheme ;
    skos:prefLabel "airConJobMode"@en ;
    skos:related haim:currentJobMode,
        haim:currentJobModeName,
        haim:jobModes ;
    prov:wasDerivedFrom <https://git.onem2m.org/MAS/Home-Appliances/-/raw/master/3.7.0/SDT-TS0023-ModuleClasses.xml> .

haim:airPurifierJobMode a skos:Concept,
        ontolex:LexicalConcept ;
    skos:broader onem2m:Module ;
    skos:definition "This ModuleClasses provides capabilities to control and monitor the job modes of an airPurifier."@en ;
    skos:inScheme onem2m:scheme ;
    skos:prefLabel "airPurifierJobMode"@en ;
    skos:related haim:currentJobMode,
        haim:currentJobModeName,
        haim:jobModes ;
    prov:wasDerivedFrom <https://git.onem2m.org/MAS/Home-Appliances/-/raw/master/3.7.0/SDT-TS0023-ModuleClasses.xml> .

haim:alarmSpeaker a skos:Concept,
        ontolex:LexicalConcept ;
    skos:broader onem2m:Module ;
    skos:definition "This ModuleClass provides the capabilites to initiate and monitor an alarm."@en ;
    skos:inScheme onem2m:scheme ;
    skos:prefLabel "alarmSpeaker"@en ;
    skos:related haim:alarmStatus,
        haim:light,
        haim:tone ;
    prov:wasDerivedFrom <https://git.onem2m.org/MAS/Home-Appliances/-/raw/master/3.7.0/SDT-TS0023-ModuleClasses.xml> .

haim:alarmStatus a skos:Concept,
        ontolex:LexicalConcept ;
    skos:broader onem2m:DataPoint ;
    skos:definition "\"True\" indicates the alarm start while \"False\" indicates the alarm stop."@en ;
    skos:inScheme onem2m:scheme ;
    skos:prefLabel "alarmStatus"@en .

haim:altitude a skos:Concept,
        ontolex:LexicalConcept ;
    skos:broader onem2m:DataPoint ;
    skos:definition "The optional current altitude part of a geo-location. The unit of measures is meters."@en ;
    skos:inScheme onem2m:scheme ;
    skos:prefLabel "altitude"@en .

haim:answer a skos:Concept,
        ontolex:LexicalConcept ;
    skos:broader onem2m:Action ;
    skos:definition "Answer (pickup) an incoming call."@en ;
    skos:inScheme onem2m:scheme ;
    skos:prefLabel "answer"@en .

haim:automode a skos:Concept,
        ontolex:LexicalConcept ;
    skos:broader onem2m:DataPoint ;
    skos:definition "Status of the automode feature. \"True\" indicates that the speed is set by the device, \"False\" indicates that the device is not controlling the speed."@en ;
    skos:inScheme onem2m:scheme ;
    skos:prefLabel "automode"@en .

haim:availableChannels a skos:Concept,
        ontolex:LexicalConcept ;
    skos:broader onem2m:DataPoint ;
    skos:definition "The list of available channel numbers which may be built by automatic scan and/or manual selection."@en ;
    skos:inScheme onem2m:scheme ;
    skos:prefLabel "availableChannels"@en .

haim:basalMetabolism a skos:Concept,
        ontolex:LexicalConcept ;
    skos:broader onem2m:DataPoint ;
    skos:definition "The measurement of muscle mass by a weight scale and a body composition analyser. The unit of measure is kilogram (kg)."@en ;
    skos:inScheme onem2m:scheme ;
    skos:prefLabel "basalMetabolism"@en .

haim:bath a skos:Concept,
        ontolex:LexicalConcept ;
    skos:broader onem2m:DataPoint ;
    skos:definition "The status of whether a bath tub is filled."@en ;
    skos:inScheme onem2m:scheme ;
    skos:prefLabel "bath"@en .

haim:batteryThreshold a skos:Concept,
        ontolex:LexicalConcept ;
    skos:broader onem2m:DataPoint ;
    skos:definition "When a battery’s \"level\" is less than \"batteryThreshold\" then the \"lowBattery\" is \"true\". This datapoint can be used to raise an alarm, depending on the implementation."@en ;
    skos:inScheme onem2m:scheme ;
    skos:prefLabel "batteryThreshold"@en .

haim:bioElectricalImpedanceAnalysis a skos:Concept,
        ontolex:LexicalConcept ;
    skos:broader onem2m:Module ;
    skos:definition "This ModuleClass provides the analysis of human body tissue based on impedance measurement."@en ;
    skos:inScheme onem2m:scheme ;
    skos:prefLabel "bioElectricalImpedanceAnalysis"@en ;
    skos:related haim:bone,
        haim:fat,
        haim:kcal,
        haim:muscle,
        haim:resistance,
        haim:visceraFat,
        haim:water ;
    prov:wasDerivedFrom <https://git.onem2m.org/MAS/Home-Appliances/-/raw/master/3.7.0/SDT-TS0023-ModuleClasses.xml> .

haim:blue a skos:Concept,
        ontolex:LexicalConcept ;
    skos:broader onem2m:DataPoint ;
    skos:definition "TThe value of the Blue colour channel of RGB. The range is [0,255]."@en ;
    skos:inScheme onem2m:scheme ;
    skos:prefLabel "blue"@en .

haim:bmi a skos:Concept,
        ontolex:LexicalConcept ;
    skos:broader onem2m:DataPoint ;
    skos:definition "The measurement of Body Mass Index (BMI) by a weight scale and a body composition analyser. The unit of measure is kg/m^2."@en ;
    skos:inScheme onem2m:scheme ;
    skos:prefLabel "bmi"@en .

haim:bodyCompositionAnalyser a skos:Concept,
        ontolex:LexicalConcept ;
    skos:broader onem2m:Module ;
    skos:definition "This ModuleClass provides the capability to report the measurement of a body composition analyser."@en ;
    skos:inScheme onem2m:scheme ;
    skos:prefLabel "bodyCompositionAnalyser"@en ;
    skos:related haim:basalMetabolism,
        haim:bmi,
        haim:bodyLength,
        haim:fatFreeMass,
        haim:impedance,
        haim:muscleMass,
        haim:softLeanMass ;
    prov:wasDerivedFrom <https://git.onem2m.org/MAS/Home-Appliances/-/raw/master/3.7.0/SDT-TS0023-ModuleClasses.xml> .

haim:bodyLength a skos:Concept,
        ontolex:LexicalConcept ;
    skos:broader onem2m:DataPoint ;
    skos:definition "The measurement of body length by Weight scale and Body composition analyser. The unit of measure is centimetre(cm).."@en ;
    skos:inScheme onem2m:scheme ;
    skos:prefLabel "bodyLength"@en .

haim:boiler a skos:Concept,
        ontolex:LexicalConcept ;
    skos:broader onem2m:Module ;
    skos:definition "This ModuleClass provides the capabilities to control the status of the boiling functionality for water heaters."@en ;
    skos:inScheme onem2m:scheme ;
    skos:prefLabel "boiler"@en ;
    skos:related haim:status ;
    prov:wasDerivedFrom <https://git.onem2m.org/MAS/Home-Appliances/-/raw/master/3.7.0/SDT-TS0023-ModuleClasses.xml> .

haim:bone a skos:Concept,
        ontolex:LexicalConcept ;
    skos:broader onem2m:DataPoint ;
    skos:definition "The bone content measurement from the BIA The unit of measure is percentage."@en ;
    skos:inScheme onem2m:scheme ;
    skos:prefLabel "bone"@en .

haim:brewing a skos:Concept,
        ontolex:LexicalConcept ;
    skos:broader onem2m:Module ;
    skos:definition "This ModuleClass provides capabilities to control and monitor a brewing process. It is intended to be part of devices that prepare hot drinks such as a coffee or a tea."@en ;
    skos:inScheme onem2m:scheme ;
    skos:prefLabel "brewing"@en ;
    skos:related haim:cupsNumber,
        haim:strength ;
    prov:wasDerivedFrom <https://git.onem2m.org/MAS/Home-Appliances/-/raw/master/3.7.0/SDT-TS0023-ModuleClasses.xml> .

haim:call a skos:Concept,
        ontolex:LexicalConcept ;
    skos:broader onem2m:Action ;
    skos:definition "Initiate an outgoing call."@en ;
    skos:inScheme onem2m:scheme ;
    skos:prefLabel "call"@en .

haim:callState a skos:Concept,
        ontolex:LexicalConcept ;
    skos:broader onem2m:DataPoint ;
    skos:definition "This data point represents the current state of an associated phone device regarding calls."@en ;
    skos:inScheme onem2m:scheme ;
    skos:prefLabel "callState"@en .

haim:callerID a skos:Concept,
        ontolex:LexicalConcept ;
    skos:broader onem2m:DataPoint ;
    skos:definition "This data point represents the initiating caller identiﬁcation of a call. In case of an outgoing call this would be the local line ID. This data point is optional. When it is empty for an incoming call, then the caller ID is unknown. When it is empty for an outgoing call, then it is expected that it is set by the PBX or the operator. The format of caller ID is not speciﬁed here."@en ;
    skos:inScheme onem2m:scheme ;
    skos:prefLabel "callerID"@en .

haim:capacity a skos:Concept,
        ontolex:LexicalConcept ;
    skos:broader onem2m:DataPoint ;
    skos:definition "The total capacity of a battery in mAh."@en ;
    skos:inScheme onem2m:scheme ;
    skos:prefLabel "capacity"@en .

haim:ch2o a skos:Concept,
        ontolex:LexicalConcept ;
    skos:broader onem2m:DataPoint ;
    skos:definition "This value indicates the CH2O level in ppm."@en ;
    skos:inScheme onem2m:scheme ;
    skos:prefLabel "ch2o"@en .

haim:channelId a skos:Concept,
        ontolex:LexicalConcept ;
    skos:broader onem2m:DataPoint ;
    skos:definition "Current channel number."@en ;
    skos:inScheme onem2m:scheme ;
    skos:prefLabel "channelId"@en .

haim:channelName a skos:Concept,
        ontolex:LexicalConcept ;
    skos:broader onem2m:DataPoint ;
    skos:definition "Current human-friendly channel name in string, for example ‘CNN’."@en ;
    skos:inScheme onem2m:scheme ;
    skos:prefLabel "channelName"@en .

haim:charging a skos:Concept,
        ontolex:LexicalConcept ;
    skos:broader onem2m:DataPoint ;
    skos:definition "The status of charging. \"True\" indicates charging, and \"False\" indicates not charging."@en ;
    skos:inScheme onem2m:scheme ;
    skos:prefLabel "charging"@en .

haim:chargingCapacity a skos:Concept,
        ontolex:LexicalConcept ;
    skos:broader onem2m:DataPoint ;
    skos:definition "Rated charging capacity. The unit of measure is ampere hours."@en ;
    skos:inScheme onem2m:scheme ;
    skos:prefLabel "chargingCapacity"@en .

haim:close a skos:Concept,
        ontolex:LexicalConcept ;
    skos:broader onem2m:Action ;
    skos:definition "Decrease the open level by the amount of the \"stepValue\" down to the \"minLevel\"."@en ;
    skos:inScheme onem2m:scheme ;
    skos:prefLabel "close"@en .

haim:clothesDryerJobMode a skos:Concept,
        ontolex:LexicalConcept ;
    skos:broader onem2m:Module ;
    skos:definition "This ModuleClasses provides capabilities to control and monitor the job modes of a clothes dryer."@en ;
    skos:inScheme onem2m:scheme ;
    skos:prefLabel "clothesDryerJobMode"@en ;
    skos:related haim:currentJobMode,
        haim:currentJobModeName ;
    prov:wasDerivedFrom <https://git.onem2m.org/MAS/Home-Appliances/-/raw/master/3.7.0/SDT-TS0023-ModuleClasses.xml> .

haim:clothesWasherDryerJobMode a skos:Concept,
        ontolex:LexicalConcept ;
    skos:broader onem2m:Module ;
    skos:definition "This ModuleClasses provides capabilities to control and monitor the job modes of clothesWasherDryer."@en ;
    skos:inScheme onem2m:scheme ;
    skos:prefLabel "clothesWasherDryerJobMode"@en ;
    skos:related haim:currentJobMode,
        haim:currentJobModeName,
        haim:jobModes ;
    prov:wasDerivedFrom <https://git.onem2m.org/MAS/Home-Appliances/-/raw/master/3.7.0/SDT-TS0023-ModuleClasses.xml> .

haim:clothesWasherJobMode a skos:Concept,
        ontolex:LexicalConcept ;
    skos:broader onem2m:Module ;
    skos:definition "This ModuleClasses provides capabilities to control and monitor the job mode of a washer."@en ;
    skos:inScheme onem2m:scheme ;
    skos:prefLabel "clothesWasherJobMode"@en ;
    skos:related haim:currentJobMode,
        haim:currentJobModeName,
        haim:jobModes ;
    prov:wasDerivedFrom <https://git.onem2m.org/MAS/Home-Appliances/-/raw/master/3.7.0/SDT-TS0023-ModuleClasses.xml> .

haim:co a skos:Concept,
        ontolex:LexicalConcept ;
    skos:broader onem2m:DataPoint ;
    skos:definition "This value indicates the CO level in ppm.."@en ;
    skos:inScheme onem2m:scheme ;
    skos:prefLabel "co"@en .

haim:co2 a skos:Concept,
        ontolex:LexicalConcept ;
    skos:broader onem2m:DataPoint ;
    skos:definition "This value indicates the CO2 level in ppm (parts per million)."@en ;
    skos:inScheme onem2m:scheme ;
    skos:prefLabel "co2"@en .

haim:coarseness a skos:Concept,
        ontolex:LexicalConcept ;
    skos:broader onem2m:DataPoint ;
    skos:definition "The wished coarseness of the solid supplies after grinding, for example for coffee beans (see clause 5.6.16)."@en ;
    skos:inScheme onem2m:scheme ;
    skos:prefLabel "coarseness"@en .

haim:coldWash a skos:Concept,
        ontolex:LexicalConcept ;
    skos:broader onem2m:DataPoint ;
    skos:definition "This data point indicates cold wash. \"True\" indicates enabled, \"False\" indicates disabled."@en ;
    skos:inScheme onem2m:scheme ;
    skos:prefLabel "coldWash"@en .

haim:colour a skos:Concept,
        ontolex:LexicalConcept ;
    skos:broader onem2m:Module ;
    skos:definition "This ModuleClass provides the capabilities to set the value of the Red, Green, and Blue colour channels for a colour device."@en ;
    skos:inScheme onem2m:scheme ;
    skos:prefLabel "colour"@en ;
    skos:related haim:blue,
        haim:green,
        haim:red ;
    prov:wasDerivedFrom <https://git.onem2m.org/MAS/Home-Appliances/-/raw/master/3.7.0/SDT-TS0023-ModuleClasses.xml> .

haim:concentration a skos:Concept,
        ontolex:LexicalConcept ;
    skos:broader onem2m:DataPoint ;
    skos:definition "The measurement of concentration by Glucometer. The unit of measure is mg/dl."@en ;
    skos:inScheme onem2m:scheme ;
    skos:prefLabel "concentration"@en .

haim:contextCarbohydratesAmount a skos:Concept,
        ontolex:LexicalConcept ;
    skos:broader onem2m:DataPoint ;
    skos:definition "The measurement of context carbohydrates by Glucometer. The unit of measure is gram (g)."@en ;
    skos:inScheme onem2m:scheme ;
    skos:prefLabel "contextCarbohydratesAmount"@en .

haim:contextCarbohydratesSource a skos:Concept,
        ontolex:LexicalConcept ;
    skos:broader onem2m:DataPoint ;
    skos:definition "The timing of meals (for example \"breakfast carbohydrates\")."@en ;
    skos:inScheme onem2m:scheme ;
    skos:prefLabel "contextCarbohydratesSource"@en .

haim:contextExercise a skos:Concept,
        ontolex:LexicalConcept ;
    skos:broader onem2m:DataPoint ;
    skos:definition "The measurement of context exercise by Glucometer. The unit of measure is percentage."@en ;
    skos:inScheme onem2m:scheme ;
    skos:prefLabel "contextExercise"@en .

haim:contextHealth a skos:Concept,
        ontolex:LexicalConcept ;
    skos:broader onem2m:DataPoint ;
    skos:definition "The severity of symptoms (for example \"minor\"),"@en ;
    skos:inScheme onem2m:scheme ;
    skos:prefLabel "contextHealth"@en .

haim:contextLocation a skos:Concept,
        ontolex:LexicalConcept ;
    skos:broader onem2m:DataPoint ;
    skos:definition "The body location where the Glucometer is worn (for example \"finger\")."@en ;
    skos:inScheme onem2m:scheme ;
    skos:prefLabel "contextLocation"@en .

haim:contextMeal a skos:Concept,
        ontolex:LexicalConcept ;
    skos:broader onem2m:DataPoint ;
    skos:definition "The style of meals (for example \"casual\")."@en ;
    skos:inScheme onem2m:scheme ;
    skos:prefLabel "contextMeal"@en .

haim:contextMedication a skos:Concept,
        ontolex:LexicalConcept ;
    skos:broader onem2m:DataPoint ;
    skos:definition "The measurement of context medication by Glucometer. The unit of measure is mg/dl."@en ;
    skos:inScheme onem2m:scheme ;
    skos:prefLabel "contextMedication"@en .

haim:contextTester a skos:Concept,
        ontolex:LexicalConcept ;
    skos:broader onem2m:DataPoint ;
    skos:definition "The test style (for example \"self\")."@en ;
    skos:inScheme onem2m:scheme ;
    skos:prefLabel "contextTester"@en .

haim:cookerHoodJobMode a skos:Concept,
        ontolex:LexicalConcept ;
    skos:broader onem2m:Module ;
    skos:definition "This ModuleClasses provides capabilities to control and monitor the job modes of a cookerHood."@en ;
    skos:inScheme onem2m:scheme ;
    skos:prefLabel "cookerHoodJobMode"@en ;
    skos:related haim:currentJobMode,
        haim:currentJobModeName,
        haim:jobModes ;
    prov:wasDerivedFrom <https://git.onem2m.org/MAS/Home-Appliances/-/raw/master/3.7.0/SDT-TS0023-ModuleClasses.xml> .

haim:cupsNumber a skos:Concept,
        ontolex:LexicalConcept ;
    skos:broader onem2m:DataPoint ;
    skos:definition "The current number of the cups requested to brew."@en ;
    skos:inScheme onem2m:scheme ;
    skos:prefLabel "cupsNumber"@en .

haim:current a skos:Concept,
        ontolex:LexicalConcept ;
    skos:broader onem2m:DataPoint ;
    skos:definition "The current of the device. The unit of measure is ampere (A)."@en ;
    skos:inScheme onem2m:scheme ;
    skos:prefLabel "current"@en .

haim:currentAdfState a skos:Concept,
        ontolex:LexicalConcept ;
    skos:broader onem2m:DataPoint ;
    skos:definition "Current state of the ADF."@en ;
    skos:inScheme onem2m:scheme ;
    skos:prefLabel "currentAdfState"@en .

haim:currentDate a skos:Concept,
        ontolex:LexicalConcept ;
    skos:broader onem2m:DataPoint ;
    skos:definition "Information of the current date."@en ;
    skos:inScheme onem2m:scheme ;
    skos:prefLabel "currentDate"@en .

haim:currentJobState a skos:Concept,
        ontolex:LexicalConcept ;
    skos:broader onem2m:DataPoint ;
    skos:definition "The currently active job state at the level of some transaction being executed by the device (see clause 5.6.18)."@en ;
    skos:inScheme onem2m:scheme ;
    skos:prefLabel "currentJobState"@en .

haim:currentMachineState a skos:Concept,
        ontolex:LexicalConcept ;
    skos:broader onem2m:DataPoint ;
    skos:definition "The currently active machine state (see clause 5.6.20)."@en ;
    skos:inScheme onem2m:scheme ;
    skos:prefLabel "currentMachineState"@en .

haim:currentPlayerMode a skos:Concept,
        ontolex:LexicalConcept ;
    skos:broader onem2m:DataPoint ;
    skos:definition "The current mode of the player."@en ;
    skos:inScheme onem2m:scheme ;
    skos:prefLabel "currentPlayerMode"@en .

haim:currentPlayerModeName a skos:Concept,
        ontolex:LexicalConcept ;
    skos:broader onem2m:DataPoint ;
    skos:definition "Name of current player mode in string. This can be used when \"currentPlayerMode\" is vendor-specific."@en ;
    skos:inScheme onem2m:scheme ;
    skos:prefLabel "currentPlayerModeName"@en .

haim:currentSecurityMode a skos:Concept,
        ontolex:LexicalConcept ;
    skos:broader onem2m:DataPoint ;
    skos:definition "Current security mode (see clause 5.6.24)."@en ;
    skos:inScheme onem2m:scheme ;
    skos:prefLabel "currentSecurityMode"@en .

haim:currentTemperature a skos:Concept,
        ontolex:LexicalConcept ;
    skos:broader onem2m:DataPoint ;
    skos:definition "The current temperature."@en ;
    skos:inScheme onem2m:scheme ;
    skos:prefLabel "currentTemperature"@en .

haim:currentTime a skos:Concept,
        ontolex:LexicalConcept ;
    skos:broader onem2m:DataPoint ;
    skos:definition "Information of the current time."@en ;
    skos:inScheme onem2m:scheme ;
    skos:prefLabel "currentTime"@en .

haim:currentTimeZone a skos:Concept,
        ontolex:LexicalConcept ;
    skos:broader onem2m:DataPoint ;
    skos:definition "Name of current time zone according to the IANA Timezone data format (TZ), for example, \"America/New York\". "@en ;
    skos:inScheme onem2m:scheme ;
    skos:prefLabel "currentTimeZone"@en .

haim:currentValue a skos:Concept,
        ontolex:LexicalConcept ;
    skos:broader onem2m:DataPoint ;
    skos:definition "The current data value of the smoke sensor."@en ;
    skos:inScheme onem2m:scheme ;
    skos:prefLabel "currentValue"@en .

haim:deactivateClockTimer a skos:Concept,
        ontolex:LexicalConcept ;
    skos:broader onem2m:Action ;
    skos:definition "Deactivate current clock timer."@en ;
    skos:inScheme onem2m:scheme ;
    skos:prefLabel "deactivateClockTimer"@en .

haim:decrementNumberValue a skos:Concept,
        ontolex:LexicalConcept ;
    skos:broader onem2m:Action ;
    skos:definition "Decrement the \"numberValue\" by the value of \"step\", down to the value of \"minimum\"."@en ;
    skos:inScheme onem2m:scheme ;
    skos:prefLabel "decrementNumberValue"@en .

haim:defrost a skos:Concept,
        ontolex:LexicalConcept ;
    skos:broader onem2m:DataPoint ;
    skos:definition "Controls the defrost cycle. \"True\" indicates active, \"False\" indicates inactive."@en ;
    skos:inScheme onem2m:scheme ;
    skos:prefLabel "defrost"@en .

haim:dehumidifierJobMode a skos:Concept,
        ontolex:LexicalConcept ;
    skos:broader onem2m:Module ;
    skos:definition "This ModuleClasses provides capabilities to control and monitor the job modes of a dehumidifier device."@en ;
    skos:inScheme onem2m:scheme ;
    skos:prefLabel "dehumidifierJobMode"@en ;
    skos:related haim:currentJobMode,
        haim:currentJobModeName,
        haim:jobModes ;
    prov:wasDerivedFrom <https://git.onem2m.org/MAS/Home-Appliances/-/raw/master/3.7.0/SDT-TS0023-ModuleClasses.xml> .

haim:description a skos:Concept,
        ontolex:LexicalConcept ;
    skos:broader onem2m:DataPoint ;
    skos:definition "The message representation of the fault."@en ;
    skos:inScheme onem2m:scheme ;
    skos:prefLabel "description"@en .

haim:desiredHumidity a skos:Concept,
        ontolex:LexicalConcept ;
    skos:broader onem2m:DataPoint ;
    skos:definition "Desired value for humidity. This data point indicates the desired humidity."@en ;
    skos:inScheme onem2m:scheme ;
    skos:prefLabel "desiredHumidity"@en .

haim:diastolicPressure a skos:Concept,
        ontolex:LexicalConcept ;
    skos:broader onem2m:DataPoint ;
    skos:definition "The measurement of diastolic pressure by sphygmomanometer. The unit of measure is millimetre of mercury (mmHg)."@en ;
    skos:inScheme onem2m:scheme ;
    skos:prefLabel "diastolicPressure"@en .

haim:discharging a skos:Concept,
        ontolex:LexicalConcept ;
    skos:broader onem2m:DataPoint ;
    skos:definition "The status of discharging. \"True\" indicates discharging, and \"False\" indicates not discharging."@en ;
    skos:inScheme onem2m:scheme ;
    skos:prefLabel "discharging"@en .

haim:dischargingCapacity a skos:Concept,
        ontolex:LexicalConcept ;
    skos:broader onem2m:DataPoint ;
    skos:definition "Rated discharging capacity."@en ;
    skos:inScheme onem2m:scheme ;
    skos:prefLabel "dischargingCapacity"@en .

haim:dishWasherJobMode a skos:Concept,
        ontolex:LexicalConcept ;
    skos:broader onem2m:Module ;
    skos:definition "This ModuleClasses provides capabilities to control and monitor the job modes of a dishWasher."@en ;
    skos:inScheme onem2m:scheme ;
    skos:prefLabel "dishWasherJobMode"@en ;
    skos:related haim:currentJobMode,
        haim:currentJobModeName,
        haim:jobModes ;
    prov:wasDerivedFrom <https://git.onem2m.org/MAS/Home-Appliances/-/raw/master/3.7.0/SDT-TS0023-ModuleClasses.xml> .

haim:doorState a skos:Concept,
        ontolex:LexicalConcept ;
    skos:broader onem2m:DataPoint ;
    skos:definition "Current state of the door "@en ;
    skos:inScheme onem2m:scheme ;
    skos:prefLabel "doorState"@en .

haim:downChannel a skos:Concept,
        ontolex:LexicalConcept ;
    skos:broader onem2m:Action ;
    skos:definition "Change the current channel to the previous channel in the stored list of available channels. If the current channel is the first one in the list, the new set channel may be the last one in the list."@en ;
    skos:inScheme onem2m:scheme ;
    skos:prefLabel "downChannel"@en .

haim:downVolume a skos:Concept,
        ontolex:LexicalConcept ;
    skos:broader onem2m:Action ;
    skos:definition "Decrease volume by the amount of the stepValue down to 0."@en ;
    skos:inScheme onem2m:scheme ;
    skos:prefLabel "downVolume"@en .

haim:electricEnergy a skos:Concept,
        ontolex:LexicalConcept ;
    skos:broader onem2m:DataPoint ;
    skos:definition "Rated electric energy. The unit of measure is ampere (A)."@en ;
    skos:inScheme onem2m:scheme ;
    skos:prefLabel "electricEnergy"@en .

haim:electricVehicleConnector a skos:Concept,
        ontolex:LexicalConcept ;
    skos:broader onem2m:Module ;
    skos:definition "This ModuleClass provides information about charging/discharging devices for electric vehicles."@en ;
    skos:inScheme onem2m:scheme ;
    skos:prefLabel "electricVehicleConnector"@en ;
    skos:related haim:chargingCapacity,
        haim:dischargingCapacity,
        haim:status ;
    prov:wasDerivedFrom <https://git.onem2m.org/MAS/Home-Appliances/-/raw/master/3.7.0/SDT-TS0023-ModuleClasses.xml> .

haim:energy a skos:Concept,
        ontolex:LexicalConcept ;
    skos:broader onem2m:DataPoint ;
    skos:definition "The measurement of energy by pulsemeter. The unit of measure is kilocalorie per hour."@en ;
    skos:inScheme onem2m:scheme ;
    skos:prefLabel "energy"@en .

haim:estimatedTimeToEnd a skos:Concept,
        ontolex:LexicalConcept ;
    skos:broader onem2m:DataPoint ;
    skos:definition "A timer (for example a time-based value, App Defined Epoch, Progressive) expressed in seconds. The value indicates the time to the end of an appliance’s operations. It is calculated at runtime by the device itself during the execution of its operation."@en ;
    skos:inScheme onem2m:scheme ;
    skos:prefLabel "estimatedTimeToEnd"@en .

haim:extraRinse a skos:Concept,
        ontolex:LexicalConcept ;
    skos:broader onem2m:DataPoint ;
    skos:definition "This data point indicates extra rinse. \"True\" indicates enabled, \"False\" indicates disabled."@en ;
    skos:inScheme onem2m:scheme ;
    skos:prefLabel "extraRinse"@en .

haim:fat a skos:Concept,
        ontolex:LexicalConcept ;
    skos:broader onem2m:DataPoint ;
    skos:definition "The fat content measurement from the BIAT he unit of measure is percentage."@en ;
    skos:inScheme onem2m:scheme ;
    skos:prefLabel "fat"@en .

haim:fatFreeMass a skos:Concept,
        ontolex:LexicalConcept ;
    skos:broader onem2m:DataPoint ;
    skos:definition "The measurement of fat free mass by a Weight scale and a Body composition analyser. The unit of measure is kilogram (kg)."@en ;
    skos:inScheme onem2m:scheme ;
    skos:prefLabel "fatFreeMass"@en .

haim:filterLifetime a skos:Concept,
        ontolex:LexicalConcept ;
    skos:broader onem2m:DataPoint ;
    skos:definition "Percentage life time remaining for the water filter."@en ;
    skos:inScheme onem2m:scheme ;
    skos:prefLabel "filterLifetime"@en .

haim:foaming a skos:Concept,
        ontolex:LexicalConcept ;
    skos:broader onem2m:Module ;
    skos:definition "This ModuleClass provides capabilities to control and monitor desired parameters of foam e.g. for foaming milk. It is initially intended to be part of a device that prepare drinks with milk (for example a coffee machine or hot chocolate machine)."@en ;
    skos:inScheme onem2m:scheme ;
    skos:prefLabel "foaming"@en ;
    skos:related haim:foamingStrength ;
    prov:wasDerivedFrom <https://git.onem2m.org/MAS/Home-Appliances/-/raw/master/3.7.0/SDT-TS0023-ModuleClasses.xml> .

haim:foamingStrength a skos:Concept,
        ontolex:LexicalConcept ;
    skos:broader onem2m:DataPoint ;
    skos:definition "The current strength of foamed milk. A higher value indicates more foamed milk (see clause 5.6.11)."@en ;
    skos:inScheme onem2m:scheme ;
    skos:prefLabel "foamingStrength"@en .

haim:frequency a skos:Concept,
        ontolex:LexicalConcept ;
    skos:broader onem2m:DataPoint ;
    skos:definition "The frequency of the device. The unit of measure is hertz (Hz)."@en ;
    skos:inScheme onem2m:scheme ;
    skos:prefLabel "frequency"@en .

haim:generationSource a skos:Concept,
        ontolex:LexicalConcept ;
    skos:broader onem2m:DataPoint ;
    skos:definition "The type of generating source."@en ;
    skos:inScheme onem2m:scheme ;
    skos:prefLabel "generationSource"@en .

haim:glucometer a skos:Concept,
        ontolex:LexicalConcept ;
    skos:broader onem2m:Module ;
    skos:definition "This ModuleClass provides the capability to report the measurement of glucose characteristics."@en ;
    skos:inScheme onem2m:scheme ;
    skos:prefLabel "glucometer"@en ;
    skos:related haim:concentration,
        haim:contextCarbohydratesAmount,
        haim:contextCarbohydratesSource,
        haim:contextExercise,
        haim:contextHealth,
        haim:contextLocation,
        haim:contextMeal,
        haim:contextMedication,
        haim:contextTester,
        haim:hba1c ;
    prov:wasDerivedFrom <https://git.onem2m.org/MAS/Home-Appliances/-/raw/master/3.7.0/SDT-TS0023-ModuleClasses.xml> .

haim:grainsRemaining a skos:Concept,
        ontolex:LexicalConcept ;
    skos:broader onem2m:DataPoint ;
    skos:definition "The level of remaining grains in a machine having a grinder, for example for remaining coffee beans in the coffee machine grinder (see clause 5.6.15)."@en ;
    skos:inScheme onem2m:scheme ;
    skos:prefLabel "grainsRemaining"@en .

haim:green a skos:Concept,
        ontolex:LexicalConcept ;
    skos:broader onem2m:DataPoint ;
    skos:definition "The value of the Green colour channel of RGB. The range is [0,255]."@en ;
    skos:inScheme onem2m:scheme ;
    skos:prefLabel "green"@en .

haim:grinder a skos:Concept,
        ontolex:LexicalConcept ;
    skos:broader onem2m:Module ;
    skos:definition "This ModuleClass is for controlling a grinder, for example in a coffee machine."@en ;
    skos:inScheme onem2m:scheme ;
    skos:prefLabel "grinder"@en ;
    skos:related haim:coarseness,
        haim:grainsRemaining,
        haim:useGrinder ;
    prov:wasDerivedFrom <https://git.onem2m.org/MAS/Home-Appliances/-/raw/master/3.7.0/SDT-TS0023-ModuleClasses.xml> .

haim:hangup a skos:Concept,
        ontolex:LexicalConcept ;
    skos:broader onem2m:Action ;
    skos:definition "Hangup an established call."@en ;
    skos:inScheme onem2m:scheme ;
    skos:prefLabel "hangup"@en .

haim:hash a skos:Concept,
        ontolex:LexicalConcept ;
    skos:broader onem2m:DataPoint ;
    skos:definition "The hash code of the blob. If present, it is used to check the decoded content of the \"object\" data point for integrity. The algorithm used for generating the hash value is SHA-2. The data point contains the hash as a hex encoded value."@en ;
    skos:inScheme onem2m:scheme ;
    skos:prefLabel "hash"@en .

haim:hba1c a skos:Concept,
        ontolex:LexicalConcept ;
    skos:broader onem2m:DataPoint ;
    skos:definition "The measurement of HbA1c by Glucometer. The unit of measure is percentage."@en ;
    skos:inScheme onem2m:scheme ;
    skos:prefLabel "hba1c"@en .

haim:heading a skos:Concept,
        ontolex:LexicalConcept ;
    skos:broader onem2m:DataPoint ;
    skos:definition "The azimuth of a device measured in degrees to true north. North is 0,0°, east is 90,0°, south is 180,0°, west is 270,0°. A negative value indicates an unknown heading."@en ;
    skos:inScheme onem2m:scheme ;
    skos:prefLabel "heading"@en .

haim:headingAccuracy a skos:Concept,
        ontolex:LexicalConcept ;
    skos:broader onem2m:DataPoint ;
    skos:definition "The optional current maximum deviation between the heading and the true geomagnetic heading. The unit of measures is degrees."@en ;
    skos:inScheme onem2m:scheme ;
    skos:prefLabel "headingAccuracy"@en .

haim:heatingLevel a skos:Concept,
        ontolex:LexicalConcept ;
    skos:broader onem2m:DataPoint ;
    skos:definition "The current heating level of the zone. The value range is from 0 (indicating that the zone is not heating) up to the maxHeatingLevel."@en ;
    skos:inScheme onem2m:scheme ;
    skos:prefLabel "heatingLevel"@en .

haim:heatingZone a skos:Concept,
        ontolex:LexicalConcept ;
    skos:broader onem2m:Module ;
    skos:definition "This ModuleClass provides the capabilities to monitor the status of the heating zone, for example for a cooktop."@en ;
    skos:inScheme onem2m:scheme ;
    skos:prefLabel "heatingZone"@en ;
    skos:related haim:heatingLevel,
        haim:maxHeatingLevel ;
    prov:wasDerivedFrom <https://git.onem2m.org/MAS/Home-Appliances/-/raw/master/3.7.0/SDT-TS0023-ModuleClasses.xml> .

haim:height a skos:Concept,
        ontolex:LexicalConcept ;
    skos:broader onem2m:DataPoint,
        onem2m:Module ;
    skos:definition "The height measurement. The common unit of measure is meter (m)."@en,
        "This ModuleClass provides the capability to report the measurement of height."@en ;
    skos:inScheme onem2m:scheme ;
    skos:prefLabel "height"@en ;
    skos:related haim:height ;
    prov:wasDerivedFrom <https://git.onem2m.org/MAS/Home-Appliances/-/raw/master/3.7.0/SDT-TS0023-ModuleClasses.xml> .

haim:horizontalAccuracy a skos:Concept,
        ontolex:LexicalConcept ;
    skos:broader onem2m:DataPoint ;
    skos:definition "The optional current horizontal accuracy of the geo-location. The unit of measures is meters and describes a radius around the latitude/longitude coordinate."@en ;
    skos:inScheme onem2m:scheme ;
    skos:prefLabel "horizontalAccuracy"@en .

haim:horizontalDirection a skos:Concept,
        ontolex:LexicalConcept ;
    skos:broader onem2m:DataPoint ;
    skos:definition "The horizontal direction of the air flow (see clause 5.6.17)."@en ;
    skos:inScheme onem2m:scheme ;
    skos:prefLabel "horizontalDirection"@en .

haim:hotWaterSupply a skos:Concept,
        ontolex:LexicalConcept ;
    skos:broader onem2m:Module ;
    skos:definition "This ModuleClass provides the information about the status of supplying hot water into tanks or bath tubes."@en ;
    skos:inScheme onem2m:scheme ;
    skos:prefLabel "hotWaterSupply"@en ;
    skos:related haim:bath ;
    prov:wasDerivedFrom <https://git.onem2m.org/MAS/Home-Appliances/-/raw/master/3.7.0/SDT-TS0023-ModuleClasses.xml> .

haim:impactDirectionHorizontal a skos:Concept,
        ontolex:LexicalConcept ;
    skos:broader onem2m:DataPoint ;
    skos:definition "The \"impactDirection\" indicates the horizontal direction where the impact comes from. The value is 0° to 360°. 0 is the front of the sensor and with clockwise increment."@en ;
    skos:inScheme onem2m:scheme ;
    skos:prefLabel "impactDirectionHorizontal"@en .

haim:impactDirectionVertical a skos:Concept,
        ontolex:LexicalConcept ;
    skos:broader onem2m:DataPoint ;
    skos:definition "The \"impactDirection\" indicates the vertical direction where the impact comes from. The value is 0° to 360°. 0 is the front of the sensor and with upward increment."@en ;
    skos:inScheme onem2m:scheme ;
    skos:prefLabel "impactDirectionVertical"@en .

haim:impactLevel a skos:Concept,
        ontolex:LexicalConcept ;
    skos:broader onem2m:DataPoint ;
    skos:definition "The \"impactLevel\" provides the level of impact. The unit of measure is \"g\" (G-force)."@en ;
    skos:inScheme onem2m:scheme ;
    skos:prefLabel "impactLevel"@en .

haim:impactSensor a skos:Concept,
        ontolex:LexicalConcept ;
    skos:broader onem2m:Module ;
    skos:definition "This ModuleClass describes the capabilities on an impact sensor. The impact is a high force or shock over a short time period and the impactSensor detects this."@en ;
    skos:inScheme onem2m:scheme ;
    skos:prefLabel "impactSensor"@en ;
    skos:related haim:impactDirectionHorizontal,
        haim:impactDirectionVertical,
        haim:impactLevel,
        haim:impactStatus ;
    prov:wasDerivedFrom <https://git.onem2m.org/MAS/Home-Appliances/-/raw/master/3.7.0/SDT-TS0023-ModuleClasses.xml> .

haim:impactStatus a skos:Concept,
        ontolex:LexicalConcept ;
    skos:broader onem2m:DataPoint ;
    skos:definition "The \"impactStatus\" indicates as follows: \"True\" means that a physical impact is detected, \"False\" means indicates a normal status (no impact detected)."@en ;
    skos:inScheme onem2m:scheme ;
    skos:prefLabel "impactStatus"@en .

haim:impedance a skos:Concept,
        ontolex:LexicalConcept ;
    skos:broader onem2m:DataPoint ;
    skos:definition "The measurement of impedance by a weight scale and a body composition analyser. The unit of measure is ohm."@en ;
    skos:inScheme onem2m:scheme ;
    skos:prefLabel "impedance"@en .

haim:incrementNumberValue a skos:Concept,
        ontolex:LexicalConcept ;
    skos:broader onem2m:Action ;
    skos:definition "Increment the \"numberValue\" by the value of \"stepValue\", up to the value of \"maxValue\"."@en ;
    skos:inScheme onem2m:scheme ;
    skos:prefLabel "incrementNumberValue"@en .

haim:jobStates a skos:Concept,
        ontolex:LexicalConcept ;
    skos:broader onem2m:DataPoint ;
    skos:definition "The list of possible job states that the device supports (see clause 5.6.18)."@en ;
    skos:inScheme onem2m:scheme ;
    skos:prefLabel "jobStates"@en .

haim:kcal a skos:Concept,
        ontolex:LexicalConcept ;
    skos:broader onem2m:DataPoint ;
    skos:definition "The kcal (kilocalories) measurement from the BIA."@en ;
    skos:inScheme onem2m:scheme ;
    skos:prefLabel "kcal"@en .

haim:keyNumber a skos:Concept,
        ontolex:LexicalConcept ;
    skos:broader onem2m:DataPoint ;
    skos:definition "The number of key."@en ;
    skos:inScheme onem2m:scheme ;
    skos:prefLabel "keyNumber"@en .

haim:latitude a skos:Concept,
        ontolex:LexicalConcept ;
    skos:broader onem2m:DataPoint ;
    skos:definition "The current latitude part of a geo-location. The unit of measures is degrees."@en ;
    skos:inScheme onem2m:scheme ;
    skos:prefLabel "latitude"@en .

haim:level a skos:Concept,
        ontolex:LexicalConcept ;
    skos:broader onem2m:DataPoint ;
    skos:definition "TThe rounded percentage of the current charging level of a battery in the range of [0, 100]. 0 percentage shall mean that no charge remains."@en ;
    skos:inScheme onem2m:scheme ;
    skos:prefLabel "level"@en .

haim:light a skos:Concept,
        ontolex:LexicalConcept ;
    skos:broader onem2m:DataPoint ;
    skos:definition "Representing the lighting mode of the alarm (see clause 5.6.5)."@en ;
    skos:inScheme onem2m:scheme ;
    skos:prefLabel "light"@en .

haim:loginName a skos:Concept,
        ontolex:LexicalConcept ;
    skos:broader onem2m:DataPoint ;
    skos:definition "The user’s login name."@en ;
    skos:inScheme onem2m:scheme ;
    skos:prefLabel "loginName"@en .

haim:longitude a skos:Concept,
        ontolex:LexicalConcept ;
    skos:broader onem2m:DataPoint ;
    skos:definition "The current longitude part of a geo-location. The unit of measures is degrees."@en ;
    skos:inScheme onem2m:scheme ;
    skos:prefLabel "longitude"@en .

haim:loudness a skos:Concept,
        ontolex:LexicalConcept ;
    skos:broader onem2m:DataPoint ;
    skos:definition "The unit of measure of the loudness is \"dB^2\"."@en ;
    skos:inScheme onem2m:scheme ;
    skos:prefLabel "loudness"@en .

haim:lowBattery a skos:Concept,
        ontolex:LexicalConcept ;
    skos:broader onem2m:DataPoint ;
    skos:definition "To indicate that the battery is in a low charge level."@en ;
    skos:inScheme onem2m:scheme ;
    skos:prefLabel "lowBattery"@en .

haim:lqi a skos:Concept,
        ontolex:LexicalConcept ;
    skos:broader onem2m:DataPoint ;
    skos:definition "The current value of link quality indicator, which reflects the scaling of rssi by dividing the received signal strength over reference signal strength. The common unit for lqi is percentage [0,100]. For the detailed definition, please see IEEE 802.15.4 [i.4], clause 6.7.8."@en ;
    skos:inScheme onem2m:scheme ;
    skos:prefLabel "lqi"@en .

haim:machineStates a skos:Concept,
        ontolex:LexicalConcept ;
    skos:broader onem2m:DataPoint ;
    skos:definition "A list of possible machine states the device supports (see clause 5.6.20)."@en ;
    skos:inScheme onem2m:scheme ;
    skos:prefLabel "machineStates"@en .

haim:material a skos:Concept,
        ontolex:LexicalConcept ;
    skos:broader onem2m:DataPoint ;
    skos:definition "The material of the cell (for example lithium ion, nickel and lead."@en ;
    skos:inScheme onem2m:scheme ;
    skos:prefLabel "material"@en .

haim:maxHeatingLevel a skos:Concept,
        ontolex:LexicalConcept ;
    skos:broader onem2m:DataPoint ;
    skos:definition "The maximum value allowed for the heating level of the zone."@en ;
    skos:inScheme onem2m:scheme ;
    skos:prefLabel "maxHeatingLevel"@en .

haim:maxLength a skos:Concept,
        ontolex:LexicalConcept ;
    skos:broader onem2m:DataPoint ;
    skos:definition "The optional maximum length in characters of the message. The default is unlimited."@en ;
    skos:inScheme onem2m:scheme ;
    skos:prefLabel "maxLength"@en .

haim:maxLevel a skos:Concept,
        ontolex:LexicalConcept ;
    skos:broader onem2m:DataPoint ;
    skos:definition "The maximum value allowed for the \"openLevel\" status. The default value is 100, which means fully opened."@en ;
    skos:inScheme onem2m:scheme ;
    skos:prefLabel "maxLevel"@en .

haim:maxSpeed a skos:Concept,
        ontolex:LexicalConcept ;
    skos:broader onem2m:DataPoint ;
    skos:definition "The maximum value for the speed level. If not present, the default is 100."@en ;
    skos:inScheme onem2m:scheme ;
    skos:prefLabel "maxSpeed"@en .

haim:meanPressure a skos:Concept,
        ontolex:LexicalConcept ;
    skos:broader onem2m:DataPoint ;
    skos:definition "The measurement of mean arterial pressure by sphygmomanometer. The unit of measure is millimetre of mercury (mmHg)."@en ;
    skos:inScheme onem2m:scheme ;
    skos:prefLabel "meanPressure"@en .

haim:measuringScope a skos:Concept,
        ontolex:LexicalConcept ;
    skos:broader onem2m:DataPoint ;
    skos:definition "The measuring scope of the meter, for example the whole house, a room, or a device."@en ;
    skos:inScheme onem2m:scheme ;
    skos:prefLabel "measuringScope"@en .

haim:mediaID a skos:Concept,
        ontolex:LexicalConcept ;
    skos:broader onem2m:DataPoint ;
    skos:definition "The numeric index of the activated media in the supported media sources list \"supportedMediaSources\"."@en ;
    skos:inScheme onem2m:scheme ;
    skos:prefLabel "mediaID"@en .

haim:mediaName a skos:Concept,
        ontolex:LexicalConcept ;
    skos:broader onem2m:DataPoint ;
    skos:definition "Specifies a pre-defined media input or output."@en ;
    skos:inScheme onem2m:scheme ;
    skos:prefLabel "mediaName"@en .

haim:mediaType a skos:Concept,
        ontolex:LexicalConcept ;
    skos:broader onem2m:DataPoint ;
    skos:definition "Specifies the type of the media (see clause 5.6.27)."@en ;
    skos:inScheme onem2m:scheme ;
    skos:prefLabel "mediaType"@en .

haim:memorySize a skos:Concept,
        ontolex:LexicalConcept ;
    skos:broader onem2m:DataPoint ;
    skos:definition "This value represents the total memory size of the printer. The unit of measure is MB(Mega Bytes)."@en ;
    skos:inScheme onem2m:scheme ;
    skos:prefLabel "memorySize"@en .

haim:messageEncoding a skos:Concept,
        ontolex:LexicalConcept ;
    skos:broader onem2m:DataPoint ;
    skos:definition "The optional expected method for character encoding of the message. The default is \"UTF8\"."@en ;
    skos:inScheme onem2m:scheme ;
    skos:prefLabel "messageEncoding"@en .

haim:minLength a skos:Concept,
        ontolex:LexicalConcept ;
    skos:broader onem2m:DataPoint ;
    skos:definition "The optional minimum length in characters of the message. The default is 0."@en ;
    skos:inScheme onem2m:scheme ;
    skos:prefLabel "minLength"@en .

haim:minLevel a skos:Concept,
        ontolex:LexicalConcept ;
    skos:broader onem2m:DataPoint ;
    skos:definition "The minimum value allowed for the \"openLevel\" status. The default value is 0, which means fully closed."@en ;
    skos:inScheme onem2m:scheme ;
    skos:prefLabel "minLevel"@en .

haim:minSpeed a skos:Concept,
        ontolex:LexicalConcept ;
    skos:broader onem2m:DataPoint ;
    skos:definition "The minimum value for the speed level. If not present, the default is 0."@en ;
    skos:inScheme onem2m:scheme ;
    skos:prefLabel "minSpeed"@en .

haim:modality a skos:Concept,
        ontolex:LexicalConcept ;
    skos:broader onem2m:DataPoint ;
    skos:definition "The modality of a particular SpO2 measurement."@en ;
    skos:inScheme onem2m:scheme ;
    skos:prefLabel "modality"@en .

haim:monitoringEnabled a skos:Concept,
        ontolex:LexicalConcept ;
    skos:broader onem2m:DataPoint ;
    skos:definition "The current status of monitoring. \"True\" indicates enabled, and \"False\" indicates not enabled."@en ;
    skos:inScheme onem2m:scheme ;
    skos:prefLabel "monitoringEnabled"@en .

haim:muscle a skos:Concept,
        ontolex:LexicalConcept ;
    skos:broader onem2m:DataPoint ;
    skos:definition "The muscle content measurement from the BIA. The unit of measure is percentage."@en ;
    skos:inScheme onem2m:scheme ;
    skos:prefLabel "muscle"@en .

haim:muscleMass a skos:Concept,
        ontolex:LexicalConcept ;
    skos:broader onem2m:DataPoint ;
    skos:definition "The measurement of muscle mass by a weight scale and a body composition analyser. The unit of measure is kilogram (kg)."@en ;
    skos:inScheme onem2m:scheme ;
    skos:prefLabel "muscleMass"@en .

haim:muteEnabled a skos:Concept,
        ontolex:LexicalConcept ;
    skos:broader onem2m:DataPoint ;
    skos:definition "The current status of the mute enablement. \"True\" indicates enabled (that is, no sound), and \"False\" indicates not enabled (that is, sound is played)."@en ;
    skos:inScheme onem2m:scheme ;
    skos:prefLabel "muteEnabled"@en .

haim:network a skos:Concept,
        ontolex:LexicalConcept ;
    skos:broader onem2m:DataPoint ;
    skos:definition "This value indicates the Wide Area Network (WAN) connectivity of the 3D printer, such as Internet or GSM. \"False\" indicates that the printer does not have network connectivity to a WAN. \"True\" indicates that the printer has WAN network connectivity."@en ;
    skos:inScheme onem2m:scheme ;
    skos:prefLabel "network"@en .

haim:nextTrack a skos:Concept,
        ontolex:LexicalConcept ;
    skos:broader onem2m:Action ;
    skos:definition "Go forward to a next chapter, section or similar marker in the media."@en ;
    skos:inScheme onem2m:scheme ;
    skos:prefLabel "nextTrack"@en .

haim:numberValue a skos:Concept,
        ontolex:LexicalConcept ;
    skos:broader onem2m:DataPoint,
        onem2m:Module ;
    skos:definition "The actual value of the number."@en,
        "This ModuleClass provides the capabilities to represent a number. It also has capabilities for controlled increment and decrement a counter. It can be used to present a number-related functionality in a technology where there is only a weak semantic specification of that functionality."@en ;
    skos:inScheme onem2m:scheme ;
    skos:prefLabel "numberValue"@en ;
    skos:related haim:decrementNumberValue,
        haim:defaultValue,
        haim:incrementNumberValue,
        haim:maxValue,
        haim:minValue,
        haim:numberValue,
        haim:resetNumberValue,
        haim:step ;
    prov:wasDerivedFrom <https://git.onem2m.org/MAS/Home-Appliances/-/raw/master/3.7.0/SDT-TS0023-ModuleClasses.xml> .

haim:object a skos:Concept,
        ontolex:LexicalConcept ;
    skos:broader onem2m:DataPoint ;
    skos:definition "This data point contains the base64 encoded binary object."@en ;
    skos:inScheme onem2m:scheme ;
    skos:prefLabel "object"@en .

haim:objectType a skos:Concept,
        ontolex:LexicalConcept ;
    skos:broader onem2m:DataPoint ;
    skos:definition "This data point contains the type and subtype of the binary object as a MIME type."@en ;
    skos:inScheme onem2m:scheme ;
    skos:prefLabel "objectType"@en .

haim:open a skos:Concept,
        ontolex:LexicalConcept ;
    skos:broader onem2m:Action ;
    skos:definition "Increase the open level by the amount of the \"stepValue\" up to the \"maxLevel\"."@en ;
    skos:inScheme onem2m:scheme ;
    skos:prefLabel "open"@en .

haim:openAlarm a skos:Concept,
        ontolex:LexicalConcept ;
    skos:broader onem2m:DataPoint ;
    skos:definition "The state of the door open alarm. \"True\" indicates that the open alarm is active. \"False\" indicates that the open alarm is not active."@en ;
    skos:inScheme onem2m:scheme ;
    skos:prefLabel "openAlarm"@en .

haim:openDuration a skos:Concept,
        ontolex:LexicalConcept ;
    skos:broader onem2m:DataPoint ;
    skos:definition "The time duration the door has been open."@en ;
    skos:inScheme onem2m:scheme ;
    skos:prefLabel "openDuration"@en .

haim:overcurrentSensor a skos:Concept,
        ontolex:LexicalConcept ;
    skos:broader onem2m:Module ;
    skos:definition "This ModuleClass provides capabilities for an over-current sensor. "@en ;
    skos:inScheme onem2m:scheme ;
    skos:prefLabel "overcurrentSensor"@en ;
    skos:related haim:detectedTime,
        haim:duration,
        haim:overcurrentStatus ;
    prov:wasDerivedFrom <https://git.onem2m.org/MAS/Home-Appliances/-/raw/master/3.7.0/SDT-TS0023-ModuleClasses.xml> .

haim:overcurrentStatus a skos:Concept,
        ontolex:LexicalConcept ;
    skos:broader onem2m:DataPoint ;
    skos:definition """The overcurrentStatus indicates as follows:
"True" indicates that an over-current is detected, and "False" indicates a normal status, this means that an over-current is not detected."""@en ;
    skos:inScheme onem2m:scheme ;
    skos:prefLabel "overcurrentStatus"@en .

haim:oximeter a skos:Concept,
        ontolex:LexicalConcept ;
    skos:broader onem2m:Module ;
    skos:definition "This ModuleClass provides the capability to report the measurement of blood oxygen characteristics."@en ;
    skos:inScheme onem2m:scheme ;
    skos:prefLabel "oximeter"@en ;
    skos:related haim:oxygenSaturation ;
    prov:wasDerivedFrom <https://git.onem2m.org/MAS/Home-Appliances/-/raw/master/3.7.0/SDT-TS0023-ModuleClasses.xml> .

haim:oxygenSaturation a skos:Concept,
        ontolex:LexicalConcept ;
    skos:broader onem2m:DataPoint ;
    skos:definition "The measurement of oxygensaturation by Oximeter. The unit of measure is in percentage."@en ;
    skos:inScheme onem2m:scheme ;
    skos:prefLabel "oxygenSaturation"@en .

haim:ozoneMeter a skos:Concept,
        ontolex:LexicalConcept ;
    skos:broader onem2m:Module ;
    skos:definition "This ModuleClass provides capabilities for an ozone meter. The \"ozoneValue…\" attributes are optional, but one of them SHALL be provided."@en ;
    skos:inScheme onem2m:scheme ;
    skos:prefLabel "ozoneMeter"@en ;
    skos:related haim:maxValue,
        haim:ozoneStatus,
        haim:ozoneValueMG,
        haim:ozoneValuePPM ;
    prov:wasDerivedFrom <https://git.onem2m.org/MAS/Home-Appliances/-/raw/master/3.7.0/SDT-TS0023-ModuleClasses.xml> .

haim:ozoneStatus a skos:Concept,
        ontolex:LexicalConcept ;
    skos:broader onem2m:DataPoint ;
    skos:definition "The ozoneStatus indicates the level of ozone status. (See clause 5.6.21)."@en ;
    skos:inScheme onem2m:scheme ;
    skos:prefLabel "ozoneStatus"@en .

haim:ozoneValueMG a skos:Concept,
        ontolex:LexicalConcept ;
    skos:broader onem2m:DataPoint ;
    skos:definition "The unit of ozone measurement is \"mg/m^3\"."@en ;
    skos:inScheme onem2m:scheme ;
    skos:prefLabel "ozoneValueMG"@en .

haim:ozoneValuePPM a skos:Concept,
        ontolex:LexicalConcept ;
    skos:broader onem2m:DataPoint ;
    skos:definition "The unit of measure of ozone measurement is \"ppm\"."@en ;
    skos:inScheme onem2m:scheme ;
    skos:prefLabel "ozoneValuePPM"@en .

haim:password a skos:Concept,
        ontolex:LexicalConcept ;
    skos:broader onem2m:DataPoint ;
    skos:definition "The user’s password."@en ;
    skos:inScheme onem2m:scheme ;
    skos:prefLabel "password"@en .

haim:power a skos:Concept,
        ontolex:LexicalConcept ;
    skos:broader onem2m:DataPoint ;
    skos:definition "The power of the device. The unit of measure is Watt (W)."@en ;
    skos:inScheme onem2m:scheme ;
    skos:prefLabel "power"@en .

haim:powerGenerationData a skos:Concept,
        ontolex:LexicalConcept ;
    skos:broader onem2m:DataPoint ;
    skos:definition "Amount of instantaneous generation data. The unit of measure is Watt (W)."@en ;
    skos:inScheme onem2m:scheme ;
    skos:prefLabel "powerGenerationData"@en .

haim:powerSaveEnabled a skos:Concept,
        ontolex:LexicalConcept ;
    skos:broader onem2m:DataPoint ;
    skos:definition "The current status of the power saving mode. \"True\" indicates enabled, and \"False\" indicates not enabled."@en ;
    skos:inScheme onem2m:scheme ;
    skos:prefLabel "powerSaveEnabled"@en .

haim:powerState a skos:Concept,
        ontolex:LexicalConcept ;
    skos:broader onem2m:DataPoint ;
    skos:definition "The current status of the binarySwitch. \"True\" indicates turned-on, and \"False\" indicates turned-off."@en ;
    skos:inScheme onem2m:scheme ;
    skos:prefLabel "powerState"@en .

haim:preWash a skos:Concept,
        ontolex:LexicalConcept ;
    skos:broader onem2m:DataPoint ;
    skos:definition "This data point indicates pre-wash. \"True\" indicates enabled, \"False\" indicates disabled."@en ;
    skos:inScheme onem2m:scheme ;
    skos:prefLabel "preWash"@en .

haim:previousChannel a skos:Concept,
        ontolex:LexicalConcept ;
    skos:broader onem2m:DataPoint ;
    skos:definition "The channel number which was selected previously."@en ;
    skos:inScheme onem2m:scheme ;
    skos:prefLabel "previousChannel"@en .

haim:previousTrack a skos:Concept,
        ontolex:LexicalConcept ;
    skos:broader onem2m:Action ;
    skos:definition "Go back to a previous chapter, section or similar marker in the media."@en ;
    skos:inScheme onem2m:scheme ;
    skos:prefLabel "previousTrack"@en .

haim:printSizeX a skos:Concept,
        ontolex:LexicalConcept ;
    skos:broader onem2m:DataPoint ;
    skos:definition "This data point represents the maximum size of a printing object in the direction of X-axis. The unit of measure is \"mm\". (1/10cm)."@en ;
    skos:inScheme onem2m:scheme ;
    skos:prefLabel "printSizeX"@en .

haim:printSizeY a skos:Concept,
        ontolex:LexicalConcept ;
    skos:broader onem2m:DataPoint ;
    skos:definition "This data point represents the maximum size of printing object in the direction of Y-axis. The unit of measure is \"mm\". (1/10cm)."@en ;
    skos:inScheme onem2m:scheme ;
    skos:prefLabel "printSizeY"@en .

haim:printSizeZ a skos:Concept,
        ontolex:LexicalConcept ;
    skos:broader onem2m:DataPoint ;
    skos:definition "This data point represents the maximum size of printing object in the direction of Z-axis. The unit of measure is “mm”. (1/10cm)."@en ;
    skos:inScheme onem2m:scheme ;
    skos:prefLabel "printSizeZ"@en .

haim:printType a skos:Concept,
        ontolex:LexicalConcept ;
    skos:broader onem2m:DataPoint ;
    skos:definition "The type of printing technology (see clause 5.6.1)."@en ;
    skos:inScheme onem2m:scheme ;
    skos:prefLabel "printType"@en .

haim:printingState a skos:Concept,
        ontolex:LexicalConcept ;
    skos:broader onem2m:DataPoint ;
    skos:definition "The printingState is indicating the status of the printing file."@en ;
    skos:inScheme onem2m:scheme ;
    skos:prefLabel "printingState"@en .

haim:progressPercentage a skos:Concept,
        ontolex:LexicalConcept ;
    skos:broader onem2m:DataPoint ;
    skos:definition "The indication of current job progress in percentage."@en ;
    skos:inScheme onem2m:scheme ;
    skos:prefLabel "progressPercentage"@en .

haim:pulseRate a skos:Concept,
        ontolex:LexicalConcept ;
    skos:broader onem2m:DataPoint ;
    skos:definition "The measurement of pulserate by pulsemeter. The unit of measure is in beats per minute."@en ;
    skos:inScheme onem2m:scheme ;
    skos:prefLabel "pulseRate"@en .

haim:pushed a skos:Concept,
        ontolex:LexicalConcept ;
    skos:broader onem2m:DataPoint ;
    skos:definition "To indicate the press of the button."@en ;
    skos:inScheme onem2m:scheme ;
    skos:prefLabel "pushed"@en .

haim:rapidCool a skos:Concept,
        ontolex:LexicalConcept ;
    skos:broader onem2m:DataPoint ;
    skos:definition "Controls the rapid cool capability. \"True\" indicates active, \"False\" indicates inactive."@en ;
    skos:inScheme onem2m:scheme ;
    skos:prefLabel "rapidCool"@en .

haim:rapidFreeze a skos:Concept,
        ontolex:LexicalConcept ;
    skos:broader onem2m:DataPoint ;
    skos:definition "Controls the rapid freeze capability. \"True\" indicates active, \"False\" indicates inactive."@en ;
    skos:inScheme onem2m:scheme ;
    skos:prefLabel "rapidFreeze"@en .

haim:recipientID a skos:Concept,
        ontolex:LexicalConcept ;
    skos:broader onem2m:DataPoint ;
    skos:definition "This data point represents the receiving caller identiﬁcation of a call. In case of an incoming call this would be the local line ID and optionally extension. The format of caller ID is not speciﬁed here."@en ;
    skos:inScheme onem2m:scheme ;
    skos:prefLabel "recipientID"@en .

haim:red a skos:Concept,
        ontolex:LexicalConcept ;
    skos:broader onem2m:DataPoint ;
    skos:definition "The value of the Red colour channel of RGB. The range is [0,255]."@en ;
    skos:inScheme onem2m:scheme ;
    skos:prefLabel "red"@en .

haim:referenceTimer a skos:Concept,
        ontolex:LexicalConcept ;
    skos:broader onem2m:DataPoint ;
    skos:definition "A timer (for example. a time-based value, App Defined Epoch, Progressive) expressed in seconds. The value indicates a time counter to be used as reference for the other time-based data points of this ModuleClass. Usually it is the time since the last event of power-on of the producer (or more in detail the since the boot of its connectivity node)."@en ;
    skos:inScheme onem2m:scheme ;
    skos:prefLabel "referenceTimer"@en .

haim:refrigeration a skos:Concept,
        ontolex:LexicalConcept ;
    skos:broader onem2m:Module ;
    skos:definition "This ModuleClass provides capabilities for a refrigeration function. "@en ;
    skos:inScheme onem2m:scheme ;
    skos:prefLabel "refrigeration"@en ;
    skos:related haim:defrost,
        haim:rapidCool,
        haim:rapidFreeze ;
    prov:wasDerivedFrom <https://git.onem2m.org/MAS/Home-Appliances/-/raw/master/3.7.0/SDT-TS0023-ModuleClasses.xml> .

haim:remoteControlEnabled a skos:Concept,
        ontolex:LexicalConcept ;
    skos:broader onem2m:DataPoint ;
    skos:definition "This data point enables or disables remote controllability and is set by a user locally. “True” indicates enabled remote access, and “False” indicates disabled remote access."@en ;
    skos:inScheme onem2m:scheme ;
    skos:prefLabel "remoteControlEnabled"@en .

haim:resetNumberValue a skos:Concept,
        ontolex:LexicalConcept ;
    skos:broader onem2m:Action ;
    skos:definition "Reset the \"numberValue\" to its \"defaultValue\"."@en ;
    skos:inScheme onem2m:scheme ;
    skos:prefLabel "resetNumberValue"@en .

haim:resetTextMessage a skos:Concept,
        ontolex:LexicalConcept ;
    skos:broader onem2m:Action ;
    skos:definition "Reset the receiver of the message to the \"defaultValue\"."@en ;
    skos:inScheme onem2m:scheme ;
    skos:prefLabel "resetTextMessage"@en .

haim:resistance a skos:Concept,
        ontolex:LexicalConcept ;
    skos:broader onem2m:DataPoint ;
    skos:definition "The resistance measurement of a human body. The unit of measure is ohm."@en ;
    skos:inScheme onem2m:scheme ;
    skos:prefLabel "resistance"@en .

haim:robotCleanerJobMode a skos:Concept,
        ontolex:LexicalConcept ;
    skos:broader onem2m:Module ;
    skos:definition "This ModuleClasses provides capabilities to control and monitor the job modes of a robotCleaner."@en ;
    skos:inScheme onem2m:scheme ;
    skos:prefLabel "robotCleanerJobMode"@en ;
    skos:related haim:currentJobMode,
        haim:currentJobModeName,
        haim:jobModes ;
    prov:wasDerivedFrom <https://git.onem2m.org/MAS/Home-Appliances/-/raw/master/3.7.0/SDT-TS0023-ModuleClasses.xml> .

haim:roundingEnergyConsumption a skos:Concept,
        ontolex:LexicalConcept ;
    skos:broader onem2m:DataPoint ;
    skos:definition "This energy consumption data is calculated by multiplying significantDigits with multiplyingFactors, and rounding down the result."@en ;
    skos:inScheme onem2m:scheme ;
    skos:prefLabel "roundingEnergyConsumption"@en .

haim:roundingEnergyGeneration a skos:Concept,
        ontolex:LexicalConcept ;
    skos:broader onem2m:DataPoint ;
    skos:definition "This energy consumption data is calculated by multiplying significantDigits with multiplyingFactors, and rounding down the result."@en ;
    skos:inScheme onem2m:scheme ;
    skos:prefLabel "roundingEnergyGeneration"@en .

haim:rr a skos:Concept,
        ontolex:LexicalConcept ;
    skos:broader onem2m:DataPoint ;
    skos:definition "The measurement of RR interval by pulsemeter. The unit of measure is millisecond (ms)."@en ;
    skos:inScheme onem2m:scheme ;
    skos:prefLabel "rr"@en .

haim:rssi a skos:Concept,
        ontolex:LexicalConcept ;
    skos:broader onem2m:DataPoint ;
    skos:definition "The current value of received signal strength indicator, which reflects the raw signal level."@en ;
    skos:inScheme onem2m:scheme ;
    skos:prefLabel "rssi"@en .

haim:runningTime a skos:Concept,
        ontolex:LexicalConcept ;
    skos:broader onem2m:DataPoint ;
    skos:definition "A timer (for example a time-based value, App Defined Epoch, Progressive) expressed in seconds. It indicates the time of the current operation. Usually its value is increasing one value per second. It starts counting from 0 when the operation starts and stops counting when the operation ends."@en ;
    skos:inScheme onem2m:scheme ;
    skos:prefLabel "runningTime"@en .

haim:sdp a skos:Concept,
        ontolex:LexicalConcept ;
    skos:broader onem2m:DataPoint ;
    skos:definition "Media description using SDP. One or more comma separated multiple SDP lines (SDP media or attribute line) can be included using SDP description syntax as defined in the SDP specification in IETF RFC4566."@en ;
    skos:inScheme onem2m:scheme ;
    skos:prefLabel "sdp"@en .

haim:securityMode a skos:Concept,
        ontolex:LexicalConcept ;
    skos:broader onem2m:Module ;
    skos:definition "This ModuleClasses provides capabilities to control and monitor a security mode."@en ;
    skos:inScheme onem2m:scheme ;
    skos:prefLabel "securityMode"@en ;
    skos:related haim:currentSecurityMode,
        haim:securityModes ;
    prov:wasDerivedFrom <https://git.onem2m.org/MAS/Home-Appliances/-/raw/master/3.7.0/SDT-TS0023-ModuleClasses.xml> .

haim:securityModes a skos:Concept,
        ontolex:LexicalConcept ;
    skos:broader onem2m:DataPoint ;
    skos:definition "List of possible security modes the device supports (see clause 5.6.24)."@en ;
    skos:inScheme onem2m:scheme ;
    skos:prefLabel "securityModes"@en .

haim:sensitivity a skos:Concept,
        ontolex:LexicalConcept ;
    skos:broader onem2m:DataPoint ;
    skos:definition "The level of the detection accuracy of the motion sensor. This data point can be used to control the number of the report."@en ;
    skos:inScheme onem2m:scheme ;
    skos:prefLabel "sensitivity"@en .

haim:sensorHumidity a skos:Concept,
        ontolex:LexicalConcept ;
    skos:broader onem2m:DataPoint ;
    skos:definition "The measured humidity. The minimum value is 0, and the maximum value is 100."@en ;
    skos:inScheme onem2m:scheme ;
    skos:prefLabel "sensorHumidity"@en .

haim:sensorOdor a skos:Concept,
        ontolex:LexicalConcept ;
    skos:broader onem2m:DataPoint ;
    skos:definition "The concentration of odor that reflects air pollution. The minimum value is 0, and the maximum value is 1 000."@en ;
    skos:inScheme onem2m:scheme ;
    skos:prefLabel "sensorOdor"@en .

haim:sensorPM1 a skos:Concept,
        ontolex:LexicalConcept ;
    skos:broader onem2m:DataPoint ;
    skos:definition "The concentration of particle matter under 1um. The minimum value is 0, and the maximum value is 1000."@en ;
    skos:inScheme onem2m:scheme ;
    skos:prefLabel "sensorPM1"@en .

haim:sensorPM10 a skos:Concept,
        ontolex:LexicalConcept ;
    skos:broader onem2m:DataPoint ;
    skos:definition "The concentration of particle matter under 10um. The minimum value is 0, and the maximum value is 1000."@en ;
    skos:inScheme onem2m:scheme ;
    skos:prefLabel "sensorPM10"@en .

haim:sensorPM2 a skos:Concept,
        ontolex:LexicalConcept ;
    skos:broader onem2m:DataPoint ;
    skos:definition "The concentration of particle matter under 2,5um. The minimum value is 0, and the maximum value is 1000."@en ;
    skos:inScheme onem2m:scheme ;
    skos:prefLabel "sensorPM2"@en .

haim:silentTime a skos:Concept,
        ontolex:LexicalConcept ;
    skos:broader onem2m:DataPoint ;
    skos:definition "The time that a motionSensor restrains from sending an alarm in case continuous motions are detected after one alarm is produced. This data point can be used to avoid repeated alarm reports. The unit of measure is seconds."@en ;
    skos:inScheme onem2m:scheme ;
    skos:prefLabel "silentTime"@en .

haim:size a skos:Concept,
        ontolex:LexicalConcept ;
    skos:broader onem2m:DataPoint ;
    skos:definition "The size of the decoded binary object."@en ;
    skos:inScheme onem2m:scheme ;
    skos:prefLabel "size"@en .

haim:smokeSensor a skos:Concept,
        ontolex:LexicalConcept ;
    skos:broader onem2m:Module ;
    skos:definition "This ModuleClass provides the capabilities to indicate the detection of smoke and raising an alarm if the triggering criterion is met."@en ;
    skos:inScheme onem2m:scheme ;
    skos:prefLabel "smokeSensor"@en ;
    skos:related haim:alarm,
        haim:currentValue,
        haim:detectedTime,
        haim:smokeThreshold ;
    prov:wasDerivedFrom <https://git.onem2m.org/MAS/Home-Appliances/-/raw/master/3.7.0/SDT-TS0023-ModuleClasses.xml> .

haim:smokeThreshold a skos:Concept,
        ontolex:LexicalConcept ;
    skos:broader onem2m:DataPoint ;
    skos:definition "The threshold to trigger the alarm. The unit of measure is ppm."@en ;
    skos:inScheme onem2m:scheme ;
    skos:prefLabel "smokeThreshold"@en .

haim:softLeanMass a skos:Concept,
        ontolex:LexicalConcept ;
    skos:broader onem2m:DataPoint ;
    skos:definition "The measurement of soft lean mass by a weight scale and a body composition analyser. The unit of measure is kilogram (kg)."@en ;
    skos:inScheme onem2m:scheme ;
    skos:prefLabel "softLeanMass"@en .

haim:soilLevel a skos:Concept,
        ontolex:LexicalConcept ;
    skos:broader onem2m:DataPoint ;
    skos:definition "This data point represents the washing level (see clause 5.6.12)."@en ;
    skos:inScheme onem2m:scheme ;
    skos:prefLabel "soilLevel"@en .

haim:speed a skos:Concept,
        ontolex:LexicalConcept ;
    skos:broader onem2m:DataPoint ;
    skos:definition "The current speed level in the range of the [minSpeed, maxSpeed] data points."@en ;
    skos:inScheme onem2m:scheme ;
    skos:prefLabel "speed"@en .

haim:speedFactor a skos:Concept,
        ontolex:LexicalConcept ;
    skos:broader onem2m:DataPoint ;
    skos:definition "The optional factor of speeding up or slowing down playback, rewind or fast forward."@en ;
    skos:inScheme onem2m:scheme ;
    skos:prefLabel "speedFactor"@en .

haim:speedWash a skos:Concept,
        ontolex:LexicalConcept ;
    skos:broader onem2m:DataPoint ;
    skos:definition "This data point indicates speed wash. \"True\" indicates enabled, \"False\" indicates disabled."@en ;
    skos:inScheme onem2m:scheme ;
    skos:prefLabel "speedWash"@en .

haim:sphygmomanometer a skos:Concept,
        ontolex:LexicalConcept ;
    skos:broader onem2m:Module ;
    skos:definition "This ModuleClass provides the capability to report the measurement of blood pressure characteristics."@en ;
    skos:inScheme onem2m:scheme ;
    skos:prefLabel "sphygmomanometer"@en ;
    skos:related haim:diastolicPressure,
        haim:meanPressure,
        haim:systolicPressure ;
    prov:wasDerivedFrom <https://git.onem2m.org/MAS/Home-Appliances/-/raw/master/3.7.0/SDT-TS0023-ModuleClasses.xml> .

haim:spinLevelStrength a skos:Concept,
        ontolex:LexicalConcept ;
    skos:broader onem2m:DataPoint ;
    skos:definition "The value of spin-dry level (see clause 5.6.25). A higher value indicates a higher spin level."@en ;
    skos:inScheme onem2m:scheme ;
    skos:prefLabel "spinLevelStrength"@en .

haim:spinSpeed a skos:Concept,
        ontolex:LexicalConcept ;
    skos:broader onem2m:DataPoint ;
    skos:definition "This data point represents the spin-dry speed level (see clause 5.6.13)."@en ;
    skos:inScheme onem2m:scheme ;
    skos:prefLabel "spinSpeed"@en .

haim:start3Dprint a skos:Concept,
        ontolex:LexicalConcept ;
    skos:broader onem2m:Action ;
    skos:definition "Start 3D printing."@en ;
    skos:inScheme onem2m:scheme ;
    skos:prefLabel "start3Dprint"@en .

haim:startPause a skos:Concept,
        ontolex:LexicalConcept ;
    skos:broader onem2m:DataPoint ;
    skos:definition "A value of \"True\" triggers or starts an operation, and \"False\" pauses the operation."@en ;
    skos:inScheme onem2m:scheme ;
    skos:prefLabel "startPause"@en .

haim:steamClosetJobMode a skos:Concept,
        ontolex:LexicalConcept ;
    skos:broader onem2m:Module ;
    skos:definition "This ModuleClass provides capabilities to control and monitor the job modes of steamCloset."@en ;
    skos:inScheme onem2m:scheme ;
    skos:prefLabel "steamClosetJobMode"@en ;
    skos:related haim:currentJobMode,
        haim:currentJobModeName,
        haim:jobModes ;
    prov:wasDerivedFrom <https://git.onem2m.org/MAS/Home-Appliances/-/raw/master/3.7.0/SDT-TS0023-ModuleClasses.xml> .

haim:steamTreat a skos:Concept,
        ontolex:LexicalConcept ;
    skos:broader onem2m:DataPoint ;
    skos:definition "This data point indicates steam treat. \"True\" indicates enabled, \"False\" indicates disabled."@en ;
    skos:inScheme onem2m:scheme ;
    skos:prefLabel "steamTreat"@en .

haim:step a skos:Concept,
        ontolex:LexicalConcept ;
    skos:broader onem2m:DataPoint ;
    skos:definition "The optional step size for controlled increment and decrement. The default is 1,0, even when this data point is not implemented."@en ;
    skos:inScheme onem2m:scheme ;
    skos:prefLabel "step"@en .

haim:stop3Dprint a skos:Concept,
        ontolex:LexicalConcept ;
    skos:broader onem2m:Action ;
    skos:definition "Stop 3D printing."@en ;
    skos:inScheme onem2m:scheme ;
    skos:prefLabel "stop3Dprint"@en .

haim:strength a skos:Concept,
        ontolex:LexicalConcept ;
    skos:broader onem2m:DataPoint ;
    skos:definition "The current strength of the drink taste (see clause 5.6.28). A higher value indicates a stronger taste."@en ;
    skos:inScheme onem2m:scheme ;
    skos:prefLabel "strength"@en .

haim:supportedHorizontalDirection a skos:Concept,
        ontolex:LexicalConcept ;
    skos:broader onem2m:DataPoint ;
    skos:definition "List of supported horizontal directions."@en ;
    skos:inScheme onem2m:scheme ;
    skos:prefLabel "supportedHorizontalDirection"@en .

haim:supportedMediaSources a skos:Concept,
        ontolex:LexicalConcept ;
    skos:broader onem2m:DataPoint ;
    skos:definition "List of supported input or output media for the given device (see clause 5.6.27)."@en ;
    skos:inScheme onem2m:scheme ;
    skos:prefLabel "supportedMediaSources"@en .

haim:supportedMessageValues a skos:Concept,
        ontolex:LexicalConcept ;
    skos:broader onem2m:DataPoint ;
    skos:definition "List of supported values for the message. Each of the values in this list shall be URL-encoded. An encoded value shall not contain white spaces."@en ;
    skos:inScheme onem2m:scheme ;
    skos:prefLabel "supportedMessageValues"@en .

haim:supportedPlayerModes a skos:Concept,
        ontolex:LexicalConcept ;
    skos:broader onem2m:DataPoint ;
    skos:definition "List of supported modes for a player."@en ;
    skos:inScheme onem2m:scheme ;
    skos:prefLabel "supportedPlayerModes"@en .

haim:supportedVerticalDirection a skos:Concept,
        ontolex:LexicalConcept ;
    skos:broader onem2m:DataPoint ;
    skos:definition "List of supported vertical directions."@en ;
    skos:inScheme onem2m:scheme ;
    skos:prefLabel "supportedVerticalDirection"@en .

haim:systolicPressure a skos:Concept,
        ontolex:LexicalConcept ;
    skos:broader onem2m:DataPoint ;
    skos:definition "The measurement of systolic pressure by sphygmomanometer. The unit of measure is millimetre of mercury (mmHg)."@en ;
    skos:inScheme onem2m:scheme ;
    skos:prefLabel "systolicPressure"@en .

haim:targetAltitude a skos:Concept,
        ontolex:LexicalConcept ;
    skos:broader onem2m:DataPoint ;
    skos:definition "The optional target altitude part of a geo-location. This can be used to move a device to a new altitude. The unit of measures is meters."@en ;
    skos:inScheme onem2m:scheme ;
    skos:prefLabel "targetAltitude"@en .

haim:targetDuration a skos:Concept,
        ontolex:LexicalConcept ;
    skos:broader onem2m:DataPoint ;
    skos:definition "A time span (for a time-based value, App Defined Epoch, Fixed) expressed in seconds. The value indicates a time that represents the target duration of the operation as per user selection."@en ;
    skos:inScheme onem2m:scheme ;
    skos:prefLabel "targetDuration"@en .

haim:targetLatitude a skos:Concept,
        ontolex:LexicalConcept ;
    skos:broader onem2m:DataPoint ;
    skos:definition "The optional target latitude part of a geo-location. This can be used to move a device to a new location. The unit of measures is degrees."@en ;
    skos:inScheme onem2m:scheme ;
    skos:prefLabel "targetLatitude"@en .

haim:targetLongitude a skos:Concept,
        ontolex:LexicalConcept ;
    skos:broader onem2m:DataPoint ;
    skos:definition "The optional target longitude part of a geo-location. This can be used to move a device to a new location. The unit of measures is degrees."@en ;
    skos:inScheme onem2m:scheme ;
    skos:prefLabel "targetLongitude"@en .

haim:targetTemperature a skos:Concept,
        ontolex:LexicalConcept ;
    skos:broader onem2m:DataPoint ;
    skos:definition "The desired temperature to reach."@en ;
    skos:inScheme onem2m:scheme ;
    skos:prefLabel "targetTemperature"@en .

haim:targetTimeToStart a skos:Concept,
        ontolex:LexicalConcept ;
    skos:broader onem2m:DataPoint ;
    skos:definition "A time span (for example a time-based value, App Defined Epoch, Fixed) expressed in seconds. The value indicates the time when the appliance is expected to start its operation, starting counting from the last \"referenceTimer\"."@en ;
    skos:inScheme onem2m:scheme ;
    skos:prefLabel "targetTimeToStart"@en .

haim:targetTimeToStop a skos:Concept,
        ontolex:LexicalConcept ;
    skos:broader onem2m:DataPoint ;
    skos:definition "A time span (for example a time-based value, App Defined Epoch, Fixed) expressed in seconds. The value indicates the time when the appliance is expected to stop its operation, starting counting from the last ”referenceTimer”."@en ;
    skos:inScheme onem2m:scheme ;
    skos:prefLabel "targetTimeToStop"@en .

haim:temperatureThreshold a skos:Concept,
        ontolex:LexicalConcept ;
    skos:broader onem2m:DataPoint ;
    skos:definition "The threshold to trigger the alarm."@en ;
    skos:inScheme onem2m:scheme ;
    skos:prefLabel "temperatureThreshold"@en .

haim:textMessage a skos:Concept,
        ontolex:LexicalConcept ;
    skos:broader onem2m:DataPoint,
        onem2m:Module ;
    skos:definition "The current message value."@en,
        "This ModuleClass provides capabilities to set and get a text message."@en ;
    skos:inScheme onem2m:scheme ;
    skos:prefLabel "textMessage"@en ;
    skos:related haim:defaultValue,
        haim:maxLength,
        haim:messageEncoding,
        haim:minLength,
        haim:resetTextMessage,
        haim:supportedMessageValues,
        haim:textMessage ;
    prov:wasDerivedFrom <https://git.onem2m.org/MAS/Home-Appliances/-/raw/master/3.7.0/SDT-TS0023-ModuleClasses.xml> .

haim:threeDPrinter a skos:Concept,
        ontolex:LexicalConcept ;
    skos:broader onem2m:Module ;
    skos:definition "This ModuleClass describes capabilities of a 3D printer."@en ;
    skos:inScheme onem2m:scheme ;
    skos:prefLabel "threeDPrinter"@en ;
    skos:related haim:memorySize,
        haim:network,
        haim:printSizeX,
        haim:printSizeY,
        haim:printSizeZ,
        haim:printType,
        haim:start3Dprint,
        haim:stop3Dprint ;
    prov:wasDerivedFrom <https://git.onem2m.org/MAS/Home-Appliances/-/raw/master/3.7.0/SDT-TS0023-ModuleClasses.xml> .

haim:time a skos:Concept,
        ontolex:LexicalConcept ;
    skos:broader onem2m:DataPoint ;
    skos:definition "The desired duration of ‘keep water warm’ function. It indicates how long water shall be kept warm, for example after the boiling in a kettle. The value indicates a time expressed in minutes."@en ;
    skos:inScheme onem2m:scheme ;
    skos:prefLabel "time"@en .

haim:toggle a skos:Concept,
        ontolex:LexicalConcept ;
    skos:broader onem2m:Action ;
    skos:definition "Toggle the switch."@en ;
    skos:inScheme onem2m:scheme ;
    skos:prefLabel "toggle"@en .

haim:token a skos:Concept,
        ontolex:LexicalConcept ;
    skos:broader onem2m:DataPoint ;
    skos:definition "An authentication token, for example an OAuth token."@en ;
    skos:inScheme onem2m:scheme ;
    skos:prefLabel "token"@en .

haim:tone a skos:Concept,
        ontolex:LexicalConcept ;
    skos:broader onem2m:DataPoint ;
    skos:definition "Representing the tones of the alarm (see clause 5.6.29)."@en ;
    skos:inScheme onem2m:scheme ;
    skos:prefLabel "tone"@en .

haim:turbo a skos:Concept,
        ontolex:LexicalConcept ;
    skos:broader onem2m:Module ;
    skos:definition "This ModuleClass provides capabilities to enable turbo mode and monitor the current status of the turbo function. It is intended to be part of devices which use turbo function such as an air conditioner, a washing machine, etc."@en ;
    skos:inScheme onem2m:scheme ;
    skos:prefLabel "turbo"@en ;
    skos:related haim:turboEnabled ;
    prov:wasDerivedFrom <https://git.onem2m.org/MAS/Home-Appliances/-/raw/master/3.7.0/SDT-TS0023-ModuleClasses.xml> .

haim:turboEnabled a skos:Concept,
        ontolex:LexicalConcept ;
    skos:broader onem2m:DataPoint ;
    skos:definition "The current status of the turbo mode. \"True\" indicates enbaled, and \"False\" indicates not enabled."@en ;
    skos:inScheme onem2m:scheme ;
    skos:prefLabel "turboEnabled"@en .

haim:unit a skos:Concept,
        ontolex:LexicalConcept ;
    skos:broader onem2m:DataPoint ;
    skos:definition "The unit of measure for the temperature values. The default is Celsius (C)."@en ;
    skos:inScheme onem2m:scheme ;
    skos:prefLabel "unit"@en .

haim:upChannel a skos:Concept,
        ontolex:LexicalConcept ;
    skos:broader onem2m:Action ;
    skos:definition "Change the current channel to the next channel in the stored list of available channels. If the current channel is the last one in the list, the new set channel may be the first one in the list."@en ;
    skos:inScheme onem2m:scheme ;
    skos:prefLabel "upChannel"@en .

haim:upVolume a skos:Concept,
        ontolex:LexicalConcept ;
    skos:broader onem2m:Action ;
    skos:definition "Increase volume by the amount of the stepValue up to the maxValue."@en ;
    skos:inScheme onem2m:scheme ;
    skos:prefLabel "upVolume"@en .

haim:uri a skos:Concept,
        ontolex:LexicalConcept ;
    skos:broader onem2m:DataPoint ;
    skos:definition "The URI of the printing file. The URI could be \"file://www.example.com/file.extension\"."@en ;
    skos:inScheme onem2m:scheme ;
    skos:prefLabel "uri"@en .

haim:url a skos:Concept,
        ontolex:LexicalConcept ;
    skos:broader onem2m:DataPoint ;
    skos:definition "A URL at which the specified media can be accessed."@en ;
    skos:inScheme onem2m:scheme ;
    skos:prefLabel "url"@en .

haim:useGrinder a skos:Concept,
        ontolex:LexicalConcept ;
    skos:broader onem2m:DataPoint ;
    skos:definition "The current status of the grinder enablement. \"True\" indicates enabled, and \"False\" indicates disabled."@en ;
    skos:inScheme onem2m:scheme ;
    skos:prefLabel "useGrinder"@en .

haim:uvSensor a skos:Concept,
        ontolex:LexicalConcept ;
    skos:broader onem2m:Module ;
    skos:definition "This ModuleClass describes the capabilities of an ultraviolet sensor."@en ;
    skos:inScheme onem2m:scheme ;
    skos:prefLabel "uvSensor"@en ;
    skos:related haim:uvStatus,
        haim:uvValue ;
    prov:wasDerivedFrom <https://git.onem2m.org/MAS/Home-Appliances/-/raw/master/3.7.0/SDT-TS0023-ModuleClasses.xml> .

haim:uvStatus a skos:Concept,
        ontolex:LexicalConcept ;
    skos:broader onem2m:DataPoint ;
    skos:definition "The \"uvStatus\" indicates the level of the UV radiation status (see clause 5.6.30)."@en ;
    skos:inScheme onem2m:scheme ;
    skos:prefLabel "uvStatus"@en .

haim:uvValue a skos:Concept,
        ontolex:LexicalConcept ;
    skos:broader onem2m:DataPoint ;
    skos:definition "The unit of measure of the UV intensity of radiation is \"mW/cm^2\"."@en ;
    skos:inScheme onem2m:scheme ;
    skos:prefLabel "uvValue"@en .

haim:verticalAccuracy a skos:Concept,
        ontolex:LexicalConcept ;
    skos:broader onem2m:DataPoint ;
    skos:definition "The optional current vertical accuracy of the altitude. The unit of measures is meters."@en ;
    skos:inScheme onem2m:scheme ;
    skos:prefLabel "verticalAccuracy"@en .

haim:verticalDirection a skos:Concept,
        ontolex:LexicalConcept ;
    skos:broader onem2m:DataPoint ;
    skos:definition "The vertical direction of the air flow (see clause 5.6.31)."@en ;
    skos:inScheme onem2m:scheme ;
    skos:prefLabel "verticalDirection"@en .

haim:visceraFat a skos:Concept,
        ontolex:LexicalConcept ;
    skos:broader onem2m:DataPoint ;
    skos:definition "The viscera fat content measurement from the BIA The unit of measure is percentage."@en ;
    skos:inScheme onem2m:scheme ;
    skos:prefLabel "visceraFat"@en .

haim:voc a skos:Concept,
        ontolex:LexicalConcept ;
    skos:broader onem2m:DataPoint ;
    skos:definition "ThThis value indicates the VOC (Volatile Organic Compounds) value in ppm."@en ;
    skos:inScheme onem2m:scheme ;
    skos:prefLabel "voc"@en .

haim:volumePercentage a skos:Concept,
        ontolex:LexicalConcept ;
    skos:broader onem2m:DataPoint ;
    skos:definition "The rounded percentage of the current volume in the range of [0, maxValue]. 0% shall mean no sound produced."@en ;
    skos:inScheme onem2m:scheme ;
    skos:prefLabel "volumePercentage"@en .

haim:washTemp a skos:Concept,
        ontolex:LexicalConcept ;
    skos:broader onem2m:DataPoint ;
    skos:definition "This data point represents the water temperature level (see clause 5.6.14)."@en ;
    skos:inScheme onem2m:scheme ;
    skos:prefLabel "washTemp"@en .

haim:water a skos:Concept,
        ontolex:LexicalConcept ;
    skos:broader onem2m:DataPoint ;
    skos:definition "The water content measurement from the BIA. The unit of measure is percentage."@en ;
    skos:inScheme onem2m:scheme ;
    skos:prefLabel "water"@en .

haim:waterFlowStrength a skos:Concept,
        ontolex:LexicalConcept ;
    skos:broader onem2m:DataPoint ;
    skos:definition "The desired level of water flow (see clause 5.6.33). A higher value indicates higher water flow."@en ;
    skos:inScheme onem2m:scheme ;
    skos:prefLabel "waterFlowStrength"@en .

haim:airFlow a skos:Concept,
        ontolex:LexicalConcept ;
    skos:broader onem2m:Module ;
    skos:definition "This ModuleClass provides capabilities for controlling the air flow of a device."@en ;
    skos:inScheme onem2m:scheme ;
    skos:prefLabel "airFlow"@en ;
    skos:related haim:automode,
        haim:horizontalDirection,
        haim:maxSpeed,
        haim:minSpeed,
        haim:speed,
        haim:supportedHorizontalDirection,
        haim:supportedVerticalDirection,
        haim:verticalDirection ;
    prov:wasDerivedFrom <https://git.onem2m.org/MAS/Home-Appliances/-/raw/master/3.7.0/SDT-TS0023-ModuleClasses.xml> .

haim:autoDocumentFeeder a skos:Concept,
        ontolex:LexicalConcept ;
    skos:broader onem2m:Module ;
    skos:definition "This ModuleClasses provides capabilities to monitor the state of autoDocumentFeeder (ADF). ADF is a feature which takes several pages and feeds the paper one page at a time into a scanner or printer, allowing the user to scan, print or fax, multiple-page documents without having to manually replace each page."@en ;
    skos:inScheme onem2m:scheme ;
    skos:prefLabel "autoDocumentFeeder"@en ;
    skos:related haim:adfStates,
        haim:currentAdfState ;
    prov:wasDerivedFrom <https://git.onem2m.org/MAS/Home-Appliances/-/raw/master/3.7.0/SDT-TS0023-ModuleClasses.xml> .

haim:clothesWasherJobModeOption a skos:Concept,
        ontolex:LexicalConcept ;
    skos:broader onem2m:Module ;
    skos:definition "This ModuleClasses provides capabilities to control and monitor the washing job mode options of a washer."@en ;
    skos:inScheme onem2m:scheme ;
    skos:prefLabel "clothesWasherJobModeOption"@en ;
    skos:related haim:coldWash,
        haim:extraRinse,
        haim:preWash,
        haim:soilLevel,
        haim:speedWash,
        haim:spinSpeed,
        haim:steamTreat,
        haim:washTemp ;
    prov:wasDerivedFrom <https://git.onem2m.org/MAS/Home-Appliances/-/raw/master/3.7.0/SDT-TS0023-ModuleClasses.xml> .

haim:code a skos:Concept,
        ontolex:LexicalConcept ;
    skos:broader onem2m:DataPoint ;
    skos:definition "The numeric representation of the fault."@en ;
    skos:inScheme onem2m:scheme ;
    skos:prefLabel "code"@en .

haim:colourSaturation a skos:Concept,
        ontolex:LexicalConcept ;
    skos:broader onem2m:DataPoint,
        onem2m:Module ;
    skos:definition "The status of colour saturation level. \"colourSaturation\" has a range of [0,100]. A \"colourSaturation\" value of 0 means that a device displays or produces black and white images. A \"colourSaturation\" value of 50 means that a  device displays or produces normal colour images. A \"colourSaturation\" value of 100 means that a device displays or produces very colourful images."@en,
        "This ModuleClass provides capabilities to control and monitor a colour saturation value."@en ;
    skos:inScheme onem2m:scheme ;
    skos:prefLabel "colourSaturation"@en ;
    skos:related haim:colourSaturation ;
    prov:wasDerivedFrom <https://git.onem2m.org/MAS/Home-Appliances/-/raw/master/3.7.0/SDT-TS0023-ModuleClasses.xml> .

haim:defaultValue a skos:Concept,
        ontolex:LexicalConcept ;
    skos:broader onem2m:DataPoint ;
    skos:definition "The optional default value for \"textMessage\". The default is an empty string."@en,
        "The optional default value for the number. The default is 0,0."@en ;
    skos:inScheme onem2m:scheme ;
    skos:prefLabel "defaultValue"@en .

haim:detectedTime a skos:Concept,
        ontolex:LexicalConcept ;
    skos:broader onem2m:DataPoint ;
    skos:definition "The date and time the smoke is detected."@en,
        "The time when the over-current was detected."@en ;
    skos:inScheme onem2m:scheme ;
    skos:prefLabel "detectedTime"@en .

haim:duration a skos:Concept,
        ontolex:LexicalConcept ;
    skos:broader onem2m:DataPoint ;
    skos:definition "The duration for video/audio recording. Set to trigger the recorder. The unit of measure is seconds."@en,
        "The duration of the detected over-current. The unit of measure is \"ms\"."@en ;
    skos:inScheme onem2m:scheme ;
    skos:prefLabel "duration"@en .

haim:energyConsumption a skos:Concept,
        ontolex:LexicalConcept ;
    skos:broader onem2m:Module ;
    skos:definition "This ModuleClass describes the measured energy consumed by the device since power up. One particular use case for the energyConsumption ModuleClass is a smart meter"@en ;
    skos:inScheme onem2m:scheme ;
    skos:prefLabel "energyConsumption"@en ;
    skos:related haim:absoluteEnergyConsumption,
        haim:current,
        haim:frequency,
        haim:measuringScope,
        haim:multiplyingFactors,
        haim:power,
        haim:roundingEnergyConsumption,
        haim:significantDigits,
        haim:voltage ;
    prov:wasDerivedFrom <https://git.onem2m.org/MAS/Home-Appliances/-/raw/master/3.7.0/SDT-TS0023-ModuleClasses.xml> .

haim:energyGeneration a skos:Concept,
        ontolex:LexicalConcept ;
    skos:broader onem2m:Module ;
    skos:definition "This ModuleClass provides information about generation data on electric generator devices such as a photo voltaic power system, fuel cells, or microgeneration"@en ;
    skos:inScheme onem2m:scheme ;
    skos:prefLabel "energyGeneration"@en ;
    skos:related haim:generationSource,
        haim:multiplyingFactors,
        haim:powerGenerationData,
        haim:roundingEnergyGeneration,
        haim:significantDigits ;
    prov:wasDerivedFrom <https://git.onem2m.org/MAS/Home-Appliances/-/raw/master/3.7.0/SDT-TS0023-ModuleClasses.xml> .

haim:keepWarm a skos:Concept,
        ontolex:LexicalConcept ;
    skos:broader onem2m:Module ;
    skos:definition "This module allows to control the ‘keep warm’ feature in devices like coffee machines, kettles etc. It allows to keep water warm for a desired time. This ModuleClass inherits from binarySwitch (see clause 5.3.12) to store setting for the ‘keep warm’ feature. If the \"powerState\" data point in a keepWarmSwitch is \"True\" then the ‘keep warm’ function will be performed just after boiling (or heating) process is finished (otherwise this function will not be applied)."@en ;
    skos:inScheme onem2m:scheme ;
    skos:prefLabel "keepWarm"@en ;
    skos:related haim:time ;
    prov:wasDerivedFrom <https://git.onem2m.org/MAS/Home-Appliances/-/raw/master/3.7.0/SDT-TS0023-ModuleClasses.xml> .

haim:liquidLevel a skos:Concept,
        ontolex:LexicalConcept ;
    skos:broader onem2m:DataPoint,
        onem2m:Module ;
    skos:definition "The desired level of water or other liquid, for example the desired level of milk in a cup of coffee (see clause 5.6.19)."@en,
        "This ModuleClass provides the desired level of water (or other liquid) for an appliance, for example the desired level of milk for a cup of coffee from a coffee machine."@en ;
    skos:inScheme onem2m:scheme ;
    skos:prefLabel "liquidLevel"@en ;
    skos:related haim:liquidLevel ;
    prov:wasDerivedFrom <https://git.onem2m.org/MAS/Home-Appliances/-/raw/master/3.7.0/SDT-TS0023-ModuleClasses.xml> .

haim:minValue a skos:Concept,
        ontolex:LexicalConcept ;
    skos:broader onem2m:DataPoint ;
    skos:definition "Minimum value of \"targetTemperature\"."@en,
        "The optional minimum value of the number. The default is the system-specific minimum value for a float value."@en ;
    skos:inScheme onem2m:scheme ;
    skos:prefLabel "minValue"@en .

haim:multiplyingFactors a skos:Concept,
        ontolex:LexicalConcept ;
    skos:broader onem2m:DataPoint ;
    skos:definition "The unit for data multiplying factors, for example 1 kWh, 0,1 kWh, 0,01 kWh, etc."@en,
        "The unit for data multiplying factors, for example. 1 kWh, 0,1 kWh, 0,01 kWh, etc."@en ;
    skos:inScheme onem2m:scheme ;
    skos:prefLabel "multiplyingFactors"@en .

haim:relativeHumidity a skos:Concept,
        ontolex:LexicalConcept ;
    skos:broader onem2m:DataPoint,
        onem2m:Module ;
    skos:definition "The measurement of the relative humidity value; the unit of measure is percentage."@en,
        "This ModuleClass provides the capability for the device to report the humidity based on a specified rule that is vendor dependent."@en ;
    skos:inScheme onem2m:scheme ;
    skos:prefLabel "relativeHumidity"@en ;
    skos:related haim:desiredHumidity,
        haim:relativeHumidity ;
    prov:wasDerivedFrom <https://git.onem2m.org/MAS/Home-Appliances/-/raw/master/3.7.0/SDT-TS0023-ModuleClasses.xml> .

haim:sessionDescription a skos:Concept,
        ontolex:LexicalConcept ;
    skos:broader onem2m:Module ;
    skos:definition "This ModuleClass provides the capabilities for a sessionDescription containing a URL at which the specified media can be accessed and the definition of media using SDP."@en ;
    skos:inScheme onem2m:scheme ;
    skos:prefLabel "sessionDescription"@en ;
    skos:related haim:sdp,
        haim:url ;
    prov:wasDerivedFrom <https://git.onem2m.org/MAS/Home-Appliances/-/raw/master/3.7.0/SDT-TS0023-ModuleClasses.xml> .

haim:significantDigits a skos:Concept,
        ontolex:LexicalConcept ;
    skos:broader onem2m:DataPoint ;
    skos:definition "The number of effective digits for data."@en ;
    skos:inScheme onem2m:scheme ;
    skos:prefLabel "significantDigits"@en .

haim:televisionChannel a skos:Concept,
        ontolex:LexicalConcept ;
    skos:broader onem2m:Module ;
    skos:definition "This ModuleClass provides capabilities to set and get channels of a device that has a channel list."@en ;
    skos:inScheme onem2m:scheme ;
    skos:prefLabel "televisionChannel"@en ;
    skos:related haim:availableChannels,
        haim:channelId,
        haim:channelName,
        haim:downChannel,
        haim:previousChannel,
        haim:upChannel ;
    prov:wasDerivedFrom <https://git.onem2m.org/MAS/Home-Appliances/-/raw/master/3.7.0/SDT-TS0023-ModuleClasses.xml> .

haim:voltage a skos:Concept,
        ontolex:LexicalConcept ;
    skos:broader onem2m:DataPoint ;
    skos:definition "Rated voltage. The unit of measure is ampere (A)."@en,
        "The voltage of the device. The unit of measure is volts (V)."@en ;
    skos:inScheme onem2m:scheme ;
    skos:prefLabel "voltage"@en .

haim:weight a skos:Concept,
        ontolex:LexicalConcept ;
    skos:broader onem2m:DataPoint,
        onem2m:Module ;
    skos:definition "The weight measurement. The common unit is kilogram (kg)."@en,
        "This ModuleClass provides the capability to report the measurement of weight."@en ;
    skos:inScheme onem2m:scheme ;
    skos:prefLabel "weight"@en ;
    skos:related haim:weight ;
    prov:wasDerivedFrom <https://git.onem2m.org/MAS/Home-Appliances/-/raw/master/3.7.0/SDT-TS0023-ModuleClasses.xml> .

haim:audioVolume a skos:Concept,
        ontolex:LexicalConcept ;
    skos:broader onem2m:Module ;
    skos:definition "This ModuleClass provides capabilities to control and monitor volume."@en ;
    skos:inScheme onem2m:scheme ;
    skos:prefLabel "audioVolume"@en ;
    skos:related haim:downVolume,
        haim:maxValue,
        haim:muteEnabled,
        haim:stepValue,
        haim:upVolume,
        haim:volumePercentage ;
    prov:wasDerivedFrom <https://git.onem2m.org/MAS/Home-Appliances/-/raw/master/3.7.0/SDT-TS0023-ModuleClasses.xml> .

haim:brightness a skos:Concept,
        ontolex:LexicalConcept ;
    skos:broader onem2m:DataPoint,
        onem2m:Module ;
    skos:definition "The status of brightness level in percentage."@en,
        "This ModuleClass provides capabilities to control and monitor the brightness of a light for example from a lamp. Brightness is scaled as a percentage. A lamp or a monitor can be adjusted to a level of light between very dim (0 % is the minimum brightness) and very bright (100 % is the maximum brightness)."@en ;
    skos:inScheme onem2m:scheme ;
    skos:prefLabel "brightness"@en ;
    skos:related haim:brightness ;
    prov:wasDerivedFrom <https://git.onem2m.org/MAS/Home-Appliances/-/raw/master/3.7.0/SDT-TS0023-ModuleClasses.xml> .

haim:clock a skos:Concept,
        ontolex:LexicalConcept ;
    skos:broader onem2m:Module ;
    skos:definition "This ModuleClass provides capabilities to control and monitor time and date information."@en ;
    skos:inScheme onem2m:scheme ;
    skos:prefLabel "clock"@en ;
    skos:related haim:currentDate,
        haim:currentTime,
        haim:currentTimeZone ;
    prov:wasDerivedFrom <https://git.onem2m.org/MAS/Home-Appliances/-/raw/master/3.7.0/SDT-TS0023-ModuleClasses.xml> .

haim:doorStatus a skos:Concept,
        ontolex:LexicalConcept ;
    skos:broader onem2m:Module ;
    skos:definition "This ModuleClass provides the status of a door. It is intended to be part of a device such as a refrigerator and an oven that might have multiple doors. "@en ;
    skos:inScheme onem2m:scheme ;
    skos:prefLabel "doorStatus"@en ;
    skos:related haim:doorState,
        haim:openAlarm,
        haim:openDuration ;
    prov:wasDerivedFrom <https://git.onem2m.org/MAS/Home-Appliances/-/raw/master/3.7.0/SDT-TS0023-ModuleClasses.xml> .

haim:filterInfo a skos:Concept,
        ontolex:LexicalConcept ;
    skos:broader onem2m:Module ;
    skos:definition "This ModuleClass provides capabilities for monitoring filter information of a device."@en ;
    skos:inScheme onem2m:scheme ;
    skos:prefLabel "filterInfo"@en ;
    skos:related haim:code,
        haim:filterLifetime,
        haim:status ;
    prov:wasDerivedFrom <https://git.onem2m.org/MAS/Home-Appliances/-/raw/master/3.7.0/SDT-TS0023-ModuleClasses.xml> .

haim:liquidRemaining a skos:Concept,
        ontolex:LexicalConcept ;
    skos:broader onem2m:DataPoint,
        onem2m:Module ;
    skos:definition "The remaining level of water or other liquid in an appliance (see clause 5.6.19)."@en,
        "This ModuleClass provides the status of water level (or other liquid) for an appliance, for example the level of remaining milk in a coffee machine."@en ;
    skos:inScheme onem2m:scheme ;
    skos:prefLabel "liquidRemaining"@en ;
    skos:related haim:liquidRemaining ;
    prov:wasDerivedFrom <https://git.onem2m.org/MAS/Home-Appliances/-/raw/master/3.7.0/SDT-TS0023-ModuleClasses.xml> .

haim:mediaSelect a skos:Concept,
        ontolex:LexicalConcept ;
    skos:broader onem2m:Module ;
    skos:definition "This ModuleClass provides capabilities to control and monitor media input and output of device such as TV or SetTopBox."@en ;
    skos:inScheme onem2m:scheme ;
    skos:prefLabel "mediaSelect"@en ;
    skos:related haim:mediaID,
        haim:mediaName,
        haim:mediaType,
        haim:status,
        haim:supportedMediaSources ;
    prov:wasDerivedFrom <https://git.onem2m.org/MAS/Home-Appliances/-/raw/master/3.7.0/SDT-TS0023-ModuleClasses.xml> .

haim:motionSensor a skos:Concept,
        ontolex:LexicalConcept ;
    skos:broader onem2m:Module ;
    skos:definition "This ModuleClass provides the capabilities to indicate the occurrence of motion and raising of an alarm if the triggering criterion is met."@en ;
    skos:inScheme onem2m:scheme ;
    skos:prefLabel "motionSensor"@en ;
    skos:related haim:alarm,
        haim:sensitivity,
        haim:silentTime ;
    prov:wasDerivedFrom <https://git.onem2m.org/MAS/Home-Appliances/-/raw/master/3.7.0/SDT-TS0023-ModuleClasses.xml> .

haim:playerControl a skos:Concept,
        ontolex:LexicalConcept ;
    skos:broader onem2m:Module ;
    skos:definition "This ModuleClass provides capabilities to control and monitor the operational modes of a media player functionality."@en ;
    skos:inScheme onem2m:scheme ;
    skos:prefLabel "playerControl"@en ;
    skos:related haim:currentPlayerMode,
        haim:currentPlayerModeName,
        haim:nextTrack,
        haim:previousTrack,
        haim:speedFactor,
        haim:supportedPlayerModes ;
    prov:wasDerivedFrom <https://git.onem2m.org/MAS/Home-Appliances/-/raw/master/3.7.0/SDT-TS0023-ModuleClasses.xml> .

haim:printQueue a skos:Concept,
        ontolex:LexicalConcept ;
    skos:broader onem2m:Module ;
    skos:definition "This ModuleClass provides the capabilities for monitoring printing list information."@en ;
    skos:inScheme onem2m:scheme ;
    skos:prefLabel "printQueue"@en ;
    skos:related haim:printingState,
        haim:uri ;
    prov:wasDerivedFrom <https://git.onem2m.org/MAS/Home-Appliances/-/raw/master/3.7.0/SDT-TS0023-ModuleClasses.xml> .

haim:pulsemeter a skos:Concept,
        ontolex:LexicalConcept ;
    skos:broader onem2m:Module ;
    skos:definition "This ModuleClass provides the capability to report the measurement of pulse characteristics."@en ;
    skos:inScheme onem2m:scheme ;
    skos:prefLabel "pulsemeter"@en ;
    skos:related haim:energy,
        haim:modality,
        haim:pulseRate,
        haim:rr ;
    prov:wasDerivedFrom <https://git.onem2m.org/MAS/Home-Appliances/-/raw/master/3.7.0/SDT-TS0023-ModuleClasses.xml> .

haim:remoteControlEnable a skos:Concept,
        ontolex:LexicalConcept ;
    skos:broader onem2m:Module ;
    skos:definition "This ModuleClasses provides capabilities to monitor the remote controllability of the appliance."@en ;
    skos:inScheme onem2m:scheme ;
    skos:prefLabel "remoteControlEnable"@en ;
    skos:related haim:remoteControlEnabled ;
    prov:wasDerivedFrom <https://git.onem2m.org/MAS/Home-Appliances/-/raw/master/3.7.0/SDT-TS0023-ModuleClasses.xml> .

haim:stepValue a skos:Concept,
        ontolex:LexicalConcept ;
    skos:broader onem2m:DataPoint ;
    skos:definition "Step value allowed for \"targetTemperature\"."@en,
        "Step value used by the \"UpVolume\" and \"DownVolume\" actions."@en,
        "The step value used by the \"open\" and \"close\" actions."@en ;
    skos:inScheme onem2m:scheme ;
    skos:prefLabel "stepValue"@en .

haim:alarm a skos:Concept,
        ontolex:LexicalConcept ;
    skos:broader onem2m:DataPoint ;
    skos:definition "The alarm is indicated as follows: \"True\" indicates that smoke has been detected, \"False\" indicates a normal status, that means that smoke is not detected."@en,
        "The detection of the motion occurrence."@en,
        "The detection of water. The alarm is indicated as follows: \"True\" indicates that water has been detected, \"False\" indicates a normal status, that means that water is not detected."@en,
        "This data point indicates the status of detection of an abnormal temperature. \"True\" indicates an abnormal temperature, \"False\" indicates a normal temperature."@en ;
    skos:inScheme onem2m:scheme ;
    skos:prefLabel "alarm"@en .

haim:lock a skos:Concept,
        ontolex:LexicalConcept ;
    skos:broader onem2m:DataPoint,
        onem2m:Module ;
    skos:definition "\"True\" indicates the object is locked, while \"False\" indicates the object is not locked."@en,
        "This ModuleClass provides the function to lock and unlock an object. "@en ;
    skos:inScheme onem2m:scheme ;
    skos:prefLabel "lock"@en ;
    skos:related haim:lock ;
    prov:wasDerivedFrom <https://git.onem2m.org/MAS/Home-Appliances/-/raw/master/3.7.0/SDT-TS0023-ModuleClasses.xml> .

haim:maxValue a skos:Concept,
        ontolex:LexicalConcept ;
    skos:broader onem2m:DataPoint ;
    skos:definition "Maximum value allowed for Volume. maxValue is 100 by default if \"maxValue\" is not provided."@en,
        "Maximum value of \"targetTemperature\"."@en,
        "The mazimum value shows the measurement range of the ozone meter (for example maxValue=5 means the range is 0 to 5 ppm). This attribute is only used that the ozoneMeter provides \"ppm\" value."@en,
        "The optional maximum value of the number. The default is the system-specific maximum value for a float value."@en ;
    skos:inScheme onem2m:scheme ;
    skos:prefLabel "maxValue"@en .

haim:openLevel a skos:Concept,
        ontolex:LexicalConcept ;
    skos:broader onem2m:DataPoint,
        onem2m:Module ;
    skos:definition "The rounded percentage of the current open level of entity in the range of [0, 100]. 0 percentage shall mean the entity is closed."@en,
        "This ModuleClass provides the capabilities to control and monitor the open status of an entity, for example a curtain."@en ;
    skos:inScheme onem2m:scheme ;
    skos:prefLabel "openLevel"@en ;
    skos:related haim:close,
        haim:maxLevel,
        haim:minLevel,
        haim:open,
        haim:openLevel,
        haim:stepValue ;
    prov:wasDerivedFrom <https://git.onem2m.org/MAS/Home-Appliances/-/raw/master/3.7.0/SDT-TS0023-ModuleClasses.xml> .

haim:powerSave a skos:Concept,
        ontolex:LexicalConcept ;
    skos:broader onem2m:Module ;
    skos:definition "This ModuleClass provides capabilities to enable the power saving mode of a device and monitor the current status."@en ;
    skos:inScheme onem2m:scheme ;
    skos:prefLabel "powerSave"@en ;
    skos:related haim:powerSaveEnabled ;
    prov:wasDerivedFrom <https://git.onem2m.org/MAS/Home-Appliances/-/raw/master/3.7.0/SDT-TS0023-ModuleClasses.xml> .

haim:airQualitySensor a skos:Concept,
        ontolex:LexicalConcept ;
    skos:broader onem2m:Module ;
    skos:definition "ThThis ModuleClass provides capabilities for a monitoring sensor that measures the air quality."@en ;
    skos:inScheme onem2m:scheme ;
    skos:prefLabel "airQualitySensor"@en ;
    skos:related haim:ch2o,
        haim:co,
        haim:co2,
        haim:monitoringEnabled,
        haim:sensorHumidity,
        haim:sensorOdor,
        haim:sensorPM1,
        haim:sensorPM10,
        haim:sensorPM2,
        haim:voc ;
    prov:wasDerivedFrom <https://git.onem2m.org/MAS/Home-Appliances/-/raw/master/3.7.0/SDT-TS0023-ModuleClasses.xml> .

haim:status a skos:Concept,
        ontolex:LexicalConcept ;
    skos:broader onem2m:DataPoint ;
    skos:definition "Specifies whether the specific media instance is selected (\"True\") or not (\"False\")."@en,
        "Status of fault detection."@en,
        "The status of boiling. \"True\" indicates boiling, \"False\" indicates not boiling."@en,
        "The status of connection. \"True\" means connected, \"False\" means not connected."@en,
        "The status of fault detection."@en ;
    skos:inScheme onem2m:scheme ;
    skos:prefLabel "status"@en .

haim:operationMode a skos:Concept,
        ontolex:LexicalConcept ;
    skos:broader onem2m:Module ;
    skos:definition "This ModuleClasses provides capabilities to control or monitor the operation mode of appliances."@en ;
    skos:inScheme onem2m:scheme ;
    skos:prefLabel "operationMode"@en ;
    skos:related haim:startPause ;
    prov:wasDerivedFrom <https://git.onem2m.org/MAS/Home-Appliances/-/raw/master/3.7.0/SDT-TS0023-ModuleClasses.xml> .

haim:jobModes a skos:Concept,
        ontolex:LexicalConcept ;
    skos:broader onem2m:DataPoint ;
    skos:definition "List of possible job states that the device supports (see clause 5.6.8)."@en,
        "List of possible job states that the device supports."@en,
        "List of possible job states the device supports (??? see clause 5.3.1)."@en,
        "List of possible job states the device supports (see clause 5.6.23)."@en,
        "List of possible job states the device supports (see clause 5.6.26)."@en,
        "List of possible job states the device supports (see clause 5.6.4)."@en,
        "List of possible job states the device supports."@en,
        "List of possible job states the device supports. "@en ;
    skos:inScheme onem2m:scheme ;
    skos:prefLabel "jobModes"@en .

haim:timer a skos:Concept,
        ontolex:LexicalConcept ;
    skos:broader onem2m:Module ;
    skos:definition "This ModuleClass provides capabilities to monitor and control the times when the appliance executes its operations, that means when it starts, when it ends, etc."@en ;
    skos:inScheme onem2m:scheme ;
    skos:prefLabel "timer"@en ;
    skos:related haim:absoluteStartTime,
        haim:absoluteStopTime,
        haim:activateClockTimer,
        haim:deactivateClockTimer,
        haim:estimatedTimeToEnd,
        haim:referenceTimer,
        haim:runningTime,
        haim:targetDuration,
        haim:targetTimeToStart,
        haim:targetTimeToStop ;
    prov:wasDerivedFrom <https://git.onem2m.org/MAS/Home-Appliances/-/raw/master/3.7.0/SDT-TS0023-ModuleClasses.xml> .

haim:currentJobMode a skos:Concept,
        ontolex:LexicalConcept ;
    skos:broader onem2m:DataPoint ;
    skos:definition "Currently active job mode  (see clause 5.6.7). "@en,
        "Currently active job mode (see clause 5.6.23)."@en,
        "Currently active job mode (see clause 5.6.26)."@en,
        "Currently active job mode (see clause 5.6.3)."@en,
        "Currently active job mode (see clause 5.6.4)."@en,
        "Currently active job mode (see clause 5.6.8)."@en,
        "Currently active job mode."@en,
        "The currently active job mode (see clause 5.6.8). "@en,
        "The currently active job mode."@en ;
    skos:inScheme onem2m:scheme ;
    skos:prefLabel "currentJobMode"@en .

haim:currentJobModeName a skos:Concept,
        ontolex:LexicalConcept ;
    skos:broader onem2m:DataPoint ;
    skos:definition "Name of current job mode as a string. This can be used when \"currentJobMode\" is vendor-specific."@en,
        "Name of the current job mode as a  string. This can be used when currentJobMode is vendor-specific."@en,
        "Name of the current job mode as a string. This can be used when currentJobMode is vendor-specific."@en,
        "The name of the current job mode as a string. This can be used when currentJobMode is vendor-specific."@en,
        "The name of the current job mode as a string. This can be used when the currentJobMode is vendor-specific."@en ;
    skos:inScheme onem2m:scheme ;
    skos:prefLabel "currentJobModeName"@en .

haim:temperature a skos:Concept,
        ontolex:LexicalConcept ;
    skos:broader onem2m:DataPoint,
        onem2m:Module ;
    skos:definition "This ModuleClass provides capabilities to represent the current temperature and target temperature of devices such as an air conditioner, refrigerator, oven, etc."@en,
        "To report the value of the temperature. The unit of measure is Celsius (C)."@en ;
    skos:inScheme onem2m:scheme ;
    skos:prefLabel "temperature"@en ;
    skos:related haim:currentTemperature,
        haim:maxValue,
        haim:minValue,
        haim:stepValue,
        haim:targetTemperature,
        haim:unit ;
    prov:wasDerivedFrom <https://git.onem2m.org/MAS/Home-Appliances/-/raw/master/3.7.0/SDT-TS0023-ModuleClasses.xml> .

haim:battery a skos:Concept,
        ontolex:LexicalConcept ;
    skos:broader onem2m:Module ;
    skos:definition "This ModuleClass provides capabilities to indicate the detection of low battery and gives an alarm if triggering criterion is met. The level data point in the module represents the current battery charge level."@en ;
    skos:inScheme onem2m:scheme ;
    skos:prefLabel "battery"@en ;
    skos:related haim:batteryThreshold,
        haim:capacity,
        haim:charging,
        haim:discharging,
        haim:electricEnergy,
        haim:level,
        haim:lowBattery,
        haim:material,
        haim:voltage ;
    prov:wasDerivedFrom <https://git.onem2m.org/MAS/Home-Appliances/-/raw/master/3.7.0/SDT-TS0023-ModuleClasses.xml> .

haim:faultDetection a skos:Concept,
        ontolex:LexicalConcept ;
    skos:broader onem2m:Module ;
    skos:definition "This ModuleClass provides information about whether a fault has occurred in a device."@en ;
    skos:inScheme onem2m:scheme ;
    skos:prefLabel "faultDetection"@en ;
    skos:related haim:code,
        haim:description,
        haim:status ;
    prov:wasDerivedFrom <https://git.onem2m.org/MAS/Home-Appliances/-/raw/master/3.7.0/SDT-TS0023-ModuleClasses.xml> .

haim:runState a skos:Concept,
        ontolex:LexicalConcept ;
    skos:broader onem2m:Module ;
    skos:definition "This ModuleClasses provides capabilities to control and the monitor machine state of appliances."@en ;
    skos:inScheme onem2m:scheme ;
    skos:prefLabel "runState"@en ;
    skos:related haim:currentJobState,
        haim:currentMachineState,
        haim:jobStates,
        haim:machineStates,
        haim:progressPercentage ;
    prov:wasDerivedFrom <https://git.onem2m.org/MAS/Home-Appliances/-/raw/master/3.7.0/SDT-TS0023-ModuleClasses.xml> .

haim:binarySwitch a skos:Concept,
        ontolex:LexicalConcept ;
    skos:broader onem2m:Module ;
    skos:definition "This ModuleClass provides capabilities to control and monitor the state of power."@en ;
    skos:inScheme onem2m:scheme ;
    skos:prefLabel "binarySwitch"@en ;
    skos:related haim:powerState,
        haim:toggle ;
    prov:wasDerivedFrom <https://git.onem2m.org/MAS/Home-Appliances/-/raw/master/3.7.0/SDT-TS0023-ModuleClasses.xml> .

