@prefix esp: <http://example.org/namespace/ble-gatt/esp#> .
@prefix ble: <http://example.org/namespace/ble-gatt#> .
@prefix skos: <http://www.w3.org/2004/02/skos/core#> .
@prefix rdfs: <http://www.w3.org/2000/01/rdf-schema#> .
@prefix owl: <http://www.w3.org/2002/07/owl#> .
@prefix xsd: <http://www.w3.org/2001/XMLSchema#> .

esp:EnvironmentalSensingProfile a skos:Concept .
esp:EnvironmentalSensingService  a skos:Concept .

esp:ESMeasurementDescriptor a skos:Concept .
esp:DescriptorValueChanged a skos:Concept .
esp:ESTriggerSettingDescriptor a skos:Concept .
esp:CharacteristicUserDescription a skos:Concept .
esp:ESConfigurationDescriptor a skos:Concept .
esp:ValidRangeDescriptor a skos:Concept .

esp:EnvironmentalSensingProfile  rdfs:label "Environmental Sensing Profile" .
esp:EnvironmentalSensingProfile rdfs:seeAlso <https://www.bluetooth.org/docman/handlers/downloaddoc.ashx?doc_id=294796> .
esp:EnvironmentalSensingProfile skos:definition "This profile enables a Collector device to connect and interact with an Environmental Sensor for use in outdoor activity applications." .
esp:EnvironmentalSensingProfile owl:versionInfo "1.0.0" .


ble:Profile skos:narrower esp:EnvironmentalSensingProfile .
ble:Service skos:narrower esp:EnvironmentalSensingService .

esp:EnvironmentalSensingProfile skos:related esp:EnvironmentalSensingService .
esp:EnvironmentalSensingProfile skos:related ble:DeviceInformationService .
esp:EnvironmentalSensingProfile skos:related ble:BatteryService.

esp:EnvironmentalSensingService rdfs:label "Environmental Sensing Service" .
esp:EnvironmentalSensingService owl:versionInfo "1.0.0" .
esp:EnvironmentalSensingService skos:definition "The Environmental Sensing Service (ESS) exposes measurement data from an environmental sensor intended for sports and fitness applications." .
esp:EnvironmentalSensingService rdfs:seeAlso <https://www.bluetooth.org/docman/handlers/downloaddoc.ashx?doc_id=294797> .


ble:Characteristic skos:narrower esp:DescriptorValueChanged .
ble:Characteristic skos:narrower esp:ESMeasurementDescriptor .
ble:Characteristic skos:narrower esp:ESTriggerSettingDescriptor .
ble:Characteristic skos:narrower esp:CharacteristicUserDescriptionDescriptor .
ble:Characteristic skos:narrower esp:ESConfigurationDescriptor .
ble:Characteristic skos:narrower esp:ValidRangeDescriptor .

esp:EnvironmentalSensingService skos:related esp:ESMeasurementDescriptor .
esp:EnvironmentalSensingService skos:related esp:DescriptorValueChanged .
esp:EnvironmentalSensingService skos:related esp:ESTriggerSettingDescriptor .
esp:EnvironmentalSensingService skos:related esp:CharacteristicUserDescription .
esp:EnvironmentalSensingService skos:related esp:ESConfigurationDescriptor .
esp:EnvironmentalSensingService skos:related esp:ValidRangeDescriptor .


esp:ESMeasurementDescriptor  rdfs:label "Environmental Sensing Measurement Descriptor" .
esp:ESTriggerSettingDescriptor rdfs:label "Environmental Sensing Trigger Setting Descriptor" .
esp:CharacteristicUserDescription rdfs:label "Characteristic User Description".
esp:ESConfigurationDescriptor rdfs:label "Environmental Sensing Configuration Descriptor" .
esp:ValidRangeDescriptor rdfs:label "Valid Range Descriptor".
esp:DescriptorValueChanged rdfs:label "Descriptor Value Changed" .

esp:ESMeasurementDescriptor skos:definition "This optional characteristic descriptor describes the associated ESS Characteristic by providing additional information pertaining to the value." .
esp:CharacteristicUserDescription skos:definition "This optional descriptor can be used to associate a verbose name with a specific ESS characteristic to allow a human-readable label to be associated with the measurement."  .
esp:ESTriggerSettingDescriptor skos:definition "Where multiple ES Trigger Setting descriptors are present for a given ESS Characteristic, the ES Trigger Setting descriptor and the ES Configuration descriptor work together to define the conditions under which the associated ESS Characteristic value can be notified" .
esp:ESConfigurationDescriptor skos:definition "The ES Configuration descriptor shall be present if more than one ES Trigger Setting descriptor is present for an associated ESS Characteristic. Otherwise it shall not be present for that characteristic" .
esp:ValidRangeDescriptor skos:definition "The Valid Range descriptor is an optional descriptor that allows a Client to read the upper and lower bounds (inclusive) of an associated ESS characteristic value that are supported by the Server".
esp:DescriptorValueChanged skos:definition "It enables a Server to alert bonded Clients that the value of one or more ESS-related descriptors for a given ESS Characteristic have changed and need to be re-read" .

esp:ESMeasurementDescriptor skos:related ble:Read  .
esp:DescriptorValueChanged skos:related ble:Indicate .
esp:ESTriggerSettingDescriptor skos:related ble:Read, ble:Write .
esp:CharacteristicUserDescription skos:related ble:Read, ble:Write .
esp:ESConfigurationDescriptor skos:related  ble:Read, ble:Write .
esp:ValidRangeDescriptor skos:related ble:Read .








