@prefix plxp:  <http://example.org/namespace/ble-gatt/plxp#> .
@prefix ftmp:  <http://example.org/namespace/ble-gatt/ftmp#> .
@prefix esp:   <http://example.org/namespace/ble-gatt/esp#> .
@prefix owl:   <http://www.w3.org/2002/07/owl#> .
@prefix fmp:   <http://example.org/namespace/ble-gatt/fmp#> .
@prefix xsd:   <http://www.w3.org/2001/XMLSchema#> .
@prefix skos:  <http://www.w3.org/2004/02/skos/core#> .
@prefix rdfs:  <http://www.w3.org/2000/01/rdf-schema#> .
@prefix lehid: <http://example.org/namespace/ble-gatt/lehid#> .
@prefix wsp:   <http://example.org/namespace/ble-gatt/wsp#> .
@prefix tip:   <http://example.org/namespace/ble-gatt/tip#> .
@prefix ble:   <http://example.org/namespace/ble-gatt#> .
@prefix rscp:  <http://example.org/namespace/ble-gatt/rscp#> .
@prefix rcp:   <http://example.org/namespace/ble-gatt/rcp#> .
@prefix anp:   <http://example.org/namespace/ble-gatt/anp#> .
@prefix cpp:   <http://example.org/namespace/ble-gatt/cpp#> .
@prefix aiop:  <http://example.org/namespace/ble-gatt/aiop#> .
@prefix scpp:  <http://example.org/namespace/ble-gatt/scpp#> .
@prefix htp:   <http://example.org/namespace/ble-gatt/htp#> .
@prefix blp:   <http://example.org/namespace/ble-gatt/blp#> .
@prefix hrp:   <http://example.org/namespace/ble-gatt/hrp#> .
@prefix cgmp:  <http://example.org/namespace/ble-gatt/cgmp#> .
@prefix pxp:   <http://example.org/namespace/ble-gatt/pxp#> .
@prefix otp:   <http://example.org/namespace/ble-gatt/otp#> .
@prefix glp:   <http://example.org/namespace/ble-gatt/glp#> .
@prefix lnp:   <http://example.org/namespace/ble-gatt/lnp#> .
@prefix cscp:  <http://example.org/namespace/ble-gatt/cscp#> .
@prefix idp:   <http://example.org/namespace/ble-gatt/idp#> .
@prefix ipsp:  <http://example.org/namespace/ble-gatt/ipsp#> .
@prefix pasp:  <http://example.org/namespace/ble-gatt/pasp#> .

pxp:Proximityprofile  a  skos:Concept ;
        rdfs:label       "Proximity profile" ;
        rdfs:seeAlso     <https://www.bluetooth.org/DocMan/handlers/DownloadDoc.ashx?doc_id=303199> ;
        owl:versionInfo  "1.0.1" ;
        skos:definition  "The Proximity profile defines the behavior when a device moves away from a peer device so that the connection is dropped or the path loss increases above a preset level, causing an immediate alert." ;
        skos:related     ble:ImmediateAlertService , pxp:TxPowerService , pxp:LinkLossService .

lehid:bCountryCode  a    skos:Concept ;
        rdfs:label       "Country Code" ;
        skos:definition  "8-bit integer identifying country HID Device hardware is localized for." ;
        skos:related     xsd:unsignedByte .

idp:BatteryMedium  a     skos:Concept ;
        rdfs:label       "Battery Medium" ;
        skos:definition  "The Insulin Delivery Device has a medium operational runtime" .

idp:TherapyControlStatefield
        a                skos:Concept ;
        rdfs:label       "Therapy Control State field" ;
        skos:definition  "The Therapy Control State field describes the therapy state of the insulin delivery (e.g., stop, pause, run)." ;
        skos:narrower    idp:Pause , idp:Run , idp:Undetermined , idp:Stop ;
        skos:related     xsd:unsignedByte .

otp:AllocatedSizeField
        a                skos:Concept ;
        rdfs:label       "Allocated Size Field" ;
        skos:definition  "This value indicates the amount of memory the Server has reserved for holding the object contents." ;
        skos:related     xsd:unsignedInt .

idp:ReservoirIssue  a    skos:Concept ;
        rdfs:label       "Reservoir Issue" ;
        skos:definition  "An error related to the replacement or functioning of the reservoir occurred." .

ble:Value  skos:narrower  lehid:bCountryCode , idp:BatteryMedium , idp:TherapyControlStatefield , otp:AllocatedSizeField , idp:ReservoirIssue , idp:Ready , ftmp:FloorsField , ftmp:RecoveryInterval , idp:MechanicalIssue , lehid:BootKeyboardInputReportValue , lnp:VDOPField , ftmp:StepperMinuteField , ftmp:MinimumInclinationfield , lnp:HDOPField , ftmp:HighSpeedOutside , ftmp:HeartRateControl , cscp:LastWheelEventTime , ftmp:CoolDown , ftmp:FitnessTest , idp:OperationalStatefield , ftmp:AverageStrokeRateField , idp:Temperature , rscp:TotalDistanceField , idp:ReservoirEmpty , ftmp:MinimumInclinationIncrementfield , anp:CategoryID , anp:TextStringInformation , idp:ReservoirRemainingAmountfield , idp:BolusCanceled , ble:TransportDataLengthField , ftmp:RemainingTimeField , ftmp:EnergyperMinuteField , lnp:TimetoFirstFixField , otp:CurrentSizeField , idp:Temperatureoutofrange , idp:Preparing , cpp:PedalPowerBalanceField , lnp:RemainingDistanceField , glp:ExerciseIntensityField , idp:BolusIDfield , cgmp:CGMGlucoseConcentrationField , glp:MedicationIDField , idp:BolusFastAmountfield , lnp:BearingField , lehid:BootProtocolMode , cpp:InstantaneousTorqueMagnitudeArrayField , idp:BolusDelayTime , lehid:ReportProtocolMode , idp:ManufacturerReserved , hrp:HeartRateValueField , ftmp:InstantaneousCadenceField , wsp:BodyWateField , ftmp:InclinationField , ftmp:MinimumSpeedfield , glp:MedicationField , rscp:InstantaneousCadenceField , lehid:bcdHID , idp:Off , lnp:BeaconsNumberViewField , ftmp:AverageStepRateField , ble:LocationNameValue , otp:ObjectFirstCreatedField , idp:AuxInfo3LowerBoundfield , plxp:SpO2PRFastfield , idp:TBROver , ble:AltitudeValue , idp:ReservoirLow , wsp:BIM , wsp:ImpedanceField , ftmp:ResistanceLevelField , ftmp:ForceonBeltField , blp:BloodPressureMeasurementCompoundValueField , lnp:ElevationField , ftmp:MinimumSpeedIncrementfield , ftmp:AveragePaceField , glp:HbA1cField , ftmp:StrokeCountField , idp:AnnunciationStatus , idp:PrimingIssue , ftmp:InstantaneousPaceField , ftmp:MinimumHeartRateIncrementfield , cpp:MinimumForceMagnitude , idp:BatteryLow , plxp:SpO2PRSlowfield , glp:SequenceNumberField , lehid:ProtocolModeValue , cgmp:CGMQualityField , idp:EventData , idp:AnnunciationInstanceID , pasp:AlertStatusValue , lehid:BootKeyboardOutputReportValue , ftmp:StrokeRateField , ble:UncertaintyValue , ftmp:MinimumPowerIncrementfield , cpp:LastWheelEventTime , glp:GlucoseConcentrationField , ftmp:PositiveElevationGainField , ftmp:PowerOutputField , lehid:ReportMapValue , wsp:MusclePercentageField , cpp:MinimumAngle , otp:ObjectIDField , idp:Priming , plxp:SpO2PRSpotCheckField , idp:BatteryEmpty , cscp:CumulativeWheelRevolutions , glp:BaseTimeField , ftmp:AverageCadenceField , idp:Confirmed , ftmp:MaximumPowerfield , idp:Pause , ftmp:EnergyperHourField , cgmp:TimeOffsetField , pxp:TxPowerLevelField , idp:PowerSourceInsufficient , htp:TemperatureMeasurementValueField , ftmp:AverageSpeedField , plxp:SpO2PRNormalfield , lnp:BeaconsNumberSolutionField , idp:Snoozed , htp:IntermediateTemperatureValueField , aiop:AnalogSignalValue , ftmp:HighIntensityInterval , ftmp:AveragePowerField , ftmp:WarmingUp , ble:LongitudeValue , lehid:ReportValue , idp:Standby , idp:BatteryFull , glp:ExerciseDurationField , blp:IntermediateCuffPressureCompoundValueField , ftmp:RampAngleSettingField , idp:SequenceNumberfield , ftmp:MinimumResistanceLevelField , glp:CarbohydrateIDField , cgmp:DTSOffsetField , idp:InsulinConcentrationfield , lnp:EHPEField , ftmp:MinimumPowerfield , otp:ObjectLastModifiedField , cgmp:cgmpSessionRunTimeField , cpp:TopDeadSpotAngleField , ftmp:MaximumHeartRatefield , idp:RelativeOffsetfield , idp:SystemIssue , wsp:FatFreeMassField , wsp:MuscleMassField , wsp:WeightField , lnp:HeadingField , idp:Pending , wsp:BodyFatPercentageField , idp:Run , lehid:BootMouseInputReportValue , ftmp:StepCountField , ftmp:Isometric , ble:LocalNorthCoordinateValue , idp:OcclusionDetected , idp:AuxInfo1Valuefield , cpp:CumulativeWheelRevolutions , rscp:InstantaneousStrideLengthField , cgmp:CGMTrendInformationField , ftmp:TrainingStatusStringField , otp:ObjectNameField , cpp:MaximumForceMagnitude , idp:AnnunciationType , ble:LatitudeValue , cpp:MinimumTorqueMagnitude , lnp:TotalDistanceField , wsp:BasalMetabolismField , ble:OrganizationIDField , idp:BolusDurationfield , glp:CarbohydrateField , lnp:EVPEField , idp:Insulin , wsp:SoftLeanMassField , ftmp:StrideCountField , cpp:AccumulatedEnergyField , lnp:EstimatedTimeArrivalField , lehid:HIDControlPointCharacteristicValue , cpp:AccumulatedTorqueField , ftmp:MinimumHeartRatefield , ftmp:PostWorkout , idp:MaxDelivery , cgmp:TimeZoneField , hrp:EnergyExpendedField , lehid:ExitSuspend , ftmp:MinimumResistanceIncrementfield , ftmp:ElapsedTimeField , ftmp:TotalEnergyField , ftmp:Idle , ftmp:MaximumSpeedfield , lnp:LocationLatitude , glp:TimeOffsetField , htp:MeasurementIntervalValue , cgmp:E2ECRCField , ftmp:ManualMode , anp:NumberofNewAlert , ftmp:HeartRateField , cgmp:SessionStartTimeField , lnp:UTCTimeField , wsp:HeightField , ftmp:MaximumInclinationfield , idp:InfusionSetDetached , ftmp:WattControl , idp:DateTimeIssue , cpp:BottomDeadSpotAngleField , plxp:PulseAmplitudeIndex , ftmp:MetabolicEquivalentField , ble:LocalEastCoordinateValue , cpp:InstantaneousForceMagnitudeArrayField , ftmp:PreWorkout , idp:GenericDevice , idp:BolusExtendedAmountfield , blp:PulseRateField , lnp:RemainingVerticalDistanceField , ble:IndoorPositioningValue , cpp:MaximumTorqueMagnitude , idp:Airpressureoutofrange , ftmp:NegativeElevationGainField , idp:Undetermined , idp:TBRCanceled , glp:MealField , cpp:MaximumAngle , ble:TransportDataField , lnp:LocationLongitude , cpp:FirstCrankMeasurementAngleField , lnp:RollingTimeField , idp:AuxInfo4UpperBoundfield , ftmp:LowSpeedOutside , idp:AuxInfo2Contextfield , ftmp:MaximumResistanceLevelField , ble:FloorNumberValue , ftmp:TotalDistanceField , cgmp:SizeField , hrp:RRIntervalField , lehid:Suspend , idp:InfusionSetIncomplete , ftmp:TrainingStatusField , idp:E2ECounterfield , idp:Stop , idp:Waiting , ftmp:LowIntensityInterval , idp:E2ECRCfield .

htp:TemperatureType  a   skos:Concept ;
        rdfs:label       "Temperature Type" ;
        skos:definition  "The Temperature Type characteristic is used to describe the type of temperature measurement in relation to the location on the human body at which the temperature was measured." ;
        skos:related     ble:Read .

ftmp:TrainingStatus  a   skos:Concept ;
        rdfs:label       "Training Status" ;
        skos:definition  "The Training Status characteristic shall be used by the Server to send the training status information to the Client." ;
        skos:related     ftmp:TrainingStatusStringField , ble:Read , ble:Notify , ftmp:TrainingStatusField .

idp:Ready  a             skos:Concept ;
        rdfs:label       "Ready" ;
        skos:definition  "The Insulin Delivery Device is ready for the insulin infusion therapy" .

ftmp:FloorsField  a      skos:Concept ;
        rdfs:label       "Floors Field" ;
        skos:definition  "The Floors field represents the total number of floors counted by the Server since the beginning of the training session." ;
        skos:related     xsd:unsignedShort .

anp:SupportedUnreadAlertCategory
        a                skos:Concept ;
        rdfs:label       "Supported Unread Alert Category" ;
        skos:definition  "A bit map showing which categories of unread alert events are supported and which are not." ;
        skos:related     ble:Read .

ftmp:RecoveryInterval
        a                skos:Concept ;
        rdfs:label       "Recovery Interval" ;
        skos:definition  "0x05 - Recovery Interval" .

ble:LocationName  a      skos:Concept ;
        rdfs:label       "Location Name" ;
        skos:definition  "The Location Name Characteristic describes the name of the location in which the device is installed in accordance to the civicLocation." ;
        skos:related     ble:Write , ble:LocationNameValue , ble:ReliableWrite , ble:Read , ble:WritewithoutResponse .

idp:MechanicalIssue  a   skos:Concept ;
        rdfs:label       "Mechanical Issue" ;
        skos:definition  "A mechanical error occurred" .

lehid:BootKeyboardInputReportValue
        a                skos:Concept ;
        rdfs:label       "Boot Keyboard Input Report Value" ;
        skos:definition  "The Boot Keyboard Input Report characteristic value is an array of octets whose meaning is defined in the USB HID Usage." ;
        skos:related     xsd:unsignedByte .

lnp:VDOPField  a         skos:Concept ;
        rdfs:label       "Vertical Dilution Of Precision Field" ;
        skos:definition  "The VDOP field represents the Vertical Dilution of Precision, a factor that influences the error in a position fix in the vertical plane." ;
        skos:related     xsd:unsignedByte .

ftmp:StepperMinuteField
        a                skos:Concept ;
        rdfs:label       "Step per Minute Field" ;
        skos:definition  "The Step per Minute Rate field represents the average step rate of a user during a period of one minute." ;
        skos:related     xsd:unsignedShort .

rcp:RCFeature  a         skos:Concept ;
        rdfs:label       "Reconnection Configuration Feature" ;
        skos:definition  "The RC Features characteristic shall be used to describe the supported features of the Reconnection Configuration server." ;
        skos:related     ble:Read .

ftmp:MinimumInclinationfield
        a                skos:Concept ;
        rdfs:label       "Minimum Inclination" ;
        skos:definition  "Minimum Percent with a resolution of 0.1" ;
        skos:related     xsd:short .

cgmp:ContinuousGlucoseMonitoringProfile
        a                skos:Concept ;
        rdfs:label       "Continuous Glucose Monitoring Profile" ;
        rdfs:seeAlso     <https://www.bluetooth.org/docman/handlers/downloaddoc.ashx?doc_id=310501> ;
        owl:versionInfo  "1.0.1" ;
        skos:definition  "The cgmp Profile is used to enable a device to obtain glucose measurement and other data from a cgmp Sensor that exposes the cgmp Service." ;
        skos:related     ble:DeviceInformationService , ble:BondManagementService , cgmp:cgmpService .

pxp:TxPowerLevel  a      skos:Concept ;
        rdfs:label       "Transmit Power Level" ;
        skos:definition  "The Tx Power Level characteristic represents the current transmit power." ;
        skos:related     pxp:TxPowerLevelField , ble:Read .

lnp:HDOPField  a         skos:Concept ;
        rdfs:label       "Horizontal Dilution Of Precision Field" ;
        skos:definition  "The HDOP field represents the Horizontal Dilution of Precision, a factor that influences the error in a position fix in the horizontal plane." ;
        skos:related     xsd:unsignedByte .

ftmp:HighSpeedOutside
        a                skos:Concept ;
        rdfs:label       "Speed Outside of Control Region - High" ;
        skos:definition  "0x0A - Speed Outside of Control Region - High (decrease speed to return to controllable region)" .

ftmp:HeartRateControl
        a                skos:Concept ;
        rdfs:label       "Heart Rate Control" ;
        skos:definition  "0x07 - Heart Rate Control" .

anp:AlertNotificationProfile
        a                skos:Concept ;
        rdfs:label       "Alert Notification Profile" ;
        rdfs:seeAlso     <https://www.bluetooth.org/docman/handlers/downloaddoc.ashx?doc_id=242286> ;
        owl:versionInfo  "1.0" ;
        skos:definition  "The Alert Notification profile allows a device like a watch to obtain information from a cellphone about incoming calls, missed calls and SMS/MMS messages." ;
        skos:related     anp:AlertNotificationService .

cscp:LastWheelEventTime
        a                skos:Concept ;
        rdfs:label       "Last Wheel Event Time Fields" ;
        skos:definition  "The Cumulative Wheel Revolutions value and the Last Wheel Event Time value allow the Client to calculate the speed (instantaneous and average) as well as the distance travelled." ;
        skos:related     xsd:unsignedShort .

ftmp:CoolDown  a         skos:Concept ;
        rdfs:label       "Cool Down" ;
        skos:definition  "0x0B - Cool Down" .

idp:IDDHistoryData  a    skos:Concept ;
        rdfs:label       "Insulin Delivery Device History Data" ;
        skos:definition  "The IDD History Data characteristic is comprised of response records from executed procedures of the IDD Record Access Control Point." ;
        skos:related     idp:EventData , idp:SequenceNumberfield , idp:RelativeOffsetfield , ble:Notify .

rcp:ReconnectionConfigurationProfile
        a                skos:Concept ;
        rdfs:label       "Reconnection Configuration Profile" ;
        rdfs:seeAlso     <https://www.bluetooth.org/docman/handlers/downloaddoc.ashx?doc_id=435662> ;
        owl:versionInfo  "1.0" ;
        skos:definition  "This Bluetooth profile specification defines requirements to enable a Reconnection Configuration Client to modify a variety of communication parameters of a Reconnection Configuration Server." ;
        skos:related     rcp:ReconnectionConfigurationService , ble:BondManagementService .

ftmp:FitnessTest  a      skos:Concept ;
        rdfs:label       "Fitness Test" ;
        skos:definition  "0x08 - Fitness Test" .

idp:OperationalStatefield
        a                skos:Concept ;
        rdfs:label       "Operational State field" ;
        skos:definition  "The Operational State field represents the operational state of the Insulin Delivery Device in the context of running an insulin infusion therapy (e.g., priming)." ;
        skos:related     idp:Ready , idp:Preparing , xsd:unsignedByte , idp:Off , idp:Priming , idp:Standby , idp:Undetermined , idp:Waiting .

glp:GlucoseMeasurementContext
        a                skos:Concept ;
        rdfs:label       "Glucose Measurement Context" ;
        skos:definition  "The Glucose Measurement Context characteristic may be used to send additional contextual information relative to a Glucose Measurement characteristic." ;
        skos:related     glp:ExerciseIntensityField , glp:MedicationIDField , glp:MedicationField , glp:HbA1cField , glp:SequenceNumberField , glp:ExerciseDurationField , glp:CarbohydrateIDField , glp:CarbohydrateField , glp:MealField .

ftmp:AverageStrokeRateField
        a                skos:Concept ;
        rdfs:label       "Average Stroke Rate Field" ;
        skos:definition  "The Average Stroke Rate field represents the average speed since the beginning of the training session." ;
        skos:related     xsd:unsignedByte .

idp:Temperature  a       skos:Concept ;
        rdfs:label       "Temperature" ;
        skos:definition  "The Insulin Delivery Device reports a temperature measurement." .

rscp:TotalDistanceField
        a                skos:Concept ;
        rdfs:label       "Total Distance Field" ;
        skos:definition  "The Total Distance field may be included in the RSC Measurement characteristic if the device supports the Total Distance feature." ;
        skos:related     xsd:unsignedInt .

esp:ESMeasurement  a     skos:Concept ;
        rdfs:label       "Environmental Sensing Measurement" ;
        skos:definition  "ESS Characteristics have been identified as being time-sensitive characteristics." ;
        skos:related     ble:Write , ble:Read , ble:Notify .

lnp:LocationandNavigationService
        a                skos:Concept ;
        rdfs:label       "Location and Navigation (LN) Service" ;
        rdfs:seeAlso     <https://www.bluetooth.org/DocMan/handlers/DownloadDoc.ashx?doc_id=271997> ;
        owl:versionInfo  "1.0" ;
        skos:definition  "The Location and Navigation Service (LN Service) exposes location and navigation-related data from a Location and Navigation sensor (Server) intended for outdoor activity applications." ;
        skos:related     lnp:Navigation , lnp:LocationandSpeed , lnp:LNControlPoint , lnp:PositionQuality , lnp:LNFeature .

idp:IDDRecordAccessControlPoint
        a                skos:Concept ;
        rdfs:label       "Insulin Delivery Device Record Access Control Point" ;
        skos:definition  "This control point is used by the Insulin Delivery Service to provide basic management functionality of the history database of the Insulin Delivery Device including historical data of the insulin therapy, device state changes, and annunciations." ;
        skos:related     ble:Write , ble:Indicate , idp:E2ECounterfield , idp:E2ECRCfield .

idp:ReservoirEmpty  a    skos:Concept ;
        rdfs:label       "Reservoir Empty" ;
        skos:definition  "The reservoir is empty" .

ftmp:MinimumInclinationIncrementfield
        a                skos:Concept ;
        rdfs:label       "Minimum Inclination Increment" ;
        skos:definition  "Minimum Percent with a resolution of 0.1" ;
        skos:related     xsd:unsignedShort .

anp:CategoryID  a        skos:Concept ;
        rdfs:label       "Category ID" ;
        skos:definition  "This field shows the category of the new alert." .

idp:IDDCommandControlPoint
        a                skos:Concept ;
        rdfs:label       "Insulin Delivery Device Command Control Point" ;
        skos:definition  "The IDD Command Control Point provides procedures to support the insulin therapy by adapting therapy parameters to operate the insulin therapy remotely and to perform a remote operation of the device maintenance." ;
        skos:related     ble:Notify , idp:E2ECounterfield , idp:E2ECRCfield .

wsp:WeightScaleFeature
        a                skos:Concept ;
        rdfs:label       "Weight Scale Feature" ;
        skos:definition  "The Weight Scale Feature characteristic shall be used to describe the supported features of the Server." ;
        skos:related     ble:Read .

anp:TextStringInformation
        a                skos:Concept ;
        rdfs:label       "Text String Information" ;
        skos:definition  "The field provides brief text information for the last alert." ;
        skos:related     xsd:string .

idp:ReservoirRemainingAmountfield
        a                skos:Concept ;
        rdfs:label       "Reservoir Remaining Amount field" ;
        skos:definition  "The Reservoir Remaining Amount field represents the remaining amount of insulin in the reservoir in IU." ;
        skos:related     xsd:float .

htp:ValidRangeDescriptor
        a                skos:Concept ;
        rdfs:label       "Valid Range" ;
        skos:definition  "The Valid Range declaration is an optional characteristic descriptor that defines the valid range of values for the Characteristic Value." ;
        skos:related     ble:Read .

htp:IntermediateTemperature
        a                skos:Concept ;
        rdfs:label       "Intermediate Temperature" ;
        skos:definition  "The Intermediate Temperature characteristic is used to send intermediate temperature values to a device for display purposes while the measurement is in progress." ;
        skos:related     ble:Notify .

idp:BolusCanceled  a     skos:Concept ;
        rdfs:label       "Bolus Canceled" ;
        skos:definition  "A running bolus was canceled (e.g., Insulin Delivery Device changed from run to standby mode)" .

idp:IDDFeatures  a       skos:Concept ;
        rdfs:label       "Insulin Delivery Device Feature" ;
        skos:definition  "The IDD Features characteristic shall be used to describe the supported features of the Server." ;
        skos:related     idp:InsulinConcentrationfield , ble:Read , idp:E2ECounterfield , idp:E2ECRCfield .

cscp:CyclingSpeedandCadenceProfile
        a                skos:Concept ;
        rdfs:label       "Cycling Speed and Cadence Profile" ;
        rdfs:seeAlso     <https://www.bluetooth.org/docman/handlers/downloaddoc.ashx?doc_id=261449> ;
        owl:versionInfo  "1.0" ;
        skos:definition  "The Cycling Speed and Cadence Profile is used to enable a data collection device to obtain data from a Cycling Speed and Cadence Sensor (CSC Sensor) that exposes the Cycling Speed and Cadence Service." ;
        skos:related     cscp:CyclingSpeedandCadenceService , ble:DeviceInformationService .

ble:TransportDataLengthField
        a                skos:Concept ;
        rdfs:label       "Transport Data Length Field" ;
        skos:definition  "This field shall contain a 1 octet value that represents the total number of octets in the Transport Data field that follows." ;
        skos:related     xsd:unsignedByte .

cpp:CyclingPowerFeature
        a                skos:Concept ;
        rdfs:label       "Cycling Power Feature" ;
        skos:definition  "The Cycling Power Feature characteristic shall be used to describe the supported features of the Server." ;
        skos:related     ble:Read .

ftmp:RemainingTimeField
        a                skos:Concept ;
        rdfs:label       "Remaining Time Field" ;
        skos:definition  "The Remaining Time field represents the remaining time of a training session that has been selected." ;
        skos:related     xsd:unsignedShort .

lehid:BootKeyboardOutputReport
        a                skos:Concept ;
        rdfs:label       "Boot Keyboard Output Report" ;
        skos:definition  "The Boot Keyboard Output Report characteristic is used to transfer fixed format and length Output Report data between a HID Host operating in Boot Protocol Mode and a HID Service corresponding to a boot keyboard." ;
        skos:related     ble:Write , lehid:BootKeyboardOutputReportValue , ble:Read , ble:WritewithoutResponse .

ftmp:EnergyperMinuteField
        a                skos:Concept ;
        rdfs:label       "Energy per Minute Field" ;
        skos:definition  "The Energy per Minute field represents the average expended energy of a user during a period of one minute." ;
        skos:related     xsd:short .

lnp:TimetoFirstFixField
        a                skos:Concept ;
        rdfs:label       "Time to First Fix Field" ;
        skos:definition  "The Time to First Fix field represents the time used to receive data and calculate the initial position after the device was switched on." ;
        skos:related     xsd:unsignedShort .

cpp:CyclingPowerVector
        a                skos:Concept ;
        rdfs:label       "Cycling Power Vector" ;
        skos:definition  "The Cycling Power Vector characteristic is used to send raw data (either force or torque)." ;
        skos:related     ble:CumulativeCrankRevolutions , cpp:InstantaneousTorqueMagnitudeArrayField , ble:LastCrankEventTime , cpp:InstantaneousForceMagnitudeArrayField , ble:Notify , cpp:FirstCrankMeasurementAngleField .

hrp:BodySensorLocation
        a                skos:Concept ;
        rdfs:label       "Body Sensor Location" ;
        skos:definition  "The Body Sensor Location characteristic of the device is used to describe the intended location of the heart rate measurement for the device." ;
        skos:related     ble:Read .

otp:CurrentSizeField  a  skos:Concept ;
        rdfs:label       "Current Size Field" ;
        skos:definition  "The value of the Current Size field represents an integer number of octets equal to the actual size of the object." ;
        skos:related     xsd:unsignedInt .

ftmp:RowerData  a        skos:Concept ;
        rdfs:label       "Rower Data" ;
        skos:definition  "The Rower Data characteristic is used to send training-related data to the Client from a rower (Server)." ;
        skos:related     ftmp:AverageStrokeRateField , ftmp:RemainingTimeField , ftmp:EnergyperMinuteField , ftmp:ResistanceLevelField , ble:InstantaneousPowerField , ftmp:AveragePaceField , ftmp:StrokeCountField , ftmp:InstantaneousPaceField , ftmp:StrokeRateField , ftmp:EnergyperHourField , ftmp:AveragePowerField , ftmp:ElapsedTimeField , ftmp:TotalEnergyField , ftmp:HeartRateField , ftmp:MetabolicEquivalentField , ble:Notify , ftmp:TotalDistanceField .

cscp:CSCFeature  a       skos:Concept ;
        rdfs:label       "Cycling Speed and Cadence Feature" ;
        skos:definition  "The CSC Feature characteristic shall be used to describe the supported features of the Server." ;
        skos:related     ble:Read .

idp:Temperatureoutofrange
        a                skos:Concept ;
        rdfs:label       "Temperature out of range" ;
        skos:definition  "The temperature is outside of the normal operating range." .

ble:RecordAccessControlPoint
        skos:related  ble:Write , ble:Indicate .

lehid:HIDoverGATTProfile
        a                skos:Concept ;
        rdfs:label       "Low Energy Human Interface Device over GATT Profile" ;
        rdfs:seeAlso     <https://www.bluetooth.org/docman/handlers/downloaddoc.ashx?doc_id=245141> ;
        owl:versionInfo  "1.0" ;
        skos:definition  "The HID over GATT profile defines the procedures and features to be used by Bluetooth low energy HID Devices using GATT and Bluetooth HID Hosts using GATT." ;
        skos:related     ble:BatteryService , ble:DeviceInformationService , lehid:HIDService , ble:ScanParametersService .

lehid:BootMouseInputReport
        a                skos:Concept ;
        rdfs:label       "Boot Mouse Input Report" ;
        skos:definition  "The Boot Mouse Input Report characteristic is used to transfer fixed format and length Input Report data between a HID Host operating in Boot Protocol Mode and a HID Service corresponding to a boot mouse." ;
        skos:related     ble:Write , lehid:BootMouseInputReportValue , ble:Read .

otp:ObjectTransferService
        a                skos:Concept ;
        rdfs:label       "Object Transfer Service" ;
        rdfs:seeAlso     <https://www.bluetooth.org/docman/handlers/DownloadDoc.ashx?doc_id=309937> ;
        owl:versionInfo  "1.0" ;
        skos:definition  "This service provides management and control features supporting bulk data transfers which occur via a separate L2CAP connection oriented channel." ;
        skos:related     otp:ObjectID , otp:ObjectListFilter , otp:OTSFeature , otp:ObjectType , otp:ObjectSize , otp:ObjectListControlPoint , otp:ObjectFirstCreated , otp:ObjectProperties , otp:ObjectChanged , otp:ObjectName , otp:ObjectLastModified , otp:ObjectActionControlPoint .

idp:Preparing  a         skos:Concept ;
        rdfs:label       "Preparing" ;
        skos:definition  "The Insulin Delivery Device prepares the insulin infusion therapy" .

otp:ObjectID  a          skos:Concept ;
        rdfs:label       "Object ID" ;
        skos:definition  "The Object ID characteristic exposes an integer value which is the Object ID of the Current Object." ;
        skos:related     otp:ObjectIDField , ble:Read .

cscp:CSCMeasurement  a   skos:Concept ;
        rdfs:label       "Cycling Speed and Cadence Measurement" ;
        skos:definition  "The CSC Measurement characteristic is used to send speed-related data and/or cadence-related data." ;
        skos:related     ble:CumulativeCrankRevolutions , cscp:LastWheelEventTime , ble:LastCrankEventTime , cscp:CumulativeWheelRevolutions , ble:Notify .

anp:AlertNotificationControlPoint
        a                skos:Concept ;
        rdfs:label       "Alert Notification Control Point" ;
        skos:definition  "This characteristic allows the client device to enable/disable the alert notification of new alert and unread alert events more selectively than can be done by setting or clearing the notification bit in the Client Characteristic configuration for each alert characteristic." ;
        skos:related     ble:Write .

cpp:PedalPowerBalanceField
        a                skos:Concept ;
        rdfs:label       "Pedal Power Balance Field" ;
        skos:definition  "The Pedal Power Balance field represents the ratio between the total amount of power measured by the sensor and a reference." ;
        skos:related     xsd:unsignedByte .

blp:BloodPressureMeasurement
        a                skos:Concept ;
        rdfs:label       "Blood Pressure Measurement" ;
        skos:definition  "The Blood Pressure Measurement characteristic shall be used to send Blood Pressure measurements" ;
        skos:related     blp:BloodPressureMeasurementCompoundValueField , ble:TimeStampField , ble:Indicate , ble:UserIDField , blp:PulseRateField .

lnp:RemainingDistanceField
        a                skos:Concept ;
        rdfs:label       "Remaining Distance Field" ;
        skos:definition  "The Remaining Distance field represents the distance from the current position to the next waypoint or final destination." ;
        skos:related     xsd:unsignedInt .

glp:ExerciseIntensityField
        a                skos:Concept ;
        rdfs:label       "xercise Intensity" ;
        skos:definition  "Field exists if the key of bit 3 of the Flags field is set to 1" ;
        skos:related     xsd:unsignedByte .

idp:BolusIDfield  a      skos:Concept ;
        rdfs:label       "Bolus ID Field" ;
        skos:definition  "The Bolus ID field represents a unique identifier as a uint16 data type created by the Server Application for a programmed bolus." ;
        skos:related     xsd:unsignedShort .

cgmp:CGMGlucoseConcentrationField
        a                skos:Concept ;
        rdfs:label       "CGM Glucose Concentration Field" ;
        skos:definition  "The CGM Glucose Concentration field contains the CGM glucose concentration." ;
        skos:related     xsd:float .

ble:IndoorPositioningService
        a                skos:Concept ;
        rdfs:label       "Indoor Positioning Service" ;
        rdfs:seeAlso     <https://www.bluetooth.org/docman/handlers/downloaddoc.ashx?doc_id=302114> ;
        owl:versionInfo  "1.0" ;
        skos:definition  "The Indoor Positioning Service exposes location information to support mobile devices to position themselves in an environment where GNSS signals are not available, for example in indoor premises." ;
        skos:related     ble:LocationName , ble:LocalEastCoordinate , ble:HTTPHeaders , ble:FloorNumber , ble:Latitude , ble:Longitude , ble:HTTPSSecurity , ble:Altitude , ble:URI , ble:HTTPStatusCode , ble:LocalNorthCoordinate , ble:HTTPControlPoint , ble:HTTPEntityBody , ble:IndoorPositioningConfiguration , ble:Uncertainty .

glp:MedicationIDField
        a                skos:Concept ;
        rdfs:label       "Medication ID" ;
        skos:definition  "Field exists if the key of bit 4 of the Flags field is set to 1" ;
        skos:related     xsd:unsignedByte .

idp:BolusFastAmountfield
        a                skos:Concept ;
        rdfs:label       "Bolus Fast Amount field" ;
        skos:definition  "The Bolus Fast Amount field represents the fast amount of the bolus." ;
        skos:related     xsd:float .

rcp:RCCP  a              skos:Concept ;
        rdfs:label       "Reconnection Configuration Control Point" ;
        skos:definition  "The Reconnection Configuration Control Point (RCCP) characteristic shall be used to execute a supported procedure on the Reconnection Configuration server." ;
        skos:related     ble:Write , ble:Indicate .

lnp:BearingField  a      skos:Concept ;
        rdfs:label       "Bearing Field" ;
        skos:definition  "The Bearing field represents the direction where the user should be heading to reach the next waypoint or final destination." ;
        skos:related     xsd:unsignedShort .

idp:IDDStatusChanged  a  skos:Concept ;
        rdfs:label       "Insulin Delivery Device Status Changed" ;
        skos:definition  "The IDD Status Changed characteristic is comprised of status changes of the insulin therapy and the Insulin Delivery Device." ;
        skos:related     ble:Indicate , ble:Read , idp:E2ECounterfield , idp:E2ECRCfield .

lehid:BootProtocolMode
        a                skos:Concept ;
        rdfs:label       "Boot Protocol Mode" ;
        skos:definition  "A HID Service shall only enter Boot Protocol Mode after this value has been written." .

rcp:ReconnectionConfigurationService
        a                skos:Concept ;
        rdfs:label       "Reconnection Configuration Service" ;
        rdfs:seeAlso     <https://www.bluetooth.org/docman/handlers/downloaddoc.ashx?doc_id=435661> ;
        owl:versionInfo  "1.0" ;
        skos:definition  "This GATT-based service enables the control of certain communication parameters of a Bluetooth Low Energy peripheral device." ;
        skos:related     rcp:RCFeature , rcp:RCCP , rcp:RCSettings .

cpp:InstantaneousTorqueMagnitudeArrayField
        a                skos:Concept ;
        rdfs:label       "Instantaneous Torque Magnitude Array Field" ;
        skos:definition  " Included in this field are one or more Instantaneous Magnitude values which are expressed in Newton meter with a resolution of 1/32 Newton meter" ;
        skos:related     xsd:short .

idp:BolusDelayTime  a    skos:Concept ;
        rdfs:label       "Bolus Delay Time" ;
        skos:definition  "The Bolus Delay Time field represents the delay time of the bolus." ;
        skos:related     xsd:unsignedShort .

lehid:ReportProtocolMode
        a                skos:Concept ;
        rdfs:label       "Report Protocol Mode" ;
        skos:definition  "Default Protocol Mode of all HID Devices." .

ble:LocalEastCoordinate
        a                skos:Concept ;
        rdfs:label       "Local East Coordinate" ;
        skos:definition  "The Local East Coordinate Characteristic describes the East coordinate of the device using a local coordinate system." ;
        skos:related     ble:Write , ble:ReliableWrite , ble:Read , ble:WritewithoutResponse , ble:LocalEastCoordinateValue .

idp:ManufacturerReserved
        a                skos:Concept ;
        rdfs:label       "Manufacturer Reserved Hamming Code Value Range" ;
        skos:definition  "All Hamming codes values in the range of 0xF000 and 0xFFF0 are manufacturer reserved" .

hrp:HeartRateValueField
        a                skos:Concept ;
        rdfs:label       "Heart Rate Measurement Value" ;
        skos:definition  "The Heart Rate Measurement Value field shall be included in the Heart Rate Measurement characteristic." ;
        skos:related     xsd:unsignedShort .

otp:ObjectListFilter  a  skos:Concept ;
        rdfs:label       "Object List Filter" ;
        skos:definition  "If Object List Filter characteristics are exposed, the filter conditions shall determine which objects are included in or excluded from the list of objects. The Object List Filter characteristics can therefore modify the behavior of the Object List Control Point." ;
        skos:related     ble:Write , ble:Read .

cgmp:cgmpMeasurement  a  skos:Concept ;
        rdfs:label       "GCM Measurement" ;
        skos:definition  "The cgmp Measurement characteristic is a variable length structure containing one or more cgmp Measurement records." ;
        skos:related     cgmp:SensorStatusAnnunciationField , cgmp:CGMGlucoseConcentrationField , cgmp:CGMQualityField , cgmp:TimeOffsetField , cgmp:CGMTrendInformationField , cgmp:E2ECRCField , ble:Notify .

ble:HTTPHeaders  a       skos:Concept ;
        rdfs:label       "HTTP Headers" ;
        skos:definition  "The HTTP Headers characteristic is used to hold the headers that would be sent with the HTTP Request or the headers contained within an HTTP response message from the HTTP Server." ;
        skos:related     ble:Write , ble:ReadLong , xsd:string , ble:WriteLong , ble:Read .

ble:FloorNumber  a       skos:Concept ;
        rdfs:label       "Floor Number" ;
        skos:definition  "The Floor Number Characteristic describes the floor number in which the device is installed." ;
        skos:related     ble:Write , ble:ReliableWrite , ble:Read , ble:WritewithoutResponse , ble:FloorNumberValue .

ftmp:InstantaneousCadenceField
        a                skos:Concept ;
        rdfs:label       "Instantaneous Cadence Field" ;
        skos:definition  "The Instantaneous Cadence field represents the instantaneous cadence of the user." ;
        skos:related     xsd:unsignedShort .

wsp:BodyWateField  a     skos:Concept ;
        rdfs:label       "Body Wate Field" ;
        skos:definition  "The Body Water Mass field may be included in the Body Composition Measurement characteristic if the device supports the Body Water Mass feature." ;
        skos:related     xsd:unsignedShort .

wsp:WeightScaleService
        a                skos:Concept ;
        rdfs:label       "Weight Scale Service" ;
        rdfs:seeAlso     <https://www.bluetooth.org/docman/handlers/downloaddoc.ashx?doc_id=293526> ;
        owl:versionInfo  "1.0" ;
        skos:definition  "This service exposes weight and related data from a weight scale intended for consumer healthcare and sports/fitness applications." ;
        skos:related     wsp:WeightScaleFeature , wsp:WeightMeasurement .

ftmp:InclinationField
        a                skos:Concept ;
        rdfs:label       "Inclination Field" ;
        skos:definition  "The Inclination field represents the current inclination of the Server. A positive value means that the user feels as if they are going uphill and a negative value means that the user feels as if they are going downhill." ;
        skos:related     xsd:short .

ftmp:MinimumSpeedfield
        a                skos:Concept ;
        rdfs:label       "Minimum Speed" ;
        skos:definition  "Minimum Kilometer per hour with a resolution of 0.01" ;
        skos:related     xsd:unsignedShort .

glp:MedicationField  a   skos:Concept ;
        rdfs:label       "Medication - units of kilograms" ;
        skos:definition  "C6: Field exists if the key of bit 4 of the Flags field is set to 1, C8: Field exists if the key of bit 5 of the Flags field is set to 0" ;
        skos:related     xsd:float .

rscp:InstantaneousCadenceField
        a                skos:Concept ;
        rdfs:label       "Instantaneous Cadence Field" ;
        skos:definition  "The Instantaneous Cadence represents the number of times per minute a foot fall occurs." ;
        skos:related     xsd:unsignedByte .

lehid:bcdHID  a          skos:Concept ;
        rdfs:label       "Version number of base USB HID Specification" ;
        skos:definition  "16-bit unsigned integer representing version number of base USB HID Specification implemented by HID Device." ;
        skos:related     xsd:unsignedShort .

idp:Off  a               skos:Concept ;
        rdfs:label       "Off" ;
        skos:definition  "The Insulin Delivery Device is switched off and no functionality is available" .

tip:TimewithDST  a       skos:Concept ;
        rdfs:label       "Time with Daylight Saving Time" ;
        skos:definition  "The Next DST Change Server returns the Time with DST to the time when the next DST change will occur and the DST offset that will be in effect after this change." ;
        skos:related     ble:Read .

lnp:BeaconsNumberViewField
        a                skos:Concept ;
        rdfs:label       "Number of Beacons in View Field" ;
        skos:definition  "The Number of Beacons in View field represents the number of beacons from which the Server is receiving data." ;
        skos:related     xsd:unsignedByte .

aiop:Aggregate  a        skos:Concept ;
        rdfs:label       "Aggregate characteristic" ;
        skos:definition  "Aggregate characteristic is used to aggregate all Digital characteristics with the Read property set (if any available) and all of the Analog characteristics with Read properties set (if any available)." ;
        skos:related     ble:Indicate , ble:Read , ble:Notify .

ftmp:AverageStepRateField
        a                skos:Concept ;
        rdfs:label       "Average Step Rate Field" ;
        skos:definition  "The Average Step Rate field represents the average step rate since the beginning of the training session." ;
        skos:related     xsd:unsignedShort .

ftmp:StairClimberData
        a                skos:Concept ;
        rdfs:label       "Stair Climber Data" ;
        skos:definition  "The Stair Climber Data characteristic is used to send training-related data to the Client from a stair climber (Server)." ;
        skos:related     ftmp:FloorsField , ftmp:RemainingTimeField , ftmp:EnergyperMinuteField , ftmp:StepperMinuteRateField , ftmp:AverageStepRateField , ftmp:PositiveElevationGainField , ftmp:EnergyperHourField , ftmp:StrideCountField , ftmp:ElapsedTimeField , ftmp:TotalEnergyField , ftmp:HeartRateField , ftmp:MetabolicEquivalentField , ble:Notify .

ble:LocationNameValue
        a                skos:Concept ;
        rdfs:label       "Location Name Value" ;
        skos:definition  "When read, the Server shall return the current value of the Location Name Characteristic." ;
        skos:related     xsd:string .

otp:ObjectFirstCreatedField
        a                skos:Concept ;
        rdfs:label       "Object First-Created Field" ;
        skos:definition  "The Object First-Created characteristic returns its associated value when read. The date and time value shall be represented in Coordinated Universal Time (UTC)." .

idp:AuxInfo3LowerBoundfield
        a                skos:Concept ;
        rdfs:label       "AuxInfo3 Lower Bound field" ;
        skos:definition  "The AuxInfo3 field shall contain the value of the lower bound of the temperature." ;
        skos:related     xsd:float .

plxp:SpO2PRFastfield  a  skos:Concept ;
        rdfs:label       "Percent oxygen saturation of hemoglobin and Pulse Rate(SpO2PR)-Fast Field" ;
        skos:definition  "The SpO2PR-Fast field reports fast responding oximetry measurements of the sensor." ;
        skos:related     xsd:float .

ble:TransportDiscoveryService
        a                skos:Concept ;
        rdfs:label       "Transport Discovery Service" ;
        rdfs:seeAlso     <https://www.bluetooth.org/docman/handlers/downloaddoc.ashx?doc_id=309929> ;
        owl:versionInfo  "1.0" ;
        skos:definition  "This service enables a device using Bluetooth low energy wireless technology to expose services that are available on a transport other than Bluetooth low energy." ;
        skos:related     ble:TransportDataLengthField , ble:TDSControlPoint , ble:OrganizationIDField , ble:TransportDataField .

idp:TBROver  a           skos:Concept ;
        rdfs:label       "The temporary basal Over" ;
        skos:definition  "The temporary basal rate expired (i.e., the programmed duration is over)." .

ble:AltitudeValue  a     skos:Concept ;
        rdfs:label       "Altitude Value" ;
        skos:definition  "When read, the Server shall return the current value of the Altitude Characteristic." ;
        skos:related     xsd:unsignedShort .

idp:ReservoirLow  a      skos:Concept ;
        rdfs:label       "Reservoir Low" ;
        skos:definition  "The reservoir fill level reached a defined low threshold." .

wsp:BIM  a               skos:Concept ;
        rdfs:label       "Body Mass Index" ;
        skos:definition  "The Body Mass Index may be included in the Weight Measurement characteristic if the device supports the BMI feature." ;
        skos:related     xsd:unsignedShort .

pasp:RingerSetting  a    skos:Concept ;
        rdfs:label       "Ringer Setting" ;
        skos:definition  "The Ringer Setting characteristic exposes the state of the server device's ringer." ;
        skos:related     xsd:unsignedByte , ble:Read , ble:Notify .

ble:Latitude  a          skos:Concept ;
        rdfs:label       "Latitude" ;
        skos:definition  "The Latitude Characteristic describes the global WGS84 North coordinate of the device." ;
        skos:related     ble:Write , ble:ReliableWrite , ble:LatitudeValue , ble:Read , ble:WritewithoutResponse .

anp:NewAlert  a          skos:Concept ;
        rdfs:label       "New Alert" ;
        skos:definition  "The count of new alerts (for a given category) in the server" ;
        skos:related     anp:CategoryID , anp:TextStringInformation , anp:NumberofNewAlert , ble:Notify .

wsp:ImpedanceField  a    skos:Concept ;
        rdfs:label       "Impedance Field" ;
        skos:definition  "The Impedance field may be included in the Body Composition Measurement characteristic if the device supports the Impedance feature." ;
        skos:related     xsd:unsignedShort .

pasp:RingerControlPoint
        a                   skos:Concept ;
        rdfs:label          "Ringer Control Point" ;
        skos:editorialNote  "Not found yet" ;
        skos:related        xsd:unsignedByte , ble:WritewithoutResponse .

ftmp:ResistanceLevelField
        a                skos:Concept ;
        rdfs:label       "Resistance Level Field" ;
        skos:definition  "The Resistance Level field represents the value of the current value of the resistance level of the Server." ;
        skos:related     xsd:short .

htp:HealthThermometerService
        a                skos:Concept ;
        rdfs:label       "Health Thermometer Service" ;
        rdfs:seeAlso     <https://www.bluetooth.org/docman/handlers/downloaddoc.ashx?doc_id=238688> ;
        owl:versionInfo  "1.0" ;
        skos:definition  "This service exposes temperature and other data from a Thermometer intended for healthcare and fitness applications." ;
        skos:related     htp:TemperatureType , htp:ValidRangeDescriptor , htp:IntermediateTemperature , htp:TemperatureMeasurement , htp:MeasurementInterval .

cscp:CyclingSpeedandCadenceService
        a                skos:Concept ;
        rdfs:label       "Cycling Speed and Cadence Service" ;
        rdfs:seeAlso     <https://www.bluetooth.org/docman/handlers/downloaddoc.ashx?doc_id=261450> ;
        owl:versionInfo  "1.0" ;
        skos:definition  "The Cycling Speed and Cadence (CSC) Service exposes speed-related data and/or cadence-related data while using the Cycling Speed and Cadence sensor (Server)." ;
        skos:related     cscp:CSCFeature , cscp:CSCMeasurement , ble:SensorLocation , ble:SCControlPoint .

ftmp:ForceonBeltField
        a                skos:Concept ;
        rdfs:label       "Force on Belt Field" ;
        skos:definition  "The Force on Belt field represents the force being applied to the treadmill belt by the user’s steps" ;
        skos:related     xsd:short .

blp:BloodPressureMeasurementCompoundValueField
        a                skos:Concept ;
        rdfs:label       "Blood Pressure Measurement Compound Value Field" ;
        skos:definition  "It is composed of three subfields: Systolic, Diastolic and Mean Arterial Pressure (MAP)" ;
        skos:related     xsd:float .

lnp:ElevationField  a    skos:Concept ;
        rdfs:label       "Elevation Field" ;
        skos:definition  "The Elevation field represents the value of the elevation measured by the sensor." ;
        skos:related     xsd:integer .

ftmp:MinimumSpeedIncrementfield
        a                skos:Concept ;
        rdfs:label       "Minimum Speed Increment" ;
        skos:definition  "Minimum Meters per second with a resolution of 0.01" ;
        skos:related     xsd:unsignedShort .

rscp:SCControlPoint  skos:related  ble:Write , ble:Indicate .

ble:Longitude  a         skos:Concept ;
        rdfs:label       "Longitude" ;
        skos:definition  "The Longitude Characteristic describes the global WGS84 East coordinate of the device." ;
        skos:related     ble:Write , ble:LongitudeValue , ble:ReliableWrite , ble:Read , ble:WritewithoutResponse .

ftmp:AveragePaceField
        a                skos:Concept ;
        rdfs:label       "Average Pace Field" ;
        skos:definition  "The Average Pace field represents the average pace of a user since the beginning of the training session." ;
        skos:related     xsd:unsignedShort .

glp:HbA1cField  a        skos:Concept ;
        rdfs:label       "Hemoglobin A1c" ;
        skos:definition  "Field exists if the key of bit 6 of the Flags field is set to 1" ;
        skos:related     xsd:float .

ftmp:StrokeCountField
        a                skos:Concept ;
        rdfs:label       "Stroke Count Field" ;
        skos:definition  "The Stroke Count field represents the total number of strokes since the beginning of the training session." ;
        skos:related     xsd:unsignedShort .

idp:AnnunciationStatus
        a                skos:Concept ;
        rdfs:label       "Annunciation Status" ;
        skos:definition  "This Annunciation Status field represents the current status of an annunciation" ;
        skos:narrower    idp:Confirmed , idp:Snoozed , idp:Pending , idp:Undetermined ;
        skos:related     xsd:unsignedByte .

idp:PrimingIssue  a      skos:Concept ;
        rdfs:label       "Priming Issue" ;
        skos:definition  "There is a priming issue after replacement of reservoir and/or infusion set" .

ftmp:InstantaneousPaceField
        a                skos:Concept ;
        rdfs:label       "Instantaneous Pace Field" ;
        skos:definition  "The Instantaneous Pace field represents the instantaneous pace of a user while exercising." ;
        skos:related     xsd:unsignedShort .

idp:InsulinDeliveryProfile
        a                   skos:Concept ;
        rdfs:label          "Insulin Delivery Profile" ;
        owl:versionInfo     "1.0" ;
        skos:editorialNote  "Not found yet, require membership ro get access." ;
        skos:related        idp:InsulinDeliveryService .

ftmp:MinimumHeartRateIncrementfield
        a                skos:Concept ;
        rdfs:label       "Minimum Heart Rate Increment" ;
        skos:definition  "Minimum Beats per minute with a resolution of 1" ;
        skos:related     xsd:unsignedByte .

cpp:MinimumForceMagnitude
        a                skos:Concept ;
        rdfs:label       "Minimum Force Magnitude" ;
        skos:definition  "The Minimum Force Magnitude field represents the minimum force value measured in a single crank revolution." ;
        skos:related     xsd:short .

idp:BatteryLow  a        skos:Concept ;
        rdfs:label       "Battery Low" ;
        skos:definition  "The Insulin Delivery Device has a low operational runtime" .

plxp:SpO2PRSlowfield  a  skos:Concept ;
        rdfs:label       "Percent oxygen saturation of hemoglobin and Pulse Rate(SpO2PR)-Slow Field" ;
        skos:definition  "The SpO2PR-Slow field reports slow responding oximetry measurements of the sensor." ;
        skos:related     xsd:float .

glp:SequenceNumberField
        a                skos:Concept ;
        rdfs:label       "Sequence Number Field" ;
        skos:definition  "The Sequence Number represents the chronological order of the patient records in the Server measurement database." ;
        skos:related     xsd:unsignedShort .

rscp:RunningSpeedandCadenceProfile
        a                skos:Concept ;
        rdfs:label       "Running Speed and Cadence Profile" ;
        rdfs:seeAlso     <https://www.bluetooth.org/docman/handlers/downloaddoc.ashx?doc_id=261266> ;
        owl:versionInfo  "1.0" ;
        skos:definition  "TThe Running Speed and Cadence Profile is used to enable a data collection device to obtain data from a Running Speed and Cadence Sensor (RSC Sensor) that exposes the Running Speed and Cadence Service." ;
        skos:related     ble:DeviceInformationService , rscp:RunningSpeedandCadenceService .

rcp:RCSettings  a        skos:Concept ;
        rdfs:label       "Reconnection Configuration Settings" ;
        skos:definition  "The RC Settings characteristic shall be used to both read and notify supported features on the Reconnection Configuration server." ;
        skos:related     ble:Read , ble:Notify .

otp:OTSFeature  a        skos:Concept ;
        rdfs:label       "Object Transfer Service Feature" ;
        skos:definition  "The OTS Feature characteristic exposes which optional features are supported by the Server implementation." ;
        skos:related     ble:Read .

idp:InsulinDeliveryService
        a                skos:Concept ;
        rdfs:label       "Insulin Delivery Service" ;
        rdfs:seeAlso     <https://www.bluetooth.org/DocMan/handlers/DownloadDoc.ashx?doc_id=447826> ;
        owl:versionInfo  "1.0" ;
        skos:definition  "The Insulin Delivery Service (IDS) exposes the control capability and the status of an Insulin Delivery Device running an insulin infusion therapy." ;
        skos:related     idp:IDDHistoryData , idp:IDDRecordAccessControlPoint , idp:IDDCommandControlPoint , idp:IDDFeatures , idp:IDDStatusChanged , idp:IDDStatus , idp:IDDStatusReaderControlPoint , idp:IDDAnnunciationStatus , idp:IDDCommandData .

lehid:ProtocolModeValue
        a                skos:Concept ;
        rdfs:label       "Protocol Mode Characteristic Value" ;
        skos:definition  "The Protocol Mode characteristic value can have the values representing the current Protocol Mode of the HID Service" ;
        skos:narrower    lehid:BootProtocolMode , lehid:ReportProtocolMode ;
        skos:related     xsd:unsignedByte .

cgmp:CGMQualityField  a  skos:Concept ;
        rdfs:label       "Continuous Glucose Monitoring Quality Field" ;
        skos:definition  "This field contains the CGM Quality information in % as an SFLOAT data type." ;
        skos:related     xsd:float .

idp:EventData  a         skos:Concept ;
        rdfs:label       "Recording Reason field" ;
        skos:definition  "The Recording Reason field specifies the reason why the Reference Time event was recorded." .

idp:AnnunciationInstanceID
        a                skos:Concept ;
        rdfs:label       "Annunciation Instance ID " ;
        skos:definition  "The Annunciation Instance ID field represents a unique identifier as a uint16 data type created by the Server application for all annunciations that occur in the course of time." ;
        skos:related     xsd:unsignedShort .

pasp:AlertStatusValue
        a                skos:Concept ;
        rdfs:label       "Alert Status Value" ;
        skos:definition  "The Alert Status characteristic returns the current value of server’s alert status when read" ;
        skos:related     xsd:unsignedByte .

lehid:BootKeyboardOutputReportValue
        a                skos:Concept ;
        rdfs:label       "Boot Keyboard Output Report Value" ;
        skos:definition  "The Boot Keyboard Output Report characteristic value is an array of octets whose meaning is defined in the USB HID Usage." ;
        skos:related     xsd:unsignedByte .

ble:Property  skos:narrower  ble:WriteLong .

pxp:TxPowerService  a    skos:Concept ;
        rdfs:label       "Transmit (Tx) Power Service" ;
        rdfs:seeAlso     <https://www.bluetooth.org/docman/handlers/downloaddoc.ashx?doc_id=239393> ;
        owl:versionInfo  "1.0" ;
        skos:definition  "This service exposes a device’s current transmit power level when in a connection." ;
        skos:related     pxp:TxPowerLevel .

glp:GlucoseProfile  a    skos:Concept ;
        rdfs:label       "Glucose Profile" ;
        rdfs:seeAlso     <https://www.bluetooth.org/DocMan/handlers/DownloadDoc.ashx?doc_id=248025> ;
        owl:versionInfo  "1.0" ;
        skos:definition  "The Glucose Profile is used to enable a device to obtain glucose measurement and other data from a Glucose Sensor that exposes the Glucose Service." ;
        skos:related     ble:DeviceInformationService , glp:GlucoseService .

ftmp:StrokeRateField  a  skos:Concept ;
        rdfs:label       "Stroke Rate Field" ;
        skos:definition  "The Stroke Rate field represents the instantaneous stroke rate measured by the Server." ;
        skos:related     xsd:unsignedByte .

ble:UncertaintyValue  a  skos:Concept ;
        rdfs:label       "Uncertainty Value" ;
        skos:definition  "When read, the Server shall return the current value of the Uncertainty Characteristic." ;
        skos:related     xsd:unsignedByte .

otp:ObjectType  a        skos:Concept ;
        rdfs:label       "Object Type" ;
        skos:definition  "This characteristic exposes the type of the Current Object, identifying the object type by UUID." ;
        skos:related     ble:Read .

ftmp:SupportedInclinationRange
        a                skos:Concept ;
        rdfs:label       "Supported Inclination Range" ;
        skos:definition  "The Supported Inclination Range characteristic is used to send the supported inclination range as well as the minimum inclination increment supported by the Server." ;
        skos:related     ftmp:MinimumInclinationfield , ftmp:MinimumInclinationIncrementfield , ble:Read , ftmp:MaximumInclinationfield .

ftmp:MinimumPowerIncrementfield
        a                skos:Concept ;
        rdfs:label       "Minimum Power Increment" ;
        skos:definition  "Minimum Watt  with a resolution of 1" ;
        skos:related     xsd:unsignedShort .

aiop:Digital  a          skos:Concept ;
        rdfs:label       "Digital characteristic" ;
        skos:definition  "The Digital characteristic is used to expose and change the state of an IOM’s digital signals." ;
        skos:related     ble:Write , xsd:unsignedByte , ble:Indicate , ble:Read , ble:WritewithoutResponse , ble:Notify .

cpp:LastWheelEventTime
        a                skos:Concept ;
        rdfs:label       "Wheel Revolution Data - Last Wheel Event Time" ;
        skos:definition  "Last Wheel Event Time is one value of The Wheel Revolution Data field pair, always goes in pair with Cumulative Wheel Revolutions field." .

plxp:PulseOximeterService
        a                skos:Concept ;
        rdfs:label       "Pulse Oximeter Service" ;
        rdfs:seeAlso     <https://www.bluetooth.org/DocMan/handlers/DownloadDoc.ashx?doc_id=304965> ;
        owl:versionInfo  "1.0" ;
        skos:definition  "This Service specification defines a pulse oximetry sensor for use in consumer and professional healthcare applications." ;
        skos:related     ble:RecordAccessControlPoint , plxp:PLXFeatures , plxp:PLXContinuousMeasurement , plxp:PLXSpotcheckMeasurement .

glp:GlucoseConcentrationField
        a                skos:Concept ;
        rdfs:label       "Glucose Concentration Field" ;
        skos:definition  "The Glucose Concentration field is optional, but if it is present, the Type-Sample Location field shall also be present." ;
        skos:related     xsd:float .

ftmp:PositiveElevationGainField
        a                skos:Concept ;
        rdfs:label       "Positive Elevation Gain Field" ;
        skos:definition  "The Positive Elevation Gain field represents the positive elevation gain since the beginning of the training session." ;
        skos:related     xsd:unsignedShort .

ftmp:SupportedResistanceLevelRange
        a                skos:Concept ;
        rdfs:label       "Supported Resistance Level Range" ;
        skos:definition  "The Supported Resistance Level Range characteristic is used to send the supported resistance level range as well as the minimum resistance increment supported by the Server." ;
        skos:related     ftmp:MinimumPowerfield , ftmp:MinimumResistanceIncrementfield , ble:Read , ftmp:MaximumResistanceLevelField .

ftmp:PowerOutputField
        a                skos:Concept ;
        rdfs:label       "Power Output Field" ;
        skos:definition  "The Power Output field represents the power being applied to the treadmill by the user’s steps" ;
        skos:related     xsd:short .

esp:EnvironmentalSensingProfile
        a                skos:Concept ;
        rdfs:label       "Environmental Sensing Profile" ;
        rdfs:seeAlso     <https://www.bluetooth.org/docman/handlers/downloaddoc.ashx?doc_id=294796> ;
        owl:versionInfo  "1.0.0" ;
        skos:definition  "This profile enables a Collector device to connect and interact with an Environmental Sensor for use in outdoor activity applications." ;
        skos:related     ble:BatteryService , ble:DeviceInformationService , esp:EnvironmentalSensingService .

lehid:ReportMapValue  a  skos:Concept ;
        rdfs:label       "Report Map Characteristic Value" ;
        skos:definition  "the Report Map characteristic value contains formatting and other information for Input Report, Output Report and Feature Report data transferred between a HID Device and HID Host." ;
        skos:related     xsd:unsignedByte .

rscp:RunningSpeedandCadenceService
        a                skos:Concept ;
        rdfs:label       "Running Speed and Cadence Service" ;
        rdfs:seeAlso     <https://www.bluetooth.org/docman/handlers/downloaddoc.ashx?doc_id=261265> ;
        owl:versionInfo  "1.0" ;
        skos:definition  "This service exposes speed, cadence and other data from a Running Speed and Cadence sensor intended for fitness applications." ;
        skos:related     rscp:SCControlPoint , ble:SensorLocation , rscp:RSCMeasurement , rscp:RSCFeature .

wsp:MusclePercentageField
        a                skos:Concept ;
        rdfs:label       "Muscle Percentage Field" ;
        skos:definition  "The Muscle Percentage field may be included in the Body Composition Measurement characteristic if the device supports the Muscle Percentage feature." ;
        skos:related     xsd:unsignedShort .

cpp:MinimumAngle  a      skos:Concept ;
        rdfs:label       "Minimum Angle Field" ;
        skos:definition  "The Minimum Angle field represents the angle of the crank when the minimum value is measured in the same crank revolution." ;
        skos:related     xsd:unsignedByte .

otp:ObjectIDField  a     skos:Concept ;
        rdfs:label       "Object ID Field" ;
        skos:definition  "The Server shall allocate an Object ID value to each object when the object is created on the Server. The Object ID characteristic returns its associated value when read." ;
        skos:related     xsd:unsignedInt .

wsp:BodyCompositionMeasurement
        a                skos:Concept ;
        rdfs:label       "Body Composition Measurement" ;
        skos:definition  "The Body Composition Measurement characteristic is used to send body composition-related data to the Client." ;
        skos:related     wsp:BodyWateField , wsp:ImpedanceField , ble:Indicate , wsp:MusclePercentageField , ble:UserIDField , wsp:FatFreeMassField , wsp:MuscleMassField , wsp:WeightField , wsp:BodyFatPercentageField , wsp:BasalMetabolismField , wsp:SoftLeanMassField , wsp:HeightField .

idp:Priming  a           skos:Concept ;
        rdfs:label       "Priming" ;
        skos:definition  "The Insulin Delivery Device fills the fluidic path from the reservoir to the body with insulin" .

wsp:BodyCompositionFeature
        a                skos:Concept ;
        rdfs:label       "Body Composition Feature" ;
        skos:definition  "The Body Composition Feature characteristic shall be used to describe the supported features of the Server." ;
        skos:related     ble:Read .

plxp:SpO2PRSpotCheckField
        a                skos:Concept ;
        rdfs:label       "Percent oxygen saturation of hemoglobin and Pulse Rate Spot Check" ;
        skos:definition  "The SpO2PR-Spot-Check field shall be included in the PLX Spot-check Measurement characteristic." ;
        skos:related     xsd:float .

otp:ObjectSize  a        skos:Concept ;
        rdfs:label       "Object Size" ;
        skos:definition  "The Object Size characteristic exposes the current size as well as the allocated size of the Current Object." ;
        skos:related     otp:AllocatedSizeField , otp:CurrentSizeField , ble:Read .

idp:IDDStatus  a         skos:Concept ;
        rdfs:label       "Insulin Delivery Device Status" ;
        skos:definition  "The IDD Status characteristic is comprised of status values of the Insulin Delivery Device and the insulin therapy." ;
        skos:related     idp:TherapyControlStatefield , idp:OperationalStatefield , idp:ReservoirRemainingAmountfield , ble:Indicate , ble:Read , idp:E2ECounterfield , idp:E2ECRCfield .

idp:BatteryEmpty  a      skos:Concept ;
        rdfs:label       "Battery Empty" ;
        skos:definition  "The Insulin Delivery Device has no operational runtime left" .

tip:NextDSTChangeService
        a                skos:Concept ;
        rdfs:label       "Daylight Saving Time Change Service" ;
        rdfs:seeAlso     <https://www.bluetooth.org/docman/handlers/downloaddoc.ashx?doc_id=241872> ;
        owl:versionInfo  "1.0" ;
        skos:definition  "This service defines how the information about an upcoming DST change can be exposed using the Generic Attribute Profile (GATT)." ;
        skos:related     tip:TimewithDST .

cscp:CumulativeWheelRevolutions
        a                skos:Concept ;
        rdfs:label       "Cumulative Wheel Revolutions" ;
        skos:definition  "The Cumulative Wheel Revolutions value and the Last Wheel Event Time value allow the Client to calculate the speed (instantaneous and average) as well as the distance travelled." ;
        skos:related     xsd:unsignedInt .

glp:BaseTimeField  a     skos:Concept ;
        rdfs:label       "Base Time Field" ;
        skos:definition  "The Base Time field represents the value of an internal real-time clock or equivalent that keeps time relative to its initial setting in resolution of seconds." .

ftmp:AverageCadenceField
        a                skos:Concept ;
        rdfs:label       "Average Cadence Field" ;
        skos:definition  "The Average Speed field represents the average cadence since the beginning of the training session." ;
        skos:related     xsd:unsignedShort .

tip:TimeProfile  a       skos:Concept ;
        rdfs:label       "Time Profile" ;
        rdfs:seeAlso     <https://www.bluetooth.org/docman/handlers/downloaddoc.ashx?doc_id=241874> ;
        owl:versionInfo  "1.0" ;
        skos:definition  "The Time profile enables the device to get the date, time, time zone, and DST information and control the functions related the time." ;
        skos:related     ble:CurrentTimeService , tip:NextDSTChangeService , tip:ReferenceTimeUpdateService .

pasp:PhoneAlertStatusProfile
        a                skos:Concept ;
        rdfs:label       "Phone Alert Status Profile" ;
        rdfs:seeAlso     <https://www.bluetooth.org/docman/handlers/downloaddoc.ashx?doc_id=241861> ;
        owl:versionInfo  "1.0" ;
        skos:definition  "This profile enables a PUID device to alert its user about the alert status of a phone connected to the PUID device." ;
        skos:related     pasp:PhoneAlertStatusService .

idp:Confirmed  a         skos:Concept ;
        rdfs:label       "Confirmed" ;
        skos:definition  "The annunciation was confirmed by the user" .

glp:GlucoseService  a    skos:Concept ;
        rdfs:label       "Glucose Service" ;
        rdfs:seeAlso     <https://www.bluetooth.org/docman/handlers/downloaddoc.ashx?doc_id=248026> ;
        owl:versionInfo  "1.0" ;
        skos:definition  "The Glucose Service exposes glucose and other data related to a personal glucose sensor for consumer healthcare applications and is not designed for clinical use." ;
        skos:related     glp:GlucoseMeasurementContext , ble:RecordAccessControlPoint , glp:GlucoseMeasurement , glp:GlucoseFeature .

ftmp:MaximumPowerfield
        a                skos:Concept ;
        rdfs:label       "Maximum Power" ;
        skos:definition  "Maximum Watt  with a resolution of 1" ;
        skos:related     xsd:short .

idp:Pause  a             skos:Concept ;
        rdfs:label       "Pause" ;
        skos:definition  "The insulin infusion therapy is paused (i.e., the device does not deliver insulin related to the therapy but delivers the missed amount of insulin after leaving state Pause and entering state Run)." .

lehid:ProtocolMode  a    skos:Concept ;
        rdfs:label       "Protocol Mode" ;
        skos:definition  "The Protocol Mode characteristic is used to expose the current protocol mode of the HID Service with which it is associated, or to set the desired protocol mode of the HID Service." ;
        skos:related     lehid:ProtocolModeValue , ble:Read , ble:WritewithoutResponse .

ftmp:EnergyperHourField
        a                skos:Concept ;
        rdfs:label       "Energy per Hour Field" ;
        skos:definition  "The Energy per Hour field represents the average expended energy of a user during a period of one hour." ;
        skos:related     xsd:short .

pasp:PhoneAlertStatusService
        a                skos:Concept ;
        rdfs:label       "Phone Alert Status Service" ;
        rdfs:seeAlso     <https://www.bluetooth.org/docman/handlers/downloaddoc.ashx?doc_id=241862> ;
        owl:versionInfo  "1.0" ;
        skos:definition  "This service exposes the phone alert status when in a connection." ;
        skos:related     pasp:RingerSetting , pasp:RingerControlPoint , pasp:AlertStatus .

cgmp:TimeOffsetField  a  skos:Concept ;
        rdfs:label       "Time Offset Field" ;
        skos:definition  "The Time Offset field is used in conjunction with the CGM Session Start Time to represent the time difference of the separate CGM measurements in relation to the session start time." ;
        skos:related     xsd:unsignedShort .

pxp:TxPowerLevelField
        a                skos:Concept ;
        rdfs:label       "Transmit Power Level Field" ;
        skos:definition  "The Tx Power Level characteristic returns the current transmit power level when read using the GATT Characteristic Read Value procedure." ;
        skos:related     xsd:byte .

hrp:HeartRateControlPoint
        a                skos:Concept ;
        rdfs:label       "Heart Rate Control Point" ;
        skos:definition  "The Heart Rate Control Point characteristic is used to enable a Client to write control points to a Server to control behavior." ;
        skos:related     ble:Write .

ftmp:FitnessMachineProfile
        a                skos:Concept ;
        rdfs:label       "Fitness Machine Profile" ;
        rdfs:seeAlso     <https://www.bluetooth.org/DocMan/handlers/DownloadDoc.ashx?doc_id=423417> ;
        owl:versionInfo  "1.0" ;
        skos:definition  "The Fitness Machine Profile is used to enable a data collection device to obtain data from a Fitness Machine that exposes the Fitness Machine Service." ;
        skos:related     ble:DeviceInformationService , ble:UserDataService , ftmp:FitnessMachineService .

idp:PowerSourceInsufficient
        a                skos:Concept ;
        rdfs:label       "Power Source Insufficient" ;
        skos:definition  "The Insulin Delivery Device has insufficient power to charge the device" .

htp:TemperatureMeasurementValueField
        a                skos:Concept ;
        rdfs:label       "Temperature Measurement Value Field" ;
        skos:definition  "This Temperature Measurement Value field shall be included in the Temperature Measurement characteristic." ;
        skos:related     xsd:float .

ftmp:AverageSpeedField
        a                skos:Concept ;
        rdfs:label       "Average Speed Field" ;
        skos:definition  "The Average Speed field represents the average speed since the beginning of the training session." ;
        skos:related     xsd:unsignedShort .

plxp:SpO2PRNormalfield
        a                skos:Concept ;
        rdfs:label       "Percent oxygen saturation of hemoglobin and Pulse Rate (SpO2PR)-Normal Field" ;
        skos:definition  "The SpO2PR-Normal field shall be included in the PLX Continuous Measurement characteristic." ;
        skos:related     xsd:float .

otp:ObjectListControlPoint
        a                skos:Concept ;
        rdfs:label       "Object List Control Point" ;
        skos:definition  "The role of the OLCP is to provide a mechanism for the Client to find the desired object and to designate it as the Current Object." ;
        skos:related     ble:Write , ble:Indicate .

htp:HealthThermometerProfile
        a                skos:Concept ;
        rdfs:label       "Health Thermometer Profile" ;
        rdfs:seeAlso     <https://www.bluetooth.org/docman/handlers/downloaddoc.ashx?doc_id=238687> ;
        owl:versionInfo  "1.0" ;
        skos:definition  "This profile enables a Collector device to connect and interact with a Thermometer sensor for use in healthcare applications." ;
        skos:related     htp:HealthThermometerService , ble:DeviceInformationService .

lnp:BeaconsNumberSolutionField
        a                skos:Concept ;
        rdfs:label       "Number of Beacons in Solution Field" ;
        skos:definition  "The Number of Beacons in Solution field represents the number of beacons used to calculate the current position." ;
        skos:related     xsd:unsignedByte .

idp:Snoozed  a           skos:Concept ;
        rdfs:label       "Snoozed" ;
        skos:definition  "The annunciation was noticed by the user and is set to pop up again at a short time later" .

cpp:CyclingPowerService
        a                skos:Concept ;
        rdfs:label       "Cycling Power Service" ;
        rdfs:seeAlso     <https://www.bluetooth.org/DocMan/handlers/DownloadDoc.ashx?doc_id=412770> ;
        owl:versionInfo  "1.1" ;
        skos:definition  "The Cycling Power (CP) Service exposes power- and force-related data and optionally speed- and cadence-related data from a Cycling Power sensor (Server) intended for sports and fitness applications." ;
        skos:related     cpp:CyclingPowerFeature , cpp:CyclingPowerVector , ble:SensorLocation , cpp:CyclingPowerMeasurement , cpp:CyclingPowerControlPoint .

aiop:AutomationIOService
        a                skos:Concept ;
        rdfs:label       "Automation Input/Output Service" ;
        rdfs:seeAlso     <https://www.bluetooth.org/DocMan/handlers/DownloadDoc.ashx?doc_id=304972> ;
        owl:versionInfo  "1.0.0" ;
        skos:definition  "The Automation IO service is used to expose the analog inputs/outputs and digital input/outputs of a generic IO module." ;
        skos:related     aiop:Aggregate , aiop:Digital , aiop:Analog .

tip:TimeUpdateState  a   skos:Concept ;
        rdfs:label       "Time Update State" ;
        skos:definition  "The Time Update State characteristic returns the current state of the reference time update on the Reference Time Update server." ;
        skos:related     xsd:unsignedByte , ble:Read .

htp:IntermediateTemperatureValueField
        a                skos:Concept ;
        rdfs:label       "Intermediate Temperature Value Field" ;
        skos:definition  "This Intermediate Temperature Value field shall be included in the Intermediate Temperature characteristic." ;
        skos:related     xsd:float , htp:TimeStampField .

aiop:AnalogSignalValue
        a                skos:Concept ;
        rdfs:label       "Value of an analog signal" ;
        skos:definition  "The Analog characteristic represents the value of an analog signal as an unsigned 16-bit integer (uint16)." ;
        skos:related     xsd:unsignedShort .

hrp:HeartRateService  a  skos:Concept ;
        rdfs:label       "Heart Rate Service" ;
        rdfs:seeAlso     <https://www.bluetooth.org/docman/handlers/downloaddoc.ashx?doc_id=239866> ;
        owl:versionInfo  "1.0" ;
        skos:definition  "The Heart Rate Service exposes heart rate and other data related to a heart rate sensor intended for fitness applications." ;
        skos:related     hrp:BodySensorLocation , hrp:HeartRateControlPoint , hrp:HeartRateMeasurement .

anp:UnreadAlertStatus
        a                skos:Concept ;
        rdfs:label       "Unread Alert Status" ;
        skos:definition  "The count of unread alert events existing in the server. The count of unread alert events is provided with the Category ID." ;
        skos:related     ble:Notify .

ftmp:HighIntensityInterval
        a                skos:Concept ;
        rdfs:label       "High Intensity Interval" ;
        skos:definition  "0x04 - High Intensity Interval" .

ftmp:AveragePowerField
        a                skos:Concept ;
        rdfs:label       "Average Power Field" ;
        skos:definition  "The Average Power field represents the value of the average power measured by the Server since the beginning of the training session." ;
        skos:related     xsd:short .

ftmp:WarmingUp  a        skos:Concept ;
        rdfs:label       "Warming Up" ;
        skos:definition  "0x02 - Warming Up" .

glp:GlucoseMeasurement
        a                skos:Concept ;
        rdfs:label       "Glucose Measurement" ;
        skos:definition  "The Glucose Measurement characteristic shall be used to send glucose measurements." ;
        skos:related     glp:SequenceNumberField , glp:GlucoseConcentrationField , glp:BaseTimeField , glp:TimeOffsetField .

ble:LongitudeValue  a    skos:Concept ;
        rdfs:label       "The current value of the Longitude Characteristic" ;
        skos:definition  "When read, the Server shall return the current value of the Longitude Characteristic." ;
        skos:related     xsd:integer .

wsp:WeightMeasurement
        a                skos:Concept ;
        rdfs:label       "Weight Measurement" ;
        skos:definition  "The Weight Measurement characteristic is used to send weight-related data to the Client." ;
        skos:related     wsp:TimeStampField , wsp:BIM , wsp:UserIDField , ble:Indicate , wsp:WeightField , wsp:HeightField .

lehid:ReportValue  a     skos:Concept ;
        rdfs:label       "Report Value" ;
        skos:definition  "The Report characteristic value contains Input Report, Output Report or Feature Report data to be transferred between the HID Device and HID Host." ;
        skos:related     xsd:unsignedByte .

lehid:HIDControlPoint
        a                skos:Concept ;
        rdfs:label       "HID Control Point" ;
        skos:definition  "The HID Control Point characteristic is a control-point attribute that defines Suspend and Exit Suspend HID Commands when written." ;
        skos:related     lehid:HIDControlPointCharacteristicValue , ble:WritewithoutResponse .

ble:Profile  skos:narrower  pxp:Proximityprofile , cgmp:ContinuousGlucoseMonitoringProfile , anp:AlertNotificationProfile , rcp:ReconnectionConfigurationProfile , cscp:CyclingSpeedandCadenceProfile , lehid:HIDoverGATTProfile , idp:InsulinDeliveryProfile , rscp:RunningSpeedandCadenceProfile , glp:GlucoseProfile , esp:EnvironmentalSensingProfile , tip:TimeProfile , pasp:PhoneAlertStatusProfile , ftmp:FitnessMachineProfile , htp:HealthThermometerProfile , cpp:CyclingPowerProfile , blp:BloodPressureProfile , lnp:LocationandNavigationProfile , scpp:ScanParametersProfile , aiop:AutomationIOProfile , otp:ObjectTransferProfile , wsp:WeightScaleProfile , hrp:HeartRateProfile , fmp:FindMeProfile , ipsp:InternetProtocolSupportProfile , plxp:PulseOximeterProfile .

idp:Standby  a           skos:Concept ;
        rdfs:label       "Stand By" ;
        skos:definition  "No insulin is delivered and resuming from this state is faster than from state Off" .

idp:BatteryFull  a       skos:Concept ;
        rdfs:label       "Battery Full" ;
        skos:definition  "The Insulin Delivery Device has a full operational runtime" .

glp:ExerciseDurationField
        a                skos:Concept ;
        rdfs:label       "Exercise Duration" ;
        skos:definition  "Field exists if the key of bit 3 of the Flags field is set to 1" ;
        skos:related     xsd:unsignedShort .

ble:TDSControlPoint  a   skos:Concept ;
        rdfs:label       "Transport Discovery Control Point" ;
        skos:definition  "The TDS Control Point characteristic is used to request activation of a transport." .

cpp:CyclingPowerProfile
        a                skos:Concept ;
        rdfs:label       "Cycling Power Profile" ;
        rdfs:seeAlso     <https://www.bluetooth.org/DocMan/handlers/DownloadDoc.ashx?doc_id=412769> ;
        owl:versionInfo  "1.1" ;
        skos:definition  "The Cycling Power Profile is used to enable a data collection device to obtain data from a Cycling Power Sensor (CP Sensor) that exposes the Cycling Power Service." ;
        skos:related     ble:BatteryService , ble:DeviceInformationService , cpp:CyclingPowerService .

htp:TemperatureMeasurement
        a                skos:Concept ;
        rdfs:label       "Temperature Measurement" ;
        skos:definition  "The Temperature Measurement characteristic is used to send a temperature measurement." ;
        skos:related     ble:TimeStampField , ble:Indicate , htp:TemperatureMeasurementValueField , htp:IntermediateTemperatureValueField .

blp:IntermediateCuffPressureCompoundValueField
        a                skos:Concept ;
        rdfs:label       "Intermediate Cuff Pressure Compound Value Field" ;
        skos:definition  "This Intermediate Cuff Pressure Compound Value field is composed of three subfields: Current Cuff Pressure and two unused subfields and is included in the Intermediate Cuff Pressure characteristic." ;
        skos:related     xsd:float .

blp:BloodPressureProfile
        a                skos:Concept ;
        rdfs:label       "Blood Pressure Profile" ;
        rdfs:seeAlso     <https://www.bluetooth.org/docman/handlers/downloaddoc.ashx?doc_id=457086> ;
        owl:versionInfo  "1.0.1" ;
        skos:definition  "The Blood Pressure Profile is used to enable a device to obtain blood pressure measurement and other data from a non-invasive blood pressure sensor that exposes the Blood Pressure Service." ;
        skos:related     ble:DeviceInformationService , blp:BloodPressureService .

ftmp:RampAngleSettingField
        a                skos:Concept ;
        rdfs:label       "Ramp Angle Setting Field" ;
        skos:definition  "The Ramp Angle Setting field represents the current setting of the ramp angle of the Server." ;
        skos:related     xsd:short .

idp:IDDStatusReaderControlPoint
        a                skos:Concept ;
        rdfs:label       "Insulin Delivery Device Status Reader Control Point" ;
        skos:definition  "The IDD Status Reader Control Point provides insulin therapy relevant status information (e.g., currently running boluses or current basal rate)." ;
        skos:related     ble:Write , idp:BolusIDfield , idp:BolusFastAmountfield , idp:BolusDelayTime , ble:Indicate , idp:BolusDurationfield , idp:BolusExtendedAmountfield , idp:E2ECounterfield , idp:E2ECRCfield .

tip:ReferenceTimeUpdateService
        a                skos:Concept ;
        rdfs:label       "Reference Time Update Service" ;
        rdfs:seeAlso     <https://www.bluetooth.org/docman/handlers/downloaddoc.ashx?doc_id=241873> ;
        owl:versionInfo  "1.0" ;
        skos:definition  "This service defines how a client can request an update from a reference time source from a time server using the Generic Attribute Profile (GATT)." ;
        skos:related     tip:TimeUpdateState , tip:TimeUpdateControlPoint .

idp:SequenceNumberfield
        a                skos:Concept ;
        rdfs:label       "Sequence Number field" ;
        skos:definition  "The Sequence Number shall be assigned to each IDD History Data characteristic value to maintain the chronological order of the history records in the Server history database." ;
        skos:related     xsd:unsignedInt .

ftmp:MinimumResistanceLevelField
        a                skos:Concept ;
        rdfs:label       "Minimum Resistance Level" ;
        skos:definition  "Unitless with a resolution of 0.1" ;
        skos:related     xsd:short .

glp:CarbohydrateIDField
        a                skos:Concept ;
        rdfs:label       "Carbohydrate ID Field" ;
        skos:definition  "Field exists if the key of bit 0 of the Flags field is set to 1." ;
        skos:related     xsd:unsignedByte .

cgmp:DTSOffsetField  a   skos:Concept ;
        rdfs:label       "Daylight Saving Time Offset Field" ;
        skos:definition  "To know an absolute Time, it is also necessary to know the Daylight Saving setting" ;
        skos:related     xsd:unsignedByte .

idp:InsulinConcentrationfield
        a                skos:Concept ;
        rdfs:label       "Insulin Concentration field" ;
        skos:definition  "The Insulin Concentration field shall be included in the IDD Features characteristic to expose the intended insulin concentration of the Insulin Delivery Device." .

lnp:EHPEField  a         skos:Concept ;
        rdfs:label       "Estimated Horizontal Position Error  Field" ;
        skos:definition  "The EHPE field represents the Estimated Horizontal Position Error, i.e., a measure of the error in a position in the horizontal plane." ;
        skos:related     xsd:unsignedInt .

otp:ObjectFirstCreated
        a                skos:Concept ;
        rdfs:label       "Object First Created" ;
        skos:definition  "The Object First-Created characteristic exposes a value representing a date and time when the object contents were first created." ;
        skos:related     ble:Write , otp:ObjectFirstCreatedField , ble:Read .

ftmp:MinimumPowerfield
        a                skos:Concept ;
        rdfs:label       "Minimum Power" ;
        skos:definition  "Minimum Watt  with a resolution of 1" ;
        skos:related     xsd:short .

otp:ObjectLastModifiedField
        a                skos:Concept ;
        rdfs:label       "Object Last-Modified Field" ;
        skos:definition  "The Object Last-Modified characteristic returns its associated value when read. The date and time value shall be represented in Coordinated Universal Time (UTC)." .

cgmp:cgmpSessionRunTimeField
        a                skos:Concept ;
        rdfs:label       "Session Run Time Field" ;
        skos:definition  "The CGM Session Run Time shall define the expected run time of the CGM session" ;
        skos:related     xsd:unsignedShort .

cpp:TopDeadSpotAngleField
        a                skos:Concept ;
        rdfs:label       "Top Dead Spot Angle Field" ;
        skos:definition  "The Top Dead Spot Angle field represents the crank angle when the value of the Instantaneous Power value becomes positive." ;
        skos:related     xsd:unsignedShort .

ftmp:MaximumHeartRatefield
        a                skos:Concept ;
        rdfs:label       "Maximum Heart Rate" ;
        skos:definition  "Maximum Beats per minute with a resolution of 1" ;
        skos:related     xsd:unsignedByte .

idp:RelativeOffsetfield
        a                skos:Concept ;
        rdfs:label       "Relative Offset field" ;
        skos:definition  "The Relative Offset field represents the elapsed time in seconds since the last recorded Reference Time event." ;
        skos:related     xsd:unsignedShort .

lehid:ReportMap  a       skos:Concept ;
        rdfs:label       "Report Map" ;
        skos:definition  "The Report Map characteristic is used to define formatting information for Input Report, Output Report, and Feature Report data transferred between a HID Device and HID Host." ;
        skos:related     lehid:ReportMapValue , ble:Read .

ftmp:FitnessMachineService
        a                skos:Concept ;
        rdfs:label       "Fitness Machine Service" ;
        rdfs:seeAlso     <https://www.bluetooth.org/DocMan/handlers/DownloadDoc.ashx?doc_id=423422> ;
        owl:versionInfo  "1.0" ;
        skos:definition  "The Fitness Machine Service (FTMS) exposes training-related data in the sports and fitness environment, which allows a Client to collect training data while a user is exercising with a fitness machine (Server)." ;
        skos:related     ftmp:TrainingStatus , ftmp:RowerData , ftmp:StairClimberData , ftmp:SupportedInclinationRange , ftmp:SupportedResistanceLevelRange , ftmp:TreadmillData , ftmp:CrossTrainerData , ftmp:FitnessMachineStatus , ftmp:SupportedHeartRateRange , ftmp:FitnessMachineControlPoint , ftmp:FitnessMachineFeature , ftmp:SupportedSpeedRange , ftmp:IndoorBikeData , ftmp:StepClimberData , ftmp:SupportedPowerRange .

ble:Service  skos:narrower  lnp:LocationandNavigationService , otp:ObjectTransferService , ble:IndoorPositioningService , rcp:ReconnectionConfigurationService , wsp:WeightScaleService , ble:TransportDiscoveryService , htp:HealthThermometerService , cscp:CyclingSpeedandCadenceService , idp:InsulinDeliveryService , pxp:TxPowerService , plxp:PulseOximeterService , rscp:RunningSpeedandCadenceService , tip:NextDSTChangeService , glp:GlucoseService , pasp:PhoneAlertStatusService , cpp:CyclingPowerService , aiop:AutomationIOService , hrp:HeartRateService , tip:ReferenceTimeUpdateService , ftmp:FitnessMachineService , pxp:LinkLossService , wsp:BodyCompositionService , esp:EnvironmentalSensingService , lehid:HIDService , blp:BloodPressureService , anp:AlertNotificationService , ble:HTTPProxyService , cgmp:cgmpService , ipsp:IPSupportService .

pxp:LinkLossService  a   skos:Concept ;
        rdfs:label       "Link Loss Service" ;
        rdfs:seeAlso     <https://www.bluetooth.org/DocMan/handlers/DownloadDoc.ashx?doc_id=303198> ;
        owl:versionInfo  "1.0.1" ;
        skos:definition  "This service defines behavior when a link is lost between two devices." ;
        skos:related     pxp:LinkLossAlertLevel .

idp:SystemIssue  a       skos:Concept ;
        rdfs:label       "System Issue" ;
        skos:definition  "A general device fault or system error occurred (e.g., electronical or software error)." .

wsp:FatFreeMassField  a  skos:Concept ;
        rdfs:label       "Fat Free Mass Field" ;
        skos:definition  "The Fat Free Mass field may be included in the Body Composition Measurement characteristic if the device supports the Fat Free Mass feature." ;
        skos:related     xsd:unsignedShort .

wsp:MuscleMassField  a   skos:Concept ;
        rdfs:label       "Muscle Mass Field" ;
        skos:definition  "The Muscle Mass field may be included in the Body Composition Measurement characteristic if the device supports the Muscle Mass feature." ;
        skos:related     xsd:unsignedShort .

otp:ObjectProperties  a  skos:Concept ;
        rdfs:label       "Object Properties" ;
        skos:definition  "This characteristic exposes a bit field representing the properties of the Current Object." ;
        skos:related     ble:Write , ble:Read .

wsp:WeightField  a       skos:Concept ;
        rdfs:label       "Weight Field" ;
        skos:definition  "The Weight field may be included in the Body Composition Measurement characteristic if the device supports the Weight feature.The Weight field shall be included in the Weight Measurement characteristic" ;
        skos:related     xsd:unsignedShort .

ftmp:TreadmillData  a    skos:Concept ;
        rdfs:label       "Treadmill Data" ;
        skos:definition  "The Treadmill Data characteristic is used to send training-related data to the Client from a treadmill (Server)." ;
        skos:related     ftmp:RemainingTimeField , ftmp:EnergyperMinuteField , ftmp:InclinationField , ftmp:ForceonBeltField , ftmp:AveragePaceField , ftmp:InstantaneousPaceField , ble:InstantaneousSpeedField , ftmp:PositiveElevationGainField , ftmp:PowerOutputField , ftmp:EnergyperHourField , ftmp:AverageSpeedField , ftmp:RampAngleSettingField , ftmp:ElapsedTimeField , ftmp:TotalEnergyField , ftmp:HeartRateField , ftmp:MetabolicEquivalentField , ble:Notify , ftmp:NegativeElevationGainField , ftmp:TotalDistanceField .

lnp:HeadingField  a      skos:Concept ;
        rdfs:label       "Heading Field" ;
        skos:definition  "The Heading field represents the direction the user is heading." ;
        skos:related     xsd:unsignedShort .

idp:Pending  a           skos:Concept ;
        rdfs:label       "Pending" ;
        skos:definition  "The annunciation is currently pending and requires a user action for snoozing or confirmation" .

lnp:LocationandNavigationProfile
        a                skos:Concept ;
        rdfs:label       "Location and Navigation Profile" ;
        rdfs:seeAlso     <https://www.bluetooth.org/DocMan/handlers/DownloadDoc.ashx?doc_id=271996> ;
        owl:versionInfo  "1.0" ;
        skos:definition  "This profile enables a Collector device to connect and interact with a Location and Navigation Sensor for use in outdoor activity applications." ;
        skos:related     ble:BatteryService , lnp:LocationandNavigationService , ble:DeviceInformationService .

wsp:BodyFatPercentageField
        a                skos:Concept ;
        rdfs:label       "Body Fat Percentage Field" ;
        skos:definition  "The Body Fat Percentage field shall be included in the Body Composition Measurement characteristic." ;
        skos:related     xsd:unsignedShort .

rscp:SCControlpoint  a   skos:Concept ;
        rdfs:label       "Speed and Cadance Control Point" ;
        skos:definition  "If the SC Control Point is supported, profiles utilizing this service are required to ensure that the Client configures the SC Control Point characteristic for indications (i.e. via the Client Characteristic Configuration descriptor) at the first connection." .

idp:Run  a               skos:Concept ;
        rdfs:label       "Run" ;
        skos:definition  "The insulin infusion therapy is running (i.e., the device delivers insulin related to the therapy)." .

scpp:ScanParametersProfile
        a                skos:Concept ;
        rdfs:label       "Scan Parameters Profile" ;
        rdfs:seeAlso     <https://www.bluetooth.org/docman/handlers/downloaddoc.ashx?doc_id=245142> ;
        owl:versionInfo  "1.0" ;
        skos:definition  "This profile defines how a Scan Client device with Bluetooth low energy wireless communications can write its scanning behavior to a Scan Server, and how a Scan Server can request updates of a Scan Client scanning behavior." ;
        skos:related     ble:ScanParametersService .

lehid:BootMouseInputReportValue
        a                skos:Concept ;
        rdfs:label       "Boot Mouse Input Report Value" ;
        skos:definition  "The Boot Mouse Input Report characteristic value is an array of octets whose meaning is defined in the USB HID Usage." ;
        skos:related     xsd:unsignedByte .

ble:HTTPSSecurity  a     skos:Concept ;
        rdfs:label       "HTTPS Security" ;
        skos:definition  "The HTTPS Security characteristic contains the known authenticity of the HTTP Server certificate for the URI." ;
        skos:related     xsd:boolean , ble:Read .

ftmp:StepCountField  a   skos:Concept ;
        rdfs:label       "Step Count Field" ;
        skos:definition  "The Step Count field represents the total number of steps counted by the Server since the beginning of the training session." ;
        skos:related     xsd:unsignedShort .

ftmp:Isometric  a        skos:Concept ;
        rdfs:label       "Isometric" ;
        skos:definition  "0x06-Isometric" .

blp:IntermediateCuffPressure
        a                skos:Concept ;
        rdfs:label       "Intermediate Cuff Pressure" ;
        skos:definition  "The Intermediate Cuff Pressure characteristic may be used to send Current Cuff Pressure values to a device for display purposes while the measurement is in progress" ;
        skos:related     ble:UserIDField , blp:IntermediateCuffPressureCompoundValueField , ble:Notify , blp:PulseRateField , blp:TimeStampField .

pxp:LinkLossAlertLevel
        a                skos:Concept ;
        rdfs:label       "Alert Level of Link Loss Service" ;
        skos:definition  "The Alert Level characteristic is used to expose the current link loss alert level that is used to determine how the device alerts when the link is lost." ;
        skos:related     ble:Write , xsd:unsignedByte , ble:Read .

ftmp:CrossTrainerData
        a                skos:Concept ;
        rdfs:label       "Cross Trainer Data" ;
        skos:definition  "The Cross Trainer Data characteristic is used to send training-related data to the Client from a cross trainer (Server)." ;
        skos:related     ftmp:StepperMinuteField , ftmp:RemainingTimeField , ftmp:EnergyperMinuteField , ftmp:InclinationField , ftmp:AverageStepRateField , ftmp:ResistanceLevelField , ble:InstantaneousPowerField , ble:InstantaneousSpeedField , ftmp:PositiveElevationGainField , ftmp:EnergyperHourField , ftmp:AverageSpeedField , ftmp:AveragePowerField , ftmp:RampAngleSettingField , ftmp:StrideCountField , ftmp:ElapsedTimeField , ftmp:TotalEnergyField , ftmp:HeartRateField , ftmp:MetabolicEquivalentField , ble:Notify , ftmp:NegativeElevationGainField , ftmp:TotalDistanceField .

ble:LocalNorthCoordinateValue
        a                skos:Concept ;
        rdfs:label       "The current value of the Local North Coordinate Characteristic" ;
        skos:definition  "When read, the Server shall return the current value of the Local North Coordinate Characteristic." ;
        skos:related     xsd:Short .

idp:OcclusionDetected
        a                skos:Concept ;
        rdfs:label       "Occlusion Detected" ;
        skos:definition  "An occlusion occurred (e.g., clogging of infusion set)." .

idp:AuxInfo1Valuefield
        a                skos:Concept ;
        rdfs:label       " AuxInfo1 Value field" ;
        skos:definition  "The AuxInfo1 field shall contain the value of the temperature." ;
        skos:related     xsd:float .

cpp:CumulativeWheelRevolutions
        a                skos:Concept ;
        rdfs:label       "Wheel Revolution Data - Cumulative Wheel Revolutions" ;
        skos:definition  "The Cumulative Wheel Revolutions value, one value of The Wheel Revolution Data field pair, represents the number of times a wheel rotates" ;
        skos:related     xsd:unsignedInt , xsd:unsignedShort .

wsp:BodyCompositionService
        a                skos:Concept ;
        rdfs:label       "Body Composition Service" ;
        rdfs:seeAlso     <https://www.bluetooth.org/docman/handlers/downloaddoc.ashx?doc_id=293523> ;
        owl:versionInfo  "1.0" ;
        skos:definition  "This service exposes data related to body composition from a body composition analyzer intended for consumer healthcare and sports/fitness applications." ;
        skos:related     wsp:BodyCompositionMeasurement , wsp:BodyCompositionFeature .

rscp:InstantaneousStrideLengthField
        a                skos:Concept ;
        rdfs:label       "Instantaneous Stride Length Field" ;
        skos:definition  "The Instantaneous Stride Length field may be included in the RSC Measurement characteristic if the device supports the Instantaneous Stride Length feature." ;
        skos:related     xsd:unsignedShort .

cgmp:CGMTrendInformationField
        a                skos:Concept ;
        rdfs:label       "Continuous Glucose Monitoring Trend Information Field" ;
        skos:definition  "This field contains the CGM Trend information in (mg/dL)/min as an SFLOAT data type" ;
        skos:related     xsd:float .

glp:GlucoseFeature  a    skos:Concept ;
        rdfs:label       "Glucose Feature" ;
        skos:definition  "The Glucose Feature characteristic shall be used to describe the supported features of the Server." .

ftmp:TrainingStatusStringField
        a                skos:Concept ;
        rdfs:label       "Training Status String Field" ;
        skos:definition  "The Training Status String field is a string-based field that can be used to give more specific information related to the training status." ;
        skos:related     xsd:string .

esp:EnvironmentalSensingService
        a                skos:Concept ;
        rdfs:label       "Environmental Sensing Service" ;
        rdfs:seeAlso     <https://www.bluetooth.org/docman/handlers/downloaddoc.ashx?doc_id=294797> ;
        owl:versionInfo  "1.0.0" ;
        skos:definition  "The Environmental Sensing Service (ESS) exposes measurement data from an environmental sensor intended for sports and fitness applications." ;
        skos:related     esp:ESMeasurement , esp:DescriptorValueChanged .

otp:ObjectNameField  a   skos:Concept ;
        rdfs:label       "Object Name Field" ;
        skos:definition  "The Object Name characteristic returns its associated value when read." ;
        skos:related     xsd:string .

lehid:HIDInformation  a  skos:Concept ;
        rdfs:label       "HID Information" ;
        skos:definition  "The HID Information characteristic is used to hold a set of values known as the HID Device’s HID Attributes." ;
        skos:related     lehid:bCountryCode , lehid:bcdHID , ble:Read .

cpp:MaximumForceMagnitude
        a                skos:Concept ;
        rdfs:label       "Maximum Force Magnitude" ;
        skos:definition  "The Maximum Force Magnitude field represents the maximum force value measured in a single crank revolution." ;
        skos:related     xsd:short .

ftmp:FitnessMachineStatus
        a                skos:Concept ;
        rdfs:label       "Fitness Machine Status" ;
        skos:definition  "The Fitness Machine Status characteristic is used to send the status of the Server." ;
        skos:related     ble:Notify .

idp:AnnunciationType  a  skos:Concept ;
        rdfs:label       "Annunciation Type" ;
        skos:definition  "This Annunciation Type field describes the kind of annunciation in the scope of the Server application" ;
        skos:narrower    idp:BatteryMedium , idp:ReservoirIssue , idp:MechanicalIssue , idp:Temperature , idp:ReservoirEmpty , idp:BolusCanceled , idp:Temperatureoutofrange , idp:ManufacturerReserved , idp:TBROver , idp:ReservoirLow , idp:PrimingIssue , idp:BatteryLow , idp:BatteryEmpty , idp:PowerSourceInsufficient , idp:BatteryFull , idp:SystemIssue , idp:OcclusionDetected , idp:MaxDelivery , idp:InfusionSetDetached , idp:DateTimeIssue , idp:Airpressureoutofrange , idp:TBRCanceled , idp:InfusionSetIncomplete ;
        skos:related     xsd:unsignedShort .

aiop:AutomationIOProfile
        a                skos:Concept ;
        rdfs:label       "Automation Input/Output Profile" ;
        rdfs:seeAlso     <https://www.bluetooth.org/docman/handlers/DownloadDoc.ashx?doc_id=304971> ;
        owl:versionInfo  "1.0.0" ;
        skos:definition  "The Automation Profile is used to enable a device to access analog and digital signals exposed by the Automation IO Service." ;
        skos:related     aiop:AutomationIOService .

aiop:Analog  a           skos:Concept ;
        rdfs:label       "Analog characteristic" ;
        skos:definition  "The Analog characteristic is used to read or write the value of one of the IOM’s analog signals." ;
        skos:related     ble:Write , ble:Indicate , aiop:AnalogSignalValue , xsd:unsignedShort , ble:Read , ble:WritewithoutResponse , ble:Notify .

ble:LatitudeValue  a     skos:Concept ;
        rdfs:label       "The current value of the Latitude Characteristic." ;
        skos:definition  "When read, the Server shall return the current value of the Latitude Characteristic." ;
        skos:related     xsd:integer .

plxp:PLXFeatures  a      skos:Concept ;
        rdfs:label       "Pulse Oximeter Feature" ;
        skos:definition  "The PLX Features characteristic shall be used to describe the supported features of the Server." ;
        skos:related     ble:Read .

cpp:MinimumTorqueMagnitude
        a                skos:Concept ;
        rdfs:label       "Minimum Torque Magnitude" ;
        skos:definition  "The Minimum Torque Magnitude field represents the minimum torque value measured in a single crank revolution." ;
        skos:related     xsd:short .

lehid:HIDService  a      skos:Concept ;
        rdfs:label       "Human Interface Device Service" ;
        rdfs:seeAlso     <https://www.bluetooth.org/docman/handlers/downloaddoc.ashx?doc_id=245140> ;
        owl:versionInfo  "1.0" ;
        skos:definition  "The HID Service exposes data and associated formatting for HID Devices and HID Hosts. " ;
        skos:related     lehid:BootKeyboardOutputReport , lehid:BootMouseInputReport , lehid:ProtocolMode , lehid:HIDControlPoint , lehid:ReportMap , lehid:HIDInformation , lehid:Report , lehid:BootKeyboardInputReport .

lnp:TotalDistanceField
        a                skos:Concept ;
        rdfs:label       "Total Distance Field" ;
        skos:definition  "The Total Distance field represents the cumulative value of the total distance measured by the sensor." ;
        skos:related     xsd:unsignedInt .

wsp:BasalMetabolismField
        a                skos:Concept ;
        rdfs:label       "Basal Metabolism Field" ;
        skos:definition  "The User ID field shall be included in the Body Composition Measurement characteristic if the device supports the Multiple Users feature" ;
        skos:related     xsd:unsignedShort .

ble:OrganizationIDField
        a                skos:Concept ;
        rdfs:label       "Organization ID Field" ;
        skos:definition  "This field shall contain a 1 octet Organization ID value from the Bluetooth SIG Assigned Numbers with the value set to the appropriate organization." ;
        skos:related     xsd:unsignedByte .

otp:ObjectChanged  a     skos:Concept ;
        rdfs:label       "Object Changed Characteristic" ;
        skos:definition  "The Object Changed characteristic enables a Client to receive an indication if the contents and/or metadata of one or more objects are changed while the Client is connected without the change being made by an action of the Client itself." ;
        skos:related     ble:Indicate , otp:ObjectIDField .

blp:BloodPressureService
        a                skos:Concept ;
        rdfs:label       "Blood Pressure Service." ;
        rdfs:seeAlso     <https://www.bluetooth.org/docman/handlers/downloaddoc.ashx?doc_id=243126> ;
        owl:versionInfo  "1.0" ;
        skos:definition  "The Blood Pressure Service exposes blood pressure and other data related to a non-invasive blood pressure monitor for consumer and professional healthcare applications." ;
        skos:related     blp:BloodPressureMeasurement , blp:IntermediateCuffPressure , blp:BloodPressureFeature .

idp:BolusDurationfield
        a                skos:Concept ;
        rdfs:label       "Bolus Duration field" ;
        skos:definition  "The Bolus Duration field represents the duration of the bolus." .

glp:CarbohydrateField
        a                skos:Concept ;
        rdfs:label       "Carbohydrate - units of kilograms" ;
        skos:definition  "Field exists if the key of bit 0 of the Flags field is set to 1." ;
        skos:related     xsd:float .

otp:ObjectTransferProfile
        a                skos:Concept ;
        rdfs:label       "Object Transfer Profile" ;
        rdfs:seeAlso     <https://www.bluetooth.org/docman/handlers/DownloadDoc.ashx?doc_id=309936> ;
        owl:versionInfo  "1.0" ;
        skos:definition  "The Object Transfer Profile defines fundamental requirements to enable an Object Client to create and delete objects and to execute a variety of actions using the currently selected object such as reading object data from or writing object data to an Object Server that exposes the Object Transfer Service." ;
        skos:related     otp:ObjectTransferService .

lnp:EVPEField  a         skos:Concept ;
        rdfs:label       "Estimated Vertical Position Error Field" ;
        skos:definition  "The EVPE field represents the Estimated Vertical Position Error, i.e., a measure of the error in a position in the vertical plane." ;
        skos:related     xsd:unsignedInt .

idp:Insulin  a           skos:Concept ;
        rdfs:label       "Insulin" ;
        skos:definition  "The reported temperature refers to the insulin delivered by the Insulin Delivery Device in general (e.g. the insulin in the reservoir)." .

wsp:SoftLeanMassField
        a                skos:Concept ;
        rdfs:label       "Soft Lean Mass Field" ;
        skos:definition  "The Soft Lean Mass field may be included in the Body Composition Measurement characteristic if the device supports the Soft Lean Mass feature." ;
        skos:related     xsd:unsignedShort .

plxp:PLXContinuousMeasurement
        a                skos:Concept ;
        rdfs:label       "Pulse Oximeter Continuous Measurement" ;
        skos:definition  "The PLX Continuous Measurement characteristic, if supported, shall be used to send periodic pulse oximetry measurements." ;
        skos:related     plxp:SpO2PRFastfield , plxp:SpO2PRSlowfield , plxp:SpO2PRNormalfield , plxp:PulseAmplitudeIndex , ble:Notify .

ftmp:StrideCountField
        a                skos:Concept ;
        rdfs:label       "Stride Count Field" ;
        skos:definition  "The Stride Count field represents the total number of strides since the beginning of the training session." ;
        skos:related     xsd:unsignedShort .

htp:MeasurementInterval
        a                skos:Concept ;
        rdfs:label       "Measurement Interval" ;
        skos:definition  "The Measurement Interval characteristic is used to enable and control the interval between consecutive temperature measurements." ;
        skos:related     ble:Read , htp:MeasurementIntervalValue .

cpp:AccumulatedEnergyField
        a                skos:Concept ;
        rdfs:label       "Accumulated Energy Field" ;
        skos:definition  "The Accumulated Energy field represents the accumulated value of the energy measured by the sensor." .

skos:definition  skos:definition  "The insulin infusion therapy is stopped but the Insulin Delivery Device can still be configured (e.g., priming)." .

ble:Altitude  a          skos:Concept ;
        rdfs:label       "Altitude" ;
        skos:definition  "The Altitude Characteristic describes the altitude of the device above the WGS84 datum." ;
        skos:related     ble:Write , ble:AltitudeValue , ble:ReliableWrite , ble:Read , ble:WritewithoutResponse .

lnp:EstimatedTimeArrivalField
        a                skos:Concept ;
        rdfs:label       "Estimated Time of Arrival Field" ;
        skos:definition  "The Estimated Time of Arrival field represents the remaining time from the current position to reach the next waypoint or final destination." .

anp:AlertNotificationService
        a                skos:Concept ;
        rdfs:label       "Alert Notification service" ;
        rdfs:seeAlso     <https://www.bluetooth.org/docman/handlers/downloaddoc.ashx?doc_id=242287> ;
        owl:versionInfo  "1.0" ;
        skos:definition  "Alert Notification service exposes the different types of alerts with the short text messages, the count of new alert messages, and the count of unread alerts" ;
        skos:related     anp:SupportedUnreadAlertCategory , anp:AlertNotificationControlPoint , anp:NewAlert , anp:UnreadAlertStatus , anp:SupportedNewAlertCategory .

lehid:HIDControlPointCharacteristicValue
        a                skos:Concept ;
        rdfs:label       "HID Control Point Characteristic Value" ;
        skos:definition  "The HID Control Point characteristic value contains an enumeration of values when written" ;
        skos:narrower    lehid:ExitSuspend , lehid:Suspend ;
        skos:related     xsd:unsignedByte .

cpp:AccumulatedTorqueField
        a                skos:Concept ;
        rdfs:label       "Accumulated Torque Field" ;
        skos:definition  "The Accumulated Torque field represents the cumulative value of the torque measured by the Sensor." ;
        skos:related     xsd:unsignedShort .

ftmp:MinimumHeartRatefield
        a                skos:Concept ;
        rdfs:label       "Minimum Heart Rate" ;
        skos:definition  "Minimum Beats per minute with a resolution of 1" ;
        skos:related     xsd:unsignedByte .

ftmp:PostWorkout  a      skos:Concept ;
        rdfs:label       "Post-Workout" ;
        skos:definition  "0x0F - Post-Workout" .

ftmp:SupportedHeartRateRange
        a                skos:Concept ;
        rdfs:label       "Supported Heart Rate Range" ;
        skos:definition  "The Supported Heart Rate Range characteristic is used to send the supported Heart Rate range as well as the minimum Heart Rate increment supported by the Server." ;
        skos:related     ftmp:MinimumHeartRateIncrementfield , ftmp:MaximumHeartRatefield , ftmp:MinimumHeartRatefield , ble:Read .

otp:ObjectName  a        skos:Concept ;
        rdfs:label       "Object Name" ;
        skos:definition  "The Object Name characteristic exposes the name of the Current Object." ;
        skos:related     ble:Write , otp:ObjectNameField , ble:Read .

idp:MaxDelivery  a       skos:Concept ;
        rdfs:label       "Max Delivery" ;
        skos:definition  "The delivery reached a defined high threshold based on maximum bolus and maximum basal rates" .

cgmp:TimeZoneField  a    skos:Concept ;
        rdfs:label       "Time zone Field" ;
        skos:definition  "To know an absolute Time, it is necessary to know the Time Zone to which the Session  Start Time is related to." ;
        skos:related     xsd:byte .

hrp:EnergyExpendedField
        a                skos:Concept ;
        rdfs:label       "Energy Expended Field" ;
        skos:definition  "The Energy Expended field represents the accumulated energy expended in kilo Joules since the last time it was reset." ;
        skos:related     xsd:unsignedShort .

lehid:ExitSuspend  a     skos:Concept ;
        rdfs:label       "Exit Suspend" ;
        skos:definition  "Informs HID Device that HID Host is exiting the Suspend State" .

ftmp:MinimumResistanceIncrementfield
        a                skos:Concept ;
        rdfs:label       "Minimum Resistance Increment" ;
        skos:definition  "Unitless with a resolution of 0.1" ;
        skos:related     xsd:unsignedShort .

ble:WriteLong  a         skos:Concept ;
        rdfs:label       "Write Long" ;
        skos:definition  "Characteristic Value is written to a server when the client knows the Characteristic Value Handle but the length of the Characteristic Value is longer than can be sent in a single Write Request Attribute protocol message." .

wsp:WeightScaleProfile
        a                skos:Concept ;
        rdfs:label       "Weight Scale Profile" ;
        rdfs:seeAlso     <https://www.bluetooth.org/docman/handlers/downloaddoc.ashx?doc_id=293525> ;
        owl:versionInfo  "1.0" ;
        skos:definition  "Weight Scale Profile enables a Collector device to connect and interact with a Weight Scale intended for consumer healthcare and sports/fitness applications." ;
        skos:related     ble:BatteryService , ble:CurrentTimeService , wsp:WeightScaleService , ble:DeviceInformationService , ble:UserDataService , wsp:BodyCompositionService .

lnp:Navigation  a        skos:Concept ;
        rdfs:label       "Navigation" ;
        skos:definition  "The Navigation characteristic is used to send navigation-related data." ;
        skos:related     lnp:RemainingDistanceField , lnp:BearingField , lnp:HeadingField , lnp:EstimatedTimeArrivalField , ble:Notify , lnp:RemainingVerticalDistanceField .

anp:SupportedNewAlertCategory
        a                skos:Concept ;
        rdfs:label       "Supported New Alert Category" ;
        skos:definition  "A bit map showing which categories of new alert are supported and which are not." ;
        skos:related     ble:Read .

ftmp:FitnessMachineControlPoint
        a                skos:Concept ;
        rdfs:label       "Fitness Machine Control Point" ;
        skos:definition  "The Fitness Machine Control Point characteristic is used to request a specific function to be executed on the Server." ;
        skos:related     ble:Write , ble:Indicate .

ble:HTTPProxyService  a  skos:Concept ;
        rdfs:label       "Hyper Text Transfer Protocol (HTTP) Proxy Service" ;
        rdfs:seeAlso     <https://www.bluetooth.org/docman/handlers/downloaddoc.ashx?doc_id=308344> ;
        owl:versionInfo  "1.0" ;
        skos:definition  "The HTTP Proxy Service (HPS) allows a device to expose HTTP Web services to a client of the HPS Server (HPS Client) using the Generic Attribute Profile (GATT)." .

ftmp:ElapsedTimeField
        a                skos:Concept ;
        rdfs:label       "Elapsed Time Field" ;
        skos:definition  "The Elapsed Time field represents the elapsed time of a training session since the training session has started." ;
        skos:related     xsd:unsignedShort .

ftmp:TotalEnergyField
        a                skos:Concept ;
        rdfs:label       "Total Energy Field" ;
        skos:definition  "The Total Energy field represents the total expended energy of a user since the training session has started." ;
        skos:related     xsd:short .

cpp:CyclingPowerMeasurement
        a                skos:Concept ;
        rdfs:label       "Cycling Power Measurement" ;
        skos:definition  "The Cycling Power Measurement characteristic is used to send power-related data, speedrelated data, and/or cadence-related data." ;
        skos:related     ble:CumulativeCrankRevolutions , cpp:PedalPowerBalanceField , ble:InstantaneousPowerField , ble:LastCrankEventTime , cpp:MinimumForceMagnitude , cpp:ExtremeTorqueMagnitudesFieldPair , cpp:LastWheelEventTime , cpp:MinimumAngle , cpp:TopDeadSpotAngleField , cpp:CumulativeWheelRevolutions , cpp:MaximumForceMagnitude , cpp:MinimumTorqueMagnitude , cpp:AccumulatedEnergyField , cpp:AccumulatedTorqueField , cpp:BottomDeadSpotAngleField , ble:Notify , cpp:MaximumAngle .

ftmp:Idle  a             skos:Concept ;
        rdfs:label       "Idle" ;
        skos:definition  "0x01 - Idle" .

ble:URI  a               skos:Concept ;
        rdfs:label       "URI" ;
        skos:definition  "The URI characteristic is used to configure the URI for a subsequent request." ;
        skos:related     ble:Write , xsd:string , ble:WriteLong .

ftmp:MaximumSpeedfield
        a                skos:Concept ;
        rdfs:label       "Maximum Speed" ;
        skos:definition  "Maximum Kilometer per hour with a resolution of 0.01" ;
        skos:related     xsd:unsignedShort .

lnp:LocationLatitude  a  skos:Concept ;
        rdfs:label       "Location - Latitude" ;
        skos:definition  "The Latitude value represents a geographic coordinate specifying the north-south position of a point on the Earth's surface in WGS-84 format." ;
        skos:related     xsd:integer .

otp:ObjectLastModified
        a                skos:Concept ;
        rdfs:label       "Object Last Modified" ;
        skos:definition  "The Object Last-Modified characteristic exposes a value representing a date and time when the object content was last modified." ;
        skos:related     ble:Write , otp:ObjectLastModifiedField , ble:Read .

glp:TimeOffsetField  a   skos:Concept ;
        rdfs:label       "Time Offset Field" ;
        skos:definition  "The Time Offset field is used in conjunction with the Base Time field to represent the user-facing date and time at the time of measurement." ;
        skos:related     xsd:short .

htp:MeasurementIntervalValue
        a                skos:Concept ;
        rdfs:label       "Measurement Interval Value" ;
        skos:definition  "The Measurement Interval characteristic returns the measurement interval value when read." ;
        skos:related     xsd:unsignedShort .

cgmp:E2ECRCField  a      skos:Concept ;
        rdfs:label       "End-to-End Cyclic Redundancy Check Field" ;
        skos:definition  "If the device supports E2E-safety (E2E-CRC Supported bit is set in CGM Features), the measurement shall be protected by a CRC calculated over all field." ;
        skos:related     xsd:unsignedShort .

ftmp:FitnessMachineFeature
        a                skos:Concept ;
        rdfs:label       "Fitness Machine Feature" ;
        skos:definition  "The Fitness Machine Feature characteristic shall be used to describe the supported features of the Server." ;
        skos:related     ble:Read .

rscp:RSCMeasurement  a   skos:Concept ;
        rdfs:label       "Running Speed and Cadence Measurement" ;
        skos:definition  "The RSC Measurement characteristic is used to send speed and cadence measurements." ;
        skos:related     rscp:TotalDistanceField , rscp:InstantaneousCadenceField , ble:InstantaneousSpeedField , rscp:InstantaneousStrideLengthField , ble:Notify .

ftmp:ManualMode  a       skos:Concept ;
        rdfs:label       "Manual Mode" ;
        skos:definition  "0x0D - Manual Mode (Quick Start)" .

cgmp:cgmpFeature  a      skos:Concept ;
        rdfs:label       "cgmp Feature" ;
        skos:definition  "The cgmp Feature characteristic is used to describe the supported features of the Server." ;
        skos:related     ble:Read , cgmp:E2ECRCField .

lehid:Report  a          skos:Concept ;
        rdfs:label       "Report" ;
        skos:definition  "The Report characteristic is used to exchange data between a HID Device and a HID Host." ;
        skos:related     ble:Write , lehid:ReportValue , ble:Read , ble:WritewithoutResponse , ble:Notify .

ble:Characteristic  skos:narrower  htp:TemperatureType , ftmp:TrainingStatus , anp:SupportedUnreadAlertCategory , ble:LocationName , rcp:RCFeature , pxp:TxPowerLevel , idp:IDDHistoryData , glp:GlucoseMeasurementContext , esp:ESMeasurement , idp:IDDRecordAccessControlPoint , idp:IDDCommandControlPoint , wsp:WeightScaleFeature , htp:ValidRangeDescriptor , htp:IntermediateTemperature , idp:IDDFeatures , cpp:CyclingPowerFeature , lehid:BootKeyboardOutputReport , cpp:CyclingPowerVector , hrp:BodySensorLocation , ftmp:RowerData , cscp:CSCFeature , ble:RecordAccessControlPoint , lehid:BootMouseInputReport , otp:ObjectID , cscp:CSCMeasurement , anp:AlertNotificationControlPoint , blp:BloodPressureMeasurement , rcp:RCCP , idp:IDDStatusChanged , ble:LocalEastCoordinate , otp:ObjectListFilter , cgmp:cgmpMeasurement , ble:HTTPHeaders , ble:FloorNumber , tip:TimewithDST , aiop:Aggregate , ftmp:StairClimberData , pasp:RingerSetting , ble:Latitude , anp:NewAlert , pasp:RingerControlPoint , rscp:SCControlPoint , ble:Longitude , rcp:RCSettings , otp:OTSFeature , otp:ObjectType , ftmp:SupportedInclinationRange , aiop:Digital , ftmp:SupportedResistanceLevelRange , wsp:BodyCompositionMeasurement , wsp:BodyCompositionFeature , otp:ObjectSize , idp:IDDStatus , lehid:ProtocolMode , hrp:HeartRateControlPoint , otp:ObjectListControlPoint , tip:TimeUpdateState , anp:UnreadAlertStatus , glp:GlucoseMeasurement , wsp:WeightMeasurement , lehid:HIDControlPoint , ble:TDSControlPoint , htp:TemperatureMeasurement , idp:IDDStatusReaderControlPoint , otp:ObjectFirstCreated , lehid:ReportMap , otp:ObjectProperties , ftmp:TreadmillData , ble:HTTPSSecurity , blp:IntermediateCuffPressure , pxp:LinkLossAlertLevel , ftmp:CrossTrainerData , glp:GlucoseFeature , lehid:HIDInformation , ble:SensorLocation , ftmp:FitnessMachineStatus , aiop:Analog , plxp:PLXFeatures , otp:ObjectChanged , plxp:PLXContinuousMeasurement , htp:MeasurementInterval , ble:Altitude , ftmp:SupportedHeartRateRange , otp:ObjectName , lnp:Navigation , anp:SupportedNewAlertCategory , ftmp:FitnessMachineControlPoint , cpp:CyclingPowerMeasurement , ble:URI , otp:ObjectLastModified , ftmp:FitnessMachineFeature , rscp:RSCMeasurement , cgmp:cgmpFeature , lehid:Report , idp:IDDAnnunciationStatus , plxp:PLXSpotcheckMeasurement , cgmp:cgmpSessionStartTime , ble:HTTPStatusCode , rscp:RSCFeature , cpp:CyclingPowerControlPoint , lnp:LocationandSpeed , lehid:BootKeyboardInputReport , ble:LocalNorthCoordinate , cgmp:cgmpSpecificOpsControlPoint , idp:IDDCommandData , cgmp:cgmpSessionRunTime , tip:TimeUpdateControlPoint , hrp:HeartRateMeasurement , lnp:LNControlPoint , lnp:PositionQuality , lnp:LNFeature , ble:HTTPControlPoint , otp:ObjectActionControlPoint , ble:HTTPEntityBody , ftmp:SupportedSpeedRange , ble:IndoorPositioningConfiguration , ftmp:IndoorBikeData , ftmp:StepClimberData , esp:DescriptorValueChanged , pasp:AlertStatus , ble:Uncertainty , ftmp:SupportedPowerRange , blp:BloodPressureFeature , cgmp:cgmpStatus .

idp:IDDAnnunciationStatus
        a                skos:Concept ;
        rdfs:label       "Insulin Delivery Device Annunciation Status" ;
        skos:definition  "The IDD Annunciation Status characteristic is a variable length structure comprising of messages that describe state changes of the Insulin Delivery Device and in the therapy relevant functions." ;
        skos:related     idp:AuxInfo3LowerBoundfield , idp:AnnunciationStatus , idp:AnnunciationInstanceID , ble:Indicate , idp:AuxInfo1Valuefield , idp:AnnunciationType , ble:Read , idp:AuxInfo4UpperBoundfield , idp:AuxInfo2Contextfield , idp:E2ECounterfield , idp:E2ECRCfield .

plxp:PLXSpotcheckMeasurement
        a                skos:Concept ;
        rdfs:label       "Pulse Oximeter Spot-check Measurement" ;
        skos:definition  "The PLX Spot-check Measurement characteristic, if supported, shall be used to send Spot-check measurements of SpO2 (Percent oxygen saturation of hemoglobin) and PR (pulse rate)." ;
        skos:related     ble:Indicate , plxp:SpO2PRSpotCheckField , ble:TimestampField , plxp:PulseAmplitudeIndex .

anp:NumberofNewAlert  a  skos:Concept ;
        rdfs:label       "Number of New Alert" ;
        skos:definition  "This characteristic provides the count of new alerts (for a given category) in the server." ;
        skos:related     xsd:unsignedByte .

ftmp:HeartRateField  a   skos:Concept ;
        rdfs:label       "Heart Rate Field" ;
        skos:definition  "The Heart Rate field represents the current heart rate value of the user (e.g., measured via the contact heart rate or any other means)." ;
        skos:related     xsd:unsignedByte .

cgmp:cgmpSessionStartTime
        a                skos:Concept ;
        rdfs:label       "cgmp Session Start Time" ;
        skos:definition  "The Session Start Time Field defines the time of the initial cgmp measurement." ;
        skos:related     ble:Write , cgmp:DTSOffsetField , cgmp:TimeZoneField , ble:Read , cgmp:E2ECRCField , cgmp:SessionStartTimeField .

cgmp:SessionStartTimeField
        a                skos:Concept ;
        rdfs:label       "Session Start Time Field" ;
        skos:definition  "The Session Start Time Field defines the time of the initial CGM measurement" ;
        skos:related     xsd:unsignedShort .

lnp:UTCTimeField  a      skos:Concept ;
        rdfs:label       "UTC Time Field" ;
        skos:definition  "This field represents the time at the Sensor when the position was received in Coordinated Universal Time format." .

wsp:HeightField  a       skos:Concept ;
        rdfs:label       "Height Field" ;
        skos:definition  "The Height field may be included in the Body Composition Measurement characteristic if the device supports the Height feature." ;
        skos:related     xsd:unsignedShort .

ftmp:MaximumInclinationfield
        a                skos:Concept ;
        rdfs:label       "Maximum Inclination" ;
        skos:definition  "Maximum Percent with a resolution of 0.1" ;
        skos:related     xsd:short .

idp:InfusionSetDetached
        a                skos:Concept ;
        rdfs:label       "Infusion Set Detached" ;
        skos:definition  "The infusion set (including tubing and/or cannula) is not attached to the body." .

ftmp:WattControl  a      skos:Concept ;
        rdfs:label       "Watt Control" ;
        skos:definition  "0x0C- Watt Control" .

ble:HTTPStatusCode  a    skos:Concept ;
        rdfs:label       "HTTP Status Code" ;
        skos:definition  "The HTTP Status Code characteristic contains the Status-Code from the Status-Line of the first line of the HTTP Response message, followed by one octet indicating the Data Status bit field indicating the status of the data received." ;
        skos:related     xsd:unsignedShort , ble:Notify .

hrp:HeartRateProfile  a  skos:Concept ;
        rdfs:label       "Heart Rate Profile" ;
        rdfs:seeAlso     <https://www.bluetooth.org/docman/handlers/downloaddoc.ashx?doc_id=239865> ;
        owl:versionInfo  "1.0" ;
        skos:definition  "The Heart Rate Profile is used to enable a data collection device to obtain data from a Heart Rate Sensor that exposes the Heart Rate Service." ;
        skos:related     ble:DeviceInformationService , hrp:HeartRateService .

cgmp:cgmpService  a      skos:Concept ;
        rdfs:label       "Continuous Glucose Monitoring Service" ;
        rdfs:seeAlso     <https://www.bluetooth.org/docman/handlers/downloaddoc.ashx?doc_id=310502> ;
        owl:versionInfo  "1.0" ;
        skos:definition  "The Continuous Glucose Monitoring (cgmp) Service exposes glucose measurement and other data related to a personal cgmp sensor for healthcare applications." ;
        skos:related     ble:RecordAccessControlPoint , cgmp:cgmpMeasurement , cgmp:cgmpFeature , cgmp:cgmpSessionStartTime , cgmp:cgmpSpecificOpsControlPoint , cgmp:cgmpSessionRunTime , cgmp:cgmpStatus .

rscp:RSCFeature  a       skos:Concept ;
        rdfs:label       "Running Speed and Cadence Feature" ;
        skos:definition  "The RSC Feature characteristic shall be used to describe the supported features of the Server." ;
        skos:related     ble:Write , ble:Read .

idp:DateTimeIssue  a     skos:Concept ;
        rdfs:label       "Date Time Issue" ;
        skos:definition  "The date time of the device was never set or has been lost (e.g., due to a battery replacement)." .

cpp:BottomDeadSpotAngleField
        a                skos:Concept ;
        rdfs:label       "Bottom Dead Spot Angle Field" ;
        skos:definition  "The Bottom Dead Spot Angle field represents the crank angle when the value of the Instantaneous Power value becomes negative." ;
        skos:related     xsd:unsignedShort .

cpp:CyclingPowerControlPoint
        a                skos:Concept ;
        rdfs:label       "Cycling Power Control Point" ;
        skos:definition  "The Cycling Power Control Point is used by a Client to control certain behaviors of the Server." ;
        skos:related     ble:Write , xsd:unsignedByte , ble:Indicate .

plxp:PulseAmplitudeIndex
        a                skos:Concept ;
        rdfs:label       "Pulse Amplitude Index" ;
        skos:definition  "The Pulse Amplitude Index is a percentage indicator indicating the perfusion level (amount of blood being delivered to the capillary bed) of a user." ;
        skos:related     xsd:float .

ftmp:MetabolicEquivalentField
        a                skos:Concept ;
        rdfs:label       "Metabolic Equivalent Field" ;
        skos:definition  "The Metabolic Equivalent field represents the metabolic equivalent of the user." ;
        skos:related     xsd:unsignedByte .

ble:LocalEastCoordinateValue
        a                skos:Concept ;
        rdfs:label       "The current value of the Local East Coordinate Characteristic" ;
        skos:definition  "When read, the Server shall return the current value of the Local East Coordinate Characteristic." ;
        skos:related     xsd:Short .

lnp:LocationandSpeed  a  skos:Concept ;
        rdfs:label       "Location and Speed" ;
        skos:definition  "The Location and Speed characteristic is used to send location and speed related data." ;
        skos:related     lnp:ElevationField , ble:InstantaneousSpeedField , lnp:HeadingField , lnp:TotalDistanceField , lnp:LocationLatitude , lnp:UTCTimeField , ble:Notify , lnp:LocationLongitude , lnp:RollingTimeField .

cpp:InstantaneousForceMagnitudeArrayField
        a                skos:Concept ;
        rdfs:label       "Instantaneous Force Magnitude Array Field" ;
        skos:definition  "Included in this field are one or more Instantaneous Magnitude values which are expressed in Newtons with a resolution of 1 Newton" ;
        skos:related     xsd:short .

lehid:BootKeyboardInputReport
        a                skos:Concept ;
        rdfs:label       "Boot Keyboard Input Report" ;
        skos:definition  "The Input Boot Keyboard Report characteristic is used to transfer fixed format and length Input Report data between a HID Host operating in Boot Protocol Mode and a HID Service corresponding to a boot keyboard." ;
        skos:related     lehid:BootKeyboardInputReportValue , ble:Read , ble:Notify .

ble:LocalNorthCoordinate
        a                skos:Concept ;
        rdfs:label       "Local North Coordinate" ;
        skos:definition  "The Local North Coordinate Characteristic describes the North coordinate of the device using a local coordinate system." ;
        skos:related     ble:Write , ble:ReliableWrite , ble:LocalNorthCoordinateValue , ble:Read , ble:WritewithoutResponse .

ftmp:PreWorkout  a       skos:Concept ;
        rdfs:label       "Pre-Workout" ;
        skos:definition  "0x0E - Pre-Workout" .

idp:GenericDevice  a     skos:Concept ;
        rdfs:label       "Generic Device" ;
        skos:definition  "The reported temperature refers to the Insulin Delivery Device in general." .

idp:BolusExtendedAmountfield
        a                skos:Concept ;
        rdfs:label       "Bolus Extended Amount field" ;
        skos:definition  "The Bolus Extended Amount field represents the extended amount of the bolus." ;
        skos:related     xsd:float .

cgmp:cgmpSpecificOpsControlPoint
        a                skos:Concept ;
        rdfs:label       "cgmp Specific Ops Control Point" ;
        skos:definition  "The Client shall perform a write to the cgmp Specific Ops Control Point to request a desired cgmp specific procedure at the Server." ;
        skos:related     ble:Write , ble:Indicate .

blp:PulseRateField  a    skos:Concept ;
        rdfs:label       "Pulse Rate Field" ;
        skos:definition  "The Pulse Rate field may be included in the Blood Pressure Measurement characteristic if the device supports pulse rate measurements." ;
        skos:related     xsd:float .

idp:IDDCommandData  a    skos:Concept ;
        rdfs:label       "Insulin Delivery Device Command Data" ;
        skos:definition  "The IDD Command Data characteristic is comprised of response records from executed procedures of the IDD Command Control Point." ;
        skos:related     ble:Write , ble:Indicate , idp:E2ECounterfield , idp:E2ECRCfield .

lnp:RemainingVerticalDistanceField
        a                skos:Concept ;
        rdfs:label       "Remaining Vertical Distance Field" ;
        skos:definition  "The Remaining Vertical Distance field represents the vertical distance from the current position to the next waypoint or final destination." ;
        skos:related     xsd:integer .

ble:IndoorPositioningValue
        a                skos:Concept ;
        rdfs:label       "The current value of  the Indoor Positioning Configuration Characteristic" ;
        skos:definition  "When read, the Indoor Positioning Configuration Characteristic shall return the current value of the characteristic." ;
        skos:related     xsd:unsignedByte .

cgmp:cgmpSessionRunTime
        a                skos:Concept ;
        rdfs:label       "cgmp Session Run Time" ;
        skos:definition  "The cgmp Session Run Time shall define the expected run time of the cgmp session." ;
        skos:related     cgmp:cgmpSessionRunTimeField , ble:Read , cgmp:E2ECRCField .

tip:TimeUpdateControlPoint
        a                skos:Concept ;
        rdfs:label       "Time Update Control Point" ;
        skos:definition  "The Time Update Control Point characteristic is used to request a reference time update on the server." ;
        skos:related     xsd:unsignedByte , ble:WritewithoutResponse .

hrp:HeartRateMeasurement
        a                skos:Concept ;
        rdfs:label       "Heart Rate Measurement" ;
        skos:definition  "The Heart Rate Measurement characteristic is used to send a heart rate measurement." ;
        skos:related     hrp:HeartRateValueField , hrp:EnergyExpendedField , ble:Notify , hrp:RRIntervalField .

lnp:LNControlPoint  a    skos:Concept ;
        rdfs:label       "Location and Navigation Control Point" ;
        skos:definition  "The LN Control Point is used by a Client to control certain behaviors of the Server." ;
        skos:related     ble:Write , xsd:unsignedByte , ble:Indicate .

lnp:PositionQuality  a   skos:Concept ;
        rdfs:label       "Position Quality" ;
        skos:definition  "The Position Quality characteristic is used to send position quality-related data" ;
        skos:related     lnp:VDOPField , lnp:HDOPField , lnp:TimetoFirstFixField , lnp:BeaconsNumberViewField , lnp:BeaconsNumberSolutionField , lnp:EHPEField , lnp:EVPEField , ble:Read .

lnp:LNFeature  a         skos:Concept ;
        rdfs:label       "Location and Navigation Feature" ;
        skos:definition  "The LN Feature characteristic shall be used to describe the supported features of the Server." ;
        skos:related     ble:Read .

ble:HTTPControlPoint  a  skos:Concept ;
        rdfs:label       "HTTP Control Point" ;
        skos:definition  "The HTTP Control Point is used to initiate a request to send an HTTP request message from the device containing the HTTP Proxy Service, acting as an HTTP Client." ;
        skos:related     ble:Write .

otp:ObjectActionControlPoint
        a                skos:Concept ;
        rdfs:label       "Object Action Control Point" ;
        skos:definition  "The Object Action Control Point is used by a Client to control certain behaviors of the Server." ;
        skos:related     ble:Write , ble:Indicate .

ble:HTTPEntityBody  a    skos:Concept ;
        rdfs:label       "HTTP Entity Body" ;
        skos:definition  "The HTTP Entity Body characteristic contains the contents of the message-body after any Transfer-Encoding has been applied." ;
        skos:related     ble:Write , ble:ReadLong , xsd:string , ble:WriteLong , ble:Read .

cpp:MaximumTorqueMagnitude
        a                skos:Concept ;
        rdfs:label       "Maximum Torque Magnitude" ;
        skos:definition  "The Maximum Torque Magnitude field represents the maximum torque value measured in a single crank revolution." ;
        skos:related     xsd:short .

idp:Airpressureoutofrange
        a                skos:Concept ;
        rdfs:label       "Air pressure out of range" ;
        skos:definition  "The air pressure is outside of the normal operating range (e.g., altitude)." .

ftmp:SupportedSpeedRange
        a                skos:Concept ;
        rdfs:label       "Supported Speed Range" ;
        skos:definition  "The Supported Speed Range characteristic is used to send the supported speed range as well as the minimum speed increment supported by the Server." ;
        skos:related     ftmp:MinimumSpeedfield , ftmp:MinimumSpeedIncrementfield , ble:Read , ftmp:MaximumSpeedfield .

ftmp:NegativeElevationGainField
        a                skos:Concept ;
        rdfs:label       "Negative Elevation Gain Field" ;
        skos:definition  "The Negative Elevation Gain field represents the negative elevation gain since the training session has started." ;
        skos:related     xsd:unsignedShort .

idp:Undetermined  a      skos:Concept ;
        rdfs:label       "Undetermined" ;
        skos:definition  "The operational state is undetermined" .

idp:TBRCanceled  a       skos:Concept ;
        rdfs:label       "The temporary basal Canceled" ;
        skos:definition  "The temporary basal rate canceled (e.g., device changed from run to standby mode)." .

glp:MealField  a         skos:Concept ;
        rdfs:label       "Meal" ;
        skos:definition  "Field exists if the key of bit 1 of the Flags field is set to 1" ;
        skos:related     xsd:unsignedByte .

cpp:MaximumAngle  a      skos:Concept ;
        rdfs:label       "Maximum Angle Field" ;
        skos:definition  "The Maximum Angle field represents the angle of the crank when the maximum value is measured in a single crank revolution." ;
        skos:related     xsd:unsignedByte .

ble:TransportDataField
        a                skos:Concept ;
        rdfs:label       "Transport Data Field" ;
        skos:definition  "If used, this field contains organization-specific data and shall be byte-aligned." .

lnp:LocationLongitude
        a                skos:Concept ;
        rdfs:label       "Location - Longitude" ;
        skos:definition  "The Longitude value represents a geographic coordinate specifying the east-west position of a point on the Earth's surface in WGS-84 format." ;
        skos:related     xsd:integer .

cpp:FirstCrankMeasurementAngleField
        a                skos:Concept ;
        rdfs:label       "First Crank Measurement Angle Field" ;
        skos:definition  "This represents the angle of the first sample at the start of a measurement and is used by the Client in conjunction with the Instantaneous Magnitude values and the Sampling Rate to assemble a force (or torque) vector array to show a user the forces throughout a crank rotation" ;
        skos:related     xsd:unsignedShort .

ble:IndoorPositioningConfiguration
        a                skos:Concept ;
        rdfs:label       "Indoor Positioning Configuration" ;
        skos:definition  "The Indoor Positioning Configuration Characteristic describes the advertise information data embedded in the Indoor Positioning Service AD type." ;
        skos:related     ble:Write , ble:ReliableWrite , ble:Read , ble:WritewithoutResponse , ble:IndoorPositioningValue .

lnp:RollingTimeField  a  skos:Concept ;
        rdfs:label       "Rolling Time Field" ;
        skos:definition  "The Rolling Time field represents the time in seconds and rolls over every 256 seconds and it can be used by the Client to keep track of the time elapsed between the position information received by the Server." ;
        skos:related     xsd:unsignedByte .

idp:AuxInfo4UpperBoundfield
        a                skos:Concept ;
        rdfs:label       "AuxInfo4 Upper Bound field" ;
        skos:definition  "The AuxInfo4 field shall contain the value of the upper bound of the temperature." ;
        skos:related     xsd:float .

ftmp:LowSpeedOutside  a  skos:Concept ;
        rdfs:label       "Speed Outside of Control Region - Low" ;
        skos:definition  "0x09 - Speed Outside of Control Region - Low (increase speed to return to controllable region)" .

ftmp:IndoorBikeData  a   skos:Concept ;
        rdfs:label       "Indoor Bike Data" ;
        skos:definition  "The Indoor Bike Data characteristic is used to send training-related data to the Client from an indoor bike (Server)." ;
        skos:related     ftmp:RemainingTimeField , ftmp:EnergyperMinuteField , ftmp:InstantaneousCadenceField , ftmp:ResistanceLevelField , ble:InstantaneousPowerField , ble:InstantaneousSpeedField , ftmp:AverageCadenceField , ftmp:EnergyperHourField , ftmp:AverageSpeedField , ftmp:AveragePowerField , ftmp:ElapsedTimeField , ftmp:TotalEnergyField , ftmp:HeartRateField , ftmp:MetabolicEquivalentField , ble:Notify , ftmp:TotalDistanceField .

ftmp:StepClimberData  a  skos:Concept ;
        rdfs:label       "Step Climber Data" ;
        skos:definition  "The Step Climber Data characteristic is used to send training-related data to the Client from a step climber (Server)." ;
        skos:related     ftmp:FloorsField , ftmp:StepperMinuteField , ftmp:RemainingTimeField , ftmp:EnergyperMinuteField , ftmp:AverageStepRateField , ftmp:PositiveElevationGainField , ftmp:EnergyperHourField , ftmp:StepCountField , ftmp:ElapsedTimeField , ftmp:TotalEnergyField , ftmp:HeartRateField , ftmp:MetabolicEquivalentField , ble:Notify .

fmp:FindMeProfile  a     skos:Concept ;
        rdfs:label       "Find Me Profile" ;
        rdfs:seeAlso     <https://www.bluetooth.org/docman/handlers/downloaddoc.ashx?doc_id=239389> ;
        owl:versionInfo  "1.0" ;
        skos:definition  "The Find Me profile defines the behavior when a button is pressed on one device to cause an alerting signal on a peer device." ;
        skos:related     ble:ImmediateAlertService .

idp:AuxInfo2Contextfield
        a                skos:Concept ;
        rdfs:label       "AuxInfo2 Context values" ;
        skos:definition  "The second octet of the AuxInfo2 field shall contain a Context field." ;
        skos:narrower    idp:Insulin , idp:GenericDevice ;
        skos:related     xsd:unsignedByte .

ftmp:MaximumResistanceLevelField
        a                skos:Concept ;
        rdfs:label       "Maximum Resistance Level" ;
        skos:definition  "Unitless with a resolution of 0.1" ;
        skos:related     xsd:short .

ipsp:InternetProtocolSupportProfile
        a                skos:Concept ;
        rdfs:label       "Internet Protocol Support Profile" ;
        rdfs:seeAlso     <https://www.bluetooth.org/docman/handlers/DownloadDoc.ashx?doc_id=296307> ;
        owl:versionInfo  "1.0" ;
        skos:definition  "This Profile Specification proposes the support of exchanging IPv6 packets between devices over the Bluetooth Low Energy transport." ;
        skos:related     ipsp:IPSupportService .

ble:FloorNumberValue  a  skos:Concept ;
        rdfs:label       "Floor Number Value" ;
        skos:definition  "When read, the Server shall return the current value of the Floor Number Characteristic." ;
        skos:related     xsd:unsignedByte .

ftmp:TotalDistanceField
        a                skos:Concept ;
        rdfs:label       "Total Distance Field" ;
        skos:definition  "The Total Distance field represents the total distance reported by the Server since the beginning of the training session." ;
        skos:related     xsd:unsignedInt .

esp:DescriptorValueChanged
        a                skos:Concept ;
        rdfs:label       "Descriptor Value Changed" ;
        skos:definition  "It enables a Server to alert bonded Clients that the value of one or more ESS-related descriptors for a given ESS Characteristic have changed and need to be re-read" ;
        skos:related     ble:Indicate .

cgmp:SizeField  a        skos:Concept ;
        rdfs:label       "Size Field" ;
        skos:definition  "The Size Field represents the size of the CGM Measurement record." ;
        skos:related     xsd:unsignedByte .

hrp:RRIntervalField  a   skos:Concept ;
        rdfs:label       "RR(Rh factor) - Interval field" ;
        skos:definition  "The RR-Interval field may be included in the Heart Rate Measurement characteristic if the device supports RR-Interval measurements." ;
        skos:related     xsd:unsignedShort .

pasp:AlertStatus  a      skos:Concept ;
        rdfs:label       "Alert Status" ;
        skos:definition  "The Alert Status Characteristic exposes the alerting status of the server device." ;
        skos:related     pasp:AlertStatusValue , ble:Read , ble:Notify .

lehid:Suspend  a         skos:Concept ;
        rdfs:label       "Suspend" ;
        skos:definition  "Informs HID Device that HID Host is entering the Suspend State" .

ble:Uncertainty  a       skos:Concept ;
        rdfs:label       "Uncertainty" ;
        skos:definition  "The Uncertainty Characteristic describes the uncertainty of the location information the device exposes." ;
        skos:related     ble:Write , ble:UncertaintyValue , ble:ReliableWrite , ble:Read , ble:WritewithoutResponse .

ipsp:IPSupportService
        a                skos:Concept ;
        rdfs:comment     "This service does not define any characteristics." ;
        rdfs:label       "IP Support Service" ;
        rdfs:seeAlso     <https://www.bluetooth.org/docman/handlers/DownloadDoc.ashx?doc_id=296307> ;
        owl:versionInfo  "1.0" ;
        skos:definition  "The IP support service is used during service discovery to determine support for the IP Support Profile’s Node role." .

ftmp:SupportedPowerRange
        a                skos:Concept ;
        rdfs:label       "Supported Power Range" ;
        skos:definition  "The Supported Power Range characteristic is used to send the supported power range as well as the minimum power increment supported by the Server." ;
        skos:related     ftmp:MinimumPowerIncrementfield , ftmp:MaximumPowerfield , ftmp:MinimumPowerfield , ble:Read .

idp:InfusionSetIncomplete
        a                skos:Concept ;
        rdfs:label       "Infusion Set Incomplete" ;
        skos:definition  "The physical connection between infusion set (including tubing and/or cannula) and the Insulin Delivery Device is incomplete." .

ftmp:TrainingStatusField
        a                skos:Concept ;
        rdfs:label       "Training Status Field" ;
        skos:definition  "The Training Status field represents the current training state while a user is exercising." ;
        skos:narrower    ftmp:RecoveryInterval , ftmp:HighSpeedOutside , ftmp:HeartRateControl , ftmp:CoolDown , ftmp:FitnessTest , ftmp:HighIntensityInterval , ftmp:WarmingUp , ftmp:Isometric , ftmp:PostWorkout , ftmp:Idle , ftmp:ManualMode , ftmp:WattControl , ftmp:PreWorkout , ftmp:LowSpeedOutside , ftmp:LowIntensityInterval ;
        skos:related     xsd:unsignedInt .

idp:E2ECounterfield  a   skos:Concept ;
        rdfs:label       "End to End Counter field" ;
        skos:definition  "The E2E-Counter field, when used correctly, provides that messages are received in the correct order." ;
        skos:related     xsd:unsignedByte .

plxp:PulseOximeterProfile
        a                skos:Concept ;
        rdfs:label       "Pulse Oximeter Profile" ;
        rdfs:seeAlso     <https://www.bluetooth.org/DocMan/handlers/DownloadDoc.ashx?doc_id=304923> ;
        owl:versionInfo  "1.0" ;
        skos:definition  "This Profile Specification defines a Pulse Oximeter (PLX) profile that enables a Collector device to connect and interact with a pulse oximeter intended for healthcare applications." ;
        skos:related     ble:BatteryService , ble:CurrentTimeService , ble:DeviceInformationService , plxp:PulseOximeterService , ble:BondManagementService .

blp:BloodPressureFeature
        a                skos:Concept ;
        rdfs:label       "Blood Pressure Feature" ;
        skos:definition  "The Blood Pressure Feature characteristic shall be used to describe the supported features of the Blood Pressure Sensor." ;
        skos:related     ble:Read .

idp:Stop  a         skos:Concept ;
        rdfs:label  "Stop" .

idp:Waiting  a           skos:Concept ;
        rdfs:label       "Waiting" ;
        skos:definition  "The Insulin Delivery Device waits for an interaction" .

ftmp:LowIntensityInterval
        a                skos:Concept ;
        rdfs:label       "Low Intensity Interval" ;
        skos:definition  "0x03-Low Intensity Interval" .

cgmp:cgmpStatus  a       skos:Concept ;
        rdfs:label       "cgmp Status cgmp Status" ;
        skos:definition  "The cgmp Status allows the client to actively request the status from the cgmp Sensor, particularly when the cgmp measurement is not running and the status cannot be given in the measurement result in the Status Annunciation Field." ;
        skos:related     cgmp:TimeOffsetField , ble:Read , cgmp:E2ECRCField .

idp:E2ECRCfield  a       skos:Concept ;
        rdfs:label       "End to End Cyclic Redundancy Check field" ;
        skos:definition  "If the Server supports E2E-Protection, all fields of a characteristic shall be secured by a CRC calculated over all fields of the characteristic payload." ;
        skos:related     xsd:unsignedShort .
