@prefix plxp:  <http://example.org/namespace/ble-gatt/plxp#> .
@prefix ftmp:  <http://example.org/namespace/ble-gatt/ftmp#> .
@prefix esp:   <http://example.org/namespace/ble-gatt/esp#> .
@prefix owl:   <http://www.w3.org/2002/07/owl#> .
@prefix fmp:   <http://example.org/namespace/ble-gatt/fmp#> .
@prefix xsd:   <http://www.w3.org/2001/XMLSchema#> .
@prefix skos:  <http://www.w3.org/2004/02/skos/core#> .
@prefix rdfs:  <http://www.w3.org/2000/01/rdf-schema#> .
@prefix lehid: <http://example.org/namespace/ble-gatt/lehid#> .
@prefix wsp:   <http://example.org/namespace/ble-gatt/wsp#> .
@prefix tip:   <http://example.org/namespace/ble-gatt/tip#> .
@prefix ble:   <http://example.org/namespace/ble-gatt#> .
@prefix rscp:  <http://example.org/namespace/ble-gatt/rscp#> .
@prefix rcp:   <http://example.org/namespace/ble-gatt/rcp#> .
@prefix cpp:   <http://example.org/namespace/ble-gatt/cpp#> .
@prefix anp:   <http://example.org/namespace/ble-gatt/anp#> .
@prefix aiop:  <http://example.org/namespace/ble-gatt/aiop#> .
@prefix scpp:  <http://example.org/namespace/ble-gatt/scpp#> .
@prefix htp:   <http://example.org/namespace/ble-gatt/htp#> .
@prefix hrp:   <http://example.org/namespace/ble-gatt/hrp#> .
@prefix blp:   <http://example.org/namespace/ble-gatt/blp#> .
@prefix pxp:   <http://example.org/namespace/ble-gatt/pxp#> .
@prefix cgmp:  <http://example.org/namespace/ble-gatt/cgmp#> .
@prefix otp:   <http://example.org/namespace/ble-gatt/otp#> .
@prefix glp:   <http://example.org/namespace/ble-gatt/glp#> .
@prefix lnp:   <http://example.org/namespace/ble-gatt/lnp#> .
@prefix cscp:  <http://example.org/namespace/ble-gatt/cscp#> .
@prefix idp:   <http://example.org/namespace/ble-gatt/idp#> .
@prefix ipsp:  <http://example.org/namespace/ble-gatt/ipsp#> .
@prefix pasp:  <http://example.org/namespace/ble-gatt/pasp#> .

ble:HTTPStatusCode  a    skos:Concept ;
        rdfs:label       "HTTP Status Code" ;
        skos:definition  "The HTTP Status Code characteristic contains the Status-Code from the Status-Line of the first line of the HTTP Response message, followed by one octet indicating the Data Status bit field indicating the status of the data received." ;
        skos:inScheme    ble: ;
        skos:related     ble:Notify , xsd:unsignedShort .

lehid:ReportValue  a     skos:Concept ;
        rdfs:label       "Report Value" ;
        skos:definition  "The Report characteristic value contains Input Report, Output Report or Feature Report data to be transferred between the HID Device and HID Host." ;
        skos:inScheme    ble: ;
        skos:related     xsd:unsignedByte .

cpp:CyclingPowerFeature
        a                skos:Concept ;
        rdfs:label       "Cycling Power Feature" ;
        skos:definition  "The Cycling Power Feature characteristic shall be used to describe the supported features of the Server." ;
        skos:inScheme    ble: ;
        skos:related     ble:Read .

ftmp:LowIntensityInterval
        a                skos:Concept ;
        rdfs:label       "Low Intensity Interval" ;
        skos:definition  "0x03-Low Intensity Interval" ;
        skos:inScheme    ble: .

lehid:BootKeyboardOutputReportValue
        a                skos:Concept ;
        rdfs:label       "Boot Keyboard Output Report Value" ;
        skos:definition  "The Boot Keyboard Output Report characteristic value is an array of octets whose meaning is defined in the USB HID Usage." ;
        skos:inScheme    ble: ;
        skos:related     xsd:unsignedByte .

ble:Value  a           skos:Concept ;
        skos:inScheme  ble: ;
        skos:narrower  wsp:BasalMetabolismField , idp:SystemIssue , ftmp:WarmingUp , lehid:Suspend , idp:BolusExtendedAmountfield , lnp:TotalDistanceField , idp:TBRCanceled , ble:BluetoothSIG , otp:ObjectIDField , idp:Off , otp:ObjectLastModifiedField , idp:ReservoirRemainingAmountfield , ftmp:AverageStepRateField , idp:Priming , idp:BatteryFull , ftmp:MinimumPowerIncrementfield , glp:MedicationIDField , idp:MechanicalIssue , ftmp:MinimumSpeedfield , ble:InstantaneousSpeedField , wsp:MusclePercentageField , ftmp:TrainingStatusField , idp:GenericDevice , plxp:SpO2PRNormalfield , idp:Preparing , glp:MealField , glp:CarbohydrateField , lnp:BeaconsNumberViewField , cpp:PedalPowerBalanceField , cpp:TopDeadSpotAngleField , ftmp:MinimumInclinationfield , ftmp:FloorsField , idp:Run , ftmp:AveragePaceField , glp:ExerciseIntensityField , ftmp:AverageSpeedField , ble:ProductVersionField , idp:DateTimeIssue , rscp:TotalDistanceField , cgmp:E2ECRCField , ble:LastCrankEventTime , idp:BolusDelayTime , idp:ReservoirLow , ble:Serverrequiresrefresh , ble:LatitudeValue , ble:USBImplementerForum , idp:BatteryMedium , plxp:PulseAmplitudeIndex , idp:TherapyControlStatefield , lnp:BeaconsNumberSolutionField , ftmp:MinimumInclinationIncrementfield , glp:MedicationField , idp:BolusFastAmountfield , cpp:CumulativeWheelRevolutions , ble:UncertaintyValue , lehid:BootMouseInputReportValue , lnp:EHPEField , cpp:MaximumTorqueMagnitude , idp:TBROver , wsp:BIM , wsp:ImpedanceField , ble:LocalNorthCoordinateValue , ble:LocalEastCoordinateValue , idp:AuxInfo4UpperBoundfield , ftmp:MinimumHeartRateIncrementfield , ftmp:StrokeRateField , idp:EventData , cpp:FirstCrankMeasurementAngleField , otp:CurrentSizeField , ftmp:AverageCadenceField , glp:BaseTimeField , ftmp:StepperMinuteField , ble:ProductIDField , ftmp:MinimumResistanceIncrementfield , ftmp:HeartRateControl , ftmp:MinimumPowerfield , glp:CarbohydrateIDField , lnp:BearingField , lnp:RemainingDistanceField , ftmp:PostWorkout , idp:Confirmed , ftmp:InstantaneousPaceField , pxp:TxPowerLevelField , ble:FloorNumberValue , idp:Waiting , ftmp:AveragePowerField , glp:GlucoseConcentrationField , lehid:ProtocolModeValue , ble:InstantaneousPowerField , ftmp:MinimumSpeedIncrementfield , anp:CategoryID , htp:MeasurementIntervalValue , ftmp:ResistanceLevelField , idp:OcclusionDetected , ftmp:RemainingTimeField , idp:Stop , idp:Pause , anp:TextStringInformation , idp:InfusionSetIncomplete , ftmp:Idle , cgmp:DTSOffsetField , ble:VendorIDField , idp:Undetermined , idp:BolusCanceled , rscp:InstantaneousStrideLengthField , idp:ReservoirIssue , ftmp:MinimumResistanceLevelField , lnp:LocationLongitude , otp:ObjectNameField , ftmp:EnergyperMinuteField , ftmp:LowSpeedOutside , cpp:MinimumTorqueMagnitude , htp:IntermediateTemperatureValueField , lehid:ReportMapValue , lehid:ReportProtocolMode , ble:LocationNameValue , ble:CumulativeCrankRevolutions , wsp:HeightField , idp:BatteryEmpty , idp:AnnunciationInstanceID , ftmp:CoolDown , rscp:InstantaneousCadenceField , ble:TransportDataField , idp:InfusionSetDetached , anp:NumberofNewAlert , cpp:MinimumForceMagnitude , wsp:BodyFatPercentageField , cgmp:CGMTrendInformationField , cpp:InstantaneousTorqueMagnitudeArrayField , ftmp:MaximumHeartRatefield , idp:InsulinConcentrationfield , otp:ObjectFirstCreatedField , lnp:ElevationField , lnp:RollingTimeField , aiop:AnalogSignalValue , idp:Ready , pasp:AlertStatusValue , ftmp:MetabolicEquivalentField , idp:MaxDelivery , plxp:SpO2PRSpotCheckField , cscp:CumulativeWheelRevolutions , idp:Snoozed , cgmp:TimeZoneField , idp:AnnunciationType , ftmp:HighIntensityInterval , idp:Temperature , glp:SequenceNumberField , idp:Pending , ftmp:MaximumResistanceLevelField , lehid:HIDControlPointCharacteristicValue , ftmp:LowIntensityInterval , idp:ReservoirEmpty , ftmp:ManualMode , cgmp:CGMGlucoseConcentrationField , ftmp:ElapsedTimeField , ble:UserIDField , ble:TimeStampField , cpp:InstantaneousForceMagnitudeArrayField , idp:BolusDurationfield , cpp:MinimumAngle , idp:ManufacturerReserved , plxp:SpO2PRSlowfield , idp:AnnunciationStatus , idp:Temperatureoutofrange , cgmp:SizeField , ble:LE_Scan_Interval , ftmp:StrokeCountField , ftmp:MinimumHeartRatefield , ftmp:NegativeElevationGainField , idp:AuxInfo2Contextfield , ftmp:InstantaneousCadenceField , otp:AllocatedSizeField , cgmp:CGMQualityField , ftmp:PositiveElevationGainField , ble:ManufacturerIdentifier , lnp:HDOPField , ftmp:InclinationField , ftmp:EnergyperHourField , cpp:MaximumForceMagnitude , blp:IntermediateCuffPressureCompoundValueField , ftmp:AverageStrokeRateField , htp:TemperatureMeasurementValueField , idp:PrimingIssue , lnp:EstimatedTimeArrivalField , idp:SequenceNumberfield , ble:VendorIDSourceField , ftmp:HeartRateField , ftmp:MaximumPowerfield , lnp:UTCTimeField , ble:DatabaseChangeIncrementValue , blp:PulseRateField , glp:TimeOffsetField , lehid:BootProtocolMode , blp:BloodPressureMeasurementCompoundValueField , idp:Standby , glp:HbA1cField , idp:BolusIDfield , cgmp:TimeOffsetField , idp:Insulin , ble:OrganizationallyUniqueIdentifier , idp:AuxInfo3LowerBoundfield , ftmp:TrainingStatusStringField , plxp:SpO2PRFastfield , ftmp:StrideCountField , ftmp:PreWorkout , idp:RelativeOffsetfield , ftmp:MaximumInclinationfield , cscp:LastWheelEventTime , lehid:ExitSuspend , ftmp:WattControl , lnp:HeadingField , ftmp:StepCountField , glp:ExerciseDurationField , ftmp:Isometric , wsp:WeightField , idp:PowerSourceInsufficient , cpp:AccumulatedTorqueField , lehid:bcdHID , lnp:TimetoFirstFixField , ble:UDSCharacteristicValue , wsp:BodyWaterField , cpp:LastWheelEventTime , wsp:SoftLeanMassField , lnp:RemainingVerticalDistanceField , hrp:HeartRateValueField , ftmp:RecoveryInterval , ble:OrganizationIDField , idp:E2ECRCfield , cgmp:SessionStartTimeField , wsp:MuscleMassField , ftmp:RampAngleSettingField , lnp:VDOPField , ftmp:TotalDistanceField , ftmp:PowerOutputField , lehid:ReportValue , ftmp:HighSpeedOutside , ftmp:TotalEnergyField , ble:IndoorPositioningValue , idp:E2ECounterfield , ftmp:ForceonBeltField , ble:LongitudeValue , ble:AltitudeValue , cpp:MaximumAngle , lnp:LocationLatitude , lehid:bCountryCode , lehid:BootKeyboardOutputReportValue , lnp:EVPEField , ftmp:MaximumSpeedfield , idp:Airpressureoutofrange , wsp:FatFreeMassField , lehid:BootKeyboardInputReportValue , hrp:RRIntervalField , ble:TransportDataLengthField , hrp:EnergyExpendedField , idp:OperationalStatefield , cgmp:cgmpSessionRunTimeField , ble:LE_Scan_Window , cpp:AccumulatedEnergyField , idp:AuxInfo1Valuefield , ftmp:FitnessTest , idp:BatteryLow , cpp:BottomDeadSpotAngleField .

glp:GlucoseMeasurementContext
        a                skos:Concept ;
        rdfs:label       "Glucose Measurement Context" ;
        skos:definition  "The Glucose Measurement Context characteristic may be used to send additional contextual information relative to a Glucose Measurement characteristic." ;
        skos:inScheme    ble: ;
        skos:related     glp:MealField , glp:ExerciseIntensityField , glp:MedicationIDField , glp:HbA1cField , glp:SequenceNumberField , glp:ExerciseDurationField , glp:CarbohydrateIDField , glp:MedicationField , glp:CarbohydrateField .

otp:OTSFeature  a        skos:Concept ;
        rdfs:label       "Object Transfer Service Feature" ;
        skos:definition  "The OTS Feature characteristic exposes which optional features are supported by the Server implementation." ;
        skos:inScheme    ble: ;
        skos:related     ble:Read .

esp:ESConfigurationDescriptor
        a                skos:Concept ;
        rdfs:label       "Environmental Sensing Configuration Descriptor" ;
        skos:definition  "The ES Configuration descriptor shall be present if more than one ES Trigger Setting descriptor is present for an associated ESS Characteristic. Otherwise it shall not be present for that characteristic" ;
        skos:inScheme    ble: ;
        skos:related     ble:Read , ble:Write .

ftmp:PowerOutputField
        a                skos:Concept ;
        rdfs:label       "Power Output Field" ;
        skos:definition  "The Power Output field represents the power being applied to the treadmill by the user’s steps" ;
        skos:inScheme    ble: ;
        skos:related     xsd:short .

idp:GenericDevice  a     skos:Concept ;
        rdfs:label       "Generic Device" ;
        skos:definition  "The reported temperature refers to the Insulin Delivery Device in general." ;
        skos:inScheme    ble: .

tip:TimewithDST  a       skos:Concept ;
        rdfs:label       "Time with Daylight Saving Time" ;
        skos:definition  "The Next DST Change Server returns the Time with DST to the time when the next DST change will occur and the DST offset that will be in effect after this change." ;
        skos:inScheme    ble: ;
        skos:related     ble:Read .

lnp:EstimatedTimeArrivalField
        a                skos:Concept ;
        rdfs:label       "Estimated Time of Arrival Field" ;
        skos:definition  "The Estimated Time of Arrival field represents the remaining time from the current position to reach the next waypoint or final destination." ;
        skos:inScheme    ble: .

pxp:LinkLossService  a   skos:Concept ;
        rdfs:label       "Link Loss Service" ;
        rdfs:seeAlso     <https://www.bluetooth.org/DocMan/handlers/DownloadDoc.ashx?doc_id=303198> ;
        owl:versionInfo  "1.0.1" ;
        skos:definition  "This service defines behavior when a link is lost between two devices." ;
        skos:inScheme    ble: ;
        skos:related     pxp:LinkLossAlertLevel .

cgmp:cgmpSessionRunTime
        a                skos:Concept ;
        rdfs:label       "cgmp Session Run Time" ;
        skos:definition  "The cgmp Session Run Time shall define the expected run time of the cgmp session." ;
        skos:inScheme    ble: ;
        skos:related     cgmp:E2ECRCField , ble:Read , cgmp:cgmpSessionRunTimeField .

ftmp:SupportedPowerRange
        a                skos:Concept ;
        rdfs:label       "Supported Power Range" ;
        skos:definition  "The Supported Power Range characteristic is used to send the supported power range as well as the minimum power increment supported by the Server." ;
        skos:inScheme    ble: ;
        skos:related     ble:Read , ftmp:MinimumPowerfield , ftmp:MaximumPowerfield , ftmp:MinimumPowerIncrementfield .

lnp:LocationandNavigationProfile
        a                skos:Concept ;
        rdfs:label       "Location and Navigation Profile" ;
        rdfs:seeAlso     <https://www.bluetooth.org/DocMan/handlers/DownloadDoc.ashx?doc_id=271996> ;
        owl:versionInfo  "1.0" ;
        skos:definition  "This profile enables a Collector device to connect and interact with a Location and Navigation Sensor for use in outdoor activity applications." ;
        skos:inScheme    ble: ;
        skos:related     ble:DeviceInformationService , lnp:LocationandNavigationService , ble:BatteryService .

blp:BloodPressureMeasurementCompoundValueField
        a                skos:Concept ;
        rdfs:label       "Blood Pressure Measurement Compound Value Field" ;
        skos:definition  "It is composed of three subfields: Systolic, Diastolic and Mean Arterial Pressure (MAP)" ;
        skos:inScheme    ble: ;
        skos:related     xsd:float .

ble:Serverrequiresrefresh
        a                skos:Concept ;
        rdfs:label       "Server requires refresh" ;
        skos:definition  "Scan Refresh characteristic value  is a single octet." ;
        skos:inScheme    ble: ;
        skos:related     xsd:unsignedByte .

plxp:PulseOximeterService
        a                skos:Concept ;
        rdfs:label       "Pulse Oximeter Service" ;
        rdfs:seeAlso     <https://www.bluetooth.org/DocMan/handlers/DownloadDoc.ashx?doc_id=304965> ;
        owl:versionInfo  "1.0" ;
        skos:definition  "This Service specification defines a pulse oximetry sensor for use in consumer and professional healthcare applications." ;
        skos:inScheme    ble: ;
        skos:related     ble:RecordAccessControlPoint , plxp:PLXContinuousMeasurement , plxp:PLXSpotcheckMeasurement , plxp:PLXFeatures .

ftmp:AverageCadenceField
        a                skos:Concept ;
        rdfs:label       "Average Cadence Field" ;
        skos:definition  "The Average Cadence field represents the average cadence since the beginning of the training session." ;
        skos:inScheme    ble: ;
        skos:related     xsd:unsignedShort .

ftmp:IndoorBikeData  a   skos:Concept ;
        rdfs:label       "Indoor Bike Data" ;
        skos:definition  "The Indoor Bike Data characteristic is used to send training-related data to the Client from an indoor bike (Server)." ;
        skos:inScheme    ble: ;
        skos:related     ble:Notify , ble:InstantaneousPowerField , ftmp:TotalDistanceField , ftmp:HeartRateField , ftmp:EnergyperHourField , ftmp:MetabolicEquivalentField , ftmp:AverageCadenceField , ftmp:ResistanceLevelField , ftmp:RemainingTimeField , ftmp:ElapsedTimeField , ftmp:TotalEnergyField , ftmp:AverageSpeedField , ftmp:EnergyperMinuteField , ble:InstantaneousSpeedField , ftmp:InstantaneousCadenceField , ftmp:AveragePowerField .

cpp:AccumulatedEnergyField
        a                skos:Concept ;
        rdfs:label       "Accumulated Energy Field" ;
        skos:definition  "The Accumulated Energy field represents the accumulated value of the energy measured by the sensor." ;
        skos:inScheme    ble: .

cgmp:SizeField  a        skos:Concept ;
        rdfs:label       "Size Field" ;
        skos:definition  "The Size Field represents the size of the CGM Measurement record." ;
        skos:inScheme    ble: ;
        skos:related     xsd:unsignedByte .

ble:SensorLocation  a    skos:Concept ;
        rdfs:label       "Sensor Location" ;
        skos:definition  "The Sensor Location characteristic of the device is used to describe the physical location of the Server when correctly fitted." ;
        skos:inScheme    ble: ;
        skos:related     ble:Read , xsd:unsignedByte .

ble:ModelNumber  a       skos:Concept ;
        rdfs:label       "Model Number" ;
        skos:definition  "The Model Number String characteristic shall represent the model number that is assigned by the device vendor." ;
        skos:inScheme    ble: ;
        skos:related     ble:Read , xsd:string .

ftmp:SupportedHeartRateRange
        a                skos:Concept ;
        rdfs:label       "Supported Heart Rate Range" ;
        skos:definition  "The Supported Heart Rate Range characteristic is used to send the supported Heart Rate range as well as the minimum Heart Rate increment supported by the Server." ;
        skos:inScheme    ble: ;
        skos:related     ble:Read , ftmp:MinimumHeartRatefield , ftmp:MaximumHeartRatefield , ftmp:MinimumHeartRateIncrementfield .

idp:Ready  a             skos:Concept ;
        rdfs:label       "Ready" ;
        skos:definition  "The Insulin Delivery Device is ready for the insulin infusion therapy" ;
        skos:inScheme    ble: .

lehid:ProtocolModeValue
        a                skos:Concept ;
        rdfs:label       "Protocol Mode Characteristic Value" ;
        skos:definition  "The Protocol Mode characteristic value can have the values representing the current Protocol Mode of the HID Service" ;
        skos:inScheme    ble: ;
        skos:narrower    lehid:ReportProtocolMode , lehid:BootProtocolMode ;
        skos:related     xsd:unsignedByte .

idp:Standby  a           skos:Concept ;
        rdfs:label       "Stand By" ;
        skos:definition  "No insulin is delivered and resuming from this state is faster than from state Off" ;
        skos:inScheme    ble: .

wsp:FatFreeMassField  a  skos:Concept ;
        rdfs:label       "Fat Free Mass Field" ;
        skos:definition  "The Fat Free Mass field may be included in the Body Composition Measurement characteristic if the device supports the Fat Free Mass feature." ;
        skos:inScheme    ble: ;
        skos:related     xsd:unsignedShort .

ble:LongitudeValue  a    skos:Concept ;
        rdfs:label       "The current value of the Longitude Characteristic" ;
        skos:definition  "When read, the Server shall return the current value of the Longitude Characteristic." ;
        skos:inScheme    ble: ;
        skos:related     xsd:integer .

idp:MechanicalIssue  a   skos:Concept ;
        rdfs:label       "Mechanical Issue" ;
        skos:definition  "A mechanical error occurred" ;
        skos:inScheme    ble: .

ble:TimeStampField  a    skos:Concept ;
        rdfs:label       "Time Stamp Field" ;
        skos:definition  "The value of the Time Stamp field is derived from a source of date and time at the time of measurement." ;
        skos:inScheme    ble: .

tip:TimeUpdateControlPoint
        a                skos:Concept ;
        rdfs:label       "Time Update Control Point" ;
        skos:definition  "The Time Update Control Point characteristic is used to request a reference time update on the server." ;
        skos:inScheme    ble: ;
        skos:related     ble:WritewithoutResponse , xsd:unsignedByte .

ble:ReliableWrite  a     skos:Concept ;
        rdfs:label       "Reliable Write" ;
        skos:definition  "Characteristic Value is written to a server when the client knows the Characteristic Value Handle, and assurance is required that the correct Characteristic Value is going to be written by transferring the Characteristic Value to be written in both directions before the write is performed." ;
        skos:inScheme    ble: .

hrp:HeartRateProfile  a  skos:Concept ;
        rdfs:label       "Heart Rate Profile" ;
        rdfs:seeAlso     <https://www.bluetooth.org/docman/handlers/downloaddoc.ashx?doc_id=239865> ;
        owl:versionInfo  "1.0" ;
        skos:definition  "The Heart Rate Profile is used to enable a data collection device to obtain data from a Heart Rate Sensor that exposes the Heart Rate Service." ;
        skos:inScheme    ble: ;
        skos:related     hrp:HeartRateService , ble:DeviceInformationService .

ble:TransportDataField
        a                skos:Concept ;
        rdfs:label       "Transport Data Field" ;
        skos:definition  "If used, this field contains organization-specific data and shall be byte-aligned." ;
        skos:inScheme    ble: .

idp:AuxInfo1Valuefield
        a                skos:Concept ;
        rdfs:label       " AuxInfo1 Value field" ;
        skos:definition  "The AuxInfo1 field shall contain the value of the temperature." ;
        skos:inScheme    ble: ;
        skos:related     xsd:float .

idp:IDDAnnunciationStatus
        a                skos:Concept ;
        rdfs:label       "Insulin Delivery Device Annunciation Status" ;
        skos:definition  "The IDD Annunciation Status characteristic is a variable length structure comprising of messages that describe state changes of the Insulin Delivery Device and in the therapy relevant functions." ;
        skos:inScheme    ble: ;
        skos:related     idp:AnnunciationInstanceID , idp:AuxInfo3LowerBoundfield , idp:E2ECounterfield , idp:AuxInfo2Contextfield , ble:Read , idp:E2ECRCfield , idp:AnnunciationStatus , ble:Indicate , idp:AnnunciationType , idp:AuxInfo4UpperBoundfield , idp:AuxInfo1Valuefield .

glp:SequenceNumberField
        a                skos:Concept ;
        rdfs:label       "Sequence Number Field" ;
        skos:definition  "The Sequence Number represents the chronological order of the patient records in the Server measurement database." ;
        skos:inScheme    ble: ;
        skos:related     xsd:unsignedShort .

esp:ESMeasurementDescriptor
        a                skos:Concept ;
        rdfs:label       "Environmental Sensing Measurement Descriptor" ;
        skos:definition  "This optional characteristic descriptor describes the associated ESS Characteristic by providing additional information pertaining to the value." ;
        skos:inScheme    ble: ;
        skos:related     ble:Read .

ipsp:InternetProtocolSupportProfile
        a                skos:Concept ;
        rdfs:label       "Internet Protocol Support Profile" ;
        rdfs:seeAlso     <https://www.bluetooth.org/docman/handlers/DownloadDoc.ashx?doc_id=296307> ;
        owl:versionInfo  "1.0" ;
        skos:definition  "This Profile Specification proposes the support of exchanging IPv6 packets between devices over the Bluetooth Low Energy transport." ;
        skos:inScheme    ble: ;
        skos:related     ipsp:IPSupportService .

rscp:RSCMeasurement  a   skos:Concept ;
        rdfs:label       "Running Speed and Cadence Measurement" ;
        skos:definition  "The RSC Measurement characteristic is used to send speed and cadence measurements." ;
        skos:inScheme    ble: ;
        skos:related     ble:Notify , rscp:InstantaneousStrideLengthField , ble:InstantaneousSpeedField , rscp:InstantaneousCadenceField , rscp:TotalDistanceField .

cgmp:CGMQualityField  a  skos:Concept ;
        rdfs:label       "Continuous Glucose Monitoring Quality Field" ;
        skos:definition  "This field contains the CGM Quality information in % as an SFLOAT data type." ;
        skos:inScheme    ble: ;
        skos:related     xsd:float .

ble:IndoorPositioningService
        a                skos:Concept ;
        rdfs:label       "Indoor Positioning Service" ;
        rdfs:seeAlso     <https://www.bluetooth.org/docman/handlers/downloaddoc.ashx?doc_id=302114> ;
        owl:versionInfo  "1.0" ;
        skos:definition  "The Indoor Positioning Service exposes location information to support mobile devices to position themselves in an environment where GNSS signals are not available, for example in indoor premises." ;
        skos:inScheme    ble: ;
        skos:related     ble:FloorNumber , ble:LocationName , ble:LocalEastCoordinate , ble:HTTPSSecurity , ble:Uncertainty , ble:LocalNorthCoordinate , ble:Altitude , ble:HTTPHeaders , ble:HTTPEntityBody , ble:IndoorPositioningConfiguration , ble:HTTPStatusCode , ble:URI , ble:Longitude , ble:HTTPControlPoint , ble:Latitude .

idp:BolusFastAmountfield
        a                skos:Concept ;
        rdfs:label       "Bolus Fast Amount field" ;
        skos:definition  "The Bolus Fast Amount field represents the fast amount of the bolus." ;
        skos:inScheme    ble: ;
        skos:related     xsd:float .

ftmp:StepperMinuteField
        a                skos:Concept ;
        rdfs:label       "Step per Minute Field" ;
        skos:definition  "The Step per Minute Rate field represents the average step rate of a user during a period of one minute." ;
        skos:inScheme    ble: ;
        skos:related     xsd:unsignedShort .

esp:EnvironmentalSensingService
        a                skos:Concept ;
        rdfs:label       "Environmental Sensing Service" ;
        rdfs:seeAlso     <https://www.bluetooth.org/docman/handlers/downloaddoc.ashx?doc_id=294797> ;
        owl:versionInfo  "1.0.0" ;
        skos:definition  "The Environmental Sensing Service (ESS) exposes measurement data from an environmental sensor intended for sports and fitness applications." ;
        skos:inScheme    ble: ;
        skos:related     esp:ESConfigurationDescriptor , esp:ESTriggerSettingDescriptor , esp:DescriptorValueChanged , esp:ValidRangeDescriptor , esp:CharacteristicUserDescription , esp:ESMeasurementDescriptor .

idp:IDDStatusReaderControlPoint
        a                skos:Concept ;
        rdfs:label       "Insulin Delivery Device Status Reader Control Point" ;
        skos:definition  "The IDD Status Reader Control Point provides insulin therapy relevant status information (e.g., currently running boluses or current basal rate)." ;
        skos:inScheme    ble: ;
        skos:related     idp:E2ECRCfield , idp:E2ECounterfield , idp:BolusDelayTime , idp:BolusExtendedAmountfield , idp:BolusFastAmountfield , idp:BolusDurationfield , ble:Write , ble:Indicate , idp:BolusIDfield .

ble:HTTPSSecurity  a     skos:Concept ;
        rdfs:label       "HTTPS Security" ;
        skos:definition  "The HTTPS Security characteristic contains the known authenticity of the HTTP Server certificate for the URI." ;
        skos:inScheme    ble: ;
        skos:related     ble:Read , xsd:boolean .

idp:Airpressureoutofrange
        a                skos:Concept ;
        rdfs:label       "Air pressure out of range" ;
        skos:definition  "The air pressure is outside of the normal operating range (e.g., altitude)." ;
        skos:inScheme    ble: .

ble:LE_Scan_Window  a    skos:Concept ;
        rdfs:label       "Low Energy_Scan_Interval" ;
        skos:definition  "The maximum LE_Scan_Interval of the Clien." ;
        skos:inScheme    ble: ;
        skos:related     xsd:unsignedShort .

wsp:SoftLeanMassField
        a                skos:Concept ;
        rdfs:label       "Soft Lean Mass Field" ;
        skos:definition  "The Soft Lean Mass field may be included in the Body Composition Measurement characteristic if the device supports the Soft Lean Mass feature." ;
        skos:inScheme    ble: ;
        skos:related     xsd:unsignedShort .

ftmp:SupportedInclinationRange
        a                skos:Concept ;
        rdfs:label       "Supported Inclination Range" ;
        skos:definition  "The Supported Inclination Range characteristic is used to send the supported inclination range as well as the minimum inclination increment supported by the Server." ;
        skos:inScheme    ble: ;
        skos:related     ftmp:MaximumInclinationfield , ble:Read , ftmp:MinimumInclinationIncrementfield , ftmp:MinimumInclinationfield .

ble:UDSCharacteristic
        a                skos:Concept ;
        rdfs:label       "User Data Service Characteristic" ;
        skos:definition  "Each UDS Characteristic is defined in the User Data Service Characteristics table" ;
        skos:inScheme    ble: ;
        skos:related     ble:Read , ble:UDSCharacteristicValue , ble:Write .

ftmp:FitnessMachineProfile
        a                skos:Concept ;
        rdfs:label       "Fitness Machine Profile" ;
        rdfs:seeAlso     <https://www.bluetooth.org/DocMan/handlers/DownloadDoc.ashx?doc_id=423417> ;
        owl:versionInfo  "1.0" ;
        skos:definition  "The Fitness Machine Profile is used to enable a data collection device to obtain data from a Fitness Machine that exposes the Fitness Machine Service." ;
        skos:inScheme    ble: ;
        skos:related     ftmp:FitnessMachineService , ble:UserDataService , ble:DeviceInformationService .

pxp:TxPowerLevelField
        a                skos:Concept ;
        rdfs:label       "Transmit Power Level Field" ;
        skos:definition  "The Tx Power Level characteristic returns the current transmit power level when read using the GATT Characteristic Read Value procedure." ;
        skos:inScheme    ble: ;
        skos:related     xsd:byte .

idp:Pause  a             skos:Concept ;
        rdfs:label       "Pause" ;
        skos:definition  "The insulin infusion therapy is paused (i.e., the device does not deliver insulin related to the therapy but delivers the missed amount of insulin after leaving state Pause and entering state Run)." ;
        skos:inScheme    ble: .

cgmp:TimeZoneField  a    skos:Concept ;
        rdfs:label       "Time zone Field" ;
        skos:definition  "To know an absolute Time, it is necessary to know the Time Zone to which the Session  Start Time is related to." ;
        skos:inScheme    ble: ;
        skos:related     xsd:byte .

cgmp:DTSOffsetField  a   skos:Concept ;
        rdfs:label       "Daylight Saving Time Offset Field" ;
        skos:definition  "To know an absolute Time, it is also necessary to know the Daylight Saving setting" ;
        skos:inScheme    ble: ;
        skos:related     xsd:unsignedByte .

tip:ReferenceTimeUpdateService
        a                skos:Concept ;
        rdfs:label       "Reference Time Update Service" ;
        rdfs:seeAlso     <https://www.bluetooth.org/docman/handlers/downloaddoc.ashx?doc_id=241873> ;
        owl:versionInfo  "1.0" ;
        skos:definition  "This service defines how a client can request an update from a reference time source from a time server using the Generic Attribute Profile (GATT)." ;
        skos:inScheme    ble: ;
        skos:related     tip:TimeUpdateControlPoint , tip:TimeUpdateState .

lnp:RemainingVerticalDistanceField
        a                skos:Concept ;
        rdfs:label       "Remaining Vertical Distance Field" ;
        skos:definition  "The Remaining Vertical Distance field represents the vertical distance from the current position to the next waypoint or final destination." ;
        skos:inScheme    ble: ;
        skos:related     xsd:integer .

cpp:CumulativeWheelRevolutions
        a                skos:Concept ;
        rdfs:label       "Wheel Revolution Data - Cumulative Wheel Revolutions" ;
        skos:definition  "The Cumulative Wheel Revolutions value, one value of The Wheel Revolution Data field pair, represents the number of times a wheel rotates" ;
        skos:inScheme    ble: ;
        skos:related     xsd:unsignedShort , xsd:unsignedInt .

otp:ObjectIDField  a     skos:Concept ;
        rdfs:label       "Object ID Field" ;
        skos:definition  "The Server shall allocate an Object ID value to each object when the object is created on the Server. The Object ID characteristic returns its associated value when read." ;
        skos:inScheme    ble: ;
        skos:related     xsd:unsignedInt .

ble:ReadLong  a          skos:Concept ;
        rdfs:label       "Read Long" ;
        skos:definition  "Characteristic Value is read from a server when the client knows the Characteristic Value Handle and the length of the Characteristic Value is longer than can be sent in a single Read Response Attribute protocol message." ;
        skos:inScheme    ble: .

lnp:PositionQuality  a   skos:Concept ;
        rdfs:label       "Position Quality" ;
        skos:definition  "The Position Quality characteristic is used to send position quality-related data" ;
        skos:inScheme    ble: ;
        skos:related     lnp:VDOPField , lnp:EHPEField , lnp:TimetoFirstFixField , ble:Read , lnp:EVPEField , lnp:BeaconsNumberViewField , lnp:HDOPField , lnp:BeaconsNumberSolutionField .

glp:GlucoseMeasurement
        a                skos:Concept ;
        rdfs:label       "Glucose Measurement" ;
        skos:definition  "The Glucose Measurement characteristic shall be used to send glucose measurements." ;
        skos:inScheme    ble: ;
        skos:related     glp:TimeOffsetField , glp:BaseTimeField , glp:GlucoseConcentrationField , glp:SequenceNumberField .

ble:BatteryService  a    skos:Concept ;
        rdfs:label       "Battery Service" ;
        rdfs:seeAlso     <https://www.bluetooth.org/docman/handlers/downloaddoc.ashx?doc_id=245138> ;
        owl:versionInfo  "1.0" ;
        skos:definition  "The Battery Service exposes the Battery Level of a single battery or set of batteries in a device." ;
        skos:inScheme    ble: ;
        skos:related     ble:BatteryLevel .

idp:TBRCanceled  a       skos:Concept ;
        rdfs:label       "The temporary basal Canceled" ;
        skos:definition  "The temporary basal rate canceled (e.g., device changed from run to standby mode)." ;
        skos:inScheme    ble: .

cscp:CyclingSpeedandCadenceService
        a                skos:Concept ;
        rdfs:label       "Cycling Speed and Cadence Service" ;
        rdfs:seeAlso     <https://www.bluetooth.org/docman/handlers/downloaddoc.ashx?doc_id=261450> ;
        owl:versionInfo  "1.0" ;
        skos:definition  "The Cycling Speed and Cadence (CSC) Service exposes speed-related data and/or cadence-related data while using the Cycling Speed and Cadence sensor (Server)." ;
        skos:inScheme    ble: ;
        skos:related     cscp:CSCFeature , ble:SCControlPoint , cscp:CSCMeasurement , ble:SensorLocation .

cpp:MaximumAngle  a      skos:Concept ;
        rdfs:label       "Maximum Angle Field" ;
        skos:definition  "The Maximum Angle field represents the angle of the crank when the maximum value is measured in a single crank revolution." ;
        skos:inScheme    ble: ;
        skos:related     xsd:unsignedByte .

ble:WriteLong  a         skos:Concept ;
        rdfs:label       "Write Long" ;
        skos:definition  "Characteristic Value is written to a server when the client knows the Characteristic Value Handle but the length of the Characteristic Value is longer than can be sent in a single Write Request Attribute protocol message." ;
        skos:inScheme    ble: .

idp:BatteryLow  a        skos:Concept ;
        rdfs:label       "Battery Low" ;
        skos:definition  "The Insulin Delivery Device has a low operational runtime" ;
        skos:inScheme    ble: .

ble:UserIDField  a       skos:Concept ;
        rdfs:label       "User ID Field" ;
        skos:definition  "The User ID field shall be included in the characteristic if the device supports the Multiple Users feature." ;
        skos:inScheme    ble: ;
        skos:related     xsd:unsignedByte .

hrp:EnergyExpendedField
        a                skos:Concept ;
        rdfs:label       "Energy Expended Field" ;
        skos:definition  "The Energy Expended field represents the accumulated energy expended in kilo Joules since the last time it was reset." ;
        skos:inScheme    ble: ;
        skos:related     xsd:unsignedShort .

ftmp:HeartRateControl
        a                skos:Concept ;
        rdfs:label       "Heart Rate Control" ;
        skos:definition  "0x07 - Heart Rate Control" ;
        skos:inScheme    ble: .

ftmp:MinimumResistanceIncrementfield
        a                skos:Concept ;
        rdfs:label       "Minimum Resistance Increment" ;
        skos:definition  "Unitless with a resolution of 0.1" ;
        skos:inScheme    ble: ;
        skos:related     xsd:unsignedShort .

idp:EventData  a         skos:Concept ;
        rdfs:label       "Recording Reason field" ;
        skos:definition  "The Recording Reason field specifies the reason why the Reference Time event was recorded." ;
        skos:inScheme    ble: .

idp:AuxInfo4UpperBoundfield
        a                skos:Concept ;
        rdfs:label       "AuxInfo4 Upper Bound field" ;
        skos:definition  "The AuxInfo4 field shall contain the value of the upper bound of the temperature." ;
        skos:inScheme    ble: ;
        skos:related     xsd:float .

ftmp:ResistanceLevelField
        a                skos:Concept ;
        rdfs:label       "Resistance Level Field" ;
        skos:definition  "The Resistance Level field represents the value of the current value of the resistance level of the Server." ;
        skos:inScheme    ble: ;
        skos:related     xsd:short .

ble:CurrentTime  a       skos:Concept ;
        rdfs:label       "Current Time" ;
        skos:definition  "The Current Time characteristic returns the current date and time in the server device." ;
        skos:inScheme    ble: ;
        skos:related     ble:Notify , ble:Read , ble:Write .

ble:ManufacturerName  a  skos:Concept ;
        rdfs:label       "Manufacturer Name" ;
        skos:definition  "The Manufacturer Name String characteristic shall represent the name of the manufacturer of the device." ;
        skos:inScheme    ble: ;
        skos:related     ble:Read , xsd:string .

ble:WritewithoutResponse
        a                skos:Concept ;
        rdfs:label       "Write without Response" ;
        skos:definition  "A Characteristic Value is writen to a server when the client knows the Characteristic Value Handle and the client does not need an acknowledgment that the write was successfully performed" ;
        skos:inScheme    ble: .

ftmp:TotalEnergyField
        a                skos:Concept ;
        rdfs:label       "Total Energy Field" ;
        skos:definition  "The Total Energy field represents the total expended energy of a user since the training session has started." ;
        skos:inScheme    ble: ;
        skos:related     xsd:short .

blp:IntermediateCuffPressureCompoundValueField
        a                skos:Concept ;
        rdfs:label       "Intermediate Cuff Pressure Compound Value Field" ;
        skos:definition  "This Intermediate Cuff Pressure Compound Value field is composed of three subfields: Current Cuff Pressure and two unused subfields and is included in the Intermediate Cuff Pressure characteristic." ;
        skos:inScheme    ble: ;
        skos:related     xsd:float .

rcp:ReconnectionConfigurationService
        a                skos:Concept ;
        rdfs:label       "Reconnection Configuration Service" ;
        rdfs:seeAlso     <https://www.bluetooth.org/docman/handlers/downloaddoc.ashx?doc_id=435661> ;
        owl:versionInfo  "1.0" ;
        skos:definition  "This GATT-based service enables the control of certain communication parameters of a Bluetooth Low Energy peripheral device." ;
        skos:inScheme    ble: ;
        skos:related     rcp:RCSettings , rcp:RCCP , rcp:RCFeature .

ftmp:InstantaneousPaceField
        a                skos:Concept ;
        rdfs:label       "Instantaneous Pace Field" ;
        skos:definition  "The Instantaneous Pace field represents the instantaneous pace of a user while exercising." ;
        skos:inScheme    ble: ;
        skos:related     xsd:unsignedShort .

glp:HbA1cField  a        skos:Concept ;
        rdfs:label       "Hemoglobin A1c" ;
        skos:definition  "Field exists if the key of bit 6 of the Flags field is set to 1" ;
        skos:inScheme    ble: ;
        skos:related     xsd:float .

ble:UncertaintyValue  a  skos:Concept ;
        rdfs:label       "Uncertainty Value" ;
        skos:definition  "When read, the Server shall return the current value of the Uncertainty Characteristic." ;
        skos:inScheme    ble: ;
        skos:related     xsd:unsignedByte .

idp:TBROver  a           skos:Concept ;
        rdfs:label       "The temporary basal Over" ;
        skos:definition  "The temporary basal rate expired (i.e., the programmed duration is over)." ;
        skos:inScheme    ble: .

rscp:InstantaneousCadenceField
        a                skos:Concept ;
        rdfs:label       "Instantaneous Cadence Field" ;
        skos:definition  "The Instantaneous Cadence represents the number of times per minute a foot fall occurs." ;
        skos:inScheme    ble: ;
        skos:related     xsd:unsignedByte .

cgmp:CGMGlucoseConcentrationField
        a                skos:Concept ;
        rdfs:label       "CGM Glucose Concentration Field" ;
        skos:definition  "The CGM Glucose Concentration field contains the CGM glucose concentration." ;
        skos:inScheme    ble: ;
        skos:related     xsd:float .

idp:ReservoirRemainingAmountfield
        a                skos:Concept ;
        rdfs:label       "Reservoir Remaining Amount field" ;
        skos:definition  "The Reservoir Remaining Amount field represents the remaining amount of insulin in the reservoir in IU." ;
        skos:inScheme    ble: ;
        skos:related     xsd:float .

lehid:ExitSuspend  a     skos:Concept ;
        rdfs:label       "Exit Suspend" ;
        skos:definition  "Informs HID Device that HID Host is exiting the Suspend State" ;
        skos:inScheme    ble: .

htp:HealthThermometerProfile
        a                skos:Concept ;
        rdfs:label       "Health Thermometer Profile" ;
        rdfs:seeAlso     <https://www.bluetooth.org/docman/handlers/downloaddoc.ashx?doc_id=238687> ;
        owl:versionInfo  "1.0" ;
        skos:definition  "This profile enables a Collector device to connect and interact with a Thermometer sensor for use in healthcare applications." ;
        skos:inScheme    ble: ;
        skos:related     ble:DeviceInformationService , htp:HealthThermometerService .

otp:ObjectSize  a        skos:Concept ;
        rdfs:label       "Object Size" ;
        skos:definition  "The Object Size characteristic exposes the current size as well as the allocated size of the Current Object." ;
        skos:inScheme    ble: ;
        skos:related     ble:Read , otp:CurrentSizeField , otp:AllocatedSizeField .

ftmp:MinimumPowerfield
        a                skos:Concept ;
        rdfs:label       "Minimum Power" ;
        skos:definition  "Minimum Watt  with a resolution of 1" ;
        skos:inScheme    ble: ;
        skos:related     xsd:short .

lnp:BearingField  a      skos:Concept ;
        rdfs:label       "Bearing Field" ;
        skos:definition  "The Bearing field represents the direction where the user should be heading to reach the next waypoint or final destination." ;
        skos:inScheme    ble: ;
        skos:related     xsd:unsignedShort .

ftmp:TotalDistanceField
        a                skos:Concept ;
        rdfs:label       "Total Distance Field" ;
        skos:definition  "The Total Distance field represents the total distance reported by the Server since the beginning of the training session." ;
        skos:inScheme    ble: ;
        skos:related     xsd:unsignedInt .

ftmp:MaximumPowerfield
        a                skos:Concept ;
        rdfs:label       "Maximum Power" ;
        skos:definition  "Maximum Watt  with a resolution of 1" ;
        skos:inScheme    ble: ;
        skos:related     xsd:short .

lehid:Report  a          skos:Concept ;
        rdfs:label       "Report" ;
        skos:definition  "The Report characteristic is used to exchange data between a HID Device and a HID Host." ;
        skos:inScheme    ble: ;
        skos:related     ble:Notify , ble:WritewithoutResponse , ble:Read , lehid:ReportValue , ble:Write .

otp:ObjectListFilter  a  skos:Concept ;
        rdfs:label       "Object List Filter" ;
        skos:definition  "If Object List Filter characteristics are exposed, the filter conditions shall determine which objects are included in or excluded from the list of objects. The Object List Filter characteristics can therefore modify the behavior of the Object List Control Point." ;
        skos:inScheme    ble: ;
        skos:related     ble:Read , ble:Write .

idp:BolusCanceled  a     skos:Concept ;
        rdfs:label       "Bolus Canceled" ;
        skos:definition  "A running bolus was canceled (e.g., Insulin Delivery Device changed from run to standby mode)" ;
        skos:inScheme    ble: .

rscp:RunningSpeedandCadenceService
        a                skos:Concept ;
        rdfs:label       "Running Speed and Cadence Service" ;
        rdfs:seeAlso     <https://www.bluetooth.org/docman/handlers/downloaddoc.ashx?doc_id=261265> ;
        owl:versionInfo  "1.0" ;
        skos:definition  "This service exposes speed, cadence and other data from a Running Speed and Cadence sensor intended for fitness applications." ;
        skos:inScheme    ble: ;
        skos:related     ble:SensorLocation , rscp:RSCFeature , rscp:RSCMeasurement , rscp:SCControlPoint .

ble:URI  a               skos:Concept ;
        rdfs:label       "URI" ;
        skos:definition  "The URI characteristic is used to configure the URI for a subsequent request." ;
        skos:inScheme    ble: ;
        skos:related     ble:WriteLong , xsd:string , ble:Write .

lehid:HIDService  a      skos:Concept ;
        rdfs:label       "Human Interface Device Service" ;
        rdfs:seeAlso     <https://www.bluetooth.org/docman/handlers/downloaddoc.ashx?doc_id=245140> ;
        owl:versionInfo  "1.0" ;
        skos:definition  "The HID Service exposes data and associated formatting for HID Devices and HID Hosts. " ;
        skos:inScheme    ble: ;
        skos:related     lehid:ProtocolMode , lehid:HIDControlPoint , lehid:BootMouseInputReport , lehid:HIDInformation , lehid:BootKeyboardOutputReport , lehid:Report , lehid:BootKeyboardInputReport , lehid:ReportMap .

ble:ImmediateAlertService
        a                skos:Concept ;
        rdfs:label       "Immediate Alert Service" ;
        rdfs:seeAlso     <https://www.bluetooth.org/docman/handlers/downloaddoc.ashx?doc_id=239390> ;
        owl:versionInfo  "1.0" ;
        skos:definition  "This service exposes a control point to allow a peer device to cause the device to immediately alert." ;
        skos:inScheme    ble: ;
        skos:related     ble:AlertLevel .

ftmp:FitnessMachineControlPoint
        a                skos:Concept ;
        rdfs:label       "Fitness Machine Control Point" ;
        skos:definition  "The Fitness Machine Control Point characteristic is used to request a specific function to be executed on the Server." ;
        skos:inScheme    ble: ;
        skos:related     ble:Indicate , ble:Write .

cgmp:SessionStartTimeField
        a                skos:Concept ;
        rdfs:label       "Session Start Time Field" ;
        skos:definition  "The Session Start Time Field defines the time of the initial CGM measurement" ;
        skos:inScheme    ble: ;
        skos:related     xsd:unsignedShort .

wsp:WeightMeasurement
        a                skos:Concept ;
        rdfs:label       "Weight Measurement" ;
        skos:definition  "The Weight Measurement characteristic is used to send weight-related data to the Client." ;
        skos:inScheme    ble: ;
        skos:related     wsp:UserIDField , wsp:BIM , wsp:TimeStampField , wsp:HeightField , wsp:WeightField , ble:Indicate .

hrp:HeartRateControlPoint
        a                skos:Concept ;
        rdfs:label       "Heart Rate Control Point" ;
        skos:definition  "The Heart Rate Control Point characteristic is used to enable a Client to write control points to a Server to control behavior." ;
        skos:inScheme    ble: ;
        skos:related     ble:Write .

cscp:LastWheelEventTime
        a                skos:Concept ;
        rdfs:label       "Last Wheel Event Time Fields" ;
        skos:definition  "The Cumulative Wheel Revolutions value and the Last Wheel Event Time value allow the Client to calculate the speed (instantaneous and average) as well as the distance travelled." ;
        skos:inScheme    ble: ;
        skos:related     xsd:unsignedShort .

idp:AuxInfo3LowerBoundfield
        a                skos:Concept ;
        rdfs:label       "AuxInfo3 Lower Bound field" ;
        skos:definition  "The AuxInfo3 field shall contain the value of the lower bound of the temperature." ;
        skos:inScheme    ble: ;
        skos:related     xsd:float .

ftmp:StairClimberData
        a                skos:Concept ;
        rdfs:label       "Stair Climber Data" ;
        skos:definition  "The Stair Climber Data characteristic is used to send training-related data to the Client from a stair climber (Server)." ;
        skos:inScheme    ble: ;
        skos:related     ftmp:EnergyperMinuteField , ftmp:StepperMinuteRateField , ftmp:HeartRateField , ftmp:PositiveElevationGainField , ftmp:RemainingTimeField , ble:Notify , ftmp:ElapsedTimeField , ftmp:StrideCountField , ftmp:TotalEnergyField , ftmp:AverageStepRateField , ftmp:FloorsField , ftmp:EnergyperHourField , ftmp:MetabolicEquivalentField .

wsp:HeightField  a       skos:Concept ;
        rdfs:label       "Height Field" ;
        skos:definition  "The Height field may be included in the Body Composition Measurement characteristic if the device supports the Height feature." ;
        skos:inScheme    ble: ;
        skos:related     xsd:unsignedShort .

idp:AuxInfo2Contextfield
        a                skos:Concept ;
        rdfs:label       "AuxInfo2 Context values" ;
        skos:definition  "The second octet of the AuxInfo2 field shall contain a Context field." ;
        skos:inScheme    ble: ;
        skos:narrower    idp:GenericDevice , idp:Insulin ;
        skos:related     xsd:unsignedByte .

otp:ObjectLastModified
        a                skos:Concept ;
        rdfs:label       "Object Last Modified" ;
        skos:definition  "The Object Last-Modified characteristic exposes a value representing a date and time when the object content was last modified." ;
        skos:inScheme    ble: ;
        skos:related     ble:Read , otp:ObjectLastModifiedField , ble:Write .

hrp:HeartRateMeasurement
        a                skos:Concept ;
        rdfs:label       "Heart Rate Measurement" ;
        skos:definition  "The Heart Rate Measurement characteristic is used to send a heart rate measurement." ;
        skos:inScheme    ble: ;
        skos:related     hrp:RRIntervalField , ble:Notify , hrp:EnergyExpendedField , hrp:HeartRateValueField .

glp:MedicationIDField
        a                skos:Concept ;
        rdfs:label       "Medication ID" ;
        skos:definition  "Field exists if the key of bit 4 of the Flags field is set to 1" ;
        skos:inScheme    ble: ;
        skos:related     xsd:unsignedByte .

htp:IntermediateTemperatureValueField
        a                skos:Concept ;
        rdfs:label       "Intermediate Temperature Value Field" ;
        skos:definition  "This Intermediate Temperature Value field shall be included in the Intermediate Temperature characteristic." ;
        skos:inScheme    ble: ;
        skos:related     htp:TimeStampField , xsd:float .

idp:PrimingIssue  a      skos:Concept ;
        rdfs:label       "Priming Issue" ;
        skos:definition  "There is a priming issue after replacement of reservoir and/or infusion set" ;
        skos:inScheme    ble: .

lnp:TimetoFirstFixField
        a                skos:Concept ;
        rdfs:label       "Time to First Fix Field" ;
        skos:definition  "The Time to First Fix field represents the time used to receive data and calculate the initial position after the device was switched on." ;
        skos:inScheme    ble: ;
        skos:related     xsd:unsignedShort .

lnp:ElevationField  a    skos:Concept ;
        rdfs:label       "Elevation Field" ;
        skos:definition  "The Elevation field represents the value of the elevation measured by the sensor." ;
        skos:inScheme    ble: ;
        skos:related     xsd:integer .

ble:InstantaneousPowerField
        a                skos:Concept ;
        rdfs:label       "Instantaneous Power Field" ;
        skos:definition  "The Instantaneous Power field represents the value of the instantaneous power measured by the Server." ;
        skos:inScheme    ble: ;
        skos:related     xsd:short .

lehid:BootMouseInputReportValue
        a                skos:Concept ;
        rdfs:label       "Boot Mouse Input Report Value" ;
        skos:definition  "The Boot Mouse Input Report characteristic value is an array of octets whose meaning is defined in the USB HID Usage." ;
        skos:inScheme    ble: ;
        skos:related     xsd:unsignedByte .

cpp:BottomDeadSpotAngleField
        a                skos:Concept ;
        rdfs:label       "Bottom Dead Spot Angle Field" ;
        skos:definition  "The Bottom Dead Spot Angle field represents the crank angle when the value of the Instantaneous Power value becomes negative." ;
        skos:inScheme    ble: ;
        skos:related     xsd:unsignedShort .

plxp:SpO2PRFastfield  a  skos:Concept ;
        rdfs:label       "Percent oxygen saturation of hemoglobin and Pulse Rate(SpO2PR)-Fast Field" ;
        skos:definition  "The SpO2PR-Fast field reports fast responding oximetry measurements of the sensor." ;
        skos:inScheme    ble: ;
        skos:related     xsd:float .

ble:IndoorPositioningConfiguration
        a                skos:Concept ;
        rdfs:label       "Indoor Positioning Configuration" ;
        skos:definition  "The Indoor Positioning Configuration Characteristic describes the advertise information data embedded in the Indoor Positioning Service AD type." ;
        skos:inScheme    ble: ;
        skos:related     ble:IndoorPositioningValue , ble:WritewithoutResponse , ble:Read , ble:ReliableWrite , ble:Write .

cpp:MinimumForceMagnitude
        a                skos:Concept ;
        rdfs:label       "Minimum Force Magnitude" ;
        skos:definition  "The Minimum Force Magnitude field represents the minimum force value measured in a single crank revolution." ;
        skos:inScheme    ble: ;
        skos:related     xsd:short .

cgmp:E2ECRCField  a      skos:Concept ;
        rdfs:label       "End-to-End Cyclic Redundancy Check Field" ;
        skos:definition  "If the device supports E2E-safety (E2E-CRC Supported bit is set in CGM Features), the measurement shall be protected by a CRC calculated over all field." ;
        skos:inScheme    ble: ;
        skos:related     xsd:unsignedShort .

idp:BatteryFull  a       skos:Concept ;
        rdfs:label       "Battery Full" ;
        skos:definition  "The Insulin Delivery Device has a full operational runtime" ;
        skos:inScheme    ble: .

idp:IDDHistoryData  a    skos:Concept ;
        rdfs:label       "Insulin Delivery Device History Data" ;
        skos:definition  "The IDD History Data characteristic is comprised of response records from executed procedures of the IDD Record Access Control Point." ;
        skos:inScheme    ble: ;
        skos:related     ble:Notify , idp:RelativeOffsetfield , idp:SequenceNumberfield , idp:EventData .

idp:OcclusionDetected
        a                skos:Concept ;
        rdfs:label       "Occlusion Detected" ;
        skos:definition  "An occlusion occurred (e.g., clogging of infusion set)." ;
        skos:inScheme    ble: .

cpp:LastWheelEventTime
        a                skos:Concept ;
        rdfs:label       "Wheel Revolution Data - Last Wheel Event Time" ;
        skos:definition  "Last Wheel Event Time is one value of The Wheel Revolution Data field pair, always goes in pair with Cumulative Wheel Revolutions field." ;
        skos:inScheme    ble: .

blp:PulseRateField  a    skos:Concept ;
        rdfs:label       "Pulse Rate Field" ;
        skos:definition  "The Pulse Rate field may be included in the Blood Pressure Measurement characteristic if the device supports pulse rate measurements." ;
        skos:inScheme    ble: ;
        skos:related     xsd:float .

idp:BolusExtendedAmountfield
        a                skos:Concept ;
        rdfs:label       "Bolus Extended Amount field" ;
        skos:definition  "The Bolus Extended Amount field represents the extended amount of the bolus." ;
        skos:inScheme    ble: ;
        skos:related     xsd:float .

ble:Longitude  a         skos:Concept ;
        rdfs:label       "Longitude" ;
        skos:definition  "The Longitude Characteristic describes the global WGS84 East coordinate of the device." ;
        skos:inScheme    ble: ;
        skos:related     ble:WritewithoutResponse , ble:Read , ble:ReliableWrite , ble:LongitudeValue , ble:Write .

blp:BloodPressureService
        a                skos:Concept ;
        rdfs:label       "Blood Pressure Service." ;
        rdfs:seeAlso     <https://www.bluetooth.org/docman/handlers/downloaddoc.ashx?doc_id=243126> ;
        owl:versionInfo  "1.0" ;
        skos:definition  "The Blood Pressure Service exposes blood pressure and other data related to a non-invasive blood pressure monitor for consumer and professional healthcare applications." ;
        skos:inScheme    ble: ;
        skos:related     blp:BloodPressureFeature , blp:IntermediateCuffPressure , blp:BloodPressureMeasurement .

plxp:PLXContinuousMeasurement
        a                skos:Concept ;
        rdfs:label       "Pulse Oximeter Continuous Measurement" ;
        skos:definition  "The PLX Continuous Measurement characteristic, if supported, shall be used to send periodic pulse oximetry measurements." ;
        skos:inScheme    ble: ;
        skos:related     ble:Notify , plxp:PulseAmplitudeIndex , plxp:SpO2PRNormalfield , plxp:SpO2PRSlowfield , plxp:SpO2PRFastfield .

plxp:SpO2PRSpotCheckField
        a                skos:Concept ;
        rdfs:label       "Percent oxygen saturation of hemoglobin and Pulse Rate Spot Check" ;
        skos:definition  "The SpO2PR-Spot-Check field shall be included in the PLX Spot-check Measurement characteristic." ;
        skos:inScheme    ble: ;
        skos:related     xsd:float .

plxp:SpO2PRSlowfield  a  skos:Concept ;
        rdfs:label       "Percent oxygen saturation of hemoglobin and Pulse Rate(SpO2PR)-Slow Field" ;
        skos:definition  "The SpO2PR-Slow field reports slow responding oximetry measurements of the sensor." ;
        skos:inScheme    ble: ;
        skos:related     xsd:float .

anp:SupportedNewAlertCategory
        a                skos:Concept ;
        rdfs:label       "Supported New Alert Category" ;
        skos:definition  "A bit map showing which categories of new alert are supported and which are not." ;
        skos:inScheme    ble: ;
        skos:related     ble:Read .

lehid:bcdHID  a          skos:Concept ;
        rdfs:label       "Version number of base USB HID Specification" ;
        skos:definition  "16-bit unsigned integer representing version number of base USB HID Specification implemented by HID Device." ;
        skos:inScheme    ble: ;
        skos:related     xsd:unsignedShort .

cpp:InstantaneousForceMagnitudeArrayField
        a                skos:Concept ;
        rdfs:label       "Instantaneous Force Magnitude Array Field" ;
        skos:definition  "Included in this field are one or more Instantaneous Magnitude values which are expressed in Newtons with a resolution of 1 Newton" ;
        skos:inScheme    ble: ;
        skos:related     xsd:short .

wsp:BodyCompositionService
        a                skos:Concept ;
        rdfs:label       "Body Composition Service" ;
        rdfs:seeAlso     <https://www.bluetooth.org/docman/handlers/downloaddoc.ashx?doc_id=293523> ;
        owl:versionInfo  "1.0" ;
        skos:definition  "This service exposes data related to body composition from a body composition analyzer intended for consumer healthcare and sports/fitness applications." ;
        skos:inScheme    ble: ;
        skos:related     wsp:BodyCompositionFeature , wsp:BodyCompositionMeasurement .

ftmp:TreadmillData  a    skos:Concept ;
        rdfs:label       "Treadmill Data" ;
        skos:definition  "The Treadmill Data characteristic is used to send training-related data to the Client from a treadmill (Server)." ;
        skos:inScheme    ble: ;
        skos:related     ftmp:InclinationField , ftmp:TotalEnergyField , ftmp:InstantaneousPaceField , ftmp:RemainingTimeField , ftmp:PositiveElevationGainField , ftmp:EnergyperHourField , ftmp:AverageSpeedField , ftmp:MetabolicEquivalentField , ftmp:PowerOutputField , ftmp:AveragePaceField , ftmp:TotalDistanceField , ble:Notify , ble:InstantaneousSpeedField , ftmp:ForceonBeltField , ftmp:ElapsedTimeField , ftmp:NegativeElevationGainField , ftmp:EnergyperMinuteField , ftmp:RampAngleSettingField , ftmp:HeartRateField .

ftmp:AverageStrokeRateField
        a                skos:Concept ;
        rdfs:label       "Average Stroke Rate Field" ;
        skos:definition  "The Average Stroke Rate field represents the average speed since the beginning of the training session." ;
        skos:inScheme    ble: ;
        skos:related     xsd:unsignedByte .

idp:ReservoirIssue  a    skos:Concept ;
        rdfs:label       "Reservoir Issue" ;
        skos:definition  "An error related to the replacement or functioning of the reservoir occurred." ;
        skos:inScheme    ble: .

ftmp:PreWorkout  a       skos:Concept ;
        rdfs:label       "Pre-Workout" ;
        skos:definition  "0x0E - Pre-Workout" ;
        skos:inScheme    ble: .

cgmp:ContinuousGlucoseMonitoringProfile
        a                skos:Concept ;
        rdfs:label       "Continuous Glucose Monitoring Profile" ;
        rdfs:seeAlso     <https://www.bluetooth.org/docman/handlers/downloaddoc.ashx?doc_id=310501> ;
        owl:versionInfo  "1.0.1" ;
        skos:definition  "The cgmp Profile is used to enable a device to obtain glucose measurement and other data from a cgmp Sensor that exposes the cgmp Service." ;
        skos:inScheme    ble: ;
        skos:related     cgmp:cgmpService , ble:BondManagementService , ble:DeviceInformationService .

lehid:HIDInformation  a  skos:Concept ;
        rdfs:label       "HID Information" ;
        skos:definition  "The HID Information characteristic is used to hold a set of values known as the HID Device’s HID Attributes." ;
        skos:inScheme    ble: ;
        skos:related     ble:Read , lehid:bcdHID , lehid:bCountryCode .

blp:BloodPressureFeature
        a                skos:Concept ;
        rdfs:label       "Blood Pressure Feature" ;
        skos:definition  "The Blood Pressure Feature characteristic shall be used to describe the supported features of the Blood Pressure Sensor." ;
        skos:inScheme    ble: ;
        skos:related     ble:Read .

ftmp:FitnessMachineStatus
        a                skos:Concept ;
        rdfs:label       "Fitness Machine Status" ;
        skos:definition  "The Fitness Machine Status characteristic is used to send the status of the Server." ;
        skos:inScheme    ble: ;
        skos:related     ble:Notify .

ble:AltitudeValue  a     skos:Concept ;
        rdfs:label       "Altitude Value" ;
        skos:definition  "When read, the Server shall return the current value of the Altitude Characteristic." ;
        skos:inScheme    ble: ;
        skos:related     xsd:unsignedShort .

ble:Altitude  a          skos:Concept ;
        rdfs:label       "Altitude" ;
        skos:definition  "The Altitude Characteristic describes the altitude of the device above the WGS84 datum." ;
        skos:inScheme    ble: ;
        skos:related     ble:WritewithoutResponse , ble:Read , ble:ReliableWrite , ble:AltitudeValue , ble:Write .

anp:NewAlert  a          skos:Concept ;
        rdfs:label       "New Alert" ;
        skos:definition  "The count of new alerts (for a given category) in the server" ;
        skos:inScheme    ble: ;
        skos:related     ble:Notify , anp:NumberofNewAlert , anp:TextStringInformation , anp:CategoryID .

rcp:RCCP  a              skos:Concept ;
        rdfs:label       "Reconnection Configuration Control Point" ;
        skos:definition  "The Reconnection Configuration Control Point (RCCP) characteristic shall be used to execute a supported procedure on the Reconnection Configuration server." ;
        skos:inScheme    ble: ;
        skos:related     ble:Indicate , ble:Write .

aiop:Digital  a          skos:Concept ;
        rdfs:label       "Digital characteristic" ;
        skos:definition  "The Digital characteristic is used to expose and change the state of an IOM’s digital signals." ;
        skos:inScheme    ble: ;
        skos:related     xsd:unsignedByte , ble:Indicate , ble:WritewithoutResponse , ble:Write , ble:Read , ble:Notify .

ble:Read  a              skos:Concept ;
        rdfs:label       "Read" ;
        skos:definition  "A Characteristic Value is read from a server when the client knows the Characteristic Value Handle" ;
        skos:inScheme    ble: .

rscp:SCControlpoint  a   skos:Concept ;
        rdfs:label       "Speed and Cadance Control Point" ;
        skos:definition  "If the SC Control Point is supported, profiles utilizing this service are required to ensure that the Client configures the SC Control Point characteristic for indications (i.e. via the Client Characteristic Configuration descriptor) at the first connection." ;
        skos:inScheme    ble: .

idp:InsulinDeliveryProfile
        a                   skos:Concept ;
        rdfs:label          "Insulin Delivery Profile" ;
        owl:versionInfo     "1.0" ;
        skos:editorialNote  "Not found yet, require membership ro get access." ;
        skos:inScheme       ble: ;
        skos:related        idp:InsulinDeliveryService .

wsp:BodyCompositionFeature
        a                skos:Concept ;
        rdfs:label       "Body Composition Feature" ;
        skos:definition  "The Body Composition Feature characteristic shall be used to describe the supported features of the Server." ;
        skos:inScheme    ble: ;
        skos:related     ble:Read .

ble:SystemID  a          skos:Concept ;
        rdfs:label       "System ID" ;
        skos:definition  "The System ID characteristic shall represent a structure containing an Organizationally Unique Identifier (OUI) followed by a manufacturer-defined identifier and is unique for each individual instance of the product" ;
        skos:inScheme    ble: ;
        skos:related     ble:Read , ble:OrganizationallyUniqueIdentifier , ble:ManufacturerIdentifier .

lnp:LNFeature  a         skos:Concept ;
        rdfs:label       "Location and Navigation Feature" ;
        skos:definition  "The LN Feature characteristic shall be used to describe the supported features of the Server." ;
        skos:inScheme    ble: ;
        skos:related     ble:Read .

lnp:HeadingField  a      skos:Concept ;
        rdfs:label       "Heading Field" ;
        skos:definition  "The Heading field represents the direction the user is heading." ;
        skos:inScheme    ble: ;
        skos:related     xsd:unsignedShort .

idp:BatteryEmpty  a      skos:Concept ;
        rdfs:label       "Battery Empty" ;
        skos:definition  "The Insulin Delivery Device has no operational runtime left" ;
        skos:inScheme    ble: .

ftmp:AverageStepRateField
        a                skos:Concept ;
        rdfs:label       "Average Step Rate Field" ;
        skos:definition  "The Average Step Rate field represents the average step rate since the beginning of the training session." ;
        skos:inScheme    ble: ;
        skos:related     xsd:unsignedShort .

glp:GlucoseService  a    skos:Concept ;
        rdfs:label       "Glucose Service" ;
        rdfs:seeAlso     <https://www.bluetooth.org/docman/handlers/downloaddoc.ashx?doc_id=248026> ;
        owl:versionInfo  "1.0" ;
        skos:definition  "The Glucose Service exposes glucose and other data related to a personal glucose sensor for consumer healthcare applications and is not designed for clinical use." ;
        skos:inScheme    ble: ;
        skos:related     glp:GlucoseMeasurementContext , glp:GlucoseFeature , ble:RecordAccessControlPoint , glp:GlucoseMeasurement .

ble:UserControlPoint  a  skos:Concept ;
        rdfs:label       "User Control Point" ;
        skos:definition  "The User Control Point characteristic is used to request a specific function to be executed on the receiving device." ;
        skos:inScheme    ble: ;
        skos:related     ble:Indicate , ble:Write .

ftmp:MinimumInclinationIncrementfield
        a                skos:Concept ;
        rdfs:label       "Minimum Inclination Increment" ;
        skos:definition  "Minimum Percent with a resolution of 0.1" ;
        skos:inScheme    ble: ;
        skos:related     xsd:unsignedShort .

idp:Waiting  a           skos:Concept ;
        rdfs:label       "Waiting" ;
        skos:definition  "The Insulin Delivery Device waits for an interaction" ;
        skos:inScheme    ble: .

cpp:FirstCrankMeasurementAngleField
        a                skos:Concept ;
        rdfs:label       "First Crank Measurement Angle Field" ;
        skos:definition  "This represents the angle of the first sample at the start of a measurement and is used by the Client in conjunction with the Instantaneous Magnitude values and the Sampling Rate to assemble a force (or torque) vector array to show a user the forces throughout a crank rotation" ;
        skos:inScheme    ble: ;
        skos:related     xsd:unsignedShort .

ble:LastCrankEventTime
        a                skos:Concept ;
        rdfs:label       "Last Crank Event Time" ;
        skos:definition  "The Last Crank Event Time is one value of Crank Revolution Data pair and always presents as a pair with Cumulative Crank Revolutions." ;
        skos:inScheme    ble: ;
        skos:related     xsd:unsignedShort .

lehid:bCountryCode  a    skos:Concept ;
        rdfs:label       "Country Code" ;
        skos:definition  "8-bit integer identifying country HID Device hardware is localized for." ;
        skos:inScheme    ble: ;
        skos:related     xsd:unsignedByte .

wsp:BodyFatPercentageField
        a                skos:Concept ;
        rdfs:label       "Body Fat Percentage Field" ;
        skos:definition  "The Body Fat Percentage field shall be included in the Body Composition Measurement characteristic." ;
        skos:inScheme    ble: ;
        skos:related     xsd:unsignedShort .

plxp:SpO2PRNormalfield
        a                skos:Concept ;
        rdfs:label       "Percent oxygen saturation of hemoglobin and Pulse Rate (SpO2PR)-Normal Field" ;
        skos:definition  "The SpO2PR-Normal field shall be included in the PLX Continuous Measurement characteristic." ;
        skos:inScheme    ble: ;
        skos:related     xsd:float .

idp:PowerSourceInsufficient
        a                skos:Concept ;
        rdfs:label       "Power Source Insufficient" ;
        skos:definition  "The Insulin Delivery Device has insufficient power to charge the device" ;
        skos:inScheme    ble: .

ble:SCControlPoint  a    skos:Concept ;
        rdfs:label       "Speed and Cadence Control Point" ;
        skos:definition  "The SC Control Point is used by a Client to control certain behaviors of the Server." ;
        skos:inScheme    ble: .

cpp:MaximumForceMagnitude
        a                skos:Concept ;
        rdfs:label       "Maximum Force Magnitude" ;
        skos:definition  "The Maximum Force Magnitude field represents the maximum force value measured in a single crank revolution." ;
        skos:inScheme    ble: ;
        skos:related     xsd:short .

ble:HTTPEntityBody  a    skos:Concept ;
        rdfs:label       "HTTP Entity Body" ;
        skos:definition  "The HTTP Entity Body characteristic contains the contents of the message-body after any Transfer-Encoding has been applied." ;
        skos:inScheme    ble: ;
        skos:related     ble:Read , ble:WriteLong , xsd:string , ble:ReadLong , ble:Write .

idp:AnnunciationType  a  skos:Concept ;
        rdfs:label       "Annunciation Type" ;
        skos:definition  "This Annunciation Type field describes the kind of annunciation in the scope of the Server application" ;
        skos:inScheme    ble: ;
        skos:narrower    idp:ReservoirIssue , idp:BatteryLow , idp:MechanicalIssue , idp:ReservoirLow , idp:InfusionSetIncomplete , idp:PrimingIssue , idp:MaxDelivery , idp:BolusCanceled , idp:ManufacturerReserved , idp:DateTimeIssue , idp:SystemIssue , idp:OcclusionDetected , idp:TBRCanceled , idp:Airpressureoutofrange , idp:TBROver , idp:Temperatureoutofrange , idp:BatteryFull , idp:ReservoirEmpty , idp:BatteryMedium , idp:Temperature , idp:BatteryEmpty , idp:PowerSourceInsufficient , idp:InfusionSetDetached ;
        skos:related     xsd:unsignedShort .

ble:TransportDiscoveryService
        a                skos:Concept ;
        rdfs:label       "Transport Discovery Service" ;
        rdfs:seeAlso     <https://www.bluetooth.org/docman/handlers/downloaddoc.ashx?doc_id=309929> ;
        owl:versionInfo  "1.0" ;
        skos:definition  "This service enables a device using Bluetooth low energy wireless technology to expose services that are available on a transport other than Bluetooth low energy." ;
        skos:inScheme    ble: ;
        skos:related     ble:TransportDataField , ble:TransportDataLengthField , ble:TDSControlPoint , ble:OrganizationIDField .

glp:GlucoseFeature  a    skos:Concept ;
        rdfs:label       "Glucose Feature" ;
        skos:definition  "The Glucose Feature characteristic shall be used to describe the supported features of the Server." ;
        skos:inScheme    ble: .

scpp:ScanParametersProfile
        a                skos:Concept ;
        rdfs:label       "Scan Parameters Profile" ;
        rdfs:seeAlso     <https://www.bluetooth.org/docman/handlers/downloaddoc.ashx?doc_id=245142> ;
        owl:versionInfo  "1.0" ;
        skos:definition  "This profile defines how a Scan Client device with Bluetooth low energy wireless communications can write its scanning behavior to a Scan Server, and how a Scan Server can request updates of a Scan Client scanning behavior." ;
        skos:inScheme    ble: ;
        skos:related     ble:ScanParametersService .

esp:ESTriggerSettingDescriptor
        a                skos:Concept ;
        rdfs:label       "Environmental Sensing Trigger Setting Descriptor" ;
        skos:definition  "Where multiple ES Trigger Setting descriptors are present for a given ESS Characteristic, the ES Trigger Setting descriptor and the ES Configuration descriptor work together to define the conditions under which the associated ESS Characteristic value can be notified" ;
        skos:inScheme    ble: ;
        skos:related     ble:Read , ble:Write .

idp:IDDStatus  a         skos:Concept ;
        rdfs:label       "Insulin Delivery Device Status" ;
        skos:definition  "The IDD Status characteristic is comprised of status values of the Insulin Delivery Device and the insulin therapy." ;
        skos:inScheme    ble: ;
        skos:related     idp:E2ECounterfield , idp:ReservoirRemainingAmountfield , idp:TherapyControlStatefield , idp:OperationalStatefield , ble:Read , ble:Indicate , idp:E2ECRCfield .

idp:Pending  a           skos:Concept ;
        rdfs:label       "Pending" ;
        skos:definition  "The annunciation is currently pending and requires a user action for snoozing or confirmation" ;
        skos:inScheme    ble: .

ftmp:InstantaneousCadenceField
        a                skos:Concept ;
        rdfs:label       "Instantaneous Cadence Field" ;
        skos:definition  "The Instantaneous Cadence field represents the instantaneous cadence of the user." ;
        skos:inScheme    ble: ;
        skos:related     xsd:unsignedShort .

ble:Latitude  a          skos:Concept ;
        rdfs:label       "Latitude" ;
        skos:definition  "The Latitude Characteristic describes the global WGS84 North coordinate of the device." ;
        skos:inScheme    ble: ;
        skos:related     ble:WritewithoutResponse , ble:Read , ble:LatitudeValue , ble:ReliableWrite , ble:Write .

cpp:MinimumTorqueMagnitude
        a                skos:Concept ;
        rdfs:label       "Minimum Torque Magnitude" ;
        skos:definition  "The Minimum Torque Magnitude field represents the minimum torque value measured in a single crank revolution." ;
        skos:inScheme    ble: ;
        skos:related     xsd:short .

ftmp:PositiveElevationGainField
        a                skos:Concept ;
        rdfs:label       "Positive Elevation Gain Field" ;
        skos:definition  "The Positive Elevation Gain field represents the positive elevation gain since the beginning of the training session." ;
        skos:inScheme    ble: ;
        skos:related     xsd:unsignedShort .

cpp:CyclingPowerVector
        a                skos:Concept ;
        rdfs:label       "Cycling Power Vector" ;
        skos:definition  "The Cycling Power Vector characteristic is used to send raw data (either force or torque)." ;
        skos:inScheme    ble: ;
        skos:related     ble:LastCrankEventTime , ble:Notify , cpp:InstantaneousForceMagnitudeArrayField , cpp:InstantaneousTorqueMagnitudeArrayField , cpp:FirstCrankMeasurementAngleField , ble:CumulativeCrankRevolutions .

idp:InfusionSetIncomplete
        a                skos:Concept ;
        rdfs:label       "Infusion Set Incomplete" ;
        skos:definition  "The physical connection between infusion set (including tubing and/or cannula) and the Insulin Delivery Device is incomplete." ;
        skos:inScheme    ble: .

wsp:BasalMetabolismField
        a                skos:Concept ;
        rdfs:label       "Basal Metabolism Field" ;
        skos:definition  "The User ID field shall be included in the Body Composition Measurement characteristic if the device supports the Multiple Users feature" ;
        skos:inScheme    ble: ;
        skos:related     xsd:unsignedShort .

otp:ObjectProperties  a  skos:Concept ;
        rdfs:label       "Object Properties" ;
        skos:definition  "This characteristic exposes a bit field representing the properties of the Current Object." ;
        skos:inScheme    ble: ;
        skos:related     ble:Read , ble:Write .

cscp:CSCMeasurement  a   skos:Concept ;
        rdfs:label       "Cycling Speed and Cadence Measurement" ;
        skos:definition  "The CSC Measurement characteristic is used to send speed-related data and/or cadence-related data." ;
        skos:inScheme    ble: ;
        skos:related     ble:Notify , cscp:CumulativeWheelRevolutions , ble:LastCrankEventTime , cscp:LastWheelEventTime , ble:CumulativeCrankRevolutions .

otp:ObjectFirstCreated
        a                skos:Concept ;
        rdfs:label       "Object First Created" ;
        skos:definition  "The Object First-Created characteristic exposes a value representing a date and time when the object contents were first created." ;
        skos:inScheme    ble: ;
        skos:related     ble:Read , otp:ObjectFirstCreatedField , ble:Write .

ble:CumulativeCrankRevolutions
        a                skos:Concept ;
        rdfs:label       "Cumulative Crank Revolutions" ;
        skos:definition  "The Cumulative Crank Revolutions value represents the number of times a crank rotates and is one value of Crank Revolution Data pair." ;
        skos:inScheme    ble: ;
        skos:related     xsd:unsignedShort .

cpp:PedalPowerBalanceField
        a                skos:Concept ;
        rdfs:label       "Pedal Power Balance Field" ;
        skos:definition  "The Pedal Power Balance field represents the ratio between the total amount of power measured by the sensor and a reference." ;
        skos:inScheme    ble: ;
        skos:related     xsd:unsignedByte .

pasp:PhoneAlertStatusProfile
        a                skos:Concept ;
        rdfs:label       "Phone Alert Status Profile" ;
        rdfs:seeAlso     <https://www.bluetooth.org/docman/handlers/downloaddoc.ashx?doc_id=241861> ;
        owl:versionInfo  "1.0" ;
        skos:definition  "This profile enables a PUID device to alert its user about the alert status of a phone connected to the PUID device." ;
        skos:inScheme    ble: ;
        skos:related     pasp:PhoneAlertStatusService .

ftmp:StrokeCountField
        a                skos:Concept ;
        rdfs:label       "Stroke Count Field" ;
        skos:definition  "The Stroke Count field represents the total number of strokes since the beginning of the training session." ;
        skos:inScheme    ble: ;
        skos:related     xsd:unsignedShort .

cpp:CyclingPowerMeasurement
        a                skos:Concept ;
        rdfs:label       "Cycling Power Measurement" ;
        skos:definition  "The Cycling Power Measurement characteristic is used to send power-related data, speedrelated data, and/or cadence-related data." ;
        skos:inScheme    ble: ;
        skos:related     ble:CumulativeCrankRevolutions , cpp:MinimumForceMagnitude , cpp:MaximumAngle , cpp:AccumulatedTorqueField , cpp:AccumulatedEnergyField , cpp:MaximumForceMagnitude , cpp:CumulativeWheelRevolutions , cpp:BottomDeadSpotAngleField , cpp:ExtremeTorqueMagnitudesFieldPair , cpp:TopDeadSpotAngleField , cpp:LastWheelEventTime , ble:LastCrankEventTime , cpp:MinimumTorqueMagnitude , ble:InstantaneousPowerField , cpp:PedalPowerBalanceField , ble:Notify , cpp:MinimumAngle .

idp:Insulin  a           skos:Concept ;
        rdfs:label       "Insulin" ;
        skos:definition  "The reported temperature refers to the insulin delivered by the Insulin Delivery Device in general (e.g. the insulin in the reservoir)." ;
        skos:inScheme    ble: .

idp:AnnunciationInstanceID
        a                skos:Concept ;
        rdfs:label       "Annunciation Instance ID " ;
        skos:definition  "The Annunciation Instance ID field represents a unique identifier as a uint16 data type created by the Server application for all annunciations that occur in the course of time." ;
        skos:inScheme    ble: ;
        skos:related     xsd:unsignedShort .

ftmp:RampAngleSettingField
        a                skos:Concept ;
        rdfs:label       "Ramp Angle Setting Field" ;
        skos:definition  "The Ramp Angle Setting field represents the current setting of the ramp angle of the Server." ;
        skos:inScheme    ble: ;
        skos:related     xsd:short .

ble:BatteryLevel  a      skos:Concept ;
        rdfs:label       "Battery Level" ;
        skos:definition  "The Battery Level characteristic is read using the GATT Read Characteristic Value subprocedure and returns the current battery level as a percentage." ;
        skos:inScheme    ble: ;
        skos:related     ble:Notify , ble:Read , xsd:unsignedByte .

cgmp:CGMTrendInformationField
        a                skos:Concept ;
        rdfs:label       "Continuous Glucose Monitoring Trend Information Field" ;
        skos:definition  "This field contains the CGM Trend information in (mg/dL)/min as an SFLOAT data type" ;
        skos:inScheme    ble: ;
        skos:related     xsd:float .

pasp:RingerControlPoint
        a                   skos:Concept ;
        rdfs:label          "Ringer Control Point" ;
        skos:editorialNote  "Not found yet" ;
        skos:inScheme       ble: ;
        skos:related        ble:WritewithoutResponse , xsd:unsignedByte .

cpp:CyclingPowerProfile
        a                skos:Concept ;
        rdfs:label       "Cycling Power Profile" ;
        rdfs:seeAlso     <https://www.bluetooth.org/DocMan/handlers/DownloadDoc.ashx?doc_id=412769> ;
        owl:versionInfo  "1.1" ;
        skos:definition  "The Cycling Power Profile is used to enable a data collection device to obtain data from a Cycling Power Sensor (CP Sensor) that exposes the Cycling Power Service." ;
        skos:inScheme    ble: ;
        skos:related     cpp:CyclingPowerService , ble:DeviceInformationService , ble:BatteryService .

ble:ScanIntervalWindow
        a                skos:Concept ;
        rdfs:label       "Scan Interval Window" ;
        skos:definition  "The Scan Interval Window characteristic is used to store the scan parameters of the Client." ;
        skos:inScheme    ble: ;
        skos:related     ble:LE_Scan_Interval , ble:LE_Scan_Window , ble:WritewithoutResponse .

blp:IntermediateCuffPressure
        a                skos:Concept ;
        rdfs:label       "Intermediate Cuff Pressure" ;
        skos:definition  "The Intermediate Cuff Pressure characteristic may be used to send Current Cuff Pressure values to a device for display purposes while the measurement is in progress" ;
        skos:inScheme    ble: ;
        skos:related     blp:TimeStampField , blp:PulseRateField , ble:Notify , blp:IntermediateCuffPressureCompoundValueField , ble:UserIDField .

hrp:RRIntervalField  a   skos:Concept ;
        rdfs:label       "RR(Rh factor) - Interval field" ;
        skos:definition  "The RR-Interval field may be included in the Heart Rate Measurement characteristic if the device supports RR-Interval measurements." ;
        skos:inScheme    ble: ;
        skos:related     xsd:unsignedShort .

glp:TimeOffsetField  a   skos:Concept ;
        rdfs:label       "Time Offset Field" ;
        skos:definition  "The Time Offset field is used in conjunction with the Base Time field to represent the user-facing date and time at the time of measurement." ;
        skos:inScheme    ble: ;
        skos:related     xsd:short .

otp:ObjectTransferProfile
        a                skos:Concept ;
        rdfs:label       "Object Transfer Profile" ;
        rdfs:seeAlso     <https://www.bluetooth.org/docman/handlers/DownloadDoc.ashx?doc_id=309936> ;
        owl:versionInfo  "1.0" ;
        skos:definition  "The Object Transfer Profile defines fundamental requirements to enable an Object Client to create and delete objects and to execute a variety of actions using the currently selected object such as reading object data from or writing object data to an Object Server that exposes the Object Transfer Service." ;
        skos:inScheme    ble: ;
        skos:related     otp:ObjectTransferService .

lnp:BeaconsNumberSolutionField
        a                skos:Concept ;
        rdfs:label       "Number of Beacons in Solution Field" ;
        skos:definition  "The Number of Beacons in Solution field represents the number of beacons used to calculate the current position." ;
        skos:inScheme    ble: ;
        skos:related     xsd:unsignedByte .

ftmp:WarmingUp  a        skos:Concept ;
        rdfs:label       "Warming Up" ;
        skos:definition  "0x02 - Warming Up" ;
        skos:inScheme    ble: .

ftmp:HighIntensityInterval
        a                skos:Concept ;
        rdfs:label       "High Intensity Interval" ;
        skos:definition  "0x04 - High Intensity Interval" ;
        skos:inScheme    ble: .

rscp:RSCFeature  a       skos:Concept ;
        rdfs:label       "Running Speed and Cadence Feature" ;
        skos:definition  "The RSC Feature characteristic shall be used to describe the supported features of the Server." ;
        skos:inScheme    ble: ;
        skos:related     ble:Read , ble:Write .

lehid:ProtocolMode  a    skos:Concept ;
        rdfs:label       "Protocol Mode" ;
        skos:definition  "The Protocol Mode characteristic is used to expose the current protocol mode of the HID Service with which it is associated, or to set the desired protocol mode of the HID Service." ;
        skos:inScheme    ble: ;
        skos:related     ble:WritewithoutResponse , ble:Read , lehid:ProtocolModeValue .

htp:ValidRangeDescriptor
        a                skos:Concept ;
        rdfs:label       "Valid Range" ;
        skos:definition  "The Valid Range declaration is an optional characteristic descriptor that defines the valid range of values for the Characteristic Value." ;
        skos:inScheme    ble: ;
        skos:related     ble:Read .

ble:AlertLevel  a        skos:Concept ;
        rdfs:label       "Alert Level" ;
        skos:definition  "The Alert Level characteristic is a control point that allows a peer to command this device to alert to a given level." ;
        skos:inScheme    ble: ;
        skos:related     ble:WritewithoutResponse .

ftmp:NegativeElevationGainField
        a                skos:Concept ;
        rdfs:label       "Negative Elevation Gain Field" ;
        skos:definition  "The Negative Elevation Gain field represents the negative elevation gain since the training session has started." ;
        skos:inScheme    ble: ;
        skos:related     xsd:unsignedShort .

ble:HTTPHeaders  a       skos:Concept ;
        rdfs:label       "HTTP Headers" ;
        skos:definition  "The HTTP Headers characteristic is used to hold the headers that would be sent with the HTTP Request or the headers contained within an HTTP response message from the HTTP Server." ;
        skos:inScheme    ble: ;
        skos:related     ble:Read , ble:WriteLong , xsd:string , ble:ReadLong , ble:Write .

otp:ObjectNameField  a   skos:Concept ;
        rdfs:label       "Object Name Field" ;
        skos:definition  "The Object Name characteristic returns its associated value when read." ;
        skos:inScheme    ble: ;
        skos:related     xsd:string .

idp:IDDFeatures  a       skos:Concept ;
        rdfs:label       "Insulin Delivery Device Feature" ;
        skos:definition  "The IDD Features characteristic shall be used to describe the supported features of the Server." ;
        skos:inScheme    ble: ;
        skos:related     idp:E2ECRCfield , idp:E2ECounterfield , ble:Read , idp:InsulinConcentrationfield .

ble:FloorNumberValue  a  skos:Concept ;
        rdfs:label       "Floor Number Value" ;
        skos:definition  "When read, the Server shall return the current value of the Floor Number Characteristic." ;
        skos:inScheme    ble: ;
        skos:related     xsd:unsignedByte .

wsp:MuscleMassField  a   skos:Concept ;
        rdfs:label       "Muscle Mass Field" ;
        skos:definition  "The Muscle Mass field may be included in the Body Composition Measurement characteristic if the device supports the Muscle Mass feature." ;
        skos:inScheme    ble: ;
        skos:related     xsd:unsignedShort .

plxp:PulseOximeterProfile
        a                skos:Concept ;
        rdfs:label       "Pulse Oximeter Profile" ;
        rdfs:seeAlso     <https://www.bluetooth.org/DocMan/handlers/DownloadDoc.ashx?doc_id=304923> ;
        owl:versionInfo  "1.0" ;
        skos:definition  "This Profile Specification defines a Pulse Oximeter (PLX) profile that enables a Collector device to connect and interact with a pulse oximeter intended for healthcare applications." ;
        skos:inScheme    ble: ;
        skos:related     ble:CurrentTimeService , ble:BatteryService , ble:DeviceInformationService , ble:BondManagementService , plxp:PulseOximeterService .

glp:ExerciseIntensityField
        a                skos:Concept ;
        rdfs:label       "xercise Intensity" ;
        skos:definition  "Field exists if the key of bit 3 of the Flags field is set to 1" ;
        skos:inScheme    ble: ;
        skos:related     xsd:unsignedByte .

anp:AlertNotificationControlPoint
        a                skos:Concept ;
        rdfs:label       "Alert Notification Control Point" ;
        skos:definition  "This characteristic allows the client device to enable/disable the alert notification of new alert and unread alert events more selectively than can be done by setting or clearing the notification bit in the Client Characteristic configuration for each alert characteristic." ;
        skos:inScheme    ble: ;
        skos:related     ble:Write .

ble:LatitudeValue  a     skos:Concept ;
        rdfs:label       "The current value of the Latitude Characteristic." ;
        skos:definition  "When read, the Server shall return the current value of the Latitude Characteristic." ;
        skos:inScheme    ble: ;
        skos:related     xsd:integer .

idp:E2ECounterfield  a   skos:Concept ;
        rdfs:label       "End to End Counter field" ;
        skos:definition  "The E2E-Counter field, when used correctly, provides that messages are received in the correct order." ;
        skos:inScheme    ble: ;
        skos:related     xsd:unsignedByte .

hrp:BodySensorLocation
        a                skos:Concept ;
        rdfs:label       "Body Sensor Location" ;
        skos:definition  "The Body Sensor Location characteristic of the device is used to describe the intended location of the heart rate measurement for the device." ;
        skos:inScheme    ble: ;
        skos:related     ble:Read .

lnp:LocationLatitude  a  skos:Concept ;
        rdfs:label       "Location - Latitude" ;
        skos:definition  "The Latitude value represents a geographic coordinate specifying the north-south position of a point on the Earth's surface in WGS-84 format." ;
        skos:inScheme    ble: ;
        skos:related     xsd:integer .

esp:ValidRangeDescriptor
        a                skos:Concept ;
        rdfs:label       "Valid Range Descriptor" ;
        skos:definition  "The Valid Range descriptor is an optional descriptor that allows a Client to read the upper and lower bounds (inclusive) of an associated ESS characteristic value that are supported by the Server" ;
        skos:inScheme    ble: ;
        skos:related     ble:Read .

otp:ObjectFirstCreatedField
        a                skos:Concept ;
        rdfs:label       "Object First-Created Field" ;
        skos:definition  "The Object First-Created characteristic returns its associated value when read. The date and time value shall be represented in Coordinated Universal Time (UTC)." ;
        skos:inScheme    ble: .

idp:Preparing  a         skos:Concept ;
        rdfs:label       "Preparing" ;
        skos:definition  "The Insulin Delivery Device prepares the insulin infusion therapy" ;
        skos:inScheme    ble: .

ftmp:MinimumSpeedfield
        a                skos:Concept ;
        rdfs:label       "Minimum Speed" ;
        skos:definition  "Minimum Kilometer per hour with a resolution of 0.01" ;
        skos:inScheme    ble: ;
        skos:related     xsd:unsignedShort .

ftmp:AverageSpeedField
        a                skos:Concept ;
        rdfs:label       "Average Speed Field" ;
        skos:definition  "The Average Speed field represents the average speed since the beginning of the training session." ;
        skos:inScheme    ble: ;
        skos:related     xsd:unsignedShort .

esp:DescriptorValueChanged
        a                skos:Concept ;
        rdfs:label       "Descriptor Value Changed" ;
        skos:definition  "It enables a Server to alert bonded Clients that the value of one or more ESS-related descriptors for a given ESS Characteristic have changed and need to be re-read" ;
        skos:inScheme    ble: ;
        skos:related     ble:Indicate .

hrp:HeartRateValueField
        a                skos:Concept ;
        rdfs:label       "Heart Rate Measurement Value" ;
        skos:definition  "The Heart Rate Measurement Value field shall be included in the Heart Rate Measurement characteristic." ;
        skos:inScheme    ble: ;
        skos:related     xsd:unsignedShort .

lehid:BootKeyboardOutputReport
        a                skos:Concept ;
        rdfs:label       "Boot Keyboard Output Report" ;
        skos:definition  "The Boot Keyboard Output Report characteristic is used to transfer fixed format and length Output Report data between a HID Host operating in Boot Protocol Mode and a HID Service corresponding to a boot keyboard." ;
        skos:inScheme    ble: ;
        skos:related     ble:WritewithoutResponse , ble:Read , lehid:BootKeyboardOutputReportValue , ble:Write .

idp:ReservoirEmpty  a    skos:Concept ;
        rdfs:label       "Reservoir Empty" ;
        skos:definition  "The reservoir is empty" ;
        skos:inScheme    ble: .

glp:GlucoseConcentrationField
        a                skos:Concept ;
        rdfs:label       "Glucose Concentration Field" ;
        skos:definition  "The Glucose Concentration field is optional, but if it is present, the Type-Sample Location field shall also be present." ;
        skos:inScheme    ble: ;
        skos:related     xsd:float .

ble:IEEE11073-20601RegulatoryCertificationDataList
        a                skos:Concept ;
        rdfs:label       "Institute of Electrical and Electronics Engineers (IEEE) 11073-20601 Regulatory Certification Data List" ;
        skos:definition  "The IEEE 11073-20601 Regulatory Certification Data List characteristic shall represent regulatory and certification information for the product in a list defined in IEEE 11073-20601" ;
        skos:inScheme    ble: ;
        skos:related     ble:Read , xsd:string .

lehid:BootKeyboardInputReportValue
        a                skos:Concept ;
        rdfs:label       "Boot Keyboard Input Report Value" ;
        skos:definition  "The Boot Keyboard Input Report characteristic value is an array of octets whose meaning is defined in the USB HID Usage." ;
        skos:inScheme    ble: ;
        skos:related     xsd:unsignedByte .

lehid:ReportMap  a       skos:Concept ;
        rdfs:label       "Report Map" ;
        skos:definition  "The Report Map characteristic is used to define formatting information for Input Report, Output Report, and Feature Report data transferred between a HID Device and HID Host." ;
        skos:inScheme    ble: ;
        skos:related     ble:Read , lehid:ReportMapValue .

idp:IDDCommandData  a    skos:Concept ;
        rdfs:label       "Insulin Delivery Device Command Data" ;
        skos:definition  "The IDD Command Data characteristic is comprised of response records from executed procedures of the IDD Command Control Point." ;
        skos:inScheme    ble: ;
        skos:related     idp:E2ECRCfield , idp:E2ECounterfield , ble:Indicate , ble:Write .

pxp:Proximityprofile  a  skos:Concept ;
        rdfs:label       "Proximity profile" ;
        rdfs:seeAlso     <https://www.bluetooth.org/DocMan/handlers/DownloadDoc.ashx?doc_id=303199> ;
        owl:versionInfo  "1.0.1" ;
        skos:definition  "The Proximity profile defines the behavior when a device moves away from a peer device so that the connection is dropped or the path loss increases above a preset level, causing an immediate alert." ;
        skos:inScheme    ble: ;
        skos:related     pxp:LinkLossService , pxp:TxPowerService , ble:ImmediateAlertService .

lnp:LNControlPoint  a    skos:Concept ;
        rdfs:label       "Location and Navigation Control Point" ;
        skos:definition  "The LN Control Point is used by a Client to control certain behaviors of the Server." ;
        skos:inScheme    ble: ;
        skos:related     ble:Indicate , xsd:unsignedByte , ble:Write .

glp:ExerciseDurationField
        a                skos:Concept ;
        rdfs:label       "Exercise Duration" ;
        skos:definition  "Field exists if the key of bit 3 of the Flags field is set to 1" ;
        skos:inScheme    ble: ;
        skos:related     xsd:unsignedShort .

htp:TemperatureMeasurementValueField
        a                skos:Concept ;
        rdfs:label       "Temperature Measurement Value Field" ;
        skos:definition  "This Temperature Measurement Value field shall be included in the Temperature Measurement characteristic." ;
        skos:inScheme    ble: ;
        skos:related     xsd:float .

aiop:AutomationIOProfile
        a                skos:Concept ;
        rdfs:label       "Automation Input/Output Profile" ;
        rdfs:seeAlso     <https://www.bluetooth.org/docman/handlers/DownloadDoc.ashx?doc_id=304971> ;
        owl:versionInfo  "1.0.0" ;
        skos:definition  "The Automation Profile is used to enable a device to access analog and digital signals exposed by the Automation IO Service." ;
        skos:inScheme    ble: ;
        skos:related     aiop:AutomationIOService .

tip:TimeProfile  a       skos:Concept ;
        rdfs:label       "Time Profile" ;
        rdfs:seeAlso     <https://www.bluetooth.org/docman/handlers/downloaddoc.ashx?doc_id=241874> ;
        owl:versionInfo  "1.0" ;
        skos:definition  "The Time profile enables the device to get the date, time, time zone, and DST information and control the functions related the time." ;
        skos:inScheme    ble: ;
        skos:related     tip:ReferenceTimeUpdateService , tip:NextDSTChangeService , ble:CurrentTimeService .

ftmp:HeartRateField  a   skos:Concept ;
        rdfs:label       "Heart Rate Field" ;
        skos:definition  "The Heart Rate field represents the current heart rate value of the user (e.g., measured via the contact heart rate or any other means)." ;
        skos:inScheme    ble: ;
        skos:related     xsd:unsignedByte .

idp:Snoozed  a           skos:Concept ;
        rdfs:label       "Snoozed" ;
        skos:definition  "The annunciation was noticed by the user and is set to pop up again at a short time later" ;
        skos:inScheme    ble: .

ble:Profile  a         skos:Concept ;
        skos:inScheme  ble: ;
        skos:narrower  esp:EnvironmentalSensingProfile , rcp:ReconnectionConfigurationProfile , htp:HealthThermometerProfile , otp:ObjectTransferProfile , aiop:AutomationIOProfile , fmp:FindMeProfile , pxp:Proximityprofile , blp:BloodPressureProfile , cpp:CyclingPowerProfile , cscp:CyclingSpeedandCadenceProfile , lnp:LocationandNavigationProfile , ipsp:InternetProtocolSupportProfile , rscp:RunningSpeedandCadenceProfile , cgmp:ContinuousGlucoseMonitoringProfile , tip:TimeProfile , scpp:ScanParametersProfile , ftmp:FitnessMachineProfile , plxp:PulseOximeterProfile , hrp:HeartRateProfile , lehid:HIDoverGATTProfile , idp:InsulinDeliveryProfile , anp:AlertNotificationProfile , wsp:WeightScaleProfile , pasp:PhoneAlertStatusProfile , glp:GlucoseProfile ;
        skos:related   ble:Service .

ble:LocalNorthCoordinateValue
        a                skos:Concept ;
        rdfs:label       "The current value of the Local North Coordinate Characteristic" ;
        skos:definition  "When read, the Server shall return the current value of the Local North Coordinate Characteristic." ;
        skos:inScheme    ble: ;
        skos:related     xsd:Short .

idp:Priming  a           skos:Concept ;
        rdfs:label       "Priming" ;
        skos:definition  "The Insulin Delivery Device fills the fluidic path from the reservoir to the body with insulin" ;
        skos:inScheme    ble: .

cpp:TopDeadSpotAngleField
        a                skos:Concept ;
        rdfs:label       "Top Dead Spot Angle Field" ;
        skos:definition  "The Top Dead Spot Angle field represents the crank angle when the value of the Instantaneous Power value becomes positive." ;
        skos:inScheme    ble: ;
        skos:related     xsd:unsignedShort .

ble:IndoorPositioningValue
        a                skos:Concept ;
        rdfs:label       "The current value of  the Indoor Positioning Configuration Characteristic" ;
        skos:definition  "When read, the Indoor Positioning Configuration Characteristic shall return the current value of the characteristic." ;
        skos:inScheme    ble: ;
        skos:related     xsd:unsignedByte .

ble:Uncertainty  a       skos:Concept ;
        rdfs:label       "Uncertainty" ;
        skos:definition  "The Uncertainty Characteristic describes the uncertainty of the location information the device exposes." ;
        skos:inScheme    ble: ;
        skos:related     ble:WritewithoutResponse , ble:Read , ble:ReliableWrite , ble:UncertaintyValue , ble:Write .

cgmp:cgmpSessionStartTime
        a                skos:Concept ;
        rdfs:label       "cgmp Session Start Time" ;
        skos:definition  "The Session Start Time Field defines the time of the initial cgmp measurement." ;
        skos:inScheme    ble: ;
        skos:related     cgmp:TimeZoneField , cgmp:DTSOffsetField , cgmp:SessionStartTimeField , ble:Read , cgmp:E2ECRCField , ble:Write .

cgmp:cgmpMeasurement  a  skos:Concept ;
        rdfs:label       "GCM Measurement" ;
        skos:definition  "The cgmp Measurement characteristic is a variable length structure containing one or more cgmp Measurement records." ;
        skos:inScheme    ble: ;
        skos:related     cgmp:CGMGlucoseConcentrationField , cgmp:CGMQualityField , ble:Notify , cgmp:SensorStatusAnnunciationField , cgmp:CGMTrendInformationField , cgmp:TimeOffsetField , cgmp:E2ECRCField .

lnp:TotalDistanceField
        a                skos:Concept ;
        rdfs:label       "Total Distance Field" ;
        skos:definition  "The Total Distance field represents the cumulative value of the total distance measured by the sensor." ;
        skos:inScheme    ble: ;
        skos:related     xsd:unsignedInt .

ftmp:MinimumHeartRatefield
        a                skos:Concept ;
        rdfs:label       "Minimum Heart Rate" ;
        skos:definition  "Minimum Beats per minute with a resolution of 1" ;
        skos:inScheme    ble: ;
        skos:related     xsd:unsignedByte .

ftmp:HighSpeedOutside
        a                skos:Concept ;
        rdfs:label       "Speed Outside of Control Region - High" ;
        skos:definition  "0x0A - Speed Outside of Control Region - High (decrease speed to return to controllable region)" ;
        skos:inScheme    ble: .

glp:BaseTimeField  a     skos:Concept ;
        rdfs:label       "Base Time Field" ;
        skos:definition  "The Base Time field represents the value of an internal real-time clock or equivalent that keeps time relative to its initial setting in resolution of seconds." ;
        skos:inScheme    ble: .

anp:AlertNotificationService
        a                skos:Concept ;
        rdfs:label       "Alert Notification service" ;
        rdfs:seeAlso     <https://www.bluetooth.org/docman/handlers/downloaddoc.ashx?doc_id=242287> ;
        owl:versionInfo  "1.0" ;
        skos:definition  "Alert Notification service exposes the different types of alerts with the short text messages, the count of new alert messages, and the count of unread alerts" ;
        skos:inScheme    ble: ;
        skos:related     anp:AlertNotificationControlPoint , anp:NewAlert , anp:SupportedNewAlertCategory , anp:SupportedUnreadAlertCategory , anp:UnreadAlertStatus .

ble:OrganizationallyUniqueIdentifier
        a                skos:Concept ;
        rdfs:label       "Organizationally Unique Identifier" ;
        skos:definition  "The System ID characteristic shall represent a structure containing an Organizationally Unique Identifier (OUI)  is unique for each individual instance of the product." ;
        skos:inScheme    ble: ;
        skos:related     xsd:unsignedInt .

plxp:PulseAmplitudeIndex
        a                skos:Concept ;
        rdfs:label       "Pulse Amplitude Index" ;
        skos:definition  "The Pulse Amplitude Index is a percentage indicator indicating the perfusion level (amount of blood being delivered to the capillary bed) of a user." ;
        skos:inScheme    ble: ;
        skos:related     xsd:float .

ble:InstantaneousSpeedField
        a                skos:Concept ;
        rdfs:label       "Instantaneous Speed Field" ;
        skos:definition  "The Instantaneous Speed field represents the instantaneous value of the speed measured by the sensor." ;
        skos:inScheme    ble: ;
        skos:related     xsd:unsignedShort .

cscp:CyclingSpeedandCadenceProfile
        a                skos:Concept ;
        rdfs:label       "Cycling Speed and Cadence Profile" ;
        rdfs:seeAlso     <https://www.bluetooth.org/docman/handlers/downloaddoc.ashx?doc_id=261449> ;
        owl:versionInfo  "1.0" ;
        skos:definition  "The Cycling Speed and Cadence Profile is used to enable a data collection device to obtain data from a Cycling Speed and Cadence Sensor (CSC Sensor) that exposes the Cycling Speed and Cadence Service." ;
        skos:inScheme    ble: ;
        skos:related     ble:DeviceInformationService , cscp:CyclingSpeedandCadenceService .

otp:ObjectType  a        skos:Concept ;
        rdfs:label       "Object Type" ;
        skos:definition  "This characteristic exposes the type of the Current Object, identifying the object type by UUID." ;
        skos:inScheme    ble: ;
        skos:related     ble:Read .

wsp:WeightScaleService
        a                skos:Concept ;
        rdfs:label       "Weight Scale Service" ;
        rdfs:seeAlso     <https://www.bluetooth.org/docman/handlers/downloaddoc.ashx?doc_id=293526> ;
        owl:versionInfo  "1.0" ;
        skos:definition  "This service exposes weight and related data from a weight scale intended for consumer healthcare and sports/fitness applications." ;
        skos:inScheme    ble: ;
        skos:related     wsp:WeightMeasurement , wsp:WeightScaleFeature .

idp:Temperatureoutofrange
        a                skos:Concept ;
        rdfs:label       "Temperature out of range" ;
        skos:definition  "The temperature is outside of the normal operating range." ;
        skos:inScheme    ble: .

esp:CharacteristicUserDescription
        a                skos:Concept ;
        rdfs:label       "Characteristic User Description" ;
        skos:definition  "This optional descriptor can be used to associate a verbose name with a specific ESS characteristic to allow a human-readable label to be associated with the measurement." ;
        skos:inScheme    ble: ;
        skos:related     ble:Read , ble:Write .

ftmp:SupportedSpeedRange
        a                skos:Concept ;
        rdfs:label       "Supported Speed Range" ;
        skos:definition  "The Supported Speed Range characteristic is used to send the supported speed range as well as the minimum speed increment supported by the Server." ;
        skos:inScheme    ble: ;
        skos:related     ftmp:MaximumSpeedfield , ble:Read , ftmp:MinimumSpeedIncrementfield , ftmp:MinimumSpeedfield .

ftmp:MaximumInclinationfield
        a                skos:Concept ;
        rdfs:label       "Maximum Inclination" ;
        skos:definition  "Maximum Percent with a resolution of 0.1" ;
        skos:inScheme    ble: ;
        skos:related     xsd:short .

ftmp:MinimumSpeedIncrementfield
        a                skos:Concept ;
        rdfs:label       "Minimum Speed Increment" ;
        skos:definition  "Minimum Meters per second with a resolution of 0.01" ;
        skos:inScheme    ble: ;
        skos:related     xsd:unsignedShort .

aiop:Analog  a           skos:Concept ;
        rdfs:label       "Analog characteristic" ;
        skos:definition  "The Analog characteristic is used to read or write the value of one of the IOM’s analog signals." ;
        skos:inScheme    ble: ;
        skos:related     xsd:unsignedShort , ble:WritewithoutResponse , ble:Write , aiop:AnalogSignalValue , ble:Notify , ble:Read , ble:Indicate .

ble:USBImplementerForum
        a                skos:Concept ;
        rdfs:label       "USB Implementer’s Forum" ;
        skos:definition  "USB Implementer’s Forum assigned Vendor ID value." ;
        skos:inScheme    ble: ;
        skos:related     xsd:unsignedByte .

ftmp:RecoveryInterval
        a                skos:Concept ;
        rdfs:label       "Recovery Interval" ;
        skos:definition  "0x05 - Recovery Interval" ;
        skos:inScheme    ble: .

lnp:BeaconsNumberViewField
        a                skos:Concept ;
        rdfs:label       "Number of Beacons in View Field" ;
        skos:definition  "The Number of Beacons in View field represents the number of beacons from which the Server is receiving data." ;
        skos:inScheme    ble: ;
        skos:related     xsd:unsignedByte .

wsp:WeightScaleFeature
        a                skos:Concept ;
        rdfs:label       "Weight Scale Feature" ;
        skos:definition  "The Weight Scale Feature characteristic shall be used to describe the supported features of the Server." ;
        skos:inScheme    ble: ;
        skos:related     ble:Read .

otp:CurrentSizeField  a  skos:Concept ;
        rdfs:label       "Current Size Field" ;
        skos:definition  "The value of the Current Size field represents an integer number of octets equal to the actual size of the object." ;
        skos:inScheme    ble: ;
        skos:related     xsd:unsignedInt .

rcp:ReconnectionConfigurationProfile
        a                skos:Concept ;
        rdfs:label       "Reconnection Configuration Profile" ;
        rdfs:seeAlso     <https://www.bluetooth.org/docman/handlers/downloaddoc.ashx?doc_id=435662> ;
        owl:versionInfo  "1.0" ;
        skos:definition  "This Bluetooth profile specification defines requirements to enable a Reconnection Configuration Client to modify a variety of communication parameters of a Reconnection Configuration Server." ;
        skos:inScheme    ble: ;
        skos:related     ble:BondManagementService , rcp:ReconnectionConfigurationService .

lnp:LocationandNavigationService
        a                skos:Concept ;
        rdfs:label       "Location and Navigation (LN) Service" ;
        rdfs:seeAlso     <https://www.bluetooth.org/DocMan/handlers/DownloadDoc.ashx?doc_id=271997> ;
        owl:versionInfo  "1.0" ;
        skos:definition  "The Location and Navigation Service (LN Service) exposes location and navigation-related data from a Location and Navigation sensor (Server) intended for outdoor activity applications." ;
        skos:inScheme    ble: ;
        skos:related     lnp:Navigation , lnp:LNFeature , lnp:PositionQuality , lnp:LocationandSpeed , lnp:LNControlPoint .

ble:UserDataService  a   skos:Concept ;
        rdfs:comment     "This allows remote access and update of user data by a Client as well as the synchronization of user data between a Server and a Client." ;
        rdfs:label       "User Data Service" ;
        rdfs:seeAlso     <https://www.bluetooth.org/docman/handlers/downloaddoc.ashx?doc_id=288352> ;
        owl:versionInfo  "1.0" ;
        skos:definition  "The User Data Service (UDS) exposes user-related data in the sports and fitness environment." ;
        skos:inScheme    ble: ;
        skos:related     ble:UserIndex , ble:UDSCharacteristic , ble:UserControlPoint , ble:DatabaseChangeIncrement .

pxp:TxPowerService  a    skos:Concept ;
        rdfs:label       "Transmit (Tx) Power Service" ;
        rdfs:seeAlso     <https://www.bluetooth.org/docman/handlers/downloaddoc.ashx?doc_id=239393> ;
        owl:versionInfo  "1.0" ;
        skos:definition  "This service exposes a device’s current transmit power level when in a connection." ;
        skos:inScheme    ble: ;
        skos:related     pxp:TxPowerLevel .

glp:MealField  a         skos:Concept ;
        rdfs:label       "Meal" ;
        skos:definition  "Field exists if the key of bit 1 of the Flags field is set to 1" ;
        skos:inScheme    ble: ;
        skos:related     xsd:unsignedByte .

rcp:RCSettings  a        skos:Concept ;
        rdfs:label       "Reconnection Configuration Settings" ;
        skos:definition  "The RC Settings characteristic shall be used to both read and notify supported features on the Reconnection Configuration server." ;
        skos:inScheme    ble: ;
        skos:related     ble:Notify , ble:Read .

lnp:HDOPField  a         skos:Concept ;
        rdfs:label       "Horizontal Dilution Of Precision Field" ;
        skos:definition  "The HDOP field represents the Horizontal Dilution of Precision, a factor that influences the error in a position fix in the horizontal plane." ;
        skos:inScheme    ble: ;
        skos:related     xsd:unsignedByte .

htp:TemperatureMeasurement
        a                skos:Concept ;
        rdfs:label       "Temperature Measurement" ;
        skos:definition  "The Temperature Measurement characteristic is used to send a temperature measurement." ;
        skos:inScheme    ble: ;
        skos:related     htp:IntermediateTemperatureValueField , htp:TemperatureMeasurementValueField , ble:Indicate , ble:TimeStampField .

lnp:RemainingDistanceField
        a                skos:Concept ;
        rdfs:label       "Remaining Distance Field" ;
        skos:definition  "The Remaining Distance field represents the distance from the current position to the next waypoint or final destination." ;
        skos:inScheme    ble: ;
        skos:related     xsd:unsignedInt .

idp:InfusionSetDetached
        a                skos:Concept ;
        rdfs:label       "Infusion Set Detached" ;
        skos:definition  "The infusion set (including tubing and/or cannula) is not attached to the body." ;
        skos:inScheme    ble: .

lehid:Suspend  a         skos:Concept ;
        rdfs:label       "Suspend" ;
        skos:definition  "Informs HID Device that HID Host is entering the Suspend State" ;
        skos:inScheme    ble: .

ftmp:TrainingStatusField
        a                skos:Concept ;
        rdfs:label       "Training Status Field" ;
        skos:definition  "The Training Status field represents the current training state while a user is exercising." ;
        skos:inScheme    ble: ;
        skos:narrower    ftmp:PreWorkout , ftmp:WattControl , ftmp:Idle , ftmp:LowSpeedOutside , ftmp:RecoveryInterval , ftmp:FitnessTest , ftmp:HeartRateControl , ftmp:ManualMode , ftmp:CoolDown , ftmp:LowIntensityInterval , ftmp:HighSpeedOutside , ftmp:PostWorkout , ftmp:WarmingUp , ftmp:HighIntensityInterval , ftmp:Isometric ;
        skos:related     xsd:unsignedInt .

pasp:AlertStatus  a      skos:Concept ;
        rdfs:label       "Alert Status" ;
        skos:definition  "The Alert Status Characteristic exposes the alerting status of the server device." ;
        skos:inScheme    ble: ;
        skos:related     ble:Notify , ble:Read , pasp:AlertStatusValue .

ble:BondManagementControlPoint
        a                skos:Concept ;
        rdfs:label       "Bond Management Control Point" ;
        skos:definition  "The Server shall evaluate a GATT Characteristic Value Write procedure or a GATT Characteristic Value Reliable Write procedure to the Bond Management Control" ;
        skos:inScheme    ble: ;
        skos:related     ble:Write .

pxp:TxPowerLevel  a      skos:Concept ;
        rdfs:label       "Transmit Power Level" ;
        skos:definition  "The Tx Power Level characteristic represents the current transmit power." ;
        skos:inScheme    ble: ;
        skos:related     ble:Read , pxp:TxPowerLevelField .

otp:ObjectName  a        skos:Concept ;
        rdfs:label       "Object Name" ;
        skos:definition  "The Object Name characteristic exposes the name of the Current Object." ;
        skos:inScheme    ble: ;
        skos:related     ble:Read , otp:ObjectNameField , ble:Write .

ble:VendorIDSourceField
        a                skos:Concept ;
        rdfs:label       "Vendor ID Source Field" ;
        skos:definition  "The Vendor ID Source field designates which organization assigned the value used in the Vendor ID field value." ;
        skos:inScheme    ble: ;
        skos:narrower    ble:BluetoothSIG , ble:USBImplementerForum .

ble:ProductVersionField
        a                skos:Concept ;
        rdfs:label       "Product Version Field" ;
        skos:definition  "The Product Version field is a numeric expression identifying the device release number in Binary-Coded Decimal." ;
        skos:inScheme    ble: ;
        skos:related     xsd:unsignedShort .

tip:TimeUpdateState  a   skos:Concept ;
        rdfs:label       "Time Update State" ;
        skos:definition  "The Time Update State characteristic returns the current state of the reference time update on the Reference Time Update server." ;
        skos:inScheme    ble: ;
        skos:related     ble:Read , xsd:unsignedByte .

ble:UDSCharacteristicValue
        a                skos:Concept ;
        rdfs:label       "User Data Service Characteristic Value" ;
        skos:definition  "A UDS Characteristic returns its associated characteristic value when read." ;
        skos:inScheme    ble: .

ble:FirmwareRevision  a  skos:Concept ;
        rdfs:label       "Firmware Revision" ;
        skos:definition  "The Firmware Revision String characteristic shall represent the firmware revision for the firmware within the device." ;
        skos:inScheme    ble: ;
        skos:related     ble:Read , xsd:string .

idp:BolusDelayTime  a    skos:Concept ;
        rdfs:label       "Bolus Delay Time" ;
        skos:definition  "The Bolus Delay Time field represents the delay time of the bolus." ;
        skos:inScheme    ble: ;
        skos:related     xsd:unsignedShort .

rscp:TotalDistanceField
        a                skos:Concept ;
        rdfs:label       "Total Distance Field" ;
        skos:definition  "The Total Distance field may be included in the RSC Measurement characteristic if the device supports the Total Distance feature." ;
        skos:inScheme    ble: ;
        skos:related     xsd:unsignedInt .

ble:BondManagementService
        a                skos:Concept ;
        rdfs:label       "Bond Management Service" ;
        rdfs:seeAlso     <https://www.bluetooth.org/docman/handlers/downloaddoc.ashx?doc_id=293524> ;
        owl:versionInfo  "1.0" ;
        skos:definition  "This Specification proposes that this service will enable users to manage their bonds on devices with a limited user interface." ;
        skos:inScheme    ble: ;
        skos:related     ble:BondManagementControlPoint , ble:BondManagementFeature .

ble:Write  a             skos:Concept ;
        rdfs:label       "Write" ;
        skos:definition  "A Characteristic Value is writen to a server when the client knows the Characteristic Value Handle" ;
        skos:inScheme    ble: .

hrp:HeartRateService  a  skos:Concept ;
        rdfs:label       "Heart Rate Service" ;
        rdfs:seeAlso     <https://www.bluetooth.org/docman/handlers/downloaddoc.ashx?doc_id=239866> ;
        owl:versionInfo  "1.0" ;
        skos:definition  "The Heart Rate Service exposes heart rate and other data related to a heart rate sensor intended for fitness applications." ;
        skos:inScheme    ble: ;
        skos:related     hrp:HeartRateMeasurement , hrp:HeartRateControlPoint , hrp:BodySensorLocation .

ble:DatabaseChangeIncrement
        a                skos:Concept ;
        rdfs:label       "Database Change Increment" ;
        skos:definition  "When read or notified, the Database Change Increment characteristic returns a value that is used by a Client to determine whether or not the UDS Characteristics need to be synchronized between the Server and the Client." ;
        skos:inScheme    ble: ;
        skos:related     ble:Read , ble:Write , ble:DatabaseChangeIncrementValue .

ftmp:MaximumHeartRatefield
        a                skos:Concept ;
        rdfs:label       "Maximum Heart Rate" ;
        skos:definition  "Maximum Beats per minute with a resolution of 1" ;
        skos:inScheme    ble: ;
        skos:related     xsd:unsignedByte .

ftmp:RemainingTimeField
        a                skos:Concept ;
        rdfs:label       "Remaining Time Field" ;
        skos:definition  "The Remaining Time field represents the remaining time of a training session that has been selected." ;
        skos:inScheme    ble: ;
        skos:related     xsd:unsignedShort .

ble:Characteristic  a  skos:Concept ;
        skos:inScheme  ble: ;
        skos:narrower  lehid:BootKeyboardInputReport , cpp:CyclingPowerMeasurement , ble:DatabaseChangeIncrement , lnp:LNControlPoint , ble:IndoorPositioningConfiguration , ble:Longitude , lehid:HIDControlPoint , cgmp:cgmpMeasurement , ftmp:SupportedResistanceLevelRange , ftmp:StairClimberData , ble:IEEE11073-20601RegulatoryCertificationDataList , esp:ESTriggerSettingDescriptor , rscp:RSCMeasurement , glp:GlucoseMeasurementContext , idp:IDDFeatures , ftmp:CrossTrainerData , cscp:CSCFeature , lnp:PositionQuality , ble:ScanRefresh , ble:UserIndex , ble:BondManagementControlPoint , plxp:PLXContinuousMeasurement , ble:BondManagementFeature , aiop:Digital , ble:HTTPSSecurity , lehid:BootMouseInputReport , otp:ObjectID , ble:SCControlPoint , ble:HTTPStatusCode , htp:MeasurementInterval , lehid:Report , otp:ObjectListControlPoint , ble:ScanIntervalWindow , anp:NewAlert , htp:IntermediateTemperature , idp:IDDAnnunciationStatus , hrp:HeartRateControlPoint , ble:URI , cpp:CyclingPowerVector , ble:FloorNumber , ble:ReferenceTimeInformation , otp:ObjectType , idp:IDDStatusChanged , ble:PnPID , ble:SystemID , ble:LocalNorthCoordinate , ble:BatteryLevel , esp:DescriptorValueChanged , ftmp:IndoorBikeData , ble:RecordAccessControlPoint , blp:BloodPressureMeasurement , ftmp:StepClimberData , ble:AlertLevel , cscp:CSCMeasurement , pxp:LinkLossAlertLevel , ble:SensorLocation , lehid:ReportMap , wsp:WeightMeasurement , wsp:BodyCompositionFeature , cgmp:cgmpSpecificOpsControlPoint , lnp:LocationandSpeed , ble:SoftwareRevision , ble:Altitude , otp:ObjectSize , ftmp:TrainingStatus , lnp:LNFeature , ftmp:SupportedSpeedRange , rscp:RSCFeature , plxp:PLXFeatures , lehid:BootKeyboardOutputReport , esp:ValidRangeDescriptor , ble:Uncertainty , cpp:CyclingPowerControlPoint , otp:ObjectName , ftmp:FitnessMachineFeature , ble:HTTPHeaders , ble:TDSControlPoint , otp:ObjectProperties , ble:SerialNumber , ftmp:RowerData , cgmp:cgmpSessionStartTime , cpp:CyclingPowerFeature , ftmp:FitnessMachineStatus , hrp:BodySensorLocation , rscp:SCControlPoint , otp:ObjectListFilter , ftmp:SupportedHeartRateRange , ftmp:SupportedInclinationRange , rcp:RCSettings , tip:TimewithDST , ble:Latitude , ble:LocalTimeInformation , otp:ObjectFirstCreated , pasp:AlertStatus , ble:ModelNumber , ble:LocalEastCoordinate , idp:IDDCommandControlPoint , ble:UDSCharacteristic , tip:TimeUpdateState , aiop:Aggregate , rcp:RCFeature , otp:OTSFeature , idp:IDDHistoryData , pasp:RingerSetting , ftmp:SupportedPowerRange , ftmp:FitnessMachineControlPoint , tip:TimeUpdateControlPoint , blp:IntermediateCuffPressure , pasp:RingerControlPoint , plxp:PLXSpotcheckMeasurement , idp:IDDStatusReaderControlPoint , cgmp:cgmpFeature , ble:HTTPEntityBody , htp:TemperatureType , htp:ValidRangeDescriptor , htp:TemperatureMeasurement , idp:IDDStatus , otp:ObjectChanged , esp:CharacteristicUserDescriptionDescriptor , wsp:WeightScaleFeature , lnp:Navigation , anp:SupportedUnreadAlertCategory , lehid:HIDInformation , lehid:ProtocolMode , ble:LocationName , idp:IDDCommandData , anp:SupportedNewAlertCategory , esp:ESMeasurementDescriptor , ble:ManufacturerName , blp:BloodPressureFeature , anp:AlertNotificationControlPoint , ble:HTTPControlPoint , ble:FirmwareRevision , rcp:RCCP , aiop:Analog , esp:ESConfigurationDescriptor , ble:HardwareRevision , wsp:BodyCompositionMeasurement , otp:ObjectLastModified , anp:UnreadAlertStatus , ble:UserControlPoint , ble:CurrentTime , glp:GlucoseFeature , ftmp:TreadmillData , cgmp:cgmpStatus , pxp:TxPowerLevel , cgmp:cgmpSessionRunTime , otp:ObjectActionControlPoint , hrp:HeartRateMeasurement , idp:IDDRecordAccessControlPoint , glp:GlucoseMeasurement ;
        skos:related   ble:Value , ble:Property .

lnp:EVPEField  a         skos:Concept ;
        rdfs:label       "Estimated Vertical Position Error Field" ;
        skos:definition  "The EVPE field represents the Estimated Vertical Position Error, i.e., a measure of the error in a position in the vertical plane." ;
        skos:inScheme    ble: ;
        skos:related     xsd:unsignedInt .

idp:DateTimeIssue  a     skos:Concept ;
        rdfs:label       "Date Time Issue" ;
        skos:definition  "The date time of the device was never set or has been lost (e.g., due to a battery replacement)." ;
        skos:inScheme    ble: .

ble:LE_Scan_Interval  a  skos:Concept ;
        rdfs:label       "Low Energy_Scan_Window" ;
        skos:definition  "The minimum LE_Scan_Window of the Client corresponding to the LE_Scan_Interval." ;
        skos:inScheme    ble: ;
        skos:related     xsd:unsignedShort .

cpp:InstantaneousTorqueMagnitudeArrayField
        a                skos:Concept ;
        rdfs:label       "Instantaneous Torque Magnitude Array Field" ;
        skos:definition  " Included in this field are one or more Instantaneous Magnitude values which are expressed in Newton meter with a resolution of 1/32 Newton meter" ;
        skos:inScheme    ble: ;
        skos:related     xsd:short .

idp:MaxDelivery  a       skos:Concept ;
        rdfs:label       "Max Delivery" ;
        skos:definition  "The delivery reached a defined high threshold based on maximum bolus and maximum basal rates" ;
        skos:inScheme    ble: .

ble:FloorNumber  a       skos:Concept ;
        rdfs:label       "Floor Number" ;
        skos:definition  "The Floor Number Characteristic describes the floor number in which the device is installed." ;
        skos:inScheme    ble: ;
        skos:related     ble:FloorNumberValue , ble:WritewithoutResponse , ble:Read , ble:ReliableWrite , ble:Write .

aiop:Aggregate  a        skos:Concept ;
        rdfs:label       "Aggregate characteristic" ;
        skos:definition  "Aggregate characteristic is used to aggregate all Digital characteristics with the Read property set (if any available) and all of the Analog characteristics with Read properties set (if any available)." ;
        skos:inScheme    ble: ;
        skos:related     ble:Notify , ble:Read , ble:Indicate .

idp:InsulinDeliveryService
        a                skos:Concept ;
        rdfs:label       "Insulin Delivery Service" ;
        rdfs:seeAlso     <https://www.bluetooth.org/DocMan/handlers/DownloadDoc.ashx?doc_id=447826> ;
        owl:versionInfo  "1.0" ;
        skos:definition  "The Insulin Delivery Service (IDS) exposes the control capability and the status of an Insulin Delivery Device running an insulin infusion therapy." ;
        skos:inScheme    ble: ;
        skos:related     idp:IDDStatusReaderControlPoint , idp:IDDStatusChanged , idp:IDDFeatures , idp:IDDCommandControlPoint , idp:IDDRecordAccessControlPoint , idp:IDDCommandData , idp:IDDHistoryData , idp:IDDAnnunciationStatus , idp:IDDStatus .

lnp:UTCTimeField  a      skos:Concept ;
        rdfs:label       "UTC Time Field" ;
        skos:definition  "This field represents the time at the Sensor when the position was received in Coordinated Universal Time format." ;
        skos:inScheme    ble: .

lnp:VDOPField  a         skos:Concept ;
        rdfs:label       "Vertical Dilution Of Precision Field" ;
        skos:definition  "The VDOP field represents the Vertical Dilution of Precision, a factor that influences the error in a position fix in the vertical plane." ;
        skos:inScheme    ble: ;
        skos:related     xsd:unsignedByte .

rcp:RCFeature  a         skos:Concept ;
        rdfs:label       "Reconnection Configuration Feature" ;
        skos:definition  "The RC Features characteristic shall be used to describe the supported features of the Reconnection Configuration server." ;
        skos:inScheme    ble: ;
        skos:related     ble:Read .

idp:TherapyControlStatefield
        a                skos:Concept ;
        rdfs:label       "Therapy Control State field" ;
        skos:definition  "The Therapy Control State field describes the therapy state of the insulin delivery (e.g., stop, pause, run)." ;
        skos:inScheme    ble: ;
        skos:narrower    idp:Stop , idp:Undetermined , idp:Run , idp:Pause ;
        skos:related     xsd:unsignedByte .

ftmp:StrokeRateField  a  skos:Concept ;
        rdfs:label       "Stroke Rate Field" ;
        skos:definition  "The Stroke Rate field represents the instantaneous stroke rate measured by the Server." ;
        skos:inScheme    ble: ;
        skos:related     xsd:unsignedByte .

ble:BondManagementFeature
        a                skos:Concept ;
        rdfs:label       "Bond Management Feature" ;
        skos:definition  "The Bond Management Feature characteristic shall be used to indicate the supported features of the server." ;
        skos:inScheme    ble: ;
        skos:related     ble:Read .

idp:RelativeOffsetfield
        a                skos:Concept ;
        rdfs:label       "Relative Offset field" ;
        skos:definition  "The Relative Offset field represents the elapsed time in seconds since the last recorded Reference Time event." ;
        skos:inScheme    ble: ;
        skos:related     xsd:unsignedShort .

idp:Temperature  a       skos:Concept ;
        rdfs:label       "Temperature" ;
        skos:definition  "The Insulin Delivery Device reports a temperature measurement." ;
        skos:inScheme    ble: .

lehid:HIDControlPoint
        a                skos:Concept ;
        rdfs:label       "HID Control Point" ;
        skos:definition  "The HID Control Point characteristic is a control-point attribute that defines Suspend and Exit Suspend HID Commands when written." ;
        skos:inScheme    ble: ;
        skos:related     ble:WritewithoutResponse , lehid:HIDControlPointCharacteristicValue .

ftmp:FitnessMachineService
        a                skos:Concept ;
        rdfs:label       "Fitness Machine Service" ;
        rdfs:seeAlso     <https://www.bluetooth.org/DocMan/handlers/DownloadDoc.ashx?doc_id=423422> ;
        owl:versionInfo  "1.0" ;
        skos:definition  "The Fitness Machine Service (FTMS) exposes training-related data in the sports and fitness environment, which allows a Client to collect training data while a user is exercising with a fitness machine (Server)." ;
        skos:inScheme    ble: ;
        skos:related     ftmp:StepClimberData , ftmp:SupportedHeartRateRange , ftmp:SupportedSpeedRange , ftmp:TrainingStatus , ftmp:SupportedPowerRange , ftmp:FitnessMachineStatus , ftmp:IndoorBikeData , ftmp:TreadmillData , ftmp:SupportedResistanceLevelRange , ftmp:FitnessMachineControlPoint , ftmp:RowerData , ftmp:SupportedInclinationRange , ftmp:StairClimberData , ftmp:CrossTrainerData , ftmp:FitnessMachineFeature .

ftmp:SupportedResistanceLevelRange
        a                skos:Concept ;
        rdfs:label       "Supported Resistance Level Range" ;
        skos:definition  "The Supported Resistance Level Range characteristic is used to send the supported resistance level range as well as the minimum resistance increment supported by the Server." ;
        skos:inScheme    ble: ;
        skos:related     ftmp:MaximumResistanceLevelField , ble:Read , ftmp:MinimumResistanceIncrementfield , ftmp:MinimumPowerfield .

ftmp:EnergyperMinuteField
        a                skos:Concept ;
        rdfs:label       "Energy per Minute Field" ;
        skos:definition  "The Energy per Minute field represents the average expended energy of a user during a period of one minute." ;
        skos:inScheme    ble: ;
        skos:related     xsd:short .

ftmp:MinimumPowerIncrementfield
        a                skos:Concept ;
        rdfs:label       "Minimum Power Increment" ;
        skos:definition  "Minimum Watt  with a resolution of 1" ;
        skos:inScheme    ble: ;
        skos:related     xsd:unsignedShort .

ble:LocalNorthCoordinate
        a                skos:Concept ;
        rdfs:label       "Local North Coordinate" ;
        skos:definition  "The Local North Coordinate Characteristic describes the North coordinate of the device using a local coordinate system." ;
        skos:inScheme    ble: ;
        skos:related     ble:WritewithoutResponse , ble:Read , ble:LocalNorthCoordinateValue , ble:ReliableWrite , ble:Write .

idp:Confirmed  a         skos:Concept ;
        rdfs:label       "Confirmed" ;
        skos:definition  "The annunciation was confirmed by the user" ;
        skos:inScheme    ble: .

wsp:BodyCompositionMeasurement
        a                skos:Concept ;
        rdfs:label       "Body Composition Measurement" ;
        skos:definition  "The Body Composition Measurement characteristic is used to send body composition-related data to the Client." ;
        skos:inScheme    ble: ;
        skos:related     wsp:WeightField , wsp:BodyFatPercentageField , ble:Indicate , wsp:HeightField , wsp:MusclePercentageField , wsp:BasalMetabolismField , wsp:FatFreeMassField , wsp:MuscleMassField , wsp:ImpedanceField , ble:UserIDField , wsp:SoftLeanMassField , wsp:BodyWaterField .

otp:AllocatedSizeField
        a                skos:Concept ;
        rdfs:label       "Allocated Size Field" ;
        skos:definition  "This value indicates the amount of memory the Server has reserved for holding the object contents." ;
        skos:inScheme    ble: ;
        skos:related     xsd:unsignedInt .

ble:DeviceInformationService
        a                skos:Concept ;
        rdfs:label       "Device Information Service." ;
        rdfs:seeAlso     <https://www.bluetooth.org/docman/handlers/downloaddoc.ashx?doc_id=244369> ;
        owl:versionInfo  "1.1" ;
        skos:definition  "The Device Information Service exposes manufacturer and/or vendor information about a device." ;
        skos:inScheme    ble: ;
        skos:related     ble:SystemID , ble:HardwareRevision , ble:PnPID , ble:SerialNumber , ble:SoftwareRevision , ble:IEEE11073-20601RegulatoryCertificationDataList , ble:FirmwareRevision , ble:ModelNumber , ble:ManufacturerName .

ftmp:InclinationField
        a                skos:Concept ;
        rdfs:label       "Inclination Field" ;
        skos:definition  "The Inclination field represents the current inclination of the Server. A positive value means that the user feels as if they are going uphill and a negative value means that the user feels as if they are going downhill." ;
        skos:inScheme    ble: ;
        skos:related     xsd:short .

ftmp:CrossTrainerData
        a                skos:Concept ;
        rdfs:label       "Cross Trainer Data" ;
        skos:definition  "The Cross Trainer Data characteristic is used to send training-related data to the Client from a cross trainer (Server)." ;
        skos:inScheme    ble: ;
        skos:related     ftmp:StepperMinuteField , ftmp:StrideCountField , ftmp:HeartRateField , ble:InstantaneousSpeedField , ftmp:EnergyperMinuteField , ble:InstantaneousPowerField , ftmp:MetabolicEquivalentField , ftmp:PositiveElevationGainField , ftmp:InclinationField , ble:Notify , ftmp:TotalEnergyField , ftmp:ElapsedTimeField , ftmp:AverageStepRateField , ftmp:EnergyperHourField , ftmp:RampAngleSettingField , ftmp:ResistanceLevelField , ftmp:RemainingTimeField , ftmp:TotalDistanceField , ftmp:AveragePowerField , ftmp:AverageSpeedField , ftmp:NegativeElevationGainField .

ftmp:Isometric  a        skos:Concept ;
        rdfs:label       "Isometric" ;
        skos:definition  "0x06-Isometric" ;
        skos:inScheme    ble: .

ble:HTTPControlPoint  a  skos:Concept ;
        rdfs:label       "HTTP Control Point" ;
        skos:definition  "The HTTP Control Point is used to initiate a request to send an HTTP request message from the device containing the HTTP Proxy Service, acting as an HTTP Client." ;
        skos:inScheme    ble: ;
        skos:related     ble:Write .

aiop:AnalogSignalValue
        a                skos:Concept ;
        rdfs:label       "Value of an analog signal" ;
        skos:definition  "The Analog characteristic represents the value of an analog signal as an unsigned 16-bit integer (uint16)." ;
        skos:inScheme    ble: ;
        skos:related     xsd:unsignedShort .

cgmp:cgmpSpecificOpsControlPoint
        a                skos:Concept ;
        rdfs:label       "cgmp Specific Ops Control Point" ;
        skos:definition  "The Client shall perform a write to the cgmp Specific Ops Control Point to request a desired cgmp specific procedure at the Server." ;
        skos:inScheme    ble: ;
        skos:related     ble:Indicate , ble:Write .

plxp:PLXSpotcheckMeasurement
        a                skos:Concept ;
        rdfs:label       "Pulse Oximeter Spot-check Measurement" ;
        skos:definition  "The PLX Spot-check Measurement characteristic, if supported, shall be used to send Spot-check measurements of SpO2 (Percent oxygen saturation of hemoglobin) and PR (pulse rate)." ;
        skos:inScheme    ble: ;
        skos:related     plxp:PulseAmplitudeIndex , ble:TimestampField , plxp:SpO2PRSpotCheckField , ble:Indicate .

ftmp:ElapsedTimeField
        a                skos:Concept ;
        rdfs:label       "Elapsed Time Field" ;
        skos:definition  "The Elapsed Time field represents the elapsed time of a training session since the training session has started." ;
        skos:inScheme    ble: ;
        skos:related     xsd:unsignedShort .

ble:Property  a        skos:Concept ;
        skos:inScheme  ble: ;
        skos:narrower  ble:Notify , ble:WritewithoutResponse , ble:WriteLong , ble:Read , ble:Write , ble:ReadLong , ble:ReliableWrite , ble:Indicate .

ble:ReferenceTimeInformation
        a                skos:Concept ;
        rdfs:label       "Reference Time Information" ;
        skos:definition  "The Reference Time Information characteristic returns the information about the reference time source." ;
        skos:inScheme    ble: ;
        skos:related     ble:Read .

ftmp:EnergyperHourField
        a                skos:Concept ;
        rdfs:label       "Energy per Hour Field" ;
        skos:definition  "The Energy per Hour field represents the average expended energy of a user during a period of one hour." ;
        skos:inScheme    ble: ;
        skos:related     xsd:short .

idp:ReservoirLow  a      skos:Concept ;
        rdfs:label       "Reservoir Low" ;
        skos:definition  "The reservoir fill level reached a defined low threshold." ;
        skos:inScheme    ble: .

htp:TemperatureType  a   skos:Concept ;
        rdfs:label       "Temperature Type" ;
        skos:definition  "The Temperature Type characteristic is used to describe the type of temperature measurement in relation to the location on the human body at which the temperature was measured." ;
        skos:inScheme    ble: ;
        skos:related     ble:Read .

blp:BloodPressureProfile
        a                skos:Concept ;
        rdfs:label       "Blood Pressure Profile" ;
        rdfs:seeAlso     <https://www.bluetooth.org/docman/handlers/downloaddoc.ashx?doc_id=457086> ;
        owl:versionInfo  "1.0.1" ;
        skos:definition  "The Blood Pressure Profile is used to enable a device to obtain blood pressure measurement and other data from a non-invasive blood pressure sensor that exposes the Blood Pressure Service." ;
        skos:inScheme    ble: ;
        skos:related     blp:BloodPressureService , ble:DeviceInformationService .

ble:HardwareRevision  a  skos:Concept ;
        rdfs:label       "Hardware Revision" ;
        skos:definition  "The Hardware Revision String characteristic shall represent the hardware revision for the hardware within the device." ;
        skos:inScheme    ble: ;
        skos:related     ble:Read , xsd:string .

idp:BolusDurationfield
        a                skos:Concept ;
        rdfs:label       "Bolus Duration field" ;
        skos:definition  "The Bolus Duration field represents the duration of the bolus." ;
        skos:inScheme    ble: .

otp:ObjectListControlPoint
        a                skos:Concept ;
        rdfs:label       "Object List Control Point" ;
        skos:definition  "The role of the OLCP is to provide a mechanism for the Client to find the desired object and to designate it as the Current Object." ;
        skos:inScheme    ble: ;
        skos:related     ble:Indicate , ble:Write .

cpp:CyclingPowerService
        a                skos:Concept ;
        rdfs:label       "Cycling Power Service" ;
        rdfs:seeAlso     <https://www.bluetooth.org/DocMan/handlers/DownloadDoc.ashx?doc_id=412770> ;
        owl:versionInfo  "1.1" ;
        skos:definition  "The Cycling Power (CP) Service exposes power- and force-related data and optionally speed- and cadence-related data from a Cycling Power sensor (Server) intended for sports and fitness applications." ;
        skos:inScheme    ble: ;
        skos:related     cpp:CyclingPowerVector , cpp:CyclingPowerControlPoint , cpp:CyclingPowerFeature , ble:SensorLocation , cpp:CyclingPowerMeasurement .

ftmp:ManualMode  a       skos:Concept ;
        rdfs:label       "Manual Mode" ;
        skos:definition  "0x0D - Manual Mode (Quick Start)" ;
        skos:inScheme    ble: .

ftmp:MaximumSpeedfield
        a                skos:Concept ;
        rdfs:label       "Maximum Speed" ;
        skos:definition  "Maximum Kilometer per hour with a resolution of 0.01" ;
        skos:inScheme    ble: ;
        skos:related     xsd:unsignedShort .

cpp:CyclingPowerControlPoint
        a                skos:Concept ;
        rdfs:label       "Cycling Power Control Point" ;
        skos:definition  "The Cycling Power Control Point is used by a Client to control certain behaviors of the Server." ;
        skos:inScheme    ble: ;
        skos:related     ble:Indicate , xsd:unsignedByte , ble:Write .

otp:ObjectID  a          skos:Concept ;
        rdfs:label       "Object ID" ;
        skos:definition  "The Object ID characteristic exposes an integer value which is the Object ID of the Current Object." ;
        skos:inScheme    ble: ;
        skos:related     ble:Read , otp:ObjectIDField .

lnp:Navigation  a        skos:Concept ;
        rdfs:label       "Navigation" ;
        skos:definition  "The Navigation characteristic is used to send navigation-related data." ;
        skos:inScheme    ble: ;
        skos:related     lnp:EstimatedTimeArrivalField , ble:Notify , lnp:BearingField , lnp:RemainingDistanceField , lnp:HeadingField , lnp:RemainingVerticalDistanceField .

idp:IDDStatusChanged  a  skos:Concept ;
        rdfs:label       "Insulin Delivery Device Status Changed" ;
        skos:definition  "The IDD Status Changed characteristic is comprised of status changes of the insulin therapy and the Insulin Delivery Device." ;
        skos:inScheme    ble: ;
        skos:related     idp:E2ECRCfield , idp:E2ECounterfield , ble:Read , ble:Indicate .

lehid:BootMouseInputReport
        a                skos:Concept ;
        rdfs:label       "Boot Mouse Input Report" ;
        skos:definition  "The Boot Mouse Input Report characteristic is used to transfer fixed format and length Input Report data between a HID Host operating in Boot Protocol Mode and a HID Service corresponding to a boot mouse." ;
        skos:inScheme    ble: ;
        skos:related     ble:Read , lehid:BootMouseInputReportValue , ble:Write .

wsp:WeightField  a       skos:Concept ;
        rdfs:label       "Weight Field" ;
        skos:definition  "The Weight field may be included in the Body Composition Measurement characteristic if the device supports the Weight feature.The Weight field shall be included in the Weight Measurement characteristic" ;
        skos:inScheme    ble: ;
        skos:related     xsd:unsignedShort .

otp:ObjectTransferService
        a                skos:Concept ;
        rdfs:label       "Object Transfer Service" ;
        rdfs:seeAlso     <https://www.bluetooth.org/docman/handlers/DownloadDoc.ashx?doc_id=309937> ;
        owl:versionInfo  "1.0" ;
        skos:definition  "This service provides management and control features supporting bulk data transfers which occur via a separate L2CAP connection oriented channel." ;
        skos:inScheme    ble: ;
        skos:related     otp:ObjectListControlPoint , otp:ObjectLastModified , otp:ObjectType , otp:ObjectID , otp:ObjectSize , otp:ObjectFirstCreated , otp:ObjectChanged , otp:ObjectProperties , otp:ObjectName , otp:OTSFeature , otp:ObjectListFilter , otp:ObjectActionControlPoint .

ble:SerialNumber  a      skos:Concept ;
        rdfs:label       "Serial Number" ;
        skos:definition  "The Serial Number String characteristic shall represent the serial number for a particular instance of the device." ;
        skos:inScheme    ble: ;
        skos:related     ble:Read , xsd:string .

glp:CarbohydrateIDField
        a                skos:Concept ;
        rdfs:label       "Carbohydrate ID Field" ;
        skos:definition  "Field exists if the key of bit 0 of the Flags field is set to 1." ;
        skos:inScheme    ble: ;
        skos:related     xsd:unsignedByte .

htp:HealthThermometerService
        a                skos:Concept ;
        rdfs:label       "Health Thermometer Service" ;
        rdfs:seeAlso     <https://www.bluetooth.org/docman/handlers/downloaddoc.ashx?doc_id=238688> ;
        owl:versionInfo  "1.0" ;
        skos:definition  "This service exposes temperature and other data from a Thermometer intended for healthcare and fitness applications." ;
        skos:inScheme    ble: ;
        skos:related     htp:MeasurementInterval , htp:IntermediateTemperature , htp:TemperatureType , htp:ValidRangeDescriptor , htp:TemperatureMeasurement .

ftmp:LowSpeedOutside  a  skos:Concept ;
        rdfs:label       "Speed Outside of Control Region - Low" ;
        skos:definition  "0x09 - Speed Outside of Control Region - Low (increase speed to return to controllable region)" ;
        skos:inScheme    ble: .

ftmp:TrainingStatusStringField
        a                skos:Concept ;
        rdfs:label       "Training Status String Field" ;
        skos:definition  "The Training Status String field is a string-based field that can be used to give more specific information related to the training status." ;
        skos:inScheme    ble: ;
        skos:related     xsd:string .

ble:HTTPProxyService  a  skos:Concept ;
        rdfs:label       "Hyper Text Transfer Protocol (HTTP) Proxy Service" ;
        rdfs:seeAlso     <https://www.bluetooth.org/docman/handlers/downloaddoc.ashx?doc_id=308344> ;
        owl:versionInfo  "1.0" ;
        skos:definition  "The HTTP Proxy Service (HPS) allows a device to expose HTTP Web services to a client of the HPS Server (HPS Client) using the Generic Attribute Profile (GATT)." ;
        skos:inScheme    ble: .

ftmp:PostWorkout  a      skos:Concept ;
        rdfs:label       "Post-Workout" ;
        skos:definition  "0x0F - Post-Workout" ;
        skos:inScheme    ble: .

cpp:MaximumTorqueMagnitude
        a                skos:Concept ;
        rdfs:label       "Maximum Torque Magnitude" ;
        skos:definition  "The Maximum Torque Magnitude field represents the maximum torque value measured in a single crank revolution." ;
        skos:inScheme    ble: ;
        skos:related     xsd:short .

ftmp:TrainingStatus  a   skos:Concept ;
        rdfs:label       "Training Status" ;
        skos:definition  "The Training Status characteristic shall be used by the Server to send the training status information to the Client." ;
        skos:inScheme    ble: ;
        skos:related     ftmp:TrainingStatusField , ble:Notify , ble:Read , ftmp:TrainingStatusStringField .

esp:EnvironmentalSensingProfile
        a                skos:Concept ;
        rdfs:label       "Environmental Sensing Profile" ;
        rdfs:seeAlso     <https://www.bluetooth.org/docman/handlers/downloaddoc.ashx?doc_id=294796> ;
        owl:versionInfo  "1.0.0" ;
        skos:definition  "This profile enables a Collector device to connect and interact with an Environmental Sensor for use in outdoor activity applications." ;
        skos:inScheme    ble: ;
        skos:related     esp:EnvironmentalSensingService , ble:DeviceInformationService , ble:BatteryService .

cscp:CSCFeature  a       skos:Concept ;
        rdfs:label       "Cycling Speed and Cadence Feature" ;
        skos:definition  "The CSC Feature characteristic shall be used to describe the supported features of the Server." ;
        skos:inScheme    ble: ;
        skos:related     ble:Read .

glp:GlucoseProfile  a    skos:Concept ;
        rdfs:label       "Glucose Profile" ;
        rdfs:seeAlso     <https://www.bluetooth.org/DocMan/handlers/DownloadDoc.ashx?doc_id=248025> ;
        owl:versionInfo  "1.0" ;
        skos:definition  "The Glucose Profile is used to enable a device to obtain glucose measurement and other data from a Glucose Sensor that exposes the Glucose Service." ;
        skos:inScheme    ble: ;
        skos:related     glp:GlucoseService , ble:DeviceInformationService .

tip:NextDSTChangeService
        a                skos:Concept ;
        rdfs:label       "Daylight Saving Time Change Service" ;
        rdfs:seeAlso     <https://www.bluetooth.org/docman/handlers/downloaddoc.ashx?doc_id=241872> ;
        owl:versionInfo  "1.0" ;
        skos:definition  "This service defines how the information about an upcoming DST change can be exposed using the Generic Attribute Profile (GATT)." ;
        skos:inScheme    ble: ;
        skos:related     tip:TimewithDST .

ble:ScanParametersService
        a                skos:Concept ;
        rdfs:label       "Scan Parameters Service" ;
        rdfs:seeAlso     <https://www.bluetooth.org/docman/handlers/downloaddoc.ashx?doc_id=245143> ;
        owl:versionInfo  "1.0" ;
        skos:definition  "The Scan Parameters Service enables a GATT Server device to expose a characteristic for the GATT Client to write its scan interval and scan window on the GATT Server device, and enables a GATT Server to request a refresh of the GATT Client scan interval and scan window." ;
        skos:inScheme    ble: ;
        skos:related     ble:ScanRefresh , ble:ScanIntervalWindow .

lehid:BootKeyboardInputReport
        a                skos:Concept ;
        rdfs:label       "Boot Keyboard Input Report" ;
        skos:definition  "The Input Boot Keyboard Report characteristic is used to transfer fixed format and length Input Report data between a HID Host operating in Boot Protocol Mode and a HID Service corresponding to a boot keyboard." ;
        skos:inScheme    ble: ;
        skos:related     ble:Notify , ble:Read , lehid:BootKeyboardInputReportValue .

ftmp:CoolDown  a         skos:Concept ;
        rdfs:label       "Cool Down" ;
        skos:definition  "0x0B - Cool Down" ;
        skos:inScheme    ble: .

ble:DatabaseChangeIncrementValue
        a                skos:Concept ;
        rdfs:label       "Database Change Increment Value" ;
        skos:definition  "When read or notified, the Database Change Increment characteristic returns a value that is used by a Client to determine whether or not the UDS Characteristics need to be synchronized between the Server and the Client." ;
        skos:inScheme    ble: ;
        skos:related     xsd:unsignedInt .

glp:MedicationField  a   skos:Concept ;
        rdfs:label       "Medication - units of kilograms" ;
        skos:definition  "C6: Field exists if the key of bit 4 of the Flags field is set to 1, C8: Field exists if the key of bit 5 of the Flags field is set to 0" ;
        skos:inScheme    ble: ;
        skos:related     xsd:float .

ble:VendorIDField  a     skos:Concept ;
        rdfs:label       "Vendor ID Field" ;
        skos:definition  "The Vendor ID field is intended to uniquely identify the vendor of the device." ;
        skos:inScheme    ble: ;
        skos:related     xsd:unsignedShort .

idp:OperationalStatefield
        a                skos:Concept ;
        rdfs:label       "Operational State field" ;
        skos:definition  "The Operational State field represents the operational state of the Insulin Delivery Device in the context of running an insulin infusion therapy (e.g., priming)." ;
        skos:inScheme    ble: ;
        skos:related     idp:Standby , idp:Preparing , idp:Ready , idp:Waiting , idp:Undetermined , xsd:unsignedByte , idp:Off , idp:Priming .

idp:Stop  a            skos:Concept ;
        rdfs:label     "Stop" ;
        skos:inScheme  ble: .

ble:ManufacturerIdentifier
        a                skos:Concept ;
        rdfs:label       "Manufacturer Identifier" ;
        skos:definition  "The System ID characteristic shall represent a structure containing a manufacturer-defined identifier following an Organizationally Unique Identifier (OUI) and is unique for each individual instance of the product." ;
        skos:inScheme    ble: ;
        skos:related     xsd:unsignedInt .

lnp:RollingTimeField  a  skos:Concept ;
        rdfs:label       "Rolling Time Field" ;
        skos:definition  "The Rolling Time field represents the time in seconds and rolls over every 256 seconds and it can be used by the Client to keep track of the time elapsed between the position information received by the Server." ;
        skos:inScheme    ble: ;
        skos:related     xsd:unsignedByte .

rscp:InstantaneousStrideLengthField
        a                skos:Concept ;
        rdfs:label       "Instantaneous Stride Length Field" ;
        skos:definition  "The Instantaneous Stride Length field may be included in the RSC Measurement characteristic if the device supports the Instantaneous Stride Length feature." ;
        skos:inScheme    ble: ;
        skos:related     xsd:unsignedShort .

ftmp:MinimumInclinationfield
        a                skos:Concept ;
        rdfs:label       "Minimum Inclination" ;
        skos:definition  "Minimum Percent with a resolution of 0.1" ;
        skos:inScheme    ble: ;
        skos:related     xsd:short .

ftmp:WattControl  a      skos:Concept ;
        rdfs:label       "Watt Control" ;
        skos:definition  "0x0C- Watt Control" ;
        skos:inScheme    ble: .

pxp:LinkLossAlertLevel
        a                skos:Concept ;
        rdfs:label       "Alert Level of Link Loss Service" ;
        skos:definition  "The Alert Level characteristic is used to expose the current link loss alert level that is used to determine how the device alerts when the link is lost." ;
        skos:inScheme    ble: ;
        skos:related     ble:Read , xsd:unsignedByte , ble:Write .

otp:ObjectLastModifiedField
        a                skos:Concept ;
        rdfs:label       "Object Last-Modified Field" ;
        skos:definition  "The Object Last-Modified characteristic returns its associated value when read. The date and time value shall be represented in Coordinated Universal Time (UTC)." ;
        skos:inScheme    ble: .

anp:CategoryID  a        skos:Concept ;
        rdfs:label       "Category ID" ;
        skos:definition  "This field shows the category of the new alert." ;
        skos:inScheme    ble: .

ftmp:MinimumResistanceLevelField
        a                skos:Concept ;
        rdfs:label       "Minimum Resistance Level" ;
        skos:definition  "Unitless with a resolution of 0.1" ;
        skos:inScheme    ble: ;
        skos:related     xsd:short .

fmp:FindMeProfile  a     skos:Concept ;
        rdfs:label       "Find Me Profile" ;
        rdfs:seeAlso     <https://www.bluetooth.org/docman/handlers/downloaddoc.ashx?doc_id=239389> ;
        owl:versionInfo  "1.0" ;
        skos:definition  "The Find Me profile defines the behavior when a button is pressed on one device to cause an alerting signal on a peer device." ;
        skos:inScheme    ble: ;
        skos:related     ble:ImmediateAlertService .

ble:TDSControlPoint  a   skos:Concept ;
        rdfs:label       "Transport Discovery Control Point" ;
        skos:definition  "The TDS Control Point characteristic is used to request activation of a transport." ;
        skos:inScheme    ble: .

ftmp:Idle  a             skos:Concept ;
        rdfs:label       "Idle" ;
        skos:definition  "0x01 - Idle" ;
        skos:inScheme    ble: .

anp:TextStringInformation
        a                skos:Concept ;
        rdfs:label       "Text String Information" ;
        skos:definition  "The field provides brief text information for the last alert." ;
        skos:inScheme    ble: ;
        skos:related     xsd:string .

ble:SoftwareRevision  a  skos:Concept ;
        rdfs:label       "SoftwareRevision" ;
        skos:definition  "The Software Revision String characteristic shall represent the software revision for the software within the device." ;
        skos:inScheme    ble: ;
        skos:related     ble:Read , xsd:string .

wsp:MusclePercentageField
        a                skos:Concept ;
        rdfs:label       "Muscle Percentage Field" ;
        skos:definition  "The Muscle Percentage field may be included in the Body Composition Measurement characteristic if the device supports the Muscle Percentage feature." ;
        skos:inScheme    ble: ;
        skos:related     xsd:unsignedShort .

ble:Indicate  a          skos:Concept ;
        rdfs:label       "Indicate" ;
        skos:definition  "A server is configured to indicate a Characteristic Value to a client and expects an Attribute Protocol layer acknowledgment that the indication was successfully received" ;
        skos:inScheme    ble: .

ftmp:StepCountField  a   skos:Concept ;
        rdfs:label       "Step Count Field" ;
        skos:definition  "The Step Count field represents the total number of steps counted by the Server since the beginning of the training session." ;
        skos:inScheme    ble: ;
        skos:related     xsd:unsignedShort .

ble:BluetoothSIG  a      skos:Concept ;
        rdfs:label       "Bluetooth Special Interest Group" ;
        skos:definition  "Bluetooth SIG- assigned Device ID Vendor ID value from the Assigned Numbers document." ;
        skos:inScheme    ble: ;
        skos:related     xsd:unsignedByte .

aiop:AutomationIOService
        a                skos:Concept ;
        rdfs:label       "Automation Input/Output Service" ;
        rdfs:seeAlso     <https://www.bluetooth.org/DocMan/handlers/DownloadDoc.ashx?doc_id=304972> ;
        owl:versionInfo  "1.0.0" ;
        skos:definition  "The Automation IO service is used to expose the analog inputs/outputs and digital input/outputs of a generic IO module." ;
        skos:inScheme    ble: ;
        skos:related     aiop:Analog , aiop:Digital , aiop:Aggregate .

lnp:EHPEField  a         skos:Concept ;
        rdfs:label       "Estimated Horizontal Position Error  Field" ;
        skos:definition  "The EHPE field represents the Estimated Horizontal Position Error, i.e., a measure of the error in a position in the horizontal plane." ;
        skos:inScheme    ble: ;
        skos:related     xsd:unsignedInt .

ftmp:MetabolicEquivalentField
        a                skos:Concept ;
        rdfs:label       "Metabolic Equivalent Field" ;
        skos:definition  "The Metabolic Equivalent field represents the metabolic equivalent of the user." ;
        skos:inScheme    ble: ;
        skos:related     xsd:unsignedByte .

ipsp:IPSupportService
        a                skos:Concept ;
        rdfs:comment     "This service does not define any characteristics." ;
        rdfs:label       "IP Support Service" ;
        rdfs:seeAlso     <https://www.bluetooth.org/docman/handlers/DownloadDoc.ashx?doc_id=296307> ;
        owl:versionInfo  "1.0" ;
        skos:definition  "The IP support service is used during service discovery to determine support for the IP Support Profile’s Node role." ;
        skos:inScheme    ble: .

idp:Off  a               skos:Concept ;
        rdfs:label       "Off" ;
        skos:definition  "The Insulin Delivery Device is switched off and no functionality is available" ;
        skos:inScheme    ble: .

idp:AnnunciationStatus
        a                skos:Concept ;
        rdfs:label       "Annunciation Status" ;
        skos:definition  "This Annunciation Status field represents the current status of an annunciation" ;
        skos:inScheme    ble: ;
        skos:narrower    idp:Undetermined , idp:Pending , idp:Snoozed , idp:Confirmed ;
        skos:related     xsd:unsignedByte .

ble:Notify  a            skos:Concept ;
        rdfs:label       "Notify" ;
        skos:definition  "A server is configured to notify a Characteristic Value to a client without expecting any Attribute Protocol layer acknowledgment that the notification was successfully received" ;
        skos:inScheme    ble: .

ble:Service  a         skos:Concept ;
        skos:inScheme  ble: ;
        skos:narrower  cscp:CyclingSpeedandCadenceService , pxp:LinkLossService , ble:HTTPProxyService , wsp:WeightScaleService , esp:EnvironmentalSensingService , ble:TransportDiscoveryService , cgmp:cgmpService , pasp:PhoneAlertStatusService , ble:UserDataService , otp:ObjectTransferService , ble:ImmediateAlertService , ble:BatteryService , anp:AlertNotificationService , plxp:PulseOximeterService , rcp:ReconnectionConfigurationService , htp:HealthThermometerService , cpp:CyclingPowerService , ble:CurrentTimeService , ble:DeviceInformationService , pxp:TxPowerService , blp:BloodPressureService , lnp:LocationandNavigationService , glp:GlucoseService , rscp:RunningSpeedandCadenceService , idp:InsulinDeliveryService , ble:BondManagementService , wsp:BodyCompositionService , tip:ReferenceTimeUpdateService , ble:ScanParametersService , ipsp:IPSupportService , ftmp:FitnessMachineService , hrp:HeartRateService , aiop:AutomationIOService , tip:NextDSTChangeService , lehid:HIDService , ble:IndoorPositioningService ;
        skos:related   ble:Characteristic .

cscp:CumulativeWheelRevolutions
        a                skos:Concept ;
        rdfs:label       "Cumulative Wheel Revolutions" ;
        skos:definition  "The Cumulative Wheel Revolutions value and the Last Wheel Event Time value allow the Client to calculate the speed (instantaneous and average) as well as the distance travelled." ;
        skos:inScheme    ble: ;
        skos:related     xsd:unsignedInt .

lehid:BootProtocolMode
        a                skos:Concept ;
        rdfs:label       "Boot Protocol Mode" ;
        skos:definition  "A HID Service shall only enter Boot Protocol Mode after this value has been written." ;
        skos:inScheme    ble: .

ble:LocationNameValue
        a                skos:Concept ;
        rdfs:label       "Location Name Value" ;
        skos:definition  "When read, the Server shall return the current value of the Location Name Characteristic." ;
        skos:inScheme    ble: ;
        skos:related     xsd:string .

lehid:HIDoverGATTProfile
        a                skos:Concept ;
        rdfs:label       "Low Energy Human Interface Device over GATT Profile" ;
        rdfs:seeAlso     <https://www.bluetooth.org/docman/handlers/downloaddoc.ashx?doc_id=245141> ;
        owl:versionInfo  "1.0" ;
        skos:definition  "The HID over GATT profile defines the procedures and features to be used by Bluetooth low energy HID Devices using GATT and Bluetooth HID Hosts using GATT." ;
        skos:inScheme    ble: ;
        skos:related     ble:BatteryService , ble:ScanParametersService , lehid:HIDService , ble:DeviceInformationService .

ble:LocationName  a      skos:Concept ;
        rdfs:label       "Location Name" ;
        skos:definition  "The Location Name Characteristic describes the name of the location in which the device is installed in accordance to the civicLocation." ;
        skos:inScheme    ble: ;
        skos:related     ble:WritewithoutResponse , ble:Read , ble:ReliableWrite , ble:LocationNameValue , ble:Write .

ftmp:MinimumHeartRateIncrementfield
        a                skos:Concept ;
        rdfs:label       "Minimum Heart Rate Increment" ;
        skos:definition  "Minimum Beats per minute with a resolution of 1" ;
        skos:inScheme    ble: ;
        skos:related     xsd:unsignedByte .

htp:MeasurementIntervalValue
        a                skos:Concept ;
        rdfs:label       "Measurement Interval Value" ;
        skos:definition  "The Measurement Interval characteristic returns the measurement interval value when read." ;
        skos:inScheme    ble: ;
        skos:related     xsd:unsignedShort .

ftmp:StepClimberData  a  skos:Concept ;
        rdfs:label       "Step Climber Data" ;
        skos:definition  "The Step Climber Data characteristic is used to send training-related data to the Client from a step climber (Server)." ;
        skos:inScheme    ble: ;
        skos:related     ftmp:EnergyperMinuteField , ftmp:MetabolicEquivalentField , ftmp:StepperMinuteField , ble:Notify , ftmp:FloorsField , ftmp:StepCountField , ftmp:EnergyperHourField , ftmp:HeartRateField , ftmp:TotalEnergyField , ftmp:PositiveElevationGainField , ftmp:RemainingTimeField , ftmp:AverageStepRateField , ftmp:ElapsedTimeField .

anp:UnreadAlertStatus
        a                skos:Concept ;
        rdfs:label       "Unread Alert Status" ;
        skos:definition  "The count of unread alert events existing in the server. The count of unread alert events is provided with the Category ID." ;
        skos:inScheme    ble: ;
        skos:related     ble:Notify .

ble:LocalEastCoordinateValue
        a                skos:Concept ;
        rdfs:label       "The current value of the Local East Coordinate Characteristic" ;
        skos:definition  "When read, the Server shall return the current value of the Local East Coordinate Characteristic." ;
        skos:inScheme    ble: ;
        skos:related     xsd:Short .

wsp:BodyWaterField  a    skos:Concept ;
        rdfs:label       "Body Wate Field" ;
        skos:definition  "The Body Water Mass field may be included in the Body Composition Measurement characteristic if the device supports the Body Water Mass feature." ;
        skos:inScheme    ble: ;
        skos:related     xsd:unsignedShort .

lnp:LocationLongitude
        a                skos:Concept ;
        rdfs:label       "Location - Longitude" ;
        skos:definition  "The Longitude value represents a geographic coordinate specifying the east-west position of a point on the Earth's surface in WGS-84 format." ;
        skos:inScheme    ble: ;
        skos:related     xsd:integer .

lehid:HIDControlPointCharacteristicValue
        a                skos:Concept ;
        rdfs:label       "HID Control Point Characteristic Value" ;
        skos:definition  "The HID Control Point characteristic value contains an enumeration of values when written" ;
        skos:inScheme    ble: ;
        skos:narrower    lehid:Suspend , lehid:ExitSuspend ;
        skos:related     xsd:unsignedByte .

ble:ScanRefresh  a       skos:Concept ;
        rdfs:label       "Scan Refresh" ;
        skos:definition  "The Scan Refresh characteristic is used to notify the Client that the Server requires the Scan Interval Window characteristic to be written with the latest values upon notification." ;
        skos:inScheme    ble: ;
        skos:related     ble:Notify , ble:Serverrequiresrefresh .

ble:CurrentTimeService
        a                skos:Concept ;
        rdfs:label       "Current Time Service" ;
        rdfs:seeAlso     <https://www.bluetooth.org/docman/handlers/downloaddoc.ashx?doc_id=292957> ;
        owl:versionInfo  "1.1" ;
        skos:definition  "This service defines how a Bluetooth device can expose date and time information to other Bluetooth devices." ;
        skos:inScheme    ble: ;
        skos:related     ble:LocalTimeInformation , ble:ReferenceTimeInformation , ble:CurrentTime .

rscp:RunningSpeedandCadenceProfile
        a                skos:Concept ;
        rdfs:label       "Running Speed and Cadence Profile" ;
        rdfs:seeAlso     <https://www.bluetooth.org/docman/handlers/downloaddoc.ashx?doc_id=261266> ;
        owl:versionInfo  "1.0" ;
        skos:definition  "TThe Running Speed and Cadence Profile is used to enable a data collection device to obtain data from a Running Speed and Cadence Sensor (RSC Sensor) that exposes the Running Speed and Cadence Service." ;
        skos:inScheme    ble: ;
        skos:related     rscp:RunningSpeedandCadenceService , ble:DeviceInformationService .

idp:InsulinConcentrationfield
        a                skos:Concept ;
        rdfs:label       "Insulin Concentration field" ;
        skos:definition  "The Insulin Concentration field shall be included in the IDD Features characteristic to expose the intended insulin concentration of the Insulin Delivery Device." ;
        skos:inScheme    ble: .

idp:SystemIssue  a       skos:Concept ;
        rdfs:label       "System Issue" ;
        skos:definition  "A general device fault or system error occurred (e.g., electronical or software error)." ;
        skos:inScheme    ble: .

idp:IDDCommandControlPoint
        a                skos:Concept ;
        rdfs:label       "Insulin Delivery Device Command Control Point" ;
        skos:definition  "The IDD Command Control Point provides procedures to support the insulin therapy by adapting therapy parameters to operate the insulin therapy remotely and to perform a remote operation of the device maintenance." ;
        skos:inScheme    ble: ;
        skos:related     idp:E2ECRCfield , idp:E2ECounterfield , ble:Notify .

idp:Undetermined  a      skos:Concept ;
        rdfs:label       "Undetermined" ;
        skos:definition  "The operational state is undetermined" ;
        skos:inScheme    ble: .

ftmp:FloorsField  a      skos:Concept ;
        rdfs:label       "Floors Field" ;
        skos:definition  "The Floors field represents the total number of floors counted by the Server since the beginning of the training session." ;
        skos:inScheme    ble: ;
        skos:related     xsd:unsignedShort .

wsp:ImpedanceField  a    skos:Concept ;
        rdfs:label       "Impedance Field" ;
        skos:definition  "The Impedance field may be included in the Body Composition Measurement characteristic if the device supports the Impedance feature." ;
        skos:inScheme    ble: ;
        skos:related     xsd:unsignedShort .

wsp:BIM  a               skos:Concept ;
        rdfs:label       "Body Mass Index" ;
        skos:definition  "The Body Mass Index may be included in the Weight Measurement characteristic if the device supports the BMI feature." ;
        skos:inScheme    ble: ;
        skos:related     xsd:unsignedShort .

ble:LocalTimeInformation
        a                skos:Concept ;
        rdfs:label       "Local Time Information" ;
        skos:definition  "The Local Time Information characteristic returns the local time information that includes time zone and DST offset." ;
        skos:inScheme    ble: ;
        skos:related     ble:Read , ble:Write .

cgmp:TimeOffsetField  a  skos:Concept ;
        rdfs:label       "Time Offset Field" ;
        skos:definition  "The Time Offset field is used in conjunction with the CGM Session Start Time to represent the time difference of the separate CGM measurements in relation to the session start time." ;
        skos:inScheme    ble: ;
        skos:related     xsd:unsignedShort .

blp:BloodPressureMeasurement
        a                skos:Concept ;
        rdfs:label       "Blood Pressure Measurement" ;
        skos:definition  "The Blood Pressure Measurement characteristic shall be used to send Blood Pressure measurements" ;
        skos:inScheme    ble: ;
        skos:related     blp:PulseRateField , ble:UserIDField , ble:Indicate , ble:TimeStampField , blp:BloodPressureMeasurementCompoundValueField .

idp:SequenceNumberfield
        a                skos:Concept ;
        rdfs:label       "Sequence Number field" ;
        skos:definition  "The Sequence Number shall be assigned to each IDD History Data characteristic value to maintain the chronological order of the history records in the Server history database." ;
        skos:inScheme    ble: ;
        skos:related     xsd:unsignedInt .

ftmp:RowerData  a        skos:Concept ;
        rdfs:label       "Rower Data" ;
        skos:definition  "The Rower Data characteristic is used to send training-related data to the Client from a rower (Server)." ;
        skos:inScheme    ble: ;
        skos:related     ftmp:EnergyperMinuteField , ftmp:MetabolicEquivalentField , ftmp:HeartRateField , ftmp:AverageStrokeRateField , ftmp:TotalEnergyField , ftmp:ElapsedTimeField , ftmp:StrokeRateField , ble:InstantaneousPowerField , ftmp:InstantaneousPaceField , ftmp:StrokeCountField , ftmp:AveragePaceField , ble:Notify , ftmp:RemainingTimeField , ftmp:ResistanceLevelField , ftmp:AveragePowerField , ftmp:TotalDistanceField , ftmp:EnergyperHourField .

htp:MeasurementInterval
        a                skos:Concept ;
        rdfs:label       "Measurement Interval" ;
        skos:definition  "The Measurement Interval characteristic is used to enable and control the interval between consecutive temperature measurements." ;
        skos:inScheme    ble: ;
        skos:related     htp:MeasurementIntervalValue , ble:Read .

ftmp:AveragePaceField
        a                skos:Concept ;
        rdfs:label       "Average Pace Field" ;
        skos:definition  "The Average Pace field represents the average pace of a user since the beginning of the training session." ;
        skos:inScheme    ble: ;
        skos:related     xsd:unsignedShort .

otp:ObjectActionControlPoint
        a                skos:Concept ;
        rdfs:label       "Object Action Control Point" ;
        skos:definition  "The Object Action Control Point is used by a Client to control certain behaviors of the Server." ;
        skos:inScheme    ble: ;
        skos:related     ble:Indicate , ble:Write .

idp:IDDRecordAccessControlPoint
        a                skos:Concept ;
        rdfs:label       "Insulin Delivery Device Record Access Control Point" ;
        skos:definition  "This control point is used by the Insulin Delivery Service to provide basic management functionality of the history database of the Insulin Delivery Device including historical data of the insulin therapy, device state changes, and annunciations." ;
        skos:inScheme    ble: ;
        skos:related     idp:E2ECRCfield , idp:E2ECounterfield , ble:Indicate , ble:Write .

ble:PnPID  a             skos:Concept ;
        rdfs:label       "Plug and Play Identification" ;
        skos:definition  "The PnP_ID characteristic is a set of values that shall be used to create a device ID value that is unique for this device. Included in the characteristic are a Vendor ID source field, a Vendor ID field, a Product ID field, and a Product Version field" ;
        skos:inScheme    ble: ;
        skos:related     ble:VendorIDSourceField , ble:ProductVersionField , ble:Read , ble:ProductIDField , ble:VendorIDField .

ble:LocalEastCoordinate
        a                skos:Concept ;
        rdfs:label       "Local East Coordinate" ;
        skos:definition  "The Local East Coordinate Characteristic describes the East coordinate of the device using a local coordinate system." ;
        skos:inScheme    ble: ;
        skos:related     ble:LocalEastCoordinateValue , ble:WritewithoutResponse , ble:Read , ble:ReliableWrite , ble:Write .

htp:IntermediateTemperature
        a                skos:Concept ;
        rdfs:label       "Intermediate Temperature" ;
        skos:definition  "The Intermediate Temperature characteristic is used to send intermediate temperature values to a device for display purposes while the measurement is in progress." ;
        skos:inScheme    ble: ;
        skos:related     ble:Notify .

ftmp:FitnessTest  a      skos:Concept ;
        rdfs:label       "Fitness Test" ;
        skos:definition  "0x08 - Fitness Test" ;
        skos:inScheme    ble: .

cgmp:cgmpStatus  a       skos:Concept ;
        rdfs:label       "cgmp Status cgmp Status" ;
        skos:definition  "The cgmp Status allows the client to actively request the status from the cgmp Sensor, particularly when the cgmp measurement is not running and the status cannot be given in the measurement result in the Status Annunciation Field." ;
        skos:inScheme    ble: ;
        skos:related     cgmp:E2ECRCField , ble:Read , cgmp:TimeOffsetField .

lnp:LocationandSpeed  a  skos:Concept ;
        rdfs:label       "Location and Speed" ;
        skos:definition  "The Location and Speed characteristic is used to send location and speed related data." ;
        skos:inScheme    ble: ;
        skos:related     lnp:TotalDistanceField , lnp:UTCTimeField , lnp:ElevationField , lnp:LocationLongitude , ble:InstantaneousSpeedField , lnp:RollingTimeField , lnp:HeadingField , ble:Notify , lnp:LocationLatitude .

idp:BolusIDfield  a      skos:Concept ;
        rdfs:label       "Bolus ID Field" ;
        skos:definition  "The Bolus ID field represents a unique identifier as a uint16 data type created by the Server Application for a programmed bolus." ;
        skos:inScheme    ble: ;
        skos:related     xsd:unsignedShort .

cgmp:cgmpService  a      skos:Concept ;
        rdfs:label       "Continuous Glucose Monitoring Service" ;
        rdfs:seeAlso     <https://www.bluetooth.org/docman/handlers/downloaddoc.ashx?doc_id=310502> ;
        owl:versionInfo  "1.0" ;
        skos:definition  "The Continuous Glucose Monitoring (cgmp) Service exposes glucose measurement and other data related to a personal cgmp sensor for healthcare applications." ;
        skos:inScheme    ble: ;
        skos:related     cgmp:cgmpSpecificOpsControlPoint , cgmp:cgmpSessionRunTime , ble:RecordAccessControlPoint , cgmp:cgmpMeasurement , cgmp:cgmpSessionStartTime , cgmp:cgmpStatus , cgmp:cgmpFeature .

idp:BatteryMedium  a     skos:Concept ;
        rdfs:label       "Battery Medium" ;
        skos:definition  "The Insulin Delivery Device has a medium operational runtime" ;
        skos:inScheme    ble: .

plxp:PLXFeatures  a      skos:Concept ;
        rdfs:label       "Pulse Oximeter Feature" ;
        skos:definition  "The PLX Features characteristic shall be used to describe the supported features of the Server." ;
        skos:inScheme    ble: ;
        skos:related     ble:Read .

ftmp:AveragePowerField
        a                skos:Concept ;
        rdfs:label       "Average Power Field" ;
        skos:definition  "The Average Power field represents the value of the average power measured by the Server since the beginning of the training session." ;
        skos:inScheme    ble: ;
        skos:related     xsd:short .

ftmp:FitnessMachineFeature
        a                skos:Concept ;
        rdfs:label       "Fitness Machine Feature" ;
        skos:definition  "The Fitness Machine Feature characteristic shall be used to describe the supported features of the Server." ;
        skos:inScheme    ble: ;
        skos:related     ble:Read .

ble:ProductIDField  a    skos:Concept ;
        rdfs:label       "Product ID Field" ;
        skos:definition  "The Product ID field is intended to distinguish between different products made by the vendor identified with the Vendor ID field." ;
        skos:inScheme    ble: ;
        skos:related     xsd:unsignedShort .

ble:RecordAccessControlPoint
        a                skos:Concept ;
        rdfs:label       "Record Access Control Point" ;
        skos:definition  "The Record Access Control Point shall be used to control notifications and other data operations." ;
        skos:inScheme    ble: ;
        skos:related     ble:Indicate , ble:Write .

cpp:AccumulatedTorqueField
        a                skos:Concept ;
        rdfs:label       "Accumulated Torque Field" ;
        skos:definition  "The Accumulated Torque field represents the cumulative value of the torque measured by the Sensor." ;
        skos:inScheme    ble: ;
        skos:related     xsd:unsignedShort .

ftmp:MaximumResistanceLevelField
        a                skos:Concept ;
        rdfs:label       "Maximum Resistance Level" ;
        skos:definition  "Unitless with a resolution of 0.1" ;
        skos:inScheme    ble: ;
        skos:related     xsd:short .

cpp:MinimumAngle  a      skos:Concept ;
        rdfs:label       "Minimum Angle Field" ;
        skos:definition  "The Minimum Angle field represents the angle of the crank when the minimum value is measured in the same crank revolution." ;
        skos:inScheme    ble: ;
        skos:related     xsd:unsignedByte .

pasp:PhoneAlertStatusService
        a                skos:Concept ;
        rdfs:label       "Phone Alert Status Service" ;
        rdfs:seeAlso     <https://www.bluetooth.org/docman/handlers/downloaddoc.ashx?doc_id=241862> ;
        owl:versionInfo  "1.0" ;
        skos:definition  "This service exposes the phone alert status when in a connection." ;
        skos:inScheme    ble: ;
        skos:related     pasp:AlertStatus , pasp:RingerControlPoint , pasp:RingerSetting .

idp:ManufacturerReserved
        a                skos:Concept ;
        rdfs:label       "Manufacturer Reserved Hamming Code Value Range" ;
        skos:definition  "All Hamming codes values in the range of 0xF000 and 0xFFF0 are manufacturer reserved" ;
        skos:inScheme    ble: .

otp:ObjectChanged  a     skos:Concept ;
        rdfs:label       "Object Changed Characteristic" ;
        skos:definition  "The Object Changed characteristic enables a Client to receive an indication if the contents and/or metadata of one or more objects are changed while the Client is connected without the change being made by an action of the Client itself." ;
        skos:inScheme    ble: ;
        skos:related     otp:ObjectIDField , ble:Indicate .

cgmp:cgmpSessionRunTimeField
        a                skos:Concept ;
        rdfs:label       "Session Run Time Field" ;
        skos:definition  "The CGM Session Run Time shall define the expected run time of the CGM session" ;
        skos:inScheme    ble: ;
        skos:related     xsd:unsignedShort .

anp:NumberofNewAlert  a  skos:Concept ;
        rdfs:label       "Number of New Alert" ;
        skos:definition  "This characteristic provides the count of new alerts (for a given category) in the server." ;
        skos:inScheme    ble: ;
        skos:related     xsd:unsignedByte .

ble:OrganizationIDField
        a                skos:Concept ;
        rdfs:label       "Organization ID Field" ;
        skos:definition  "This field shall contain a 1 octet Organization ID value from the Bluetooth SIG Assigned Numbers with the value set to the appropriate organization." ;
        skos:inScheme    ble: ;
        skos:related     xsd:unsignedByte .

ble:UserIndex  a         skos:Concept ;
        rdfs:label       "User Index" ;
        skos:definition  "When read, the User Index characteristic returns the index of the current user (i.e. the user that has given consent) to access the UDS Characteristics." ;
        skos:inScheme    ble: ;
        skos:related     ble:Read .

cgmp:cgmpFeature  a      skos:Concept ;
        rdfs:label       "cgmp Feature" ;
        skos:definition  "The cgmp Feature characteristic is used to describe the supported features of the Server." ;
        skos:inScheme    ble: ;
        skos:related     cgmp:E2ECRCField , ble:Read .

ble:TransportDataLengthField
        a                skos:Concept ;
        rdfs:label       "Transport Data Length Field" ;
        skos:definition  "This field shall contain a 1 octet value that represents the total number of octets in the Transport Data field that follows." ;
        skos:inScheme    ble: ;
        skos:related     xsd:unsignedByte .

lehid:ReportMapValue  a  skos:Concept ;
        rdfs:label       "Report Map Characteristic Value" ;
        skos:definition  "the Report Map characteristic value contains formatting and other information for Input Report, Output Report and Feature Report data transferred between a HID Device and HID Host." ;
        skos:inScheme    ble: ;
        skos:related     xsd:unsignedByte .

ftmp:ForceonBeltField
        a                skos:Concept ;
        rdfs:label       "Force on Belt Field" ;
        skos:definition  "The Force on Belt field represents the force being applied to the treadmill belt by the user’s steps" ;
        skos:inScheme    ble: ;
        skos:related     xsd:short .

pasp:AlertStatusValue
        a                skos:Concept ;
        rdfs:label       "Alert Status Value" ;
        skos:definition  "The Alert Status characteristic returns the current value of server’s alert status when read" ;
        skos:inScheme    ble: ;
        skos:related     xsd:unsignedByte .

ftmp:StrideCountField
        a                skos:Concept ;
        rdfs:label       "Stride Count Field" ;
        skos:definition  "The Stride Count field represents the total number of strides since the beginning of the training session." ;
        skos:inScheme    ble: ;
        skos:related     xsd:unsignedShort .

pasp:RingerSetting  a    skos:Concept ;
        rdfs:label       "Ringer Setting" ;
        skos:definition  "The Ringer Setting characteristic exposes the state of the server device's ringer." ;
        skos:inScheme    ble: ;
        skos:related     ble:Notify , ble:Read , xsd:unsignedByte .

anp:AlertNotificationProfile
        a                skos:Concept ;
        rdfs:label       "Alert Notification Profile" ;
        rdfs:seeAlso     <https://www.bluetooth.org/docman/handlers/downloaddoc.ashx?doc_id=242286> ;
        owl:versionInfo  "1.0" ;
        skos:definition  "The Alert Notification profile allows a device like a watch to obtain information from a cellphone about incoming calls, missed calls and SMS/MMS messages." ;
        skos:inScheme    ble: ;
        skos:related     anp:AlertNotificationService .

glp:CarbohydrateField
        a                skos:Concept ;
        rdfs:label       "Carbohydrate - units of kilograms" ;
        skos:definition  "Field exists if the key of bit 0 of the Flags field is set to 1." ;
        skos:inScheme    ble: ;
        skos:related     xsd:float .

anp:SupportedUnreadAlertCategory
        a                skos:Concept ;
        rdfs:label       "Supported Unread Alert Category" ;
        skos:definition  "A bit map showing which categories of unread alert events are supported and which are not." ;
        skos:inScheme    ble: ;
        skos:related     ble:Read .

idp:E2ECRCfield  a       skos:Concept ;
        rdfs:label       "End to End Cyclic Redundancy Check field" ;
        skos:definition  "If the Server supports E2E-Protection, all fields of a characteristic shall be secured by a CRC calculated over all fields of the characteristic payload." ;
        skos:inScheme    ble: ;
        skos:related     xsd:unsignedShort .

wsp:WeightScaleProfile
        a                skos:Concept ;
        rdfs:label       "Weight Scale Profile" ;
        rdfs:seeAlso     <https://www.bluetooth.org/docman/handlers/downloaddoc.ashx?doc_id=293525> ;
        owl:versionInfo  "1.0" ;
        skos:definition  "Weight Scale Profile enables a Collector device to connect and interact with a Weight Scale intended for consumer healthcare and sports/fitness applications." ;
        skos:inScheme    ble: ;
        skos:related     ble:BatteryService , wsp:BodyCompositionService , ble:UserDataService , wsp:WeightScaleService , ble:CurrentTimeService , ble:DeviceInformationService .

idp:Run  a               skos:Concept ;
        rdfs:label       "Run" ;
        skos:definition  "The insulin infusion therapy is running (i.e., the device delivers insulin related to the therapy)." ;
        skos:inScheme    ble: .

lehid:ReportProtocolMode
        a                skos:Concept ;
        rdfs:label       "Report Protocol Mode" ;
        skos:definition  "Default Protocol Mode of all HID Devices." ;
        skos:inScheme    ble: .
